<?xml version="1.0" encoding="UTF-8"?>
<rdf:RDF
	xmlns="http://www.semanticweb.org/chengluotong/ontologies/2024/7/untitled-ontology-185#"
	xmlns:lrmoo="http://iflastandards.info/ns/lrm/lrmoo/"
	xmlns:owl="http://www.w3.org/2002/07/owl#"
	xmlns:rdf="http://www.w3.org/1999/02/22-rdf-syntax-ns#"
	xmlns:terms="http://purl.org/dc/terms/"
	xmlns:cidoc-crm="http://www.cidoc-crm.org/cidoc-crm/"
	xmlns:DnS="http://www.loa-cnr.it/ontologies/DnS#"
	xmlns:xsd="http://www.w3.org/2001/XMLSchema#"
	xmlns:skos="http://www.w3.org/2004/02/skos/core#"
	xmlns:rdfs="http://www.w3.org/2000/01/rdf-schema#"
	xmlns:academictourism="http://academictourism.com/academictourism#"
	xmlns:fn="http://www.w3.org/2005/xpath-functions#"
	xmlns:sesame="http://www.openrdf.org/schema/sesame#"
	xmlns:ato="http://academictourism.com/entity/"
	xmlns:rdf4j="http://rdf4j.org/schema/rdf4j#">

<rdf:Description rdf:about="http://www.semanticweb.org/chengluotong/ontologies/2024/7/untitled-ontology-185">
	<rdf:type rdf:resource="http://www.w3.org/2002/07/owl#Ontology"/>
	<terms:contributor>Dave Beckett</terms:contributor>
	<terms:contributor>Nikki Rogers</terms:contributor>
	<terms:contributor>Participants in W3C's Semantic Web Deployment Working Group.</terms:contributor>
	<terms:creator>Alistair Miles</terms:creator>
	<terms:creator>Sean Bechhofer</terms:creator>
	<terms:description xml:lang="en">An RDF vocabulary for describing the basic structure and content of concept schemes such as thesauri, classification schemes, subject heading lists, taxonomies, 'folksonomies', other types of controlled vocabulary, and also concept schemes embedded in glossaries and terminologies.</terms:description>
	<terms:title xml:lang="en">SKOS Vocabulary</terms:title>
	<rdfs:comment xml:lang="en">CIDOC CRM v7.1.3 implemented in RDFS

This is the implementation approved by the 58th CRM-SIG meeting (March 2024)
as the current RDFS version for the CIDOC CRM namespace.
Note that this is NOT a definition of the CIDOC CRM, but a CIDOC CRM compatible implementation
of an RDF Schema derived from the authoritative release of the CIDOC CRM v7.1.3 on February 2024
https://cidoc-crm.org/Version/version-7.1.3 by an automated algorithm. It is intended for an
assumed majority of uses. Depending on the application, users may create adequate extensions 
compatible with the logical definitions of the CIDOC CRM.

Created by FORTH-ICS February 13, 2024
CC BY 4.0 https://creativecommons.org/licenses/by/4.0/legalcode



Encoding Rules:
1. The RDF spelling rules do not allow blanks. Hence we have replaced them by underscores.
   For instance "E63_Beginning_of_Existence" or "P2i_is_type_of".

2. RDF does not allow to instantiate properties beginning from a range value.
   Therefore, each CRM property is represented as two RDFS properties.
   For instance "P2 has type (is type of)" is represented as:
   "P2_has_type" for the domain to range direction and "P2i_is_type_of" for the range to domain direction.

3. The primitive values "E60 Number", "E61 Time Primitive", "E62 String", "E94 Space Primitive" and 
   "E95 Spacetime Primitive" referred in the Model for formal completeness are interpreted as rdfs:literal.

4. RDF does not support properties of properties, therefore, users may create their own
   subProperties for CRM properties that have a type property such as "P3 has note":
   Instead of P3 has note (P3-1 has type : parts description) declare
   &lt;rdf:Property rdf:about="P3_parts_description"&gt;
      &lt;rdfs:domain rdf:resource="E1_CRM_Entity"/&gt;
      &lt;rdfs:range rdf:resource="http://www.w3.org/2000/01/rdf-schema#Literal"/&gt;
      &lt;rdfs:subPropertyOf rdf:resource="P3_has_note"/&gt;
   &lt;/rdf:Property&gt;

5. Scope notes are represented as &lt;rdfs:comment&gt; elements.

6. In addition this encoding contains labels in languages different from English, 
   which are taken from translations of previous versions of the CIDOC CRM.    

7. Any other differences in labels, scope notes  and semantic relationships of this encoding 
   to the authoritative definition of the CIDOC CRM v7.1.3 (February 2024) are not intended transfer errors. 
   FORTH appreciates your feed-back on such errors.

8. CRM time extension 1.0 Encoded in RDFS (http://old.cidoc-crm.org/docs/How_to%20implement%20CRM_Time_in%20RDF.pdf)
   Since the Time Primitive of the CRM can not directly be implemented in RDF Triple Stores, we define in this extension
   of 4 properties replacing P81 and P82 adequately using xsd:dateTime. 
   Property P81 is dedicated for modeling the Time-Span's maximum known temporal extent i.e. ongoing_throughout. 
   Property P82 is for modeling the minimum outer bounds of events i.e. at_some_time_within. 
   P81 has its time interval redefined by P81a and P81b. Similarly, we redefine P82 by P82a and P82b.
## RDFS Generation Policies

### Sources

Policies followed for the RDFS implementation of CIDOC v.7.1.3 were created w.r.t.:

- Implementing the CIDOC Conceptual Reference Model in RDF (http://www.cidoc-crm.org/Resources/implementing-the-cidoc-conceptual-reference-model-in-rdf)
- How to implement CRM Time in RDF (http://old.cidoc-crm.org/docs/How_to%20implement%20CRM_Time_in%20RDF.pdf)
- CIDOC-CRM SIG feedback and the general guidelines:
  - Each property is declared twice, forward and backwards, unless no inverse name is defined in parentheses, or domain or range is interpreted as literal
  - All Primitive Values become rdfs:Literal
  - All IsA declarations from/to and between Primitive values are ignored

### Policies

#### **A. CIDOC Classes implementation in RDFS**

The CIDOC-CRM model defines classes, that in Triple Stores are typically implemented as primitive values. These classes are all subclasses of `E59 Primitive Value` and in RDFS they are interpreted as Literal. There are some classes in the CIDOC-CRM model that are both subclasses of `E59 Primitive Value` and E41 Appellation. So far we have followed the decision by CRM-SIG in "Issue 394: Solution for Dualism of E41 Appellation and rdfs:label" in 28-11-2018 wrt the question whether these classes should be implemented as rdfs:Class or still be interpreted as rdfs:Literal.

In this version we have followed the following policy regarding CIDOC Classes implementation in RDFS:

&gt; A1. CIDOC Classes that are subClasses of `E59 Primitive Value` are interpreted as rdfs:Literal regardless of whether they are also subClasses of another Class.

As a result, the following CIDOC classes were not defined in RDFS:

- `E59 Primitive Value`
- `E60 Number`
- `E61 Time Primitive`
- `E62 String`
- `E94 Space Primitive`
- `E95 Spacetime Primitive`

Additionally, the following isA relationships were not defined in RDFS:

- `E59 Primitive Value` `subClassOf` `E1 CRM Entity`
- `E60 Number` `subClassOf` `E59 Primitive Value`
- `E61 Time Primitive` `subClassOf` `E41 Appellation`
- `E61 Time Primitive` `subClassOf` `E59 Primitive Value`
- `E62 String` `subClassOf` `E59 Primitive Value`
- `E94 Space Primitive` `subClassOf` `E41 Appellation`
- `E94 Space Primitive` `subClassOf` `E59 Primitive Value`
- `E95 Spacetime Primitive` `subClassOf` `E41 Appellation`
- `E95 Spacetime Primitive` `subClassOf` `E59 Primitive Value`

#### **B. CIDOC Properties implementation in RDFS**

The decisions in policy A affect the implementation of CIDOC Properties in RDFS. A property cannot define an rdfs:Literal as rdfs:domain, and the backwards direction of a property with an rdfs:Literal as rdfs:range cannot be created for the exact same reason.

Further, the property ranges defined as rdfs:Literal in this implementation do not inherit the properties of the superclasses defined in the CIDOC Model. A separate guideline will describe how to instantiate such properties if at all needed.

Another aspect considered for the implementation of properties in RDFS is whether a distinct inverse property definition should be provided.

In this version we followed the following policies regarding CIDOC Properties implementation in RDFS:

&gt; B1. CIDOC Property backwards/inverse direction is **not** defined, whenever no inverse name for the property has been specified in parentheses in the official CIDOC documentation and property domain is not equal with property range.

As a result, the following properties do not define an inverse direction.

- `E1 CRM Entity. P3 has note: E62 String`
- `E19 Physical Object. P57 has number of parts: E60 Number`
- `E52 Time-Span. P79 beginning is qualified by: E62 String`
- `E52 Time-Span. P80 end is qualified by: E62 String`
- `E52 Time-Span. P81 ongoing throughout: E61 Time Primitive`
- `E52 Time-Span. P82 at some time within: E61 Time Primitive`
- `E54 Dimension. P90 has value: E60 Number`
- `E53 Place. P171 at some place within: E94 Space Primitive`
- `E53 Place. P172 contains: E94 Space Primitive`
- `E90 Symbolic Object. P190 has symbolic content: E62 String`

&gt; B2. CIDOC Property forward direction is **not** defined whenever property domain is interpreted as rdfs:Literal (A.1). Similarly, CIDOC Property backwards/inverse direction is **not** defined, whenever property range is interpreted as rdfs:Literal (A.1). Further, the instances of classes interpreted as rdfs:Literal, cannot express in RDFs their **inherited** properties that could be expressed according to CIDOC Model.

As a result,

a) The following **direct forward direction** CIDOC Properties **cannot** be expressed and are **not defined** in RDFS:

- `E95 Spacetime Primitive. P169 defines spacetime volume (spacetime volume is defined by): E92 Spacetime Volume`
- `E61 Time Primitive. P170 defines time (time is defined by): E52 Time-Span`

b) The following **direct backwards direction** CIDOC Properties **cannot** be expressed and are **not defined** in RDFS:

- `E94 Space Primitive. P168i defines place (place is defined by): E53 Place`

&gt; B3. Whenever no backwards/inverse property name is specified and property domain matches with property range, then the forward/direct property direction should be used for **both** directions and **no backwards/inverse property** needs to be defined.

As a result, we did not implement a separate backwards/inverse direction for the following CIDOC Properties:

- `E53 Place. P121 overlaps with: E53 Place`
- `E53 Place. P122 borders with: E53 Place`
- `E92 Spacetime Volume. P132 spatiotemporally overlaps with: E92 Spacetime Volume`
- `E92 Spacetime Volume. P133 is spatiotemporally separated from: E92 Spacetime Volume`

Additionally, all aforementioned redundant backwards/inverse CIDOC Property direction references, are replaced by the respective direct/forward CIDOC Property direction.

- The hierarchical link of  `P10i` subPropertyOf `P132i` was replaced with `P10i` subPropertyOf `P132`.

#### **C. Labels and appellations**

CIDOC-CRM version 7.1.3 defines the below subpropertyOf relations:

- `P168 place is defined by` `subPropertyOf` `P1 is identified by`
- `P169i spacetime volume is defined by` `subPropertyOf` `P1 is identified by`
- `P170i time is defined by` `subPropertyOf` `P1 is identified by`

The range of P168, P169i and P170i is `E94 Space Primitive`, `E95 Spacetime Primitive` and `E61 Time Primitive` respectively, which are all subclasses of `E41 Appellation` and interpreted as `rdfs:Literal` in RDFS, i.e. these three properties are datatype properties. However, the P1 property has range E41 Appellation, i.e. this property is an object property. Since OWL 2 distinguishes between object subproperties (https://www.w3.org/TR/2012/REC-owl2-syntax-20121211/#Object_Subproperties), data subproperties (https://www.w3.org/TR/2012/REC-owl2-syntax-20121211/#Data_Subproperties) and annotation subproperties (https://www.w3.org/TR/2012/REC-owl2-syntax-20121211/#Annotation_Subproperties), and also in OWL-DL the subject and object of a subproperty statement must be either both datatype properties or both object properties (see here (https://www.w3.org/TR/owl-ref/#subPropertyOf-def)), we do not include these three subPropertyOf relations in the provided RDFS implementation to avoid inconsistencies when reasoning with OWL 2 and OWL DL. Instead, we provide them in a separate ‘supplementary’ RDFS file which one can use if such inconsistencies are not expected.

In addition, since in the current practice, the property `rdfs:label` is widely used to denote appellations (see CRM-SIG Issue 394 (http://cidoc-crm.org/Issue/ID-394-solution-for-dualism-of-e41-appellation-and-rdfslabel)), the following `subPropertyOf` relation was also included in the supplementary RDFS file:

- `rdfs:label` subPropertyOf `P1 is identified by`

Note that according to the RDF Schema 1.1 specification, the domain (or range) of a property does not necessarily need to be 'subClassOf' or 'equal' to the domain (or range) of its superproperties. By including this subproperty relation, one can either directly use `rdfs:label` for providing a non-URI identifier/appellation for an instance of `E1 CRM Entity`, or use `P1 is identified by` for associating an additional URI-identifier with an instance of `E1 CRM Entity`, or use `P1 is identified by` and create an intermediate node (i.e. a URI-identifier for instance of `E41_Appellation`) for providing more detailed information about this appellation.

#### **D. Implementing Value Intervals**

The following are property pairs needed to simulate the interval-valued primitive values foreseen by the CRM:

&gt; D1. addition of two new properties, defined as subproperties of `E52 Time-Span. P81 ongoing throughout: E61 Time Primitive`, for the 'maximum known temporal extent' boundaries specification of `E61 Time Primitive`.

As a result, we have created the following property definitions:

- `E52 Time-Span. P81a end of the begin: rdfs:Literal` (subPropertyOf `E52 Time-Span. P81 ongoing throughout: E61 Time Primitive`)
- `E52 Time-Span. P81b begin of the end: rdfs:Literal` (subPropertyOf `E52 Time-Span. P81 ongoing throughout: E61 Time Primitive`)

&gt; D2. addition of two new properties, defined as subproperties of `E52 Time-Span. P82 at some time within: E61 Time Primitive`, for the 'minimum outer bounds' specification of `E61 Time Primitive`.

Consequently, we have created the following property definitions:

- `E52 Time-Span. P82a begin of the begin: rdfs:Literal` (subPropertyOf `E52 Time-Span. P82 at some time within: E61 Time Primitive`)
- `E52 Time-Span. P82b end of the end: rdfs:Literal` (subPropertyOf `E52 Time-Span. P82 at some time within: E61 Time Primitive`)

&gt; D3. addition of two new properties, defined as subproperties of `E54 Dimension. P90 has value: E60 Number`, for the upper and lower boundaries specification of `E60 Number`.

Consequently, we have created the following property definitions:

- `E54 Dimension. P90a has lower value limit: rdfs:Literal` (subPropertyOf `E54 Dimension. P90 has value: E60 Number`)
- `E54 Dimension. P90b has upper value limit: rdfs:Literal` (subPropertyOf `E54 Dimension. P90 has value: E60 Number`)

#### **E. Multiple ISA custom declaration Classes**

The following are declarations of frequently used multiple instantiations as classes with respective multiple IsA (so far only one):

&gt; E1. addition of a new class, defined as subClassOf `E41 Appellation` and `E33 Linguistic Object`, for all Appellations being regarded
specific to or characteristic for a language group and being described indirectly via a URI.

As a result, we have created the following class definition:

- `E33_E41_Linguistic_Appellation` subClass of `E33_Linguistic_Object` and `E41_Appellation`

#### **F. Translations and Scope notes**

&gt; F1. **Translations** Each RDFS Class or Property definition is accompanied by a set of translations expressed as rdfs:labels separated by xml:lang tags. The translation label used for each language is **the most recent** still **valid** translation. Still valid translation may be interpreted in the following ways:

- The English label of the `CurrentVersion` that the current RDFS file is referring to is *almost equal* (accepting only differences regarding multiple spaces) to the English label of the `TranslationVersion` that the translated label was created for. For example, in order to accept a translation for `E22 Human-Made Object` in the CurrentVersion (7.1.3) we should have a translation for E22 that was created based on a CIDOC version that used the same name for E22. The class name of E22 was changed from `E22 Man-Made Object` to `E22 Human-Made Object` in version 6.2.7. So the only **valid** translations would be these that were created based on version 6.2.7 or later. Currently no such translation has been created, so `E22 Human-Made Object` in CurrentVersion (7.1.3) does not define any translation in the RDFS file.

- Another option is to qualify translations as **valid** based on the scope note comparison of `CurrentVersion` and `TranslationVersion`. Since scope notes include formatting information, the comparison should ignore formatting changes.

Currently in this version we follow the option to qualify translations as valid based on the comparison of the respective labels in the corresponding CIDOC versions.

&gt; F2. **Scope notes** are defined as rdfs:comment and include only the text of the official CIDOC-CRM version in English language. Since scope notes are not just simple texts but include formatting data, a simple removal of the formatting data does not always produce a readable format. Therefore we followed the below simple conventions for the transformation of CIDOC-CRM scope note text into a readable rdfs:comment:

- Each Paragraph defines a new line
- Each element in an unordered list defines a new line
- Each element in an ordered list defines a new line prefixed with `'{order}. '`
- Each superscript text is separated from its base with `'-'`
- Each subscript text is separated from its base with `'_'` (none found)

&gt; F3. **Scope notes of Inverse Properties**. Scope notes for the inverse/backwards direction of properties are not defined as they are covered by the definition of the direct/forward direction definition. Whenever the direct/forward property direction of a property `Pxxx` is not defined due to policy **B1**, then its scope note is used as scope note for the inverse/backwards property `Pxxxi`, and labeled as `Scope note for 'Pxxx':`.

As a result, the direct/forward property definition was used for the rdfs:comment definition of

- `E92 Spacetime Volume. P169i spacetime volume is defined by: rdfs:Literal`
- `E52 Time-Span. P170i time is defined by: rdfs:Literal`

</rdfs:comment>
	<rdfs:label xml:lang="en">LRMoo 1.0 / OWL</rdfs:label>
	<rdfs:seeAlso rdf:resource="http://www.w3.org/TR/skos-reference/"/>
	<owl:versionInfo xml:lang="en">LRMoo Ontology 1.0 (May, 2024) including references to CIDOC-CRM 7.1.3</owl:versionInfo>
	<owl:versionInfo xml:lang="en">RDFs Implementation (February 2024) of CIDOC-CRM 7.1.3</owl:versionInfo>
</rdf:Description>

<rdf:Description rdf:about="http://purl.org/dc/terms/contributor">
	<rdf:type rdf:resource="http://www.w3.org/2002/07/owl#AnnotationProperty"/>
</rdf:Description>

<rdf:Description rdf:about="http://purl.org/dc/terms/creator">
	<rdf:type rdf:resource="http://www.w3.org/2002/07/owl#AnnotationProperty"/>
</rdf:Description>

<rdf:Description rdf:about="http://purl.org/dc/terms/description">
	<rdf:type rdf:resource="http://www.w3.org/2002/07/owl#AnnotationProperty"/>
</rdf:Description>

<rdf:Description rdf:about="http://purl.org/dc/terms/title">
	<rdf:type rdf:resource="http://www.w3.org/2002/07/owl#AnnotationProperty"/>
</rdf:Description>

<rdf:Description rdf:about="http://www.w3.org/2004/02/skos/core#altLabel">
	<rdf:type rdf:resource="http://www.w3.org/2002/07/owl#AnnotationProperty"/>
	<rdfs:comment xml:lang="en">The range of skos:altLabel is the class of RDF plain literals.</rdfs:comment>
	<rdfs:comment xml:lang="en">skos:prefLabel, skos:altLabel and skos:hiddenLabel are pairwise disjoint properties.</rdfs:comment>
	<rdfs:isDefinedBy rdf:resource="http://www.w3.org/2004/02/skos/core"/>
	<rdfs:label xml:lang="en">alternative label</rdfs:label>
	<skos:definition xml:lang="en">An alternative lexical label for a resource.</skos:definition>
	<skos:example xml:lang="en">Acronyms, abbreviations, spelling variants, and irregular plural/singular forms may be included among the alternative labels for a concept. Mis-spelled terms are normally included as hidden labels (see skos:hiddenLabel).</skos:example>
</rdf:Description>

<rdf:Description rdf:about="http://www.w3.org/2004/02/skos/core#definition">
	<rdf:type rdf:resource="http://www.w3.org/2002/07/owl#AnnotationProperty"/>
	<rdfs:isDefinedBy rdf:resource="http://www.w3.org/2004/02/skos/core"/>
	<rdfs:label xml:lang="en">definition</rdfs:label>
	<skos:definition xml:lang="en">A statement or formal explanation of the meaning of a concept.</skos:definition>
</rdf:Description>

<rdf:Description rdf:about="http://www.w3.org/2004/02/skos/core#example">
	<rdf:type rdf:resource="http://www.w3.org/2002/07/owl#AnnotationProperty"/>
	<rdfs:isDefinedBy rdf:resource="http://www.w3.org/2004/02/skos/core"/>
	<rdfs:label xml:lang="en">example</rdfs:label>
	<skos:definition xml:lang="en">An example of the use of a concept.</skos:definition>
</rdf:Description>

<rdf:Description rdf:about="http://www.w3.org/2004/02/skos/core#notation">
	<rdf:type rdf:resource="http://www.w3.org/2002/07/owl#AnnotationProperty"/>
	<rdfs:isDefinedBy rdf:resource="http://www.w3.org/2004/02/skos/core"/>
	<rdfs:label xml:lang="en">notation</rdfs:label>
	<skos:definition xml:lang="en">A notation, also known as classification code, is a string of characters such as "T58.5" or "303.4833" used to uniquely identify a concept within the scope of a given concept scheme.</skos:definition>
	<skos:scopeNote xml:lang="en">By convention, skos:notation is used with a typed literal in the object position of the triple.</skos:scopeNote>
</rdf:Description>

<rdf:Description rdf:about="http://www.w3.org/2004/02/skos/core#prefLabel">
	<rdf:type rdf:resource="http://www.w3.org/2002/07/owl#AnnotationProperty"/>
	<rdfs:comment xml:lang="en">A resource has no more than one value of skos:prefLabel per language tag, and no more than one value of skos:prefLabel without language tag.</rdfs:comment>
	<rdfs:comment xml:lang="en">The range of skos:prefLabel is the class of RDF plain literals.</rdfs:comment>
	<rdfs:comment xml:lang="en">skos:prefLabel, skos:altLabel and skos:hiddenLabel are pairwise
      disjoint properties.</rdfs:comment>
	<rdfs:isDefinedBy rdf:resource="http://www.w3.org/2004/02/skos/core"/>
	<rdfs:label xml:lang="en">preferred label</rdfs:label>
	<skos:definition xml:lang="en">The preferred lexical label for a resource, in a given language.</skos:definition>
</rdf:Description>

<rdf:Description rdf:about="http://www.w3.org/2004/02/skos/core#scopeNote">
	<rdf:type rdf:resource="http://www.w3.org/2002/07/owl#AnnotationProperty"/>
	<rdfs:isDefinedBy rdf:resource="http://www.w3.org/2004/02/skos/core"/>
	<rdfs:label xml:lang="en">scope note</rdfs:label>
	<skos:definition xml:lang="en">A note that helps to clarify the meaning and/or the use of a concept.</skos:definition>
</rdf:Description>

<rdf:Description rdf:about="http://academictourism.com/academictourism#conveys">
	<rdf:type rdf:resource="http://www.w3.org/2002/07/owl#ObjectProperty"/>
	<owl:inverseOf rdf:resource="http://academictourism.com/academictourism#is_conveyed_by"/>
	<rdfs:domain rdf:resource="http://www.cidoc-crm.org/cidoc-crm/E7_Activity"/>
	<rdfs:range rdf:resource="http://www.cidoc-crm.org/cidoc-crm/E89_Propositional_Object"/>
</rdf:Description>

<rdf:Description rdf:about="http://academictourism.com/academictourism#is_conveyed_by">
	<rdf:type rdf:resource="http://www.w3.org/2002/07/owl#ObjectProperty"/>
	<rdfs:domain rdf:resource="http://www.cidoc-crm.org/cidoc-crm/E89_Propositional_Object"/>
	<rdfs:range rdf:resource="http://www.cidoc-crm.org/cidoc-crm/E7_Activity"/>
</rdf:Description>

<rdf:Description rdf:about="http://iflastandards.info/ns/lrm/lrmoo/R10_is_member_of">
	<rdf:type rdf:resource="http://www.w3.org/2002/07/owl#ObjectProperty"/>
	<owl:inverseOf rdf:resource="http://iflastandards.info/ns/lrm/lrmoo/R10i_has_member"/>
	<rdfs:domain rdf:resource="http://iflastandards.info/ns/lrm/lrmoo/F1_Work"/>
	<rdfs:range rdf:resource="http://www.cidoc-crm.org/cidoc-crm/E28_Conceptual_Object"/>
	<rdfs:comment xml:lang="en">Quantification: many to many (0,n:0,n)

Scope note:
This property associates an instance of F1 Work with an instance of E28 Conceptual Object that represents a generalization of the work. The property can be used to group variant, alternative or related works that are considered to share a common concept.
Whereas instances of F1 Work are always realised in instances of F2 Expression, there is no particular expression that fully conveys the instance of Conceptual Object that a work may be a member of.
Intended usage of the property includes what is discussed as “superwork” in the library community. Typical examples are novels that can be grouped by fictional universes or common characters, paintings or graphical works that exist as a family of alternatives, musical compositions that are referred to as the same although they exist as particular versions that are each identified as an individual work. The instance of E28 Conceptual Object that has works as members will often be constructed for a specific purpose, such as bibliographic organization or retrieval.

Examples:
- Auguste Rodin’s ‘Le penseur’ (E28) has member Auguste Rodin’s ‘Le penseur’ in monumental size (F1). [In original size this sculpture forms part of (R67i) Rodin’s ‘La Porte de l’Enfer’ (F1); in monumental size it is an autonomous work. All scale variants are members of (R10) the superwork ‘Le penseur’(E28).]
- Edward Munch’s ‘Madonna’ (E28) has member Edward Munch’s black and white graphical work ‘Madonna’ (F1).
- Edward Munch’s ‘Madonna’ (E28) has member Edward Munch’s painting ‘Madonna’ (F1).
- Ludwig van Beethoven’s opera Op. 72 ‘Fidelio’ (E28) has member Ludwig van Beethoven’s opera ‘Leonore, oder Der Triumph der ehelichen Liebe’ (the initial version that was performed in 1805) (F1).
- Ludwig van Beethoven’s opera Op. 72 ‘Fidelio’ (E28) has member Ludwig van Beethoven’s opera ‘Fidelio’ (the final version that was first performed in 1814) (F1).
- The fictional universe created by Terry Pratchett referred to as ‘Discworld’ (E28) has member Terry Pratchett’s novel ‘The Light Fantastic’ (F1).
- The fictional universe created by Terry Pratchett referred to as ‘Discworld’ (E28) has member ‘Where’s my Cow’, a picture book by Terry Pratchett and Melvyn Grant (F1).
</rdfs:comment>
	<rdfs:label xml:lang="en">R10 is member of</rdfs:label>
	<skos:notation>R10</skos:notation>
	<skos:prefLabel xml:lang="en">is member of</skos:prefLabel>
</rdf:Description>

<rdf:Description rdf:about="http://iflastandards.info/ns/lrm/lrmoo/R10i_has_member">
	<rdf:type rdf:resource="http://www.w3.org/2002/07/owl#ObjectProperty"/>
	<rdfs:domain rdf:resource="http://www.cidoc-crm.org/cidoc-crm/E28_Conceptual_Object"/>
	<rdfs:range rdf:resource="http://iflastandards.info/ns/lrm/lrmoo/F1_Work"/>
	<rdfs:comment xml:lang="en">Quantification of the inverse property: many to many (0,n:0,n)

Scope note of the inverse property:
This property associates an instance of F1 Work with an instance of E28 Conceptual Object that represents a generalization of the work. The property can be used to group variant, alternative or related works that are considered to share a common concept.
Whereas instances of F1 Work are always realised in instances of F2 Expression, there is no particular expression that fully conveys the instance of Conceptual Object that a work may be a member of.
Intended usage of the property includes what is discussed as “superwork” in the library community. Typical examples are novels that can be grouped by fictional universes or common characters, paintings or graphical works that exist as a family of alternatives, musical compositions that are referred to as the same although they exist as particular versions that are each identified as an individual work. The instance of E28 Conceptual Object that has works as members will often be constructed for a specific purpose, such as bibliographic organization or retrieval.

Examples of the inverse property:
- Auguste Rodin’s ‘Le penseur’ (E28) has member Auguste Rodin’s ‘Le penseur’ in monumental size (F1). [In original size this sculpture forms part of (R67i) Rodin’s ‘La Porte de l’Enfer’ (F1); in monumental size it is an autonomous work. All scale variants are members of (R10) the superwork ‘Le penseur’(E28).]
- Edward Munch’s ‘Madonna’ (E28) has member Edward Munch’s black and white graphical work ‘Madonna’ (F1).
- Edward Munch’s ‘Madonna’ (E28) has member Edward Munch’s painting ‘Madonna’ (F1).
- Ludwig van Beethoven’s opera Op. 72 ‘Fidelio’ (E28) has member Ludwig van Beethoven’s opera ‘Leonore, oder Der Triumph der ehelichen Liebe’ (the initial version that was performed in 1805) (F1).
- Ludwig van Beethoven’s opera Op. 72 ‘Fidelio’ (E28) has member Ludwig van Beethoven’s opera ‘Fidelio’ (the final version that was first performed in 1814) (F1).
- The fictional universe created by Terry Pratchett referred to as ‘Discworld’ (E28) has member Terry Pratchett’s novel ‘The Light Fantastic’ (F1).
- The fictional universe created by Terry Pratchett referred to as ‘Discworld’ (E28) has member ‘Where’s my Cow’, a picture book by Terry Pratchett and Melvyn Grant (F1).
</rdfs:comment>
	<rdfs:label xml:lang="en">R10i has member</rdfs:label>
	<skos:notation>R10i</skos:notation>
	<skos:prefLabel xml:lang="en">has member</skos:prefLabel>
</rdf:Description>

<rdf:Description rdf:about="http://iflastandards.info/ns/lrm/lrmoo/R11_has_issuing_rule">
	<rdf:type rdf:resource="http://www.w3.org/2002/07/owl#ObjectProperty"/>
	<owl:inverseOf rdf:resource="http://iflastandards.info/ns/lrm/lrmoo/R11i_is_issuing_rule_of"/>
	<rdfs:domain rdf:resource="http://iflastandards.info/ns/lrm/lrmoo/F18_Serial_Work"/>
	<rdfs:range rdf:resource="http://www.cidoc-crm.org/cidoc-crm/E29_Design_or_Procedure"/>
	<rdfs:comment xml:lang="en">Quantification: many to many (0,n:0,n)

Shortcut Of: F18 Serial Work. R19i was realised through: F30 Manifestation Creation. P16 used specific object (was used for): E29 Design or Procedure

Scope note:
This property associates an instance of F18 Serial Work with the instance of E29 Design or Procedure that specifies the issuing policy planned by this instance of F18 Serial Work, such as sequencing pattern, expected frequency and expected regularity.

Examples:
- [Editor’s note: Transfer this property to PRESS(OO) once version 2.0 has a stable draft. Implement this property only in conjunction with an implementation of PRESS(OO).]
- The serial entitled ‘Quarterly journal of pure and applied mathematics’, identified by ISSN ‘1549-6724’ (F18) has issuing rule to be issued every three months, on a regular basis, with each issue being numbered according to the pattern ‘Vol. 1, no. 1 (2005)’ that was observed by the Library of Congress’s cataloguers on an exemplar of the first issue (E29).
</rdfs:comment>
	<rdfs:label xml:lang="en">R11 has issuing rule</rdfs:label>
	<skos:notation>R11</skos:notation>
	<skos:prefLabel xml:lang="en">has issuing rule</skos:prefLabel>
</rdf:Description>

<rdf:Description rdf:about="http://iflastandards.info/ns/lrm/lrmoo/R11i_is_issuing_rule_of">
	<rdf:type rdf:resource="http://www.w3.org/2002/07/owl#ObjectProperty"/>
	<rdfs:domain rdf:resource="http://www.cidoc-crm.org/cidoc-crm/E29_Design_or_Procedure"/>
	<rdfs:range rdf:resource="http://iflastandards.info/ns/lrm/lrmoo/F18_Serial_Work"/>
	<rdfs:comment xml:lang="en">Quantification of the inverse property: many to many (0,n:0,n)

Shortcut Of of the inverse property: F18 Serial Work. R19i was realised through: F30 Manifestation Creation. P16 used specific object (was used for): E29 Design or Procedure

Scope note of the inverse property:
This property associates an instance of F18 Serial Work with the instance of E29 Design or Procedure that specifies the issuing policy planned by this instance of F18 Serial Work, such as sequencing pattern, expected frequency and expected regularity.

Examples of the inverse property:
- [Editor’s note: Transfer this property to PRESS(OO) once version 2.0 has a stable draft. Implement this property only in conjunction with an implementation of PRESS(OO).]
- The serial entitled ‘Quarterly journal of pure and applied mathematics’, identified by ISSN ‘1549-6724’ (F18) has issuing rule to be issued every three months, on a regular basis, with each issue being numbered according to the pattern ‘Vol. 1, no. 1 (2005)’ that was observed by the Library of Congress’s cataloguers on an exemplar of the first issue (E29).
</rdfs:comment>
	<rdfs:label xml:lang="en">R11i is issuing rule of</rdfs:label>
	<skos:notation>R11i</skos:notation>
	<skos:prefLabel xml:lang="en">is issuing rule of</skos:prefLabel>
</rdf:Description>

<rdf:Description rdf:about="http://iflastandards.info/ns/lrm/lrmoo/R15_has_fragment">
	<rdf:type rdf:resource="http://www.w3.org/2002/07/owl#ObjectProperty"/>
	<rdfs:subPropertyOf rdf:resource="http://www.cidoc-crm.org/cidoc-crm/P106_is_composed_of"/>
	<owl:inverseOf rdf:resource="http://iflastandards.info/ns/lrm/lrmoo/R15i_is_fragment_of"/>
	<rdfs:domain rdf:resource="http://iflastandards.info/ns/lrm/lrmoo/F2_Expression"/>
	<rdfs:range rdf:resource="http://www.cidoc-crm.org/cidoc-crm/E90_Symbolic_Object"/>
	<rdfs:comment xml:lang="en">Quantification: many to many (0,n:0,n)

Scope note:
This property associates an instance of E90 Symbolic Object with an instance of F2 Expression of which it is a fragment. The fragment is not itself an instance of F2 Expression as it does not express any instance of F1 Work. When the fragment consists of intelligible words it is an instance of E33 Linguistic Object.
An instance of E90 Symbolic Object is only considered a fragment of an instance of F2 Expression when related to its occurrence in a known or assumed whole by the R15 has fragment (is fragment of) property. The size of an instance of E90 Symbolic Object ranges from more than 99% of an instance of F2 Expression to tiny bits (a few words from a text, one bar from a musical composition, one detail from a still image, a two-second clip from a video, etc.).
An instance of E90 Symbolic Object can become a fragment of an instance of F2 Expression through the deterioration over time of a carrier of the expression, such as when only fragments of a manuscript of an ancient text survive. Typically instances of E90 Symbolic Object that are of interest as fragments of expressions are formed deliberately, such as when excerpts are taken from a text by the compiler of a collection of excerpts, or citations from one expression are used in another text.

Examples:
- The ancient Greek text of the four stanzas from an ode by Sappho (E33) that were quoted by Pseudo-Longinus in his textual work entitled ‘On the sublime’ is fragment of the complete ancient Greek text, now irremediably lost, of Sappho’s ode currently identified as Sappho’s poem #2 (F2).
- The phrase ‘Beati pauperes spiritu’ (E33) is fragment of the Latin text of the Gospel according to St. Matthew (F2). [excerpt from Matthew 5,3]
- The stanza ‘Nel mezzo del cammin di nostra vita / mi ritrovai per una selva oscura / ché la diritta via era smarrita’ (E33) is fragment of the Italian text of Dante Alighieri’s ‘Inferno’ from the ‘Divina Commedia’ (F2).
- The widely recognized ominous four-note opening motif (E73) is fragment of Beethoven’s Fifth Symphony (F2).
- The melting clock (E36) is fragment of the painting ‘Persistence of Memory’ by Salvador Dali, 1931 (F2).
</rdfs:comment>
	<rdfs:label xml:lang="en">R15 has fragment</rdfs:label>
	<skos:notation>R15</skos:notation>
	<skos:prefLabel xml:lang="en">has fragment</skos:prefLabel>
</rdf:Description>

<rdf:Description rdf:about="http://iflastandards.info/ns/lrm/lrmoo/R15i_is_fragment_of">
	<rdf:type rdf:resource="http://www.w3.org/2002/07/owl#ObjectProperty"/>
	<rdfs:subPropertyOf rdf:resource="http://www.cidoc-crm.org/cidoc-crm/P106i_forms_part_of"/>
	<rdfs:domain rdf:resource="http://www.cidoc-crm.org/cidoc-crm/E90_Symbolic_Object"/>
	<rdfs:range rdf:resource="http://iflastandards.info/ns/lrm/lrmoo/F2_Expression"/>
	<rdfs:comment xml:lang="en">Quantification of the inverse property: many to many (0,n:0,n)

Scope note of the inverse property:
This property associates an instance of E90 Symbolic Object with an instance of F2 Expression of which it is a fragment. The fragment is not itself an instance of F2 Expression as it does not express any instance of F1 Work. When the fragment consists of intelligible words it is an instance of E33 Linguistic Object.
An instance of E90 Symbolic Object is only considered a fragment of an instance of F2 Expression when related to its occurrence in a known or assumed whole by the R15 has fragment (is fragment of) property. The size of an instance of E90 Symbolic Object ranges from more than 99% of an instance of F2 Expression to tiny bits (a few words from a text, one bar from a musical composition, one detail from a still image, a two-second clip from a video, etc.).
An instance of E90 Symbolic Object can become a fragment of an instance of F2 Expression through the deterioration over time of a carrier of the expression, such as when only fragments of a manuscript of an ancient text survive. Typically instances of E90 Symbolic Object that are of interest as fragments of expressions are formed deliberately, such as when excerpts are taken from a text by the compiler of a collection of excerpts, or citations from one expression are used in another text.

Examples of the inverse property:
- The ancient Greek text of the four stanzas from an ode by Sappho (E33) that were quoted by Pseudo-Longinus in his textual work entitled ‘On the sublime’ is fragment of the complete ancient Greek text, now irremediably lost, of Sappho’s ode currently identified as Sappho’s poem #2 (F2).
- The phrase ‘Beati pauperes spiritu’ (E33) is fragment of the Latin text of the Gospel according to St. Matthew (F2). [excerpt from Matthew 5,3]
- The stanza ‘Nel mezzo del cammin di nostra vita / mi ritrovai per una selva oscura / ché la diritta via era smarrita’ (E33) is fragment of the Italian text of Dante Alighieri’s ‘Inferno’ from the ‘Divina Commedia’ (F2).
- The widely recognized ominous four-note opening motif (E73) is fragment of Beethoven’s Fifth Symphony (F2).
- The melting clock (E36) is fragment of the painting ‘Persistence of Memory’ by Salvador Dali, 1931 (F2).
</rdfs:comment>
	<rdfs:label xml:lang="en">R15i is fragment of</rdfs:label>
	<skos:notation>R15i</skos:notation>
	<skos:prefLabel xml:lang="en">is fragment of</skos:prefLabel>
</rdf:Description>

<rdf:Description rdf:about="http://iflastandards.info/ns/lrm/lrmoo/R16_created">
	<rdf:type rdf:resource="http://www.w3.org/2002/07/owl#ObjectProperty"/>
	<rdfs:subPropertyOf rdf:resource="http://www.cidoc-crm.org/cidoc-crm/P94_has_created"/>
	<owl:inverseOf rdf:resource="http://iflastandards.info/ns/lrm/lrmoo/R16i_was_created_by"/>
	<rdfs:domain rdf:resource="http://iflastandards.info/ns/lrm/lrmoo/F27_Work_Creation"/>
	<rdfs:range rdf:resource="http://iflastandards.info/ns/lrm/lrmoo/F1_Work"/>
	<rdfs:comment xml:lang="en">Quantification: one to many, necessary, dependent (1,n:1,1)

Scope note:
This property associates the initial creation of a work and the instance of F1 Work that was created.

Examples:
- Agatha Christie creating ‘Murder on the Orient Express’ (F27), created the work ‘Murder on the Orient Express’ (F1).
- Mary Shelley creating ‘Frankenstein, or, The Modern Prometheus’ (F27), created the work ‘Frankenstein, or, The Modern Prometheus’ (F1).
- Dante creating the poem ‘Divina Commedia’ (F27), created the work ‘Divina Commedia’ (F1).
- William Shakespeare creating ‘The Tragedy of Hamlet, Prince of Denmark’(F27), created the work ‘The Tragedy of Hamlet, Prince of Denmark’ (F1).
- René Goscinny and Albert Uderzo (collaboratively) creating ‘Astérix le Gaulois’ (F27) created the work ‘Astérix le Gaulois’ (F1).
- The work creation event of Ludwig van Beethoven composing his ‘Symphony No. 9’ (F27) created the work ‘Beethoven’s Symphony No. 9’ (F1).
- Johann Sebastian Bach composing the ‘Goldberg Variations’ (F27) created the work the ‘Goldberg Variations’ (F1).
- The making of ‘Jules et Jim’, directed by François Truffault (F27) created the work ‘Jules et Jim’ (F1).
- The making of ‘Psycho’, directed by Alfred Hitchcock (F27) created the work ‘Psycho’ (F1).
- Auguste Rodin creating ‘Le Penseur’ (The Thinker) (F27), created the work ‘Le Penseur’ (The Thinker) (F1).
- Picasso creating ‘Guernica’ (F27) created the work ‘Guernica’ (F1).
</rdfs:comment>
	<rdfs:label xml:lang="en">R16 created</rdfs:label>
	<skos:notation>R16</skos:notation>
	<skos:prefLabel xml:lang="en">created</skos:prefLabel>
</rdf:Description>

<rdf:Description rdf:about="http://iflastandards.info/ns/lrm/lrmoo/R16i_was_created_by">
	<rdf:type rdf:resource="http://www.w3.org/2002/07/owl#ObjectProperty"/>
	<rdfs:subPropertyOf rdf:resource="http://www.cidoc-crm.org/cidoc-crm/P94i_was_created_by"/>
	<rdfs:domain rdf:resource="http://iflastandards.info/ns/lrm/lrmoo/F1_Work"/>
	<rdfs:range rdf:resource="http://iflastandards.info/ns/lrm/lrmoo/F27_Work_Creation"/>
	<rdfs:comment xml:lang="en">Quantification of the inverse property: one to many, necessary, dependent (1,n:1,1)

Scope note of the inverse property:
This property associates the initial creation of a work and the instance of F1 Work that was created.

Examples of the inverse property:
- Agatha Christie creating ‘Murder on the Orient Express’ (F27), created the work ‘Murder on the Orient Express’ (F1).
- Mary Shelley creating ‘Frankenstein, or, The Modern Prometheus’ (F27), created the work ‘Frankenstein, or, The Modern Prometheus’ (F1).
- Dante creating the poem ‘Divina Commedia’ (F27), created the work ‘Divina Commedia’ (F1).
- William Shakespeare creating ‘The Tragedy of Hamlet, Prince of Denmark’(F27), created the work ‘The Tragedy of Hamlet, Prince of Denmark’ (F1).
- René Goscinny and Albert Uderzo (collaboratively) creating ‘Astérix le Gaulois’ (F27) created the work ‘Astérix le Gaulois’ (F1).
- The work creation event of Ludwig van Beethoven composing his ‘Symphony No. 9’ (F27) created the work ‘Beethoven’s Symphony No. 9’ (F1).
- Johann Sebastian Bach composing the ‘Goldberg Variations’ (F27) created the work the ‘Goldberg Variations’ (F1).
- The making of ‘Jules et Jim’, directed by François Truffault (F27) created the work ‘Jules et Jim’ (F1).
- The making of ‘Psycho’, directed by Alfred Hitchcock (F27) created the work ‘Psycho’ (F1).
- Auguste Rodin creating ‘Le Penseur’ (The Thinker) (F27), created the work ‘Le Penseur’ (The Thinker) (F1).
- Picasso creating ‘Guernica’ (F27) created the work ‘Guernica’ (F1).
</rdfs:comment>
	<rdfs:label xml:lang="en">R16i was created by</rdfs:label>
	<skos:notation>R16i</skos:notation>
	<skos:prefLabel xml:lang="en">was created by</skos:prefLabel>
</rdf:Description>

<rdf:Description rdf:about="http://iflastandards.info/ns/lrm/lrmoo/R17_created">
	<rdf:type rdf:resource="http://www.w3.org/2002/07/owl#ObjectProperty"/>
	<rdfs:subPropertyOf rdf:resource="http://www.cidoc-crm.org/cidoc-crm/P94_has_created"/>
	<owl:inverseOf rdf:resource="http://iflastandards.info/ns/lrm/lrmoo/R17i_was_created_by"/>
	<rdfs:domain rdf:resource="http://iflastandards.info/ns/lrm/lrmoo/F28_Expression_Creation"/>
	<rdfs:range rdf:resource="http://iflastandards.info/ns/lrm/lrmoo/F2_Expression"/>
	<rdfs:comment xml:lang="en">Quantification: one to many, necessary, dependent (1,n:1,1)

Scope note:
This property associates an instance of F2 Expression that was externalised during a particular instance of F28 Expression Creation event with that particular creation event. An instance of expression creation creates an instance of expression and also creates any expressions that are parts of that expression.

Examples:
- Agatha Christie creating the text for her novel ‘Murder on the Orient Express’ (F28) created the original English text of Agatha Christie’s ‘Murder on the Orient Express’ (F2).
- Elisabeth van Bebber creating the text of her translation of Agatha Christie’s ‘Murder on the Orient Express’ (F28) created the German text of Agatha Christie’s ‘Murder on the Orient Express’ (F2).
- Ludwig van Beethoven composing his ‘Symphony No. 9’ (F28) created the original score for the 9th Symphony (F2).
- The making of the censored version of Hitchcock’s movie ‘Psycho’ (F28) created the original version (cut) of the movie that was released in Britain (F2).
- The making of the first plaster version of ‘The Thinker’ sculpture by Auguste Rodin (F28) created the plaster version of ‘The Thinker’ (F2).
- The making of the large-scale version of ‘The Thinker’ by the Fonderie Alexis Rudier in 1904 (F28) created the large-scale version of ‘The Thinker’ (F2).
</rdfs:comment>
	<rdfs:label xml:lang="en">R17 created</rdfs:label>
	<skos:notation>R17</skos:notation>
	<skos:prefLabel xml:lang="en">created</skos:prefLabel>
</rdf:Description>

<rdf:Description rdf:about="http://iflastandards.info/ns/lrm/lrmoo/R17i_was_created_by">
	<rdf:type rdf:resource="http://www.w3.org/2002/07/owl#ObjectProperty"/>
	<rdfs:subPropertyOf rdf:resource="http://www.cidoc-crm.org/cidoc-crm/P94i_was_created_by"/>
	<rdfs:domain rdf:resource="http://iflastandards.info/ns/lrm/lrmoo/F2_Expression"/>
	<rdfs:range rdf:resource="http://iflastandards.info/ns/lrm/lrmoo/F28_Expression_Creation"/>
	<rdfs:comment xml:lang="en">Quantification of the inverse property: one to many, necessary, dependent (1,n:1,1)

Scope note of the inverse property:
This property associates an instance of F2 Expression that was externalised during a particular instance of F28 Expression Creation event with that particular creation event. An instance of expression creation creates an instance of expression and also creates any expressions that are parts of that expression.

Examples of the inverse property:
- Agatha Christie creating the text for her novel ‘Murder on the Orient Express’ (F28) created the original English text of Agatha Christie’s ‘Murder on the Orient Express’ (F2).
- Elisabeth van Bebber creating the text of her translation of Agatha Christie’s ‘Murder on the Orient Express’ (F28) created the German text of Agatha Christie’s ‘Murder on the Orient Express’ (F2).
- Ludwig van Beethoven composing his ‘Symphony No. 9’ (F28) created the original score for the 9th Symphony (F2).
- The making of the censored version of Hitchcock’s movie ‘Psycho’ (F28) created the original version (cut) of the movie that was released in Britain (F2).
- The making of the first plaster version of ‘The Thinker’ sculpture by Auguste Rodin (F28) created the plaster version of ‘The Thinker’ (F2).
- The making of the large-scale version of ‘The Thinker’ by the Fonderie Alexis Rudier in 1904 (F28) created the large-scale version of ‘The Thinker’ (F2).
</rdfs:comment>
	<rdfs:label xml:lang="en">R17i was created by</rdfs:label>
	<skos:notation>R17i</skos:notation>
	<skos:prefLabel xml:lang="en">was created by</skos:prefLabel>
</rdf:Description>

<rdf:Description rdf:about="http://iflastandards.info/ns/lrm/lrmoo/R19_created_a_realisation_of">
	<rdf:type rdf:resource="http://www.w3.org/2002/07/owl#ObjectProperty"/>
	<rdfs:subPropertyOf rdf:resource="http://www.cidoc-crm.org/cidoc-crm/P16_used_specific_object"/>
	<owl:inverseOf rdf:resource="http://iflastandards.info/ns/lrm/lrmoo/R19i_was_realised_through"/>
	<rdfs:domain rdf:resource="http://iflastandards.info/ns/lrm/lrmoo/F28_Expression_Creation"/>
	<rdfs:range rdf:resource="http://iflastandards.info/ns/lrm/lrmoo/F1_Work"/>
	<rdfs:comment xml:lang="en">Quantification: many to one, necessary, dependent (1,1:1,n)

Scope note:
This property associates an instance of F28 Expression Creation with the instance of F1 Work which was externalised in an instance of F2 Expression created by this creation event.

Examples:
- Agatha Christie writing the text for her novel ‘Murder on the Orient Express’ (F28) created a realization of Agatha Christie’s ‘Murder on the Orient Express’ (F1).
- Elisabeth van Bebber creating the text of her translation of Agatha Christie’s ‘Murder on the Orient Express’ (F28) created a realization of Agatha Christie’s ‘Murder on the Orient Express’ (F1).
- Ludwig van Beethoven composing his 9th symphony (F28) created a realization of Beethoven’s ‘Symphony No. 9’ (F1).
- The making of the censored version of Hitchcock’s movie ‘Psycho’ (F28) created a realization of Hitchcock’s movie ‘Psycho’ (F1).
- Auguste Rodin making the first plaster version of ‘The Thinker’ sculpture (F28) created a realization of Auguste Rodin’s ‘The Thinker’ (F1).
- The making of the large-scale version of ‘The Thinker’ by the Fonderie Alexis Rudier in 1904 (F28) created a realization of Auguste Rodin’s ‘The Thinker’ (F1).
</rdfs:comment>
	<rdfs:label xml:lang="en">R19 created a realisation of</rdfs:label>
	<skos:notation>R19</skos:notation>
	<skos:prefLabel xml:lang="en">created a realisation of</skos:prefLabel>
</rdf:Description>

<rdf:Description rdf:about="http://iflastandards.info/ns/lrm/lrmoo/R19i_was_realised_through">
	<rdf:type rdf:resource="http://www.w3.org/2002/07/owl#ObjectProperty"/>
	<rdfs:subPropertyOf rdf:resource="http://www.cidoc-crm.org/cidoc-crm/P16i_was_used_for"/>
	<rdfs:domain rdf:resource="http://iflastandards.info/ns/lrm/lrmoo/F1_Work"/>
	<rdfs:range rdf:resource="http://iflastandards.info/ns/lrm/lrmoo/F28_Expression_Creation"/>
	<rdfs:comment xml:lang="en">Quantification of the inverse property: many to one, necessary, dependent (1,1:1,n)

Scope note of the inverse property:
This property associates an instance of F28 Expression Creation with the instance of F1 Work which was externalised in an instance of F2 Expression created by this creation event.

Examples of the inverse property:
- Agatha Christie writing the text for her novel ‘Murder on the Orient Express’ (F28) created a realization of Agatha Christie’s ‘Murder on the Orient Express’ (F1).
- Elisabeth van Bebber creating the text of her translation of Agatha Christie’s ‘Murder on the Orient Express’ (F28) created a realization of Agatha Christie’s ‘Murder on the Orient Express’ (F1).
- Ludwig van Beethoven composing his 9th symphony (F28) created a realization of Beethoven’s ‘Symphony No. 9’ (F1).
- The making of the censored version of Hitchcock’s movie ‘Psycho’ (F28) created a realization of Hitchcock’s movie ‘Psycho’ (F1).
- Auguste Rodin making the first plaster version of ‘The Thinker’ sculpture (F28) created a realization of Auguste Rodin’s ‘The Thinker’ (F1).
- The making of the large-scale version of ‘The Thinker’ by the Fonderie Alexis Rudier in 1904 (F28) created a realization of Auguste Rodin’s ‘The Thinker’ (F1).
</rdfs:comment>
	<rdfs:label xml:lang="en">R19i was realised through</rdfs:label>
	<skos:notation>R19i</skos:notation>
	<skos:prefLabel xml:lang="en">was realised through</skos:prefLabel>
</rdf:Description>

<rdf:Description rdf:about="http://iflastandards.info/ns/lrm/lrmoo/R1_is_logical_successor_of">
	<rdf:type rdf:resource="http://www.w3.org/2002/07/owl#ObjectProperty"/>
	<rdfs:subPropertyOf rdf:resource="http://www.cidoc-crm.org/cidoc-crm/P130_shows_features_of"/>
	<owl:inverseOf rdf:resource="http://iflastandards.info/ns/lrm/lrmoo/R1i_has_successor"/>
	<rdfs:domain rdf:resource="http://iflastandards.info/ns/lrm/lrmoo/F1_Work"/>
	<rdfs:range rdf:resource="http://iflastandards.info/ns/lrm/lrmoo/F1_Work"/>
	<rdfs:comment xml:lang="en">Quantification: many to many (0,n:0,n)

Scope note:
This property associates an instance of F1 Work which logically continues the content of another instance of F1 Work with the latter. This property is not transitive. It is asymmetric and irreflexive.

Examples:
- Ursula K. Le Guin’s novel ‘The Tombs of Atuan’ (F1) is logical successor of Ursula K. Le Guin’s novel ‘A Wizard of Earthsea’ (F1).
- Miguel de Cervantes’ ‘Segunda Parte del Ingenioso Cavallero Don Quixote de la Mancha’ (F1) is logical successor of Miguel de Cervantes’ ‘El ingenioso hidalgo Don Quixote de la Mancha’ (F1).
- The TV series ‘Breaking Bad’ (F1) is logical successor of the TV series ‘Better Call Saul’ (F1).
- The first ‘Star Wars’ trilogy, 1977-1983 (F1) is logical successor of the second ‘Star Wars’ trilogy, 1999-2005 (F1). [Note that the logical order does not follow, in either of the two last examples, the chronological order of creation]
</rdfs:comment>
	<rdfs:label xml:lang="en">R1 is logical successor of</rdfs:label>
	<skos:notation>R1</skos:notation>
	<skos:prefLabel xml:lang="en">is logical successor of</skos:prefLabel>
</rdf:Description>

<rdf:Description rdf:about="http://iflastandards.info/ns/lrm/lrmoo/R1i_has_successor">
	<rdf:type rdf:resource="http://www.w3.org/2002/07/owl#ObjectProperty"/>
	<rdfs:subPropertyOf rdf:resource="http://www.cidoc-crm.org/cidoc-crm/P130i_features_are_also_found_on"/>
	<rdfs:domain rdf:resource="http://iflastandards.info/ns/lrm/lrmoo/F1_Work"/>
	<rdfs:range rdf:resource="http://iflastandards.info/ns/lrm/lrmoo/F1_Work"/>
	<rdfs:comment xml:lang="en">Quantification of the inverse property: many to many (0,n:0,n)

Scope note of the inverse property:
This property associates an instance of F1 Work which logically continues the content of another instance of F1 Work with the latter. This property is not transitive. It is asymmetric and irreflexive.

Examples of the inverse property:
- Ursula K. Le Guin’s novel ‘The Tombs of Atuan’ (F1) is logical successor of Ursula K. Le Guin’s novel ‘A Wizard of Earthsea’ (F1).
- Miguel de Cervantes’ ‘Segunda Parte del Ingenioso Cavallero Don Quixote de la Mancha’ (F1) is logical successor of Miguel de Cervantes’ ‘El ingenioso hidalgo Don Quixote de la Mancha’ (F1).
- The TV series ‘Breaking Bad’ (F1) is logical successor of the TV series ‘Better Call Saul’ (F1).
- The first ‘Star Wars’ trilogy, 1977-1983 (F1) is logical successor of the second ‘Star Wars’ trilogy, 1999-2005 (F1). [Note that the logical order does not follow, in either of the two last examples, the chronological order of creation]
</rdfs:comment>
	<rdfs:label xml:lang="en">R1i has successor</rdfs:label>
	<skos:notation>R1i</skos:notation>
	<skos:prefLabel xml:lang="en">has successor</skos:prefLabel>
</rdf:Description>

<rdf:Description rdf:about="http://iflastandards.info/ns/lrm/lrmoo/R24_created">
	<rdf:type rdf:resource="http://www.w3.org/2002/07/owl#ObjectProperty"/>
	<rdfs:subPropertyOf rdf:resource="http://www.cidoc-crm.org/cidoc-crm/P94_has_created"/>
	<owl:inverseOf rdf:resource="http://iflastandards.info/ns/lrm/lrmoo/R24i_was_created_through"/>
	<rdfs:domain rdf:resource="http://iflastandards.info/ns/lrm/lrmoo/F30_Manifestation_Creation"/>
	<rdfs:range rdf:resource="http://iflastandards.info/ns/lrm/lrmoo/F3_Manifestation"/>
	<rdfs:comment xml:lang="en">Quantification: one to many, necessary, dependent (1,n:1,1)

Scope note:
This property associates the instance of F3 Manifestation that was created during a particular instance of F30 Manifestation Creation with that instance of F30 Manifestation Creation event.

Examples:
- The process of creating the publication ‘Murder on the Orient Express / Agatha Christie’ as published by HarperCollins in 2017 (F30) created ‘Murder on the Orient Express / Agatha Christie’ published by HarperCollins in 2017 (F3).
- The process of making the HTML-version of the English text of Homer’s ‘Odyssey’ (as available online from the Gutenberg Project) (F30) created the HTML-version of the English text of Homer’s ‘Odyssey’ (F3).
- The process of making the CD publication ‘Bach Goldberg Variations’ (as published by Hyperion Records in 2016) (F30) created ‘Bach Goldberg Variations’, published by Hyperion Records in 2016 (F3).
</rdfs:comment>
	<rdfs:label xml:lang="en">R24 created</rdfs:label>
	<skos:notation>R24</skos:notation>
	<skos:prefLabel xml:lang="en">created</skos:prefLabel>
</rdf:Description>

<rdf:Description rdf:about="http://iflastandards.info/ns/lrm/lrmoo/R24i_was_created_through">
	<rdf:type rdf:resource="http://www.w3.org/2002/07/owl#ObjectProperty"/>
	<rdfs:subPropertyOf rdf:resource="http://www.cidoc-crm.org/cidoc-crm/P94i_was_created_by"/>
	<rdfs:domain rdf:resource="http://iflastandards.info/ns/lrm/lrmoo/F3_Manifestation"/>
	<rdfs:range rdf:resource="http://iflastandards.info/ns/lrm/lrmoo/F30_Manifestation_Creation"/>
	<rdfs:comment xml:lang="en">Quantification of the inverse property: one to many, necessary, dependent (1,n:1,1)

Scope note of the inverse property:
This property associates the instance of F3 Manifestation that was created during a particular instance of F30 Manifestation Creation with that instance of F30 Manifestation Creation event.

Examples of the inverse property:
- The process of creating the publication ‘Murder on the Orient Express / Agatha Christie’ as published by HarperCollins in 2017 (F30) created ‘Murder on the Orient Express / Agatha Christie’ published by HarperCollins in 2017 (F3).
- The process of making the HTML-version of the English text of Homer’s ‘Odyssey’ (as available online from the Gutenberg Project) (F30) created the HTML-version of the English text of Homer’s ‘Odyssey’ (F3).
- The process of making the CD publication ‘Bach Goldberg Variations’ (as published by Hyperion Records in 2016) (F30) created ‘Bach Goldberg Variations’, published by Hyperion Records in 2016 (F3).
</rdfs:comment>
	<rdfs:label xml:lang="en">R24i was created through</rdfs:label>
	<skos:notation>R24i</skos:notation>
	<skos:prefLabel xml:lang="en">was created through</skos:prefLabel>
</rdf:Description>

<rdf:Description rdf:about="http://iflastandards.info/ns/lrm/lrmoo/R27_materialized">
	<rdf:type rdf:resource="http://www.w3.org/2002/07/owl#ObjectProperty"/>
	<rdfs:subPropertyOf rdf:resource="http://www.cidoc-crm.org/cidoc-crm/P16_used_specific_object"/>
	<owl:inverseOf rdf:resource="http://iflastandards.info/ns/lrm/lrmoo/R27i_was_materialized_by"/>
	<rdfs:domain rdf:resource="http://iflastandards.info/ns/lrm/lrmoo/F32_Item_Production_Event"/>
	<rdfs:range rdf:resource="http://iflastandards.info/ns/lrm/lrmoo/F3_Manifestation"/>
	<rdfs:comment xml:lang="en">Quantification: many to many (0,n:0,n)

Scope note:
This property associates an instance of F32 Item Production Event with the set of signs provided by the publisher to be carried by all of the produced items (i.e., the instances of F5 Item) and any other physical features foreseen as integral to the instance of F3 Manifestation that is materialised.

Examples:
- The production of copies of the paperback edition of the HarperCollins 2017 publication ‘Murder on the Orient Express / Agatha Christie’ (F32) materialized the publication ‘Murder on the Orient Express / Agatha Christie’ published by HarperCollins 2017 (F3).
- The printing of the score of Bach’s ‘Goldberg Variations’ by Balthasar Schmid in 1741 (F32) materialized the publication Bach’s ‘Goldberg Variations’ as published by Balthasar Schmid in 1741 (F3).
</rdfs:comment>
	<rdfs:label xml:lang="en">R27 materialized</rdfs:label>
	<skos:notation>R27</skos:notation>
	<skos:prefLabel xml:lang="en">materialized</skos:prefLabel>
</rdf:Description>

<rdf:Description rdf:about="http://iflastandards.info/ns/lrm/lrmoo/R27i_was_materialized_by">
	<rdf:type rdf:resource="http://www.w3.org/2002/07/owl#ObjectProperty"/>
	<rdfs:subPropertyOf rdf:resource="http://www.cidoc-crm.org/cidoc-crm/P16i_was_used_for"/>
	<rdfs:domain rdf:resource="http://iflastandards.info/ns/lrm/lrmoo/F3_Manifestation"/>
	<rdfs:range rdf:resource="http://iflastandards.info/ns/lrm/lrmoo/F32_Item_Production_Event"/>
	<rdfs:comment xml:lang="en">Quantification of the inverse property: many to many (0,n:0,n)

Scope note of the inverse property:
This property associates an instance of F32 Item Production Event with the set of signs provided by the publisher to be carried by all of the produced items (i.e., the instances of F5 Item) and any other physical features foreseen as integral to the instance of F3 Manifestation that is materialised.

Examples of the inverse property:
- The production of copies of the paperback edition of the HarperCollins 2017 publication ‘Murder on the Orient Express / Agatha Christie’ (F32) materialized the publication ‘Murder on the Orient Express / Agatha Christie’ published by HarperCollins 2017 (F3).
- The printing of the score of Bach’s ‘Goldberg Variations’ by Balthasar Schmid in 1741 (F32) materialized the publication Bach’s ‘Goldberg Variations’ as published by Balthasar Schmid in 1741 (F3).
</rdfs:comment>
	<rdfs:label xml:lang="en">R27i was materialized by</rdfs:label>
	<skos:notation>R27i</skos:notation>
	<skos:prefLabel xml:lang="en">was materialized by</skos:prefLabel>
</rdf:Description>

<rdf:Description rdf:about="http://iflastandards.info/ns/lrm/lrmoo/R28_produced">
	<rdf:type rdf:resource="http://www.w3.org/2002/07/owl#ObjectProperty"/>
	<rdfs:subPropertyOf rdf:resource="http://www.cidoc-crm.org/cidoc-crm/P108_has_produced"/>
	<owl:inverseOf rdf:resource="http://iflastandards.info/ns/lrm/lrmoo/R28i_was_produced_by"/>
	<rdfs:domain rdf:resource="http://iflastandards.info/ns/lrm/lrmoo/F32_Item_Production_Event"/>
	<rdfs:range rdf:resource="http://iflastandards.info/ns/lrm/lrmoo/F5_Item"/>
	<rdfs:comment xml:lang="en">Quantification: one to many, necessary, dependent (1,n:1,1)

Scope note:
This property associates an instance of F32 Item Production Event with any one of the produced items (i.e., the instances of F5 Item).

Examples:
- The production of copies of the paperback edition of the HarperCollins 2017 publication ‘Murder on the Orient Express / Agatha Christie’ (F32) produced the copy (item) of this publication that is held by the Deichman public library in Oslo, Norway, and which is identified by inventory number ‘9138513’ (F5).
- The printing of the score of Bach’s ‘Goldberg Variations’ by Balthasar Schmid in 1741 (F32) produced the copy of this score (item) that is held by the National Library in France (F5).
- The second print run, occurring in 1978, of the publication dated of 1972 and entitled ‘The complete poems of Stephen Crane, edited with an introduction by Joseph Katz’ (identified by ISBN ‘0-8014-9130-4’) (F32) produced Universitätsbibliothek Passau’s holding identified by call number ‘00/HT 4801.978 K2’ (F5).
</rdfs:comment>
	<rdfs:label xml:lang="en">R28 produced</rdfs:label>
	<skos:notation>R28</skos:notation>
	<skos:prefLabel xml:lang="en">produced</skos:prefLabel>
</rdf:Description>

<rdf:Description rdf:about="http://iflastandards.info/ns/lrm/lrmoo/R28i_was_produced_by">
	<rdf:type rdf:resource="http://www.w3.org/2002/07/owl#ObjectProperty"/>
	<rdfs:subPropertyOf rdf:resource="http://www.cidoc-crm.org/cidoc-crm/P108i_was_produced_by"/>
	<rdfs:domain rdf:resource="http://iflastandards.info/ns/lrm/lrmoo/F5_Item"/>
	<rdfs:range rdf:resource="http://iflastandards.info/ns/lrm/lrmoo/F32_Item_Production_Event"/>
	<rdfs:comment xml:lang="en">Quantification of the inverse property: one to many, necessary, dependent (1,n:1,1)

Scope note of the inverse property:
This property associates an instance of F32 Item Production Event with any one of the produced items (i.e., the instances of F5 Item).

Examples of the inverse property:
- The production of copies of the paperback edition of the HarperCollins 2017 publication ‘Murder on the Orient Express / Agatha Christie’ (F32) produced the copy (item) of this publication that is held by the Deichman public library in Oslo, Norway, and which is identified by inventory number ‘9138513’ (F5).
- The printing of the score of Bach’s ‘Goldberg Variations’ by Balthasar Schmid in 1741 (F32) produced the copy of this score (item) that is held by the National Library in France (F5).
- The second print run, occurring in 1978, of the publication dated of 1972 and entitled ‘The complete poems of Stephen Crane, edited with an introduction by Joseph Katz’ (identified by ISBN ‘0-8014-9130-4’) (F32) produced Universitätsbibliothek Passau’s holding identified by call number ‘00/HT 4801.978 K2’ (F5).
</rdfs:comment>
	<rdfs:label xml:lang="en">R28i was produced by</rdfs:label>
	<skos:notation>R28i</skos:notation>
	<skos:prefLabel xml:lang="en">was produced by</skos:prefLabel>
</rdf:Description>

<rdf:Description rdf:about="http://iflastandards.info/ns/lrm/lrmoo/R29_reproduced_object">
	<rdf:type rdf:resource="http://www.w3.org/2002/07/owl#ObjectProperty"/>
	<rdfs:subPropertyOf rdf:resource="http://www.cidoc-crm.org/cidoc-crm/P16_used_specific_object"/>
	<owl:inverseOf rdf:resource="http://iflastandards.info/ns/lrm/lrmoo/R29i_was_object_reproduced_by"/>
	<rdfs:domain rdf:resource="http://iflastandards.info/ns/lrm/lrmoo/F33_Reproduction_Event"/>
	<rdfs:range rdf:resource="http://iflastandards.info/ns/lrm/lrmoo/F5_Item"/>
	<rdfs:comment xml:lang="en">Quantification: many to many, necessary (1,n:0,n)

Scope note:
This property associates an instance of F33 Reproduction Event with an instance of F5 Item it reproduces.

Examples:
- The activity performed by Schott when producing the 2015 publication of Harry Partch’s ‘Two studies on ancient Greek scales’ (F33) reproduced object Harry Partch’s holograph manuscript of ‘Two studies on ancient Greek scales’ (F5).
</rdfs:comment>
	<rdfs:label xml:lang="en">R29 reproduced object</rdfs:label>
	<skos:notation>R29</skos:notation>
	<skos:prefLabel xml:lang="en">reproduced object</skos:prefLabel>
</rdf:Description>

<rdf:Description rdf:about="http://iflastandards.info/ns/lrm/lrmoo/R29i_was_object_reproduced_by">
	<rdf:type rdf:resource="http://www.w3.org/2002/07/owl#ObjectProperty"/>
	<rdfs:subPropertyOf rdf:resource="http://www.cidoc-crm.org/cidoc-crm/P16i_was_used_for"/>
	<rdfs:domain rdf:resource="http://iflastandards.info/ns/lrm/lrmoo/F5_Item"/>
	<rdfs:range rdf:resource="http://iflastandards.info/ns/lrm/lrmoo/F33_Reproduction_Event"/>
	<rdfs:comment xml:lang="en">Quantification of the inverse property: many to many, necessary (1,n:0,n)

Scope note of the inverse property:
This property associates an instance of F33 Reproduction Event with an instance of F5 Item it reproduces.

Examples of the inverse property:
- The activity performed by Schott when producing the 2015 publication of Harry Partch’s ‘Two studies on ancient Greek scales’ (F33) reproduced object Harry Partch’s holograph manuscript of ‘Two studies on ancient Greek scales’ (F5).
</rdfs:comment>
	<rdfs:label xml:lang="en">R29i was object reproduced by</rdfs:label>
	<skos:notation>R29i</skos:notation>
	<skos:prefLabel xml:lang="en">was object reproduced by</skos:prefLabel>
</rdf:Description>

<rdf:Description rdf:about="http://iflastandards.info/ns/lrm/lrmoo/R2_is_derivative_of">
	<rdf:type rdf:resource="http://www.w3.org/2002/07/owl#ObjectProperty"/>
	<rdfs:subPropertyOf rdf:resource="http://iflastandards.info/ns/lrm/lrmoo/R68_is_inspired_by"/>
	<owl:inverseOf rdf:resource="http://iflastandards.info/ns/lrm/lrmoo/R2i_has_derivative"/>
	<rdfs:domain rdf:resource="http://iflastandards.info/ns/lrm/lrmoo/F1_Work"/>
	<rdfs:range rdf:resource="http://iflastandards.info/ns/lrm/lrmoo/F1_Work"/>
	<rdfs:comment xml:lang="en">Quantification: many to many (0,n:0,n)

Scope note:
This property associates an instance of F1 Work which modifies the content of another instance of F1 Work with the latter. This property is transitive, asymmetric and irreflexive.
The inverse of this property is equivalent to the developed path: F1 Work(1). R3 is realised in: F2 Expression(1). P16i was used for: F28 Expression Creation. R17 created: F2 Expression(2). R3i realises: F1 Work(2). That is, F1 Work(1). R2i has derivative: F1 Work (2), without needing to specify the specific expressions involved in the derivation.

Examples:
- The movie ‘Murder on the Orient Express’ directed by Kenneth Branagh (F1) is derivative of the novel ‘Murder on the Orient Express’ by Agatha Christie (F1) with has type Movie adaptation (E55).
- The movie ‘A Clockwork Orange’ directed by Stanley Kubrick (F1) is derivative of the novel ‘A Clockwork Orange’ by Anthony Burgess (F1) with has type Movie adaptation (E55).
- Seth Grahame-Smith’s novel ‘Pride and prejudice and zombies’(F1) is derivative of Jane Austen’s novel ‘Pride and prejudice’ (F1) with has type Parody (E55).

Properties:
- R2.1 has type: 
  Scope note:
    This property allows for specifying the kind of derivation, such as adaptation, summarisation, etc.
</rdfs:comment>
	<rdfs:label xml:lang="en">R2 is derivative of</rdfs:label>
	<skos:notation>R2</skos:notation>
	<skos:prefLabel xml:lang="en">is derivative of</skos:prefLabel>
</rdf:Description>

<rdf:Description rdf:about="http://iflastandards.info/ns/lrm/lrmoo/R2i_has_derivative">
	<rdf:type rdf:resource="http://www.w3.org/2002/07/owl#ObjectProperty"/>
	<rdfs:subPropertyOf rdf:resource="http://iflastandards.info/ns/lrm/lrmoo/R68i_is_inspiration_for"/>
	<rdfs:domain rdf:resource="http://iflastandards.info/ns/lrm/lrmoo/F1_Work"/>
	<rdfs:range rdf:resource="http://iflastandards.info/ns/lrm/lrmoo/F1_Work"/>
	<rdfs:comment xml:lang="en">Quantification of the inverse property: many to many (0,n:0,n)

Scope note of the inverse property:
This property associates an instance of F1 Work which modifies the content of another instance of F1 Work with the latter. This property is transitive, asymmetric and irreflexive.
The inverse of this property is equivalent to the developed path: F1 Work(1). R3 is realised in: F2 Expression(1). P16i was used for: F28 Expression Creation. R17 created: F2 Expression(2). R3i realises: F1 Work(2). That is, F1 Work(1). R2i has derivative: F1 Work (2), without needing to specify the specific expressions involved in the derivation.

Examples of the inverse property:
- The movie ‘Murder on the Orient Express’ directed by Kenneth Branagh (F1) is derivative of the novel ‘Murder on the Orient Express’ by Agatha Christie (F1) with has type Movie adaptation (E55).
- The movie ‘A Clockwork Orange’ directed by Stanley Kubrick (F1) is derivative of the novel ‘A Clockwork Orange’ by Anthony Burgess (F1) with has type Movie adaptation (E55).
- Seth Grahame-Smith’s novel ‘Pride and prejudice and zombies’(F1) is derivative of Jane Austen’s novel ‘Pride and prejudice’ (F1) with has type Parody (E55).
</rdfs:comment>
	<rdfs:label xml:lang="en">R2i has derivative</rdfs:label>
	<skos:notation>R2i</skos:notation>
	<skos:prefLabel xml:lang="en">has derivative</skos:prefLabel>
</rdf:Description>

<rdf:Description rdf:about="http://iflastandards.info/ns/lrm/lrmoo/R30_reproduced_publication">
	<rdf:type rdf:resource="http://www.w3.org/2002/07/owl#ObjectProperty"/>
	<rdfs:subPropertyOf rdf:resource="http://www.cidoc-crm.org/cidoc-crm/P16_used_specific_object"/>
	<owl:inverseOf rdf:resource="http://iflastandards.info/ns/lrm/lrmoo/R30i_was_publication_reproduced_by"/>
	<rdfs:domain rdf:resource="http://iflastandards.info/ns/lrm/lrmoo/F33_Reproduction_Event"/>
	<rdfs:range rdf:resource="http://iflastandards.info/ns/lrm/lrmoo/F3_Manifestation"/>
	<rdfs:comment xml:lang="en">Quantification: many to many, necessary (1,n:0,n)

Scope note:
This property associates an instance of F33 Reproduction Event with an instance of F3 Manifestation it reproduces.

Examples:
- The activity performed by Cambridge University Press when producing the 2014 publication of Daniel Wilson’s ‘Caliban: the missing link’ (F33) reproduced publication the 1873 publication of Daniel Wilson’s ‘Caliban: the missing link’ by Macmillan (F3).
- The activity performed by the Éditions du Seuil when producing the 2007 publication of Hubert Reeve’s ‘Malicorne: réflexions d’un observateur de la nature’ as number 179 in the series ‘Points. Science’ (identified by ISBN ‘978-2-02-096760-0’) (F33) reproduced publication the 1990 publication by the Éditions du Seuil in the series ‘Science ouverte’ (identified by ISBN ‘2-02-012644-3’) (F3).
</rdfs:comment>
	<rdfs:label xml:lang="en">R30 reproduced publication</rdfs:label>
	<skos:notation>R30</skos:notation>
	<skos:prefLabel xml:lang="en">reproduced publication</skos:prefLabel>
</rdf:Description>

<rdf:Description rdf:about="http://iflastandards.info/ns/lrm/lrmoo/R30i_was_publication_reproduced_by">
	<rdf:type rdf:resource="http://www.w3.org/2002/07/owl#ObjectProperty"/>
	<rdfs:subPropertyOf rdf:resource="http://www.cidoc-crm.org/cidoc-crm/P16i_was_used_for"/>
	<rdfs:domain rdf:resource="http://iflastandards.info/ns/lrm/lrmoo/F3_Manifestation"/>
	<rdfs:range rdf:resource="http://iflastandards.info/ns/lrm/lrmoo/F33_Reproduction_Event"/>
	<rdfs:comment xml:lang="en">Quantification of the inverse property: many to many, necessary (1,n:0,n)

Scope note of the inverse property:
This property associates an instance of F33 Reproduction Event with an instance of F3 Manifestation it reproduces.

Examples of the inverse property:
- The activity performed by Cambridge University Press when producing the 2014 publication of Daniel Wilson’s ‘Caliban: the missing link’ (F33) reproduced publication the 1873 publication of Daniel Wilson’s ‘Caliban: the missing link’ by Macmillan (F3).
- The activity performed by the Éditions du Seuil when producing the 2007 publication of Hubert Reeve’s ‘Malicorne: réflexions d’un observateur de la nature’ as number 179 in the series ‘Points. Science’ (identified by ISBN ‘978-2-02-096760-0’) (F33) reproduced publication the 1990 publication by the Éditions du Seuil in the series ‘Science ouverte’ (identified by ISBN ‘2-02-012644-3’) (F3).
</rdfs:comment>
	<rdfs:label xml:lang="en">R30i was publication reproduced by</rdfs:label>
	<skos:notation>R30i</skos:notation>
	<skos:prefLabel xml:lang="en">was publication reproduced by</skos:prefLabel>
</rdf:Description>

<rdf:Description rdf:about="http://iflastandards.info/ns/lrm/lrmoo/R35_is_specified_by">
	<rdf:type rdf:resource="http://www.w3.org/2002/07/owl#ObjectProperty"/>
	<rdfs:subPropertyOf rdf:resource="http://www.cidoc-crm.org/cidoc-crm/P67i_is_referred_to_by"/>
	<owl:inverseOf rdf:resource="http://iflastandards.info/ns/lrm/lrmoo/R35i_specifies"/>
	<rdfs:domain rdf:resource="http://iflastandards.info/ns/lrm/lrmoo/F12_Nomen"/>
	<rdfs:range rdf:resource="http://iflastandards.info/ns/lrm/lrmoo/F2_Expression"/>
	<rdfs:comment xml:lang="en">Quantification: many to one, necessary, dependent (1,1:1,n)

Scope note:
This property associates an instance of F12 Nomen with an instance of F2 Expression which documents, defines or provides evidence for the particular nomen in the stated sense.

Examples:
- ‘acoustic surface wave device’ as a term for the device (F12) is specified by INSPEC Thesaurus version January 1973 (F2).
- ‘595.7’ as a classification number for the taxonomic class Insecta (insects) (F12) is specified by the 23(rd) edition of the Dewey Decimal Classification (DDC) (F2).
- ‘Martin Doerr’ as the name of a co-chair of the CIDOC CRM SIG (F12) is specified by the statement on the title page of the Definition of the ‘CIDOC Conceptual Reference Model’, Version 7.1.3, February 2024 (F2).
</rdfs:comment>
	<rdfs:label xml:lang="en">R35 is specified by</rdfs:label>
	<skos:notation>R35</skos:notation>
	<skos:prefLabel xml:lang="en">is specified by</skos:prefLabel>
</rdf:Description>

<rdf:Description rdf:about="http://iflastandards.info/ns/lrm/lrmoo/R35i_specifies">
	<rdf:type rdf:resource="http://www.w3.org/2002/07/owl#ObjectProperty"/>
	<rdfs:subPropertyOf rdf:resource="http://www.cidoc-crm.org/cidoc-crm/P67_refers_to"/>
	<rdfs:domain rdf:resource="http://iflastandards.info/ns/lrm/lrmoo/F2_Expression"/>
	<rdfs:range rdf:resource="http://iflastandards.info/ns/lrm/lrmoo/F12_Nomen"/>
	<rdfs:comment xml:lang="en">Quantification of the inverse property: many to one, necessary, dependent (1,1:1,n)

Scope note of the inverse property:
This property associates an instance of F12 Nomen with an instance of F2 Expression which documents, defines or provides evidence for the particular nomen in the stated sense.

Examples of the inverse property:
- ‘acoustic surface wave device’ as a term for the device (F12) is specified by INSPEC Thesaurus version January 1973 (F2).
- ‘595.7’ as a classification number for the taxonomic class Insecta (insects) (F12) is specified by the 23(rd) edition of the Dewey Decimal Classification (DDC) (F2).
- ‘Martin Doerr’ as the name of a co-chair of the CIDOC CRM SIG (F12) is specified by the statement on the title page of the Definition of the ‘CIDOC Conceptual Reference Model’, Version 7.1.3, February 2024 (F2).
</rdfs:comment>
	<rdfs:label xml:lang="en">R35i specifies</rdfs:label>
	<skos:notation>R35i</skos:notation>
	<skos:prefLabel xml:lang="en">specifies</skos:prefLabel>
</rdf:Description>

<rdf:Description rdf:about="http://iflastandards.info/ns/lrm/lrmoo/R36_uses_script_conversion">
	<rdf:type rdf:resource="http://www.w3.org/2002/07/owl#ObjectProperty"/>
	<owl:inverseOf rdf:resource="http://iflastandards.info/ns/lrm/lrmoo/R36i_is_script_conversion_used_in"/>
	<rdfs:domain rdf:resource="http://iflastandards.info/ns/lrm/lrmoo/F12_Nomen"/>
	<rdfs:range rdf:resource="http://iflastandards.info/ns/lrm/lrmoo/F36_Script_Conversion"/>
	<rdfs:comment xml:lang="en">Quantification: many to many (0,n:0,n)

Shortcut Of: F12 Nomen. R17i was created by (created): E65 Creation. P33 used specific technique (was used by): E29 Design or Procedure

Scope note:
This property associates an instance of F12 Nomen with an instance of F36 Script Conversion that is used to create the E62 String used in that instance of F12 Nomen from the string used in another instance of F12 Nomen that co-refers with the first nomen (the instances of F12 Nomen are related via the R56 has related form (is related form of) property). The source of this conversion may or may not be explicitly mentioned.

Examples:
- ‘Du Fu’ as the name for a Chinese poet of the 8(th) century (F12) uses script conversion Pinyin (F36).
- ‘Čajkovskij, Petr Ilʹič’ as the name of a Russian composer (F12) uses script conversion ‘ISO 9:1995 Information and documentation — Transliteration of Cyrillic characters into Latin characters — Slavic and non-Slavic languages’ (F36).
</rdfs:comment>
	<rdfs:label xml:lang="en">R36 uses script conversion</rdfs:label>
	<skos:notation>R36</skos:notation>
	<skos:prefLabel xml:lang="en">uses script conversion</skos:prefLabel>
</rdf:Description>

<rdf:Description rdf:about="http://iflastandards.info/ns/lrm/lrmoo/R36i_is_script_conversion_used_in">
	<rdf:type rdf:resource="http://www.w3.org/2002/07/owl#ObjectProperty"/>
	<rdfs:domain rdf:resource="http://iflastandards.info/ns/lrm/lrmoo/F36_Script_Conversion"/>
	<rdfs:range rdf:resource="http://iflastandards.info/ns/lrm/lrmoo/F12_Nomen"/>
	<rdfs:comment xml:lang="en">Quantification of the inverse property: many to many (0,n:0,n)

Shortcut Of of the inverse property: F12 Nomen. R17i was created by (created): E65 Creation. P33 used specific technique (was used by): E29 Design or Procedure

Scope note of the inverse property:
This property associates an instance of F12 Nomen with an instance of F36 Script Conversion that is used to create the E62 String used in that instance of F12 Nomen from the string used in another instance of F12 Nomen that co-refers with the first nomen (the instances of F12 Nomen are related via the R56 has related form (is related form of) property). The source of this conversion may or may not be explicitly mentioned.

Examples of the inverse property:
- ‘Du Fu’ as the name for a Chinese poet of the 8(th) century (F12) uses script conversion Pinyin (F36).
- ‘Čajkovskij, Petr Ilʹič’ as the name of a Russian composer (F12) uses script conversion ‘ISO 9:1995 Information and documentation — Transliteration of Cyrillic characters into Latin characters — Slavic and non-Slavic languages’ (F36).
</rdfs:comment>
	<rdfs:label xml:lang="en">R36i is script conversion used in</rdfs:label>
	<skos:notation>R36i</skos:notation>
	<skos:prefLabel xml:lang="en">is script conversion used in</skos:prefLabel>
</rdf:Description>

<rdf:Description rdf:about="http://iflastandards.info/ns/lrm/lrmoo/R3_is_realised_in">
	<rdf:type rdf:resource="http://www.w3.org/2002/07/owl#ObjectProperty"/>
	<rdfs:subPropertyOf rdf:resource="http://www.cidoc-crm.org/cidoc-crm/P130_shows_features_of"/>
	<owl:inverseOf rdf:resource="http://iflastandards.info/ns/lrm/lrmoo/R3i_realises"/>
	<rdfs:domain rdf:resource="http://iflastandards.info/ns/lrm/lrmoo/F1_Work"/>
	<rdfs:range rdf:resource="http://iflastandards.info/ns/lrm/lrmoo/F2_Expression"/>
	<rdfs:comment xml:lang="en">Quantification: one to many, necessary, dependent (1,n:1,1)

Scope note:
This property associates an instance of F2 Expression with an instance of F1 Work.
This property expresses the association that exists between an expression and the work that this expression conveys. Our factual knowledge of how a given work is historically realised into expressions is often limited. Therefore, this property makes it possible to express the association between an instance of F2 Expression and the instance of F1 Work it conveys without identifying the particular instances of F2 Expression that were part of a chain of derivation from the source.

Examples:
- Agatha Christie’s work entitled ‘Murder on the Orient Express’ (F1) is realised in the original text written by Agatha Christie for the novel (F2).
- Agatha Christie’s work entitled ‘Murder on the Orient Express’ (F1) is realised in the German translation created by Elisabeth van Bebber (F2).
- Agatha Christie’s work entitled ‘Murder on the Orient Express’ (F1) is realised in the narration of the English text by David Suchet (F2).
- Dante’s work entitled ‘Inferno’ (F1) is realised in the Italian text of Dante’s ‘Inferno’ as found in the authoritative critical edition ‘La Commedia secondo l’antica issolu’ a cura di Giorgio Petrocchi, Milano: Mondadori, 1966-67 (= ‘Le Opere di Dante Alighieri’, Edizione Nazionale a cura della Società Dantesca Italiana, VII, 1-4) (F2).
- Johann Sebastian Bach’s ‘Goldberg Variations’ (F1) is realised in the score of the ‘Goldberg Variations’ (as published by Balthasar Schmid in 1741) (F2).
- Auguste Rodin’s work ‘The Thinker’ (F1) is realised in the first plaster version of ‘The thinker’ (F2) that Auguste Rodin made around 1881.
- Auguste Rodin’s work ‘The Thinker’ (F1) is realised in the large-scale version of ‘The thinker’ (F2) created at the Fonderie Alexis Rudier in 1904.
</rdfs:comment>
	<rdfs:label xml:lang="en">R3 is realised in</rdfs:label>
	<skos:notation>R3</skos:notation>
	<skos:prefLabel xml:lang="en">is realised in</skos:prefLabel>
</rdf:Description>

<rdf:Description rdf:about="http://iflastandards.info/ns/lrm/lrmoo/R3i_realises">
	<rdf:type rdf:resource="http://www.w3.org/2002/07/owl#ObjectProperty"/>
	<rdfs:subPropertyOf rdf:resource="http://www.cidoc-crm.org/cidoc-crm/P130i_features_are_also_found_on"/>
	<rdfs:domain rdf:resource="http://iflastandards.info/ns/lrm/lrmoo/F2_Expression"/>
	<rdfs:range rdf:resource="http://iflastandards.info/ns/lrm/lrmoo/F1_Work"/>
	<rdfs:comment xml:lang="en">Quantification of the inverse property: one to many, necessary, dependent (1,n:1,1)

Scope note of the inverse property:
This property associates an instance of F2 Expression with an instance of F1 Work.
This property expresses the association that exists between an expression and the work that this expression conveys. Our factual knowledge of how a given work is historically realised into expressions is often limited. Therefore, this property makes it possible to express the association between an instance of F2 Expression and the instance of F1 Work it conveys without identifying the particular instances of F2 Expression that were part of a chain of derivation from the source.

Examples of the inverse property:
- Agatha Christie’s work entitled ‘Murder on the Orient Express’ (F1) is realised in the original text written by Agatha Christie for the novel (F2).
- Agatha Christie’s work entitled ‘Murder on the Orient Express’ (F1) is realised in the German translation created by Elisabeth van Bebber (F2).
- Agatha Christie’s work entitled ‘Murder on the Orient Express’ (F1) is realised in the narration of the English text by David Suchet (F2).
- Dante’s work entitled ‘Inferno’ (F1) is realised in the Italian text of Dante’s ‘Inferno’ as found in the authoritative critical edition ‘La Commedia secondo l’antica issolu’ a cura di Giorgio Petrocchi, Milano: Mondadori, 1966-67 (= ‘Le Opere di Dante Alighieri’, Edizione Nazionale a cura della Società Dantesca Italiana, VII, 1-4) (F2).
- Johann Sebastian Bach’s ‘Goldberg Variations’ (F1) is realised in the score of the ‘Goldberg Variations’ (as published by Balthasar Schmid in 1741) (F2).
- Auguste Rodin’s work ‘The Thinker’ (F1) is realised in the first plaster version of ‘The thinker’ (F2) that Auguste Rodin made around 1881.
- Auguste Rodin’s work ‘The Thinker’ (F1) is realised in the large-scale version of ‘The thinker’ (F2) created at the Fonderie Alexis Rudier in 1904.
</rdfs:comment>
	<rdfs:label xml:lang="en">R3i realises</rdfs:label>
	<skos:notation>R3i</skos:notation>
	<skos:prefLabel xml:lang="en">realises</skos:prefLabel>
</rdf:Description>

<rdf:Description rdf:about="http://iflastandards.info/ns/lrm/lrmoo/R4_embodies">
	<rdf:type rdf:resource="http://www.w3.org/2002/07/owl#ObjectProperty"/>
	<rdfs:subPropertyOf rdf:resource="http://www.cidoc-crm.org/cidoc-crm/P165_incorporates"/>
	<owl:inverseOf rdf:resource="http://iflastandards.info/ns/lrm/lrmoo/R4i_is_embodied_in"/>
	<rdfs:domain rdf:resource="http://iflastandards.info/ns/lrm/lrmoo/F3_Manifestation"/>
	<rdfs:range rdf:resource="http://iflastandards.info/ns/lrm/lrmoo/F2_Expression"/>
	<rdfs:comment xml:lang="en">Quantification: many to many, necessary, dependent (1,n:1,n)

Scope note:
This property associates an instance of F3 Manifestation with one or more instances of F2 Expression which are rendered by this instance of F3 Manifestation. The manifestation formats the expression(s) in the way they are to be presented to some public, including specifying the intended sensory impression (such as visual appearance or audio rendition).

Examples:
- The publication ‘Murder on the Orient Express / Agatha Christie’, published by Collins Crime Club in 1934 (F3) embodies the original text in English by Agatha Christie (F2).
- The publication ‘Mord im Orientexpress: ein Hercule-Poirot-Roman / Agatha Christie’, published by Deutscher Bücherbund in 1975 (F3) embodies the German translation by Elisabeth van Bebber (F2).
- The publication ‘The Illustrated Odyssey’, published by Sidgwick &amp; Jackson Ltd in 1980 (F3) embodies the translated text by E. V. Rieu (F2), the introductory text by Jacquetta Hawkes (F2) and photographs by Tim Mercer (F2).
- The publication entitled ‘Alfred Hitchcock’s Psycho: 60th Anniversary Edition’ which was released in 2020 (F3), embodies the original cut of the movie (F2) and the censored version that was released in Britain (F2).
- The publication identified by ISBN ‘2-222-00835-2’ (F3) embodies the text of Marin Mersenne’s ‘Harmonie universelle’ (F2).
- The CD publication ‘Bach Goldberg Variations’ published by Hyperion Records in 2016 (F3), embodies Angela Hewitt’s performances of Bach’s ‘Goldberg Variations’ recorded in Christuskirche (Berlin) on 14-17 December 2015 (F2).
</rdfs:comment>
	<rdfs:label xml:lang="en">R4 embodies</rdfs:label>
	<skos:notation>R4</skos:notation>
	<skos:prefLabel xml:lang="en">embodies</skos:prefLabel>
</rdf:Description>

<rdf:Description rdf:about="http://iflastandards.info/ns/lrm/lrmoo/R4i_is_embodied_in">
	<rdf:type rdf:resource="http://www.w3.org/2002/07/owl#ObjectProperty"/>
	<rdfs:subPropertyOf rdf:resource="http://www.cidoc-crm.org/cidoc-crm/P165i_is_incorporated_in"/>
	<rdfs:domain rdf:resource="http://iflastandards.info/ns/lrm/lrmoo/F2_Expression"/>
	<rdfs:range rdf:resource="http://iflastandards.info/ns/lrm/lrmoo/F3_Manifestation"/>
	<rdfs:comment xml:lang="en">Quantification of the inverse property: many to many, necessary, dependent (1,n:1,n)

Scope note of the inverse property:
This property associates an instance of F3 Manifestation with one or more instances of F2 Expression which are rendered by this instance of F3 Manifestation. The manifestation formats the expression(s) in the way they are to be presented to some public, including specifying the intended sensory impression (such as visual appearance or audio rendition).

Examples of the inverse property:
- The publication ‘Murder on the Orient Express / Agatha Christie’, published by Collins Crime Club in 1934 (F3) embodies the original text in English by Agatha Christie (F2).
- The publication ‘Mord im Orientexpress: ein Hercule-Poirot-Roman / Agatha Christie’, published by Deutscher Bücherbund in 1975 (F3) embodies the German translation by Elisabeth van Bebber (F2).
- The publication ‘The Illustrated Odyssey’, published by Sidgwick &amp; Jackson Ltd in 1980 (F3) embodies the translated text by E. V. Rieu (F2), the introductory text by Jacquetta Hawkes (F2) and photographs by Tim Mercer (F2).
- The publication entitled ‘Alfred Hitchcock’s Psycho: 60th Anniversary Edition’ which was released in 2020 (F3), embodies the original cut of the movie (F2) and the censored version that was released in Britain (F2).
- The publication identified by ISBN ‘2-222-00835-2’ (F3) embodies the text of Marin Mersenne’s ‘Harmonie universelle’ (F2).
- The CD publication ‘Bach Goldberg Variations’ published by Hyperion Records in 2016 (F3), embodies Angela Hewitt’s performances of Bach’s ‘Goldberg Variations’ recorded in Christuskirche (Berlin) on 14-17 December 2015 (F2).
</rdfs:comment>
	<rdfs:label xml:lang="en">R4i is embodied in</rdfs:label>
	<skos:notation>R4i</skos:notation>
	<skos:prefLabel xml:lang="en">is embodied in</skos:prefLabel>
</rdf:Description>

<rdf:Description rdf:about="http://iflastandards.info/ns/lrm/lrmoo/R54_has_language">
	<rdf:type rdf:resource="http://www.w3.org/2002/07/owl#ObjectProperty"/>
	<rdfs:subPropertyOf rdf:resource="http://www.cidoc-crm.org/cidoc-crm/P2_has_type"/>
	<owl:inverseOf rdf:resource="http://iflastandards.info/ns/lrm/lrmoo/R54i_is_language_of"/>
	<rdfs:domain rdf:resource="http://iflastandards.info/ns/lrm/lrmoo/F12_Nomen"/>
	<rdfs:range rdf:resource="http://www.cidoc-crm.org/cidoc-crm/E56_Language"/>
	<rdfs:comment xml:lang="en">Quantification: many to many (0,n:0,n)

Scope note:
This property associates an instance of F12 Nomen with an instance of E56 Language which is the language used for or associated with the nomen.

Examples:
- ‘Colón Cristóbal’ as a name of the explorer and navigator (F12) has language Spanish [encoded as ‘spa’ in set 2 of ISO 639:2023] (E56).
- ‘Columbus Christopher’ as a name of the explorer and navigator (F12) has language English [encoded as ‘eng’ in set 2 of ISO 639:2023] (E56).
- ‘Conseil international des musées’ as a name of ICOM, the International Council of Museums (F12) has language French [encoded as ‘fre’ in set 2 of ISO 639:2023] (E56).
- ‘Internationaler Museumsrat’ as a name of ICOM, the International Council of Museums (F12) has language German [encoded as ‘ger’ in set 2 of ISO 639:2023] (E56).
- ‘Union européenne’ as a name of the European Union (F12) has language French [encoded as ‘fre’ in set 2 of ISO 639:2023] (E56).
- ‘Vienna’ as a name of the city which is the capital of Austria (F12) has language English [encoded as ‘eng’ in set 2 of ISO 639:2023] (E56).
- ‘Organic chemistry’ as a term for the branch of chemistry concerned with organic compounds (F12) has language English [encoded as ‘eng’ in set 2 of ISO 639:2023] (E56).
</rdfs:comment>
	<rdfs:label xml:lang="en">R54 has language</rdfs:label>
	<skos:notation>R54</skos:notation>
	<skos:prefLabel xml:lang="en">has language</skos:prefLabel>
</rdf:Description>

<rdf:Description rdf:about="http://iflastandards.info/ns/lrm/lrmoo/R54i_is_language_of">
	<rdf:type rdf:resource="http://www.w3.org/2002/07/owl#ObjectProperty"/>
	<rdfs:subPropertyOf rdf:resource="http://www.cidoc-crm.org/cidoc-crm/P2i_is_type_of"/>
	<rdfs:domain rdf:resource="http://www.cidoc-crm.org/cidoc-crm/E56_Language"/>
	<rdfs:range rdf:resource="http://iflastandards.info/ns/lrm/lrmoo/F12_Nomen"/>
	<rdfs:comment xml:lang="en">Quantification of the inverse property: many to many (0,n:0,n)

Scope note of the inverse property:
This property associates an instance of F12 Nomen with an instance of E56 Language which is the language used for or associated with the nomen.

Examples of the inverse property:
- ‘Colón Cristóbal’ as a name of the explorer and navigator (F12) has language Spanish [encoded as ‘spa’ in set 2 of ISO 639:2023] (E56).
- ‘Columbus Christopher’ as a name of the explorer and navigator (F12) has language English [encoded as ‘eng’ in set 2 of ISO 639:2023] (E56).
- ‘Conseil international des musées’ as a name of ICOM, the International Council of Museums (F12) has language French [encoded as ‘fre’ in set 2 of ISO 639:2023] (E56).
- ‘Internationaler Museumsrat’ as a name of ICOM, the International Council of Museums (F12) has language German [encoded as ‘ger’ in set 2 of ISO 639:2023] (E56).
- ‘Union européenne’ as a name of the European Union (F12) has language French [encoded as ‘fre’ in set 2 of ISO 639:2023] (E56).
- ‘Vienna’ as a name of the city which is the capital of Austria (F12) has language English [encoded as ‘eng’ in set 2 of ISO 639:2023] (E56).
- ‘Organic chemistry’ as a term for the branch of chemistry concerned with organic compounds (F12) has language English [encoded as ‘eng’ in set 2 of ISO 639:2023] (E56).
</rdfs:comment>
	<rdfs:label xml:lang="en">R54i is language of</rdfs:label>
	<skos:notation>R54i</skos:notation>
	<skos:prefLabel xml:lang="en">is language of</skos:prefLabel>
</rdf:Description>

<rdf:Description rdf:about="http://iflastandards.info/ns/lrm/lrmoo/R56_has_related_form">
	<rdf:type rdf:resource="http://www.w3.org/2002/07/owl#ObjectProperty"/>
	<owl:inverseOf rdf:resource="http://iflastandards.info/ns/lrm/lrmoo/R56i_is_related_form_of"/>
	<rdfs:domain rdf:resource="http://iflastandards.info/ns/lrm/lrmoo/F12_Nomen"/>
	<rdfs:range rdf:resource="http://iflastandards.info/ns/lrm/lrmoo/F12_Nomen"/>
	<rdfs:comment xml:lang="en">Quantification: many to many (0,n:0,n)

Shortcut Of: E89 Propositional Object (1). P67 refers to: E1 CRM Entity. P67i is referred to by: E89 Propositional Object (2)

Scope note:
This property associates an instance of F12 Nomen with another instance of F12 Nomen which co-refers to the same instance of E1 CRM Entity. This property is not transitive. It is symmetric and irreflexive.

Examples:
- ‘Čajkovskij, Petr Ilʹič’ as the name of the Russian composer (F12) has related form ‘Пётр Ильич Чайковский’ as the name of the Russian composer (F12) with has type Transliteration (E55).
- ‘The Lord of the Rings’ as the title of the work by J. R. R. Tolkien (F12) has related form ‘Le Seigneur des anneaux’ as the title of the work by J. R. R. Tolkien (F12) with has type Original language (E55).
- ‘IFLA’ as the name of the international association in the library field (F12) has related form ‘International Federation of Library Associations and Institutions’ as the name of the international association in the library field (F12) with has type Acronym (E55).
- ‘Siam’ as the name of the country in South Asia (F12) has related form ‘Thailand’ as the name of the country in South Asia (F12).
- ‘595.7’ as a classification number referring to the taxonomic class insects (F12) has related form ‘Insecta’ as a term referring to the taxonomic class insects (F12). [The latter being the caption for the Dewey Decimal Classification number in the English language 23(rd) edition.]

Properties:
- R56.1 has type: 
  Scope note:
    This property allows for specifying the particular kind of relationship that holds between the domain nomen and the range nomen, such as by being a derivation, an alternative, a lexical variant, etc. Typing the association may cause loss of symmetry.
</rdfs:comment>
	<rdfs:label xml:lang="en">R56 has related form</rdfs:label>
	<skos:notation>R56</skos:notation>
	<skos:prefLabel xml:lang="en">has related form</skos:prefLabel>
</rdf:Description>

<rdf:Description rdf:about="http://iflastandards.info/ns/lrm/lrmoo/R56i_is_related_form_of">
	<rdf:type rdf:resource="http://www.w3.org/2002/07/owl#ObjectProperty"/>
	<rdfs:domain rdf:resource="http://iflastandards.info/ns/lrm/lrmoo/F12_Nomen"/>
	<rdfs:range rdf:resource="http://iflastandards.info/ns/lrm/lrmoo/F12_Nomen"/>
	<rdfs:comment xml:lang="en">Quantification of the inverse property: many to many (0,n:0,n)

Shortcut Of of the inverse property: E89 Propositional Object (1). P67 refers to: E1 CRM Entity. P67i is referred to by: E89 Propositional Object (2)

Scope note of the inverse property:
This property associates an instance of F12 Nomen with another instance of F12 Nomen which co-refers to the same instance of E1 CRM Entity. This property is not transitive. It is symmetric and irreflexive.

Examples of the inverse property:
- ‘Čajkovskij, Petr Ilʹič’ as the name of the Russian composer (F12) has related form ‘Пётр Ильич Чайковский’ as the name of the Russian composer (F12) with has type Transliteration (E55).
- ‘The Lord of the Rings’ as the title of the work by J. R. R. Tolkien (F12) has related form ‘Le Seigneur des anneaux’ as the title of the work by J. R. R. Tolkien (F12) with has type Original language (E55).
- ‘IFLA’ as the name of the international association in the library field (F12) has related form ‘International Federation of Library Associations and Institutions’ as the name of the international association in the library field (F12) with has type Acronym (E55).
- ‘Siam’ as the name of the country in South Asia (F12) has related form ‘Thailand’ as the name of the country in South Asia (F12).
- ‘595.7’ as a classification number referring to the taxonomic class insects (F12) has related form ‘Insecta’ as a term referring to the taxonomic class insects (F12). [The latter being the caption for the Dewey Decimal Classification number in the English language 23(rd) edition.]
</rdfs:comment>
	<rdfs:label xml:lang="en">R56i is related form of</rdfs:label>
	<skos:notation>R56i</skos:notation>
	<skos:prefLabel xml:lang="en">is related form of</skos:prefLabel>
</rdf:Description>

<rdf:Description rdf:about="http://iflastandards.info/ns/lrm/lrmoo/R5_has_component">
	<rdf:type rdf:resource="http://www.w3.org/2002/07/owl#ObjectProperty"/>
	<rdfs:subPropertyOf rdf:resource="http://www.cidoc-crm.org/cidoc-crm/P148_has_component"/>
	<owl:inverseOf rdf:resource="http://iflastandards.info/ns/lrm/lrmoo/R5i_is_component_of"/>
	<rdfs:domain rdf:resource="http://iflastandards.info/ns/lrm/lrmoo/F2_Expression"/>
	<rdfs:range rdf:resource="http://iflastandards.info/ns/lrm/lrmoo/F2_Expression"/>
	<rdfs:comment xml:lang="en">Quantification: many to many (0,n:0,n)

Scope note:
This property associates an instance of an F2 Expression X with a structural component Y that conveys a part of the overall work realized by X, such as volumes, chapters, or sections. This property is transitive, asymmetric and irreflexive.
Any part of an expression that conveys complete propositions, such as a single phrase, can be documented using the more general property P148 has component (is component of).
Any part of an expression that does not completely follow meaningful boundaries, such as lines or pages of text or portions visible on images, can be documented using the property P106 is composed of (forms part of), and not with R5 has component (is component of). Fragments, in particular, can be documented with the more specific property R15 has fragment (is fragment of).
This property does not cover the relationship that exists between expressions that are realisations of different works, where one is re-used in a new, larger expression. Such a relationship is modelled by R75 incorporates (is incorporated in).

Examples:
- The musical notation for Bach’s ‘Goldberg Variations’ (F2) has component the musical notation for ‘Variatio 1. a 1 Clav’ (F2).
- The Italian text of Dante’s textual work entitled ‘Divina Commedia’ (F2) has component the Italian text of Dante’s textual work entitled ‘Inferno’ (F2).
- The musical notation of Mozart’s Singspiel entitled ‘Die Zauberflöte’ (F2) has component the musical notation of Mozart’s aria entitled ‘Der Hölle Rache’, also known as ‘The Queen of the Night’s Aria’ (F2).
- The visual content of the map entitled ‘Wales – The Midlands – South West England’, scale 1:400,000, issued by Michelin in 2005 (F2) has component the visual content of the inset entitled ‘Liverpool’, scale 1:200,000, set within the compass of the map titled ‘Wales – The Midlands – South West England’, scale 1:400,000, issued by Michelin in 2005 (F2).
</rdfs:comment>
	<rdfs:label xml:lang="en">R5 has component</rdfs:label>
	<skos:notation>R5</skos:notation>
	<skos:prefLabel xml:lang="en">has component</skos:prefLabel>
</rdf:Description>

<rdf:Description rdf:about="http://iflastandards.info/ns/lrm/lrmoo/R5i_is_component_of">
	<rdf:type rdf:resource="http://www.w3.org/2002/07/owl#ObjectProperty"/>
	<rdfs:subPropertyOf rdf:resource="http://www.cidoc-crm.org/cidoc-crm/P148i_is_component_of"/>
	<rdfs:domain rdf:resource="http://iflastandards.info/ns/lrm/lrmoo/F2_Expression"/>
	<rdfs:range rdf:resource="http://iflastandards.info/ns/lrm/lrmoo/F2_Expression"/>
	<rdfs:comment xml:lang="en">Quantification of the inverse property: many to many (0,n:0,n)

Scope note of the inverse property:
This property associates an instance of an F2 Expression X with a structural component Y that conveys a part of the overall work realized by X, such as volumes, chapters, or sections. This property is transitive, asymmetric and irreflexive.
Any part of an expression that conveys complete propositions, such as a single phrase, can be documented using the more general property P148 has component (is component of).
Any part of an expression that does not completely follow meaningful boundaries, such as lines or pages of text or portions visible on images, can be documented using the property P106 is composed of (forms part of), and not with R5 has component (is component of). Fragments, in particular, can be documented with the more specific property R15 has fragment (is fragment of).
This property does not cover the relationship that exists between expressions that are realisations of different works, where one is re-used in a new, larger expression. Such a relationship is modelled by R75 incorporates (is incorporated in).

Examples of the inverse property:
- The musical notation for Bach’s ‘Goldberg Variations’ (F2) has component the musical notation for ‘Variatio 1. a 1 Clav’ (F2).
- The Italian text of Dante’s textual work entitled ‘Divina Commedia’ (F2) has component the Italian text of Dante’s textual work entitled ‘Inferno’ (F2).
- The musical notation of Mozart’s Singspiel entitled ‘Die Zauberflöte’ (F2) has component the musical notation of Mozart’s aria entitled ‘Der Hölle Rache’, also known as ‘The Queen of the Night’s Aria’ (F2).
- The visual content of the map entitled ‘Wales – The Midlands – South West England’, scale 1:400,000, issued by Michelin in 2005 (F2) has component the visual content of the inset entitled ‘Liverpool’, scale 1:200,000, set within the compass of the map titled ‘Wales – The Midlands – South West England’, scale 1:400,000, issued by Michelin in 2005 (F2).
</rdfs:comment>
	<rdfs:label xml:lang="en">R5i is component of</rdfs:label>
	<skos:notation>R5i</skos:notation>
	<skos:prefLabel xml:lang="en">is component of</skos:prefLabel>
</rdf:Description>

<rdf:Description rdf:about="http://iflastandards.info/ns/lrm/lrmoo/R67_has_part">
	<rdf:type rdf:resource="http://www.w3.org/2002/07/owl#ObjectProperty"/>
	<rdfs:subPropertyOf rdf:resource="http://www.cidoc-crm.org/cidoc-crm/P148_has_component"/>
	<owl:inverseOf rdf:resource="http://iflastandards.info/ns/lrm/lrmoo/R67i_forms_part_of"/>
	<rdfs:domain rdf:resource="http://iflastandards.info/ns/lrm/lrmoo/F1_Work"/>
	<rdfs:range rdf:resource="http://iflastandards.info/ns/lrm/lrmoo/F1_Work"/>
	<rdfs:comment xml:lang="en">Quantification: many to many (0,n:0,n)

Scope note:
This property associates an instance of F1 Work with another instance of F1 Work that forms part of it in a complementary role to other sibling parts, conceived at some point in time to form together a logical whole, such as the parts of a trilogy. This property is transitive, asymmetric and irreflexive.

Examples:
- Ursula K. Le Guin’s textual work ‘The Earthsea trilogy’ (F1) has part Ursula K. Le Guin’s textual work ‘The tombs of Atuan’ (F1).
- Dante Alighieri’s textual work entitled ‘Divina Commedia’ (F1) has part Dante Alighieri’s textual work entitled ‘Inferno’ (F1).
- Miguel de Cervantes’ textual work entitled ‘Don Quixote’ (F1) has part Miguel de Cervantes’ textual work entitled ‘El ingenioso hidalgo Don Quixote de la Mancha’ (F1).
- Miguel de Cervantes’ textual work entitled ‘Don Quixote’ (F1) has part Miguel de Cervantes’ textual work entitled ‘Segunda Parte del Ingenioso Cavallero Don Quixote de la Mancha’ (F1).
- J. R. R. Tolkien’s textual work ‘The Lord of the Rings’ (F1) has part J. R. R. Tolkien’s textual work ‘The Two Towers’ (F1).
- Cormac McCarthy’s textual work ‘The Border Trilogy’ (F1) has part Cormac McCarthy’s textual work ‘All the Pretty Horses’ (F1).
- Giovanni Battista Piranesi’s graphic work entitled ‘Carceri’ (F1) has part Giovanni Battista Piranesi’s graphic work entitled ‘Carcere XVI: the pier with chains’ (F1).
- Ludwig van Beethoven’s musical work entitled ‘Symphony No. 9’ (F1) has part Ludwig van Beethoven’s musical work ‘Finale’ (4(th) movement) (F1).
- Johann Sebastian Bach’s musical work ‘Goldberg Variations’ (F1) has part the musical work entitled ‘Variatio 1. a 1 Clav’ (F1).
</rdfs:comment>
	<rdfs:label xml:lang="en">R67 has part</rdfs:label>
	<skos:notation>R67</skos:notation>
	<skos:prefLabel xml:lang="en">has part</skos:prefLabel>
</rdf:Description>

<rdf:Description rdf:about="http://iflastandards.info/ns/lrm/lrmoo/R67i_forms_part_of">
	<rdf:type rdf:resource="http://www.w3.org/2002/07/owl#ObjectProperty"/>
	<rdfs:subPropertyOf rdf:resource="http://www.cidoc-crm.org/cidoc-crm/P148i_is_component_of"/>
	<rdfs:domain rdf:resource="http://iflastandards.info/ns/lrm/lrmoo/F1_Work"/>
	<rdfs:range rdf:resource="http://iflastandards.info/ns/lrm/lrmoo/F1_Work"/>
	<rdfs:comment xml:lang="en">Quantification of the inverse property: many to many (0,n:0,n)

Scope note of the inverse property:
This property associates an instance of F1 Work with another instance of F1 Work that forms part of it in a complementary role to other sibling parts, conceived at some point in time to form together a logical whole, such as the parts of a trilogy. This property is transitive, asymmetric and irreflexive.

Examples of the inverse property:
- Ursula K. Le Guin’s textual work ‘The Earthsea trilogy’ (F1) has part Ursula K. Le Guin’s textual work ‘The tombs of Atuan’ (F1).
- Dante Alighieri’s textual work entitled ‘Divina Commedia’ (F1) has part Dante Alighieri’s textual work entitled ‘Inferno’ (F1).
- Miguel de Cervantes’ textual work entitled ‘Don Quixote’ (F1) has part Miguel de Cervantes’ textual work entitled ‘El ingenioso hidalgo Don Quixote de la Mancha’ (F1).
- Miguel de Cervantes’ textual work entitled ‘Don Quixote’ (F1) has part Miguel de Cervantes’ textual work entitled ‘Segunda Parte del Ingenioso Cavallero Don Quixote de la Mancha’ (F1).
- J. R. R. Tolkien’s textual work ‘The Lord of the Rings’ (F1) has part J. R. R. Tolkien’s textual work ‘The Two Towers’ (F1).
- Cormac McCarthy’s textual work ‘The Border Trilogy’ (F1) has part Cormac McCarthy’s textual work ‘All the Pretty Horses’ (F1).
- Giovanni Battista Piranesi’s graphic work entitled ‘Carceri’ (F1) has part Giovanni Battista Piranesi’s graphic work entitled ‘Carcere XVI: the pier with chains’ (F1).
- Ludwig van Beethoven’s musical work entitled ‘Symphony No. 9’ (F1) has part Ludwig van Beethoven’s musical work ‘Finale’ (4(th) movement) (F1).
- Johann Sebastian Bach’s musical work ‘Goldberg Variations’ (F1) has part the musical work entitled ‘Variatio 1. a 1 Clav’ (F1).
</rdfs:comment>
	<rdfs:label xml:lang="en">R67i forms part of</rdfs:label>
	<skos:notation>R67i</skos:notation>
	<skos:prefLabel xml:lang="en">forms part of</skos:prefLabel>
</rdf:Description>

<rdf:Description rdf:about="http://iflastandards.info/ns/lrm/lrmoo/R68_is_inspired_by">
	<rdf:type rdf:resource="http://www.w3.org/2002/07/owl#ObjectProperty"/>
	<rdfs:subPropertyOf rdf:resource="http://www.cidoc-crm.org/cidoc-crm/P130_shows_features_of"/>
	<owl:inverseOf rdf:resource="http://iflastandards.info/ns/lrm/lrmoo/R68i_is_inspiration_for"/>
	<rdfs:domain rdf:resource="http://iflastandards.info/ns/lrm/lrmoo/F1_Work"/>
	<rdfs:range rdf:resource="http://iflastandards.info/ns/lrm/lrmoo/F1_Work"/>
	<rdfs:comment xml:lang="en">Quantification: many to many (0,n:0,n)

Shortcut Of: F1 Work (2). R16i was created by: F27 Work Creation. P15 was influenced by: F1 Work (1)

Scope note:
This property associates an instance of F1 Work with another instance of F1 Work whose content was inspired by that instance of F1 Work. The content of the range work instance served in some way as a source of ideas for the domain work instance. Neither instance of F1 Work may be a part of the other. This property is not transitive. It is irreflexive.

Examples:
- The musical ‘West Side Story’ (F1) is inspired by the play ‘Romeo and Juliet’ by William Shakespeare (F1).
- The play ‘Rosencrantz and Guildenstern are Dead’ by Tom Stoppard (F1) is inspired by the play ‘The Tragedy of Hamlet, Prince of Denmark’ by William Shakespeare (F1).
- The musical work ‘The Great Gate of Kiev’ (F1) from ‘Pictures at an Exhibition’ by Modest Mussorgsky is inspired by the painting ‘Plan for a City Gate in Kiev’ by Viktor Hartmann (F1).
- The board game ‘War of the Ring’ by Roberto Di Meglio, Marco Maggi and Francesco Nepitello (F1) is inspired by the literary work ‘The Lord of the Rings’ by J. R. R. Tolkien (F1).
- The literary work ‘Girl with a Pearl Earring’ by Tracy Chevalier (F1) is inspired by the painting ‘Girl with a Pearl Earring’ by Johannes Vermeer (F1).
</rdfs:comment>
	<rdfs:label xml:lang="en">R68 is inspired by</rdfs:label>
	<skos:notation>R68</skos:notation>
	<skos:prefLabel xml:lang="en">is inspired by</skos:prefLabel>
</rdf:Description>

<rdf:Description rdf:about="http://iflastandards.info/ns/lrm/lrmoo/R68i_is_inspiration_for">
	<rdf:type rdf:resource="http://www.w3.org/2002/07/owl#ObjectProperty"/>
	<rdfs:subPropertyOf rdf:resource="http://www.cidoc-crm.org/cidoc-crm/P130i_features_are_also_found_on"/>
	<rdfs:domain rdf:resource="http://iflastandards.info/ns/lrm/lrmoo/F1_Work"/>
	<rdfs:range rdf:resource="http://iflastandards.info/ns/lrm/lrmoo/F1_Work"/>
	<rdfs:comment xml:lang="en">Quantification of the inverse property: many to many (0,n:0,n)

Shortcut Of of the inverse property: F1 Work (2). R16i was created by: F27 Work Creation. P15 was influenced by: F1 Work (1)

Scope note of the inverse property:
This property associates an instance of F1 Work with another instance of F1 Work whose content was inspired by that instance of F1 Work. The content of the range work instance served in some way as a source of ideas for the domain work instance. Neither instance of F1 Work may be a part of the other. This property is not transitive. It is irreflexive.

Examples of the inverse property:
- The musical ‘West Side Story’ (F1) is inspired by the play ‘Romeo and Juliet’ by William Shakespeare (F1).
- The play ‘Rosencrantz and Guildenstern are Dead’ by Tom Stoppard (F1) is inspired by the play ‘The Tragedy of Hamlet, Prince of Denmark’ by William Shakespeare (F1).
- The musical work ‘The Great Gate of Kiev’ (F1) from ‘Pictures at an Exhibition’ by Modest Mussorgsky is inspired by the painting ‘Plan for a City Gate in Kiev’ by Viktor Hartmann (F1).
- The board game ‘War of the Ring’ by Roberto Di Meglio, Marco Maggi and Francesco Nepitello (F1) is inspired by the literary work ‘The Lord of the Rings’ by J. R. R. Tolkien (F1).
- The literary work ‘Girl with a Pearl Earring’ by Tracy Chevalier (F1) is inspired by the painting ‘Girl with a Pearl Earring’ by Johannes Vermeer (F1).
</rdfs:comment>
	<rdfs:label xml:lang="en">R68i is inspiration for</rdfs:label>
	<skos:notation>R68i</skos:notation>
	<skos:prefLabel xml:lang="en">is inspiration for</skos:prefLabel>
</rdf:Description>

<rdf:Description rdf:about="http://iflastandards.info/ns/lrm/lrmoo/R69_has_physical_form">
	<rdf:type rdf:resource="http://www.w3.org/2002/07/owl#ObjectProperty"/>
	<rdfs:subPropertyOf rdf:resource="http://www.cidoc-crm.org/cidoc-crm/P2_has_type"/>
	<owl:inverseOf rdf:resource="http://iflastandards.info/ns/lrm/lrmoo/R69i_is_physical_form_of"/>
	<rdfs:domain rdf:resource="http://iflastandards.info/ns/lrm/lrmoo/F3_Manifestation"/>
	<rdfs:range rdf:resource="http://www.cidoc-crm.org/cidoc-crm/E55_Type"/>
	<rdfs:comment xml:lang="en">Quantification: many to many, necessary (1,n:0,n)

Scope note:
This property associates an instance of F3 Manifestation with an instance of E55 Type describing the kind of physical form that characterizes instances of F5 Item carrying this F3 Manifestation.
In the case of instances of manifestations intended to be rendered by mediation (such as with electronic devices), the form also indicates the kind of equipment and software tools necessary.

Examples:
- The publication entitled ‘A clockwork orange’ by Anthony Burgess, published by Penguin Books Ltd in 2008, identified by ISBN ‘0141037229’ (F3) has physical form Printed book (E55).
- The sound recording entitled ‘The Glory (????) of the human voice’, identified by label and label number ‘RCA Victor Gold Seal GD61175’, containing recordings of musical works performed by Florence Foster Jenkins (F3) has physical form Compact Disc (E55).
- The photograph of Billie Holiday by Carl Van Vechten dated 23 March 1949, owned by the Library of Congress and identified by call number LOT 12735, no. 524 [P&amp;P] (F3) has physical form Gelatin silver print (E55).
- The Long Play record entitled ‘Help!’ by The Beatles, released by Parlophone, 6 August 1965, with catalogue number PMC1255 (F3) has physical form Vinyl Long Play record (E55).
- The ebook ‘Christianity: the first three thousand years’ by Diarmaid MacCulloch published by Viking in 2010 and identified by ISBN ‘978-1-101-18999-3’ (F3) has physical form Digital file in EPUB format for Kobo ebook reader (E55).
</rdfs:comment>
	<rdfs:label xml:lang="en">R69 has physical form</rdfs:label>
	<skos:notation>R69</skos:notation>
	<skos:prefLabel xml:lang="en">has physical form</skos:prefLabel>
</rdf:Description>

<rdf:Description rdf:about="http://iflastandards.info/ns/lrm/lrmoo/R69i_is_physical_form_of">
	<rdf:type rdf:resource="http://www.w3.org/2002/07/owl#ObjectProperty"/>
	<rdfs:subPropertyOf rdf:resource="http://www.cidoc-crm.org/cidoc-crm/P2i_is_type_of"/>
	<rdfs:domain rdf:resource="http://www.cidoc-crm.org/cidoc-crm/E55_Type"/>
	<rdfs:range rdf:resource="http://iflastandards.info/ns/lrm/lrmoo/F3_Manifestation"/>
	<rdfs:comment xml:lang="en">Quantification of the inverse property: many to many, necessary (1,n:0,n)

Scope note of the inverse property:
This property associates an instance of F3 Manifestation with an instance of E55 Type describing the kind of physical form that characterizes instances of F5 Item carrying this F3 Manifestation.
In the case of instances of manifestations intended to be rendered by mediation (such as with electronic devices), the form also indicates the kind of equipment and software tools necessary.

Examples of the inverse property:
- The publication entitled ‘A clockwork orange’ by Anthony Burgess, published by Penguin Books Ltd in 2008, identified by ISBN ‘0141037229’ (F3) has physical form Printed book (E55).
- The sound recording entitled ‘The Glory (????) of the human voice’, identified by label and label number ‘RCA Victor Gold Seal GD61175’, containing recordings of musical works performed by Florence Foster Jenkins (F3) has physical form Compact Disc (E55).
- The photograph of Billie Holiday by Carl Van Vechten dated 23 March 1949, owned by the Library of Congress and identified by call number LOT 12735, no. 524 [P&amp;P] (F3) has physical form Gelatin silver print (E55).
- The Long Play record entitled ‘Help!’ by The Beatles, released by Parlophone, 6 August 1965, with catalogue number PMC1255 (F3) has physical form Vinyl Long Play record (E55).
- The ebook ‘Christianity: the first three thousand years’ by Diarmaid MacCulloch published by Viking in 2010 and identified by ISBN ‘978-1-101-18999-3’ (F3) has physical form Digital file in EPUB format for Kobo ebook reader (E55).
</rdfs:comment>
	<rdfs:label xml:lang="en">R69i is physical form of</rdfs:label>
	<skos:notation>R69i</skos:notation>
	<skos:prefLabel xml:lang="en">is physical form of</skos:prefLabel>
</rdf:Description>

<rdf:Description rdf:about="http://iflastandards.info/ns/lrm/lrmoo/R70_has_dimension">
	<rdf:type rdf:resource="http://www.w3.org/2002/07/owl#ObjectProperty"/>
	<rdfs:subPropertyOf rdf:resource="http://www.cidoc-crm.org/cidoc-crm/P43_has_dimension"/>
	<owl:inverseOf rdf:resource="http://iflastandards.info/ns/lrm/lrmoo/R70i_is_dimension_of"/>
	<rdfs:domain rdf:resource="http://iflastandards.info/ns/lrm/lrmoo/F3_Manifestation"/>
	<rdfs:range rdf:resource="http://www.cidoc-crm.org/cidoc-crm/E54_Dimension"/>
	<rdfs:comment xml:lang="en">Quantification: one to many, necessary, dependent (1,n:1,1)

Scope note:
This property associates an instance of F3 Manifestation with an instance of E54 Dimension that describes aspects of its symbolic content, such as word counts, or describes the kind of physical form that characterizes instances of F5 Item carrying this F3 Manifestation, such as number of pages.
This inference is an induction along the path that can be modelled as: F3 Manifestation. R7i is exemplified by: F5 Item. P43 has dimension (is dimension of): E54 Dimension.
It can happen that a given item, or subset of items, originally produced, or intended to be produced, with a certain value for a particular kind of dimension, has a different value for this kind of dimension by accident. This fact should be recorded as a property of F5 Item, and not of F3 Manifestation.

Examples:
- The publication (printed book) entitled ‘Functional Requirements for Bibliographic Records: final report’, published by K. G. Saur in 1998, identified by ISBN ‘3-598-11382-X’ (F3) has dimension height (E54) [which has value (P90) 24 (E60) and has unit (P91) cm (E58)].
- The publication (printed book) entitled ‘A clockwork orange’ by Anthony Burgess, published by Penguin Books Ltd in 2008, identified by ISBN ‘0141037229’ (F3) has dimension number of pages (E54) [which has value (P90) 176 (E60)].
- The publication (Blu-ray box set) entitled ‘Marvel Agents of S.H.I.E.L.D. the Complete Fourth Season’ produced by abc Studios, released in 2018 and identified by EAN ‘8717418521622’ (F3) has dimension number of discs (E54) [which has value (P90) 6 (E60)].
- The jigsaw puzzle entitled ‘Map of the New York city subway system’, designed by Stephen J. Voorhies and released around 1954 by the Union Dimes Savings Bank (F3) has dimension length and height (E54) [which has note (P3) ‘46 x 29 cm’ (E62)].
- The jigsaw puzzle entitled ‘Map of the New York city subway system’, designed by Stephen J. Voorhies and released around 1954 by the Union Dimes Savings Bank (F3) has dimension number of pieces (E54) [which has value (P90) 76 (E60)].
</rdfs:comment>
	<rdfs:label xml:lang="en">R70 has dimension</rdfs:label>
	<skos:notation>R70</skos:notation>
	<skos:prefLabel xml:lang="en">has dimension</skos:prefLabel>
</rdf:Description>

<rdf:Description rdf:about="http://iflastandards.info/ns/lrm/lrmoo/R70i_is_dimension_of">
	<rdf:type rdf:resource="http://www.w3.org/2002/07/owl#ObjectProperty"/>
	<rdfs:subPropertyOf rdf:resource="http://www.cidoc-crm.org/cidoc-crm/P43i_is_dimension_of"/>
	<rdfs:domain rdf:resource="http://www.cidoc-crm.org/cidoc-crm/E54_Dimension"/>
	<rdfs:range rdf:resource="http://iflastandards.info/ns/lrm/lrmoo/F3_Manifestation"/>
	<rdfs:comment xml:lang="en">Quantification of the inverse property: one to many, necessary, dependent (1,n:1,1)

Scope note of the inverse property:
This property associates an instance of F3 Manifestation with an instance of E54 Dimension that describes aspects of its symbolic content, such as word counts, or describes the kind of physical form that characterizes instances of F5 Item carrying this F3 Manifestation, such as number of pages.
This inference is an induction along the path that can be modelled as: F3 Manifestation. R7i is exemplified by: F5 Item. P43 has dimension (is dimension of): E54 Dimension.
It can happen that a given item, or subset of items, originally produced, or intended to be produced, with a certain value for a particular kind of dimension, has a different value for this kind of dimension by accident. This fact should be recorded as a property of F5 Item, and not of F3 Manifestation.

Examples of the inverse property:
- The publication (printed book) entitled ‘Functional Requirements for Bibliographic Records: final report’, published by K. G. Saur in 1998, identified by ISBN ‘3-598-11382-X’ (F3) has dimension height (E54) [which has value (P90) 24 (E60) and has unit (P91) cm (E58)].
- The publication (printed book) entitled ‘A clockwork orange’ by Anthony Burgess, published by Penguin Books Ltd in 2008, identified by ISBN ‘0141037229’ (F3) has dimension number of pages (E54) [which has value (P90) 176 (E60)].
- The publication (Blu-ray box set) entitled ‘Marvel Agents of S.H.I.E.L.D. the Complete Fourth Season’ produced by abc Studios, released in 2018 and identified by EAN ‘8717418521622’ (F3) has dimension number of discs (E54) [which has value (P90) 6 (E60)].
- The jigsaw puzzle entitled ‘Map of the New York city subway system’, designed by Stephen J. Voorhies and released around 1954 by the Union Dimes Savings Bank (F3) has dimension length and height (E54) [which has note (P3) ‘46 x 29 cm’ (E62)].
- The jigsaw puzzle entitled ‘Map of the New York city subway system’, designed by Stephen J. Voorhies and released around 1954 by the Union Dimes Savings Bank (F3) has dimension number of pieces (E54) [which has value (P90) 76 (E60)].
</rdfs:comment>
	<rdfs:label xml:lang="en">R70i is dimension of</rdfs:label>
	<skos:notation>R70i</skos:notation>
	<skos:prefLabel xml:lang="en">is dimension of</skos:prefLabel>
</rdf:Description>

<rdf:Description rdf:about="http://iflastandards.info/ns/lrm/lrmoo/R71_has_part">
	<rdf:type rdf:resource="http://www.w3.org/2002/07/owl#ObjectProperty"/>
	<rdfs:subPropertyOf rdf:resource="http://www.cidoc-crm.org/cidoc-crm/P148_has_component"/>
	<owl:inverseOf rdf:resource="http://iflastandards.info/ns/lrm/lrmoo/R71i_is_part_of"/>
	<rdfs:domain rdf:resource="http://iflastandards.info/ns/lrm/lrmoo/F3_Manifestation"/>
	<rdfs:range rdf:resource="http://iflastandards.info/ns/lrm/lrmoo/F3_Manifestation"/>
	<rdfs:comment xml:lang="en">Quantification: many to many (0,n:0,n)

Scope note:
This property associates an instance of F3 Manifestation with a structural part of it that is itself an instance of F3 Manifestation. This property is transitive, asymmetric and irreflexive.

Examples:
- The publication (set of 3 books) containing J. R. R. Tolkien’s ‘The Lord of the rings’ identified by ISBN ‘0618260587’ (F3) has part the publication containing J. R. R. Tolkien’s ‘The two towers’ identified by ISBN ‘0618260595’ (F3).
- The compact disc publication issued by Deutsche Grammophon in 1998 and consisting of a recording of Richard Wagner’s ‘Der fliegende Holländer’ as performed in 1991 by Plácido Domingo, Cheryl Studer et al., and conducted by Giuseppe Sinopoli (F3) has part a publication consisting of the printed program notes and libretto (F3).
- The compact disc publication issued as a 2-CD set identified as ‘M2K 42270’ by CBS Records in 1987 and consisting of recordings of J. S. Bach’s concertos for keyboard/clavier and strings performed by Glenn Gould (F3) has part the compact disc publication identified as ‘DIDC 10370’ consisting of the Glenn Gould recordings of Bach’s ‘Concertos nos. 1-4’ (F3).
</rdfs:comment>
	<rdfs:label xml:lang="en">R71 has part</rdfs:label>
	<skos:notation>R71</skos:notation>
	<skos:prefLabel xml:lang="en">has part</skos:prefLabel>
</rdf:Description>

<rdf:Description rdf:about="http://iflastandards.info/ns/lrm/lrmoo/R71i_is_part_of">
	<rdf:type rdf:resource="http://www.w3.org/2002/07/owl#ObjectProperty"/>
	<rdfs:subPropertyOf rdf:resource="http://www.cidoc-crm.org/cidoc-crm/P148i_is_component_of"/>
	<rdfs:domain rdf:resource="http://iflastandards.info/ns/lrm/lrmoo/F3_Manifestation"/>
	<rdfs:range rdf:resource="http://iflastandards.info/ns/lrm/lrmoo/F3_Manifestation"/>
	<rdfs:comment xml:lang="en">Quantification of the inverse property: many to many (0,n:0,n)

Scope note of the inverse property:
This property associates an instance of F3 Manifestation with a structural part of it that is itself an instance of F3 Manifestation. This property is transitive, asymmetric and irreflexive.

Examples of the inverse property:
- The publication (set of 3 books) containing J. R. R. Tolkien’s ‘The Lord of the rings’ identified by ISBN ‘0618260587’ (F3) has part the publication containing J. R. R. Tolkien’s ‘The two towers’ identified by ISBN ‘0618260595’ (F3).
- The compact disc publication issued by Deutsche Grammophon in 1998 and consisting of a recording of Richard Wagner’s ‘Der fliegende Holländer’ as performed in 1991 by Plácido Domingo, Cheryl Studer et al., and conducted by Giuseppe Sinopoli (F3) has part a publication consisting of the printed program notes and libretto (F3).
- The compact disc publication issued as a 2-CD set identified as ‘M2K 42270’ by CBS Records in 1987 and consisting of recordings of J. S. Bach’s concertos for keyboard/clavier and strings performed by Glenn Gould (F3) has part the compact disc publication identified as ‘DIDC 10370’ consisting of the Glenn Gould recordings of Bach’s ‘Concertos nos. 1-4’ (F3).
</rdfs:comment>
	<rdfs:label xml:lang="en">R71i is part of</rdfs:label>
	<skos:notation>R71i</skos:notation>
	<skos:prefLabel xml:lang="en">is part of</skos:prefLabel>
</rdf:Description>

<rdf:Description rdf:about="http://iflastandards.info/ns/lrm/lrmoo/R73_takes_representative_attribute_from">
	<rdf:type rdf:resource="http://www.w3.org/2002/07/owl#ObjectProperty"/>
	<owl:inverseOf rdf:resource="http://iflastandards.info/ns/lrm/lrmoo/R73i_bears_representative_attribute_for"/>
	<rdfs:domain rdf:resource="http://iflastandards.info/ns/lrm/lrmoo/F1_Work"/>
	<rdfs:range rdf:resource="http://iflastandards.info/ns/lrm/lrmoo/F2_Expression"/>
	<rdfs:comment xml:lang="en">Quantification: one to many, necessary (1,n:0,1)

Shortcut Of: F1 Work. P140i was attributed by: E13 Attribute Assignment. P16 uses specific object: F2 Expression

Scope note:
This property associates an instance of F1 Work with instances of F2 Expression that bear attributes which are used to characterize the work. The instance of F2 Expression in question must be one that realizes that instance of F1 Work. An instance of F2 Expression may or may not serve as source of representative expression attributes for its associated instance of F1 Work. If it does, it may provide one attribute or many. Only one or more than one of the instances of F2 Expression associated with an instance of F1 Work may provide attributes that characterize that instance of F1 Work. The representative expression attributes can all come from the same expression or from more than one expressions.

Examples:
- The work ‘Reading for life, a first book for adults and their tutors’ by Virginia French Allen (F1) takes representative attribute from the expression first published in 1987 by Spring Institute for International Studies with ISBN ‘094072300X’ (F2). [One attribute is the value for intended audience, which is adult literacy learners in the English language, another attribute is the language English.]
- The expression of the work ‘Piglet has a bath’ by A. A. Milne, with illustrations by Ernest H. Shepard, realised in the edition published on sealed plastic pages by Dutton Children’s Books in 1998 with ISBN ‘0525460926’ (F2) bears representative attribute for the work ‘Piglet has a bath’ by A. A. Milne (F1). [One attribute is the language English; another is the value for intended audience, which is children.]
- The work ‘Fugue in G Minor, BWV 1000’ by Johann Sebastian Bach (F1) takes representative attribute from the original expression (F2) (as composed around 1723). [The attribute is lute as the mode of performance; it is now mostly performed on the guitar.]
</rdfs:comment>
	<rdfs:label xml:lang="en">R73 takes representative attribute from</rdfs:label>
	<skos:notation>R73</skos:notation>
	<skos:prefLabel xml:lang="en">takes representative attribute from</skos:prefLabel>
</rdf:Description>

<rdf:Description rdf:about="http://iflastandards.info/ns/lrm/lrmoo/R73i_bears_representative_attribute_for">
	<rdf:type rdf:resource="http://www.w3.org/2002/07/owl#ObjectProperty"/>
	<rdfs:domain rdf:resource="http://iflastandards.info/ns/lrm/lrmoo/F2_Expression"/>
	<rdfs:range rdf:resource="http://iflastandards.info/ns/lrm/lrmoo/F1_Work"/>
	<rdfs:comment xml:lang="en">Quantification of the inverse property: one to many, necessary (1,n:0,1)

Shortcut Of of the inverse property: F1 Work. P140i was attributed by: E13 Attribute Assignment. P16 uses specific object: F2 Expression

Scope note of the inverse property:
This property associates an instance of F1 Work with instances of F2 Expression that bear attributes which are used to characterize the work. The instance of F2 Expression in question must be one that realizes that instance of F1 Work. An instance of F2 Expression may or may not serve as source of representative expression attributes for its associated instance of F1 Work. If it does, it may provide one attribute or many. Only one or more than one of the instances of F2 Expression associated with an instance of F1 Work may provide attributes that characterize that instance of F1 Work. The representative expression attributes can all come from the same expression or from more than one expressions.

Examples of the inverse property:
- The work ‘Reading for life, a first book for adults and their tutors’ by Virginia French Allen (F1) takes representative attribute from the expression first published in 1987 by Spring Institute for International Studies with ISBN ‘094072300X’ (F2). [One attribute is the value for intended audience, which is adult literacy learners in the English language, another attribute is the language English.]
- The expression of the work ‘Piglet has a bath’ by A. A. Milne, with illustrations by Ernest H. Shepard, realised in the edition published on sealed plastic pages by Dutton Children’s Books in 1998 with ISBN ‘0525460926’ (F2) bears representative attribute for the work ‘Piglet has a bath’ by A. A. Milne (F1). [One attribute is the language English; another is the value for intended audience, which is children.]
- The work ‘Fugue in G Minor, BWV 1000’ by Johann Sebastian Bach (F1) takes representative attribute from the original expression (F2) (as composed around 1723). [The attribute is lute as the mode of performance; it is now mostly performed on the guitar.]
</rdfs:comment>
	<rdfs:label xml:lang="en">R73i bears representative attribute for</rdfs:label>
	<skos:notation>R73i</skos:notation>
	<skos:prefLabel xml:lang="en">bears representative attribute for</skos:prefLabel>
</rdf:Description>

<rdf:Description rdf:about="http://iflastandards.info/ns/lrm/lrmoo/R74_uses_expression_of">
	<rdf:type rdf:resource="http://www.w3.org/2002/07/owl#ObjectProperty"/>
	<rdfs:subPropertyOf rdf:resource="http://www.cidoc-crm.org/cidoc-crm/P130_shows_features_of"/>
	<owl:inverseOf rdf:resource="http://iflastandards.info/ns/lrm/lrmoo/R74i_has_expression_used_in"/>
	<rdfs:domain rdf:resource="http://iflastandards.info/ns/lrm/lrmoo/F1_Work"/>
	<rdfs:range rdf:resource="http://iflastandards.info/ns/lrm/lrmoo/F1_Work"/>
	<rdfs:comment xml:lang="en">Quantification: many to many (0,n:0,n)

Scope note:
This property associates an instance of F1 Work with another instance of F1 Work where all expressions of the former will include some expression of the latter. This property is not transitive. It is irreflexive. This property represents the generalized relationship between works that is described at the expression level using R75 incorporates (is incorporated in).

Examples:
- Ludwig van Beethoven’s ‘Symphony No. 9’ (F1) uses expression of the poem ‘An die Freude’ by Friedrich Schiller (F1).
- Franz Schubert’s kunstlied ‘Erlkönig’ (F1) uses expression of the poem ‘Erlkönig’ by Johann Wolfgang von Goethe (F1).
- The symphonic poem ‘Vltava’ by Bedřich Smetana (F1) uses expression of the melody ‘La Mantovana’ attributed to Giuseppe Cenci (F1).
</rdfs:comment>
	<rdfs:label xml:lang="en">R74 uses expression of</rdfs:label>
	<skos:notation>R74</skos:notation>
	<skos:prefLabel xml:lang="en">uses expression of</skos:prefLabel>
</rdf:Description>

<rdf:Description rdf:about="http://iflastandards.info/ns/lrm/lrmoo/R74i_has_expression_used_in">
	<rdf:type rdf:resource="http://www.w3.org/2002/07/owl#ObjectProperty"/>
	<rdfs:subPropertyOf rdf:resource="http://www.cidoc-crm.org/cidoc-crm/P130i_features_are_also_found_on"/>
	<rdfs:domain rdf:resource="http://iflastandards.info/ns/lrm/lrmoo/F1_Work"/>
	<rdfs:range rdf:resource="http://iflastandards.info/ns/lrm/lrmoo/F1_Work"/>
	<rdfs:comment xml:lang="en">Quantification of the inverse property: many to many (0,n:0,n)

Scope note of the inverse property:
This property associates an instance of F1 Work with another instance of F1 Work where all expressions of the former will include some expression of the latter. This property is not transitive. It is irreflexive. This property represents the generalized relationship between works that is described at the expression level using R75 incorporates (is incorporated in).

Examples of the inverse property:
- Ludwig van Beethoven’s ‘Symphony No. 9’ (F1) uses expression of the poem ‘An die Freude’ by Friedrich Schiller (F1).
- Franz Schubert’s kunstlied ‘Erlkönig’ (F1) uses expression of the poem ‘Erlkönig’ by Johann Wolfgang von Goethe (F1).
- The symphonic poem ‘Vltava’ by Bedřich Smetana (F1) uses expression of the melody ‘La Mantovana’ attributed to Giuseppe Cenci (F1).
</rdfs:comment>
	<rdfs:label xml:lang="en">R74i has expression used in</rdfs:label>
	<skos:notation>R74i</skos:notation>
	<skos:prefLabel xml:lang="en">has expression used in</skos:prefLabel>
</rdf:Description>

<rdf:Description rdf:about="http://iflastandards.info/ns/lrm/lrmoo/R75_incorporates">
	<rdf:type rdf:resource="http://www.w3.org/2002/07/owl#ObjectProperty"/>
	<rdfs:subPropertyOf rdf:resource="http://www.cidoc-crm.org/cidoc-crm/P165_incorporates"/>
	<owl:inverseOf rdf:resource="http://iflastandards.info/ns/lrm/lrmoo/R75i_is_incorporated_in"/>
	<rdfs:domain rdf:resource="http://iflastandards.info/ns/lrm/lrmoo/F2_Expression"/>
	<rdfs:range rdf:resource="http://iflastandards.info/ns/lrm/lrmoo/F2_Expression"/>
	<rdfs:comment xml:lang="en">Quantification: many to many (0,n:0,n)

Scope note:
This property associates an instance of F2 Expression with an instance of F2 Expression that is an integral part of the first, but where the latter realises a different instance of F1 Work from the first. This property is transitive, asymmetric and irreflexive.

Examples:
- The 1964 recording of Beethoven’s ‘Symphony No. 9’ by Leonard Bernstein and the New York Philharmonic (F2) incorporates the German text of the poem ‘An die Freude’ by Friedrich Schiller (F2).
- Franz Schubert’s score for the kunstlied ‘Erlkönig’ that was created in 1815 (F2) incorporates the German text of the poem ‘Erlkönig’ by Johann Wolfgang von Goethe (F2).
- Pyotr Ilyich Tchaikovsky’s graduation cantata performed by Leslie Head and the Kensington Symphony Orchestra in 1978 (F2) incorporates a Russian translation of the poem ‘An die Freude’ by Friedrich Schiller (F2).
</rdfs:comment>
	<rdfs:label xml:lang="en">R75 incorporates</rdfs:label>
	<skos:notation>R75</skos:notation>
	<skos:prefLabel xml:lang="en">incorporates</skos:prefLabel>
</rdf:Description>

<rdf:Description rdf:about="http://iflastandards.info/ns/lrm/lrmoo/R75i_is_incorporated_in">
	<rdf:type rdf:resource="http://www.w3.org/2002/07/owl#ObjectProperty"/>
	<rdfs:subPropertyOf rdf:resource="http://www.cidoc-crm.org/cidoc-crm/P165i_is_incorporated_in"/>
	<rdfs:domain rdf:resource="http://iflastandards.info/ns/lrm/lrmoo/F2_Expression"/>
	<rdfs:range rdf:resource="http://iflastandards.info/ns/lrm/lrmoo/F2_Expression"/>
	<rdfs:comment xml:lang="en">Quantification of the inverse property: many to many (0,n:0,n)

Scope note of the inverse property:
This property associates an instance of F2 Expression with an instance of F2 Expression that is an integral part of the first, but where the latter realises a different instance of F1 Work from the first. This property is transitive, asymmetric and irreflexive.

Examples of the inverse property:
- The 1964 recording of Beethoven’s ‘Symphony No. 9’ by Leonard Bernstein and the New York Philharmonic (F2) incorporates the German text of the poem ‘An die Freude’ by Friedrich Schiller (F2).
- Franz Schubert’s score for the kunstlied ‘Erlkönig’ that was created in 1815 (F2) incorporates the German text of the poem ‘Erlkönig’ by Johann Wolfgang von Goethe (F2).
- Pyotr Ilyich Tchaikovsky’s graduation cantata performed by Leslie Head and the Kensington Symphony Orchestra in 1978 (F2) incorporates a Russian translation of the poem ‘An die Freude’ by Friedrich Schiller (F2).
</rdfs:comment>
	<rdfs:label xml:lang="en">R75i is incorporated in</rdfs:label>
	<skos:notation>R75i</skos:notation>
	<skos:prefLabel xml:lang="en">is incorporated in</skos:prefLabel>
</rdf:Description>

<rdf:Description rdf:about="http://iflastandards.info/ns/lrm/lrmoo/R76_is_derivative_of">
	<rdf:type rdf:resource="http://www.w3.org/2002/07/owl#ObjectProperty"/>
	<rdfs:subPropertyOf rdf:resource="http://www.cidoc-crm.org/cidoc-crm/P130_shows_features_of"/>
	<owl:inverseOf rdf:resource="http://iflastandards.info/ns/lrm/lrmoo/R76i_has_derivative"/>
	<rdfs:domain rdf:resource="http://iflastandards.info/ns/lrm/lrmoo/F2_Expression"/>
	<rdfs:range rdf:resource="http://iflastandards.info/ns/lrm/lrmoo/F2_Expression"/>
	<rdfs:comment xml:lang="en">Quantification: many to many (0,n:0,n)

Scope note:
This property associates an instance of F2 Expression with another instance of F2 Expression which was its source or one of its sources. This property is not transitive. It is asymmetric and irreflexive.
This property is also a shortcut of the fully developed path: F2 Expression (1). P16i was used for: F28 Expression Creation. R17 created: F2 Expression (2).

Examples:
- Elisabeth van Bebber’s German text of Agatha Christie’s ‘Murder on the Orient Express’ (F2) is derivative of the original text written by Agatha Christie for the novel (F2) with has type Translation (E55).
- The text of Agatha Christie’s ‘Murder on the Orient Express Abridged’ (as published by HarperCollins) (F2) is derivative of the original text written by Agatha Christie for the novel (F2) with has type Abridgement (E55).
- The musical score for Dmitry Sitkovetsky’s ‘Goldberg Variations’ arranged for string (F2) is derivative of the musical score for Johann Sebastian Bach’s ‘Goldberg Variations’ (F2) with has type Arrangement (E55).
- The score for Beethoven’s 9th Symphony edited by Jonathan Del Mar (F2) is derivation of Beethoven’s original score for the 9th Symphony (F2) with has type Revision (E55).

Properties:
- R76.1 has type: 
  Scope note:
    This property allows for specifying the kind of derivation, such as translation, revision, etc.
</rdfs:comment>
	<rdfs:label xml:lang="en">R76 is derivative of</rdfs:label>
	<skos:notation>R76</skos:notation>
	<skos:prefLabel xml:lang="en">is derivative of</skos:prefLabel>
</rdf:Description>

<rdf:Description rdf:about="http://iflastandards.info/ns/lrm/lrmoo/R76i_has_derivative">
	<rdf:type rdf:resource="http://www.w3.org/2002/07/owl#ObjectProperty"/>
	<rdfs:subPropertyOf rdf:resource="http://www.cidoc-crm.org/cidoc-crm/P130i_features_are_also_found_on"/>
	<rdfs:domain rdf:resource="http://iflastandards.info/ns/lrm/lrmoo/F2_Expression"/>
	<rdfs:range rdf:resource="http://iflastandards.info/ns/lrm/lrmoo/F2_Expression"/>
	<rdfs:comment xml:lang="en">Quantification of the inverse property: many to many (0,n:0,n)

Scope note of the inverse property:
This property associates an instance of F2 Expression with another instance of F2 Expression which was its source or one of its sources. This property is not transitive. It is asymmetric and irreflexive.
This property is also a shortcut of the fully developed path: F2 Expression (1). P16i was used for: F28 Expression Creation. R17 created: F2 Expression (2).

Examples of the inverse property:
- Elisabeth van Bebber’s German text of Agatha Christie’s ‘Murder on the Orient Express’ (F2) is derivative of the original text written by Agatha Christie for the novel (F2) with has type Translation (E55).
- The text of Agatha Christie’s ‘Murder on the Orient Express Abridged’ (as published by HarperCollins) (F2) is derivative of the original text written by Agatha Christie for the novel (F2) with has type Abridgement (E55).
- The musical score for Dmitry Sitkovetsky’s ‘Goldberg Variations’ arranged for string (F2) is derivative of the musical score for Johann Sebastian Bach’s ‘Goldberg Variations’ (F2) with has type Arrangement (E55).
- The score for Beethoven’s 9th Symphony edited by Jonathan Del Mar (F2) is derivation of Beethoven’s original score for the 9th Symphony (F2) with has type Revision (E55).
</rdfs:comment>
	<rdfs:label xml:lang="en">R76i has derivative</rdfs:label>
	<skos:notation>R76i</skos:notation>
	<skos:prefLabel xml:lang="en">has derivative</skos:prefLabel>
</rdf:Description>

<rdf:Description rdf:about="http://iflastandards.info/ns/lrm/lrmoo/R77_accompanies_or_complements">
	<rdf:type rdf:resource="http://www.w3.org/2002/07/owl#ObjectProperty"/>
	<owl:inverseOf rdf:resource="http://iflastandards.info/ns/lrm/lrmoo/R77i_is_accompanied_or_complemented_by"/>
	<rdfs:domain rdf:resource="http://iflastandards.info/ns/lrm/lrmoo/F1_Work"/>
	<rdfs:range rdf:resource="http://iflastandards.info/ns/lrm/lrmoo/F1_Work"/>
	<rdfs:comment xml:lang="en">Quantification: many to many (0,n:0,n)

Shortcut Of: F1 Work. P19i was made for: E7 Activity. P19 was intended use of: F1 Work

Scope note:
This property associates one instance of F1 Work with another instance of F1 Work which is intended to accompany it or to function as a complement for it. This property is neither transitive nor intransitive. It is generally not symmetric and it is irreflexive.
In many but not all cases, one of the instances of F1 Work is primary and can be used without the other work, while the other is secondary and depends on the first work (such as a work that is a concordance for another work).
In some cases a work may have been created to accompany or complement a specific expression of another work. The link to the source expression can be indicated using the property P16 used specific object (was used for) using the path: F1 Work(1). R3 is realised in: F2 Expression(1). P16i was used for: F27 Work Creation. R16 created: F1 Work(2).

Examples:
- Leigh Lowe’s ‘Prima Latina: an introduction to Christian Latin. Teacher manual’ (F1) accompanies or complements Leigh Lowe’s ‘Prima Latina: an introduction to Christian Latin. Student book’ (F1).
- Eric Gill’s set of illustrations for the Song of Songs (F1) accompanies or complements the ‘Song of Songs’ in the 1931 publication by the Cranach Press (F1).
- The periodical ‘Applied economics quarterly’ (ISSN 1611-6607) (F1) is accompanied or complemented by the periodical ‘Applied economics quarterly. Supplement’ (ISSN 1612-2127) (F1).
- The novel ‘Le chevalier au lion’ by Chrétien de Troyes (F1) is accompanied or complemented by the concordance created by Pascal Bonnefois and Marie-Louise Ollier ‘Yvain ou Le chevalier au lion : concordance lemmatisée’ (F1). [The concordance is specifically based on the 1960 edition of the novel by Mario Roques.]
</rdfs:comment>
	<rdfs:label xml:lang="en">R77 accompanies or complements</rdfs:label>
	<skos:notation>R77</skos:notation>
	<skos:prefLabel xml:lang="en">accompanies or complements</skos:prefLabel>
</rdf:Description>

<rdf:Description rdf:about="http://iflastandards.info/ns/lrm/lrmoo/R77i_is_accompanied_or_complemented_by">
	<rdf:type rdf:resource="http://www.w3.org/2002/07/owl#ObjectProperty"/>
	<rdfs:domain rdf:resource="http://iflastandards.info/ns/lrm/lrmoo/F1_Work"/>
	<rdfs:range rdf:resource="http://iflastandards.info/ns/lrm/lrmoo/F1_Work"/>
	<rdfs:comment xml:lang="en">Quantification of the inverse property: many to many (0,n:0,n)

Shortcut Of of the inverse property: F1 Work. P19i was made for: E7 Activity. P19 was intended use of: F1 Work

Scope note of the inverse property:
This property associates one instance of F1 Work with another instance of F1 Work which is intended to accompany it or to function as a complement for it. This property is neither transitive nor intransitive. It is generally not symmetric and it is irreflexive.
In many but not all cases, one of the instances of F1 Work is primary and can be used without the other work, while the other is secondary and depends on the first work (such as a work that is a concordance for another work).
In some cases a work may have been created to accompany or complement a specific expression of another work. The link to the source expression can be indicated using the property P16 used specific object (was used for) using the path: F1 Work(1). R3 is realised in: F2 Expression(1). P16i was used for: F27 Work Creation. R16 created: F1 Work(2).

Examples of the inverse property:
- Leigh Lowe’s ‘Prima Latina: an introduction to Christian Latin. Teacher manual’ (F1) accompanies or complements Leigh Lowe’s ‘Prima Latina: an introduction to Christian Latin. Student book’ (F1).
- Eric Gill’s set of illustrations for the Song of Songs (F1) accompanies or complements the ‘Song of Songs’ in the 1931 publication by the Cranach Press (F1).
- The periodical ‘Applied economics quarterly’ (ISSN 1611-6607) (F1) is accompanied or complemented by the periodical ‘Applied economics quarterly. Supplement’ (ISSN 1612-2127) (F1).
- The novel ‘Le chevalier au lion’ by Chrétien de Troyes (F1) is accompanied or complemented by the concordance created by Pascal Bonnefois and Marie-Louise Ollier ‘Yvain ou Le chevalier au lion : concordance lemmatisée’ (F1). [The concordance is specifically based on the 1960 edition of the novel by Mario Roques.]
</rdfs:comment>
	<rdfs:label xml:lang="en">R77i is accompanied or complemented by</rdfs:label>
	<skos:notation>R77i</skos:notation>
	<skos:prefLabel xml:lang="en">is accompanied or complemented by</skos:prefLabel>
</rdf:Description>

<rdf:Description rdf:about="http://iflastandards.info/ns/lrm/lrmoo/R78_has_alternate">
	<rdf:type rdf:resource="http://www.w3.org/2002/07/owl#ObjectProperty"/>
	<rdfs:domain rdf:resource="http://iflastandards.info/ns/lrm/lrmoo/F3_Manifestation"/>
	<rdfs:range rdf:resource="http://iflastandards.info/ns/lrm/lrmoo/F3_Manifestation"/>
	<rdfs:comment xml:lang="en">Quantification: many to many (0,n:0,n)

Inverse Shortcut Of: F3 Manifestation. R4 embodies: F2 Expression. R4i is embodied by: F3 Manifestation

Scope note:
This property associates one instance of F3 Manifestation with another instance of F3 Manifestation that exemplifies the same instance of F2 Expression, when the two instances of F3 Manifestation can be used as alternatives for each other in particular use cases. This property is transitive and symmetric. It is irreflexive.
The alternative manifestations may be in the same physical form, for example, simultaneous publications in different markets. More frequently, the alternative relationship is established when the alternative manifestations are in different physical forms, designed to enable use of the same content with different playback equipment (such as a DVD and Blu-ray disc version of the same videorecording).

Examples:
- Agatha Christie’s ‘The Sittaford Mystery’ published in 1931 in the UK by William Collins &amp; Sons (F3) has alternate the simultaneous US edition published as ‘The Murder at Hazelmoor’ by Dodd, Mead &amp; Co. (F3).
- The LP release of the punk rock band the Soviettes’ album titled ‘LP III’ (F3) has alternate the CD release of the punk rock band the Soviettes’ album titled ‘LP III’ (F3).
</rdfs:comment>
	<rdfs:label xml:lang="en">R78 has alternate</rdfs:label>
	<skos:notation>R78</skos:notation>
	<skos:prefLabel xml:lang="en">has alternate</skos:prefLabel>
</rdf:Description>

<rdf:Description rdf:about="http://iflastandards.info/ns/lrm/lrmoo/R79_has_representative_expression_attribute">
	<rdf:type rdf:resource="http://www.w3.org/2002/07/owl#ObjectProperty"/>
	<rdfs:subPropertyOf rdf:resource="http://www.cidoc-crm.org/cidoc-crm/P2_has_type"/>
	<owl:inverseOf rdf:resource="http://iflastandards.info/ns/lrm/lrmoo/R79i_is_representative_expression_attribute_of"/>
	<rdfs:domain rdf:resource="http://iflastandards.info/ns/lrm/lrmoo/F1_Work"/>
	<rdfs:range rdf:resource="http://www.cidoc-crm.org/cidoc-crm/E55_Type"/>
	<rdfs:comment xml:lang="en">Quantification: many to many (0,n:0,n)

Scope note:
This property associates an instance of F1 Work with an instance of E55 Type that describes a category of attribute that is considered essential in characterizing instances of F1 Work. The types of interest will vary depending on the kind of work.
The value of the attribute is considered representative of the instance of F1 Work. It is normally inferred from the values attributed to instances of F2 Expression that realize the work and that are considered canonical or best representative of the work. The values may also be assigned from characteristics abstracted from a more or less nebulous network of similar expressions. There is no requirement to precisely identify one or more expressions which serve as sources for the values of the types serving as representative expression attributes; however, if this is known, an instance of F2 Expression considered representative of an F1 Work may be related to the instance of F1 Work using the R73 takes representative attribute from (bears representative attribute for) property.

Examples:
- The work ‘Reading for life, a first book for adults and their tutors’ by Virginia French Allen (F1) has representative expression attribute language ‘English’ (E56).
- The work ‘Piglet has a bath’ by A. A. Milne (F1) has representative expression attribute intended audience ‘children’ (E55).
- The work ‘Fugue in G Minor, BWV 1000’ by Johann Sebastian Bach (F1) has representative expression attribute medium of performance ‘lute’ (E55). [The original 1723 composition was for lute; it is now mostly performed on the guitar.]
</rdfs:comment>
	<rdfs:label xml:lang="en">R79 has representative expression attribute</rdfs:label>
	<skos:notation>R79</skos:notation>
	<skos:prefLabel xml:lang="en">has representative expression attribute</skos:prefLabel>
</rdf:Description>

<rdf:Description rdf:about="http://iflastandards.info/ns/lrm/lrmoo/R79i_is_representative_expression_attribute_of">
	<rdf:type rdf:resource="http://www.w3.org/2002/07/owl#ObjectProperty"/>
	<rdfs:subPropertyOf rdf:resource="http://www.cidoc-crm.org/cidoc-crm/P2i_is_type_of"/>
	<rdfs:domain rdf:resource="http://www.cidoc-crm.org/cidoc-crm/E55_Type"/>
	<rdfs:range rdf:resource="http://iflastandards.info/ns/lrm/lrmoo/F1_Work"/>
	<rdfs:comment xml:lang="en">Quantification of the inverse property: many to many (0,n:0,n)

Scope note of the inverse property:
This property associates an instance of F1 Work with an instance of E55 Type that describes a category of attribute that is considered essential in characterizing instances of F1 Work. The types of interest will vary depending on the kind of work.
The value of the attribute is considered representative of the instance of F1 Work. It is normally inferred from the values attributed to instances of F2 Expression that realize the work and that are considered canonical or best representative of the work. The values may also be assigned from characteristics abstracted from a more or less nebulous network of similar expressions. There is no requirement to precisely identify one or more expressions which serve as sources for the values of the types serving as representative expression attributes; however, if this is known, an instance of F2 Expression considered representative of an F1 Work may be related to the instance of F1 Work using the R73 takes representative attribute from (bears representative attribute for) property.

Examples of the inverse property:
- The work ‘Reading for life, a first book for adults and their tutors’ by Virginia French Allen (F1) has representative expression attribute language ‘English’ (E56).
- The work ‘Piglet has a bath’ by A. A. Milne (F1) has representative expression attribute intended audience ‘children’ (E55).
- The work ‘Fugue in G Minor, BWV 1000’ by Johann Sebastian Bach (F1) has representative expression attribute medium of performance ‘lute’ (E55). [The original 1723 composition was for lute; it is now mostly performed on the guitar.]
</rdfs:comment>
	<rdfs:label xml:lang="en">R79i is representative expression attribute of</rdfs:label>
	<skos:notation>R79i</skos:notation>
	<skos:prefLabel xml:lang="en">is representative expression attribute of</skos:prefLabel>
</rdf:Description>

<rdf:Description rdf:about="http://iflastandards.info/ns/lrm/lrmoo/R7_exemplifies">
	<rdf:type rdf:resource="http://www.w3.org/2002/07/owl#ObjectProperty"/>
	<rdfs:subPropertyOf rdf:resource="http://www.cidoc-crm.org/cidoc-crm/P128_carries"/>
	<owl:inverseOf rdf:resource="http://iflastandards.info/ns/lrm/lrmoo/R7i_is_exemplified_by"/>
	<rdfs:domain rdf:resource="http://iflastandards.info/ns/lrm/lrmoo/F5_Item"/>
	<rdfs:range rdf:resource="http://iflastandards.info/ns/lrm/lrmoo/F3_Manifestation"/>
	<rdfs:comment xml:lang="en">Quantification: many to one, necessary (1,1:0,n)

Scope note:
This property associates an instance of F3 Manifestation with an instance of F5 Item that is one of its exemplars or its only exemplar.
Instances of F5 Item correspond to the kinds of physical unit(s) specified in the manifestation, regardless of possible later changes.
Even though an item may exhibit defects with respect to the intended manifestation, it is still regarded to carry the manifestation, as long as it is produced or made accessible as a functional item by its creators.

Examples:
- The item held by the Deichman public library in Oslo, identified by inventory number ‘9138513’ (F5) exemplifies the publication ‘Murder on the Orient Express / Agatha Christie’, HarperCollins 2017 (F3).
- The item held by the National Library of France and identified by shelf mark ‘Res 8 P 10’ (F5) exemplifies the edition of Amerigo Vespucci’s textual and cartographic work entitled ‘Mundus novus’ issued in Paris ca. 1503-1504 (F3).
</rdfs:comment>
	<rdfs:label xml:lang="en">R7 exemplifies</rdfs:label>
	<skos:notation>R7</skos:notation>
	<skos:prefLabel xml:lang="en">exemplifies</skos:prefLabel>
</rdf:Description>

<rdf:Description rdf:about="http://iflastandards.info/ns/lrm/lrmoo/R7i_is_exemplified_by">
	<rdf:type rdf:resource="http://www.w3.org/2002/07/owl#ObjectProperty"/>
	<rdfs:subPropertyOf rdf:resource="http://www.cidoc-crm.org/cidoc-crm/P128i_is_carried_by"/>
	<rdfs:domain rdf:resource="http://iflastandards.info/ns/lrm/lrmoo/F3_Manifestation"/>
	<rdfs:range rdf:resource="http://iflastandards.info/ns/lrm/lrmoo/F5_Item"/>
	<rdfs:comment xml:lang="en">Quantification of the inverse property: many to one, necessary (1,1:0,n)

Scope note of the inverse property:
This property associates an instance of F3 Manifestation with an instance of F5 Item that is one of its exemplars or its only exemplar.
Instances of F5 Item correspond to the kinds of physical unit(s) specified in the manifestation, regardless of possible later changes.
Even though an item may exhibit defects with respect to the intended manifestation, it is still regarded to carry the manifestation, as long as it is produced or made accessible as a functional item by its creators.

Examples of the inverse property:
- The item held by the Deichman public library in Oslo, identified by inventory number ‘9138513’ (F5) exemplifies the publication ‘Murder on the Orient Express / Agatha Christie’, HarperCollins 2017 (F3).
- The item held by the National Library of France and identified by shelf mark ‘Res 8 P 10’ (F5) exemplifies the edition of Amerigo Vespucci’s textual and cartographic work entitled ‘Mundus novus’ issued in Paris ca. 1503-1504 (F3).
</rdfs:comment>
	<rdfs:label xml:lang="en">R7i is exemplified by</rdfs:label>
	<skos:notation>R7i</skos:notation>
	<skos:prefLabel xml:lang="en">is exemplified by</skos:prefLabel>
</rdf:Description>

<rdf:Description rdf:about="http://iflastandards.info/ns/lrm/lrmoo/R80_performed">
	<rdf:type rdf:resource="http://www.w3.org/2002/07/owl#ObjectProperty"/>
	<rdfs:subPropertyOf rdf:resource="http://academictourism.com/academictourism#conveys"/>
	<rdfs:subPropertyOf rdf:resource="http://www.cidoc-crm.org/cidoc-crm/P130_shows_features_of"/>
	<owl:inverseOf rdf:resource="http://iflastandards.info/ns/lrm/lrmoo/R80i_is_performed_in"/>
	<rdfs:domain rdf:resource="http://iflastandards.info/ns/lrm/lrmoo/F31_Performance"/>
	<rdfs:range rdf:resource="http://iflastandards.info/ns/lrm/lrmoo/F1_Work"/>
	<rdfs:comment xml:lang="en">Quantification: many to one, necessary (1,1:0,n)

Scope note:
This property associates an instance of F31 Performance with an instance of F1 Work.
The property is used to express the association between an instance of F31 Performance and the instance of F1 Work it conveys.

Examples:
- The performance of ‘Hamlet’ on 17 June 1909 in Berlin, Deutsches Theater, by Alexander Moissi, directed by Max Reinhardt (F31) performed William Shakespeare’s work ‘Hamlet’ (F1).
- The performance (at the Salzburg Festival in 2005) of Verdi’s ‘La Traviata’ that was staged by Willy Decker, directed by Brian Large and featuring Anna Netrebko and Rolando Villazón (F31) performed Giuseppe Verdi’s work ‘La Traviata’ (F1).
- The performance on July 7, 1995 (at the Popes’ Palace in Avignon) of the ballet entitled ‘Rite of spring’ (F31) performed the choreographic work ‘Rite of spring’ by Pina Bausch (F1).
- The Mariinsky Orchestra and Ballet’s performance of Michel Fokine’s choreography and libretto (choreographic work) for Stravinsky’s ‘The Firebird’ at the Mariinsky Theatre in Saint Petersburg, June 2008 (F31) performed Michel Fokine’s choreography and libretto (choreographic work) for Stravinsky’s ‘The Firebird’ (F1).
- The performance of Daniel Humair (drums) and Damien Varaillon (double bass) improvising their ‘Hommage à John Coltrane’ in the Bal Blomet (Paris), on 18 January 2018 (F31) performed Daniel Humair and Damien Varaillon’s work ‘Hommage à John Coltrane’ (F1).
</rdfs:comment>
	<rdfs:label xml:lang="en">R80 performed</rdfs:label>
	<skos:notation>R80</skos:notation>
	<skos:prefLabel xml:lang="en">performed</skos:prefLabel>
</rdf:Description>

<rdf:Description rdf:about="http://iflastandards.info/ns/lrm/lrmoo/R80i_is_performed_in">
	<rdf:type rdf:resource="http://www.w3.org/2002/07/owl#ObjectProperty"/>
	<rdfs:subPropertyOf rdf:resource="http://academictourism.com/academictourism#is_conveyed_by"/>
	<rdfs:subPropertyOf rdf:resource="http://www.cidoc-crm.org/cidoc-crm/P130i_features_are_also_found_on"/>
	<rdfs:domain rdf:resource="http://iflastandards.info/ns/lrm/lrmoo/F1_Work"/>
	<rdfs:range rdf:resource="http://iflastandards.info/ns/lrm/lrmoo/F31_Performance"/>
	<rdfs:comment xml:lang="en">Quantification of the inverse property: many to one, necessary (1,1:0,n)

Scope note of the inverse property:
This property associates an instance of F31 Performance with an instance of F1 Work.
The property is used to express the association between an instance of F31 Performance and the instance of F1 Work it conveys.

Examples of the inverse property:
- The performance of ‘Hamlet’ on 17 June 1909 in Berlin, Deutsches Theater, by Alexander Moissi, directed by Max Reinhardt (F31) performed William Shakespeare’s work ‘Hamlet’ (F1).
- The performance (at the Salzburg Festival in 2005) of Verdi’s ‘La Traviata’ that was staged by Willy Decker, directed by Brian Large and featuring Anna Netrebko and Rolando Villazón (F31) performed Giuseppe Verdi’s work ‘La Traviata’ (F1).
- The performance on July 7, 1995 (at the Popes’ Palace in Avignon) of the ballet entitled ‘Rite of spring’ (F31) performed the choreographic work ‘Rite of spring’ by Pina Bausch (F1).
- The Mariinsky Orchestra and Ballet’s performance of Michel Fokine’s choreography and libretto (choreographic work) for Stravinsky’s ‘The Firebird’ at the Mariinsky Theatre in Saint Petersburg, June 2008 (F31) performed Michel Fokine’s choreography and libretto (choreographic work) for Stravinsky’s ‘The Firebird’ (F1).
- The performance of Daniel Humair (drums) and Damien Varaillon (double bass) improvising their ‘Hommage à John Coltrane’ in the Bal Blomet (Paris), on 18 January 2018 (F31) performed Daniel Humair and Damien Varaillon’s work ‘Hommage à John Coltrane’ (F1).
</rdfs:comment>
	<rdfs:label xml:lang="en">R80i is performed in</rdfs:label>
	<skos:notation>R80i</skos:notation>
	<skos:prefLabel xml:lang="en">is performed in</skos:prefLabel>
</rdf:Description>

<rdf:Description rdf:about="http://iflastandards.info/ns/lrm/lrmoo/R81_recorded">
	<rdf:type rdf:resource="http://www.w3.org/2002/07/owl#ObjectProperty"/>
	<owl:inverseOf rdf:resource="http://iflastandards.info/ns/lrm/lrmoo/R81i_is_recorded_in"/>
	<rdfs:domain rdf:resource="http://iflastandards.info/ns/lrm/lrmoo/F28_Expression_Creation"/>
	<rdfs:range rdf:resource="http://iflastandards.info/ns/lrm/lrmoo/F31_Performance"/>
	<rdfs:comment xml:lang="en">Quantification: many to one (0,1:0,n)

Scope note:
This property associates an instance of F28 Expression Creation with an instance of F31 Performance that it records.
This property allows for the documentation of the association that exists between the outcome of an instance of F28 Expression Creation such as a performance recording, and the instance of F31 Performance that it is a recording of. For documenting performances that are more integral and planned parts of an expression creation (such as the recording of a performance solely done for the purpose of audio or video productions), the use of the property P9 consist of (forms part of) is more specific (and appropriate).

Examples:
- The Hyperion production (for CD release) of Angela Hewitt performing the ‘Goldberg Variations’ (F28) recorded Angela Hewitt’s performance of the ‘Goldberg Variations’ in Christuskirche (Berlin) on 14-17 December 2015 (F31).
- The Deutsche Grammophon video production of Verdi’s ‘La Traviata’ from the Salzburg Festival in 2005 (F28) recorded the live performance of ‘La Traviata’ that was staged by Willy Decker, directed by Brian Large and featuring Anna Netrebko and Rolando Villazón (F31).
- The Deutsche Grammophon audio production of Verdi’s ‘La Traviata’ from the Salzburg Festival in 2005 (F28) recorded the live performance of ‘La Traviata’ performed by the Vienna Philharmonic, conducted by Carlo Rizzi featuring Anna Netrebko and Rolando Villazón (F31).
- The Belair production (DVD) produced by François Duplat and directed for video by Denis Calozzi, of Michel Fokine’s choreography and libretto for Stravinsky’s ‘The Firebird’ (F28) recorded the Mariinsky Orchestra and Ballet’s performance of Michel Fokine’s choreography and libretto (choreographic work) for Stravinsky’s ‘The Firebird’, at the Mariinsky Theatre in Saint Petersburg, June 2008 (F31).
- The Music Development Company production (for CD release) of Daniel Humair (drums) and Damien Varaillon (double bass) performing their improvisation ‘Hommage à John Coltrane’ (F28) recorded Daniel Humair and Damien Varaillon’s performance in the Bal Blomet (Paris), on 18 January 2018 (F31).
</rdfs:comment>
	<rdfs:label xml:lang="en">R81 recorded</rdfs:label>
	<skos:notation>R81</skos:notation>
	<skos:prefLabel xml:lang="en">recorded</skos:prefLabel>
</rdf:Description>

<rdf:Description rdf:about="http://iflastandards.info/ns/lrm/lrmoo/R81i_is_recorded_in">
	<rdf:type rdf:resource="http://www.w3.org/2002/07/owl#ObjectProperty"/>
	<rdfs:domain rdf:resource="http://iflastandards.info/ns/lrm/lrmoo/F31_Performance"/>
	<rdfs:range rdf:resource="http://iflastandards.info/ns/lrm/lrmoo/F28_Expression_Creation"/>
	<rdfs:comment xml:lang="en">Quantification of the inverse property: many to one (0,1:0,n)

Scope note of the inverse property:
This property associates an instance of F28 Expression Creation with an instance of F31 Performance that it records.
This property allows for the documentation of the association that exists between the outcome of an instance of F28 Expression Creation such as a performance recording, and the instance of F31 Performance that it is a recording of. For documenting performances that are more integral and planned parts of an expression creation (such as the recording of a performance solely done for the purpose of audio or video productions), the use of the property P9 consist of (forms part of) is more specific (and appropriate).

Examples of the inverse property:
- The Hyperion production (for CD release) of Angela Hewitt performing the ‘Goldberg Variations’ (F28) recorded Angela Hewitt’s performance of the ‘Goldberg Variations’ in Christuskirche (Berlin) on 14-17 December 2015 (F31).
- The Deutsche Grammophon video production of Verdi’s ‘La Traviata’ from the Salzburg Festival in 2005 (F28) recorded the live performance of ‘La Traviata’ that was staged by Willy Decker, directed by Brian Large and featuring Anna Netrebko and Rolando Villazón (F31).
- The Deutsche Grammophon audio production of Verdi’s ‘La Traviata’ from the Salzburg Festival in 2005 (F28) recorded the live performance of ‘La Traviata’ performed by the Vienna Philharmonic, conducted by Carlo Rizzi featuring Anna Netrebko and Rolando Villazón (F31).
- The Belair production (DVD) produced by François Duplat and directed for video by Denis Calozzi, of Michel Fokine’s choreography and libretto for Stravinsky’s ‘The Firebird’ (F28) recorded the Mariinsky Orchestra and Ballet’s performance of Michel Fokine’s choreography and libretto (choreographic work) for Stravinsky’s ‘The Firebird’, at the Mariinsky Theatre in Saint Petersburg, June 2008 (F31).
- The Music Development Company production (for CD release) of Daniel Humair (drums) and Damien Varaillon (double bass) performing their improvisation ‘Hommage à John Coltrane’ (F28) recorded Daniel Humair and Damien Varaillon’s performance in the Bal Blomet (Paris), on 18 January 2018 (F31).
</rdfs:comment>
	<rdfs:label xml:lang="en">R81i is recorded in</rdfs:label>
	<skos:notation>R81i</skos:notation>
	<skos:prefLabel xml:lang="en">is recorded in</skos:prefLabel>
</rdf:Description>

<rdf:Description rdf:about="http://iflastandards.info/ns/lrm/lrmoo/R8_combines">
	<rdf:type rdf:resource="http://www.w3.org/2002/07/owl#ObjectProperty"/>
	<owl:inverseOf rdf:resource="http://iflastandards.info/ns/lrm/lrmoo/R8i_is_combined_to_form"/>
	<rdfs:domain rdf:resource="http://iflastandards.info/ns/lrm/lrmoo/F12_Nomen"/>
	<rdfs:range rdf:resource="http://iflastandards.info/ns/lrm/lrmoo/F12_Nomen"/>
	<rdfs:comment xml:lang="en">Quantification: many to many (0,n:0,n)

Shortcut Of: F12 Nomen (1). R33 has string: E62 String (1). P190i is symbolic content of: E90 Symbolic Object (1): P106 is composed of: E90 Symbolic Object (2). P190 has symbolic content: E62 String (2). R33i is string of: F12 Nomen (2)

Scope note:
This property associates an instance of F12 Nomen with another instance of F12 Nomen where the string of the domain instance of F12 Nomen includes the complete symbolic content of the string of the range instance of F12 Nomen. This property is not transitive. It is asymmetric and irreflexive.

Examples:
- ‘The Adoration of the Shepherds (Coventry)’ as a controlled access point for the work (F12) combines ‘The Adoration of the Shepherds’ as the preferred title of the work (F12).
- ‘The Adoration of the Shepherds (Coventry)’ as a controlled access point for the work (F12) combines ‘Coventry’ as a term that refers to a place (F12).
- ‘Guillaume, de Machaut, ca. 1300-1377’ as a controlled access point for the French composer and poet (F12) combines ‘ca. 1300-1377’ as a term that refers to a time-span (F12).
- ‘Guillaume, de Machaut, ca. 1300-1377’ as a controlled access point for the French composer and poet (F12) combines ‘Guillaume de Machaut’ as a name for the person (F12).
- ‘Univerza v Ljubljani. Oddelek za bibliotekarstvo’ as a controlled access point for a corporate body (F12) combines ‘Univerza v Ljubljani’ as a controlled access point for a parent corporate body (F12).
- ‘Univerza v Ljubljani. Oddelek za bibliotekarstvo’ as a controlled access point for a corporate body (F12) combines ‘Oddelek za bibliotekarstvo’ the preferred name that refers to a subordinate corporate body (F12).
- ISBN-10 ‘978-002-002-0’ as an identifier for the publication entitled ‘Nigeria’s international economic relations’ (F12) combines ‘978’ as a code indicating the Nigerian ISBN Agency (F12).
- ISBN-10 ‘978-002-002-0’ as an identifier for the publication entitled ‘Nigeria’s international economic relations’ (F12) combines ‘002’ as a code indicating the Nigerian Institute of International Affairs (F12).
- ISBN-10 ‘978-002-002-0’ as an identifier for the publication entitled ‘Nigeria’s international economic relations’ (F12) combines ‘002’ as a code for the publication entitled ‘Nigeria’s international economic relations’ (F12).
- ‘History -- France -- 14th century’ as a controlled subject term for the concept (F12) combines ‘History’ as the preferred term for the concept (F12). [Subject term constructed according to the order and syntax prescribed in the Library of Congress Subject Headings (LCSH) subject headings language.]
- ‘History -- France -- 14th century’ as a controlled subject term for the concept (F12) combines ‘France’ as the preferred term for the country (F12). [Subject term constructed according to the order and syntax prescribed in the Library of Congress Subject Headings (LCSH) subject headings language.]
- ‘History -- France -- 14th century’ as a controlled subject term for the concept (F12) combines ‘14th century’ as the preferred term for the time-span (F12). [Subject term constructed according to the order and syntax prescribed in the Library of Congress Subject Headings (LCSH) subject headings language.]
- ‘595.7096’ as a classification number for insects in Africa (F12) combines ‘595.7’ as the classification number for the taxonomic class Insecta (insects) (F12). [Classification number according to the 23rd edition of the Dewey Decimal Classification (DDC23).]
- ‘595.7096’ as a classification number for insects in Africa (F12) combines ‘096’ as the notation corresponding to the continent Africa (F12). [Classification number constructed using the geographic regions table in the 23rd edition of the Dewey Decimal Classification (DDC23).]
- ‘Orange (Colour)’ as a controlled subject term for the concept (F12) combines ‘Orange’ the English language term for the colour (F12). [Terms combined according to the syntax of the Art and Architecture Thesaurus (AAT).]
- ‘Orange (Colour)’ as a controlled subject term for the concept (F12) combines ‘Colour’ the English language term for the concept (F12). [Terms combined according to the syntax of the Art and Architecture Thesaurus (AAT).]
</rdfs:comment>
	<rdfs:label xml:lang="en">R8 combines</rdfs:label>
	<skos:notation>R8</skos:notation>
	<skos:prefLabel xml:lang="en">combines</skos:prefLabel>
</rdf:Description>

<rdf:Description rdf:about="http://iflastandards.info/ns/lrm/lrmoo/R8i_is_combined_to_form">
	<rdf:type rdf:resource="http://www.w3.org/2002/07/owl#ObjectProperty"/>
	<rdfs:domain rdf:resource="http://iflastandards.info/ns/lrm/lrmoo/F12_Nomen"/>
	<rdfs:range rdf:resource="http://iflastandards.info/ns/lrm/lrmoo/F12_Nomen"/>
	<rdfs:comment xml:lang="en">Quantification of the inverse property: many to many (0,n:0,n)

Shortcut Of of the inverse property: F12 Nomen (1). R33 has string: E62 String (1). P190i is symbolic content of: E90 Symbolic Object (1): P106 is composed of: E90 Symbolic Object (2). P190 has symbolic content: E62 String (2). R33i is string of: F12 Nomen (2)

Scope note of the inverse property:
This property associates an instance of F12 Nomen with another instance of F12 Nomen where the string of the domain instance of F12 Nomen includes the complete symbolic content of the string of the range instance of F12 Nomen. This property is not transitive. It is asymmetric and irreflexive.

Examples of the inverse property:
- ‘The Adoration of the Shepherds (Coventry)’ as a controlled access point for the work (F12) combines ‘The Adoration of the Shepherds’ as the preferred title of the work (F12).
- ‘The Adoration of the Shepherds (Coventry)’ as a controlled access point for the work (F12) combines ‘Coventry’ as a term that refers to a place (F12).
- ‘Guillaume, de Machaut, ca. 1300-1377’ as a controlled access point for the French composer and poet (F12) combines ‘ca. 1300-1377’ as a term that refers to a time-span (F12).
- ‘Guillaume, de Machaut, ca. 1300-1377’ as a controlled access point for the French composer and poet (F12) combines ‘Guillaume de Machaut’ as a name for the person (F12).
- ‘Univerza v Ljubljani. Oddelek za bibliotekarstvo’ as a controlled access point for a corporate body (F12) combines ‘Univerza v Ljubljani’ as a controlled access point for a parent corporate body (F12).
- ‘Univerza v Ljubljani. Oddelek za bibliotekarstvo’ as a controlled access point for a corporate body (F12) combines ‘Oddelek za bibliotekarstvo’ the preferred name that refers to a subordinate corporate body (F12).
- ISBN-10 ‘978-002-002-0’ as an identifier for the publication entitled ‘Nigeria’s international economic relations’ (F12) combines ‘978’ as a code indicating the Nigerian ISBN Agency (F12).
- ISBN-10 ‘978-002-002-0’ as an identifier for the publication entitled ‘Nigeria’s international economic relations’ (F12) combines ‘002’ as a code indicating the Nigerian Institute of International Affairs (F12).
- ISBN-10 ‘978-002-002-0’ as an identifier for the publication entitled ‘Nigeria’s international economic relations’ (F12) combines ‘002’ as a code for the publication entitled ‘Nigeria’s international economic relations’ (F12).
- ‘History -- France -- 14th century’ as a controlled subject term for the concept (F12) combines ‘History’ as the preferred term for the concept (F12). [Subject term constructed according to the order and syntax prescribed in the Library of Congress Subject Headings (LCSH) subject headings language.]
- ‘History -- France -- 14th century’ as a controlled subject term for the concept (F12) combines ‘France’ as the preferred term for the country (F12). [Subject term constructed according to the order and syntax prescribed in the Library of Congress Subject Headings (LCSH) subject headings language.]
- ‘History -- France -- 14th century’ as a controlled subject term for the concept (F12) combines ‘14th century’ as the preferred term for the time-span (F12). [Subject term constructed according to the order and syntax prescribed in the Library of Congress Subject Headings (LCSH) subject headings language.]
- ‘595.7096’ as a classification number for insects in Africa (F12) combines ‘595.7’ as the classification number for the taxonomic class Insecta (insects) (F12). [Classification number according to the 23rd edition of the Dewey Decimal Classification (DDC23).]
- ‘595.7096’ as a classification number for insects in Africa (F12) combines ‘096’ as the notation corresponding to the continent Africa (F12). [Classification number constructed using the geographic regions table in the 23rd edition of the Dewey Decimal Classification (DDC23).]
- ‘Orange (Colour)’ as a controlled subject term for the concept (F12) combines ‘Orange’ the English language term for the colour (F12). [Terms combined according to the syntax of the Art and Architecture Thesaurus (AAT).]
- ‘Orange (Colour)’ as a controlled subject term for the concept (F12) combines ‘Colour’ the English language term for the concept (F12). [Terms combined according to the syntax of the Art and Architecture Thesaurus (AAT).]
</rdfs:comment>
	<rdfs:label xml:lang="en">R8i is combined to form</rdfs:label>
	<skos:notation>R8i</skos:notation>
	<skos:prefLabel xml:lang="en">is combined to form</skos:prefLabel>
</rdf:Description>

<rdf:Description rdf:about="http://www.cidoc-crm.org/cidoc-crm/P100_was_death_of">
	<rdf:type rdf:resource="http://www.w3.org/2002/07/owl#ObjectProperty"/>
	<rdfs:subPropertyOf rdf:resource="http://www.cidoc-crm.org/cidoc-crm/P93_took_out_of_existence"/>
	<owl:inverseOf rdf:resource="http://www.cidoc-crm.org/cidoc-crm/P100i_died_in"/>
	<rdfs:domain rdf:resource="http://www.cidoc-crm.org/cidoc-crm/E69_Death"/>
	<rdfs:range rdf:resource="http://www.cidoc-crm.org/cidoc-crm/E21_Person"/>
	<rdfs:comment xml:lang="en">This property links an instance of E69 Death to the instance of E21 Person that died.
An instance of E69 Death may involve multiple people, for example in the case of a battle or disaster.
This is not intended for use with general natural history material, only people.</rdfs:comment>
	<rdfs:label xml:lang="de">Tod von</rdfs:label>
	<rdfs:label xml:lang="fr">a été la mort de</rdfs:label>
	<rdfs:label xml:lang="pt">foi a morte para</rdfs:label>
	<rdfs:label xml:lang="en">was death of</rdfs:label>
	<rdfs:label xml:lang="el">ήταν θάνατος του/της</rdfs:label>
	<rdfs:label xml:lang="ru">был смертью для</rdfs:label>
	<rdfs:label xml:lang="zh">死亡的是</rdfs:label>
</rdf:Description>

<rdf:Description rdf:about="http://www.cidoc-crm.org/cidoc-crm/P100i_died_in">
	<rdf:type rdf:resource="http://www.w3.org/2002/07/owl#ObjectProperty"/>
	<rdfs:subPropertyOf rdf:resource="http://www.cidoc-crm.org/cidoc-crm/P93i_was_taken_out_of_existence_by"/>
	<rdfs:domain rdf:resource="http://www.cidoc-crm.org/cidoc-crm/E21_Person"/>
	<rdfs:range rdf:resource="http://www.cidoc-crm.org/cidoc-crm/E69_Death"/>
	<rdfs:label xml:lang="en">died in</rdfs:label>
	<rdfs:label xml:lang="fr">est mort par</rdfs:label>
	<rdfs:label xml:lang="pt">morreu em</rdfs:label>
	<rdfs:label xml:lang="de">starb in</rdfs:label>
	<rdfs:label xml:lang="el">πέθανε σε</rdfs:label>
	<rdfs:label xml:lang="ru">умер в</rdfs:label>
	<rdfs:label xml:lang="zh">死于</rdfs:label>
</rdf:Description>

<rdf:Description rdf:about="http://www.cidoc-crm.org/cidoc-crm/P101_had_as_general_use">
	<rdf:type rdf:resource="http://www.w3.org/2002/07/owl#ObjectProperty"/>
	<owl:inverseOf rdf:resource="http://www.cidoc-crm.org/cidoc-crm/P101i_was_use_of"/>
	<rdfs:domain rdf:resource="http://www.cidoc-crm.org/cidoc-crm/E70_Thing"/>
	<rdfs:range rdf:resource="http://www.cidoc-crm.org/cidoc-crm/E55_Type"/>
	<rdfs:comment xml:lang="en">This property associates an instance of E70 Thing with an instance of E55 Type that describes the type of use that it was actually employed for.
It allows the relationship between particular things, both physical and immaterial, and the general methods and techniques of real use to be documented. This may well be different from the intended functional purpose of the instance of E70 Thing (which can be documented with P103 was intended for (was intention of)). For example, it could be recorded that a particular wooden crate had a general use as a shelf support on a market stall even though it had been originally intended for carrying vegetables.
The use of this property is intended to allow the documentation of usage patterns attested in historical records or through scientific investigation (for instance ceramic residue analysis). It should not be used to document the intended, and thus assumed, use of an object.</rdfs:comment>
	<rdfs:label xml:lang="fr">a eu pour usage général</rdfs:label>
	<rdfs:label xml:lang="en">had as general use</rdfs:label>
	<rdfs:label xml:lang="de">hatte die allgemeine Verwendung</rdfs:label>
	<rdfs:label xml:lang="pt">tem como uso geral</rdfs:label>
	<rdfs:label xml:lang="el">είχε ως γενική χρήση</rdfs:label>
	<rdfs:label xml:lang="ru">имел основное применение</rdfs:label>
	<rdfs:label xml:lang="zh">有一般用途</rdfs:label>
</rdf:Description>

<rdf:Description rdf:about="http://www.cidoc-crm.org/cidoc-crm/P101i_was_use_of">
	<rdf:type rdf:resource="http://www.w3.org/2002/07/owl#ObjectProperty"/>
	<rdfs:domain rdf:resource="http://www.cidoc-crm.org/cidoc-crm/E55_Type"/>
	<rdfs:range rdf:resource="http://www.cidoc-crm.org/cidoc-crm/E70_Thing"/>
	<rdfs:label xml:lang="fr">a été l'usage général de</rdfs:label>
	<rdfs:label xml:lang="pt">foi uso de</rdfs:label>
	<rdfs:label xml:lang="de">war die Verwendung von</rdfs:label>
	<rdfs:label xml:lang="en">was use of</rdfs:label>
	<rdfs:label xml:lang="el">ήταν χρήση του/της</rdfs:label>
	<rdfs:label xml:lang="ru">был применением для</rdfs:label>
	<rdfs:label xml:lang="zh">被用于</rdfs:label>
</rdf:Description>

<rdf:Description rdf:about="http://www.cidoc-crm.org/cidoc-crm/P102_has_title">
	<rdf:type rdf:resource="http://www.w3.org/2002/07/owl#ObjectProperty"/>
	<rdfs:subPropertyOf rdf:resource="http://www.cidoc-crm.org/cidoc-crm/P1_is_identified_by"/>
	<owl:inverseOf rdf:resource="http://www.cidoc-crm.org/cidoc-crm/P102i_is_title_of"/>
	<rdfs:domain rdf:resource="http://www.cidoc-crm.org/cidoc-crm/E71_Human-Made_Thing"/>
	<rdfs:range rdf:resource="http://www.cidoc-crm.org/cidoc-crm/E35_Title"/>
	<rdfs:comment xml:lang="en">This property associates an instance of E35 Title that has been applied to an instance of E71 Human-Made Thing.
The P102.1 has type property of the P102 has title (is title of) property enables the relationship between the title and the thing to be further clarified, for example, if the title was a given title, a supplied title etc.
It allows any human-made material or immaterial thing to be given a title. It is possible to imagine a title being created without a specific object in mind.</rdfs:comment>
	<rdfs:label xml:lang="fr">a pour titre</rdfs:label>
	<rdfs:label xml:lang="en">has title</rdfs:label>
	<rdfs:label xml:lang="pt">tem título</rdfs:label>
	<rdfs:label xml:lang="de">trägt den Titel</rdfs:label>
	<rdfs:label xml:lang="el">έχει τίτλο</rdfs:label>
	<rdfs:label xml:lang="ru">имеет заголовок</rdfs:label>
	<rdfs:label xml:lang="zh">有题名</rdfs:label>
</rdf:Description>

<rdf:Description rdf:about="http://www.cidoc-crm.org/cidoc-crm/P102i_is_title_of">
	<rdf:type rdf:resource="http://www.w3.org/2002/07/owl#ObjectProperty"/>
	<rdfs:subPropertyOf rdf:resource="http://www.cidoc-crm.org/cidoc-crm/P1i_identifies"/>
	<rdfs:domain rdf:resource="http://www.cidoc-crm.org/cidoc-crm/E35_Title"/>
	<rdfs:range rdf:resource="http://www.cidoc-crm.org/cidoc-crm/E71_Human-Made_Thing"/>
	<rdfs:label xml:lang="fr">est le titre de</rdfs:label>
	<rdfs:label xml:lang="en">is title of</rdfs:label>
	<rdfs:label xml:lang="de">ist der Titel von</rdfs:label>
	<rdfs:label xml:lang="pt">é título de</rdfs:label>
	<rdfs:label xml:lang="el">είναι τίτλος του/της</rdfs:label>
	<rdfs:label xml:lang="ru">является заголовком для</rdfs:label>
	<rdfs:label xml:lang="zh">题名是</rdfs:label>
</rdf:Description>

<rdf:Description rdf:about="http://www.cidoc-crm.org/cidoc-crm/P103_was_intended_for">
	<rdf:type rdf:resource="http://www.w3.org/2002/07/owl#ObjectProperty"/>
	<owl:inverseOf rdf:resource="http://www.cidoc-crm.org/cidoc-crm/P103i_was_intention_of"/>
	<rdfs:domain rdf:resource="http://www.cidoc-crm.org/cidoc-crm/E71_Human-Made_Thing"/>
	<rdfs:range rdf:resource="http://www.cidoc-crm.org/cidoc-crm/E55_Type"/>
	<rdfs:comment xml:lang="en">This property links an instance of E71 Human-Made Thing to an instance of E55 Type of usage or audience. It creates a relation between specific human-made things, both physical and immaterial, to E55 Types. This property can be used to specify intended methods and techniques of use or to characterise the intended audience by indicating a type of personal characteristic that everyone falling into the target audience has.
Note: A link between specific human-made things and a specific use activity should be expressed using P19 was intended use of (was made for).</rdfs:comment>
	<rdfs:label xml:lang="fr">a eu pour raison d'être</rdfs:label>
	<rdfs:label xml:lang="de">bestimmt für</rdfs:label>
	<rdfs:label xml:lang="pt">era destinado à</rdfs:label>
	<rdfs:label xml:lang="en">was intended for</rdfs:label>
	<rdfs:label xml:lang="el">προοριζόταν για</rdfs:label>
	<rdfs:label xml:lang="ru">был задуман для</rdfs:label>
	<rdfs:label xml:lang="zh">被用于</rdfs:label>
</rdf:Description>

<rdf:Description rdf:about="http://www.cidoc-crm.org/cidoc-crm/P103i_was_intention_of">
	<rdf:type rdf:resource="http://www.w3.org/2002/07/owl#ObjectProperty"/>
	<rdfs:domain rdf:resource="http://www.cidoc-crm.org/cidoc-crm/E55_Type"/>
	<rdfs:range rdf:resource="http://www.cidoc-crm.org/cidoc-crm/E71_Human-Made_Thing"/>
	<rdfs:label xml:lang="fr">a été la raison d'être de</rdfs:label>
	<rdfs:label xml:lang="pt">era a destinação de</rdfs:label>
	<rdfs:label xml:lang="de">war Bestimmung von</rdfs:label>
	<rdfs:label xml:lang="en">was intention of</rdfs:label>
	<rdfs:label xml:lang="el">ήταν προορισμός του</rdfs:label>
	<rdfs:label xml:lang="ru">был интенцией для</rdfs:label>
	<rdfs:label xml:lang="zh">目的是</rdfs:label>
</rdf:Description>

<rdf:Description rdf:about="http://www.cidoc-crm.org/cidoc-crm/P104_is_subject_to">
	<rdf:type rdf:resource="http://www.w3.org/2002/07/owl#ObjectProperty"/>
	<owl:inverseOf rdf:resource="http://www.cidoc-crm.org/cidoc-crm/P104i_applies_to"/>
	<rdfs:domain rdf:resource="http://www.cidoc-crm.org/cidoc-crm/E72_Legal_Object"/>
	<rdfs:range rdf:resource="http://www.cidoc-crm.org/cidoc-crm/E30_Right"/>
	<rdfs:comment xml:lang="en">This property links a particular instance of E72 Legal Object to the instances of E30 Right to which it is subject.
The Right is held by an instance of E39 Actor as described by P75 possesses (is possessed by).</rdfs:comment>
	<rdfs:label xml:lang="de">Gegenstand von</rdfs:label>
	<rdfs:label xml:lang="fr">est soumis à</rdfs:label>
	<rdfs:label xml:lang="pt">está sujeito à</rdfs:label>
	<rdfs:label xml:lang="en">is subject to</rdfs:label>
	<rdfs:label xml:lang="el">υπόκειται σε</rdfs:label>
	<rdfs:label xml:lang="ru">является объектом для</rdfs:label>
	<rdfs:label xml:lang="zh">服从</rdfs:label>
</rdf:Description>

<rdf:Description rdf:about="http://www.cidoc-crm.org/cidoc-crm/P104i_applies_to">
	<rdf:type rdf:resource="http://www.w3.org/2002/07/owl#ObjectProperty"/>
	<rdfs:domain rdf:resource="http://www.cidoc-crm.org/cidoc-crm/E30_Right"/>
	<rdfs:range rdf:resource="http://www.cidoc-crm.org/cidoc-crm/E72_Legal_Object"/>
	<rdfs:label xml:lang="en">applies to</rdfs:label>
	<rdfs:label xml:lang="de">findet Anwendung auf</rdfs:label>
	<rdfs:label xml:lang="pt">se aplicam à</rdfs:label>
	<rdfs:label xml:lang="fr">s’applique à</rdfs:label>
	<rdfs:label xml:lang="el">ισχύει για</rdfs:label>
	<rdfs:label xml:lang="ru">применяется к</rdfs:label>
	<rdfs:label xml:lang="zh">适用于</rdfs:label>
</rdf:Description>

<rdf:Description rdf:about="http://www.cidoc-crm.org/cidoc-crm/P105_right_held_by">
	<rdf:type rdf:resource="http://www.w3.org/2002/07/owl#ObjectProperty"/>
	<owl:inverseOf rdf:resource="http://www.cidoc-crm.org/cidoc-crm/P105i_has_right_on"/>
	<rdfs:domain rdf:resource="http://www.cidoc-crm.org/cidoc-crm/E72_Legal_Object"/>
	<rdfs:range rdf:resource="http://www.cidoc-crm.org/cidoc-crm/E39_Actor"/>
	<rdfs:comment xml:lang="en">This property identifies the instance of E39 Actor who holds the instances of E30 Right to an instance of E72 Legal Object.
It is a superproperty of P52 has current owner (is current owner of) because ownership is a right that is held on the owned object.
This property is a shortcut of the fully developed path from E72 Legal Object, P104 is subject to, E30 Right, P75i is possessed by to E39 Actor.</rdfs:comment>
	<rdfs:label xml:lang="de">Rechte stehen zu</rdfs:label>
	<rdfs:label xml:lang="fr">droit détenu par</rdfs:label>
	<rdfs:label xml:lang="en">right held by</rdfs:label>
	<rdfs:label xml:lang="pt">são direitos de</rdfs:label>
	<rdfs:label xml:lang="el">δικαίωμα κατέχεται από</rdfs:label>
	<rdfs:label xml:lang="ru">право принадлежит</rdfs:label>
	<rdfs:label xml:lang="zh">持有权利的是</rdfs:label>
</rdf:Description>

<rdf:Description rdf:about="http://www.cidoc-crm.org/cidoc-crm/P105i_has_right_on">
	<rdf:type rdf:resource="http://www.w3.org/2002/07/owl#ObjectProperty"/>
	<rdfs:domain rdf:resource="http://www.cidoc-crm.org/cidoc-crm/E39_Actor"/>
	<rdfs:range rdf:resource="http://www.cidoc-crm.org/cidoc-crm/E72_Legal_Object"/>
	<rdfs:label xml:lang="fr">détient le droit sur</rdfs:label>
	<rdfs:label xml:lang="en">has right on</rdfs:label>
	<rdfs:label xml:lang="de">hat Rechte an</rdfs:label>
	<rdfs:label xml:lang="pt">possui direitos sobre</rdfs:label>
	<rdfs:label xml:lang="el">έχει δικαίωμα σε</rdfs:label>
	<rdfs:label xml:lang="ru">владеет правом на</rdfs:label>
	<rdfs:label xml:lang="zh">有权利</rdfs:label>
</rdf:Description>

<rdf:Description rdf:about="http://www.cidoc-crm.org/cidoc-crm/P106_is_composed_of">
	<rdf:type rdf:resource="http://www.w3.org/2002/07/owl#ObjectProperty"/>
	<owl:inverseOf rdf:resource="http://www.cidoc-crm.org/cidoc-crm/P106i_forms_part_of"/>
	<rdfs:domain rdf:resource="http://www.cidoc-crm.org/cidoc-crm/E90_Symbolic_Object"/>
	<rdfs:range rdf:resource="http://www.cidoc-crm.org/cidoc-crm/E90_Symbolic_Object"/>
	<rdfs:comment xml:lang="en">This property associates an instance of E90 Symbolic Object with a part of it that is by itself an instance of E90 Symbolic Object, such as fragments of texts or clippings from an image.
This property is transitive asymmetric.</rdfs:comment>
	<rdfs:label xml:lang="fr">est composé de</rdfs:label>
	<rdfs:label xml:lang="en">is composed of</rdfs:label>
	<rdfs:label xml:lang="de">ist zusammengesetzt aus</rdfs:label>
	<rdfs:label xml:lang="pt">é composto de</rdfs:label>
	<rdfs:label xml:lang="el">αποτελείται από</rdfs:label>
	<rdfs:label xml:lang="ru">составлен из</rdfs:label>
	<rdfs:label xml:lang="zh">组成成分是</rdfs:label>
</rdf:Description>

<rdf:Description rdf:about="http://www.cidoc-crm.org/cidoc-crm/P106i_forms_part_of">
	<rdf:type rdf:resource="http://www.w3.org/2002/07/owl#ObjectProperty"/>
	<rdfs:domain rdf:resource="http://www.cidoc-crm.org/cidoc-crm/E90_Symbolic_Object"/>
	<rdfs:range rdf:resource="http://www.cidoc-crm.org/cidoc-crm/E90_Symbolic_Object"/>
	<rdfs:label xml:lang="de">bildet Teil von</rdfs:label>
	<rdfs:label xml:lang="fr">fait partie de</rdfs:label>
	<rdfs:label xml:lang="pt">faz parte de</rdfs:label>
	<rdfs:label xml:lang="en">forms part of</rdfs:label>
	<rdfs:label xml:lang="el">αποτελεί μέρος του/της</rdfs:label>
	<rdfs:label xml:lang="ru">формирует часть</rdfs:label>
	<rdfs:label xml:lang="zh">构成部分</rdfs:label>
</rdf:Description>

<rdf:Description rdf:about="http://www.cidoc-crm.org/cidoc-crm/P107_has_current_or_former_member">
	<rdf:type rdf:resource="http://www.w3.org/2002/07/owl#ObjectProperty"/>
	<owl:inverseOf rdf:resource="http://www.cidoc-crm.org/cidoc-crm/P107i_is_current_or_former_member_of"/>
	<rdfs:domain rdf:resource="http://www.cidoc-crm.org/cidoc-crm/E74_Group"/>
	<rdfs:range rdf:resource="http://www.cidoc-crm.org/cidoc-crm/E39_Actor"/>
	<rdfs:comment xml:lang="en">This property associates an instance of E74 Group with an instance of E39 Actor that is or has been a member thereof.
Instances of E74 Group and E21 Person may all be members of instances of E74 Group. An instance of E74 Group may be founded initially without any member.
This property is a shortcut of the more fully developed path from E74 Group, P144i gained member by, E85 Joining, P143 joined to E39 Actor.
The property P107.1 kind of member can be used to specify the type of membership or the role the member has in the group.</rdfs:comment>
	<rdfs:label xml:lang="fr">a pour membre actuel ou antérieur</rdfs:label>
	<rdfs:label xml:lang="en">has current or former member</rdfs:label>
	<rdfs:label xml:lang="de">hat derzeitiges oder früheres Mitglied</rdfs:label>
	<rdfs:label xml:lang="pt">tem ou teve membro</rdfs:label>
	<rdfs:label xml:lang="el">έχει ή είχε μέλος</rdfs:label>
	<rdfs:label xml:lang="ru">имеет действующего или бывшего члена</rdfs:label>
	<rdfs:label xml:lang="zh">有当前或以往成员</rdfs:label>
</rdf:Description>

<rdf:Description rdf:about="http://www.cidoc-crm.org/cidoc-crm/P107i_is_current_or_former_member_of">
	<rdf:type rdf:resource="http://www.w3.org/2002/07/owl#ObjectProperty"/>
	<rdfs:domain rdf:resource="http://www.cidoc-crm.org/cidoc-crm/E39_Actor"/>
	<rdfs:range rdf:resource="http://www.cidoc-crm.org/cidoc-crm/E74_Group"/>
	<rdfs:label xml:lang="fr">est le membre actuel ou antérieur de</rdfs:label>
	<rdfs:label xml:lang="en">is current or former member of</rdfs:label>
	<rdfs:label xml:lang="de">ist derzeitiges oder früheres Mitglied von</rdfs:label>
	<rdfs:label xml:lang="pt">é ou foi membro de</rdfs:label>
	<rdfs:label xml:lang="el">είναι ή ήταν μέλος του/της</rdfs:label>
	<rdfs:label xml:lang="ru">является действующим или бывшим членом</rdfs:label>
	<rdfs:label xml:lang="zh">是当前或以往成员</rdfs:label>
</rdf:Description>

<rdf:Description rdf:about="http://www.cidoc-crm.org/cidoc-crm/P108_has_produced">
	<rdf:type rdf:resource="http://www.w3.org/2002/07/owl#ObjectProperty"/>
	<rdfs:subPropertyOf rdf:resource="http://www.cidoc-crm.org/cidoc-crm/P31_has_modified"/>
	<rdfs:subPropertyOf rdf:resource="http://www.cidoc-crm.org/cidoc-crm/P92_brought_into_existence"/>
	<owl:inverseOf rdf:resource="http://www.cidoc-crm.org/cidoc-crm/P108i_was_produced_by"/>
	<rdfs:domain rdf:resource="http://www.cidoc-crm.org/cidoc-crm/E12_Production"/>
	<rdfs:range rdf:resource="http://www.cidoc-crm.org/cidoc-crm/E24_Physical_Human-Made_Thing"/>
	<rdfs:comment xml:lang="en">This property identifies the instance of E24 Physical Human-Made Thing that came into existence as a result of the instance of E12 Production.
The identity of an instance of E24 Physical Human-Made Thing is not defined by its matter, but by its existence as a subject of documentation. An E12 Production can result in the creation of multiple instances of E24 Physical Human-Made Thing.</rdfs:comment>
	<rdfs:label xml:lang="fr">a produit</rdfs:label>
	<rdfs:label xml:lang="en">has produced</rdfs:label>
	<rdfs:label xml:lang="de">hat hergestellt</rdfs:label>
	<rdfs:label xml:lang="pt">produziu</rdfs:label>
	<rdfs:label xml:lang="el">παρήγαγε</rdfs:label>
	<rdfs:label xml:lang="ru">произвел</rdfs:label>
	<rdfs:label xml:lang="zh">已产生了</rdfs:label>
</rdf:Description>

<rdf:Description rdf:about="http://www.cidoc-crm.org/cidoc-crm/P108i_was_produced_by">
	<rdf:type rdf:resource="http://www.w3.org/2002/07/owl#ObjectProperty"/>
	<rdfs:subPropertyOf rdf:resource="http://www.cidoc-crm.org/cidoc-crm/P31i_was_modified_by"/>
	<rdfs:subPropertyOf rdf:resource="http://www.cidoc-crm.org/cidoc-crm/P92i_was_brought_into_existence_by"/>
	<rdfs:domain rdf:resource="http://www.cidoc-crm.org/cidoc-crm/E24_Physical_Human-Made_Thing"/>
	<rdfs:range rdf:resource="http://www.cidoc-crm.org/cidoc-crm/E12_Production"/>
	<rdfs:label xml:lang="fr">a été produit par</rdfs:label>
	<rdfs:label xml:lang="pt">foi produzido por</rdfs:label>
	<rdfs:label xml:lang="en">was produced by</rdfs:label>
	<rdfs:label xml:lang="de">wurde hergestellt durch</rdfs:label>
	<rdfs:label xml:lang="el">παρήχθη από</rdfs:label>
	<rdfs:label xml:lang="ru">был произведен посредством</rdfs:label>
	<rdfs:label xml:lang="zh">被产生</rdfs:label>
</rdf:Description>

<rdf:Description rdf:about="http://www.cidoc-crm.org/cidoc-crm/P109_has_current_or_former_curator">
	<rdf:type rdf:resource="http://www.w3.org/2002/07/owl#ObjectProperty"/>
	<rdfs:subPropertyOf rdf:resource="http://www.cidoc-crm.org/cidoc-crm/P49_has_former_or_current_keeper"/>
	<owl:inverseOf rdf:resource="http://www.cidoc-crm.org/cidoc-crm/P109i_is_current_or_former_curator_of"/>
	<rdfs:domain rdf:resource="http://www.cidoc-crm.org/cidoc-crm/E78_Curated_Holding"/>
	<rdfs:range rdf:resource="http://www.cidoc-crm.org/cidoc-crm/E39_Actor"/>
	<rdfs:comment xml:lang="en">This property identifies the instance of E39 Actor who assumed or has assumed overall curatorial responsibility for an instance of E78 Curated Holding.
It does not allow a history of curation to be recorded. This would require use of an event initiating a curator being responsible for a collection.</rdfs:comment>
	<rdfs:label xml:lang="fr">a pour responsable actuel ou antérieur de la collection</rdfs:label>
	<rdfs:label xml:lang="en">has current or former curator</rdfs:label>
	<rdfs:label xml:lang="de">hat derzeitigen oder früheren Kurator</rdfs:label>
	<rdfs:label xml:lang="pt">tem ou teve curador</rdfs:label>
	<rdfs:label xml:lang="el">έχει ή είχε επιμελητή</rdfs:label>
	<rdfs:label xml:lang="ru">имеет действующего или бывшего хранителя</rdfs:label>
	<rdfs:label xml:lang="zh">有当前或以往管理者</rdfs:label>
</rdf:Description>

<rdf:Description rdf:about="http://www.cidoc-crm.org/cidoc-crm/P109i_is_current_or_former_curator_of">
	<rdf:type rdf:resource="http://www.w3.org/2002/07/owl#ObjectProperty"/>
	<rdfs:subPropertyOf rdf:resource="http://www.cidoc-crm.org/cidoc-crm/P49i_is_former_or_current_keeper_of"/>
	<rdfs:domain rdf:resource="http://www.cidoc-crm.org/cidoc-crm/E39_Actor"/>
	<rdfs:range rdf:resource="http://www.cidoc-crm.org/cidoc-crm/E78_Curated_Holding"/>
	<rdfs:label xml:lang="fr">est responsable actuel ou antérieur de la collection</rdfs:label>
	<rdfs:label xml:lang="en">is current or former curator of</rdfs:label>
	<rdfs:label xml:lang="de">ist derzeitiger oder früherer Kurator von</rdfs:label>
	<rdfs:label xml:lang="pt">é ou foi curador de</rdfs:label>
	<rdfs:label xml:lang="el">είναι ή ήταν επιμελητής του/της</rdfs:label>
	<rdfs:label xml:lang="ru">является действующим или бывшим хранителем</rdfs:label>
	<rdfs:label xml:lang="zh">是当前或以往管理者</rdfs:label>
</rdf:Description>

<rdf:Description rdf:about="http://www.cidoc-crm.org/cidoc-crm/P10_falls_within">
	<rdf:type rdf:resource="http://www.w3.org/2002/07/owl#ObjectProperty"/>
	<rdfs:subPropertyOf rdf:resource="http://www.cidoc-crm.org/cidoc-crm/P132_spatiotemporally_overlaps_with"/>
	<owl:inverseOf rdf:resource="http://www.cidoc-crm.org/cidoc-crm/P10i_contains"/>
	<rdfs:domain rdf:resource="http://www.cidoc-crm.org/cidoc-crm/E92_Spacetime_Volume"/>
	<rdfs:range rdf:resource="http://www.cidoc-crm.org/cidoc-crm/E92_Spacetime_Volume"/>
	<rdfs:comment xml:lang="en">This property associates an instance of E92 Spacetime Volume with another instance of E92 Spacetime Volume that falls within the latter. In other words, all points in the former are also points in the latter.
This property is transitive and reflexive.</rdfs:comment>
	<rdfs:label xml:lang="pt">está contido em</rdfs:label>
	<rdfs:label xml:lang="en">falls within</rdfs:label>
	<rdfs:label xml:lang="de">fällt in</rdfs:label>
	<rdfs:label xml:lang="fr">s’insère dans</rdfs:label>
	<rdfs:label xml:lang="el">εμπίπτει</rdfs:label>
	<rdfs:label xml:lang="ru">находится в пределах</rdfs:label>
	<rdfs:label xml:lang="zh">属于</rdfs:label>
</rdf:Description>

<rdf:Description rdf:about="http://www.cidoc-crm.org/cidoc-crm/P10i_contains">
	<rdf:type rdf:resource="http://www.w3.org/2002/07/owl#ObjectProperty"/>
	<rdfs:subPropertyOf rdf:resource="http://www.cidoc-crm.org/cidoc-crm/P132_spatiotemporally_overlaps_with"/>
	<rdfs:domain rdf:resource="http://www.cidoc-crm.org/cidoc-crm/E92_Spacetime_Volume"/>
	<rdfs:range rdf:resource="http://www.cidoc-crm.org/cidoc-crm/E92_Spacetime_Volume"/>
	<rdfs:label xml:lang="en">contains</rdfs:label>
	<rdfs:label xml:lang="fr">contient</rdfs:label>
	<rdfs:label xml:lang="pt">contém</rdfs:label>
	<rdfs:label xml:lang="de">enthält</rdfs:label>
	<rdfs:label xml:lang="el">περιλαμβάνει</rdfs:label>
	<rdfs:label xml:lang="ru">содержит</rdfs:label>
	<rdfs:label xml:lang="zh">包含</rdfs:label>
</rdf:Description>

<rdf:Description rdf:about="http://www.cidoc-crm.org/cidoc-crm/P110_augmented">
	<rdf:type rdf:resource="http://www.w3.org/2002/07/owl#ObjectProperty"/>
	<rdfs:subPropertyOf rdf:resource="http://www.cidoc-crm.org/cidoc-crm/P31_has_modified"/>
	<owl:inverseOf rdf:resource="http://www.cidoc-crm.org/cidoc-crm/P110i_was_augmented_by"/>
	<rdfs:domain rdf:resource="http://www.cidoc-crm.org/cidoc-crm/E79_Part_Addition"/>
	<rdfs:range rdf:resource="http://www.cidoc-crm.org/cidoc-crm/E18_Physical_Thing"/>
	<rdfs:comment xml:lang="en">This property identifies the instance of E18 Physical Thing that is added to (augmented) in an instance of E79 Part Addition.
Although an instance of E79 Part Addition event normally concerns only one instance of E18 Physical Thing, it is possible to imagine circumstances under which more than one item might be added to (augmented). For example, the artist Jackson Pollock trailing paint onto multiple canvasses.</rdfs:comment>
	<rdfs:label xml:lang="fr">a augmenté</rdfs:label>
	<rdfs:label xml:lang="en">augmented</rdfs:label>
	<rdfs:label xml:lang="pt">aumentou</rdfs:label>
	<rdfs:label xml:lang="de">erweiterte</rdfs:label>
	<rdfs:label xml:lang="el">επαύξησε</rdfs:label>
	<rdfs:label xml:lang="ru">увеличил</rdfs:label>
	<rdfs:label xml:lang="zh">增强了</rdfs:label>
</rdf:Description>

<rdf:Description rdf:about="http://www.cidoc-crm.org/cidoc-crm/P110i_was_augmented_by">
	<rdf:type rdf:resource="http://www.w3.org/2002/07/owl#ObjectProperty"/>
	<rdfs:subPropertyOf rdf:resource="http://www.cidoc-crm.org/cidoc-crm/P31i_was_modified_by"/>
	<rdfs:domain rdf:resource="http://www.cidoc-crm.org/cidoc-crm/E18_Physical_Thing"/>
	<rdfs:range rdf:resource="http://www.cidoc-crm.org/cidoc-crm/E79_Part_Addition"/>
	<rdfs:label xml:lang="fr">a été augmenté par</rdfs:label>
	<rdfs:label xml:lang="pt">foi aumentada por</rdfs:label>
	<rdfs:label xml:lang="en">was augmented by</rdfs:label>
	<rdfs:label xml:lang="de">wurde erweitert durch</rdfs:label>
	<rdfs:label xml:lang="el">επαυξήθηκε από</rdfs:label>
	<rdfs:label xml:lang="ru">был увеличен посредством</rdfs:label>
	<rdfs:label xml:lang="zh">被增强</rdfs:label>
</rdf:Description>

<rdf:Description rdf:about="http://www.cidoc-crm.org/cidoc-crm/P111_added">
	<rdf:type rdf:resource="http://www.w3.org/2002/07/owl#ObjectProperty"/>
	<rdfs:subPropertyOf rdf:resource="http://www.cidoc-crm.org/cidoc-crm/P16_used_specific_object"/>
	<owl:inverseOf rdf:resource="http://www.cidoc-crm.org/cidoc-crm/P111i_was_added_by"/>
	<rdfs:domain rdf:resource="http://www.cidoc-crm.org/cidoc-crm/E79_Part_Addition"/>
	<rdfs:range rdf:resource="http://www.cidoc-crm.org/cidoc-crm/E18_Physical_Thing"/>
	<rdfs:comment xml:lang="en">This property identifies the instance of E18 Physical Thing that is added during an instance of E79 Part Addition activity.</rdfs:comment>
	<rdfs:label xml:lang="fr">a ajouté</rdfs:label>
	<rdfs:label xml:lang="en">added</rdfs:label>
	<rdfs:label xml:lang="pt">adicionou</rdfs:label>
	<rdfs:label xml:lang="de">fügte hinzu</rdfs:label>
	<rdfs:label xml:lang="el">προσέθεσε</rdfs:label>
	<rdfs:label xml:lang="ru">добавил</rdfs:label>
	<rdfs:label xml:lang="zh">增加了</rdfs:label>
</rdf:Description>

<rdf:Description rdf:about="http://www.cidoc-crm.org/cidoc-crm/P111i_was_added_by">
	<rdf:type rdf:resource="http://www.w3.org/2002/07/owl#ObjectProperty"/>
	<rdfs:subPropertyOf rdf:resource="http://www.cidoc-crm.org/cidoc-crm/P16i_was_used_for"/>
	<rdfs:domain rdf:resource="http://www.cidoc-crm.org/cidoc-crm/E18_Physical_Thing"/>
	<rdfs:range rdf:resource="http://www.cidoc-crm.org/cidoc-crm/E79_Part_Addition"/>
	<rdfs:label xml:lang="fr">a été ajouté par</rdfs:label>
	<rdfs:label xml:lang="pt">foi adicionado por</rdfs:label>
	<rdfs:label xml:lang="en">was added by</rdfs:label>
	<rdfs:label xml:lang="de">wurde hinzugefügt durch</rdfs:label>
	<rdfs:label xml:lang="el">προστέθηκε από</rdfs:label>
	<rdfs:label xml:lang="ru">был добавлен посредством</rdfs:label>
	<rdfs:label xml:lang="zh">被增加</rdfs:label>
</rdf:Description>

<rdf:Description rdf:about="http://www.cidoc-crm.org/cidoc-crm/P112_diminished">
	<rdf:type rdf:resource="http://www.w3.org/2002/07/owl#ObjectProperty"/>
	<rdfs:subPropertyOf rdf:resource="http://www.cidoc-crm.org/cidoc-crm/P31_has_modified"/>
	<owl:inverseOf rdf:resource="http://www.cidoc-crm.org/cidoc-crm/P112i_was_diminished_by"/>
	<rdfs:domain rdf:resource="http://www.cidoc-crm.org/cidoc-crm/E80_Part_Removal"/>
	<rdfs:range rdf:resource="http://www.cidoc-crm.org/cidoc-crm/E18_Physical_Thing"/>
	<rdfs:comment xml:lang="en">This property identifies the instance of E18 Physical Thing that was diminished by an instance of E80 Part Removal.
Although an instance of E80 Part removal activity normally concerns only one instance of E18 Physical Thing, it is possible to imagine circumstances under which more than one item might be diminished by a single instance of E80 Part Removal activity.</rdfs:comment>
	<rdfs:label xml:lang="fr">a diminué</rdfs:label>
	<rdfs:label xml:lang="en">diminished</rdfs:label>
	<rdfs:label xml:lang="pt">diminuiu</rdfs:label>
	<rdfs:label xml:lang="de">verminderte</rdfs:label>
	<rdfs:label xml:lang="el">εξάλειψε</rdfs:label>
	<rdfs:label xml:lang="ru">уменьшил</rdfs:label>
	<rdfs:label xml:lang="zh">减少了</rdfs:label>
</rdf:Description>

<rdf:Description rdf:about="http://www.cidoc-crm.org/cidoc-crm/P112i_was_diminished_by">
	<rdf:type rdf:resource="http://www.w3.org/2002/07/owl#ObjectProperty"/>
	<rdfs:subPropertyOf rdf:resource="http://www.cidoc-crm.org/cidoc-crm/P31i_was_modified_by"/>
	<rdfs:domain rdf:resource="http://www.cidoc-crm.org/cidoc-crm/E18_Physical_Thing"/>
	<rdfs:range rdf:resource="http://www.cidoc-crm.org/cidoc-crm/E80_Part_Removal"/>
	<rdfs:label xml:lang="fr">a été diminué par</rdfs:label>
	<rdfs:label xml:lang="pt">foi diminuído por</rdfs:label>
	<rdfs:label xml:lang="en">was diminished by</rdfs:label>
	<rdfs:label xml:lang="de">wurde vermindert durch</rdfs:label>
	<rdfs:label xml:lang="el">εξαλείφθηκε από</rdfs:label>
	<rdfs:label xml:lang="ru">был уменьшен посредством</rdfs:label>
	<rdfs:label xml:lang="zh">被减少</rdfs:label>
</rdf:Description>

<rdf:Description rdf:about="http://www.cidoc-crm.org/cidoc-crm/P113_removed">
	<rdf:type rdf:resource="http://www.w3.org/2002/07/owl#ObjectProperty"/>
	<rdfs:subPropertyOf rdf:resource="http://www.cidoc-crm.org/cidoc-crm/P12_occurred_in_the_presence_of"/>
	<owl:inverseOf rdf:resource="http://www.cidoc-crm.org/cidoc-crm/P113i_was_removed_by"/>
	<rdfs:domain rdf:resource="http://www.cidoc-crm.org/cidoc-crm/E80_Part_Removal"/>
	<rdfs:range rdf:resource="http://www.cidoc-crm.org/cidoc-crm/E18_Physical_Thing"/>
	<rdfs:comment xml:lang="en">This property identifies the instance of E18 Physical Thing that is removed during an instance of E80 Part Removal activity.</rdfs:comment>
	<rdfs:label xml:lang="fr">a retiré</rdfs:label>
	<rdfs:label xml:lang="de">entfernte</rdfs:label>
	<rdfs:label xml:lang="en">removed</rdfs:label>
	<rdfs:label xml:lang="pt">removeu</rdfs:label>
	<rdfs:label xml:lang="el">αφαίρεσε</rdfs:label>
	<rdfs:label xml:lang="ru">удален</rdfs:label>
	<rdfs:label xml:lang="zh">去除了</rdfs:label>
</rdf:Description>

<rdf:Description rdf:about="http://www.cidoc-crm.org/cidoc-crm/P113i_was_removed_by">
	<rdf:type rdf:resource="http://www.w3.org/2002/07/owl#ObjectProperty"/>
	<rdfs:subPropertyOf rdf:resource="http://www.cidoc-crm.org/cidoc-crm/P12i_was_present_at"/>
	<rdfs:domain rdf:resource="http://www.cidoc-crm.org/cidoc-crm/E18_Physical_Thing"/>
	<rdfs:range rdf:resource="http://www.cidoc-crm.org/cidoc-crm/E80_Part_Removal"/>
	<rdfs:label xml:lang="fr">a été retiré par</rdfs:label>
	<rdfs:label xml:lang="pt">foi removido por</rdfs:label>
	<rdfs:label xml:lang="en">was removed by</rdfs:label>
	<rdfs:label xml:lang="de">wurde entfernt durch</rdfs:label>
	<rdfs:label xml:lang="el">αφαιρέθηκε από</rdfs:label>
	<rdfs:label xml:lang="ru">был удален посредством</rdfs:label>
	<rdfs:label xml:lang="zh">被去除</rdfs:label>
</rdf:Description>

<rdf:Description rdf:about="http://www.cidoc-crm.org/cidoc-crm/P11_had_participant">
	<rdf:type rdf:resource="http://www.w3.org/2002/07/owl#ObjectProperty"/>
	<rdfs:subPropertyOf rdf:resource="http://www.cidoc-crm.org/cidoc-crm/P12_occurred_in_the_presence_of"/>
	<owl:inverseOf rdf:resource="http://www.cidoc-crm.org/cidoc-crm/P11i_participated_in"/>
	<rdfs:domain rdf:resource="http://www.cidoc-crm.org/cidoc-crm/E5_Event"/>
	<rdfs:range rdf:resource="http://www.cidoc-crm.org/cidoc-crm/E39_Actor"/>
	<rdfs:comment xml:lang="en">This property describes the active or passive participation of instances of E39 Actors in an instance of E5 Event.
It documents known events in which an instance of E39 Actor has participated during the course of that actor’s life or history. The instances of E53 Place and E52 Time-Span where and when these events happened provide constraints about the presence of the related instances of E39 Actor in the past. Collective actors, i.e. instances of E74 Group, may physically participate in events via their representing instances of E21 Persons only. The participation of multiple actors in an event is most likely an indication of their acquaintance and interaction.
The property implies that the actor was involved in the event but does not imply any causal relationship. For instance, someone having been portrayed can be said to have participated in the creation of the portrait.</rdfs:comment>
	<rdfs:label xml:lang="fr">a eu pour actant participant</rdfs:label>
	<rdfs:label xml:lang="en">had participant</rdfs:label>
	<rdfs:label xml:lang="de">hatte Teilnehmer</rdfs:label>
	<rdfs:label xml:lang="pt">tem participante</rdfs:label>
	<rdfs:label xml:lang="el">είχε συμμέτοχο</rdfs:label>
	<rdfs:label xml:lang="ru">имел участника</rdfs:label>
	<rdfs:label xml:lang="zh">有参与者</rdfs:label>
</rdf:Description>

<rdf:Description rdf:about="http://www.cidoc-crm.org/cidoc-crm/P11i_participated_in">
	<rdf:type rdf:resource="http://www.w3.org/2002/07/owl#ObjectProperty"/>
	<rdfs:subPropertyOf rdf:resource="http://www.cidoc-crm.org/cidoc-crm/P12i_was_present_at"/>
	<rdfs:domain rdf:resource="http://www.cidoc-crm.org/cidoc-crm/E39_Actor"/>
	<rdfs:range rdf:resource="http://www.cidoc-crm.org/cidoc-crm/E5_Event"/>
	<rdfs:label xml:lang="fr">a participé à</rdfs:label>
	<rdfs:label xml:lang="de">nahm Teil an</rdfs:label>
	<rdfs:label xml:lang="pt">participa em</rdfs:label>
	<rdfs:label xml:lang="en">participated in</rdfs:label>
	<rdfs:label xml:lang="el">συμμετείχε σε</rdfs:label>
	<rdfs:label xml:lang="ru">участвовал в</rdfs:label>
	<rdfs:label xml:lang="zh">参与</rdfs:label>
</rdf:Description>

<rdf:Description rdf:about="http://www.cidoc-crm.org/cidoc-crm/P121_overlaps_with">
	<rdf:type rdf:resource="http://www.w3.org/2002/07/owl#ObjectProperty"/>
	<rdfs:domain rdf:resource="http://www.cidoc-crm.org/cidoc-crm/E53_Place"/>
	<rdfs:range rdf:resource="http://www.cidoc-crm.org/cidoc-crm/E53_Place"/>
	<rdfs:comment xml:lang="en">This symmetric property associates an instance of E53 Place with another instance of E53 Place geometrically overlapping it.
It does not specify anything about the shared area. This property is purely spatial. It does not imply that phenomena that define, by their extent, places related by P121 overlaps with have ever covered a common area at the same time or even coexisted. In contrast, spatiotemporal overlaps described by P132 spatiotemporally overlaps are the total of areas simultaneously covered by the related spacetime volumes.
This property is symmetric. This property is reflexive.</rdfs:comment>
	<rdfs:label xml:lang="en">overlaps with</rdfs:label>
	<rdfs:label xml:lang="fr">se superpose partiellement à</rdfs:label>
	<rdfs:label xml:lang="pt">sobrepõe com</rdfs:label>
	<rdfs:label xml:lang="de">überlappt mit</rdfs:label>
	<rdfs:label xml:lang="el">επικαλύπτεται με</rdfs:label>
	<rdfs:label xml:lang="ru">пересекается с</rdfs:label>
	<rdfs:label xml:lang="zh">重叠于</rdfs:label>
</rdf:Description>

<rdf:Description rdf:about="http://www.cidoc-crm.org/cidoc-crm/P122_borders_with">
	<rdf:type rdf:resource="http://www.w3.org/2002/07/owl#ObjectProperty"/>
	<rdfs:domain rdf:resource="http://www.cidoc-crm.org/cidoc-crm/E53_Place"/>
	<rdfs:range rdf:resource="http://www.cidoc-crm.org/cidoc-crm/E53_Place"/>
	<rdfs:comment xml:lang="en">This symmetric property associates an instance of E53 Place with another instance of E53 Place which shares a part of its border.
This property is purely spatial. It does not imply that the phenomena that define, by their extent, places related by P122 borders with have ever shared a respective border at the same time or even coexisted. In particular, this may be the case when the respective common border is formed by a natural feature.
This property is not transitive. This property is symmetric.</rdfs:comment>
	<rdfs:label xml:lang="en">borders with</rdfs:label>
	<rdfs:label xml:lang="fr">est limitrophe de</rdfs:label>
	<rdfs:label xml:lang="pt">fronteira com</rdfs:label>
	<rdfs:label xml:lang="de">grenzt an</rdfs:label>
	<rdfs:label xml:lang="el">συνορεύει με</rdfs:label>
	<rdfs:label xml:lang="ru">граничит с</rdfs:label>
	<rdfs:label xml:lang="zh">接壤于</rdfs:label>
</rdf:Description>

<rdf:Description rdf:about="http://www.cidoc-crm.org/cidoc-crm/P123_resulted_in">
	<rdf:type rdf:resource="http://www.w3.org/2002/07/owl#ObjectProperty"/>
	<rdfs:subPropertyOf rdf:resource="http://www.cidoc-crm.org/cidoc-crm/P92_brought_into_existence"/>
	<owl:inverseOf rdf:resource="http://www.cidoc-crm.org/cidoc-crm/P123i_resulted_from"/>
	<rdfs:domain rdf:resource="http://www.cidoc-crm.org/cidoc-crm/E81_Transformation"/>
	<rdfs:range rdf:resource="http://www.cidoc-crm.org/cidoc-crm/E18_Physical_Thing"/>
	<rdfs:comment xml:lang="en">This property identifies the instance or instances of E18 Physical Thing that are the result of an instance of E81 Transformation. New items replace the transformed item or items, which cease to exist as units of documentation. The physical continuity between the old and the new is expressed by the links to the common instance of E81 Transformation.</rdfs:comment>
	<rdfs:label xml:lang="fr">a eu pour résultat</rdfs:label>
	<rdfs:label xml:lang="de">ergab</rdfs:label>
	<rdfs:label xml:lang="en">resulted in</rdfs:label>
	<rdfs:label xml:lang="pt">resultou em</rdfs:label>
	<rdfs:label xml:lang="el">είχε ως αποτέλεσμα</rdfs:label>
	<rdfs:label xml:lang="ru">повлек появление</rdfs:label>
	<rdfs:label xml:lang="zh">结果造成</rdfs:label>
</rdf:Description>

<rdf:Description rdf:about="http://www.cidoc-crm.org/cidoc-crm/P123i_resulted_from">
	<rdf:type rdf:resource="http://www.w3.org/2002/07/owl#ObjectProperty"/>
	<rdfs:subPropertyOf rdf:resource="http://www.cidoc-crm.org/cidoc-crm/P92i_was_brought_into_existence_by"/>
	<rdfs:domain rdf:resource="http://www.cidoc-crm.org/cidoc-crm/E18_Physical_Thing"/>
	<rdfs:range rdf:resource="http://www.cidoc-crm.org/cidoc-crm/E81_Transformation"/>
	<rdfs:label xml:lang="fr">a résulté de</rdfs:label>
	<rdfs:label xml:lang="de">ergab sich aus</rdfs:label>
	<rdfs:label xml:lang="pt">resultado de</rdfs:label>
	<rdfs:label xml:lang="en">resulted from</rdfs:label>
	<rdfs:label xml:lang="el">προέκυψε από</rdfs:label>
	<rdfs:label xml:lang="ru">был результатом</rdfs:label>
	<rdfs:label xml:lang="zh">起因于</rdfs:label>
</rdf:Description>

<rdf:Description rdf:about="http://www.cidoc-crm.org/cidoc-crm/P124_transformed">
	<rdf:type rdf:resource="http://www.w3.org/2002/07/owl#ObjectProperty"/>
	<rdfs:subPropertyOf rdf:resource="http://www.cidoc-crm.org/cidoc-crm/P93_took_out_of_existence"/>
	<owl:inverseOf rdf:resource="http://www.cidoc-crm.org/cidoc-crm/P124i_was_transformed_by"/>
	<rdfs:domain rdf:resource="http://www.cidoc-crm.org/cidoc-crm/E81_Transformation"/>
	<rdfs:range rdf:resource="http://www.cidoc-crm.org/cidoc-crm/E18_Physical_Thing"/>
	<rdfs:comment xml:lang="en">This property identifies the instance or instances E18 Physical Thing that have ceased to exist due to an instance of E81 Transformation.
The item that has ceased to exist and was replaced by the result of the Transformation. The continuity between both items, the new and the old, is expressed by the links to the common instance of E81 Transformation.</rdfs:comment>
	<rdfs:label xml:lang="fr">a transformé</rdfs:label>
	<rdfs:label xml:lang="en">transformed</rdfs:label>
	<rdfs:label xml:lang="pt">transformou</rdfs:label>
	<rdfs:label xml:lang="de">wandelte um</rdfs:label>
	<rdfs:label xml:lang="el">μετέτρεψε</rdfs:label>
	<rdfs:label xml:lang="ru">трансформировал</rdfs:label>
	<rdfs:label xml:lang="zh">转变了</rdfs:label>
</rdf:Description>

<rdf:Description rdf:about="http://www.cidoc-crm.org/cidoc-crm/P124i_was_transformed_by">
	<rdf:type rdf:resource="http://www.w3.org/2002/07/owl#ObjectProperty"/>
	<rdfs:subPropertyOf rdf:resource="http://www.cidoc-crm.org/cidoc-crm/P93i_was_taken_out_of_existence_by"/>
	<rdfs:domain rdf:resource="http://www.cidoc-crm.org/cidoc-crm/E18_Physical_Thing"/>
	<rdfs:range rdf:resource="http://www.cidoc-crm.org/cidoc-crm/E81_Transformation"/>
	<rdfs:label xml:lang="fr">a été transformé par</rdfs:label>
	<rdfs:label xml:lang="pt">foi transformado por</rdfs:label>
	<rdfs:label xml:lang="en">was transformed by</rdfs:label>
	<rdfs:label xml:lang="de">wurde umgewandelt durch</rdfs:label>
	<rdfs:label xml:lang="el">μετατράπηκε από</rdfs:label>
	<rdfs:label xml:lang="ru">был трансформирован посредством</rdfs:label>
	<rdfs:label xml:lang="zh">被转变</rdfs:label>
</rdf:Description>

<rdf:Description rdf:about="http://www.cidoc-crm.org/cidoc-crm/P125_used_object_of_type">
	<rdf:type rdf:resource="http://www.w3.org/2002/07/owl#ObjectProperty"/>
	<owl:inverseOf rdf:resource="http://www.cidoc-crm.org/cidoc-crm/P125i_was_type_of_object_used_in"/>
	<rdfs:domain rdf:resource="http://www.cidoc-crm.org/cidoc-crm/E7_Activity"/>
	<rdfs:range rdf:resource="http://www.cidoc-crm.org/cidoc-crm/E55_Type"/>
	<rdfs:comment xml:lang="en">This property associates an instance of E7 Activity to an instance of E55 Type, which classifies an instance of E70 Thing used in an instance of E7 Activity, when the specific instance is either unknown or not of interest, such as use of “a hammer”.
This property is a shortcut of the more fully developed path from E7 Activity through P16 used specific object, E70 Thing, P2 has type, to E55 Type.</rdfs:comment>
	<rdfs:label xml:lang="fr">a mobilisé l’objet du type</rdfs:label>
	<rdfs:label xml:lang="de">benutzte Objekt des Typus</rdfs:label>
	<rdfs:label xml:lang="en">used object of type</rdfs:label>
	<rdfs:label xml:lang="pt">usou objeto do tipo</rdfs:label>
	<rdfs:label xml:lang="el">χρησιμοποίησε αντικείμενο τύπου</rdfs:label>
	<rdfs:label xml:lang="ru">использовал объект типа</rdfs:label>
	<rdfs:label xml:lang="zh">使用对象类型</rdfs:label>
</rdf:Description>

<rdf:Description rdf:about="http://www.cidoc-crm.org/cidoc-crm/P125i_was_type_of_object_used_in">
	<rdf:type rdf:resource="http://www.w3.org/2002/07/owl#ObjectProperty"/>
	<rdfs:domain rdf:resource="http://www.cidoc-crm.org/cidoc-crm/E55_Type"/>
	<rdfs:range rdf:resource="http://www.cidoc-crm.org/cidoc-crm/E7_Activity"/>
	<rdfs:label xml:lang="de">Objekt des Typus ... wurde benutzt in</rdfs:label>
	<rdfs:label xml:lang="fr">a été le type d’objet employé pour</rdfs:label>
	<rdfs:label xml:lang="pt">foi tipo do objeto usado em</rdfs:label>
	<rdfs:label xml:lang="en">was type of object used in</rdfs:label>
	<rdfs:label xml:lang="el">ήταν o τύπος αντικείμενου που χρησιμοποιήθηκε σε</rdfs:label>
	<rdfs:label xml:lang="ru">был типом объекта использованного в</rdfs:label>
	<rdfs:label xml:lang="zh">是使用的对象类型</rdfs:label>
</rdf:Description>

<rdf:Description rdf:about="http://www.cidoc-crm.org/cidoc-crm/P126_employed">
	<rdf:type rdf:resource="http://www.w3.org/2002/07/owl#ObjectProperty"/>
	<owl:inverseOf rdf:resource="http://www.cidoc-crm.org/cidoc-crm/P126i_was_employed_in"/>
	<rdfs:domain rdf:resource="http://www.cidoc-crm.org/cidoc-crm/E11_Modification"/>
	<rdfs:range rdf:resource="http://www.cidoc-crm.org/cidoc-crm/E57_Material"/>
	<rdfs:comment xml:lang="en">This property identifies the instance of E57 Material employed in an instance of E11 Modification.
The instance of E57 Material used during the instance of E11 Modification does not necessarily become incorporated into the instance of E24 Physical Human-Made Thing that forms the subject of the instance of E11 Modification.</rdfs:comment>
	<rdfs:label xml:lang="fr">a employé</rdfs:label>
	<rdfs:label xml:lang="en">employed</rdfs:label>
	<rdfs:label xml:lang="pt">empregou</rdfs:label>
	<rdfs:label xml:lang="de">verwendete</rdfs:label>
	<rdfs:label xml:lang="el">χρησιμοποίησε</rdfs:label>
	<rdfs:label xml:lang="ru">использовал</rdfs:label>
	<rdfs:label xml:lang="zh">使用</rdfs:label>
</rdf:Description>

<rdf:Description rdf:about="http://www.cidoc-crm.org/cidoc-crm/P126i_was_employed_in">
	<rdf:type rdf:resource="http://www.w3.org/2002/07/owl#ObjectProperty"/>
	<rdfs:domain rdf:resource="http://www.cidoc-crm.org/cidoc-crm/E57_Material"/>
	<rdfs:range rdf:resource="http://www.cidoc-crm.org/cidoc-crm/E11_Modification"/>
	<rdfs:label xml:lang="fr">a été employé dans</rdfs:label>
	<rdfs:label xml:lang="pt">foi empregado em</rdfs:label>
	<rdfs:label xml:lang="en">was employed in</rdfs:label>
	<rdfs:label xml:lang="de">wurde verwendet bei</rdfs:label>
	<rdfs:label xml:lang="el">χρησιμοποιήθηκε σε</rdfs:label>
	<rdfs:label xml:lang="ru">использовался в</rdfs:label>
	<rdfs:label xml:lang="zh">被用于</rdfs:label>
</rdf:Description>

<rdf:Description rdf:about="http://www.cidoc-crm.org/cidoc-crm/P127_has_broader_term">
	<rdf:type rdf:resource="http://www.w3.org/2002/07/owl#ObjectProperty"/>
	<owl:inverseOf rdf:resource="http://www.cidoc-crm.org/cidoc-crm/P127i_has_narrower_term"/>
	<rdfs:domain rdf:resource="http://www.cidoc-crm.org/cidoc-crm/E55_Type"/>
	<rdfs:range rdf:resource="http://www.cidoc-crm.org/cidoc-crm/E55_Type"/>
	<rdfs:comment xml:lang="en">This property associates an instance of E55 Type with another instance of E55 Type that has a broader meaning.
It allows instances of E55 Types to be organised into hierarchies. This is the sense of “broader term generic (BTG)” as defined in ISO 25964-2:2013 (International Organization for Standardization 2013).
This property is transitive. This property is asymmetric.</rdfs:comment>
	<rdfs:label xml:lang="fr">a pour terme général</rdfs:label>
	<rdfs:label xml:lang="en">has broader term</rdfs:label>
	<rdfs:label xml:lang="de">hat den Oberbegriff</rdfs:label>
	<rdfs:label xml:lang="pt">tem termo genérico</rdfs:label>
	<rdfs:label xml:lang="el">έχει ευρύτερο όρο</rdfs:label>
	<rdfs:label xml:lang="ru">имеет вышестоящий термин</rdfs:label>
	<rdfs:label xml:lang="zh">上位词</rdfs:label>
</rdf:Description>

<rdf:Description rdf:about="http://www.cidoc-crm.org/cidoc-crm/P127i_has_narrower_term">
	<rdf:type rdf:resource="http://www.w3.org/2002/07/owl#ObjectProperty"/>
	<rdfs:domain rdf:resource="http://www.cidoc-crm.org/cidoc-crm/E55_Type"/>
	<rdfs:range rdf:resource="http://www.cidoc-crm.org/cidoc-crm/E55_Type"/>
	<rdfs:label xml:lang="fr">a pour terme spécifique</rdfs:label>
	<rdfs:label xml:lang="en">has narrower term</rdfs:label>
	<rdfs:label xml:lang="de">hat den Unterbegriff</rdfs:label>
	<rdfs:label xml:lang="pt">tem termo específico</rdfs:label>
	<rdfs:label xml:lang="el">έχει στενότερο όρο</rdfs:label>
	<rdfs:label xml:lang="ru">имеет нижестоящий термин</rdfs:label>
	<rdfs:label xml:lang="zh">下位词</rdfs:label>
</rdf:Description>

<rdf:Description rdf:about="http://www.cidoc-crm.org/cidoc-crm/P128_carries">
	<rdf:type rdf:resource="http://www.w3.org/2002/07/owl#ObjectProperty"/>
	<rdfs:subPropertyOf rdf:resource="http://www.cidoc-crm.org/cidoc-crm/P130_shows_features_of"/>
	<owl:inverseOf rdf:resource="http://www.cidoc-crm.org/cidoc-crm/P128i_is_carried_by"/>
	<rdfs:domain rdf:resource="http://www.cidoc-crm.org/cidoc-crm/E18_Physical_Thing"/>
	<rdfs:range rdf:resource="http://www.cidoc-crm.org/cidoc-crm/E90_Symbolic_Object"/>
	<rdfs:comment xml:lang="en">This property identifies an instance E90 Symbolic Object carried by an instance of E18 Physical Thing. Since an instance of E90 Symbolic Object is defined as an immaterial idealization over potentially multiple carriers, any individual realization on a particular physical carrier may be defective, due to deterioration or shortcomings in the process of creating the realization compared to the intended ideal. As long as such defects do not substantially affect the complete recognition of the respective symbolic object, it is still regarded as carrying an instance of this E90 Symbolic Object. If these defects are of scholarly interest, the particular realization can be modelled as an instance of E25 Human-Made Feature. Note, that any instance of E90 Symbolic Object incorporated (P165) in the carried symbolic object is also carried by the same instance of E18 Physical Thing.</rdfs:comment>
	<rdfs:label xml:lang="en">carries</rdfs:label>
	<rdfs:label xml:lang="fr">est le support de</rdfs:label>
	<rdfs:label xml:lang="de">trägt</rdfs:label>
	<rdfs:label xml:lang="pt">é o suporte de</rdfs:label>
	<rdfs:label xml:lang="el">φέρει</rdfs:label>
	<rdfs:label xml:lang="ru">несет</rdfs:label>
	<rdfs:label xml:lang="zh">承载</rdfs:label>
</rdf:Description>

<rdf:Description rdf:about="http://www.cidoc-crm.org/cidoc-crm/P128i_is_carried_by">
	<rdf:type rdf:resource="http://www.w3.org/2002/07/owl#ObjectProperty"/>
	<rdfs:subPropertyOf rdf:resource="http://www.cidoc-crm.org/cidoc-crm/P130i_features_are_also_found_on"/>
	<rdfs:domain rdf:resource="http://www.cidoc-crm.org/cidoc-crm/E90_Symbolic_Object"/>
	<rdfs:range rdf:resource="http://www.cidoc-crm.org/cidoc-crm/E18_Physical_Thing"/>
	<rdfs:label xml:lang="fr">a pour support</rdfs:label>
	<rdfs:label xml:lang="en">is carried by</rdfs:label>
	<rdfs:label xml:lang="de">wird getragen von</rdfs:label>
	<rdfs:label xml:lang="pt">é suportado por</rdfs:label>
	<rdfs:label xml:lang="el">φέρεται από</rdfs:label>
	<rdfs:label xml:lang="ru">переносится посредством</rdfs:label>
	<rdfs:label xml:lang="zh">被承载</rdfs:label>
</rdf:Description>

<rdf:Description rdf:about="http://www.cidoc-crm.org/cidoc-crm/P129_is_about">
	<rdf:type rdf:resource="http://www.w3.org/2002/07/owl#ObjectProperty"/>
	<rdfs:subPropertyOf rdf:resource="http://www.cidoc-crm.org/cidoc-crm/P67_refers_to"/>
	<owl:inverseOf rdf:resource="http://www.cidoc-crm.org/cidoc-crm/P129i_is_subject_of"/>
	<rdfs:domain rdf:resource="http://www.cidoc-crm.org/cidoc-crm/E89_Propositional_Object"/>
	<rdfs:range rdf:resource="http://www.cidoc-crm.org/cidoc-crm/E1_CRM_Entity"/>
	<rdfs:comment xml:lang="en">This property documents that an instance of E89 Propositional Object has as subject an instance of E1 CRM Entity.
This differs from P67 refers to (is referred to by), which refers to an instance of E1 CRM Entity, in that it describes the primary subject or subjects of an instance of E89 Propositional Object.</rdfs:comment>
	<rdfs:label xml:lang="fr">a pour sujet</rdfs:label>
	<rdfs:label xml:lang="de">handelt über</rdfs:label>
	<rdfs:label xml:lang="en">is about</rdfs:label>
	<rdfs:label xml:lang="pt">é sobre</rdfs:label>
	<rdfs:label xml:lang="el">έχει ως θέμα</rdfs:label>
	<rdfs:label xml:lang="ru">касается</rdfs:label>
	<rdfs:label xml:lang="zh">有关</rdfs:label>
</rdf:Description>

<rdf:Description rdf:about="http://www.cidoc-crm.org/cidoc-crm/P129i_is_subject_of">
	<rdf:type rdf:resource="http://www.w3.org/2002/07/owl#ObjectProperty"/>
	<rdfs:subPropertyOf rdf:resource="http://www.cidoc-crm.org/cidoc-crm/P67i_is_referred_to_by"/>
	<rdfs:domain rdf:resource="http://www.cidoc-crm.org/cidoc-crm/E1_CRM_Entity"/>
	<rdfs:range rdf:resource="http://www.cidoc-crm.org/cidoc-crm/E89_Propositional_Object"/>
	<rdfs:label xml:lang="fr">est le sujet de</rdfs:label>
	<rdfs:label xml:lang="en">is subject of</rdfs:label>
	<rdfs:label xml:lang="de">wird behandelt in</rdfs:label>
	<rdfs:label xml:lang="pt">é assunto de</rdfs:label>
	<rdfs:label xml:lang="el">είναι θέμα του/της</rdfs:label>
	<rdfs:label xml:lang="ru">является предметом для</rdfs:label>
	<rdfs:label xml:lang="zh">是主题</rdfs:label>
</rdf:Description>

<rdf:Description rdf:about="http://www.cidoc-crm.org/cidoc-crm/P12_occurred_in_the_presence_of">
	<rdf:type rdf:resource="http://www.w3.org/2002/07/owl#ObjectProperty"/>
	<owl:inverseOf rdf:resource="http://www.cidoc-crm.org/cidoc-crm/P12i_was_present_at"/>
	<rdfs:domain rdf:resource="http://www.cidoc-crm.org/cidoc-crm/E5_Event"/>
	<rdfs:range rdf:resource="http://www.cidoc-crm.org/cidoc-crm/E77_Persistent_Item"/>
	<rdfs:comment xml:lang="en">This property describes the active or passive presence of an E77 Persistent Item in an instance of E5 Event without implying any specific role.
It documents known events in which an instance of E77 Persistent Item was present during the course of its life or history. For example, an object may be the desk, now in a museum, on which a treaty was signed. The instance of E53 Place and the instance of E52 Time-Span where and when these events happened provide constraints about the presence of the related instance E77 Persistent Item in the past. Instances of E90 Symbolic Object, in particular information objects, are physically present in events via at least one of the instances of E18 Physical Thing carrying them. Note, that the human mind can be such a carrier. A precondition for a transfer of information to a person or another new physical carrier is the presence of the respective information object and this person or physical thing in one event.</rdfs:comment>
	<rdfs:label xml:lang="fr">a eu lieu en présence de</rdfs:label>
	<rdfs:label xml:lang="de">fand statt im Beisein von</rdfs:label>
	<rdfs:label xml:lang="en">occurred in the presence of</rdfs:label>
	<rdfs:label xml:lang="pt">ocorreu na presença de</rdfs:label>
	<rdfs:label xml:lang="el">συνέβη παρουσία του/της</rdfs:label>
	<rdfs:label xml:lang="ru">появился в присутствии</rdfs:label>
	<rdfs:label xml:lang="zh">已出现</rdfs:label>
</rdf:Description>

<rdf:Description rdf:about="http://www.cidoc-crm.org/cidoc-crm/P12i_was_present_at">
	<rdf:type rdf:resource="http://www.w3.org/2002/07/owl#ObjectProperty"/>
	<rdfs:domain rdf:resource="http://www.cidoc-crm.org/cidoc-crm/E77_Persistent_Item"/>
	<rdfs:range rdf:resource="http://www.cidoc-crm.org/cidoc-crm/E5_Event"/>
	<rdfs:label xml:lang="fr">a été présent à</rdfs:label>
	<rdfs:label xml:lang="pt">estava presente no</rdfs:label>
	<rdfs:label xml:lang="de">war anwesend bei</rdfs:label>
	<rdfs:label xml:lang="en">was present at</rdfs:label>
	<rdfs:label xml:lang="el">ήταν παρών/παρούσα/παρόν σε</rdfs:label>
	<rdfs:label xml:lang="ru">присутствовал при</rdfs:label>
	<rdfs:label xml:lang="zh">出现在</rdfs:label>
</rdf:Description>

<rdf:Description rdf:about="http://www.cidoc-crm.org/cidoc-crm/P130_shows_features_of">
	<rdf:type rdf:resource="http://www.w3.org/2002/07/owl#ObjectProperty"/>
	<owl:inverseOf rdf:resource="http://www.cidoc-crm.org/cidoc-crm/P130i_features_are_also_found_on"/>
	<rdfs:domain rdf:resource="http://www.cidoc-crm.org/cidoc-crm/E70_Thing"/>
	<rdfs:range rdf:resource="http://www.cidoc-crm.org/cidoc-crm/E70_Thing"/>
	<rdfs:comment xml:lang="en">This property generalises the notions of “copy of” and “similar to” into a directed relationship, where the domain expresses the derivative or influenced item and the range the source or influencing item, if such a direction can be established. The property can also be used to express similarity in cases that can be stated between two objects only, without historical knowledge about its reasons. The property expresses a symmetric relationship in case no direction of influence can be established either from evidence on the item itself or from historical knowledge. This holds in particular for siblings of a derivation process from a common source or non-causal cultural parallels, such as some weaving patterns.
The P130.1 kind of similarity property of the P130 shows features of (features are also found on) property enables the relationship between the domain and the range to be further clarified, in the sense from domain to range, if applicable. For example, it may be expressed if both items are product “of the same mould”, or if two texts “contain identical paragraphs”.
If the reason for similarity is a sort of derivation process, i.e. that the creator has used or had in mind the form of a particular thing during the creation or production, this process should be explicitly modelled. In these cases, P130 shows features of can be regarded as a shortcut of such a process. However, the current model does not contain any path specific enough to infer this property. Specializations of the CIDOC CRM may however be more explicit, for instance describing the use of moulds etc.
This property is not transitive. This property is irreflexive.</rdfs:comment>
	<rdfs:label xml:lang="pt">apresenta características de</rdfs:label>
	<rdfs:label xml:lang="fr">présente les caractéristiques de</rdfs:label>
	<rdfs:label xml:lang="en">shows features of</rdfs:label>
	<rdfs:label xml:lang="de">zeigt Merkmale von</rdfs:label>
	<rdfs:label xml:lang="el">παρουσιάζει χαρακτηριστικά του/της</rdfs:label>
	<rdfs:label xml:lang="ru">демонстрирует признаки</rdfs:label>
	<rdfs:label xml:lang="zh">显示特征</rdfs:label>
</rdf:Description>

<rdf:Description rdf:about="http://www.cidoc-crm.org/cidoc-crm/P130i_features_are_also_found_on">
	<rdf:type rdf:resource="http://www.w3.org/2002/07/owl#ObjectProperty"/>
	<rdfs:domain rdf:resource="http://www.cidoc-crm.org/cidoc-crm/E70_Thing"/>
	<rdfs:range rdf:resource="http://www.cidoc-crm.org/cidoc-crm/E70_Thing"/>
	<rdfs:label xml:lang="de">Merkmale auch auf</rdfs:label>
	<rdfs:label xml:lang="fr">a les caractéristiques aussi présentes sur</rdfs:label>
	<rdfs:label xml:lang="pt">características são também encontradas em</rdfs:label>
	<rdfs:label xml:lang="en">features are also found on</rdfs:label>
	<rdfs:label xml:lang="el">χαρακτηριστικά του βρίσκονται επίσης σε</rdfs:label>
	<rdfs:label xml:lang="ru">признаки также найдены на</rdfs:label>
	<rdfs:label xml:lang="zh">发现特征</rdfs:label>
</rdf:Description>

<rdf:Description rdf:about="http://www.cidoc-crm.org/cidoc-crm/P132_spatiotemporally_overlaps_with">
	<rdf:type rdf:resource="http://www.w3.org/2002/07/owl#ObjectProperty"/>
	<rdfs:domain rdf:resource="http://www.cidoc-crm.org/cidoc-crm/E92_Spacetime_Volume"/>
	<rdfs:range rdf:resource="http://www.cidoc-crm.org/cidoc-crm/E92_Spacetime_Volume"/>
	<rdfs:comment xml:lang="en">This symmetric property associates two instances of E92 Spacetime Volume that have some of their extents in common. If only the fuzzy boundaries of the instances of E92 Spacetime Volume overlap, this property cannot be determined from observation alone and therefore should not be applied. However, there may be other forms of justification that the two instances of E92 Spacetime Volume must have some of their extents in common regardless of where and when precisely.
If this property holds for two instances of E92 Spacetime Volume then it cannot be the case that P133 is spatiotemporally separated from also holds for the same two instances. Furthermore, there are cases where neither P132 spatiotemporally overlaps with nor P133 is spatiotemporally separated from holds between two instances of E92 Spacetime Volume. This would occur where only an overlap of the fuzzy boundaries of the two instances of E92 Spacetime Volume occurs and no other evidence is available.
This property is not transitive. This property is symmetric. This property is reflexive.</rdfs:comment>
	<rdfs:label xml:lang="fr">recoupe spatio-temporellement</rdfs:label>
	<rdfs:label xml:lang="en">spatiotemporally overlaps with</rdfs:label>
</rdf:Description>

<rdf:Description rdf:about="http://www.cidoc-crm.org/cidoc-crm/P133_is_spatiotemporally_separated_from">
	<rdf:type rdf:resource="http://www.w3.org/2002/07/owl#ObjectProperty"/>
	<rdfs:domain rdf:resource="http://www.cidoc-crm.org/cidoc-crm/E92_Spacetime_Volume"/>
	<rdfs:range rdf:resource="http://www.cidoc-crm.org/cidoc-crm/E92_Spacetime_Volume"/>
	<rdfs:comment xml:lang="en">This symmetric property associates two instances of E92 Spacetime Volume that have no extents in common. If only the fuzzy boundaries of the instances of E92 Spacetime Volume overlap, this property cannot be determined from observation alone and therefore should not be applied. However, there may be other forms of justification that the two instances of E92 Spacetime Volume must not have any of their extents in common regardless of where and when precisely.
If this property holds for two instances of E92 Spacetime Volume then it cannot be the case that P132 spatiotemporally overlaps with also holds for the same two instances. Furthermore, there are cases where neither P132 spatiotemporally overlaps with nor P133 is spatiotemporally separated from holds between two instances of E92 Spacetime Volume. This would occur where only an overlap of the fuzzy boundaries of the two instances of E92 Spacetime Volume occurs and no other evidence is available.
This property is not transitive. This property is symmetric. This property is irreflexive.</rdfs:comment>
	<rdfs:label xml:lang="fr">est distinct spatio-temporellement de</rdfs:label>
	<rdfs:label xml:lang="en">is spatiotemporally separated from</rdfs:label>
</rdf:Description>

<rdf:Description rdf:about="http://www.cidoc-crm.org/cidoc-crm/P134_continued">
	<rdf:type rdf:resource="http://www.w3.org/2002/07/owl#ObjectProperty"/>
	<rdfs:subPropertyOf rdf:resource="http://www.cidoc-crm.org/cidoc-crm/P15_was_influenced_by"/>
	<rdfs:subPropertyOf rdf:resource="http://www.cidoc-crm.org/cidoc-crm/P176i_starts_after_the_start_of"/>
	<owl:inverseOf rdf:resource="http://www.cidoc-crm.org/cidoc-crm/P134i_was_continued_by"/>
	<rdfs:domain rdf:resource="http://www.cidoc-crm.org/cidoc-crm/E7_Activity"/>
	<rdfs:range rdf:resource="http://www.cidoc-crm.org/cidoc-crm/E7_Activity"/>
	<rdfs:comment xml:lang="en">This property associates two instances of E7 Activity, where the domain is considered as an intentional continuation of the range. A continuation of an activity may happen when the continued activity is still ongoing or after the continued activity has completely ended. The continuing activity may have started already before it decided to continue the other one. Continuation implies a coherence of intentions and outcomes of the involved activities.
This property is not transitive. This property is asymmetric.</rdfs:comment>
	<rdfs:label xml:lang="fr">a continué</rdfs:label>
	<rdfs:label xml:lang="en">continued</rdfs:label>
	<rdfs:label xml:lang="pt">continuou</rdfs:label>
	<rdfs:label xml:lang="de">setzte sich fort in</rdfs:label>
	<rdfs:label xml:lang="el">συνέχισε</rdfs:label>
	<rdfs:label xml:lang="ru">продолжил</rdfs:label>
	<rdfs:label xml:lang="zh">继续</rdfs:label>
</rdf:Description>

<rdf:Description rdf:about="http://www.cidoc-crm.org/cidoc-crm/P134i_was_continued_by">
	<rdf:type rdf:resource="http://www.w3.org/2002/07/owl#ObjectProperty"/>
	<rdfs:subPropertyOf rdf:resource="http://www.cidoc-crm.org/cidoc-crm/P15i_influenced"/>
	<rdfs:subPropertyOf rdf:resource="http://www.cidoc-crm.org/cidoc-crm/P176_starts_before_the_start_of"/>
	<rdfs:domain rdf:resource="http://www.cidoc-crm.org/cidoc-crm/E7_Activity"/>
	<rdfs:range rdf:resource="http://www.cidoc-crm.org/cidoc-crm/E7_Activity"/>
	<rdfs:label xml:lang="fr">a été continué par</rdfs:label>
	<rdfs:label xml:lang="pt">foi continuada por</rdfs:label>
	<rdfs:label xml:lang="en">was continued by</rdfs:label>
	<rdfs:label xml:lang="de">wurde fortgesetzt durch</rdfs:label>
	<rdfs:label xml:lang="el">συνεχίστηκε από</rdfs:label>
	<rdfs:label xml:lang="ru">был продолжен</rdfs:label>
	<rdfs:label xml:lang="zh">被继续</rdfs:label>
</rdf:Description>

<rdf:Description rdf:about="http://www.cidoc-crm.org/cidoc-crm/P135_created_type">
	<rdf:type rdf:resource="http://www.w3.org/2002/07/owl#ObjectProperty"/>
	<rdfs:subPropertyOf rdf:resource="http://www.cidoc-crm.org/cidoc-crm/P94_has_created"/>
	<owl:inverseOf rdf:resource="http://www.cidoc-crm.org/cidoc-crm/P135i_was_created_by"/>
	<rdfs:domain rdf:resource="http://www.cidoc-crm.org/cidoc-crm/E83_Type_Creation"/>
	<rdfs:range rdf:resource="http://www.cidoc-crm.org/cidoc-crm/E55_Type"/>
	<rdfs:comment xml:lang="en">This property identifies the instance of E55 Type, which is created in an instance of E83 Type Creation activity.</rdfs:comment>
	<rdfs:label xml:lang="fr">a créé le type</rdfs:label>
	<rdfs:label xml:lang="en">created type</rdfs:label>
	<rdfs:label xml:lang="pt">criou tipo</rdfs:label>
	<rdfs:label xml:lang="de">erschuf Typus</rdfs:label>
	<rdfs:label xml:lang="el">δημιούργησε τύπο</rdfs:label>
	<rdfs:label xml:lang="ru">создал тип</rdfs:label>
	<rdfs:label xml:lang="zh">创建类型</rdfs:label>
</rdf:Description>

<rdf:Description rdf:about="http://www.cidoc-crm.org/cidoc-crm/P135i_was_created_by">
	<rdf:type rdf:resource="http://www.w3.org/2002/07/owl#ObjectProperty"/>
	<rdfs:subPropertyOf rdf:resource="http://www.cidoc-crm.org/cidoc-crm/P94i_was_created_by"/>
	<rdfs:domain rdf:resource="http://www.cidoc-crm.org/cidoc-crm/E55_Type"/>
	<rdfs:range rdf:resource="http://www.cidoc-crm.org/cidoc-crm/E83_Type_Creation"/>
	<rdfs:label xml:lang="fr">a été créé par</rdfs:label>
	<rdfs:label xml:lang="pt">foi criado por</rdfs:label>
	<rdfs:label xml:lang="en">was created by</rdfs:label>
	<rdfs:label xml:lang="de">wurde geschaffen durch</rdfs:label>
	<rdfs:label xml:lang="el">δημιουργήθηκε από</rdfs:label>
	<rdfs:label xml:lang="ru">был создан посредством</rdfs:label>
	<rdfs:label xml:lang="zh">被创建</rdfs:label>
</rdf:Description>

<rdf:Description rdf:about="http://www.cidoc-crm.org/cidoc-crm/P136_was_based_on">
	<rdf:type rdf:resource="http://www.w3.org/2002/07/owl#ObjectProperty"/>
	<rdfs:subPropertyOf rdf:resource="http://www.cidoc-crm.org/cidoc-crm/P15_was_influenced_by"/>
	<owl:inverseOf rdf:resource="http://www.cidoc-crm.org/cidoc-crm/P136i_supported_type_creation"/>
	<rdfs:domain rdf:resource="http://www.cidoc-crm.org/cidoc-crm/E83_Type_Creation"/>
	<rdfs:range rdf:resource="http://www.cidoc-crm.org/cidoc-crm/E1_CRM_Entity"/>
	<rdfs:comment xml:lang="en">This property identifies one or more instances of E1 CRM Entity that were used as evidence to declare a new instance of E55 Type.
The examination of these items is often the only objective way to understand the precise characteristics of a new type. Such items should be deposited in a museum or similar institution for that reason. The taxonomic role renders the specific relationship of each item to the type, such as “holotype” or “original element”.</rdfs:comment>
	<rdfs:label xml:lang="fr">a été fondé sur</rdfs:label>
	<rdfs:label xml:lang="pt">foi baseado em</rdfs:label>
	<rdfs:label xml:lang="de">stützte sich auf</rdfs:label>
	<rdfs:label xml:lang="en">was based on</rdfs:label>
	<rdfs:label xml:lang="el">βασίστηκε σε</rdfs:label>
	<rdfs:label xml:lang="ru">был основан на</rdfs:label>
	<rdfs:label xml:lang="zh">基于</rdfs:label>
</rdf:Description>

<rdf:Description rdf:about="http://www.cidoc-crm.org/cidoc-crm/P136i_supported_type_creation">
	<rdf:type rdf:resource="http://www.w3.org/2002/07/owl#ObjectProperty"/>
	<rdfs:subPropertyOf rdf:resource="http://www.cidoc-crm.org/cidoc-crm/P15i_influenced"/>
	<rdfs:domain rdf:resource="http://www.cidoc-crm.org/cidoc-crm/E1_CRM_Entity"/>
	<rdfs:range rdf:resource="http://www.cidoc-crm.org/cidoc-crm/E83_Type_Creation"/>
	<rdfs:label xml:lang="fr">a fondé la création du type</rdfs:label>
	<rdfs:label xml:lang="de">belegte</rdfs:label>
	<rdfs:label xml:lang="pt">suportou a criação de tipo</rdfs:label>
	<rdfs:label xml:lang="en">supported type creation</rdfs:label>
	<rdfs:label xml:lang="el">υποστήριξε τη δημιουργία τύπου</rdfs:label>
	<rdfs:label xml:lang="ru">поддержал создание типа</rdfs:label>
	<rdfs:label xml:lang="zh">支持类型创建</rdfs:label>
</rdf:Description>

<rdf:Description rdf:about="http://www.cidoc-crm.org/cidoc-crm/P137_exemplifies">
	<rdf:type rdf:resource="http://www.w3.org/2002/07/owl#ObjectProperty"/>
	<rdfs:subPropertyOf rdf:resource="http://www.cidoc-crm.org/cidoc-crm/P2_has_type"/>
	<owl:inverseOf rdf:resource="http://www.cidoc-crm.org/cidoc-crm/P137i_is_exemplified_by"/>
	<rdfs:domain rdf:resource="http://www.cidoc-crm.org/cidoc-crm/E1_CRM_Entity"/>
	<rdfs:range rdf:resource="http://www.cidoc-crm.org/cidoc-crm/E55_Type"/>
	<rdfs:comment xml:lang="en">This property associates an instance of E1 CRM Entity with an instance of E55 Type for which it has been declared to be a particularly characteristic example.
The P137.1 in the taxonomic role property of P137 exemplifies (is exemplified by) allows differentiation of taxonomic roles. The taxonomic role renders the specific relationship of this example to the type, such as “prototypical”, “archetypical”, “lectotype”, etc. The taxonomic role “lectotype” is not associated with the instance of E83 Type Creation itself but is selected in a later phase.</rdfs:comment>
	<rdfs:label xml:lang="de">erläutert</rdfs:label>
	<rdfs:label xml:lang="fr">exemplifie</rdfs:label>
	<rdfs:label xml:lang="en">exemplifies</rdfs:label>
	<rdfs:label xml:lang="pt">é exemplificado por</rdfs:label>
	<rdfs:label xml:lang="el">δειγματίζει</rdfs:label>
	<rdfs:label xml:lang="ru">поясняет</rdfs:label>
	<rdfs:label xml:lang="zh">例示</rdfs:label>
</rdf:Description>

<rdf:Description rdf:about="http://www.cidoc-crm.org/cidoc-crm/P137i_is_exemplified_by">
	<rdf:type rdf:resource="http://www.w3.org/2002/07/owl#ObjectProperty"/>
	<rdfs:subPropertyOf rdf:resource="http://www.cidoc-crm.org/cidoc-crm/P2i_is_type_of"/>
	<rdfs:domain rdf:resource="http://www.cidoc-crm.org/cidoc-crm/E55_Type"/>
	<rdfs:range rdf:resource="http://www.cidoc-crm.org/cidoc-crm/E1_CRM_Entity"/>
	<rdfs:label xml:lang="de">erläutert durch Beispiel</rdfs:label>
	<rdfs:label xml:lang="fr">est exemplifié par</rdfs:label>
	<rdfs:label xml:lang="pt">exemplifica</rdfs:label>
	<rdfs:label xml:lang="en">is exemplified by</rdfs:label>
	<rdfs:label xml:lang="el">δειγματίζεται από</rdfs:label>
	<rdfs:label xml:lang="ru">поясняется посредством</rdfs:label>
	<rdfs:label xml:lang="zh">被例示</rdfs:label>
</rdf:Description>

<rdf:Description rdf:about="http://www.cidoc-crm.org/cidoc-crm/P138_represents">
	<rdf:type rdf:resource="http://www.w3.org/2002/07/owl#ObjectProperty"/>
	<rdfs:subPropertyOf rdf:resource="http://www.cidoc-crm.org/cidoc-crm/P67_refers_to"/>
	<owl:inverseOf rdf:resource="http://www.cidoc-crm.org/cidoc-crm/P138i_has_representation"/>
	<rdfs:domain rdf:resource="http://www.cidoc-crm.org/cidoc-crm/E36_Visual_Item"/>
	<rdfs:range rdf:resource="http://www.cidoc-crm.org/cidoc-crm/E1_CRM_Entity"/>
	<rdfs:comment xml:lang="en">This property establishes the relationship between an instance of E36 Visual Item and the instance of E1 CRM Entity that it visually represents.
Any entity may be represented visually. This property is part of the fully developed path from E24 Physical Human-Made Thing through P65 shows visual item (is shown by), E36 Visual Item, P138 represents (has representation) to E1 CRM Entity, which is shortcut by P62 depicts (is depicted by). P138.1 mode of representation allows the nature of the representation to be refined.
This property is also used for the relationship between an original and a digitisation of the original by the use of techniques such as digital photography, flatbed or infrared scanning. Digitisation is here seen as a process with a mechanical, causal component rendering the spatial distribution of structural and optical properties of the original and does not necessarily include any visual similarity identifiable by human observation.</rdfs:comment>
	<rdfs:label xml:lang="pt">representa</rdfs:label>
	<rdfs:label xml:lang="en">represents</rdfs:label>
	<rdfs:label xml:lang="fr">représente</rdfs:label>
	<rdfs:label xml:lang="de">stellt dar</rdfs:label>
	<rdfs:label xml:lang="el">παριστάνει</rdfs:label>
	<rdfs:label xml:lang="ru">представляет</rdfs:label>
	<rdfs:label xml:lang="zh">描绘</rdfs:label>
</rdf:Description>

<rdf:Description rdf:about="http://www.cidoc-crm.org/cidoc-crm/P138i_has_representation">
	<rdf:type rdf:resource="http://www.w3.org/2002/07/owl#ObjectProperty"/>
	<rdfs:subPropertyOf rdf:resource="http://www.cidoc-crm.org/cidoc-crm/P67i_is_referred_to_by"/>
	<rdfs:domain rdf:resource="http://www.cidoc-crm.org/cidoc-crm/E1_CRM_Entity"/>
	<rdfs:range rdf:resource="http://www.cidoc-crm.org/cidoc-crm/E36_Visual_Item"/>
	<rdfs:label xml:lang="fr">est représenté par</rdfs:label>
	<rdfs:label xml:lang="en">has representation</rdfs:label>
	<rdfs:label xml:lang="pt">tem representação</rdfs:label>
	<rdfs:label xml:lang="de">wird dargestellt durch</rdfs:label>
	<rdfs:label xml:lang="el">παριστάνεται από</rdfs:label>
	<rdfs:label xml:lang="ru">имеет представление</rdfs:label>
	<rdfs:label xml:lang="zh">有描绘</rdfs:label>
</rdf:Description>

<rdf:Description rdf:about="http://www.cidoc-crm.org/cidoc-crm/P139_has_alternative_form">
	<rdf:type rdf:resource="http://www.w3.org/2002/07/owl#ObjectProperty"/>
	<owl:inverseOf rdf:resource="http://www.cidoc-crm.org/cidoc-crm/P139i_is_alternative_form_of"/>
	<rdfs:domain rdf:resource="http://www.cidoc-crm.org/cidoc-crm/E41_Appellation"/>
	<rdfs:range rdf:resource="http://www.cidoc-crm.org/cidoc-crm/E41_Appellation"/>
	<rdfs:comment xml:lang="en">This property associates an instance of E41 Appellation with another instance of E41 Appellation that constitutes a derivative or variant of the former and that may also be used for identifying items identified by the former, in suitable contexts, independent from the particular item to be identified. This property should not be confused with additional variants of names used characteristically for a single, particular item, such as individual nicknames. It is a directed relationship, where the range expresses the derivative or variant and the domain the source of derivation or original form of variation, if such a direction can be established. Otherwise, the relationship is symmetric.
Multiple names assigned to an object, which do not apply to all things identified with the specific instance of E41 Appellation, should be modelled as repeated values of P1 is identified by (identifies) of this object.
P139.1 has type allows the type of derivation to be refined, for instance “transliteration from Latin 1 to ASCII”.</rdfs:comment>
	<rdfs:label xml:lang="fr">a pour forme alternative</rdfs:label>
	<rdfs:label xml:lang="en">has alternative form</rdfs:label>
	<rdfs:label xml:lang="de">hat alternative Form</rdfs:label>
	<rdfs:label xml:lang="pt">tem forma alternativa</rdfs:label>
	<rdfs:label xml:lang="el">έχει εναλλακτική μορφή</rdfs:label>
	<rdfs:label xml:lang="ru">имеет альтернативную форму</rdfs:label>
	<rdfs:label xml:lang="zh">有交替形式</rdfs:label>
</rdf:Description>

<rdf:Description rdf:about="http://www.cidoc-crm.org/cidoc-crm/P139i_is_alternative_form_of">
	<rdf:type rdf:resource="http://www.w3.org/2002/07/owl#ObjectProperty"/>
	<rdfs:domain rdf:resource="http://www.cidoc-crm.org/cidoc-crm/E41_Appellation"/>
	<rdfs:range rdf:resource="http://www.cidoc-crm.org/cidoc-crm/E41_Appellation"/>
	<rdfs:label xml:lang="fr">est la forme alternative de</rdfs:label>
	<rdfs:label xml:lang="en">is alternative form of</rdfs:label>
</rdf:Description>

<rdf:Description rdf:about="http://www.cidoc-crm.org/cidoc-crm/P13_destroyed">
	<rdf:type rdf:resource="http://www.w3.org/2002/07/owl#ObjectProperty"/>
	<rdfs:subPropertyOf rdf:resource="http://www.cidoc-crm.org/cidoc-crm/P93_took_out_of_existence"/>
	<owl:inverseOf rdf:resource="http://www.cidoc-crm.org/cidoc-crm/P13i_was_destroyed_by"/>
	<rdfs:domain rdf:resource="http://www.cidoc-crm.org/cidoc-crm/E6_Destruction"/>
	<rdfs:range rdf:resource="http://www.cidoc-crm.org/cidoc-crm/E18_Physical_Thing"/>
	<rdfs:comment xml:lang="en">This property links an instance of E6 Destruction to an instance of E18 Physical Thing that has been destroyed by it.
Destruction implies the end of an item’s life as a subject of cultural documentation – the physical matter of which the item was composed may in fact continue to exist. An instance of E6 Destruction may be contiguous with an instance of E12 Production that brings into existence a derived object composed partly of matter from the destroyed object.</rdfs:comment>
	<rdfs:label xml:lang="fr">a détruit</rdfs:label>
	<rdfs:label xml:lang="en">destroyed</rdfs:label>
	<rdfs:label xml:lang="pt">destruiu</rdfs:label>
	<rdfs:label xml:lang="de">zerstörte</rdfs:label>
	<rdfs:label xml:lang="el">κατέστρεψε</rdfs:label>
	<rdfs:label xml:lang="ru">уничтожил</rdfs:label>
	<rdfs:label xml:lang="zh">破坏了</rdfs:label>
</rdf:Description>

<rdf:Description rdf:about="http://www.cidoc-crm.org/cidoc-crm/P13i_was_destroyed_by">
	<rdf:type rdf:resource="http://www.w3.org/2002/07/owl#ObjectProperty"/>
	<rdfs:subPropertyOf rdf:resource="http://www.cidoc-crm.org/cidoc-crm/P93i_was_taken_out_of_existence_by"/>
	<rdfs:domain rdf:resource="http://www.cidoc-crm.org/cidoc-crm/E18_Physical_Thing"/>
	<rdfs:range rdf:resource="http://www.cidoc-crm.org/cidoc-crm/E6_Destruction"/>
	<rdfs:label xml:lang="fr">a été détruit par</rdfs:label>
	<rdfs:label xml:lang="pt">foi destruído por</rdfs:label>
	<rdfs:label xml:lang="en">was destroyed by</rdfs:label>
	<rdfs:label xml:lang="de">wurde zerstört durch</rdfs:label>
	<rdfs:label xml:lang="el">καταστράφηκε από</rdfs:label>
	<rdfs:label xml:lang="ru">был уничтожен посредством</rdfs:label>
	<rdfs:label xml:lang="zh">被破坏</rdfs:label>
</rdf:Description>

<rdf:Description rdf:about="http://www.cidoc-crm.org/cidoc-crm/P140_assigned_attribute_to">
	<rdf:type rdf:resource="http://www.w3.org/2002/07/owl#ObjectProperty"/>
	<owl:inverseOf rdf:resource="http://www.cidoc-crm.org/cidoc-crm/P140i_was_attributed_by"/>
	<rdfs:domain rdf:resource="http://www.cidoc-crm.org/cidoc-crm/E13_Attribute_Assignment"/>
	<rdfs:range rdf:resource="http://www.cidoc-crm.org/cidoc-crm/E1_CRM_Entity"/>
	<rdfs:comment xml:lang="en">This property associates an instance of E13 Attribute Assignment with the instance of E1 CRM Entity about which it made an attribution. The instance of E1 CRM Entity plays the role of the domain of the attribution.
The kind of attribution made should be documented using P177 assigned property of type (is type of property assigned).</rdfs:comment>
	<rdfs:label xml:lang="fr">a assigné l’attribut à</rdfs:label>
	<rdfs:label xml:lang="en">assigned attribute to</rdfs:label>
	<rdfs:label xml:lang="pt">atribuiu atributo para</rdfs:label>
	<rdfs:label xml:lang="de">wies Merkmal zu</rdfs:label>
	<rdfs:label xml:lang="el">απέδωσε ιδιότητα σε</rdfs:label>
	<rdfs:label xml:lang="ru">присвоил атрибут для</rdfs:label>
	<rdfs:label xml:lang="zh">分配属性于</rdfs:label>
</rdf:Description>

<rdf:Description rdf:about="http://www.cidoc-crm.org/cidoc-crm/P140i_was_attributed_by">
	<rdf:type rdf:resource="http://www.w3.org/2002/07/owl#ObjectProperty"/>
	<rdfs:domain rdf:resource="http://www.cidoc-crm.org/cidoc-crm/E1_CRM_Entity"/>
	<rdfs:range rdf:resource="http://www.cidoc-crm.org/cidoc-crm/E13_Attribute_Assignment"/>
	<rdfs:label xml:lang="fr">a reçu l’attribut par</rdfs:label>
	<rdfs:label xml:lang="de">bekam Merkmal zugewiesen durch</rdfs:label>
	<rdfs:label xml:lang="pt">foi atribuído por</rdfs:label>
	<rdfs:label xml:lang="en">was attributed by</rdfs:label>
	<rdfs:label xml:lang="el">χαρακτηρίστηκε από</rdfs:label>
	<rdfs:label xml:lang="ru">получил атрибут посредством</rdfs:label>
	<rdfs:label xml:lang="zh">接受属性</rdfs:label>
</rdf:Description>

<rdf:Description rdf:about="http://www.cidoc-crm.org/cidoc-crm/P141_assigned">
	<rdf:type rdf:resource="http://www.w3.org/2002/07/owl#ObjectProperty"/>
	<owl:inverseOf rdf:resource="http://www.cidoc-crm.org/cidoc-crm/P141i_was_assigned_by"/>
	<rdfs:domain rdf:resource="http://www.cidoc-crm.org/cidoc-crm/E13_Attribute_Assignment"/>
	<rdfs:range rdf:resource="http://www.cidoc-crm.org/cidoc-crm/E1_CRM_Entity"/>
	<rdfs:comment xml:lang="en">This property associates an instance of E13 Attribute Assignment with the instance of E1 CRM Entity used in the attribution. The instance of E1 CRM Entity here plays the role of the range of the attribution.
The kind of attribution made should be documented using P177 assigned property of type (is type of property assigned).</rdfs:comment>
	<rdfs:label xml:lang="fr">a attribué</rdfs:label>
	<rdfs:label xml:lang="en">assigned</rdfs:label>
	<rdfs:label xml:lang="pt">atribuiu</rdfs:label>
	<rdfs:label xml:lang="de">wies zu</rdfs:label>
	<rdfs:label xml:lang="el">απέδωσε</rdfs:label>
	<rdfs:label xml:lang="ru">присвоил</rdfs:label>
	<rdfs:label xml:lang="zh">分配</rdfs:label>
</rdf:Description>

<rdf:Description rdf:about="http://www.cidoc-crm.org/cidoc-crm/P141i_was_assigned_by">
	<rdf:type rdf:resource="http://www.w3.org/2002/07/owl#ObjectProperty"/>
	<rdfs:domain rdf:resource="http://www.cidoc-crm.org/cidoc-crm/E1_CRM_Entity"/>
	<rdfs:range rdf:resource="http://www.cidoc-crm.org/cidoc-crm/E13_Attribute_Assignment"/>
	<rdfs:label xml:lang="fr">a été attribué par</rdfs:label>
	<rdfs:label xml:lang="pt">foi atribuído por</rdfs:label>
	<rdfs:label xml:lang="en">was assigned by</rdfs:label>
	<rdfs:label xml:lang="de">wurde zugewiesen durch</rdfs:label>
	<rdfs:label xml:lang="el">αποδόθηκε από</rdfs:label>
	<rdfs:label xml:lang="ru">был присвоен посредством</rdfs:label>
	<rdfs:label xml:lang="zh">被分配</rdfs:label>
</rdf:Description>

<rdf:Description rdf:about="http://www.cidoc-crm.org/cidoc-crm/P142_used_constituent">
	<rdf:type rdf:resource="http://www.w3.org/2002/07/owl#ObjectProperty"/>
	<rdfs:subPropertyOf rdf:resource="http://www.cidoc-crm.org/cidoc-crm/P16_used_specific_object"/>
	<owl:inverseOf rdf:resource="http://www.cidoc-crm.org/cidoc-crm/P142i_was_used_in"/>
	<rdfs:domain rdf:resource="http://www.cidoc-crm.org/cidoc-crm/E15_Identifier_Assignment"/>
	<rdfs:range rdf:resource="http://www.cidoc-crm.org/cidoc-crm/E90_Symbolic_Object"/>
	<rdfs:comment xml:lang="en">This property associates an instance of E15 Identifier Assignment with the instance of E90 Symbolic Object used as constituent of an instance of E42 Identifier in this act of assignment.</rdfs:comment>
	<rdfs:label xml:lang="fr">a mobilisé comme élément</rdfs:label>
	<rdfs:label xml:lang="de">benutzte Bestandteil</rdfs:label>
	<rdfs:label xml:lang="en">used constituent</rdfs:label>
	<rdfs:label xml:lang="zh">使用构成成分</rdfs:label>
</rdf:Description>

<rdf:Description rdf:about="http://www.cidoc-crm.org/cidoc-crm/P142i_was_used_in">
	<rdf:type rdf:resource="http://www.w3.org/2002/07/owl#ObjectProperty"/>
	<rdfs:subPropertyOf rdf:resource="http://www.cidoc-crm.org/cidoc-crm/P16i_was_used_for"/>
	<rdfs:domain rdf:resource="http://www.cidoc-crm.org/cidoc-crm/E90_Symbolic_Object"/>
	<rdfs:range rdf:resource="http://www.cidoc-crm.org/cidoc-crm/E15_Identifier_Assignment"/>
	<rdfs:label xml:lang="fr">a été mobilisé dans</rdfs:label>
	<rdfs:label xml:lang="en">was used in</rdfs:label>
	<rdfs:label xml:lang="de">wurde benutzt in</rdfs:label>
	<rdfs:label xml:lang="zh">用于</rdfs:label>
</rdf:Description>

<rdf:Description rdf:about="http://www.cidoc-crm.org/cidoc-crm/P143_joined">
	<rdf:type rdf:resource="http://www.w3.org/2002/07/owl#ObjectProperty"/>
	<rdfs:subPropertyOf rdf:resource="http://www.cidoc-crm.org/cidoc-crm/P11_had_participant"/>
	<owl:inverseOf rdf:resource="http://www.cidoc-crm.org/cidoc-crm/P143i_was_joined_by"/>
	<rdfs:domain rdf:resource="http://www.cidoc-crm.org/cidoc-crm/E85_Joining"/>
	<rdfs:range rdf:resource="http://www.cidoc-crm.org/cidoc-crm/E39_Actor"/>
	<rdfs:comment xml:lang="en">This property identifies the instance of E39 Actor that becomes member of an instance of E74 Group in an instance of E85 Joining.
Joining events allow for describing actors becoming members of a group with the more detailed path E74 Group, P144i gained member by, E85 Joining, P143 joined, E39 Actor, compared to the shortcut offered by P107 has current or former member (is current or former member of).</rdfs:comment>
	<rdfs:label xml:lang="fr">a fait adhérer</rdfs:label>
	<rdfs:label xml:lang="en">joined</rdfs:label>
	<rdfs:label xml:lang="de">verband</rdfs:label>
	<rdfs:label xml:lang="zh">加入</rdfs:label>
</rdf:Description>

<rdf:Description rdf:about="http://www.cidoc-crm.org/cidoc-crm/P143i_was_joined_by">
	<rdf:type rdf:resource="http://www.w3.org/2002/07/owl#ObjectProperty"/>
	<rdfs:subPropertyOf rdf:resource="http://www.cidoc-crm.org/cidoc-crm/P11i_participated_in"/>
	<rdfs:domain rdf:resource="http://www.cidoc-crm.org/cidoc-crm/E39_Actor"/>
	<rdfs:range rdf:resource="http://www.cidoc-crm.org/cidoc-crm/E85_Joining"/>
	<rdfs:label xml:lang="fr">a adhéré par</rdfs:label>
	<rdfs:label xml:lang="en">was joined by</rdfs:label>
	<rdfs:label xml:lang="de">wurde verbunden durch</rdfs:label>
	<rdfs:label xml:lang="zh">被加入</rdfs:label>
</rdf:Description>

<rdf:Description rdf:about="http://www.cidoc-crm.org/cidoc-crm/P144_joined_with">
	<rdf:type rdf:resource="http://www.w3.org/2002/07/owl#ObjectProperty"/>
	<rdfs:subPropertyOf rdf:resource="http://www.cidoc-crm.org/cidoc-crm/P11_had_participant"/>
	<owl:inverseOf rdf:resource="http://www.cidoc-crm.org/cidoc-crm/P144i_gained_member_by"/>
	<rdfs:domain rdf:resource="http://www.cidoc-crm.org/cidoc-crm/E85_Joining"/>
	<rdfs:range rdf:resource="http://www.cidoc-crm.org/cidoc-crm/E74_Group"/>
	<rdfs:comment xml:lang="en">This property identifies the instance of E74 Group of which an instance of E39 Actor becomes a member through an instance of E85 Joining.
Although a joining activity normally concerns only one instance of E74 Group, it is possible to imagine circumstances under which becoming member of one Group implies becoming member of another Group as well.
Joining events allow for describing people becoming members of a group with a more detailed path from E74 Group through, P144i gained member by, E85 Joining, P143 joined, E39 Actor, compared to the shortcut offered by P107 has current or former member (is current or former member of).
The property P144.1 kind of member can be used to specify the type of membership or the role the member has in the group.</rdfs:comment>
	<rdfs:label xml:lang="fr">a fait adhérer à</rdfs:label>
	<rdfs:label xml:lang="en">joined with</rdfs:label>
	<rdfs:label xml:lang="de">verband mit</rdfs:label>
	<rdfs:label xml:lang="zh">加入</rdfs:label>
</rdf:Description>

<rdf:Description rdf:about="http://www.cidoc-crm.org/cidoc-crm/P144i_gained_member_by">
	<rdf:type rdf:resource="http://www.w3.org/2002/07/owl#ObjectProperty"/>
	<rdfs:subPropertyOf rdf:resource="http://www.cidoc-crm.org/cidoc-crm/P11i_participated_in"/>
	<rdfs:domain rdf:resource="http://www.cidoc-crm.org/cidoc-crm/E74_Group"/>
	<rdfs:range rdf:resource="http://www.cidoc-crm.org/cidoc-crm/E85_Joining"/>
	<rdfs:label xml:lang="fr">a accueilli le membre par</rdfs:label>
	<rdfs:label xml:lang="de">erwarb Mitglied durch</rdfs:label>
	<rdfs:label xml:lang="en">gained member by</rdfs:label>
	<rdfs:label xml:lang="zh">获得成员</rdfs:label>
</rdf:Description>

<rdf:Description rdf:about="http://www.cidoc-crm.org/cidoc-crm/P145_separated">
	<rdf:type rdf:resource="http://www.w3.org/2002/07/owl#ObjectProperty"/>
	<rdfs:subPropertyOf rdf:resource="http://www.cidoc-crm.org/cidoc-crm/P11_had_participant"/>
	<owl:inverseOf rdf:resource="http://www.cidoc-crm.org/cidoc-crm/P145i_left_by"/>
	<rdfs:domain rdf:resource="http://www.cidoc-crm.org/cidoc-crm/E86_Leaving"/>
	<rdfs:range rdf:resource="http://www.cidoc-crm.org/cidoc-crm/E39_Actor"/>
	<rdfs:comment xml:lang="en">This property identifies the instance of E39 Actor that leaves an instance of E74 Group through an instance of E86 Leaving.</rdfs:comment>
	<rdfs:label xml:lang="fr">a dissocié</rdfs:label>
	<rdfs:label xml:lang="de">entließ</rdfs:label>
	<rdfs:label xml:lang="en">separated</rdfs:label>
	<rdfs:label xml:lang="zh">离开</rdfs:label>
</rdf:Description>

<rdf:Description rdf:about="http://www.cidoc-crm.org/cidoc-crm/P145i_left_by">
	<rdf:type rdf:resource="http://www.w3.org/2002/07/owl#ObjectProperty"/>
	<rdfs:subPropertyOf rdf:resource="http://www.cidoc-crm.org/cidoc-crm/P11i_participated_in"/>
	<rdfs:domain rdf:resource="http://www.cidoc-crm.org/cidoc-crm/E39_Actor"/>
	<rdfs:range rdf:resource="http://www.cidoc-crm.org/cidoc-crm/E86_Leaving"/>
	<rdfs:label xml:lang="fr">est dissocié par</rdfs:label>
	<rdfs:label xml:lang="en">left by</rdfs:label>
	<rdfs:label xml:lang="de">wurde entlassen durch</rdfs:label>
	<rdfs:label xml:lang="zh">留下</rdfs:label>
</rdf:Description>

<rdf:Description rdf:about="http://www.cidoc-crm.org/cidoc-crm/P146_separated_from">
	<rdf:type rdf:resource="http://www.w3.org/2002/07/owl#ObjectProperty"/>
	<rdfs:subPropertyOf rdf:resource="http://www.cidoc-crm.org/cidoc-crm/P11_had_participant"/>
	<owl:inverseOf rdf:resource="http://www.cidoc-crm.org/cidoc-crm/P146i_lost_member_by"/>
	<rdfs:domain rdf:resource="http://www.cidoc-crm.org/cidoc-crm/E86_Leaving"/>
	<rdfs:range rdf:resource="http://www.cidoc-crm.org/cidoc-crm/E74_Group"/>
	<rdfs:comment xml:lang="en">This property identifies the instance of E74 Group an instance of E39 Actor leaves through an instance of E86 Leaving.
Although a leaving activity normally concerns only one instance of E74 Group, it is possible to imagine circumstances under which leaving one E74 Group implies leaving another E74 Group as well.</rdfs:comment>
	<rdfs:label xml:lang="fr">a dissocié de</rdfs:label>
	<rdfs:label xml:lang="de">entließ von</rdfs:label>
	<rdfs:label xml:lang="en">separated from</rdfs:label>
	<rdfs:label xml:lang="zh">脱离</rdfs:label>
</rdf:Description>

<rdf:Description rdf:about="http://www.cidoc-crm.org/cidoc-crm/P146i_lost_member_by">
	<rdf:type rdf:resource="http://www.w3.org/2002/07/owl#ObjectProperty"/>
	<rdfs:subPropertyOf rdf:resource="http://www.cidoc-crm.org/cidoc-crm/P11i_participated_in"/>
	<rdfs:domain rdf:resource="http://www.cidoc-crm.org/cidoc-crm/E74_Group"/>
	<rdfs:range rdf:resource="http://www.cidoc-crm.org/cidoc-crm/E86_Leaving"/>
	<rdfs:label xml:lang="fr">a perdu le membre par</rdfs:label>
	<rdfs:label xml:lang="en">lost member by</rdfs:label>
	<rdfs:label xml:lang="de">verlor Mitglied durch</rdfs:label>
	<rdfs:label xml:lang="zh">失去成员</rdfs:label>
</rdf:Description>

<rdf:Description rdf:about="http://www.cidoc-crm.org/cidoc-crm/P147_curated">
	<rdf:type rdf:resource="http://www.w3.org/2002/07/owl#ObjectProperty"/>
	<owl:inverseOf rdf:resource="http://www.cidoc-crm.org/cidoc-crm/P147i_was_curated_by"/>
	<rdfs:domain rdf:resource="http://www.cidoc-crm.org/cidoc-crm/E87_Curation_Activity"/>
	<rdfs:range rdf:resource="http://www.cidoc-crm.org/cidoc-crm/E78_Curated_Holding"/>
	<rdfs:comment xml:lang="en">This property associates an instance of E87 Curation Activity with the instance of E78 Curated Holding with that is subject of that curation activity following some implicit or explicit curation plan.</rdfs:comment>
	<rdfs:label xml:lang="fr">a géré</rdfs:label>
	<rdfs:label xml:lang="de">betreute kuratorisch</rdfs:label>
	<rdfs:label xml:lang="en">curated</rdfs:label>
	<rdfs:label xml:lang="zh">管理</rdfs:label>
</rdf:Description>

<rdf:Description rdf:about="http://www.cidoc-crm.org/cidoc-crm/P147i_was_curated_by">
	<rdf:type rdf:resource="http://www.w3.org/2002/07/owl#ObjectProperty"/>
	<rdfs:domain rdf:resource="http://www.cidoc-crm.org/cidoc-crm/E78_Curated_Holding"/>
	<rdfs:range rdf:resource="http://www.cidoc-crm.org/cidoc-crm/E87_Curation_Activity"/>
	<rdfs:label xml:lang="fr">a été géré par</rdfs:label>
	<rdfs:label xml:lang="en">was curated by</rdfs:label>
	<rdfs:label xml:lang="de">wurde kuratorisch betreut durch</rdfs:label>
	<rdfs:label xml:lang="zh">被管理</rdfs:label>
</rdf:Description>

<rdf:Description rdf:about="http://www.cidoc-crm.org/cidoc-crm/P148_has_component">
	<rdf:type rdf:resource="http://www.w3.org/2002/07/owl#ObjectProperty"/>
	<owl:inverseOf rdf:resource="http://www.cidoc-crm.org/cidoc-crm/P148i_is_component_of"/>
	<rdfs:domain rdf:resource="http://www.cidoc-crm.org/cidoc-crm/E89_Propositional_Object"/>
	<rdfs:range rdf:resource="http://www.cidoc-crm.org/cidoc-crm/E89_Propositional_Object"/>
	<rdfs:comment xml:lang="en">This property associates an instance of E89 Propositional Object with a structural part of it that is by itself an instance of E89 Propositional Object.
This property is transitive. This property is asymmetric.</rdfs:comment>
	<rdfs:label xml:lang="fr">a pour composant</rdfs:label>
	<rdfs:label xml:lang="en">has component</rdfs:label>
	<rdfs:label xml:lang="de">hat Bestandteil</rdfs:label>
	<rdfs:label xml:lang="zh">有组件</rdfs:label>
</rdf:Description>

<rdf:Description rdf:about="http://www.cidoc-crm.org/cidoc-crm/P148i_is_component_of">
	<rdf:type rdf:resource="http://www.w3.org/2002/07/owl#ObjectProperty"/>
	<rdfs:domain rdf:resource="http://www.cidoc-crm.org/cidoc-crm/E89_Propositional_Object"/>
	<rdfs:range rdf:resource="http://www.cidoc-crm.org/cidoc-crm/E89_Propositional_Object"/>
	<rdfs:label xml:lang="fr">est le composant de</rdfs:label>
	<rdfs:label xml:lang="en">is component of</rdfs:label>
	<rdfs:label xml:lang="de">ist Bestandteil von</rdfs:label>
	<rdfs:label xml:lang="zh">是组件</rdfs:label>
</rdf:Description>

<rdf:Description rdf:about="http://www.cidoc-crm.org/cidoc-crm/P14_carried_out_by">
	<rdf:type rdf:resource="http://www.w3.org/2002/07/owl#ObjectProperty"/>
	<rdfs:subPropertyOf rdf:resource="http://www.cidoc-crm.org/cidoc-crm/P11_had_participant"/>
	<owl:inverseOf rdf:resource="http://www.cidoc-crm.org/cidoc-crm/P14i_performed"/>
	<rdfs:domain rdf:resource="http://www.cidoc-crm.org/cidoc-crm/E7_Activity"/>
	<rdfs:range rdf:resource="http://www.cidoc-crm.org/cidoc-crm/E39_Actor"/>
	<rdfs:comment xml:lang="en">This property describes the active participation of an instance of E39 Actor in an instance of E7 Activity.
It implies causal or legal responsibility. The P14.1 in the role of property of the property specifies the nature of an Actor’s participation.</rdfs:comment>
	<rdfs:label xml:lang="fr">a été effectué par</rdfs:label>
	<rdfs:label xml:lang="en">carried out by</rdfs:label>
	<rdfs:label xml:lang="pt">realizada por</rdfs:label>
	<rdfs:label xml:lang="de">wurde ausgeführt von</rdfs:label>
	<rdfs:label xml:lang="el">πραγματοποιήθηκε από</rdfs:label>
	<rdfs:label xml:lang="ru">выполнялся</rdfs:label>
	<rdfs:label xml:lang="zh">执行者是</rdfs:label>
</rdf:Description>

<rdf:Description rdf:about="http://www.cidoc-crm.org/cidoc-crm/P14i_performed">
	<rdf:type rdf:resource="http://www.w3.org/2002/07/owl#ObjectProperty"/>
	<rdfs:subPropertyOf rdf:resource="http://www.cidoc-crm.org/cidoc-crm/P11i_participated_in"/>
	<rdfs:domain rdf:resource="http://www.cidoc-crm.org/cidoc-crm/E39_Actor"/>
	<rdfs:range rdf:resource="http://www.cidoc-crm.org/cidoc-crm/E7_Activity"/>
	<rdfs:label xml:lang="fr">a effectué</rdfs:label>
	<rdfs:label xml:lang="pt">executou</rdfs:label>
	<rdfs:label xml:lang="de">führte aus</rdfs:label>
	<rdfs:label xml:lang="en">performed</rdfs:label>
	<rdfs:label xml:lang="el">πραγματοποίησε</rdfs:label>
	<rdfs:label xml:lang="ru">выполнял</rdfs:label>
	<rdfs:label xml:lang="zh">执行</rdfs:label>
</rdf:Description>

<rdf:Description rdf:about="http://www.cidoc-crm.org/cidoc-crm/P150_defines_typical_parts_of">
	<rdf:type rdf:resource="http://www.w3.org/2002/07/owl#ObjectProperty"/>
	<owl:inverseOf rdf:resource="http://www.cidoc-crm.org/cidoc-crm/P150i_defines_typical_wholes_for"/>
	<rdfs:domain rdf:resource="http://www.cidoc-crm.org/cidoc-crm/E55_Type"/>
	<rdfs:range rdf:resource="http://www.cidoc-crm.org/cidoc-crm/E55_Type"/>
	<rdfs:comment xml:lang="en">This property associates an instance of E55 Type “A” with an instance of E55 Type “B”, when items of type “A” typically form part of items of type “B”, such as “car motors” and “cars”.
It allows types to be organised into hierarchies based on one type describing a typical part of another. This property is equivalent to “broader term partitive (BTP)” as defined in ISO 2788 and “broaderPartitive” in SKOS.
This property is not transitive. This property is asymmetric.</rdfs:comment>
	<rdfs:label xml:lang="en">defines typical parts of</rdfs:label>
	<rdfs:label xml:lang="fr">définit les éléments typiques de</rdfs:label>
</rdf:Description>

<rdf:Description rdf:about="http://www.cidoc-crm.org/cidoc-crm/P150i_defines_typical_wholes_for">
	<rdf:type rdf:resource="http://www.w3.org/2002/07/owl#ObjectProperty"/>
	<rdfs:domain rdf:resource="http://www.cidoc-crm.org/cidoc-crm/E55_Type"/>
	<rdfs:range rdf:resource="http://www.cidoc-crm.org/cidoc-crm/E55_Type"/>
	<rdfs:label xml:lang="en">defines typical wholes for</rdfs:label>
	<rdfs:label xml:lang="fr">définit l’ensemble typique pour</rdfs:label>
</rdf:Description>

<rdf:Description rdf:about="http://www.cidoc-crm.org/cidoc-crm/P151_was_formed_from">
	<rdf:type rdf:resource="http://www.w3.org/2002/07/owl#ObjectProperty"/>
	<rdfs:subPropertyOf rdf:resource="http://www.cidoc-crm.org/cidoc-crm/P11_had_participant"/>
	<owl:inverseOf rdf:resource="http://www.cidoc-crm.org/cidoc-crm/P151i_participated_in"/>
	<rdfs:domain rdf:resource="http://www.cidoc-crm.org/cidoc-crm/E66_Formation"/>
	<rdfs:range rdf:resource="http://www.cidoc-crm.org/cidoc-crm/E74_Group"/>
	<rdfs:comment xml:lang="en">This property associates an instance of E66 Formation with an instance of E74 Group from which the new group was formed preserving a sense of continuity such as in mission, membership or tradition.</rdfs:comment>
	<rdfs:label xml:lang="fr">a été formé à partir de</rdfs:label>
	<rdfs:label xml:lang="en">was formed from</rdfs:label>
</rdf:Description>

<rdf:Description rdf:about="http://www.cidoc-crm.org/cidoc-crm/P151i_participated_in">
	<rdf:type rdf:resource="http://www.w3.org/2002/07/owl#ObjectProperty"/>
	<rdfs:subPropertyOf rdf:resource="http://www.cidoc-crm.org/cidoc-crm/P11i_participated_in"/>
	<rdfs:domain rdf:resource="http://www.cidoc-crm.org/cidoc-crm/E74_Group"/>
	<rdfs:range rdf:resource="http://www.cidoc-crm.org/cidoc-crm/E66_Formation"/>
	<rdfs:label xml:lang="fr">a participé à</rdfs:label>
	<rdfs:label xml:lang="en">participated in</rdfs:label>
</rdf:Description>

<rdf:Description rdf:about="http://www.cidoc-crm.org/cidoc-crm/P152_has_parent">
	<rdf:type rdf:resource="http://www.w3.org/2002/07/owl#ObjectProperty"/>
	<owl:inverseOf rdf:resource="http://www.cidoc-crm.org/cidoc-crm/P152i_is_parent_of"/>
	<rdfs:domain rdf:resource="http://www.cidoc-crm.org/cidoc-crm/E21_Person"/>
	<rdfs:range rdf:resource="http://www.cidoc-crm.org/cidoc-crm/E21_Person"/>
	<rdfs:comment xml:lang="en">This property associates an instance of E21 Person with another instance of E21 Person who plays the role of the first instance’s parent, regardless of whether the relationship is biological parenthood, assumed or pretended biological parenthood or an equivalent legal status of rights and obligations obtained by a social or legal act.
This property is, among others, a shortcut of the fully developed paths from E21 Person through P98i was born, E67 Birth, P96 by mother to E21 Person, and from E21 Person through P98i was born, E67 Birth, P97 from father to E21 Person.
This property is not transitive. This property is irreflexive.</rdfs:comment>
	<rdfs:label xml:lang="fr">a pour parent</rdfs:label>
	<rdfs:label xml:lang="en">has parent</rdfs:label>
</rdf:Description>

<rdf:Description rdf:about="http://www.cidoc-crm.org/cidoc-crm/P152i_is_parent_of">
	<rdf:type rdf:resource="http://www.w3.org/2002/07/owl#ObjectProperty"/>
	<rdfs:domain rdf:resource="http://www.cidoc-crm.org/cidoc-crm/E21_Person"/>
	<rdfs:range rdf:resource="http://www.cidoc-crm.org/cidoc-crm/E21_Person"/>
	<rdfs:label xml:lang="fr">est le parent de</rdfs:label>
	<rdfs:label xml:lang="en">is parent of</rdfs:label>
</rdf:Description>

<rdf:Description rdf:about="http://www.cidoc-crm.org/cidoc-crm/P156_occupies">
	<rdf:type rdf:resource="http://www.w3.org/2002/07/owl#ObjectProperty"/>
	<rdfs:subPropertyOf rdf:resource="http://www.cidoc-crm.org/cidoc-crm/P157i_provides_reference_space_for"/>
	<rdfs:subPropertyOf rdf:resource="http://www.cidoc-crm.org/cidoc-crm/P53_has_former_or_current_location"/>
	<owl:inverseOf rdf:resource="http://www.cidoc-crm.org/cidoc-crm/P156i_is_occupied_by"/>
	<rdfs:domain rdf:resource="http://www.cidoc-crm.org/cidoc-crm/E18_Physical_Thing"/>
	<rdfs:range rdf:resource="http://www.cidoc-crm.org/cidoc-crm/E53_Place"/>
	<rdfs:comment xml:lang="en">This property describes the largest volume in space, an instance of E53 Place, that an instance of E18 Physical Thing has occupied at any time during its existence, with respect to the reference space relative to the physical thing itself. This allows for describing the thing itself as a place that may contain other things, such as a box that may contain coins. In other words, it is the volume that contains all the points which the thing has covered at some time during its existence. The reference space for the associated place must be the one that is permanently at rest (P157 is at rest relative to) relative to the physical thing. For instances of E19 Physical Objects it is the one which is at rest relative to the object itself, i.e., which moves together with the object. For instances of E26 Physical Feature it is one which is at rest relative to the physical feature itself and the surrounding matter immediately connected to it. Therefore, there is a 1:1 relation between the instance E18 Physical Thing and the instance of E53 Place it occupies. We include in the occupied space the space filled by the matter of the physical thing and all its inner spaces.
This property implies the fully developed path from E18 Physical Thing through P196 defines, E92 Spacetime Volume, P161 has spatial projection to E53 Place. However, in contrast to P156 occupies, the property P161 has spatial projection does not constrain the reference space of the referred instance of E53 Place.
In contrast to P156 occupies, for the property P53 has former or current location the following holds:
It does not constrain the reference space of the referred instance of E53 Place.
It identifies a possibly wider instance of E53 Place at which a thing is or has been for some unspecified time-span.
If the reference space of the referred instance of E53 Place is not at rest with respect to the physical thing found there, the physical thing may move away after some time to another place and/or may have been at some other place before. The same holds for the fully developed path from E18 Physical Thing through P196 defines, E92 Spacetime Volume, P161 has spatial projection to E53 Place.</rdfs:comment>
	<rdfs:label xml:lang="fr">occupe</rdfs:label>
	<rdfs:label xml:lang="en">occupies</rdfs:label>
</rdf:Description>

<rdf:Description rdf:about="http://www.cidoc-crm.org/cidoc-crm/P156i_is_occupied_by">
	<rdf:type rdf:resource="http://www.w3.org/2002/07/owl#ObjectProperty"/>
	<rdfs:subPropertyOf rdf:resource="http://www.cidoc-crm.org/cidoc-crm/P157_is_at_rest_relative_to"/>
	<rdfs:subPropertyOf rdf:resource="http://www.cidoc-crm.org/cidoc-crm/P53i_is_former_or_current_location_of"/>
	<rdfs:domain rdf:resource="http://www.cidoc-crm.org/cidoc-crm/E53_Place"/>
	<rdfs:range rdf:resource="http://www.cidoc-crm.org/cidoc-crm/E18_Physical_Thing"/>
	<rdfs:label xml:lang="fr">est occupé par</rdfs:label>
	<rdfs:label xml:lang="en">is occupied by</rdfs:label>
</rdf:Description>

<rdf:Description rdf:about="http://www.cidoc-crm.org/cidoc-crm/P157_is_at_rest_relative_to">
	<rdf:type rdf:resource="http://www.w3.org/2002/07/owl#ObjectProperty"/>
	<owl:inverseOf rdf:resource="http://www.cidoc-crm.org/cidoc-crm/P157i_provides_reference_space_for"/>
	<rdfs:domain rdf:resource="http://www.cidoc-crm.org/cidoc-crm/E53_Place"/>
	<rdfs:range rdf:resource="http://www.cidoc-crm.org/cidoc-crm/E18_Physical_Thing"/>
	<rdfs:comment xml:lang="en">This property associates an instance of E53 Place with the instance of E18 Physical Thing that determines a reference space for this instance of E53 Place by being at rest with respect to this reference space. The relative stability of form of an instance of E18 Physical Thing defines its default reference space. The reference space is not spatially limited to the referred thing. For example, a ship determines a reference space in terms of which other ships in its neighbourhood may be described. Larger constellations of matter, such as continental plates, may comprise many physical features that are at rest with them and define the same reference space.</rdfs:comment>
	<rdfs:label xml:lang="fr">est à l’arrêt par rapport à</rdfs:label>
	<rdfs:label xml:lang="en">is at rest relative to</rdfs:label>
</rdf:Description>

<rdf:Description rdf:about="http://www.cidoc-crm.org/cidoc-crm/P157i_provides_reference_space_for">
	<rdf:type rdf:resource="http://www.w3.org/2002/07/owl#ObjectProperty"/>
	<rdfs:domain rdf:resource="http://www.cidoc-crm.org/cidoc-crm/E18_Physical_Thing"/>
	<rdfs:range rdf:resource="http://www.cidoc-crm.org/cidoc-crm/E53_Place"/>
	<rdfs:label xml:lang="fr">procure l’espace de référence pour</rdfs:label>
	<rdfs:label xml:lang="en">provides reference space for</rdfs:label>
</rdf:Description>

<rdf:Description rdf:about="http://www.cidoc-crm.org/cidoc-crm/P15_was_influenced_by">
	<rdf:type rdf:resource="http://www.w3.org/2002/07/owl#ObjectProperty"/>
	<owl:inverseOf rdf:resource="http://www.cidoc-crm.org/cidoc-crm/P15i_influenced"/>
	<rdfs:domain rdf:resource="http://www.cidoc-crm.org/cidoc-crm/E7_Activity"/>
	<rdfs:range rdf:resource="http://www.cidoc-crm.org/cidoc-crm/E1_CRM_Entity"/>
	<rdfs:comment xml:lang="en">This is a high-level property, which captures the relationship between an instance of E7 Activity and anything, that is, an instance of E1 CRM Entity, that may have had some bearing upon it.
The property has more specific subproperties.</rdfs:comment>
	<rdfs:label xml:lang="fr">a été influencé par</rdfs:label>
	<rdfs:label xml:lang="pt">foi influenciado por</rdfs:label>
	<rdfs:label xml:lang="en">was influenced by</rdfs:label>
	<rdfs:label xml:lang="de">wurde beeinflußt durch</rdfs:label>
	<rdfs:label xml:lang="el">επηρεάστηκε από</rdfs:label>
	<rdfs:label xml:lang="ru">находился под влиянием</rdfs:label>
	<rdfs:label xml:lang="zh">被影响</rdfs:label>
</rdf:Description>

<rdf:Description rdf:about="http://www.cidoc-crm.org/cidoc-crm/P15i_influenced">
	<rdf:type rdf:resource="http://www.w3.org/2002/07/owl#ObjectProperty"/>
	<rdfs:domain rdf:resource="http://www.cidoc-crm.org/cidoc-crm/E1_CRM_Entity"/>
	<rdfs:range rdf:resource="http://www.cidoc-crm.org/cidoc-crm/E7_Activity"/>
	<rdfs:label xml:lang="fr">a influencé</rdfs:label>
	<rdfs:label xml:lang="de">beeinflußte</rdfs:label>
	<rdfs:label xml:lang="en">influenced</rdfs:label>
	<rdfs:label xml:lang="pt">influenciou</rdfs:label>
	<rdfs:label xml:lang="el">επηρέασε</rdfs:label>
	<rdfs:label xml:lang="ru">оказал влияние на</rdfs:label>
	<rdfs:label xml:lang="zh">影响</rdfs:label>
</rdf:Description>

<rdf:Description rdf:about="http://www.cidoc-crm.org/cidoc-crm/P160_has_temporal_projection">
	<rdf:type rdf:resource="http://www.w3.org/2002/07/owl#ObjectProperty"/>
	<owl:inverseOf rdf:resource="http://www.cidoc-crm.org/cidoc-crm/P160i_is_temporal_projection_of"/>
	<rdfs:domain rdf:resource="http://www.cidoc-crm.org/cidoc-crm/E92_Spacetime_Volume"/>
	<rdfs:range rdf:resource="http://www.cidoc-crm.org/cidoc-crm/E52_Time-Span"/>
	<rdfs:comment xml:lang="en">This property describes the temporal projection of an instance of E92 Spacetime Volume. The property P4 has time-span is the same as P160 has temporal projection if it is used to document an instance of E4 Period or any subclass of it.</rdfs:comment>
	<rdfs:label xml:lang="fr">a pour projection temporelle</rdfs:label>
	<rdfs:label xml:lang="en">has temporal projection</rdfs:label>
</rdf:Description>

<rdf:Description rdf:about="http://www.cidoc-crm.org/cidoc-crm/P160i_is_temporal_projection_of">
	<rdf:type rdf:resource="http://www.w3.org/2002/07/owl#ObjectProperty"/>
	<rdfs:domain rdf:resource="http://www.cidoc-crm.org/cidoc-crm/E52_Time-Span"/>
	<rdfs:range rdf:resource="http://www.cidoc-crm.org/cidoc-crm/E92_Spacetime_Volume"/>
	<rdfs:label xml:lang="fr">est la projection temporelle de</rdfs:label>
	<rdfs:label xml:lang="en">is temporal projection of</rdfs:label>
</rdf:Description>

<rdf:Description rdf:about="http://www.cidoc-crm.org/cidoc-crm/P161_has_spatial_projection">
	<rdf:type rdf:resource="http://www.w3.org/2002/07/owl#ObjectProperty"/>
	<owl:inverseOf rdf:resource="http://www.cidoc-crm.org/cidoc-crm/P161i_is_spatial_projection_of"/>
	<rdfs:domain rdf:resource="http://www.cidoc-crm.org/cidoc-crm/E92_Spacetime_Volume"/>
	<rdfs:range rdf:resource="http://www.cidoc-crm.org/cidoc-crm/E53_Place"/>
	<rdfs:comment xml:lang="en">This property associates an instance of E92 Spacetime Volume with an instance of E53 Place that is the result of the spatial projection of the instance of the E92 Spacetime Volume on a reference space.
In general, there can be more than one useful reference space (for reference space see P156 occupies and P157 is at rest relative to) to describe the spatial projection of a spacetime volume, for example, in describing a sea battle, the difference between the battle ship and the seafloor as reference spaces. Thus, it can be seen that the projection is not unique.
The spatial projection is the actual spatial coverage of a spacetime volume, which normally has fuzzy boundaries except for instances of E92 Spacetime Volume which are geometrically defined in the same reference system as the range of this property and are an exception to this and do not have fuzzy boundaries. Modelling explicitly fuzzy spatial projections serves therefore as a common topological reference of different spatial approximations rather than absolute geometric determination, for instance for relating outer or inner spatial boundaries for the respective spacetime volumes.
The spatial projection is unique with respect to the reference system. For instance, there is exactly one spatial projection of Lord Nelson’s dying relative to the ship HMS Victory, i.e. the location of his body relative to the ship HMS Victory at the time of his death.
In case the domain of an instance of P161 has spatial projection is an instance of E4 Period, the spatial projection describes all areas that period was ever present at, for instance, the Roman Empire.
This property is part of the fully developed path from E18 Physical Thing through P196 defines, E92 Spacetime Volume, P161 has spatial projection to E53 Place, which in turn is implied by P156 occupies (is occupied by).</rdfs:comment>
	<rdfs:label xml:lang="fr">a pour projection spatiale</rdfs:label>
	<rdfs:label xml:lang="en">has spatial projection</rdfs:label>
</rdf:Description>

<rdf:Description rdf:about="http://www.cidoc-crm.org/cidoc-crm/P161i_is_spatial_projection_of">
	<rdf:type rdf:resource="http://www.w3.org/2002/07/owl#ObjectProperty"/>
	<rdfs:domain rdf:resource="http://www.cidoc-crm.org/cidoc-crm/E53_Place"/>
	<rdfs:range rdf:resource="http://www.cidoc-crm.org/cidoc-crm/E92_Spacetime_Volume"/>
	<rdfs:label xml:lang="fr">est la projection spatiale de</rdfs:label>
	<rdfs:label xml:lang="en">is spatial projection of</rdfs:label>
</rdf:Description>

<rdf:Description rdf:about="http://www.cidoc-crm.org/cidoc-crm/P164_is_temporally_specified_by">
	<rdf:type rdf:resource="http://www.w3.org/2002/07/owl#ObjectProperty"/>
	<rdfs:subPropertyOf rdf:resource="http://www.cidoc-crm.org/cidoc-crm/P160_has_temporal_projection"/>
	<owl:inverseOf rdf:resource="http://www.cidoc-crm.org/cidoc-crm/P164i_temporally_specifies"/>
	<rdfs:domain rdf:resource="http://www.cidoc-crm.org/cidoc-crm/E93_Presence"/>
	<rdfs:range rdf:resource="http://www.cidoc-crm.org/cidoc-crm/E52_Time-Span"/>
	<rdfs:comment xml:lang="en">This property relates an instance of E93 Presence with the instance of E52 Time-Span that defines the time-slice of the spacetime volume that this instance of E93 Presence is related to via the property P166 was a presence of (had presence).
There are two typical cases for the determination of the related instance of E52 Time-Span. In the first, it is the temporal extent of an instance of E2 Temporal Entity (documented with P4 has time-span (is time-span of)): this then documents the simultaneity of the instance of E93 Presence and the instance of E2 Temporal Entity, even if the absolute time-span is not known, and can be regarded as a phenomenal time-span. In the second, the instance of E52 Time-Span is a date range declared in or derived from historical sources or provided by dating methods: this is a declarative time-span.</rdfs:comment>
	<rdfs:label xml:lang="fr">est temporellement spécifié par</rdfs:label>
	<rdfs:label xml:lang="en">is temporally specified by</rdfs:label>
</rdf:Description>

<rdf:Description rdf:about="http://www.cidoc-crm.org/cidoc-crm/P164i_temporally_specifies">
	<rdf:type rdf:resource="http://www.w3.org/2002/07/owl#ObjectProperty"/>
	<rdfs:subPropertyOf rdf:resource="http://www.cidoc-crm.org/cidoc-crm/P160i_is_temporal_projection_of"/>
	<rdfs:domain rdf:resource="http://www.cidoc-crm.org/cidoc-crm/E52_Time-Span"/>
	<rdfs:range rdf:resource="http://www.cidoc-crm.org/cidoc-crm/E93_Presence"/>
	<rdfs:label xml:lang="fr">spécifie temporellement</rdfs:label>
	<rdfs:label xml:lang="en">temporally specifies</rdfs:label>
</rdf:Description>

<rdf:Description rdf:about="http://www.cidoc-crm.org/cidoc-crm/P165_incorporates">
	<rdf:type rdf:resource="http://www.w3.org/2002/07/owl#ObjectProperty"/>
	<rdfs:subPropertyOf rdf:resource="http://www.cidoc-crm.org/cidoc-crm/P106_is_composed_of"/>
	<owl:inverseOf rdf:resource="http://www.cidoc-crm.org/cidoc-crm/P165i_is_incorporated_in"/>
	<rdfs:domain rdf:resource="http://www.cidoc-crm.org/cidoc-crm/E73_Information_Object"/>
	<rdfs:range rdf:resource="http://www.cidoc-crm.org/cidoc-crm/E90_Symbolic_Object"/>
	<rdfs:comment xml:lang="en">This property associates an instance of E73 Information Object with an instance of E90 Symbolic Object (or any of its subclasses) that was included in it.
This property makes it possible to recognise the autonomous status of the incorporated signs, which were created in a distinct context, and can be incorporated in many instances of E73 Information Object, and to highlight the difference between structural and accidental whole-part relationships between conceptual entities.
It accounts for many cultural facts that are quite frequent and significant: the inclusion of a poem in an anthology, the re-use of an operatic aria in a new opera, the use of a reproduction of a painting for a book cover or a CD booklet, the integration of textual quotations, the presence of lyrics in a song that sets those lyrics to music, the presence of the text of a play in a movie based on that play, etc.
In particular, this property allows for modelling relationships of different levels of symbolic specificity, such as the natural language words making up a particular text, the characters making up the words and punctuation, the choice of fonts and page layout for the characters.
When restricted to information objects, that is, seen as a property with E73 Information Object as domain and range the property is transitive.
A digital photograph of a manuscript page incorporates the text of a manuscript page, if the respective text is defined as a sequence of symbols of a particular type, such as Latin characters, and the resolution and quality of the digital image is sufficient to resolve these symbols so they are readable on the digital image.
This property is asymmetric.</rdfs:comment>
	<rdfs:label xml:lang="fr">inclut</rdfs:label>
	<rdfs:label xml:lang="en">incorporates</rdfs:label>
</rdf:Description>

<rdf:Description rdf:about="http://www.cidoc-crm.org/cidoc-crm/P165i_is_incorporated_in">
	<rdf:type rdf:resource="http://www.w3.org/2002/07/owl#ObjectProperty"/>
	<rdfs:subPropertyOf rdf:resource="http://www.cidoc-crm.org/cidoc-crm/P106i_forms_part_of"/>
	<rdfs:domain rdf:resource="http://www.cidoc-crm.org/cidoc-crm/E90_Symbolic_Object"/>
	<rdfs:range rdf:resource="http://www.cidoc-crm.org/cidoc-crm/E73_Information_Object"/>
	<rdfs:label xml:lang="fr">est inclus dans</rdfs:label>
	<rdfs:label xml:lang="en">is incorporated in</rdfs:label>
</rdf:Description>

<rdf:Description rdf:about="http://www.cidoc-crm.org/cidoc-crm/P166_was_a_presence_of">
	<rdf:type rdf:resource="http://www.w3.org/2002/07/owl#ObjectProperty"/>
	<rdfs:subPropertyOf rdf:resource="http://www.cidoc-crm.org/cidoc-crm/P10_falls_within"/>
	<owl:inverseOf rdf:resource="http://www.cidoc-crm.org/cidoc-crm/P166i_had_presence"/>
	<rdfs:domain rdf:resource="http://www.cidoc-crm.org/cidoc-crm/E93_Presence"/>
	<rdfs:range rdf:resource="http://www.cidoc-crm.org/cidoc-crm/E92_Spacetime_Volume"/>
	<rdfs:comment xml:lang="en">This property associates an instance of E93 Presence with the instance of E92 Spacetime Volume of which it represents a temporal restriction (i.e. a time-slice). Instantiating this property constitutes a necessary part of the identity of the respective instance of E93 Presence.</rdfs:comment>
	<rdfs:label xml:lang="fr">a été une présence de</rdfs:label>
	<rdfs:label xml:lang="en">was a presence of</rdfs:label>
</rdf:Description>

<rdf:Description rdf:about="http://www.cidoc-crm.org/cidoc-crm/P166i_had_presence">
	<rdf:type rdf:resource="http://www.w3.org/2002/07/owl#ObjectProperty"/>
	<rdfs:subPropertyOf rdf:resource="http://www.cidoc-crm.org/cidoc-crm/P10i_contains"/>
	<rdfs:domain rdf:resource="http://www.cidoc-crm.org/cidoc-crm/E92_Spacetime_Volume"/>
	<rdfs:range rdf:resource="http://www.cidoc-crm.org/cidoc-crm/E93_Presence"/>
	<rdfs:label xml:lang="fr">a eu pour présence</rdfs:label>
	<rdfs:label xml:lang="en">had presence</rdfs:label>
</rdf:Description>

<rdf:Description rdf:about="http://www.cidoc-crm.org/cidoc-crm/P167_was_within">
	<rdf:type rdf:resource="http://www.w3.org/2002/07/owl#ObjectProperty"/>
	<owl:inverseOf rdf:resource="http://www.cidoc-crm.org/cidoc-crm/P167i_includes"/>
	<rdfs:domain rdf:resource="http://www.cidoc-crm.org/cidoc-crm/E93_Presence"/>
	<rdfs:range rdf:resource="http://www.cidoc-crm.org/cidoc-crm/E53_Place"/>
	<rdfs:comment xml:lang="en">This property associates an instance of E93 Presence with an instance of E53 Place that geometrically includes the spatial projection of the respective instance of E93 Presence. Besides others, this property may be used to state in which space an object has been for some known time, such as a room of a castle or in a drawer. It may also be used to describe a confinement of the spatial extent of some realm during a known time-span.
This property is a shortcut of the more fully developed path from E93 Presence through P161 has spatial projection, E53 Place, P89 falls within (contains) to E53 Place.</rdfs:comment>
	<rdfs:label xml:lang="fr">s’inscrivait dans</rdfs:label>
	<rdfs:label xml:lang="en">was within</rdfs:label>
</rdf:Description>

<rdf:Description rdf:about="http://www.cidoc-crm.org/cidoc-crm/P167i_includes">
	<rdf:type rdf:resource="http://www.w3.org/2002/07/owl#ObjectProperty"/>
	<rdfs:domain rdf:resource="http://www.cidoc-crm.org/cidoc-crm/E53_Place"/>
	<rdfs:range rdf:resource="http://www.cidoc-crm.org/cidoc-crm/E93_Presence"/>
	<rdfs:label xml:lang="fr">comporte</rdfs:label>
	<rdfs:label xml:lang="en">includes</rdfs:label>
</rdf:Description>

<rdf:Description rdf:about="http://www.cidoc-crm.org/cidoc-crm/P16_used_specific_object">
	<rdf:type rdf:resource="http://www.w3.org/2002/07/owl#ObjectProperty"/>
	<rdfs:subPropertyOf rdf:resource="http://www.cidoc-crm.org/cidoc-crm/P12_occurred_in_the_presence_of"/>
	<rdfs:subPropertyOf rdf:resource="http://www.cidoc-crm.org/cidoc-crm/P15_was_influenced_by"/>
	<owl:inverseOf rdf:resource="http://www.cidoc-crm.org/cidoc-crm/P16i_was_used_for"/>
	<rdfs:domain rdf:resource="http://www.cidoc-crm.org/cidoc-crm/E7_Activity"/>
	<rdfs:range rdf:resource="http://www.cidoc-crm.org/cidoc-crm/E70_Thing"/>
	<rdfs:comment xml:lang="en">This property describes the use of material or immaterial things in a way essential to the performance or the outcome of an instance of E7 Activity.
This property typically applies to tools, instruments, moulds, raw materials and items embedded in a product. It implies that the presence of the object in question was a necessary condition for the action. For example, the activity of writing this text required the use of a computer. An immaterial thing can be used if at least one of its carriers is present. For example, the software tools on a computer.
Another example is the use of a particular name by a particular group of people over some span to identify a thing, such as a settlement. In this case, the physical carriers of this name are at least the people understanding its use.</rdfs:comment>
	<rdfs:label xml:lang="fr">a mobilisé l’objet spécifique</rdfs:label>
	<rdfs:label xml:lang="de">benutzte das bestimmte Objekt</rdfs:label>
	<rdfs:label xml:lang="en">used specific object</rdfs:label>
	<rdfs:label xml:lang="pt">usou objeto específico</rdfs:label>
	<rdfs:label xml:lang="el">χρησιμοποίησε αντικείμενο</rdfs:label>
	<rdfs:label xml:lang="ru">использовал особый объект</rdfs:label>
	<rdfs:label xml:lang="zh">使用特定对象</rdfs:label>
</rdf:Description>

<rdf:Description rdf:about="http://www.cidoc-crm.org/cidoc-crm/P16i_was_used_for">
	<rdf:type rdf:resource="http://www.w3.org/2002/07/owl#ObjectProperty"/>
	<rdfs:subPropertyOf rdf:resource="http://www.cidoc-crm.org/cidoc-crm/P12i_was_present_at"/>
	<rdfs:subPropertyOf rdf:resource="http://www.cidoc-crm.org/cidoc-crm/P15i_influenced"/>
	<rdfs:domain rdf:resource="http://www.cidoc-crm.org/cidoc-crm/E70_Thing"/>
	<rdfs:range rdf:resource="http://www.cidoc-crm.org/cidoc-crm/E7_Activity"/>
	<rdfs:label xml:lang="fr">a été mobilisé pour</rdfs:label>
	<rdfs:label xml:lang="pt">foi usado por</rdfs:label>
	<rdfs:label xml:lang="en">was used for</rdfs:label>
	<rdfs:label xml:lang="de">wurde benutzt für</rdfs:label>
	<rdfs:label xml:lang="el">χρησιμοποιήθηκε για</rdfs:label>
	<rdfs:label xml:lang="ru">был использован для</rdfs:label>
	<rdfs:label xml:lang="zh">用于</rdfs:label>
</rdf:Description>

<rdf:Description rdf:about="http://www.cidoc-crm.org/cidoc-crm/P173_starts_before_or_with_the_end_of">
	<rdf:type rdf:resource="http://www.w3.org/2002/07/owl#ObjectProperty"/>
	<owl:inverseOf rdf:resource="http://www.cidoc-crm.org/cidoc-crm/P173i_ends_after_or_with_the_start_of"/>
	<rdfs:domain rdf:resource="http://www.cidoc-crm.org/cidoc-crm/E2_Temporal_Entity"/>
	<rdfs:range rdf:resource="http://www.cidoc-crm.org/cidoc-crm/E2_Temporal_Entity"/>
	<rdfs:comment xml:lang="en">This property specifies that the temporal extent of the domain instance A of E2 Temporal Entity starts before or simultaneously with the end of the temporal extent of the range instance B of E2 Temporal Entity.
In other words, if A = [A-start, A-end] and B = [B-start, B-end], it means A-start ≤ B-end is true.
This property is part of the set of temporal primitives P173 – P176, P182 – P185.
This property corresponds to the disjunction (logical OR) of the following Allen temporal relations (Allen, 1983): {before, meets, met-by, overlaps, starts, started-by, contains, finishes, finished-by, equals, during, overlapped by}.
This property is not transitive.

Figure 8: Temporal entity A starts before or with the end of temporal entity B. Here A is longer than B

Figure 9: Temporal entity A starts before or with the end of temporal entity B. Here A is shorter than B</rdfs:comment>
	<rdfs:label xml:lang="fr">commence avant ou au moment de la fin de</rdfs:label>
	<rdfs:label xml:lang="en">starts before or with the end of</rdfs:label>
</rdf:Description>

<rdf:Description rdf:about="http://www.cidoc-crm.org/cidoc-crm/P173i_ends_after_or_with_the_start_of">
	<rdf:type rdf:resource="http://www.w3.org/2002/07/owl#ObjectProperty"/>
	<rdfs:domain rdf:resource="http://www.cidoc-crm.org/cidoc-crm/E2_Temporal_Entity"/>
	<rdfs:range rdf:resource="http://www.cidoc-crm.org/cidoc-crm/E2_Temporal_Entity"/>
	<rdfs:label xml:lang="en">ends after or with the start of</rdfs:label>
	<rdfs:label xml:lang="fr">se termine après ou au moment du début de</rdfs:label>
</rdf:Description>

<rdf:Description rdf:about="http://www.cidoc-crm.org/cidoc-crm/P174_starts_before_the_end_of">
	<rdf:type rdf:resource="http://www.w3.org/2002/07/owl#ObjectProperty"/>
	<rdfs:subPropertyOf rdf:resource="http://www.cidoc-crm.org/cidoc-crm/P173_starts_before_or_with_the_end_of"/>
	<owl:inverseOf rdf:resource="http://www.cidoc-crm.org/cidoc-crm/P174i_ends_after_the_start_of"/>
	<rdfs:domain rdf:resource="http://www.cidoc-crm.org/cidoc-crm/E2_Temporal_Entity"/>
	<rdfs:range rdf:resource="http://www.cidoc-crm.org/cidoc-crm/E2_Temporal_Entity"/>
	<rdfs:comment xml:lang="en">This property specifies that the temporal extent of the domain instance A of E2 Temporal Entity starts definitely before the end of the temporal extent of the range instance B of E2 Temporal Entity.
In other words, if A = [A-start, A-end] and B = [B-start, B-end], it means A-start &amp;lt; B-end is true.
This property is part of the set of temporal primitives P173 – P176, P182 – P185.
This property corresponds to a disjunction (logical OR) of the following Allen temporal relations (Allen, 1983): {before, meets, overlaps, starts, started-by, contains, finishes, finished-by, equals, during, overlapped by}
Typically, this property is a consequence of a known influence of some event on another event or activity, such as a novel written by someone being continued by someone else, or the knowledge of a defeat on a distant battlefield causing people to end their ongoing activities. This property is not transitive. This property is irreflexive.

Figure 10: Temporal entity A starts before the end of temporal entity B. Here A is longer than B

Figure 11: Temporal entity A starts before the end of temporal entity B. Here A is shorter than B</rdfs:comment>
	<rdfs:label xml:lang="fr">commence avant la fin de</rdfs:label>
	<rdfs:label xml:lang="en">starts before the end of</rdfs:label>
</rdf:Description>

<rdf:Description rdf:about="http://www.cidoc-crm.org/cidoc-crm/P174i_ends_after_the_start_of">
	<rdf:type rdf:resource="http://www.w3.org/2002/07/owl#ObjectProperty"/>
	<rdfs:subPropertyOf rdf:resource="http://www.cidoc-crm.org/cidoc-crm/P173i_ends_after_or_with_the_start_of"/>
	<rdfs:domain rdf:resource="http://www.cidoc-crm.org/cidoc-crm/E2_Temporal_Entity"/>
	<rdfs:range rdf:resource="http://www.cidoc-crm.org/cidoc-crm/E2_Temporal_Entity"/>
	<rdfs:label xml:lang="en">ends after the start of</rdfs:label>
	<rdfs:label xml:lang="fr">se termine après le début de</rdfs:label>
</rdf:Description>

<rdf:Description rdf:about="http://www.cidoc-crm.org/cidoc-crm/P175_starts_before_or_with_the_start_of">
	<rdf:type rdf:resource="http://www.w3.org/2002/07/owl#ObjectProperty"/>
	<rdfs:subPropertyOf rdf:resource="http://www.cidoc-crm.org/cidoc-crm/P174_starts_before_the_end_of"/>
	<owl:inverseOf rdf:resource="http://www.cidoc-crm.org/cidoc-crm/P175i_starts_after_or_with_the_start_of"/>
	<rdfs:domain rdf:resource="http://www.cidoc-crm.org/cidoc-crm/E2_Temporal_Entity"/>
	<rdfs:range rdf:resource="http://www.cidoc-crm.org/cidoc-crm/E2_Temporal_Entity"/>
	<rdfs:comment xml:lang="en">This property specifies that the temporal extent of the domain instance A of E2 Temporal Entity starts before or simultaneously with the start of the temporal extent of the range instance B of E2 Temporal Entity.
In other words, if A = [A-start, A-end] and B = [B-start, B-end], it means A-start ≤ B-start is true.
This property is part of the set of temporal primitives P173 – P176, P182 – P185.
This property corresponds to a disjunction (logical OR) of the following Allen temporal relations (Allen, 1983): {before, meets, overlaps, starts, started-by, contains, finished-by, equals}
In a model with fuzzy borders, this property will not be transitive.
This property is irreflexive.

Figure 12: Temporal entity A starts before or with the start of temporal entity B. Here A is longer than B

Figure 13: Temporal entity A starts before or with the start of temporal entity B. Here A is shorter than B</rdfs:comment>
	<rdfs:label xml:lang="fr">commence avant ou au moment du début de</rdfs:label>
	<rdfs:label xml:lang="en">starts before or with the start of</rdfs:label>
</rdf:Description>

<rdf:Description rdf:about="http://www.cidoc-crm.org/cidoc-crm/P175i_starts_after_or_with_the_start_of">
	<rdf:type rdf:resource="http://www.w3.org/2002/07/owl#ObjectProperty"/>
	<rdfs:subPropertyOf rdf:resource="http://www.cidoc-crm.org/cidoc-crm/P174i_ends_after_the_start_of"/>
	<rdfs:domain rdf:resource="http://www.cidoc-crm.org/cidoc-crm/E2_Temporal_Entity"/>
	<rdfs:range rdf:resource="http://www.cidoc-crm.org/cidoc-crm/E2_Temporal_Entity"/>
	<rdfs:label xml:lang="fr">commence après ou au moment du début de</rdfs:label>
	<rdfs:label xml:lang="en">starts after or with the start of</rdfs:label>
</rdf:Description>

<rdf:Description rdf:about="http://www.cidoc-crm.org/cidoc-crm/P176_starts_before_the_start_of">
	<rdf:type rdf:resource="http://www.w3.org/2002/07/owl#ObjectProperty"/>
	<rdfs:subPropertyOf rdf:resource="http://www.cidoc-crm.org/cidoc-crm/P175_starts_before_or_with_the_start_of"/>
	<owl:inverseOf rdf:resource="http://www.cidoc-crm.org/cidoc-crm/P176i_starts_after_the_start_of"/>
	<rdfs:domain rdf:resource="http://www.cidoc-crm.org/cidoc-crm/E2_Temporal_Entity"/>
	<rdfs:range rdf:resource="http://www.cidoc-crm.org/cidoc-crm/E2_Temporal_Entity"/>
	<rdfs:comment xml:lang="en">This property specifies that the temporal extent of the domain instance A of E2 Temporal Entity starts definitely before the start of the temporal extent of the range instance B of E2 Temporal Entity.
In other words, if A = [A-start, A-end] and B = [B-start, B-end], it means A-start &amp;lt; B-start is true.
This property is part of the set of temporal primitives P173 – P176, P182 – P185.
This property corresponds to a disjunction (logical OR) of the following Allen temporal relations (Allen, 1983): {before, meets, overlaps, contains, finished-by}. This property is transitive. This property is asymmetric.

Figure 14: Temporal entity A starts before the start of temporal entity B. Here A is longer than B

Figure 15: Temporal entity A starts before the start of temporal entity B. Here A is shorter than B</rdfs:comment>
	<rdfs:label xml:lang="fr">commence avant le début de</rdfs:label>
	<rdfs:label xml:lang="en">starts before the start of</rdfs:label>
</rdf:Description>

<rdf:Description rdf:about="http://www.cidoc-crm.org/cidoc-crm/P176i_starts_after_the_start_of">
	<rdf:type rdf:resource="http://www.w3.org/2002/07/owl#ObjectProperty"/>
	<rdfs:subPropertyOf rdf:resource="http://www.cidoc-crm.org/cidoc-crm/P175i_starts_after_or_with_the_start_of"/>
	<rdfs:domain rdf:resource="http://www.cidoc-crm.org/cidoc-crm/E2_Temporal_Entity"/>
	<rdfs:range rdf:resource="http://www.cidoc-crm.org/cidoc-crm/E2_Temporal_Entity"/>
	<rdfs:label xml:lang="fr">commence après le début de</rdfs:label>
	<rdfs:label xml:lang="en">starts after the start of</rdfs:label>
</rdf:Description>

<rdf:Description rdf:about="http://www.cidoc-crm.org/cidoc-crm/P177_assigned_property_of_type">
	<rdf:type rdf:resource="http://www.w3.org/2002/07/owl#ObjectProperty"/>
	<rdfs:subPropertyOf rdf:resource="http://www.cidoc-crm.org/cidoc-crm/P2_has_type"/>
	<owl:inverseOf rdf:resource="http://www.cidoc-crm.org/cidoc-crm/P177i_is_type_of_property_assigned"/>
	<rdfs:domain rdf:resource="http://www.cidoc-crm.org/cidoc-crm/E13_Attribute_Assignment"/>
	<rdfs:range rdf:resource="http://www.cidoc-crm.org/cidoc-crm/E55_Type"/>
	<rdfs:comment xml:lang="en">This property associates an instance of E13 Attribute Assignment with the type of property or relation that this assignment maintains to hold between the item to which it assigns an attribute and the attribute itself. Note that the properties defined by the CIDOC CRM also constitute instances of E55 Type themselves. The direction of the assigned property of type is understood to be from the attributed item (the range of property P140 assigned attribute to) to the attribute item (the range of the property P141 assigned). More than one property type may be assigned to hold between two items.
A comprehensive explanation about refining CIDOC CRM concepts by E55 Type is given in the section “About Types” in the section on “Specific Modelling Constructs” of this document.</rdfs:comment>
	<rdfs:label xml:lang="fr">a assigné le type de propriété</rdfs:label>
	<rdfs:label xml:lang="en">assigned property of type</rdfs:label>
</rdf:Description>

<rdf:Description rdf:about="http://www.cidoc-crm.org/cidoc-crm/P177i_is_type_of_property_assigned">
	<rdf:type rdf:resource="http://www.w3.org/2002/07/owl#ObjectProperty"/>
	<rdfs:subPropertyOf rdf:resource="http://www.cidoc-crm.org/cidoc-crm/P2i_is_type_of"/>
	<rdfs:domain rdf:resource="http://www.cidoc-crm.org/cidoc-crm/E55_Type"/>
	<rdfs:range rdf:resource="http://www.cidoc-crm.org/cidoc-crm/E13_Attribute_Assignment"/>
	<rdfs:label xml:lang="fr">est le type de propriété assigné</rdfs:label>
	<rdfs:label xml:lang="en">is type of property assigned</rdfs:label>
</rdf:Description>

<rdf:Description rdf:about="http://www.cidoc-crm.org/cidoc-crm/P179_had_sales_price">
	<rdf:type rdf:resource="http://www.w3.org/2002/07/owl#ObjectProperty"/>
	<owl:inverseOf rdf:resource="http://www.cidoc-crm.org/cidoc-crm/P179i_was_sales_price_of"/>
	<rdfs:domain rdf:resource="http://www.cidoc-crm.org/cidoc-crm/E96_Purchase"/>
	<rdfs:range rdf:resource="http://www.cidoc-crm.org/cidoc-crm/E97_Monetary_Amount"/>
	<rdfs:comment xml:lang="en">This property establishes the relationship between an instance of E96 Purchase and the instance of E97 Monetary Amount that forms the compensation for the transaction. The monetary amount agreed upon may change in the course of the purchase activity.</rdfs:comment>
	<rdfs:label xml:lang="fr">a eu pour prix de vente</rdfs:label>
	<rdfs:label xml:lang="en">had sales price</rdfs:label>
</rdf:Description>

<rdf:Description rdf:about="http://www.cidoc-crm.org/cidoc-crm/P179i_was_sales_price_of">
	<rdf:type rdf:resource="http://www.w3.org/2002/07/owl#ObjectProperty"/>
	<rdfs:domain rdf:resource="http://www.cidoc-crm.org/cidoc-crm/E97_Monetary_Amount"/>
	<rdfs:range rdf:resource="http://www.cidoc-crm.org/cidoc-crm/E96_Purchase"/>
	<rdfs:label xml:lang="fr">a été le prix de vente de</rdfs:label>
	<rdfs:label xml:lang="en">was sales price of</rdfs:label>
</rdf:Description>

<rdf:Description rdf:about="http://www.cidoc-crm.org/cidoc-crm/P17_was_motivated_by">
	<rdf:type rdf:resource="http://www.w3.org/2002/07/owl#ObjectProperty"/>
	<rdfs:subPropertyOf rdf:resource="http://www.cidoc-crm.org/cidoc-crm/P15_was_influenced_by"/>
	<owl:inverseOf rdf:resource="http://www.cidoc-crm.org/cidoc-crm/P17i_motivated"/>
	<rdfs:domain rdf:resource="http://www.cidoc-crm.org/cidoc-crm/E7_Activity"/>
	<rdfs:range rdf:resource="http://www.cidoc-crm.org/cidoc-crm/E1_CRM_Entity"/>
	<rdfs:comment xml:lang="en">This property describes an item or items that are regarded as a reason for carrying out the instance of E7 Activity.
For example, the discovery of a large hoard of treasure may call for a celebration, an order from headquarters can start a military manoeuvre.</rdfs:comment>
	<rdfs:label xml:lang="fr">a été motivé par</rdfs:label>
	<rdfs:label xml:lang="pt">foi motivado por</rdfs:label>
	<rdfs:label xml:lang="en">was motivated by</rdfs:label>
	<rdfs:label xml:lang="de">wurde angeregt durch</rdfs:label>
	<rdfs:label xml:lang="el">είχε ως αφορμή</rdfs:label>
	<rdfs:label xml:lang="ru">был обусловлен посредством</rdfs:label>
	<rdfs:label xml:lang="zh">被促动</rdfs:label>
</rdf:Description>

<rdf:Description rdf:about="http://www.cidoc-crm.org/cidoc-crm/P17i_motivated">
	<rdf:type rdf:resource="http://www.w3.org/2002/07/owl#ObjectProperty"/>
	<rdfs:subPropertyOf rdf:resource="http://www.cidoc-crm.org/cidoc-crm/P15i_influenced"/>
	<rdfs:domain rdf:resource="http://www.cidoc-crm.org/cidoc-crm/E1_CRM_Entity"/>
	<rdfs:range rdf:resource="http://www.cidoc-crm.org/cidoc-crm/E7_Activity"/>
	<rdfs:label xml:lang="fr">a motivé</rdfs:label>
	<rdfs:label xml:lang="en">motivated</rdfs:label>
	<rdfs:label xml:lang="pt">motivou</rdfs:label>
	<rdfs:label xml:lang="de">regte an</rdfs:label>
	<rdfs:label xml:lang="el">ήταν αφορμή</rdfs:label>
	<rdfs:label xml:lang="ru">обусловил</rdfs:label>
	<rdfs:label xml:lang="zh">促动</rdfs:label>
</rdf:Description>

<rdf:Description rdf:about="http://www.cidoc-crm.org/cidoc-crm/P180_has_currency">
	<rdf:type rdf:resource="http://www.w3.org/2002/07/owl#ObjectProperty"/>
	<rdfs:subPropertyOf rdf:resource="http://www.cidoc-crm.org/cidoc-crm/P91_has_unit"/>
	<owl:inverseOf rdf:resource="http://www.cidoc-crm.org/cidoc-crm/P180i_was_currency_of"/>
	<rdfs:domain rdf:resource="http://www.cidoc-crm.org/cidoc-crm/E97_Monetary_Amount"/>
	<rdfs:range rdf:resource="http://www.cidoc-crm.org/cidoc-crm/E98_Currency"/>
	<rdfs:comment xml:lang="en">This property establishes the relationship between an instance of E97 Monetary Amount and the instance of E98 Currency that it is measured in.</rdfs:comment>
	<rdfs:label xml:lang="fr">a pour unité monétaire</rdfs:label>
	<rdfs:label xml:lang="en">has currency</rdfs:label>
</rdf:Description>

<rdf:Description rdf:about="http://www.cidoc-crm.org/cidoc-crm/P180i_was_currency_of">
	<rdf:type rdf:resource="http://www.w3.org/2002/07/owl#ObjectProperty"/>
	<rdfs:subPropertyOf rdf:resource="http://www.cidoc-crm.org/cidoc-crm/P91i_is_unit_of"/>
	<rdfs:domain rdf:resource="http://www.cidoc-crm.org/cidoc-crm/E98_Currency"/>
	<rdfs:range rdf:resource="http://www.cidoc-crm.org/cidoc-crm/E97_Monetary_Amount"/>
	<rdfs:label xml:lang="en">was currency of</rdfs:label>
	<rdfs:label xml:lang="fr">était l’unité monétaire de</rdfs:label>
</rdf:Description>

<rdf:Description rdf:about="http://www.cidoc-crm.org/cidoc-crm/P182_ends_before_or_with_the_start_of">
	<rdf:type rdf:resource="http://www.w3.org/2002/07/owl#ObjectProperty"/>
	<rdfs:subPropertyOf rdf:resource="http://www.cidoc-crm.org/cidoc-crm/P176_starts_before_the_start_of"/>
	<rdfs:subPropertyOf rdf:resource="http://www.cidoc-crm.org/cidoc-crm/P185_ends_before_the_end_of"/>
	<owl:inverseOf rdf:resource="http://www.cidoc-crm.org/cidoc-crm/P182i_starts_after_or_with_the_end_of"/>
	<rdfs:domain rdf:resource="http://www.cidoc-crm.org/cidoc-crm/E2_Temporal_Entity"/>
	<rdfs:range rdf:resource="http://www.cidoc-crm.org/cidoc-crm/E2_Temporal_Entity"/>
	<rdfs:comment xml:lang="en">This property specifies that the temporal extent of the domain instance A of E2 Temporal Entity ends before or simultaneously with the start of the temporal extent of the range instance B of E2 Temporal Entity.
In other words, if A = [A-start, A-end] and B = [B-start, B-end], it means A-end ≤ B-start is true.
This property is part of the set of temporal primitives P173 – P176, P182 – P185.
This property corresponds to a disjunction (logical OR) of the following Allen temporal relations (Allen, 1983): {before, meets}.
This property is transitive. This property is asymmetric.

Figure 16: Temporal entity A ends before or with the start of temporal entity B. Here A is longer than B

Figure 17: Temporal entity A ends before or with the start of temporal entity B. Here A is shorter than B</rdfs:comment>
	<rdfs:label xml:lang="en">ends before or with the start of</rdfs:label>
	<rdfs:label xml:lang="fr">se termine avant ou au moment du début de</rdfs:label>
</rdf:Description>

<rdf:Description rdf:about="http://www.cidoc-crm.org/cidoc-crm/P182i_starts_after_or_with_the_end_of">
	<rdf:type rdf:resource="http://www.w3.org/2002/07/owl#ObjectProperty"/>
	<rdfs:subPropertyOf rdf:resource="http://www.cidoc-crm.org/cidoc-crm/P176i_starts_after_the_start_of"/>
	<rdfs:subPropertyOf rdf:resource="http://www.cidoc-crm.org/cidoc-crm/P185i_ends_after_the_end_of"/>
	<rdfs:domain rdf:resource="http://www.cidoc-crm.org/cidoc-crm/E2_Temporal_Entity"/>
	<rdfs:range rdf:resource="http://www.cidoc-crm.org/cidoc-crm/E2_Temporal_Entity"/>
	<rdfs:label xml:lang="fr">commence après ou au moment de la fin de</rdfs:label>
	<rdfs:label xml:lang="en">starts after or with the end of</rdfs:label>
</rdf:Description>

<rdf:Description rdf:about="http://www.cidoc-crm.org/cidoc-crm/P183_ends_before_the_start_of">
	<rdf:type rdf:resource="http://www.w3.org/2002/07/owl#ObjectProperty"/>
	<rdfs:subPropertyOf rdf:resource="http://www.cidoc-crm.org/cidoc-crm/P182_ends_before_or_with_the_start_of"/>
	<owl:inverseOf rdf:resource="http://www.cidoc-crm.org/cidoc-crm/P183i_starts_after_the_end_of"/>
	<rdfs:domain rdf:resource="http://www.cidoc-crm.org/cidoc-crm/E2_Temporal_Entity"/>
	<rdfs:range rdf:resource="http://www.cidoc-crm.org/cidoc-crm/E2_Temporal_Entity"/>
	<rdfs:comment xml:lang="en">This property specifies that the temporal extent of the domain instance A of E2 Temporal Entity ends definitely before the start of the temporal extent of the range instance B of E2 Temporal Entity.
In other words, if A = [A-start, A-end] and B = [B-start, B-end], it means A-end &amp;lt; B-start is true.
This property is part of the set of temporal primitives P173 – P176, P182 – P185.
This property corresponds to the following Allen temporal relation (Allen, 1983) : {before}.
This property is transitive. This property is asymmetric.

Figure 18: Temporal entity A ends before the start of temporal entity B. Here A is longer than B

Figure 19: Temporal entity A ends before the start of temporal entity B. Here A is shorter than B</rdfs:comment>
	<rdfs:label xml:lang="en">ends before the start of</rdfs:label>
	<rdfs:label xml:lang="fr">se termine avant le début de</rdfs:label>
</rdf:Description>

<rdf:Description rdf:about="http://www.cidoc-crm.org/cidoc-crm/P183i_starts_after_the_end_of">
	<rdf:type rdf:resource="http://www.w3.org/2002/07/owl#ObjectProperty"/>
	<rdfs:subPropertyOf rdf:resource="http://www.cidoc-crm.org/cidoc-crm/P182i_starts_after_or_with_the_end_of"/>
	<rdfs:domain rdf:resource="http://www.cidoc-crm.org/cidoc-crm/E2_Temporal_Entity"/>
	<rdfs:range rdf:resource="http://www.cidoc-crm.org/cidoc-crm/E2_Temporal_Entity"/>
	<rdfs:label xml:lang="fr">commence après la fin de</rdfs:label>
	<rdfs:label xml:lang="en">starts after the end of</rdfs:label>
</rdf:Description>

<rdf:Description rdf:about="http://www.cidoc-crm.org/cidoc-crm/P184_ends_before_or_with_the_end_of">
	<rdf:type rdf:resource="http://www.w3.org/2002/07/owl#ObjectProperty"/>
	<rdfs:subPropertyOf rdf:resource="http://www.cidoc-crm.org/cidoc-crm/P174_starts_before_the_end_of"/>
	<owl:inverseOf rdf:resource="http://www.cidoc-crm.org/cidoc-crm/P184i_ends_with_or_after_the_end_of"/>
	<rdfs:domain rdf:resource="http://www.cidoc-crm.org/cidoc-crm/E2_Temporal_Entity"/>
	<rdfs:range rdf:resource="http://www.cidoc-crm.org/cidoc-crm/E2_Temporal_Entity"/>
	<rdfs:comment xml:lang="en">This property specifies that the temporal extent of the domain instance A of E2 Temporal Entity ends before or simultaneously with the end of the temporal extent of the range instance B of E2 Temporal Entity.
In other words, if A = [A-start, A-end] and B = [B-start, B-end], it means A-end ≤ B-end is true.
This property is part of the set of temporal primitives P173 – P176, P182 – P185.
This property corresponds to a disjunction (logical OR) of the following Allen temporal relations (Allen, 1983): {before, meets, overlaps, finished by, start, equals, during, finishes}.
This property is irreflexive

Figure 20: Temporal entity A ends before or with the end of temporal entity B. Here A is longer than B

Figure 21: Temporal entity A ends before or with the end of temporal entity B. Here A is shorter than B</rdfs:comment>
	<rdfs:label xml:lang="en">ends before or with the end of</rdfs:label>
	<rdfs:label xml:lang="fr">se termine avant ou au moment de la fin de</rdfs:label>
</rdf:Description>

<rdf:Description rdf:about="http://www.cidoc-crm.org/cidoc-crm/P184i_ends_with_or_after_the_end_of">
	<rdf:type rdf:resource="http://www.w3.org/2002/07/owl#ObjectProperty"/>
	<rdfs:subPropertyOf rdf:resource="http://www.cidoc-crm.org/cidoc-crm/P174i_ends_after_the_start_of"/>
	<rdfs:domain rdf:resource="http://www.cidoc-crm.org/cidoc-crm/E2_Temporal_Entity"/>
	<rdfs:range rdf:resource="http://www.cidoc-crm.org/cidoc-crm/E2_Temporal_Entity"/>
	<rdfs:label xml:lang="en">ends with or after the end of</rdfs:label>
	<rdfs:label xml:lang="fr">se termine au moment de ou après la fin de</rdfs:label>
</rdf:Description>

<rdf:Description rdf:about="http://www.cidoc-crm.org/cidoc-crm/P185_ends_before_the_end_of">
	<rdf:type rdf:resource="http://www.w3.org/2002/07/owl#ObjectProperty"/>
	<rdfs:subPropertyOf rdf:resource="http://www.cidoc-crm.org/cidoc-crm/P184_ends_before_or_with_the_end_of"/>
	<owl:inverseOf rdf:resource="http://www.cidoc-crm.org/cidoc-crm/P185i_ends_after_the_end_of"/>
	<rdfs:domain rdf:resource="http://www.cidoc-crm.org/cidoc-crm/E2_Temporal_Entity"/>
	<rdfs:range rdf:resource="http://www.cidoc-crm.org/cidoc-crm/E2_Temporal_Entity"/>
	<rdfs:comment xml:lang="en">This property specifies that the temporal extent of the domain instance A of E2 Temporal Entity ends definitely before the end of the temporal extent of the range instance B of E2 Temporal Entity.
In other words, if A = [A-start, A-end] and B = [B-start, B-end], it means A-end &amp;lt; B-end is true.
This property is part of the set of temporal primitives P173 – P176, P182 – P185.
This property corresponds to a disjunction (logical OR) of the following Allen temporal relations (Allen, 1983): {before, meets, overlaps, starts, during}.
This property is transitive. This property is asymmetric.

Figure 22: Temporal entity A ends before the end of temporal entity B. Here A is longer than B

Figure 23: Temporal entity A ends before the end of temporal entity B. Here A is shorter than B</rdfs:comment>
	<rdfs:label xml:lang="en">ends before the end of</rdfs:label>
	<rdfs:label xml:lang="fr">se termine avant la fin de</rdfs:label>
</rdf:Description>

<rdf:Description rdf:about="http://www.cidoc-crm.org/cidoc-crm/P185i_ends_after_the_end_of">
	<rdf:type rdf:resource="http://www.w3.org/2002/07/owl#ObjectProperty"/>
	<rdfs:subPropertyOf rdf:resource="http://www.cidoc-crm.org/cidoc-crm/P184i_ends_with_or_after_the_end_of"/>
	<rdfs:domain rdf:resource="http://www.cidoc-crm.org/cidoc-crm/E2_Temporal_Entity"/>
	<rdfs:range rdf:resource="http://www.cidoc-crm.org/cidoc-crm/E2_Temporal_Entity"/>
	<rdfs:label xml:lang="en">ends after the end of</rdfs:label>
	<rdfs:label xml:lang="fr">se termine après la fin de</rdfs:label>
</rdf:Description>

<rdf:Description rdf:about="http://www.cidoc-crm.org/cidoc-crm/P186_produced_thing_of_product_type">
	<rdf:type rdf:resource="http://www.w3.org/2002/07/owl#ObjectProperty"/>
	<owl:inverseOf rdf:resource="http://www.cidoc-crm.org/cidoc-crm/P186i_is_produced_by"/>
	<rdfs:domain rdf:resource="http://www.cidoc-crm.org/cidoc-crm/E12_Production"/>
	<rdfs:range rdf:resource="http://www.cidoc-crm.org/cidoc-crm/E99_Product_Type"/>
	<rdfs:comment xml:lang="en">This property associates an instance of E12 Production with the instance of E99 Production Type, that is, the type of the things it produces.</rdfs:comment>
	<rdfs:label xml:lang="fr">a produit la chose du type</rdfs:label>
	<rdfs:label xml:lang="en">produced thing of product type</rdfs:label>
</rdf:Description>

<rdf:Description rdf:about="http://www.cidoc-crm.org/cidoc-crm/P186i_is_produced_by">
	<rdf:type rdf:resource="http://www.w3.org/2002/07/owl#ObjectProperty"/>
	<rdfs:domain rdf:resource="http://www.cidoc-crm.org/cidoc-crm/E99_Product_Type"/>
	<rdfs:range rdf:resource="http://www.cidoc-crm.org/cidoc-crm/E12_Production"/>
	<rdfs:label xml:lang="fr">est produit par</rdfs:label>
	<rdfs:label xml:lang="en">is produced by</rdfs:label>
</rdf:Description>

<rdf:Description rdf:about="http://www.cidoc-crm.org/cidoc-crm/P187_has_production_plan">
	<rdf:type rdf:resource="http://www.w3.org/2002/07/owl#ObjectProperty"/>
	<owl:inverseOf rdf:resource="http://www.cidoc-crm.org/cidoc-crm/P187i_is_production_plan_for"/>
	<rdfs:domain rdf:resource="http://www.cidoc-crm.org/cidoc-crm/E99_Product_Type"/>
	<rdfs:range rdf:resource="http://www.cidoc-crm.org/cidoc-crm/E29_Design_or_Procedure"/>
	<rdfs:comment xml:lang="en">This property associates an instance of E99 Product Type with an instance of E29 Design or Procedure that completely determines the production of instances of E18 Physical Thing. The resulting instances of E18 Physical Thing are considered exemplars of this instance of E99 Product Type when the process specified is correctly executed. Note that the respective instance of E29 Design or Procedure may not necessarily be fixed in a written/graphical form, and may require the use of tools or models unique to the product type. The same instance of E99 Product Type may be associated with several variant plans.</rdfs:comment>
	<rdfs:label xml:lang="fr">a pour plan de production</rdfs:label>
	<rdfs:label xml:lang="en">has production plan</rdfs:label>
</rdf:Description>

<rdf:Description rdf:about="http://www.cidoc-crm.org/cidoc-crm/P187i_is_production_plan_for">
	<rdf:type rdf:resource="http://www.w3.org/2002/07/owl#ObjectProperty"/>
	<rdfs:domain rdf:resource="http://www.cidoc-crm.org/cidoc-crm/E29_Design_or_Procedure"/>
	<rdfs:range rdf:resource="http://www.cidoc-crm.org/cidoc-crm/E99_Product_Type"/>
	<rdfs:label xml:lang="fr">est le plan de production de</rdfs:label>
	<rdfs:label xml:lang="en">is production plan for</rdfs:label>
</rdf:Description>

<rdf:Description rdf:about="http://www.cidoc-crm.org/cidoc-crm/P188_requires_production_tool">
	<rdf:type rdf:resource="http://www.w3.org/2002/07/owl#ObjectProperty"/>
	<owl:inverseOf rdf:resource="http://www.cidoc-crm.org/cidoc-crm/P188i_is_production_tool_for"/>
	<rdfs:domain rdf:resource="http://www.cidoc-crm.org/cidoc-crm/E99_Product_Type"/>
	<rdfs:range rdf:resource="http://www.cidoc-crm.org/cidoc-crm/E19_Physical_Object"/>
	<rdfs:comment xml:lang="en">This property associates an instance of E99 Product Type with an instance of E19 Physical Object that is needed for the production of an instance of E18 Physical Thing. When the process of production is correctly executed in accordance with the plan and using the specified instance of E19 Physical Object, the resulting instance of E18 Physical Thing is considered an exemplar of this instance of E99 Product Type. The instance of E19 Physical Object may bear distinct features that are transformed into characteristic features of the resulting instance of E18 Physical Thing. Examples include models and moulds.</rdfs:comment>
	<rdfs:label xml:lang="fr">nécessite l'outil</rdfs:label>
	<rdfs:label xml:lang="en">requires production tool</rdfs:label>
</rdf:Description>

<rdf:Description rdf:about="http://www.cidoc-crm.org/cidoc-crm/P188i_is_production_tool_for">
	<rdf:type rdf:resource="http://www.w3.org/2002/07/owl#ObjectProperty"/>
	<rdfs:domain rdf:resource="http://www.cidoc-crm.org/cidoc-crm/E19_Physical_Object"/>
	<rdfs:range rdf:resource="http://www.cidoc-crm.org/cidoc-crm/E99_Product_Type"/>
	<rdfs:label xml:lang="fr">est l'outil de production de</rdfs:label>
	<rdfs:label xml:lang="en">is production tool for</rdfs:label>
</rdf:Description>

<rdf:Description rdf:about="http://www.cidoc-crm.org/cidoc-crm/P189_approximates">
	<rdf:type rdf:resource="http://www.w3.org/2002/07/owl#ObjectProperty"/>
	<owl:inverseOf rdf:resource="http://www.cidoc-crm.org/cidoc-crm/P189i_is_approximated_by"/>
	<rdfs:domain rdf:resource="http://www.cidoc-crm.org/cidoc-crm/E53_Place"/>
	<rdfs:range rdf:resource="http://www.cidoc-crm.org/cidoc-crm/E53_Place"/>
	<rdfs:comment xml:lang="en">This property associates an instance of E53 Place with another instance of E53 Place, which is defined in the same reference space, and which is used to approximate the former. The property does not necessarily state the quality or accuracy of this approximation, but rather indicates the use of the first instance of place to approximate the second.
In common documentation practice, find or encounter spots e.g. in archaeology, botany or zoology are often related to the closest village, river or other named place without detailing the relation, e.g. if it is located within the village or in a certain distance of the specified place. In this case the stated “phenomenal” place found in the documentation can be seen as an approximation of the actual encounter spot without more specific knowledge.
In more recent documentation often point coordinate information is provided that originates from GPS measurements or georeferencing from a map. This point coordinate information does not state the actual place of the encounter spot but tries to approximate it with a “declarative” place. The accuracy depends on the methodology used when creating the coordinates. It may be dependent on technical limitations like GPS accuracy but also on the method where the GPS location is taken in relation to the measured feature. If the methodology is known a maximum deviation from the measured point can be calculated and the encounter spot or feature may be related to the resulting circle using an instance of P171 at some place within.
This property is not transitive. This property is reflexive.</rdfs:comment>
	<rdfs:label xml:lang="en">approximates</rdfs:label>
	<rdfs:label xml:lang="fr">approxime</rdfs:label>
</rdf:Description>

<rdf:Description rdf:about="http://www.cidoc-crm.org/cidoc-crm/P189i_is_approximated_by">
	<rdf:type rdf:resource="http://www.w3.org/2002/07/owl#ObjectProperty"/>
	<rdfs:domain rdf:resource="http://www.cidoc-crm.org/cidoc-crm/E53_Place"/>
	<rdfs:range rdf:resource="http://www.cidoc-crm.org/cidoc-crm/E53_Place"/>
	<rdfs:label xml:lang="fr">est approximé par</rdfs:label>
	<rdfs:label xml:lang="en">is approximated by</rdfs:label>
</rdf:Description>

<rdf:Description rdf:about="http://www.cidoc-crm.org/cidoc-crm/P191_had_duration">
	<rdf:type rdf:resource="http://www.w3.org/2002/07/owl#ObjectProperty"/>
	<owl:inverseOf rdf:resource="http://www.cidoc-crm.org/cidoc-crm/P191i_was_duration_of"/>
	<rdfs:domain rdf:resource="http://www.cidoc-crm.org/cidoc-crm/E52_Time-Span"/>
	<rdfs:range rdf:resource="http://www.cidoc-crm.org/cidoc-crm/E54_Dimension"/>
	<rdfs:comment xml:lang="en">This property describes the length of time covered by an instance of E52 Time-Span. It allows an instance of E52 Time-Span to be associated with an instance of E54 Dimension representing duration independent from the actual beginning and end. Indeterminacy of the duration value can be expressed by assigning a numerical interval to the property P90 has value of E54 Dimension.</rdfs:comment>
	<rdfs:label xml:lang="fr">a eu pour durée</rdfs:label>
	<rdfs:label xml:lang="en">had duration</rdfs:label>
</rdf:Description>

<rdf:Description rdf:about="http://www.cidoc-crm.org/cidoc-crm/P191i_was_duration_of">
	<rdf:type rdf:resource="http://www.w3.org/2002/07/owl#ObjectProperty"/>
	<rdfs:domain rdf:resource="http://www.cidoc-crm.org/cidoc-crm/E54_Dimension"/>
	<rdfs:range rdf:resource="http://www.cidoc-crm.org/cidoc-crm/E52_Time-Span"/>
	<rdfs:label xml:lang="en">was duration of</rdfs:label>
	<rdfs:label xml:lang="fr">était la durée de</rdfs:label>
</rdf:Description>

<rdf:Description rdf:about="http://www.cidoc-crm.org/cidoc-crm/P195_was_a_presence_of">
	<rdf:type rdf:resource="http://www.w3.org/2002/07/owl#ObjectProperty"/>
	<owl:inverseOf rdf:resource="http://www.cidoc-crm.org/cidoc-crm/P195i_had_presence"/>
	<rdfs:domain rdf:resource="http://www.cidoc-crm.org/cidoc-crm/E93_Presence"/>
	<rdfs:range rdf:resource="http://www.cidoc-crm.org/cidoc-crm/E18_Physical_Thing"/>
	<rdfs:comment xml:lang="en">This property associates an instance of E93 Presence with the instance of E18 Physical Thing of which it represents a temporal restriction (i.e. a time-slice) of the thing’s trajectory through spacetime. In other words, it describes where the instance of E18 Physical Thing was or moved around within a given time-span. Instantiating this property constitutes a necessary part of the identity of the respective instance of E93 Presence.
This property is a shortcut of the fully developed path from E18 Physical Thing through P196 defines, E92 Spacetime Volume, P166 was a presence of (had presence) to E93 Presence.</rdfs:comment>
	<rdfs:label xml:lang="fr">a été une présence de</rdfs:label>
	<rdfs:label xml:lang="en">was a presence of</rdfs:label>
</rdf:Description>

<rdf:Description rdf:about="http://www.cidoc-crm.org/cidoc-crm/P195i_had_presence">
	<rdf:type rdf:resource="http://www.w3.org/2002/07/owl#ObjectProperty"/>
	<rdfs:domain rdf:resource="http://www.cidoc-crm.org/cidoc-crm/E18_Physical_Thing"/>
	<rdfs:range rdf:resource="http://www.cidoc-crm.org/cidoc-crm/E93_Presence"/>
	<rdfs:label xml:lang="fr">a eu pour présence</rdfs:label>
	<rdfs:label xml:lang="en">had presence</rdfs:label>
</rdf:Description>

<rdf:Description rdf:about="http://www.cidoc-crm.org/cidoc-crm/P196_defines">
	<rdf:type rdf:resource="http://www.w3.org/2002/07/owl#ObjectProperty"/>
	<owl:inverseOf rdf:resource="http://www.cidoc-crm.org/cidoc-crm/P196i_is_defined_by"/>
	<rdfs:domain rdf:resource="http://www.cidoc-crm.org/cidoc-crm/E18_Physical_Thing"/>
	<rdfs:range rdf:resource="http://www.cidoc-crm.org/cidoc-crm/E92_Spacetime_Volume"/>
	<rdfs:comment xml:lang="en">This property associates an instance of E18 Physical Thing with the instance of E92 Spacetime Volume that constitutes the complete trajectory of its geometric extent through spacetime for the whole time of the existence of the instance of E18 Physical Thing.
An instance of E18 Physical Thing not only occupies a particular geometric space at each instant of its existence, but in the course of its existence it also forms a trajectory through spacetime, which occupies a real, that is phenomenal, volume in spacetime, i.e. the instance of E92 Spacetime Volume this property associates it with. This real spatiotemporal extent of the instance of E18 Physical Thing is regarded as being unique, in all its details and fuzziness; the identity and existence of the instance of E92 Spacetime Volume depend uniquely on the identity of the instance of E18 Physical Thing, whose existence defines it. It constitutes a phenomenal spacetime volume as defined in CRMgeo (Doerr &amp;amp; Hiebel, 2013).
Included in this spacetime volume are both the spaces filled by the matter of the physical thing and any inner space that may exist, for instance the interior of a box. Physical things consisting of aggregations of physically unconnected objects, such as a set of chessmen, occupy a finite number of individually contiguous subsets of this spacetime volume equal to the number of objects that constitute the set and that are never connected during its existence.</rdfs:comment>
	<rdfs:label xml:lang="en">defines</rdfs:label>
	<rdfs:label xml:lang="fr">définit</rdfs:label>
</rdf:Description>

<rdf:Description rdf:about="http://www.cidoc-crm.org/cidoc-crm/P196i_is_defined_by">
	<rdf:type rdf:resource="http://www.w3.org/2002/07/owl#ObjectProperty"/>
	<rdfs:domain rdf:resource="http://www.cidoc-crm.org/cidoc-crm/E92_Spacetime_Volume"/>
	<rdfs:range rdf:resource="http://www.cidoc-crm.org/cidoc-crm/E18_Physical_Thing"/>
	<rdfs:label xml:lang="fr">est défini par</rdfs:label>
	<rdfs:label xml:lang="en">is defined by</rdfs:label>
</rdf:Description>

<rdf:Description rdf:about="http://www.cidoc-crm.org/cidoc-crm/P197_covered_parts_of">
	<rdf:type rdf:resource="http://www.w3.org/2002/07/owl#ObjectProperty"/>
	<owl:inverseOf rdf:resource="http://www.cidoc-crm.org/cidoc-crm/P197i_was_partially_covered_by"/>
	<rdfs:domain rdf:resource="http://www.cidoc-crm.org/cidoc-crm/E93_Presence"/>
	<rdfs:range rdf:resource="http://www.cidoc-crm.org/cidoc-crm/E53_Place"/>
	<rdfs:comment xml:lang="en">This property associates an instance of E93 Presence with an instance of E53 Place that geometrically overlaps with the spatial projection of the respective instance of E93 Presence. A use case of this property is to state through which places an object or an instance of E21 Person has or was moved within a given time-span. It may also be used to describe a partial or complete, temporary or permanent extension of the spatial extent of some realm into a neighbouring region during a known time-span. It may also be used to describe a partial or complete, temporary or permanent extension of the spatial extent of some realm into a neighbouring region during a known time-span.
This property is a shortcut of the more fully developed path from E93 Presence through P161 has spatial projection, E53 Place, P121 overlaps with, to E53 Place.</rdfs:comment>
	<rdfs:label xml:lang="fr">a couvert des parties de</rdfs:label>
	<rdfs:label xml:lang="en">covered parts of</rdfs:label>
</rdf:Description>

<rdf:Description rdf:about="http://www.cidoc-crm.org/cidoc-crm/P197i_was_partially_covered_by">
	<rdf:type rdf:resource="http://www.w3.org/2002/07/owl#ObjectProperty"/>
	<rdfs:domain rdf:resource="http://www.cidoc-crm.org/cidoc-crm/E53_Place"/>
	<rdfs:range rdf:resource="http://www.cidoc-crm.org/cidoc-crm/E93_Presence"/>
	<rdfs:label xml:lang="fr">a été partiellement couvert par</rdfs:label>
	<rdfs:label xml:lang="en">was partially covered by</rdfs:label>
</rdf:Description>

<rdf:Description rdf:about="http://www.cidoc-crm.org/cidoc-crm/P198_holds_or_supports">
	<rdf:type rdf:resource="http://www.w3.org/2002/07/owl#ObjectProperty"/>
	<owl:inverseOf rdf:resource="http://www.cidoc-crm.org/cidoc-crm/P198i_is_held_or_supported_by"/>
	<rdfs:domain rdf:resource="http://www.cidoc-crm.org/cidoc-crm/E18_Physical_Thing"/>
	<rdfs:range rdf:resource="http://www.cidoc-crm.org/cidoc-crm/E18_Physical_Thing"/>
	<rdfs:comment xml:lang="en">This property relates one instance of E18 Physical Thing which acts as a container or support to a supported or contained instance of E18 Physical Thing. Typical examples of E18 Physical Things which are intended to function as a container or support include shelves, folders or boxes. These containers or supports provide a stable surface which is intended for other physical objects to be placed upon for storage, display, transport or other similar functions.
This property is a shortcut of the more fully developed path from E18 Physical Thing through P59 has section, E53 Place, P53i is former or current location of, to E18 Physical Thing. It is not a sub-property of P46 is composed of, as the held or supported object is not a component of the container or support.
This property can be used to avoid explicitly instantiating the E53 Place which is defined by an instance of E18 Physical Thing, especially when the only intended use of that instance of E18 Physical Thing is to act as a container or surface for the storage of other instances of E18 Physical Thing. The place’s existence is defined by the existence of the container or surface, and will go out of existence at the same time as the destruction of the container or surface.
This property is transitive. This property is asymmetric.</rdfs:comment>
	<rdfs:label xml:lang="fr">contient ou soutient</rdfs:label>
	<rdfs:label xml:lang="en">holds or supports</rdfs:label>
</rdf:Description>

<rdf:Description rdf:about="http://www.cidoc-crm.org/cidoc-crm/P198i_is_held_or_supported_by">
	<rdf:type rdf:resource="http://www.w3.org/2002/07/owl#ObjectProperty"/>
	<rdfs:domain rdf:resource="http://www.cidoc-crm.org/cidoc-crm/E18_Physical_Thing"/>
	<rdfs:range rdf:resource="http://www.cidoc-crm.org/cidoc-crm/E18_Physical_Thing"/>
	<rdfs:label xml:lang="fr">est contenu ou soutenu par</rdfs:label>
	<rdfs:label xml:lang="en">is held or supported by</rdfs:label>
</rdf:Description>

<rdf:Description rdf:about="http://www.cidoc-crm.org/cidoc-crm/P19_was_intended_use_of">
	<rdf:type rdf:resource="http://www.w3.org/2002/07/owl#ObjectProperty"/>
	<owl:inverseOf rdf:resource="http://www.cidoc-crm.org/cidoc-crm/P19i_was_made_for"/>
	<rdfs:domain rdf:resource="http://www.cidoc-crm.org/cidoc-crm/E7_Activity"/>
	<rdfs:range rdf:resource="http://www.cidoc-crm.org/cidoc-crm/E71_Human-Made_Thing"/>
	<rdfs:comment xml:lang="en">This property relates an instance of E7 Activity with instances of E71 Human-Made Thing, created specifically for use in the activity.
This is distinct from the intended use of an item in some general type of activity such as the book of common prayer which was intended for use in Church of England services (see P101 had as general use (was use of)).</rdfs:comment>
	<rdfs:label xml:lang="fr">a été l’usage prévu de</rdfs:label>
	<rdfs:label xml:lang="pt">era prevista a utilização de</rdfs:label>
	<rdfs:label xml:lang="de">war beabsichtigteter Gebrauch von</rdfs:label>
	<rdfs:label xml:lang="en">was intended use of</rdfs:label>
	<rdfs:label xml:lang="el">ήταν προορισμένη χρήση του</rdfs:label>
	<rdfs:label xml:lang="ru">был предполагаемым использованием для</rdfs:label>
	<rdfs:label xml:lang="zh">特定用途是</rdfs:label>
</rdf:Description>

<rdf:Description rdf:about="http://www.cidoc-crm.org/cidoc-crm/P19i_was_made_for">
	<rdf:type rdf:resource="http://www.w3.org/2002/07/owl#ObjectProperty"/>
	<rdfs:domain rdf:resource="http://www.cidoc-crm.org/cidoc-crm/E71_Human-Made_Thing"/>
	<rdfs:range rdf:resource="http://www.cidoc-crm.org/cidoc-crm/E7_Activity"/>
	<rdfs:label xml:lang="fr">a été élaboré pour</rdfs:label>
	<rdfs:label xml:lang="pt">foi feito para</rdfs:label>
	<rdfs:label xml:lang="en">was made for</rdfs:label>
	<rdfs:label xml:lang="de">wurde hergestellt für</rdfs:label>
	<rdfs:label xml:lang="el">έγινε για</rdfs:label>
	<rdfs:label xml:lang="ru">был создан для</rdfs:label>
	<rdfs:label xml:lang="zh">用于</rdfs:label>
</rdf:Description>

<rdf:Description rdf:about="http://www.cidoc-crm.org/cidoc-crm/P1_is_identified_by">
	<rdf:type rdf:resource="http://www.w3.org/2002/07/owl#ObjectProperty"/>
	<owl:inverseOf rdf:resource="http://www.cidoc-crm.org/cidoc-crm/P1i_identifies"/>
	<rdfs:domain rdf:resource="http://www.cidoc-crm.org/cidoc-crm/E1_CRM_Entity"/>
	<rdfs:range rdf:resource="http://www.cidoc-crm.org/cidoc-crm/E41_Appellation"/>
	<rdfs:comment xml:lang="en">This property describes the naming or identification of any real-world item by a name or any other identifier.
This property is intended for identifiers in general use, which form part of the world the model intends to describe, and not merely for internal database identifiers which are specific to a technical system, unless these latter also have a more general use outside the technical context. This property includes in particular identification by mathematical expressions such as coordinate systems used for the identification of instances of E53 Place. The property does not reveal anything about when, where and by whom this identifier was used. A more detailed representation can be made using the fully developed (i.e. indirect) path through E15 Identifier Assignment.
This property is a shortcut for the path from E1 CRM Entity through P140i was attributed by, E15 Identifier Assignment, P37 assigned to E42 Identifier.
It is also a shortcut for the path from E1 CRM Entity through P1 is identified by, E41 Appellation, P139 has alternative form to E41 Appellation.</rdfs:comment>
	<rdfs:label xml:lang="fr">est identifié par</rdfs:label>
	<rdfs:label xml:lang="en">is identified by</rdfs:label>
	<rdfs:label xml:lang="de">wird bezeichnet als</rdfs:label>
	<rdfs:label xml:lang="pt">é identificado por</rdfs:label>
	<rdfs:label xml:lang="el">αναγνωρίζεται ως</rdfs:label>
	<rdfs:label xml:lang="ru">идентифицируется посредством</rdfs:label>
	<rdfs:label xml:lang="zh">被标识为</rdfs:label>
</rdf:Description>

<rdf:Description rdf:about="http://www.cidoc-crm.org/cidoc-crm/P1i_identifies">
	<rdf:type rdf:resource="http://www.w3.org/2002/07/owl#ObjectProperty"/>
	<rdfs:domain rdf:resource="http://www.cidoc-crm.org/cidoc-crm/E41_Appellation"/>
	<rdfs:range rdf:resource="http://www.cidoc-crm.org/cidoc-crm/E1_CRM_Entity"/>
	<rdfs:label xml:lang="de">bezeichnet</rdfs:label>
	<rdfs:label xml:lang="pt">identifica</rdfs:label>
	<rdfs:label xml:lang="fr">identifie</rdfs:label>
	<rdfs:label xml:lang="en">identifies</rdfs:label>
	<rdfs:label xml:lang="el">είναι αναγνωριστικό</rdfs:label>
	<rdfs:label xml:lang="ru">идентифицирует</rdfs:label>
	<rdfs:label xml:lang="zh">标识</rdfs:label>
</rdf:Description>

<rdf:Description rdf:about="http://www.cidoc-crm.org/cidoc-crm/P20_had_specific_purpose">
	<rdf:type rdf:resource="http://www.w3.org/2002/07/owl#ObjectProperty"/>
	<owl:inverseOf rdf:resource="http://www.cidoc-crm.org/cidoc-crm/P20i_was_purpose_of"/>
	<rdfs:domain rdf:resource="http://www.cidoc-crm.org/cidoc-crm/E7_Activity"/>
	<rdfs:range rdf:resource="http://www.cidoc-crm.org/cidoc-crm/E5_Event"/>
	<rdfs:comment xml:lang="en">This property describes the relationship between a preparatory activity, an instance of E7 Activity and the instance of E5 Event that it is intended as a preparation for.
This includes activities, orders and other organisational actions, taken in preparation for other activities or events.
P20 had specific purpose (was purpose of) implies that the activity succeeded in achieving its aim. If it does not succeed, such as the setting of a trap that did not catch anything, the unrealized intention should be documented using P21 had general purpose (was purpose of): E55 Type and/or P33 used specific technique (was used by): E29 Design or Procedure.</rdfs:comment>
	<rdfs:label xml:lang="fr">a eu pour finalité spécifique</rdfs:label>
	<rdfs:label xml:lang="en">had specific purpose</rdfs:label>
	<rdfs:label xml:lang="de">hatte den bestimmten Zweck</rdfs:label>
	<rdfs:label xml:lang="pt">tinha propósito específico</rdfs:label>
	<rdfs:label xml:lang="el">είχε συγκεκριμένο σκοπό</rdfs:label>
	<rdfs:label xml:lang="ru">имел конкретную цель</rdfs:label>
	<rdfs:label xml:lang="zh">有特定目的</rdfs:label>
</rdf:Description>

<rdf:Description rdf:about="http://www.cidoc-crm.org/cidoc-crm/P20i_was_purpose_of">
	<rdf:type rdf:resource="http://www.w3.org/2002/07/owl#ObjectProperty"/>
	<rdfs:domain rdf:resource="http://www.cidoc-crm.org/cidoc-crm/E5_Event"/>
	<rdfs:range rdf:resource="http://www.cidoc-crm.org/cidoc-crm/E7_Activity"/>
	<rdfs:label xml:lang="fr">a été la finalité de</rdfs:label>
	<rdfs:label xml:lang="pt">era o propósito de</rdfs:label>
	<rdfs:label xml:lang="de">war Zweck von</rdfs:label>
	<rdfs:label xml:lang="en">was purpose of</rdfs:label>
	<rdfs:label xml:lang="el">ήταν σκοπός του/της</rdfs:label>
	<rdfs:label xml:lang="ru">был целью для</rdfs:label>
	<rdfs:label xml:lang="zh">是为了</rdfs:label>
</rdf:Description>

<rdf:Description rdf:about="http://www.cidoc-crm.org/cidoc-crm/P21_had_general_purpose">
	<rdf:type rdf:resource="http://www.w3.org/2002/07/owl#ObjectProperty"/>
	<owl:inverseOf rdf:resource="http://www.cidoc-crm.org/cidoc-crm/P21i_was_purpose_of"/>
	<rdfs:domain rdf:resource="http://www.cidoc-crm.org/cidoc-crm/E7_Activity"/>
	<rdfs:range rdf:resource="http://www.cidoc-crm.org/cidoc-crm/E55_Type"/>
	<rdfs:comment xml:lang="en">This property describes an intentional relationship between an instance of E7 Activity and some general goal or purpose, described as an instance of E55 Type.
This may involve activities intended as preparation for some type of activity or event. P21 had general purpose (was purpose of) differs from P20 had specific purpose (was purpose of in that no specific event is implied as the purpose.</rdfs:comment>
	<rdfs:label xml:lang="fr">a eu pour finalité générale</rdfs:label>
	<rdfs:label xml:lang="en">had general purpose</rdfs:label>
	<rdfs:label xml:lang="de">hatte den allgemeinen Zweck</rdfs:label>
	<rdfs:label xml:lang="pt">tinha propósito geral</rdfs:label>
	<rdfs:label xml:lang="el">είχε γενικό σκοπό</rdfs:label>
	<rdfs:label xml:lang="ru">имел общую цель</rdfs:label>
	<rdfs:label xml:lang="zh">有一般目的</rdfs:label>
</rdf:Description>

<rdf:Description rdf:about="http://www.cidoc-crm.org/cidoc-crm/P21i_was_purpose_of">
	<rdf:type rdf:resource="http://www.w3.org/2002/07/owl#ObjectProperty"/>
	<rdfs:domain rdf:resource="http://www.cidoc-crm.org/cidoc-crm/E55_Type"/>
	<rdfs:range rdf:resource="http://www.cidoc-crm.org/cidoc-crm/E7_Activity"/>
	<rdfs:label xml:lang="fr">a été la finalité de</rdfs:label>
	<rdfs:label xml:lang="pt">era o propósito de</rdfs:label>
	<rdfs:label xml:lang="de">war Zweck von</rdfs:label>
	<rdfs:label xml:lang="en">was purpose of</rdfs:label>
	<rdfs:label xml:lang="el">ήταν σκοπός του/της</rdfs:label>
	<rdfs:label xml:lang="ru">был целью для</rdfs:label>
	<rdfs:label xml:lang="zh">是为了</rdfs:label>
</rdf:Description>

<rdf:Description rdf:about="http://www.cidoc-crm.org/cidoc-crm/P22_transferred_title_to">
	<rdf:type rdf:resource="http://www.w3.org/2002/07/owl#ObjectProperty"/>
	<rdfs:subPropertyOf rdf:resource="http://www.cidoc-crm.org/cidoc-crm/P14_carried_out_by"/>
	<owl:inverseOf rdf:resource="http://www.cidoc-crm.org/cidoc-crm/P22i_acquired_title_through"/>
	<rdfs:domain rdf:resource="http://www.cidoc-crm.org/cidoc-crm/E8_Acquisition"/>
	<rdfs:range rdf:resource="http://www.cidoc-crm.org/cidoc-crm/E39_Actor"/>
	<rdfs:comment xml:lang="en">This property identifies the instance of E39 Actor that acquires the legal ownership of an object as a result of an instance of E8 Acquisition.
The property will typically describe an Actor purchasing or otherwise acquiring an object from another Actor. However, title may also be acquired without any corresponding loss of title by another Actor, through legal fieldwork such as hunting, shooting, or fishing.
In reality, the title is either transferred to or from someone, or both.</rdfs:comment>
	<rdfs:label xml:lang="fr">a transféré le titre de propriété à</rdfs:label>
	<rdfs:label xml:lang="pt">transferiu os direitos de propriedade para</rdfs:label>
	<rdfs:label xml:lang="en">transferred title to</rdfs:label>
	<rdfs:label xml:lang="de">übertrug Besitztitel auf</rdfs:label>
	<rdfs:label xml:lang="el">μετεβίβασε τον τίτλο σε</rdfs:label>
	<rdfs:label xml:lang="ru">передал право собственности</rdfs:label>
	<rdfs:label xml:lang="zh">转移所有权至</rdfs:label>
</rdf:Description>

<rdf:Description rdf:about="http://www.cidoc-crm.org/cidoc-crm/P22i_acquired_title_through">
	<rdf:type rdf:resource="http://www.w3.org/2002/07/owl#ObjectProperty"/>
	<rdfs:subPropertyOf rdf:resource="http://www.cidoc-crm.org/cidoc-crm/P14i_performed"/>
	<rdfs:domain rdf:resource="http://www.cidoc-crm.org/cidoc-crm/E39_Actor"/>
	<rdfs:range rdf:resource="http://www.cidoc-crm.org/cidoc-crm/E8_Acquisition"/>
	<rdfs:label xml:lang="fr">a acquis le titre de propriété par</rdfs:label>
	<rdfs:label xml:lang="en">acquired title through</rdfs:label>
	<rdfs:label xml:lang="pt">adquiriu os direitos de propriedade por meio da</rdfs:label>
	<rdfs:label xml:lang="de">erwarb Besitztitel durch</rdfs:label>
	<rdfs:label xml:lang="el">απέκτησε τον τίτλο μέσω</rdfs:label>
	<rdfs:label xml:lang="ru">получил право собственности через</rdfs:label>
	<rdfs:label xml:lang="zh">获得所有权</rdfs:label>
</rdf:Description>

<rdf:Description rdf:about="http://www.cidoc-crm.org/cidoc-crm/P23_transferred_title_from">
	<rdf:type rdf:resource="http://www.w3.org/2002/07/owl#ObjectProperty"/>
	<rdfs:subPropertyOf rdf:resource="http://www.cidoc-crm.org/cidoc-crm/P14_carried_out_by"/>
	<owl:inverseOf rdf:resource="http://www.cidoc-crm.org/cidoc-crm/P23i_surrendered_title_through"/>
	<rdfs:domain rdf:resource="http://www.cidoc-crm.org/cidoc-crm/E8_Acquisition"/>
	<rdfs:range rdf:resource="http://www.cidoc-crm.org/cidoc-crm/E39_Actor"/>
	<rdfs:comment xml:lang="en">This property identifies the instance(s) of E39 Actor who relinquish legal ownership as the result of an instance of E8 Acquisition.
The property will typically be used to describe a person donating or selling an object to a museum. In reality, the title is either transferred to or from someone, or both.</rdfs:comment>
	<rdfs:label xml:lang="fr">a transféré le titre de propriété de</rdfs:label>
	<rdfs:label xml:lang="pt">transferiu os direitos de propriedade de</rdfs:label>
	<rdfs:label xml:lang="en">transferred title from</rdfs:label>
	<rdfs:label xml:lang="de">übertrug Besitztitel von</rdfs:label>
	<rdfs:label xml:lang="el">μετεβίβασε τον τίτλο από</rdfs:label>
	<rdfs:label xml:lang="ru">передал право собственности от</rdfs:label>
	<rdfs:label xml:lang="zh">转移所有权自</rdfs:label>
</rdf:Description>

<rdf:Description rdf:about="http://www.cidoc-crm.org/cidoc-crm/P23i_surrendered_title_through">
	<rdf:type rdf:resource="http://www.w3.org/2002/07/owl#ObjectProperty"/>
	<rdfs:subPropertyOf rdf:resource="http://www.cidoc-crm.org/cidoc-crm/P14i_performed"/>
	<rdfs:domain rdf:resource="http://www.cidoc-crm.org/cidoc-crm/E39_Actor"/>
	<rdfs:range rdf:resource="http://www.cidoc-crm.org/cidoc-crm/E8_Acquisition"/>
	<rdfs:label xml:lang="fr">a cédé le titre de propriété à</rdfs:label>
	<rdfs:label xml:lang="pt">perdeu os direitos de propriedade por meio da</rdfs:label>
	<rdfs:label xml:lang="en">surrendered title through</rdfs:label>
	<rdfs:label xml:lang="de">trat Besitztitel ab in</rdfs:label>
	<rdfs:label xml:lang="el">παρέδωσε τον τίτλο μέσω</rdfs:label>
	<rdfs:label xml:lang="ru">право собственности отдано через</rdfs:label>
	<rdfs:label xml:lang="zh">出让所有权</rdfs:label>
</rdf:Description>

<rdf:Description rdf:about="http://www.cidoc-crm.org/cidoc-crm/P24_transferred_title_of">
	<rdf:type rdf:resource="http://www.w3.org/2002/07/owl#ObjectProperty"/>
	<owl:inverseOf rdf:resource="http://www.cidoc-crm.org/cidoc-crm/P24i_changed_ownership_through"/>
	<rdfs:domain rdf:resource="http://www.cidoc-crm.org/cidoc-crm/E8_Acquisition"/>
	<rdfs:range rdf:resource="http://www.cidoc-crm.org/cidoc-crm/E18_Physical_Thing"/>
	<rdfs:comment xml:lang="en">This property identifies the instance(s) of E18 Physical Thing involved in an instance of E8 Acquisition.
In reality, an acquisition must refer to at least one transferred item.</rdfs:comment>
	<rdfs:label xml:lang="fr">a transféré le titre de propriété de</rdfs:label>
	<rdfs:label xml:lang="pt">transferiu os direitos de propriedade sobre o</rdfs:label>
	<rdfs:label xml:lang="en">transferred title of</rdfs:label>
	<rdfs:label xml:lang="de">übertrug Besitz über</rdfs:label>
	<rdfs:label xml:lang="el">μετεβίβασε τον τίτλο του/της</rdfs:label>
	<rdfs:label xml:lang="ru">передал право собственности на</rdfs:label>
	<rdfs:label xml:lang="zh">转移所有权的是</rdfs:label>
</rdf:Description>

<rdf:Description rdf:about="http://www.cidoc-crm.org/cidoc-crm/P24i_changed_ownership_through">
	<rdf:type rdf:resource="http://www.w3.org/2002/07/owl#ObjectProperty"/>
	<rdfs:domain rdf:resource="http://www.cidoc-crm.org/cidoc-crm/E18_Physical_Thing"/>
	<rdfs:range rdf:resource="http://www.cidoc-crm.org/cidoc-crm/E8_Acquisition"/>
	<rdfs:label xml:lang="fr">a changé de propriétaire par</rdfs:label>
	<rdfs:label xml:lang="en">changed ownership through</rdfs:label>
	<rdfs:label xml:lang="de">ging über in Besitz durch</rdfs:label>
	<rdfs:label xml:lang="pt">mudou de proprietário por meio de</rdfs:label>
	<rdfs:label xml:lang="el">άλλαξε ιδιοκτησία μέσω</rdfs:label>
	<rdfs:label xml:lang="ru">сменил владельца через</rdfs:label>
	<rdfs:label xml:lang="zh">变更所有权</rdfs:label>
</rdf:Description>

<rdf:Description rdf:about="http://www.cidoc-crm.org/cidoc-crm/P25_moved">
	<rdf:type rdf:resource="http://www.w3.org/2002/07/owl#ObjectProperty"/>
	<rdfs:subPropertyOf rdf:resource="http://www.cidoc-crm.org/cidoc-crm/P12_occurred_in_the_presence_of"/>
	<owl:inverseOf rdf:resource="http://www.cidoc-crm.org/cidoc-crm/P25i_moved_by"/>
	<rdfs:domain rdf:resource="http://www.cidoc-crm.org/cidoc-crm/E9_Move"/>
	<rdfs:range rdf:resource="http://www.cidoc-crm.org/cidoc-crm/E19_Physical_Object"/>
	<rdfs:comment xml:lang="en">This property identifies an instance of E19 Physical Object that was moved by an instance of E9 Move. A move must concern at least one object.
The property implies the object’s passive participation. For example, Monet’s painting “Impression sunrise” was moved for the first Impressionist exhibition in 1874.</rdfs:comment>
	<rdfs:label xml:lang="fr">a déplacé</rdfs:label>
	<rdfs:label xml:lang="de">bewegte</rdfs:label>
	<rdfs:label xml:lang="pt">locomoveu</rdfs:label>
	<rdfs:label xml:lang="en">moved</rdfs:label>
	<rdfs:label xml:lang="el">μετεκίνησε</rdfs:label>
	<rdfs:label xml:lang="ru">переместил</rdfs:label>
	<rdfs:label xml:lang="zh">移动</rdfs:label>
</rdf:Description>

<rdf:Description rdf:about="http://www.cidoc-crm.org/cidoc-crm/P25i_moved_by">
	<rdf:type rdf:resource="http://www.w3.org/2002/07/owl#ObjectProperty"/>
	<rdfs:subPropertyOf rdf:resource="http://www.cidoc-crm.org/cidoc-crm/P12i_was_present_at"/>
	<rdfs:domain rdf:resource="http://www.cidoc-crm.org/cidoc-crm/E19_Physical_Object"/>
	<rdfs:range rdf:resource="http://www.cidoc-crm.org/cidoc-crm/E9_Move"/>
	<rdfs:label xml:lang="fr">a été déplacé par</rdfs:label>
	<rdfs:label xml:lang="pt">foi locomovido por</rdfs:label>
	<rdfs:label xml:lang="en">moved by</rdfs:label>
	<rdfs:label xml:lang="de">wurde bewegt durch</rdfs:label>
	<rdfs:label xml:lang="el">μετακινήθηκε από</rdfs:label>
	<rdfs:label xml:lang="ru">перемещен посредством</rdfs:label>
	<rdfs:label xml:lang="zh">被移动</rdfs:label>
</rdf:Description>

<rdf:Description rdf:about="http://www.cidoc-crm.org/cidoc-crm/P26_moved_to">
	<rdf:type rdf:resource="http://www.w3.org/2002/07/owl#ObjectProperty"/>
	<owl:inverseOf rdf:resource="http://www.cidoc-crm.org/cidoc-crm/P26i_was_destination_of"/>
	<rdfs:domain rdf:resource="http://www.cidoc-crm.org/cidoc-crm/E9_Move"/>
	<rdfs:range rdf:resource="http://www.cidoc-crm.org/cidoc-crm/E53_Place"/>
	<rdfs:comment xml:lang="en">This property identifies a destination, an instance of E53 Place, of an instance of E9 Move.
A move will be linked to a destination, such as the move of an artifact from storage to display. A move may be linked to many terminal instances of E53 Place by multiple instances of this property. In this case the move describes a distribution of a set of objects. The area of the move includes the origin(s), route and destination(s).
Therefore, the described destination is an instance of E53 Place which P89 falls within (contains) the instance of E53 Place the move P7 took place at.</rdfs:comment>
	<rdfs:label xml:lang="fr">a déplacé vers</rdfs:label>
	<rdfs:label xml:lang="de">bewegte bis zu</rdfs:label>
	<rdfs:label xml:lang="pt">locomoveu para</rdfs:label>
	<rdfs:label xml:lang="en">moved to</rdfs:label>
	<rdfs:label xml:lang="el">μετακινήθηκε προς</rdfs:label>
	<rdfs:label xml:lang="ru">перемещен в</rdfs:label>
	<rdfs:label xml:lang="zh">移至</rdfs:label>
</rdf:Description>

<rdf:Description rdf:about="http://www.cidoc-crm.org/cidoc-crm/P26i_was_destination_of">
	<rdf:type rdf:resource="http://www.w3.org/2002/07/owl#ObjectProperty"/>
	<rdfs:domain rdf:resource="http://www.cidoc-crm.org/cidoc-crm/E53_Place"/>
	<rdfs:range rdf:resource="http://www.cidoc-crm.org/cidoc-crm/E9_Move"/>
	<rdfs:label xml:lang="fr">a été la destination de</rdfs:label>
	<rdfs:label xml:lang="pt">era destinação de</rdfs:label>
	<rdfs:label xml:lang="de">war Zielort von</rdfs:label>
	<rdfs:label xml:lang="en">was destination of</rdfs:label>
	<rdfs:label xml:lang="el">ήταν προορισμός του/της</rdfs:label>
	<rdfs:label xml:lang="ru">был пунктом назначения для</rdfs:label>
	<rdfs:label xml:lang="zh">是目的地</rdfs:label>
</rdf:Description>

<rdf:Description rdf:about="http://www.cidoc-crm.org/cidoc-crm/P27_moved_from">
	<rdf:type rdf:resource="http://www.w3.org/2002/07/owl#ObjectProperty"/>
	<owl:inverseOf rdf:resource="http://www.cidoc-crm.org/cidoc-crm/P27i_was_origin_of"/>
	<rdfs:domain rdf:resource="http://www.cidoc-crm.org/cidoc-crm/E9_Move"/>
	<rdfs:range rdf:resource="http://www.cidoc-crm.org/cidoc-crm/E53_Place"/>
	<rdfs:comment xml:lang="en">This property identifies an origin, an instance of E53 Place, of an instance of E9 Move.
A move will be linked to an origin, such as the move of an artifact from storage to display. A move may be linked to many starting instances of E53 Place by multiple instances of this property. In this case the move describes the picking up of a set of objects. The area of the move includes the origin(s), route and destination(s).
Therefore, the described origin is an instance of E53 Place which P89 falls within (contains) the instance of E53 Place the move P7 took place at.</rdfs:comment>
	<rdfs:label xml:lang="fr">a déplacé depuis</rdfs:label>
	<rdfs:label xml:lang="de">bewegte weg von</rdfs:label>
	<rdfs:label xml:lang="pt">locomoveu de</rdfs:label>
	<rdfs:label xml:lang="en">moved from</rdfs:label>
	<rdfs:label xml:lang="el">μετακινήθηκε από</rdfs:label>
	<rdfs:label xml:lang="ru">перемещен из</rdfs:label>
	<rdfs:label xml:lang="zh">移自</rdfs:label>
</rdf:Description>

<rdf:Description rdf:about="http://www.cidoc-crm.org/cidoc-crm/P27i_was_origin_of">
	<rdf:type rdf:resource="http://www.w3.org/2002/07/owl#ObjectProperty"/>
	<rdfs:domain rdf:resource="http://www.cidoc-crm.org/cidoc-crm/E53_Place"/>
	<rdfs:range rdf:resource="http://www.cidoc-crm.org/cidoc-crm/E9_Move"/>
	<rdfs:label xml:lang="fr">a été le point de départ de</rdfs:label>
	<rdfs:label xml:lang="pt">era origem de</rdfs:label>
	<rdfs:label xml:lang="de">war Ausgangsort von</rdfs:label>
	<rdfs:label xml:lang="en">was origin of</rdfs:label>
	<rdfs:label xml:lang="el">ήταν αφετηρία του/της</rdfs:label>
	<rdfs:label xml:lang="ru">был исходной точкой для</rdfs:label>
	<rdfs:label xml:lang="zh">是起点</rdfs:label>
</rdf:Description>

<rdf:Description rdf:about="http://www.cidoc-crm.org/cidoc-crm/P28_custody_surrendered_by">
	<rdf:type rdf:resource="http://www.w3.org/2002/07/owl#ObjectProperty"/>
	<rdfs:subPropertyOf rdf:resource="http://www.cidoc-crm.org/cidoc-crm/P14_carried_out_by"/>
	<owl:inverseOf rdf:resource="http://www.cidoc-crm.org/cidoc-crm/P28i_surrendered_custody_through"/>
	<rdfs:domain rdf:resource="http://www.cidoc-crm.org/cidoc-crm/E10_Transfer_of_Custody"/>
	<rdfs:range rdf:resource="http://www.cidoc-crm.org/cidoc-crm/E39_Actor"/>
	<rdfs:comment xml:lang="en">This property identifies the instance(s) of E39 Actor who surrender custody of an instance of E18 Physical Thing in an instance of E10 Transfer of Custody.
The property will typically describe an Actor surrendering custody of an object when it is handed over to someone else’s care. On occasion, physical custody may be surrendered involuntarily, e.g. through accident, loss, or theft.
In reality, custody is either transferred to someone or from someone, or both.</rdfs:comment>
	<rdfs:label xml:lang="fr">a mis fin à la garde par</rdfs:label>
	<rdfs:label xml:lang="en">custody surrendered by</rdfs:label>
	<rdfs:label xml:lang="pt">custódia concedida por</rdfs:label>
	<rdfs:label xml:lang="de">übergab Gewahrsam an</rdfs:label>
	<rdfs:label xml:lang="el">μετεβίβασε κατοχή από</rdfs:label>
	<rdfs:label xml:lang="ru">опека отдана</rdfs:label>
	<rdfs:label xml:lang="zh">监护权转自</rdfs:label>
</rdf:Description>

<rdf:Description rdf:about="http://www.cidoc-crm.org/cidoc-crm/P28i_surrendered_custody_through">
	<rdf:type rdf:resource="http://www.w3.org/2002/07/owl#ObjectProperty"/>
	<rdfs:subPropertyOf rdf:resource="http://www.cidoc-crm.org/cidoc-crm/P14i_performed"/>
	<rdfs:domain rdf:resource="http://www.cidoc-crm.org/cidoc-crm/E39_Actor"/>
	<rdfs:range rdf:resource="http://www.cidoc-crm.org/cidoc-crm/E10_Transfer_of_Custody"/>
	<rdfs:label xml:lang="fr">a cédé la garde par</rdfs:label>
	<rdfs:label xml:lang="pt">final da custódia por meio de</rdfs:label>
	<rdfs:label xml:lang="en">surrendered custody through</rdfs:label>
	<rdfs:label xml:lang="de">wurde Gewahrsam übergeben durch</rdfs:label>
	<rdfs:label xml:lang="el">παρέδωσε κατοχή μέσω</rdfs:label>
	<rdfs:label xml:lang="ru">опека отдана через</rdfs:label>
	<rdfs:label xml:lang="zh">出让监护权</rdfs:label>
</rdf:Description>

<rdf:Description rdf:about="http://www.cidoc-crm.org/cidoc-crm/P29_custody_received_by">
	<rdf:type rdf:resource="http://www.w3.org/2002/07/owl#ObjectProperty"/>
	<rdfs:subPropertyOf rdf:resource="http://www.cidoc-crm.org/cidoc-crm/P14_carried_out_by"/>
	<owl:inverseOf rdf:resource="http://www.cidoc-crm.org/cidoc-crm/P29i_received_custody_through"/>
	<rdfs:domain rdf:resource="http://www.cidoc-crm.org/cidoc-crm/E10_Transfer_of_Custody"/>
	<rdfs:range rdf:resource="http://www.cidoc-crm.org/cidoc-crm/E39_Actor"/>
	<rdfs:comment xml:lang="en">This property identifies the instance(s) of E39 Actor who receive custody of an instance of E18 Physical Thing in an instance of E10 Transfer of Custody.
The property will typically describe Actors receiving custody of an object when it is handed over from another Actor’s care. On occasion, physical custody may be received involuntarily or illegally, e.g. through accident, unsolicited donation, or theft.
In reality, custody is either transferred to someone or from someone, or both.</rdfs:comment>
	<rdfs:label xml:lang="fr">a confié la garde par</rdfs:label>
	<rdfs:label xml:lang="en">custody received by</rdfs:label>
	<rdfs:label xml:lang="pt">custódia recebida por</rdfs:label>
	<rdfs:label xml:lang="de">übertrug Gewahrsam auf</rdfs:label>
	<rdfs:label xml:lang="el">μετεβίβασε κατοχή σε</rdfs:label>
	<rdfs:label xml:lang="ru">опека получена</rdfs:label>
	<rdfs:label xml:lang="zh">监护权转至</rdfs:label>
</rdf:Description>

<rdf:Description rdf:about="http://www.cidoc-crm.org/cidoc-crm/P29i_received_custody_through">
	<rdf:type rdf:resource="http://www.w3.org/2002/07/owl#ObjectProperty"/>
	<rdfs:subPropertyOf rdf:resource="http://www.cidoc-crm.org/cidoc-crm/P14i_performed"/>
	<rdfs:domain rdf:resource="http://www.cidoc-crm.org/cidoc-crm/E39_Actor"/>
	<rdfs:range rdf:resource="http://www.cidoc-crm.org/cidoc-crm/E10_Transfer_of_Custody"/>
	<rdfs:label xml:lang="fr">a reçu la garde par</rdfs:label>
	<rdfs:label xml:lang="de">erhielt Gewahrsam durch</rdfs:label>
	<rdfs:label xml:lang="pt">início da custódia por meio de</rdfs:label>
	<rdfs:label xml:lang="en">received custody through</rdfs:label>
	<rdfs:label xml:lang="el">παρέλαβε κατοχή μέσω</rdfs:label>
	<rdfs:label xml:lang="ru">получил опеку через</rdfs:label>
	<rdfs:label xml:lang="zh">获得监护权</rdfs:label>
</rdf:Description>

<rdf:Description rdf:about="http://www.cidoc-crm.org/cidoc-crm/P2_has_type">
	<rdf:type rdf:resource="http://www.w3.org/2002/07/owl#ObjectProperty"/>
	<owl:inverseOf rdf:resource="http://www.cidoc-crm.org/cidoc-crm/P2i_is_type_of"/>
	<rdfs:domain rdf:resource="http://www.cidoc-crm.org/cidoc-crm/E1_CRM_Entity"/>
	<rdfs:range rdf:resource="http://www.cidoc-crm.org/cidoc-crm/E55_Type"/>
	<rdfs:comment xml:lang="en">This property allows sub-typing of CIDOC CRM entities –a form of specialisation – through the use of a terminological hierarchy, or thesaurus.
The CIDOC CRM is intended to focus on the high-level entities and relationships needed to describe data structures. Consequently, it does not specialise entities any further than is required for this immediate purpose. However, entities in the isA hierarchy of the CIDOC CRM may by specialised into any number of sub-entities, which can be defined in the E55 Type hierarchy. E41 Appellation, for example, may be specialised into “e-mail address”, “telephone number”, “post office box”, “URL”, etc., none of which figures explicitly in the CIDOC CRM class hierarchy. A comprehensive explanation about refining CIDOC CRM concepts by E55 Type is given in the section “About Types” in the section on “Specific Modelling Constructs” of this document.
This property is a shortcut for the path from E1 CRM Entity through P41i was classified by, E17 Type Assignment, P42 assigned to E55 Type.</rdfs:comment>
	<rdfs:label xml:lang="fr">a pour type</rdfs:label>
	<rdfs:label xml:lang="en">has type</rdfs:label>
	<rdfs:label xml:lang="de">hat den Typus</rdfs:label>
	<rdfs:label xml:lang="pt">é do tipo</rdfs:label>
	<rdfs:label xml:lang="el">έχει τύπο</rdfs:label>
	<rdfs:label xml:lang="ru">имеет тип</rdfs:label>
	<rdfs:label xml:lang="zh">有类型</rdfs:label>
</rdf:Description>

<rdf:Description rdf:about="http://www.cidoc-crm.org/cidoc-crm/P2i_is_type_of">
	<rdf:type rdf:resource="http://www.w3.org/2002/07/owl#ObjectProperty"/>
	<rdfs:domain rdf:resource="http://www.cidoc-crm.org/cidoc-crm/E55_Type"/>
	<rdfs:range rdf:resource="http://www.cidoc-crm.org/cidoc-crm/E1_CRM_Entity"/>
	<rdfs:label xml:lang="fr">est le type de</rdfs:label>
	<rdfs:label xml:lang="en">is type of</rdfs:label>
	<rdfs:label xml:lang="de">ist Typus von</rdfs:label>
	<rdfs:label xml:lang="pt">é o tipo de</rdfs:label>
	<rdfs:label xml:lang="el">είναι ο τύπος του/της</rdfs:label>
	<rdfs:label xml:lang="ru">является типом для</rdfs:label>
	<rdfs:label xml:lang="zh">是类型</rdfs:label>
</rdf:Description>

<rdf:Description rdf:about="http://www.cidoc-crm.org/cidoc-crm/P30_transferred_custody_of">
	<rdf:type rdf:resource="http://www.w3.org/2002/07/owl#ObjectProperty"/>
	<owl:inverseOf rdf:resource="http://www.cidoc-crm.org/cidoc-crm/P30i_custody_transferred_through"/>
	<rdfs:domain rdf:resource="http://www.cidoc-crm.org/cidoc-crm/E10_Transfer_of_Custody"/>
	<rdfs:range rdf:resource="http://www.cidoc-crm.org/cidoc-crm/E18_Physical_Thing"/>
	<rdfs:comment xml:lang="en">This property identifies the instance(s) of E18 Physical Thing concerned in an instance of E10 Transfer of Custody.
The property will typically describe the object that is handed over by an instance of E39 Actor to the custody of another instance of E39 Actor. On occasion, physical custody may be transferred involuntarily or illegally, e.g. through accident, unsolicited donation, or theft.</rdfs:comment>
	<rdfs:label xml:lang="fr">a transféré la garde de</rdfs:label>
	<rdfs:label xml:lang="pt">transferida custódia de</rdfs:label>
	<rdfs:label xml:lang="en">transferred custody of</rdfs:label>
	<rdfs:label xml:lang="de">übertrug Gewahrsam über</rdfs:label>
	<rdfs:label xml:lang="el">μετεβίβασε κατοχή του/της/των</rdfs:label>
	<rdfs:label xml:lang="ru">передало опеку на</rdfs:label>
	<rdfs:label xml:lang="zh">转移监护权的是</rdfs:label>
</rdf:Description>

<rdf:Description rdf:about="http://www.cidoc-crm.org/cidoc-crm/P30i_custody_transferred_through">
	<rdf:type rdf:resource="http://www.w3.org/2002/07/owl#ObjectProperty"/>
	<rdfs:domain rdf:resource="http://www.cidoc-crm.org/cidoc-crm/E18_Physical_Thing"/>
	<rdfs:range rdf:resource="http://www.cidoc-crm.org/cidoc-crm/E10_Transfer_of_Custody"/>
	<rdfs:label xml:lang="fr">a été l’objet d’un transfert de garde par</rdfs:label>
	<rdfs:label xml:lang="en">custody transferred through</rdfs:label>
	<rdfs:label xml:lang="pt">custódia transferida por meio de</rdfs:label>
	<rdfs:label xml:lang="de">wechselte Gewahrsam durch</rdfs:label>
	<rdfs:label xml:lang="el">άλλαξε κατοχή μέσω</rdfs:label>
	<rdfs:label xml:lang="ru">опека передана через</rdfs:label>
	<rdfs:label xml:lang="zh">变更监护权</rdfs:label>
</rdf:Description>

<rdf:Description rdf:about="http://www.cidoc-crm.org/cidoc-crm/P31_has_modified">
	<rdf:type rdf:resource="http://www.w3.org/2002/07/owl#ObjectProperty"/>
	<rdfs:subPropertyOf rdf:resource="http://www.cidoc-crm.org/cidoc-crm/P12_occurred_in_the_presence_of"/>
	<owl:inverseOf rdf:resource="http://www.cidoc-crm.org/cidoc-crm/P31i_was_modified_by"/>
	<rdfs:domain rdf:resource="http://www.cidoc-crm.org/cidoc-crm/E11_Modification"/>
	<rdfs:range rdf:resource="http://www.cidoc-crm.org/cidoc-crm/E18_Physical_Thing"/>
	<rdfs:comment xml:lang="en">This property identifies the instance of E18 Physical Thing modified in an instance of E11 Modification.</rdfs:comment>
	<rdfs:label xml:lang="fr">a modifié</rdfs:label>
	<rdfs:label xml:lang="en">has modified</rdfs:label>
	<rdfs:label xml:lang="pt">modificou</rdfs:label>
	<rdfs:label xml:lang="de">veränderte</rdfs:label>
	<rdfs:label xml:lang="el">τροποποίησε</rdfs:label>
	<rdfs:label xml:lang="ru">изменил</rdfs:label>
	<rdfs:label xml:lang="zh">已更改</rdfs:label>
</rdf:Description>

<rdf:Description rdf:about="http://www.cidoc-crm.org/cidoc-crm/P31i_was_modified_by">
	<rdf:type rdf:resource="http://www.w3.org/2002/07/owl#ObjectProperty"/>
	<rdfs:subPropertyOf rdf:resource="http://www.cidoc-crm.org/cidoc-crm/P12i_was_present_at"/>
	<rdfs:domain rdf:resource="http://www.cidoc-crm.org/cidoc-crm/E18_Physical_Thing"/>
	<rdfs:range rdf:resource="http://www.cidoc-crm.org/cidoc-crm/E11_Modification"/>
	<rdfs:label xml:lang="fr">a été modifié par</rdfs:label>
	<rdfs:label xml:lang="pt">foi modificada por</rdfs:label>
	<rdfs:label xml:lang="en">was modified by</rdfs:label>
	<rdfs:label xml:lang="de">wurde verändert durch</rdfs:label>
	<rdfs:label xml:lang="el">τροποποιήθηκε από</rdfs:label>
	<rdfs:label xml:lang="ru">был изменен посредством</rdfs:label>
	<rdfs:label xml:lang="zh">被更改</rdfs:label>
</rdf:Description>

<rdf:Description rdf:about="http://www.cidoc-crm.org/cidoc-crm/P32_used_general_technique">
	<rdf:type rdf:resource="http://www.w3.org/2002/07/owl#ObjectProperty"/>
	<rdfs:subPropertyOf rdf:resource="http://www.cidoc-crm.org/cidoc-crm/P125_used_object_of_type"/>
	<owl:inverseOf rdf:resource="http://www.cidoc-crm.org/cidoc-crm/P32i_was_technique_of"/>
	<rdfs:domain rdf:resource="http://www.cidoc-crm.org/cidoc-crm/E7_Activity"/>
	<rdfs:range rdf:resource="http://www.cidoc-crm.org/cidoc-crm/E55_Type"/>
	<rdfs:comment xml:lang="en">This property identifies the technique or method, modelled as an instance of E55 Type, that was employed in an instance of E7 Activity.
These techniques should be drawn from an external E55 Type hierarchy of consistent terminology of general techniques or methods such as embroidery, oil-painting, carbon dating, etc. Specific documented techniques should be described as instances of E29 Design or Procedure.</rdfs:comment>
	<rdfs:label xml:lang="fr">a mobilisé comme technique générale</rdfs:label>
	<rdfs:label xml:lang="de">benutzte das allgemeine Verfahren</rdfs:label>
	<rdfs:label xml:lang="en">used general technique</rdfs:label>
	<rdfs:label xml:lang="pt">usou técnica geral</rdfs:label>
	<rdfs:label xml:lang="el">χρησιμοποίησε γενική τεχνική</rdfs:label>
	<rdfs:label xml:lang="ru">использовал общую технику</rdfs:label>
	<rdfs:label xml:lang="zh">使用通用技术</rdfs:label>
</rdf:Description>

<rdf:Description rdf:about="http://www.cidoc-crm.org/cidoc-crm/P32i_was_technique_of">
	<rdf:type rdf:resource="http://www.w3.org/2002/07/owl#ObjectProperty"/>
	<rdfs:subPropertyOf rdf:resource="http://www.cidoc-crm.org/cidoc-crm/P125i_was_type_of_object_used_in"/>
	<rdfs:domain rdf:resource="http://www.cidoc-crm.org/cidoc-crm/E55_Type"/>
	<rdfs:range rdf:resource="http://www.cidoc-crm.org/cidoc-crm/E7_Activity"/>
	<rdfs:label xml:lang="fr">a été la technique générale mise en œuvre dans</rdfs:label>
	<rdfs:label xml:lang="pt">foi técnica da</rdfs:label>
	<rdfs:label xml:lang="de">war Verfahren von</rdfs:label>
	<rdfs:label xml:lang="en">was technique of</rdfs:label>
	<rdfs:label xml:lang="el">ήταν τεχνική του/της</rdfs:label>
	<rdfs:label xml:lang="ru">был техникой для</rdfs:label>
	<rdfs:label xml:lang="zh">是技术</rdfs:label>
</rdf:Description>

<rdf:Description rdf:about="http://www.cidoc-crm.org/cidoc-crm/P33_used_specific_technique">
	<rdf:type rdf:resource="http://www.w3.org/2002/07/owl#ObjectProperty"/>
	<rdfs:subPropertyOf rdf:resource="http://www.cidoc-crm.org/cidoc-crm/P16_used_specific_object"/>
	<owl:inverseOf rdf:resource="http://www.cidoc-crm.org/cidoc-crm/P33i_was_used_by"/>
	<rdfs:domain rdf:resource="http://www.cidoc-crm.org/cidoc-crm/E7_Activity"/>
	<rdfs:range rdf:resource="http://www.cidoc-crm.org/cidoc-crm/E29_Design_or_Procedure"/>
	<rdfs:comment xml:lang="en">This property identifies a specific instance of E29 Design or Procedure in order to carry out an instance of E7 Activity or parts of it.
The property differs from P32 used general technique (was technique of) in that P33 refers to an instance of E29 Design or Procedure, which is a concrete information object in its own right rather than simply being a term or a method known by tradition.
Typical examples would include intervention plans for conservation or the construction plans of a building.</rdfs:comment>
	<rdfs:label xml:lang="fr">a mobilisé comme technique spécifique</rdfs:label>
	<rdfs:label xml:lang="de">benutzte das bestimmte Verfahren</rdfs:label>
	<rdfs:label xml:lang="en">used specific technique</rdfs:label>
	<rdfs:label xml:lang="pt">usou técnica específica</rdfs:label>
	<rdfs:label xml:lang="el">χρησιμοποίησε συγκεκριμένη τεχνική</rdfs:label>
	<rdfs:label xml:lang="ru">использовал особую технику</rdfs:label>
	<rdfs:label xml:lang="zh">使用特定技术</rdfs:label>
</rdf:Description>

<rdf:Description rdf:about="http://www.cidoc-crm.org/cidoc-crm/P33i_was_used_by">
	<rdf:type rdf:resource="http://www.w3.org/2002/07/owl#ObjectProperty"/>
	<rdfs:subPropertyOf rdf:resource="http://www.cidoc-crm.org/cidoc-crm/P16i_was_used_for"/>
	<rdfs:domain rdf:resource="http://www.cidoc-crm.org/cidoc-crm/E29_Design_or_Procedure"/>
	<rdfs:range rdf:resource="http://www.cidoc-crm.org/cidoc-crm/E7_Activity"/>
	<rdfs:label xml:lang="fr">a été la technique spécifique mise en œuvre dans</rdfs:label>
	<rdfs:label xml:lang="pt">foi usada por</rdfs:label>
	<rdfs:label xml:lang="en">was used by</rdfs:label>
	<rdfs:label xml:lang="de">wurde benutzt von</rdfs:label>
	<rdfs:label xml:lang="el">χρησιμοποιήθηκε για</rdfs:label>
	<rdfs:label xml:lang="ru">был использован посредством</rdfs:label>
	<rdfs:label xml:lang="zh">被使用</rdfs:label>
</rdf:Description>

<rdf:Description rdf:about="http://www.cidoc-crm.org/cidoc-crm/P34_concerned">
	<rdf:type rdf:resource="http://www.w3.org/2002/07/owl#ObjectProperty"/>
	<rdfs:subPropertyOf rdf:resource="http://www.cidoc-crm.org/cidoc-crm/P140_assigned_attribute_to"/>
	<owl:inverseOf rdf:resource="http://www.cidoc-crm.org/cidoc-crm/P34i_was_assessed_by"/>
	<rdfs:domain rdf:resource="http://www.cidoc-crm.org/cidoc-crm/E14_Condition_Assessment"/>
	<rdfs:range rdf:resource="http://www.cidoc-crm.org/cidoc-crm/E18_Physical_Thing"/>
	<rdfs:comment xml:lang="en">This property identifies the instance of E18 Physical Thing that was assessed during an instance of E14 Condition Assessment.
Conditions may be assessed either by direct observation or using recorded evidence. In the latter case the instance of E18 Physical Thing does not need to be present or extant at the time of assessment.</rdfs:comment>
	<rdfs:label xml:lang="fr">a porté sur</rdfs:label>
	<rdfs:label xml:lang="de">betraf</rdfs:label>
	<rdfs:label xml:lang="en">concerned</rdfs:label>
	<rdfs:label xml:lang="pt">interessada</rdfs:label>
	<rdfs:label xml:lang="el">αφορούσε σε</rdfs:label>
	<rdfs:label xml:lang="ru">имел дело с</rdfs:label>
	<rdfs:label xml:lang="zh">已评估</rdfs:label>
</rdf:Description>

<rdf:Description rdf:about="http://www.cidoc-crm.org/cidoc-crm/P34i_was_assessed_by">
	<rdf:type rdf:resource="http://www.w3.org/2002/07/owl#ObjectProperty"/>
	<rdfs:subPropertyOf rdf:resource="http://www.cidoc-crm.org/cidoc-crm/P140i_was_attributed_by"/>
	<rdfs:domain rdf:resource="http://www.cidoc-crm.org/cidoc-crm/E18_Physical_Thing"/>
	<rdfs:range rdf:resource="http://www.cidoc-crm.org/cidoc-crm/E14_Condition_Assessment"/>
	<rdfs:label xml:lang="fr">a été évalué par</rdfs:label>
	<rdfs:label xml:lang="pt">foi avaliada por</rdfs:label>
	<rdfs:label xml:lang="en">was assessed by</rdfs:label>
	<rdfs:label xml:lang="de">wurde beurteilt durch</rdfs:label>
	<rdfs:label xml:lang="el">εκτιμήθηκε από</rdfs:label>
	<rdfs:label xml:lang="ru">был оценен посредством</rdfs:label>
	<rdfs:label xml:lang="zh">被评估</rdfs:label>
</rdf:Description>

<rdf:Description rdf:about="http://www.cidoc-crm.org/cidoc-crm/P35_has_identified">
	<rdf:type rdf:resource="http://www.w3.org/2002/07/owl#ObjectProperty"/>
	<rdfs:subPropertyOf rdf:resource="http://www.cidoc-crm.org/cidoc-crm/P141_assigned"/>
	<owl:inverseOf rdf:resource="http://www.cidoc-crm.org/cidoc-crm/P35i_was_identified_by"/>
	<rdfs:domain rdf:resource="http://www.cidoc-crm.org/cidoc-crm/E14_Condition_Assessment"/>
	<rdfs:range rdf:resource="http://www.cidoc-crm.org/cidoc-crm/E3_Condition_State"/>
	<rdfs:comment xml:lang="en">This property identifies the instance of E3 Condition State that was observed in an instance of E14 Condition Assessment activity.</rdfs:comment>
	<rdfs:label xml:lang="fr">a identifié</rdfs:label>
	<rdfs:label xml:lang="en">has identified</rdfs:label>
	<rdfs:label xml:lang="de">hat identifiziert</rdfs:label>
	<rdfs:label xml:lang="pt">identificou</rdfs:label>
	<rdfs:label xml:lang="el">έχει διαπιστώσει</rdfs:label>
	<rdfs:label xml:lang="ru">идентифицировал</rdfs:label>
	<rdfs:label xml:lang="zh">有标识</rdfs:label>
</rdf:Description>

<rdf:Description rdf:about="http://www.cidoc-crm.org/cidoc-crm/P35i_was_identified_by">
	<rdf:type rdf:resource="http://www.w3.org/2002/07/owl#ObjectProperty"/>
	<rdfs:subPropertyOf rdf:resource="http://www.cidoc-crm.org/cidoc-crm/P141i_was_assigned_by"/>
	<rdfs:domain rdf:resource="http://www.cidoc-crm.org/cidoc-crm/E3_Condition_State"/>
	<rdfs:range rdf:resource="http://www.cidoc-crm.org/cidoc-crm/E14_Condition_Assessment"/>
	<rdfs:label xml:lang="fr">a été identifié par</rdfs:label>
	<rdfs:label xml:lang="pt">foi identificado por</rdfs:label>
	<rdfs:label xml:lang="en">was identified by</rdfs:label>
	<rdfs:label xml:lang="de">wurde identifiziert durch</rdfs:label>
	<rdfs:label xml:lang="el">έχει διαπιστωθεί από</rdfs:label>
	<rdfs:label xml:lang="ru">идентифицирован посредством</rdfs:label>
	<rdfs:label xml:lang="zh">被标识</rdfs:label>
</rdf:Description>

<rdf:Description rdf:about="http://www.cidoc-crm.org/cidoc-crm/P37_assigned">
	<rdf:type rdf:resource="http://www.w3.org/2002/07/owl#ObjectProperty"/>
	<rdfs:subPropertyOf rdf:resource="http://www.cidoc-crm.org/cidoc-crm/P141_assigned"/>
	<owl:inverseOf rdf:resource="http://www.cidoc-crm.org/cidoc-crm/P37i_was_assigned_by"/>
	<rdfs:domain rdf:resource="http://www.cidoc-crm.org/cidoc-crm/E15_Identifier_Assignment"/>
	<rdfs:range rdf:resource="http://www.cidoc-crm.org/cidoc-crm/E42_Identifier"/>
	<rdfs:comment xml:lang="en">This property records the identifier that was assigned to an item in an instance of E15 Identifier Assignment.
The same identifier may be assigned on more than one occasion.
An identifier might be created prior to an assignment.</rdfs:comment>
	<rdfs:label xml:lang="fr">a assigné</rdfs:label>
	<rdfs:label xml:lang="en">assigned</rdfs:label>
	<rdfs:label xml:lang="pt">atribuiu</rdfs:label>
	<rdfs:label xml:lang="de">wies zu</rdfs:label>
	<rdfs:label xml:lang="el">απέδωσε</rdfs:label>
	<rdfs:label xml:lang="ru">назначил</rdfs:label>
	<rdfs:label xml:lang="zh">分配了</rdfs:label>
</rdf:Description>

<rdf:Description rdf:about="http://www.cidoc-crm.org/cidoc-crm/P37i_was_assigned_by">
	<rdf:type rdf:resource="http://www.w3.org/2002/07/owl#ObjectProperty"/>
	<rdfs:subPropertyOf rdf:resource="http://www.cidoc-crm.org/cidoc-crm/P141i_was_assigned_by"/>
	<rdfs:domain rdf:resource="http://www.cidoc-crm.org/cidoc-crm/E42_Identifier"/>
	<rdfs:range rdf:resource="http://www.cidoc-crm.org/cidoc-crm/E15_Identifier_Assignment"/>
	<rdfs:label xml:lang="fr">a été assigné par</rdfs:label>
	<rdfs:label xml:lang="pt">foi atribuído por</rdfs:label>
	<rdfs:label xml:lang="en">was assigned by</rdfs:label>
	<rdfs:label xml:lang="de">wurde zugewiesen durch</rdfs:label>
	<rdfs:label xml:lang="el">αποδόθηκε ως ιδιότητα από</rdfs:label>
	<rdfs:label xml:lang="ru">был присвоен посредством</rdfs:label>
	<rdfs:label xml:lang="zh">被分配</rdfs:label>
</rdf:Description>

<rdf:Description rdf:about="http://www.cidoc-crm.org/cidoc-crm/P38_deassigned">
	<rdf:type rdf:resource="http://www.w3.org/2002/07/owl#ObjectProperty"/>
	<rdfs:subPropertyOf rdf:resource="http://www.cidoc-crm.org/cidoc-crm/P141_assigned"/>
	<owl:inverseOf rdf:resource="http://www.cidoc-crm.org/cidoc-crm/P38i_was_deassigned_by"/>
	<rdfs:domain rdf:resource="http://www.cidoc-crm.org/cidoc-crm/E15_Identifier_Assignment"/>
	<rdfs:range rdf:resource="http://www.cidoc-crm.org/cidoc-crm/E42_Identifier"/>
	<rdfs:comment xml:lang="en">This property records the identifier that was deassigned from an instance of E1 CRM Entity.
De-assignment of an identifier may be necessary when an item is taken out of an inventory, a new numbering system is introduced or items are merged or split up.
The same identifier may be deassigned on more than one occasion.</rdfs:comment>
	<rdfs:label xml:lang="fr">a retiré l'assignation</rdfs:label>
	<rdfs:label xml:lang="en">deassigned</rdfs:label>
	<rdfs:label xml:lang="de">hob Zuweisung auf von</rdfs:label>
	<rdfs:label xml:lang="pt">retirou a atribuição do</rdfs:label>
	<rdfs:label xml:lang="el">ακύρωσε</rdfs:label>
	<rdfs:label xml:lang="ru">отменил назначение</rdfs:label>
	<rdfs:label xml:lang="zh">取消了</rdfs:label>
</rdf:Description>

<rdf:Description rdf:about="http://www.cidoc-crm.org/cidoc-crm/P38i_was_deassigned_by">
	<rdf:type rdf:resource="http://www.w3.org/2002/07/owl#ObjectProperty"/>
	<rdfs:subPropertyOf rdf:resource="http://www.cidoc-crm.org/cidoc-crm/P141i_was_assigned_by"/>
	<rdfs:domain rdf:resource="http://www.cidoc-crm.org/cidoc-crm/E42_Identifier"/>
	<rdfs:range rdf:resource="http://www.cidoc-crm.org/cidoc-crm/E15_Identifier_Assignment"/>
	<rdfs:label xml:lang="fr">a été retiré par</rdfs:label>
	<rdfs:label xml:lang="pt">foi retirada a atribuição por</rdfs:label>
	<rdfs:label xml:lang="en">was deassigned by</rdfs:label>
	<rdfs:label xml:lang="de">wurde aufgehoben durch</rdfs:label>
	<rdfs:label xml:lang="el">ακυρώθηκε από</rdfs:label>
	<rdfs:label xml:lang="ru">был отменен посредством</rdfs:label>
	<rdfs:label xml:lang="zh">被取消</rdfs:label>
</rdf:Description>

<rdf:Description rdf:about="http://www.cidoc-crm.org/cidoc-crm/P39_measured">
	<rdf:type rdf:resource="http://www.w3.org/2002/07/owl#ObjectProperty"/>
	<rdfs:subPropertyOf rdf:resource="http://www.cidoc-crm.org/cidoc-crm/P140_assigned_attribute_to"/>
	<owl:inverseOf rdf:resource="http://www.cidoc-crm.org/cidoc-crm/P39i_was_measured_by"/>
	<rdfs:domain rdf:resource="http://www.cidoc-crm.org/cidoc-crm/E16_Measurement"/>
	<rdfs:range rdf:resource="http://www.cidoc-crm.org/cidoc-crm/E18_Physical_Thing"/>
	<rdfs:comment xml:lang="en">This property associates an instance of E16 Measurement with the instance of E18 Physical Thing upon which it acted. The instance of E16 Measurement is specific to the measured object. An instance of E18 Physical Thing may be measured more than once with different results, constituting different instances of E16 Measurement.</rdfs:comment>
	<rdfs:label xml:lang="fr">a mesuré</rdfs:label>
	<rdfs:label xml:lang="en">measured</rdfs:label>
	<rdfs:label xml:lang="pt">mediu</rdfs:label>
	<rdfs:label xml:lang="de">vermaß</rdfs:label>
	<rdfs:label xml:lang="el">μέτρησε</rdfs:label>
	<rdfs:label xml:lang="ru">измерил</rdfs:label>
	<rdfs:label xml:lang="zh">测量了</rdfs:label>
</rdf:Description>

<rdf:Description rdf:about="http://www.cidoc-crm.org/cidoc-crm/P39i_was_measured_by">
	<rdf:type rdf:resource="http://www.w3.org/2002/07/owl#ObjectProperty"/>
	<rdfs:subPropertyOf rdf:resource="http://www.cidoc-crm.org/cidoc-crm/P140i_was_attributed_by"/>
	<rdfs:domain rdf:resource="http://www.cidoc-crm.org/cidoc-crm/E18_Physical_Thing"/>
	<rdfs:range rdf:resource="http://www.cidoc-crm.org/cidoc-crm/E16_Measurement"/>
	<rdfs:label xml:lang="fr">a été mesuré par</rdfs:label>
	<rdfs:label xml:lang="pt">foi medida por</rdfs:label>
	<rdfs:label xml:lang="en">was measured by</rdfs:label>
	<rdfs:label xml:lang="de">wurde vermessen durch</rdfs:label>
	<rdfs:label xml:lang="el">μετρήθηκε από</rdfs:label>
	<rdfs:label xml:lang="ru">был измерен посредством</rdfs:label>
	<rdfs:label xml:lang="zh">被测量</rdfs:label>
</rdf:Description>

<rdf:Description rdf:about="http://www.cidoc-crm.org/cidoc-crm/P40_observed_dimension">
	<rdf:type rdf:resource="http://www.w3.org/2002/07/owl#ObjectProperty"/>
	<rdfs:subPropertyOf rdf:resource="http://www.cidoc-crm.org/cidoc-crm/P141_assigned"/>
	<owl:inverseOf rdf:resource="http://www.cidoc-crm.org/cidoc-crm/P40i_was_observed_in"/>
	<rdfs:domain rdf:resource="http://www.cidoc-crm.org/cidoc-crm/E16_Measurement"/>
	<rdfs:range rdf:resource="http://www.cidoc-crm.org/cidoc-crm/E54_Dimension"/>
	<rdfs:comment xml:lang="en">This property records the dimension that was observed in an E16 Measurement Event.
E54 Dimension can be any quantifiable aspect of E70 Thing. Weight, image colour depth and monetary value are dimensions in this sense. One measurement activity may determine more than one dimension of one object.
Dimensions may be determined either by direct observation or using recorded evidence. In the latter case the measured Thing does not need to be present or extant.
Even though knowledge of the value of a dimension requires measurement, the dimension may be an object of discourse prior to, or even without, any measurement being made.</rdfs:comment>
	<rdfs:label xml:lang="fr">a relevé comme dimension</rdfs:label>
	<rdfs:label xml:lang="de">beobachtete Dimension</rdfs:label>
	<rdfs:label xml:lang="en">observed dimension</rdfs:label>
	<rdfs:label xml:lang="pt">verificou a dimensão</rdfs:label>
	<rdfs:label xml:lang="el">παρατήρησε</rdfs:label>
	<rdfs:label xml:lang="ru">определил величину</rdfs:label>
	<rdfs:label xml:lang="zh">观测度量规格</rdfs:label>
</rdf:Description>

<rdf:Description rdf:about="http://www.cidoc-crm.org/cidoc-crm/P40i_was_observed_in">
	<rdf:type rdf:resource="http://www.w3.org/2002/07/owl#ObjectProperty"/>
	<rdfs:subPropertyOf rdf:resource="http://www.cidoc-crm.org/cidoc-crm/P141i_was_assigned_by"/>
	<rdfs:domain rdf:resource="http://www.cidoc-crm.org/cidoc-crm/E54_Dimension"/>
	<rdfs:range rdf:resource="http://www.cidoc-crm.org/cidoc-crm/E16_Measurement"/>
	<rdfs:label xml:lang="fr">a été relevé par</rdfs:label>
	<rdfs:label xml:lang="pt">foi verificada durante</rdfs:label>
	<rdfs:label xml:lang="en">was observed in</rdfs:label>
	<rdfs:label xml:lang="de">wurde beobachtet in</rdfs:label>
	<rdfs:label xml:lang="el">παρατηρήθηκε από</rdfs:label>
	<rdfs:label xml:lang="ru">наблюдался в</rdfs:label>
	<rdfs:label xml:lang="zh">被观测</rdfs:label>
</rdf:Description>

<rdf:Description rdf:about="http://www.cidoc-crm.org/cidoc-crm/P41_classified">
	<rdf:type rdf:resource="http://www.w3.org/2002/07/owl#ObjectProperty"/>
	<rdfs:subPropertyOf rdf:resource="http://www.cidoc-crm.org/cidoc-crm/P140_assigned_attribute_to"/>
	<owl:inverseOf rdf:resource="http://www.cidoc-crm.org/cidoc-crm/P41i_was_classified_by"/>
	<rdfs:domain rdf:resource="http://www.cidoc-crm.org/cidoc-crm/E17_Type_Assignment"/>
	<rdfs:range rdf:resource="http://www.cidoc-crm.org/cidoc-crm/E1_CRM_Entity"/>
	<rdfs:comment xml:lang="en">This property records the item to which a type was assigned in an E17 Type Assignment activity.
Any instance of a CIDOC CRM entity may be assigned a type through type assignment. Type assignment events allow a more detailed path from E1 CRM Entity through P41i was classified by, E17 Type Assignment, P42 assigned, to E55 Type for assigning types to objects compared to the shortcut offered by P2 has type (is type of).</rdfs:comment>
	<rdfs:label xml:lang="fr">a classifié</rdfs:label>
	<rdfs:label xml:lang="pt">classificou</rdfs:label>
	<rdfs:label xml:lang="en">classified</rdfs:label>
	<rdfs:label xml:lang="de">klassifizierte</rdfs:label>
	<rdfs:label xml:lang="el">χαρακτήρισε</rdfs:label>
	<rdfs:label xml:lang="ru">классифицировал</rdfs:label>
	<rdfs:label xml:lang="zh">分类</rdfs:label>
</rdf:Description>

<rdf:Description rdf:about="http://www.cidoc-crm.org/cidoc-crm/P41i_was_classified_by">
	<rdf:type rdf:resource="http://www.w3.org/2002/07/owl#ObjectProperty"/>
	<rdfs:subPropertyOf rdf:resource="http://www.cidoc-crm.org/cidoc-crm/P140i_was_attributed_by"/>
	<rdfs:domain rdf:resource="http://www.cidoc-crm.org/cidoc-crm/E1_CRM_Entity"/>
	<rdfs:range rdf:resource="http://www.cidoc-crm.org/cidoc-crm/E17_Type_Assignment"/>
	<rdfs:label xml:lang="fr">a été classifié par</rdfs:label>
	<rdfs:label xml:lang="pt">foi classificada por</rdfs:label>
	<rdfs:label xml:lang="en">was classified by</rdfs:label>
	<rdfs:label xml:lang="de">wurde klassifiziert durch</rdfs:label>
	<rdfs:label xml:lang="el">χαρακτηρίσθηκε από</rdfs:label>
	<rdfs:label xml:lang="ru">был классифицирован посредством</rdfs:label>
	<rdfs:label xml:lang="zh">被分类</rdfs:label>
</rdf:Description>

<rdf:Description rdf:about="http://www.cidoc-crm.org/cidoc-crm/P42_assigned">
	<rdf:type rdf:resource="http://www.w3.org/2002/07/owl#ObjectProperty"/>
	<rdfs:subPropertyOf rdf:resource="http://www.cidoc-crm.org/cidoc-crm/P141_assigned"/>
	<owl:inverseOf rdf:resource="http://www.cidoc-crm.org/cidoc-crm/P42i_was_assigned_by"/>
	<rdfs:domain rdf:resource="http://www.cidoc-crm.org/cidoc-crm/E17_Type_Assignment"/>
	<rdfs:range rdf:resource="http://www.cidoc-crm.org/cidoc-crm/E55_Type"/>
	<rdfs:comment xml:lang="en">This property records the type that was assigned to an entity by an E17 Type Assignment activity.
Type assignment events allow a more detailed path from E1 CRM Entity through P41i was classified by, E17 Type Assignment, P42 assigned, to E55 Type for assigning types to objects compared to the shortcut offered by P2 has type (is type of).
For example, a fragment of an antique vessel could be assigned the type “attic red figured belly handled amphora” by expert A. The same fragment could be assigned the type “shoulder handled amphora” by expert B.
A Type may be intellectually constructed independent from assigning an instance of it.</rdfs:comment>
	<rdfs:label xml:lang="fr">a assigné</rdfs:label>
	<rdfs:label xml:lang="en">assigned</rdfs:label>
	<rdfs:label xml:lang="pt">atribuiu</rdfs:label>
	<rdfs:label xml:lang="de">wies zu</rdfs:label>
	<rdfs:label xml:lang="el">απέδωσε ως ιδιότητα</rdfs:label>
	<rdfs:label xml:lang="ru">назначил</rdfs:label>
	<rdfs:label xml:lang="zh">分配类型</rdfs:label>
</rdf:Description>

<rdf:Description rdf:about="http://www.cidoc-crm.org/cidoc-crm/P42i_was_assigned_by">
	<rdf:type rdf:resource="http://www.w3.org/2002/07/owl#ObjectProperty"/>
	<rdfs:subPropertyOf rdf:resource="http://www.cidoc-crm.org/cidoc-crm/P141i_was_assigned_by"/>
	<rdfs:domain rdf:resource="http://www.cidoc-crm.org/cidoc-crm/E55_Type"/>
	<rdfs:range rdf:resource="http://www.cidoc-crm.org/cidoc-crm/E17_Type_Assignment"/>
	<rdfs:label xml:lang="fr">a été assigné par</rdfs:label>
	<rdfs:label xml:lang="pt">foi atribuído por</rdfs:label>
	<rdfs:label xml:lang="en">was assigned by</rdfs:label>
	<rdfs:label xml:lang="de">wurde zugewiesen durch</rdfs:label>
	<rdfs:label xml:lang="el">αποδόθηκε από</rdfs:label>
	<rdfs:label xml:lang="ru">был присвоен посредством</rdfs:label>
	<rdfs:label xml:lang="zh">被分配类型</rdfs:label>
</rdf:Description>

<rdf:Description rdf:about="http://www.cidoc-crm.org/cidoc-crm/P43_has_dimension">
	<rdf:type rdf:resource="http://www.w3.org/2002/07/owl#ObjectProperty"/>
	<owl:inverseOf rdf:resource="http://www.cidoc-crm.org/cidoc-crm/P43i_is_dimension_of"/>
	<rdfs:domain rdf:resource="http://www.cidoc-crm.org/cidoc-crm/E70_Thing"/>
	<rdfs:range rdf:resource="http://www.cidoc-crm.org/cidoc-crm/E54_Dimension"/>
	<rdfs:comment xml:lang="en">This property records an instance of E54 Dimension of some instance of E70 Thing.
In the case that the recorded property is a result of a measurement of an instance of E18 Physical Thing, this property is a shortcut of the more fully developed path from E18 Physical Thing through P39i was measured by, E16 Measurement, P40 observed dimension to E54 Dimension.
It offers no information about how and when an E54 Dimension was established, nor by whom. Knowledge about an instance of E54 Dimension need not be the result of a measurement; it may be the result of evaluating data or other information, which should be documented as an instance of E13 Attribute Assignment.
An instance of E54 Dimension is specific to an instance of E70 Thing.</rdfs:comment>
	<rdfs:label xml:lang="fr">a pour dimension</rdfs:label>
	<rdfs:label xml:lang="en">has dimension</rdfs:label>
	<rdfs:label xml:lang="de">hat Dimension</rdfs:label>
	<rdfs:label xml:lang="pt">tem dimensão</rdfs:label>
	<rdfs:label xml:lang="el">έχει μέγεθος</rdfs:label>
	<rdfs:label xml:lang="ru">имеет величину</rdfs:label>
	<rdfs:label xml:lang="zh">有度量规格</rdfs:label>
</rdf:Description>

<rdf:Description rdf:about="http://www.cidoc-crm.org/cidoc-crm/P43i_is_dimension_of">
	<rdf:type rdf:resource="http://www.w3.org/2002/07/owl#ObjectProperty"/>
	<rdfs:domain rdf:resource="http://www.cidoc-crm.org/cidoc-crm/E54_Dimension"/>
	<rdfs:range rdf:resource="http://www.cidoc-crm.org/cidoc-crm/E70_Thing"/>
	<rdfs:label xml:lang="fr">est la dimension de</rdfs:label>
	<rdfs:label xml:lang="en">is dimension of</rdfs:label>
	<rdfs:label xml:lang="de">ist Dimension von</rdfs:label>
	<rdfs:label xml:lang="pt">é dimensão de</rdfs:label>
	<rdfs:label xml:lang="el">είναι μέγεθος του</rdfs:label>
	<rdfs:label xml:lang="ru">является величиной для</rdfs:label>
	<rdfs:label xml:lang="zh">是度量规格</rdfs:label>
</rdf:Description>

<rdf:Description rdf:about="http://www.cidoc-crm.org/cidoc-crm/P44_has_condition">
	<rdf:type rdf:resource="http://www.w3.org/2002/07/owl#ObjectProperty"/>
	<owl:inverseOf rdf:resource="http://www.cidoc-crm.org/cidoc-crm/P44i_is_condition_of"/>
	<rdfs:domain rdf:resource="http://www.cidoc-crm.org/cidoc-crm/E18_Physical_Thing"/>
	<rdfs:range rdf:resource="http://www.cidoc-crm.org/cidoc-crm/E3_Condition_State"/>
	<rdfs:comment xml:lang="en">This property records an E3 Condition State for some E18 Physical Thing.
This property is a shortcut of the more fully developed path from E18 Physical Thing through P34i was assessed by, E14 Condition Assessment, P35 has identified to E3 Condition State. It offers no information about how and when the E3 Condition State was established, nor by whom.
An instance of E3 Condition State is specific to an instance of E18 Physical Thing.</rdfs:comment>
	<rdfs:label xml:lang="fr">a pour état matériel</rdfs:label>
	<rdfs:label xml:lang="en">has condition</rdfs:label>
	<rdfs:label xml:lang="de">hat Zustand</rdfs:label>
	<rdfs:label xml:lang="pt">tem estado material</rdfs:label>
	<rdfs:label xml:lang="el">έχει κατάσταση</rdfs:label>
	<rdfs:label xml:lang="ru">имеет условие</rdfs:label>
	<rdfs:label xml:lang="zh">有状况</rdfs:label>
</rdf:Description>

<rdf:Description rdf:about="http://www.cidoc-crm.org/cidoc-crm/P44i_is_condition_of">
	<rdf:type rdf:resource="http://www.w3.org/2002/07/owl#ObjectProperty"/>
	<rdfs:domain rdf:resource="http://www.cidoc-crm.org/cidoc-crm/E3_Condition_State"/>
	<rdfs:range rdf:resource="http://www.cidoc-crm.org/cidoc-crm/E18_Physical_Thing"/>
	<rdfs:label xml:lang="fr">est l'état matériel de</rdfs:label>
	<rdfs:label xml:lang="pt">estado material de</rdfs:label>
	<rdfs:label xml:lang="en">is condition of</rdfs:label>
	<rdfs:label xml:lang="de">ist Zustand von</rdfs:label>
	<rdfs:label xml:lang="el">είναι κατάσταση του</rdfs:label>
	<rdfs:label xml:lang="ru">является условием для</rdfs:label>
	<rdfs:label xml:lang="zh">是状况</rdfs:label>
</rdf:Description>

<rdf:Description rdf:about="http://www.cidoc-crm.org/cidoc-crm/P45_consists_of">
	<rdf:type rdf:resource="http://www.w3.org/2002/07/owl#ObjectProperty"/>
	<owl:inverseOf rdf:resource="http://www.cidoc-crm.org/cidoc-crm/P45i_is_incorporated_in"/>
	<rdfs:domain rdf:resource="http://www.cidoc-crm.org/cidoc-crm/E18_Physical_Thing"/>
	<rdfs:range rdf:resource="http://www.cidoc-crm.org/cidoc-crm/E57_Material"/>
	<rdfs:comment xml:lang="en">This property identifies the instances of E57 Materials of which an instance of E18 Physical Thing is composed.
All physical things consist of physical materials. P45 consists of (is incorporated in) allows the different materials to be recorded. P45 consists of (is incorporated in) refers here to observed material as opposed to the consumed raw material.
A material, such as a theoretical alloy, may not have any physical instances.</rdfs:comment>
	<rdfs:label xml:lang="de">besteht aus</rdfs:label>
	<rdfs:label xml:lang="fr">comprend</rdfs:label>
	<rdfs:label xml:lang="pt">consiste de</rdfs:label>
	<rdfs:label xml:lang="en">consists of</rdfs:label>
	<rdfs:label xml:lang="el">αποτελείται από</rdfs:label>
	<rdfs:label xml:lang="ru">составлен из</rdfs:label>
	<rdfs:label xml:lang="zh">包含</rdfs:label>
</rdf:Description>

<rdf:Description rdf:about="http://www.cidoc-crm.org/cidoc-crm/P45i_is_incorporated_in">
	<rdf:type rdf:resource="http://www.w3.org/2002/07/owl#ObjectProperty"/>
	<rdfs:domain rdf:resource="http://www.cidoc-crm.org/cidoc-crm/E57_Material"/>
	<rdfs:range rdf:resource="http://www.cidoc-crm.org/cidoc-crm/E18_Physical_Thing"/>
	<rdfs:label xml:lang="fr">est inclus dans</rdfs:label>
	<rdfs:label xml:lang="pt">está presente em</rdfs:label>
	<rdfs:label xml:lang="en">is incorporated in</rdfs:label>
	<rdfs:label xml:lang="de">ist enthalten in</rdfs:label>
	<rdfs:label xml:lang="el">είναι ενσωματωμένος/η/ο σε</rdfs:label>
	<rdfs:label xml:lang="ru">входит в состав</rdfs:label>
	<rdfs:label xml:lang="zh">结合在</rdfs:label>
</rdf:Description>

<rdf:Description rdf:about="http://www.cidoc-crm.org/cidoc-crm/P46_is_composed_of">
	<rdf:type rdf:resource="http://www.w3.org/2002/07/owl#ObjectProperty"/>
	<owl:inverseOf rdf:resource="http://www.cidoc-crm.org/cidoc-crm/P46i_forms_part_of"/>
	<rdfs:domain rdf:resource="http://www.cidoc-crm.org/cidoc-crm/E18_Physical_Thing"/>
	<rdfs:range rdf:resource="http://www.cidoc-crm.org/cidoc-crm/E18_Physical_Thing"/>
	<rdfs:comment xml:lang="en">This property associates an instance of E18 Physical Thing with another instance of Physical Thing that forms part of it. The spatial extent of the composing part is included in the spatial extent of the whole.
Component elements, since they are themselves instances of E18 Physical Thing, may be further analysed into sub-components, thereby creating a hierarchy of part decomposition. An instance of E18 Physical Thing may be shared between multiple wholes, for example two buildings may share a common wall. This property does not specify when and for how long a component element resided in the respective whole. If a component is not part of a whole from the beginning of existence or until the end of existence of the whole, the classes E79 Part Addition and E90 Part Removal can be used to document when a component became part of a particular whole and/or when it stopped being a part of it. For the time-span of being part of the respective whole, the component is completely contained in the place the whole occupies.
This property is intended to describe specific components that are individually documented, rather than general aspects. Overall descriptions of the structure of an instance of E18 Physical Thing are captured by the P3 has note property.
The instances of E57 Material of which an instance of E18 Physical Thing is composed should be documented using P45 consists of (is incorporated in).
This property is transitive and asymmetric.</rdfs:comment>
	<rdfs:label xml:lang="fr">est composé de</rdfs:label>
	<rdfs:label xml:lang="en">is composed of</rdfs:label>
	<rdfs:label xml:lang="de">ist zusammengesetzt aus</rdfs:label>
	<rdfs:label xml:lang="pt">é composto de</rdfs:label>
	<rdfs:label xml:lang="el">αποτελείται από</rdfs:label>
	<rdfs:label xml:lang="ru">составлен из</rdfs:label>
	<rdfs:label xml:lang="zh">组成成分是</rdfs:label>
</rdf:Description>

<rdf:Description rdf:about="http://www.cidoc-crm.org/cidoc-crm/P46i_forms_part_of">
	<rdf:type rdf:resource="http://www.w3.org/2002/07/owl#ObjectProperty"/>
	<rdfs:domain rdf:resource="http://www.cidoc-crm.org/cidoc-crm/E18_Physical_Thing"/>
	<rdfs:range rdf:resource="http://www.cidoc-crm.org/cidoc-crm/E18_Physical_Thing"/>
	<rdfs:label xml:lang="de">bildet Teil von</rdfs:label>
	<rdfs:label xml:lang="fr">fait partie de</rdfs:label>
	<rdfs:label xml:lang="pt">faz parte de</rdfs:label>
	<rdfs:label xml:lang="en">forms part of</rdfs:label>
	<rdfs:label xml:lang="el">αποτελεί μέρος του/της</rdfs:label>
	<rdfs:label xml:lang="ru">формирует часть</rdfs:label>
	<rdfs:label xml:lang="zh">构成部分</rdfs:label>
</rdf:Description>

<rdf:Description rdf:about="http://www.cidoc-crm.org/cidoc-crm/P48_has_preferred_identifier">
	<rdf:type rdf:resource="http://www.w3.org/2002/07/owl#ObjectProperty"/>
	<rdfs:subPropertyOf rdf:resource="http://www.cidoc-crm.org/cidoc-crm/P1_is_identified_by"/>
	<owl:inverseOf rdf:resource="http://www.cidoc-crm.org/cidoc-crm/P48i_is_preferred_identifier_of"/>
	<rdfs:domain rdf:resource="http://www.cidoc-crm.org/cidoc-crm/E1_CRM_Entity"/>
	<rdfs:range rdf:resource="http://www.cidoc-crm.org/cidoc-crm/E42_Identifier"/>
	<rdfs:comment xml:lang="en">This property records the preferred instance of E42 Identifier that was used to identify an instance of E1 CRM Entity at the time this property was recorded.
More than one preferred identifier may have been assigned to an item over time.
Use of this property requires an external mechanism for assigning temporal validity to the respective CIDOC CRM instance.
The fact that an identifier is a preferred one for an organisation can be better expressed in a context independent form by assigning a suitable instance of E55 Type to the respective instance of E15 Identifier Assignment using the P2 has type property.</rdfs:comment>
	<rdfs:label xml:lang="fr">a pour identifiant préférentiel</rdfs:label>
	<rdfs:label xml:lang="en">has preferred identifier</rdfs:label>
	<rdfs:label xml:lang="de">hat bevorzugtes Kennzeichen</rdfs:label>
	<rdfs:label xml:lang="pt">tem identificador preferido</rdfs:label>
	<rdfs:label xml:lang="el">έχει προτιμώμενο αναγνωριστικό</rdfs:label>
	<rdfs:label xml:lang="ru">имеет предпочтительный идентификатор</rdfs:label>
	<rdfs:label xml:lang="zh">有优选标识符</rdfs:label>
</rdf:Description>

<rdf:Description rdf:about="http://www.cidoc-crm.org/cidoc-crm/P48i_is_preferred_identifier_of">
	<rdf:type rdf:resource="http://www.w3.org/2002/07/owl#ObjectProperty"/>
	<rdfs:subPropertyOf rdf:resource="http://www.cidoc-crm.org/cidoc-crm/P1i_identifies"/>
	<rdfs:domain rdf:resource="http://www.cidoc-crm.org/cidoc-crm/E42_Identifier"/>
	<rdfs:range rdf:resource="http://www.cidoc-crm.org/cidoc-crm/E1_CRM_Entity"/>
	<rdfs:label xml:lang="fr">est l’identifiant préférentiel de</rdfs:label>
	<rdfs:label xml:lang="en">is preferred identifier of</rdfs:label>
	<rdfs:label xml:lang="de">ist bevorzugtes Kennzeichen für</rdfs:label>
	<rdfs:label xml:lang="pt">é o identificador preferido de</rdfs:label>
	<rdfs:label xml:lang="el">είναι προτιμώμενο αναγνωριστικό</rdfs:label>
	<rdfs:label xml:lang="ru">является предпочтительным идентификатором для</rdfs:label>
	<rdfs:label xml:lang="zh">是优选标识符</rdfs:label>
</rdf:Description>

<rdf:Description rdf:about="http://www.cidoc-crm.org/cidoc-crm/P49_has_former_or_current_keeper">
	<rdf:type rdf:resource="http://www.w3.org/2002/07/owl#ObjectProperty"/>
	<owl:inverseOf rdf:resource="http://www.cidoc-crm.org/cidoc-crm/P49i_is_former_or_current_keeper_of"/>
	<rdfs:domain rdf:resource="http://www.cidoc-crm.org/cidoc-crm/E18_Physical_Thing"/>
	<rdfs:range rdf:resource="http://www.cidoc-crm.org/cidoc-crm/E39_Actor"/>
	<rdfs:comment xml:lang="en">This property identifies the instance of E39 Actor who has or has had custody of an instance of E18 Physical Thing at some time. This property leaves open the question if parts of this physical thing have been added or removed during the time-spans it has been under the custody of this actor, but it is required that at least a part which can unambiguously be identified as representing the whole has been under this custody for its whole time. The way, in which a representative part is defined, should ensure that it is unambiguous who keeps a part and who the whole and should be consistent with the identity criteria of the kept instance of E18 Physical Thing.
The distinction with P50 has current keeper (is current keeper of) is that P49 has former or current keeper (is former or current keeper of) leaves open the question as to whether the specified keepers are current.
This property is a shortcut for the more detailed path from E18 Physical Thing through P30i custody transferred through, E10 Transfer of Custody, P28 custody surrendered by or P29 custody received by to E39 Actor.</rdfs:comment>
	<rdfs:label xml:lang="fr">a pour actant détenteur actuel ou antérieur</rdfs:label>
	<rdfs:label xml:lang="en">has former or current keeper</rdfs:label>
	<rdfs:label xml:lang="de">hat früheren oder derzeitigen Betreuer</rdfs:label>
	<rdfs:label xml:lang="pt">é ou foi guardada por</rdfs:label>
	<rdfs:label xml:lang="el">είναι ή ήταν στην κατοχή του</rdfs:label>
	<rdfs:label xml:lang="ru">имеет бывшего или текущего смотрителя</rdfs:label>
	<rdfs:label xml:lang="zh">有以往或当前保管者</rdfs:label>
</rdf:Description>

<rdf:Description rdf:about="http://www.cidoc-crm.org/cidoc-crm/P49i_is_former_or_current_keeper_of">
	<rdf:type rdf:resource="http://www.w3.org/2002/07/owl#ObjectProperty"/>
	<rdfs:domain rdf:resource="http://www.cidoc-crm.org/cidoc-crm/E39_Actor"/>
	<rdfs:range rdf:resource="http://www.cidoc-crm.org/cidoc-crm/E18_Physical_Thing"/>
	<rdfs:label xml:lang="fr">est l’actant détenteur actuel ou antérieur de</rdfs:label>
	<rdfs:label xml:lang="en">is former or current keeper of</rdfs:label>
	<rdfs:label xml:lang="de">ist früherer oder derzeitiger Betreuer von</rdfs:label>
	<rdfs:label xml:lang="pt">é ou foi guardador de</rdfs:label>
	<rdfs:label xml:lang="el">κατέχει ή κατείχε</rdfs:label>
	<rdfs:label xml:lang="ru">является бывшим или текущим смотрителем для</rdfs:label>
	<rdfs:label xml:lang="zh">是以往或当前保管者</rdfs:label>
</rdf:Description>

<rdf:Description rdf:about="http://www.cidoc-crm.org/cidoc-crm/P4_has_time-span">
	<rdf:type rdf:resource="http://www.w3.org/2002/07/owl#ObjectProperty"/>
	<owl:inverseOf rdf:resource="http://www.cidoc-crm.org/cidoc-crm/P4i_is_time-span_of"/>
	<rdfs:domain rdf:resource="http://www.cidoc-crm.org/cidoc-crm/E2_Temporal_Entity"/>
	<rdfs:range rdf:resource="http://www.cidoc-crm.org/cidoc-crm/E52_Time-Span"/>
	<rdfs:comment xml:lang="en">This property associates an instance of E2 Temporal Entity with the instance of E52 Time-Span during which it was on-going. The associated instance of E52 Time-Span is understood as the real time-span during which the phenomena making up the temporal entity instance were active. More than one instance of E2 Temporal Entity may share a common instance of E52 Time-Span only if they come into being and end being due to identical declarations or events.</rdfs:comment>
	<rdfs:label xml:lang="fr">a pour intervalle temporel</rdfs:label>
	<rdfs:label xml:lang="en">has time-span</rdfs:label>
	<rdfs:label xml:lang="de">hat Zeitspanne</rdfs:label>
	<rdfs:label xml:lang="pt">tem período de tempo</rdfs:label>
	<rdfs:label xml:lang="el">βρισκόταν σε εξέλιξη</rdfs:label>
	<rdfs:label xml:lang="ru">имеет временной отрезок</rdfs:label>
	<rdfs:label xml:lang="zh">发生时段是</rdfs:label>
</rdf:Description>

<rdf:Description rdf:about="http://www.cidoc-crm.org/cidoc-crm/P4i_is_time-span_of">
	<rdf:type rdf:resource="http://www.w3.org/2002/07/owl#ObjectProperty"/>
	<rdfs:domain rdf:resource="http://www.cidoc-crm.org/cidoc-crm/E52_Time-Span"/>
	<rdfs:range rdf:resource="http://www.cidoc-crm.org/cidoc-crm/E2_Temporal_Entity"/>
	<rdfs:label xml:lang="fr">est l’intervalle temporel de</rdfs:label>
	<rdfs:label xml:lang="en">is time-span of</rdfs:label>
	<rdfs:label xml:lang="de">ist Zeitspanne von</rdfs:label>
	<rdfs:label xml:lang="pt">é o período de tempo de</rdfs:label>
	<rdfs:label xml:lang="el">είναι χρονικό διάστημα του/της</rdfs:label>
	<rdfs:label xml:lang="ru">является временным отрезком для</rdfs:label>
	<rdfs:label xml:lang="zh">是时段</rdfs:label>
</rdf:Description>

<rdf:Description rdf:about="http://www.cidoc-crm.org/cidoc-crm/P50_has_current_keeper">
	<rdf:type rdf:resource="http://www.w3.org/2002/07/owl#ObjectProperty"/>
	<rdfs:subPropertyOf rdf:resource="http://www.cidoc-crm.org/cidoc-crm/P49_has_former_or_current_keeper"/>
	<owl:inverseOf rdf:resource="http://www.cidoc-crm.org/cidoc-crm/P50i_is_current_keeper_of"/>
	<rdfs:domain rdf:resource="http://www.cidoc-crm.org/cidoc-crm/E18_Physical_Thing"/>
	<rdfs:range rdf:resource="http://www.cidoc-crm.org/cidoc-crm/E39_Actor"/>
	<rdfs:comment xml:lang="en">This property identifies the instance of E39 Actor that had custody of an instance of E18 Physical Thing at the time of validity of the record or database containing the statement that uses this property.
This property is a shortcut for the more detailed path from E18 Physical Thing through, P30i custody transferred through, E10 Transfer of Custody, P29 custody received by to E39 Actor, if and only if the custody has not been surrendered by the receiving actor at any later time</rdfs:comment>
	<rdfs:label xml:lang="fr">a pour actant détenteur actuel</rdfs:label>
	<rdfs:label xml:lang="en">has current keeper</rdfs:label>
	<rdfs:label xml:lang="de">hat derzeitigen Betreuer</rdfs:label>
	<rdfs:label xml:lang="pt">é guardada por</rdfs:label>
	<rdfs:label xml:lang="el">είναι στην κατοχή του</rdfs:label>
	<rdfs:label xml:lang="ru">имеет текущего смотрителя</rdfs:label>
	<rdfs:label xml:lang="zh">有当前保管者</rdfs:label>
</rdf:Description>

<rdf:Description rdf:about="http://www.cidoc-crm.org/cidoc-crm/P50i_is_current_keeper_of">
	<rdf:type rdf:resource="http://www.w3.org/2002/07/owl#ObjectProperty"/>
	<rdfs:subPropertyOf rdf:resource="http://www.cidoc-crm.org/cidoc-crm/P49i_is_former_or_current_keeper_of"/>
	<rdfs:domain rdf:resource="http://www.cidoc-crm.org/cidoc-crm/E39_Actor"/>
	<rdfs:range rdf:resource="http://www.cidoc-crm.org/cidoc-crm/E18_Physical_Thing"/>
	<rdfs:label xml:lang="fr">est l’actant détenteur actuel</rdfs:label>
	<rdfs:label xml:lang="en">is current keeper of</rdfs:label>
	<rdfs:label xml:lang="de">ist derzeitiger Betreuer von</rdfs:label>
	<rdfs:label xml:lang="pt">é guardador de</rdfs:label>
	<rdfs:label xml:lang="el">κατέχει</rdfs:label>
	<rdfs:label xml:lang="ru">является текущим смотрителем для</rdfs:label>
	<rdfs:label xml:lang="zh">是当前保管者</rdfs:label>
</rdf:Description>

<rdf:Description rdf:about="http://www.cidoc-crm.org/cidoc-crm/P51_has_former_or_current_owner">
	<rdf:type rdf:resource="http://www.w3.org/2002/07/owl#ObjectProperty"/>
	<owl:inverseOf rdf:resource="http://www.cidoc-crm.org/cidoc-crm/P51i_is_former_or_current_owner_of"/>
	<rdfs:domain rdf:resource="http://www.cidoc-crm.org/cidoc-crm/E18_Physical_Thing"/>
	<rdfs:range rdf:resource="http://www.cidoc-crm.org/cidoc-crm/E39_Actor"/>
	<rdfs:comment xml:lang="en">This property identifies an instance of E39 Actor that is or had been the legal owner (i.e. title holder) of an instance of E18 Physical Thing at some time.
The distinction with P52 has current owner (is current owner of) is that P51 has former or current owner (is former or current owner of) does not indicate whether the specified owners are current.
This property is a shortcut for the more detailed path from E18 Physical Thing through P24i changed ownership through, E8 Acquisition, P23 transferred title from, or P22 transferred title to to E39 Actor.</rdfs:comment>
	<rdfs:label xml:lang="fr">a pour propriétaire actuel ou antérieur</rdfs:label>
	<rdfs:label xml:lang="en">has former or current owner</rdfs:label>
	<rdfs:label xml:lang="de">hat früheren oder derzeitigen Besitzer</rdfs:label>
	<rdfs:label xml:lang="pt">é ou foi propriedade de</rdfs:label>
	<rdfs:label xml:lang="el">έχει ή είχε ιδιοκτήτη</rdfs:label>
	<rdfs:label xml:lang="ru">имеет бывшего или текущего владельца</rdfs:label>
	<rdfs:label xml:lang="zh">有以往或当前所有者</rdfs:label>
</rdf:Description>

<rdf:Description rdf:about="http://www.cidoc-crm.org/cidoc-crm/P51i_is_former_or_current_owner_of">
	<rdf:type rdf:resource="http://www.w3.org/2002/07/owl#ObjectProperty"/>
	<rdfs:domain rdf:resource="http://www.cidoc-crm.org/cidoc-crm/E39_Actor"/>
	<rdfs:range rdf:resource="http://www.cidoc-crm.org/cidoc-crm/E18_Physical_Thing"/>
	<rdfs:label xml:lang="fr">est l’actant propriétaire actuel ou antérieur de</rdfs:label>
	<rdfs:label xml:lang="en">is former or current owner of</rdfs:label>
	<rdfs:label xml:lang="de">ist früherer oder derzeitiger Besitzer von</rdfs:label>
	<rdfs:label xml:lang="pt">é ou foi proprietário de</rdfs:label>
	<rdfs:label xml:lang="el">είναι ή ήταν ιδιοκτήτης του/της</rdfs:label>
	<rdfs:label xml:lang="ru">является бывшим или текущим владельцем для</rdfs:label>
	<rdfs:label xml:lang="zh">是以往或当前所有者</rdfs:label>
</rdf:Description>

<rdf:Description rdf:about="http://www.cidoc-crm.org/cidoc-crm/P52_has_current_owner">
	<rdf:type rdf:resource="http://www.w3.org/2002/07/owl#ObjectProperty"/>
	<rdfs:subPropertyOf rdf:resource="http://www.cidoc-crm.org/cidoc-crm/P105_right_held_by"/>
	<rdfs:subPropertyOf rdf:resource="http://www.cidoc-crm.org/cidoc-crm/P51_has_former_or_current_owner"/>
	<owl:inverseOf rdf:resource="http://www.cidoc-crm.org/cidoc-crm/P52i_is_current_owner_of"/>
	<rdfs:domain rdf:resource="http://www.cidoc-crm.org/cidoc-crm/E18_Physical_Thing"/>
	<rdfs:range rdf:resource="http://www.cidoc-crm.org/cidoc-crm/E39_Actor"/>
	<rdfs:comment xml:lang="en">This property identifies the instance of E21 Person or E74 Group that was the owner of an instance of E18 Physical Thing at the time of validity of the record or database containing the statement that uses this property.
This property is a shortcut for the more detailed path from E18 Physical Thing through, P24i changed ownership through, E8 Acquisition, P22 transferred title to to E39 Actor, if and only if this acquisition event is the most recent.</rdfs:comment>
	<rdfs:label xml:lang="fr">a pour propriétaire actuel</rdfs:label>
	<rdfs:label xml:lang="en">has current owner</rdfs:label>
	<rdfs:label xml:lang="de">hat derzeitigen Besitzer</rdfs:label>
	<rdfs:label xml:lang="pt">é propriedade de</rdfs:label>
	<rdfs:label xml:lang="el">έχει ιδιοκτήτη</rdfs:label>
	<rdfs:label xml:lang="ru">имеет текущего владельца</rdfs:label>
	<rdfs:label xml:lang="zh">有当前所有者</rdfs:label>
</rdf:Description>

<rdf:Description rdf:about="http://www.cidoc-crm.org/cidoc-crm/P52i_is_current_owner_of">
	<rdf:type rdf:resource="http://www.w3.org/2002/07/owl#ObjectProperty"/>
	<rdfs:subPropertyOf rdf:resource="http://www.cidoc-crm.org/cidoc-crm/P105i_has_right_on"/>
	<rdfs:subPropertyOf rdf:resource="http://www.cidoc-crm.org/cidoc-crm/P51i_is_former_or_current_owner_of"/>
	<rdfs:domain rdf:resource="http://www.cidoc-crm.org/cidoc-crm/E39_Actor"/>
	<rdfs:range rdf:resource="http://www.cidoc-crm.org/cidoc-crm/E18_Physical_Thing"/>
	<rdfs:label xml:lang="fr">est l'actant propriétaire actuel de</rdfs:label>
	<rdfs:label xml:lang="en">is current owner of</rdfs:label>
	<rdfs:label xml:lang="de">ist derzeitiger Besitzer von</rdfs:label>
	<rdfs:label xml:lang="pt">é proprietário de</rdfs:label>
	<rdfs:label xml:lang="el">είναι ιδιοκτήτης του</rdfs:label>
	<rdfs:label xml:lang="ru">является текущим владельцем для</rdfs:label>
	<rdfs:label xml:lang="zh">是当前所有者</rdfs:label>
</rdf:Description>

<rdf:Description rdf:about="http://www.cidoc-crm.org/cidoc-crm/P53_has_former_or_current_location">
	<rdf:type rdf:resource="http://www.w3.org/2002/07/owl#ObjectProperty"/>
	<owl:inverseOf rdf:resource="http://www.cidoc-crm.org/cidoc-crm/P53i_is_former_or_current_location_of"/>
	<rdfs:domain rdf:resource="http://www.cidoc-crm.org/cidoc-crm/E18_Physical_Thing"/>
	<rdfs:range rdf:resource="http://www.cidoc-crm.org/cidoc-crm/E53_Place"/>
	<rdfs:comment xml:lang="en">This property identifies an instance of E53 Place as the former or current location of an instance of E18 Physical Thing.
In the case of instances of E19 Physical Object, the property does not allow any indication of the Time-Span during which the instance of E19 Physical Object was located at this instance of E53 Place, nor if this is the current location.
In the case of immobile objects, the Place would normally correspond to the Place of creation.
This property is a shortcut. A more detailed representation can make use of the fully developed (i.e. indirect) path from E19 Physical Object, though, P25i moved by, E9 Move, P26 moved to or P27 moved from to E53 Place.</rdfs:comment>
	<rdfs:label xml:lang="fr">a pour localisation actuelle ou antérieure</rdfs:label>
	<rdfs:label xml:lang="en">has former or current location</rdfs:label>
	<rdfs:label xml:lang="de">hat früheren oder derzeitigen Standort</rdfs:label>
	<rdfs:label xml:lang="pt">é ou foi localizada em</rdfs:label>
	<rdfs:label xml:lang="el">βρίσκεται ή βρισκόταν σε</rdfs:label>
	<rdfs:label xml:lang="ru">имеет текущее или бывшее местоположение</rdfs:label>
	<rdfs:label xml:lang="zh">有之前或当前位置</rdfs:label>
</rdf:Description>

<rdf:Description rdf:about="http://www.cidoc-crm.org/cidoc-crm/P53i_is_former_or_current_location_of">
	<rdf:type rdf:resource="http://www.w3.org/2002/07/owl#ObjectProperty"/>
	<rdfs:domain rdf:resource="http://www.cidoc-crm.org/cidoc-crm/E53_Place"/>
	<rdfs:range rdf:resource="http://www.cidoc-crm.org/cidoc-crm/E18_Physical_Thing"/>
	<rdfs:label xml:lang="fr">est la localisation actuelle ou antérieure de</rdfs:label>
	<rdfs:label xml:lang="en">is former or current location of</rdfs:label>
	<rdfs:label xml:lang="de">ist früherer oder derzeitiger Standort von</rdfs:label>
	<rdfs:label xml:lang="pt">é ou foi localização de</rdfs:label>
	<rdfs:label xml:lang="el">είναι ή ήταν θέση του</rdfs:label>
	<rdfs:label xml:lang="ru">является текущим или бывшим местоположением для</rdfs:label>
	<rdfs:label xml:lang="zh">是之前或当前位置</rdfs:label>
</rdf:Description>

<rdf:Description rdf:about="http://www.cidoc-crm.org/cidoc-crm/P54_has_current_permanent_location">
	<rdf:type rdf:resource="http://www.w3.org/2002/07/owl#ObjectProperty"/>
	<owl:inverseOf rdf:resource="http://www.cidoc-crm.org/cidoc-crm/P54i_is_current_permanent_location_of"/>
	<rdfs:domain rdf:resource="http://www.cidoc-crm.org/cidoc-crm/E19_Physical_Object"/>
	<rdfs:range rdf:resource="http://www.cidoc-crm.org/cidoc-crm/E53_Place"/>
	<rdfs:comment xml:lang="en">This property records the foreseen permanent location of an instance of E19 Physical Object at the time of validity of the record or database containing the statement that uses this property.
P54 has current permanent location (is current permanent location of) is similar to P55 has current location (currently holds). However, it indicates the E53 Place currently reserved for an object, such as the permanent storage location or a permanent exhibit location. The object may be temporarily removed from the permanent location, for example when used in temporary exhibitions or loaned to another institution. The object may never actually be located at its permanent location.</rdfs:comment>
	<rdfs:label xml:lang="fr">a actuellement pour localisation fixe</rdfs:label>
	<rdfs:label xml:lang="en">has current permanent location</rdfs:label>
	<rdfs:label xml:lang="de">hat derzeitigen permanenten Standort</rdfs:label>
	<rdfs:label xml:lang="pt">é localizado permanentemente em</rdfs:label>
	<rdfs:label xml:lang="el">έχει μόνιμη θέση</rdfs:label>
	<rdfs:label xml:lang="ru">имеет текущее постоянное местоположение</rdfs:label>
	<rdfs:label xml:lang="zh">有当前永久位置</rdfs:label>
</rdf:Description>

<rdf:Description rdf:about="http://www.cidoc-crm.org/cidoc-crm/P54i_is_current_permanent_location_of">
	<rdf:type rdf:resource="http://www.w3.org/2002/07/owl#ObjectProperty"/>
	<rdfs:domain rdf:resource="http://www.cidoc-crm.org/cidoc-crm/E53_Place"/>
	<rdfs:range rdf:resource="http://www.cidoc-crm.org/cidoc-crm/E19_Physical_Object"/>
	<rdfs:label xml:lang="fr">est actuellement la location fixe de</rdfs:label>
	<rdfs:label xml:lang="en">is current permanent location of</rdfs:label>
	<rdfs:label xml:lang="de">ist derzeitiger permanenter Standort von</rdfs:label>
	<rdfs:label xml:lang="pt">é localização permanente de</rdfs:label>
	<rdfs:label xml:lang="el">είναι μόνιμη θέση του/της</rdfs:label>
	<rdfs:label xml:lang="ru">является текущим постоянным местоположением для</rdfs:label>
	<rdfs:label xml:lang="zh">是当前永久位置</rdfs:label>
</rdf:Description>

<rdf:Description rdf:about="http://www.cidoc-crm.org/cidoc-crm/P55_has_current_location">
	<rdf:type rdf:resource="http://www.w3.org/2002/07/owl#ObjectProperty"/>
	<rdfs:subPropertyOf rdf:resource="http://www.cidoc-crm.org/cidoc-crm/P53_has_former_or_current_location"/>
	<owl:inverseOf rdf:resource="http://www.cidoc-crm.org/cidoc-crm/P55i_currently_holds"/>
	<rdfs:domain rdf:resource="http://www.cidoc-crm.org/cidoc-crm/E19_Physical_Object"/>
	<rdfs:range rdf:resource="http://www.cidoc-crm.org/cidoc-crm/E53_Place"/>
	<rdfs:comment xml:lang="en">This property records the location of an instance of E19 Physical Object at the time of validity of the record or database containing the statement that uses this property.
This property is a specialisation of P53 has former or current location (is former or current location of). It indicates that the instance of E53 Place associated with the instance of E19 Physical Object is the current location of the object. The property does not allow any indication of how long the object has been at the current location.
This property is a shortcut. A more detailed representation can make use of the fully developed (i.e., indirect) path from E19 Physical Object, through, P25i moved by, E9 Move, P26 moved to to E53 Place if and only if this Move is the most recent.</rdfs:comment>
	<rdfs:label xml:lang="fr">a actuellement pour localisation</rdfs:label>
	<rdfs:label xml:lang="en">has current location</rdfs:label>
	<rdfs:label xml:lang="de">hat derzeitigen Standort</rdfs:label>
	<rdfs:label xml:lang="pt">é localizado em</rdfs:label>
	<rdfs:label xml:lang="el">βρίσκεται σε</rdfs:label>
	<rdfs:label xml:lang="ru">в данный момент находится в</rdfs:label>
	<rdfs:label xml:lang="zh">有当前位置</rdfs:label>
</rdf:Description>

<rdf:Description rdf:about="http://www.cidoc-crm.org/cidoc-crm/P55i_currently_holds">
	<rdf:type rdf:resource="http://www.w3.org/2002/07/owl#ObjectProperty"/>
	<rdfs:subPropertyOf rdf:resource="http://www.cidoc-crm.org/cidoc-crm/P53i_is_former_or_current_location_of"/>
	<rdfs:domain rdf:resource="http://www.cidoc-crm.org/cidoc-crm/E53_Place"/>
	<rdfs:range rdf:resource="http://www.cidoc-crm.org/cidoc-crm/E19_Physical_Object"/>
	<rdfs:label xml:lang="en">currently holds</rdfs:label>
	<rdfs:label xml:lang="fr">est actuellement la localisation de</rdfs:label>
	<rdfs:label xml:lang="de">hält derzeitig</rdfs:label>
	<rdfs:label xml:lang="pt">é localização atual de</rdfs:label>
	<rdfs:label xml:lang="el">είναι θέση του</rdfs:label>
	<rdfs:label xml:lang="ru">в данный момент содержит</rdfs:label>
	<rdfs:label xml:lang="zh">当前拥有</rdfs:label>
</rdf:Description>

<rdf:Description rdf:about="http://www.cidoc-crm.org/cidoc-crm/P56_bears_feature">
	<rdf:type rdf:resource="http://www.w3.org/2002/07/owl#ObjectProperty"/>
	<rdfs:subPropertyOf rdf:resource="http://www.cidoc-crm.org/cidoc-crm/P46_is_composed_of"/>
	<owl:inverseOf rdf:resource="http://www.cidoc-crm.org/cidoc-crm/P56i_is_found_on"/>
	<rdfs:domain rdf:resource="http://www.cidoc-crm.org/cidoc-crm/E19_Physical_Object"/>
	<rdfs:range rdf:resource="http://www.cidoc-crm.org/cidoc-crm/E26_Physical_Feature"/>
	<rdfs:comment xml:lang="en">This property links an instance of E19 Physical Object to an instance of E26 Physical Feature that it bears.
An instance of E26 Physical Feature can only exist on one object. One object may bear more than one E26 Physical Feature. An instance of E27 Site should be considered as an instance of E26 Physical Feature on the surface of the Earth.
An instance B of E26 Physical Feature being a detail of the structure of another instance A of E26 Physical Feature can be linked to B by use of the property P46 is composed of (forms part of). This implies that the subfeature B is P56i is found on the same E19 Physical Object as A.
This property is a shortcut. A more detailed representation can make use of the fully developed (i.e. indirect) path E19 Physical Object, through, P59 has section, E53 Place, P53i is former or current location of to E26 Physical Feature.</rdfs:comment>
	<rdfs:label xml:lang="fr">a pour caractéristique</rdfs:label>
	<rdfs:label xml:lang="en">bears feature</rdfs:label>
	<rdfs:label xml:lang="pt">possui característica</rdfs:label>
	<rdfs:label xml:lang="de">trägt Merkmal</rdfs:label>
	<rdfs:label xml:lang="el">φέρει μόρφωμα</rdfs:label>
	<rdfs:label xml:lang="ru">несет признак</rdfs:label>
	<rdfs:label xml:lang="zh">有特征</rdfs:label>
</rdf:Description>

<rdf:Description rdf:about="http://www.cidoc-crm.org/cidoc-crm/P56i_is_found_on">
	<rdf:type rdf:resource="http://www.w3.org/2002/07/owl#ObjectProperty"/>
	<rdfs:subPropertyOf rdf:resource="http://www.cidoc-crm.org/cidoc-crm/P46i_forms_part_of"/>
	<rdfs:domain rdf:resource="http://www.cidoc-crm.org/cidoc-crm/E26_Physical_Feature"/>
	<rdfs:range rdf:resource="http://www.cidoc-crm.org/cidoc-crm/E19_Physical_Object"/>
	<rdfs:label xml:lang="en">is found on</rdfs:label>
	<rdfs:label xml:lang="fr">se trouve sur</rdfs:label>
	<rdfs:label xml:lang="de">wird gefunden auf</rdfs:label>
	<rdfs:label xml:lang="pt">é encontrada em</rdfs:label>
	<rdfs:label xml:lang="el">βρίσκεται σε</rdfs:label>
	<rdfs:label xml:lang="ru">найден на</rdfs:label>
	<rdfs:label xml:lang="zh">发现于</rdfs:label>
</rdf:Description>

<rdf:Description rdf:about="http://www.cidoc-crm.org/cidoc-crm/P59_has_section">
	<rdf:type rdf:resource="http://www.w3.org/2002/07/owl#ObjectProperty"/>
	<rdfs:subPropertyOf rdf:resource="http://www.cidoc-crm.org/cidoc-crm/P157i_provides_reference_space_for"/>
	<owl:inverseOf rdf:resource="http://www.cidoc-crm.org/cidoc-crm/P59i_is_located_on_or_within"/>
	<rdfs:domain rdf:resource="http://www.cidoc-crm.org/cidoc-crm/E18_Physical_Thing"/>
	<rdfs:range rdf:resource="http://www.cidoc-crm.org/cidoc-crm/E53_Place"/>
	<rdfs:comment xml:lang="en">This property links an area, i.e., an instance of E53 Place to the instance of E18 Physical Thing upon which it is found. This area may either be identified by a name, or by a geometry in terms of a coordinate system adapted to the shape of the respective instance of E18 Physical Thing. Typically, names identifying sections of physical objects are composed of the name of a kind of part and the name of the object itself, such as “The poop deck of H.M.S. Victory”, which is composed of “poop deck” and “H.M.S. Victory”.</rdfs:comment>
	<rdfs:label xml:lang="fr">a pour section</rdfs:label>
	<rdfs:label xml:lang="en">has section</rdfs:label>
	<rdfs:label xml:lang="de">hat Bereich</rdfs:label>
	<rdfs:label xml:lang="pt">tem seção</rdfs:label>
	<rdfs:label xml:lang="el">έχει τομέα</rdfs:label>
	<rdfs:label xml:lang="ru">имеет район</rdfs:label>
	<rdfs:label xml:lang="zh">有区域</rdfs:label>
</rdf:Description>

<rdf:Description rdf:about="http://www.cidoc-crm.org/cidoc-crm/P59i_is_located_on_or_within">
	<rdf:type rdf:resource="http://www.w3.org/2002/07/owl#ObjectProperty"/>
	<rdfs:subPropertyOf rdf:resource="http://www.cidoc-crm.org/cidoc-crm/P157_is_at_rest_relative_to"/>
	<rdfs:domain rdf:resource="http://www.cidoc-crm.org/cidoc-crm/E53_Place"/>
	<rdfs:range rdf:resource="http://www.cidoc-crm.org/cidoc-crm/E18_Physical_Thing"/>
	<rdfs:label xml:lang="de">befindet sich auf oder in</rdfs:label>
	<rdfs:label xml:lang="pt">está localizada sobre ou dentro de</rdfs:label>
	<rdfs:label xml:lang="en">is located on or within</rdfs:label>
	<rdfs:label xml:lang="fr">se situe sur ou dans</rdfs:label>
	<rdfs:label xml:lang="el">βρίσκεται σε ή εντός</rdfs:label>
	<rdfs:label xml:lang="ru">находится на или внутри</rdfs:label>
	<rdfs:label xml:lang="zh">位于</rdfs:label>
</rdf:Description>

<rdf:Description rdf:about="http://www.cidoc-crm.org/cidoc-crm/P5_consists_of">
	<rdf:type rdf:resource="http://www.w3.org/2002/07/owl#ObjectProperty"/>
	<owl:inverseOf rdf:resource="http://www.cidoc-crm.org/cidoc-crm/P5i_forms_part_of"/>
	<rdfs:domain rdf:resource="http://www.cidoc-crm.org/cidoc-crm/E3_Condition_State"/>
	<rdfs:range rdf:resource="http://www.cidoc-crm.org/cidoc-crm/E3_Condition_State"/>
	<rdfs:comment xml:lang="en">This property describes the decomposition of an instance of E3 Condition State into discrete, subsidiary states.
It is assumed that the sub-states into which the condition state is analysed form a logical whole, although the entire story may not be completely known, and that the sub-states are in fact constitutive of the general condition state. For example, a general condition state of “in ruins” may be decomposed into the individual stages of decay.
This property is transitive and asymmetric.</rdfs:comment>
	<rdfs:label xml:lang="de">besteht aus</rdfs:label>
	<rdfs:label xml:lang="fr">comprend</rdfs:label>
	<rdfs:label xml:lang="pt">consiste de</rdfs:label>
	<rdfs:label xml:lang="en">consists of</rdfs:label>
	<rdfs:label xml:lang="el">αποτελείται από</rdfs:label>
	<rdfs:label xml:lang="ru">состоит из</rdfs:label>
	<rdfs:label xml:lang="zh">包括</rdfs:label>
</rdf:Description>

<rdf:Description rdf:about="http://www.cidoc-crm.org/cidoc-crm/P5i_forms_part_of">
	<rdf:type rdf:resource="http://www.w3.org/2002/07/owl#ObjectProperty"/>
	<rdfs:domain rdf:resource="http://www.cidoc-crm.org/cidoc-crm/E3_Condition_State"/>
	<rdfs:range rdf:resource="http://www.cidoc-crm.org/cidoc-crm/E3_Condition_State"/>
	<rdfs:label xml:lang="de">bildet Teil von</rdfs:label>
	<rdfs:label xml:lang="fr">fait partie de</rdfs:label>
	<rdfs:label xml:lang="pt">faz parte de</rdfs:label>
	<rdfs:label xml:lang="en">forms part of</rdfs:label>
	<rdfs:label xml:lang="el">αποτελεί μέρος του/της</rdfs:label>
	<rdfs:label xml:lang="ru">формирует часть</rdfs:label>
	<rdfs:label xml:lang="zh">组成部分</rdfs:label>
</rdf:Description>

<rdf:Description rdf:about="http://www.cidoc-crm.org/cidoc-crm/P62_depicts">
	<rdf:type rdf:resource="http://www.w3.org/2002/07/owl#ObjectProperty"/>
	<owl:inverseOf rdf:resource="http://www.cidoc-crm.org/cidoc-crm/P62i_is_depicted_by"/>
	<rdfs:domain rdf:resource="http://www.cidoc-crm.org/cidoc-crm/E24_Physical_Human-Made_Thing"/>
	<rdfs:range rdf:resource="http://www.cidoc-crm.org/cidoc-crm/E1_CRM_Entity"/>
	<rdfs:comment xml:lang="en">This property identifies something that is depicted by an instance of E24 Physical Human-Made Thing. Depicting is meant in the sense that an instance of E24 Physical Human-Made Thing intentionally shows, through its optical qualities or form, a representation of the entity depicted. Photographs are by default regarded as being intentional in this sense. Anything that is designed to change the properties of the depiction, such as an e-book reader, is specifically excluded. The property does not pertain to inscriptions or any other information encoding.
This property is a shortcut of the more fully developed path from E24 Physical Human-Made Thing through P65 shows visual item, E36 Visual Item, P138 represents to E1 CRM Entity. P62.1 mode of depiction allows the nature of the depiction to be refined.</rdfs:comment>
	<rdfs:label xml:lang="de">bildet ab</rdfs:label>
	<rdfs:label xml:lang="en">depicts</rdfs:label>
	<rdfs:label xml:lang="fr">illustre</rdfs:label>
	<rdfs:label xml:lang="pt">retrata</rdfs:label>
	<rdfs:label xml:lang="el">απεικονίζει</rdfs:label>
	<rdfs:label xml:lang="ru">описывает</rdfs:label>
	<rdfs:label xml:lang="zh">描绘了</rdfs:label>
</rdf:Description>

<rdf:Description rdf:about="http://www.cidoc-crm.org/cidoc-crm/P62i_is_depicted_by">
	<rdf:type rdf:resource="http://www.w3.org/2002/07/owl#ObjectProperty"/>
	<rdfs:domain rdf:resource="http://www.cidoc-crm.org/cidoc-crm/E1_CRM_Entity"/>
	<rdfs:range rdf:resource="http://www.cidoc-crm.org/cidoc-crm/E24_Physical_Human-Made_Thing"/>
	<rdfs:label xml:lang="fr">est illustré par</rdfs:label>
	<rdfs:label xml:lang="en">is depicted by</rdfs:label>
	<rdfs:label xml:lang="de">wird abgebildet durch</rdfs:label>
	<rdfs:label xml:lang="pt">é retratada por</rdfs:label>
	<rdfs:label xml:lang="el">απεικονίζεται σε</rdfs:label>
	<rdfs:label xml:lang="ru">описан посредством</rdfs:label>
	<rdfs:label xml:lang="zh">被描绘</rdfs:label>
</rdf:Description>

<rdf:Description rdf:about="http://www.cidoc-crm.org/cidoc-crm/P65_shows_visual_item">
	<rdf:type rdf:resource="http://www.w3.org/2002/07/owl#ObjectProperty"/>
	<rdfs:subPropertyOf rdf:resource="http://www.cidoc-crm.org/cidoc-crm/P128_carries"/>
	<owl:inverseOf rdf:resource="http://www.cidoc-crm.org/cidoc-crm/P65i_is_shown_by"/>
	<rdfs:domain rdf:resource="http://www.cidoc-crm.org/cidoc-crm/E24_Physical_Human-Made_Thing"/>
	<rdfs:range rdf:resource="http://www.cidoc-crm.org/cidoc-crm/E36_Visual_Item"/>
	<rdfs:comment xml:lang="en">This property documents an instance of E36 Visual Item shown by an instance of E24 Physical Human-Made Thing.
This property is similar to P62 depicts (is depicted by) in that it associates an instance of E24 Physical Human-Made Thing with a visual representation. However, P65 shows visual item (is shown by) differs from the P62 depicts (is depicted by) property in that it makes no claims about what the instance of E36 Visual Item is deemed to represent. An instance of E36 Visual Item identifies a recognisable image or visual symbol, regardless of what this image may or may not represent.
For example, all recent British coins bear a portrait of Queen Elizabeth II, a fact that is correctly documented using P62 depicts (is depicted by). Different portraits have been used at different periods, however. P65 shows visual item (is shown by) can be used to refer to a particular portrait.
P65 shows visual item (is shown by) may also be used for Visual Items such as signs, marks and symbols, for example the 'Maltese Cross' or the 'copyright symbol’ that have no particular representational content.
This property is part of the fully developed path E24 Physical Human-Made Thing, P65 shows visual item, E36 Visual Item, P138 represents to E1 CRM Entity which is shortcut by, P62 depicts (is depicted by).</rdfs:comment>
	<rdfs:label xml:lang="pt">apresenta item visual</rdfs:label>
	<rdfs:label xml:lang="fr">représente l'entité visuelle</rdfs:label>
	<rdfs:label xml:lang="en">shows visual item</rdfs:label>
	<rdfs:label xml:lang="de">zeigt Bildliches</rdfs:label>
	<rdfs:label xml:lang="el">εμφανίζει οπτικό στοιχείο</rdfs:label>
	<rdfs:label xml:lang="ru">показывает визуальный предмет</rdfs:label>
	<rdfs:label xml:lang="zh">展示可视项</rdfs:label>
</rdf:Description>

<rdf:Description rdf:about="http://www.cidoc-crm.org/cidoc-crm/P65i_is_shown_by">
	<rdf:type rdf:resource="http://www.w3.org/2002/07/owl#ObjectProperty"/>
	<rdfs:subPropertyOf rdf:resource="http://www.cidoc-crm.org/cidoc-crm/P128i_is_carried_by"/>
	<rdfs:domain rdf:resource="http://www.cidoc-crm.org/cidoc-crm/E36_Visual_Item"/>
	<rdfs:range rdf:resource="http://www.cidoc-crm.org/cidoc-crm/E24_Physical_Human-Made_Thing"/>
	<rdfs:label xml:lang="fr">est représenté par</rdfs:label>
	<rdfs:label xml:lang="en">is shown by</rdfs:label>
	<rdfs:label xml:lang="de">wird gezeigt durch</rdfs:label>
	<rdfs:label xml:lang="pt">é apresentado por</rdfs:label>
	<rdfs:label xml:lang="el">εμφανίζεται σε</rdfs:label>
	<rdfs:label xml:lang="ru">показан посредством</rdfs:label>
	<rdfs:label xml:lang="zh">被展示</rdfs:label>
</rdf:Description>

<rdf:Description rdf:about="http://www.cidoc-crm.org/cidoc-crm/P67_refers_to">
	<rdf:type rdf:resource="http://www.w3.org/2002/07/owl#ObjectProperty"/>
	<owl:inverseOf rdf:resource="http://www.cidoc-crm.org/cidoc-crm/P67i_is_referred_to_by"/>
	<rdfs:domain rdf:resource="http://www.cidoc-crm.org/cidoc-crm/E89_Propositional_Object"/>
	<rdfs:range rdf:resource="http://www.cidoc-crm.org/cidoc-crm/E1_CRM_Entity"/>
	<rdfs:comment xml:lang="en">This property documents that an instance of E89 Propositional Object makes a statement about an instance of E1 CRM Entity. P67 refers to (is referred to by) has the P67.1 has type link to an instance of E55 Type. This is intended to allow a more detailed description of the type of reference. This differs from P129 is about (is subject of), which describes the primary subject or subjects of the instance of E89 Propositional Object.</rdfs:comment>
	<rdfs:label xml:lang="pt">referencia</rdfs:label>
	<rdfs:label xml:lang="en">refers to</rdfs:label>
	<rdfs:label xml:lang="fr">renvoie à</rdfs:label>
	<rdfs:label xml:lang="de">verweist auf</rdfs:label>
	<rdfs:label xml:lang="el">αναφέρεται σε</rdfs:label>
	<rdfs:label xml:lang="ru">ссылается на</rdfs:label>
	<rdfs:label xml:lang="zh">涉及</rdfs:label>
</rdf:Description>

<rdf:Description rdf:about="http://www.cidoc-crm.org/cidoc-crm/P67i_is_referred_to_by">
	<rdf:type rdf:resource="http://www.w3.org/2002/07/owl#ObjectProperty"/>
	<rdfs:domain rdf:resource="http://www.cidoc-crm.org/cidoc-crm/E1_CRM_Entity"/>
	<rdfs:range rdf:resource="http://www.cidoc-crm.org/cidoc-crm/E89_Propositional_Object"/>
	<rdfs:label xml:lang="fr">fait l'objet d'un renvoi par</rdfs:label>
	<rdfs:label xml:lang="en">is referred to by</rdfs:label>
	<rdfs:label xml:lang="de">wird angeführt von</rdfs:label>
	<rdfs:label xml:lang="pt">é referenciado por</rdfs:label>
	<rdfs:label xml:lang="el">αναφέρεται από</rdfs:label>
	<rdfs:label xml:lang="ru">имеет ссылку на себя от</rdfs:label>
	<rdfs:label xml:lang="zh">被涉及</rdfs:label>
</rdf:Description>

<rdf:Description rdf:about="http://www.cidoc-crm.org/cidoc-crm/P68_foresees_use_of">
	<rdf:type rdf:resource="http://www.w3.org/2002/07/owl#ObjectProperty"/>
	<rdfs:subPropertyOf rdf:resource="http://www.cidoc-crm.org/cidoc-crm/P67_refers_to"/>
	<owl:inverseOf rdf:resource="http://www.cidoc-crm.org/cidoc-crm/P68i_use_foreseen_by"/>
	<rdfs:domain rdf:resource="http://www.cidoc-crm.org/cidoc-crm/E29_Design_or_Procedure"/>
	<rdfs:range rdf:resource="http://www.cidoc-crm.org/cidoc-crm/E57_Material"/>
	<rdfs:comment xml:lang="en">This property identifies an instance of E57 Material foreseen to be used by an instance of E29 Design or Procedure.
E29 Designs and procedures commonly foresee the use of particular instances of E57 Material. The fabrication of adobe bricks, for example, requires straw, clay and water. This property enables this to be documented.
This property is not intended for the documentation of instances of E57 Materials that were used on a particular occasion when an instance of E29 Design or Procedure was executed.</rdfs:comment>
	<rdfs:label xml:lang="en">foresees use of</rdfs:label>
	<rdfs:label xml:lang="pt">normalmente emprega</rdfs:label>
	<rdfs:label xml:lang="fr">prévoit l'usage de</rdfs:label>
	<rdfs:label xml:lang="de">sieht den Gebrauch vor von</rdfs:label>
	<rdfs:label xml:lang="el">συνήθως χρησιμοποιεί</rdfs:label>
	<rdfs:label xml:lang="ru">обычно применяет</rdfs:label>
	<rdfs:label xml:lang="zh">预知使用</rdfs:label>
</rdf:Description>

<rdf:Description rdf:about="http://www.cidoc-crm.org/cidoc-crm/P68i_use_foreseen_by">
	<rdf:type rdf:resource="http://www.w3.org/2002/07/owl#ObjectProperty"/>
	<rdfs:subPropertyOf rdf:resource="http://www.cidoc-crm.org/cidoc-crm/P67i_is_referred_to_by"/>
	<rdfs:domain rdf:resource="http://www.cidoc-crm.org/cidoc-crm/E57_Material"/>
	<rdfs:range rdf:resource="http://www.cidoc-crm.org/cidoc-crm/E29_Design_or_Procedure"/>
	<rdfs:label xml:lang="fr">usage prévu de</rdfs:label>
	<rdfs:label xml:lang="en">use foreseen by</rdfs:label>
	<rdfs:label xml:lang="de">vorgesehen für Gebrauch durch defined</rdfs:label>
	<rdfs:label xml:lang="pt">é empregado por</rdfs:label>
	<rdfs:label xml:lang="el">συνήθως χρησιμοποιείται από</rdfs:label>
	<rdfs:label xml:lang="ru">обычно используется посредством</rdfs:label>
	<rdfs:label xml:lang="zh">被预知使用</rdfs:label>
</rdf:Description>

<rdf:Description rdf:about="http://www.cidoc-crm.org/cidoc-crm/P69_has_association_with">
	<rdf:type rdf:resource="http://www.w3.org/2002/07/owl#ObjectProperty"/>
	<owl:inverseOf rdf:resource="http://www.cidoc-crm.org/cidoc-crm/P69i_is_associated_with"/>
	<rdfs:domain rdf:resource="http://www.cidoc-crm.org/cidoc-crm/E29_Design_or_Procedure"/>
	<rdfs:range rdf:resource="http://www.cidoc-crm.org/cidoc-crm/E29_Design_or_Procedure"/>
	<rdfs:comment xml:lang="en">This property generalises relationships like whole-part, sequence, prerequisite or inspired by between instances of E29 Design or Procedure. Any instance of E29 Design or Procedure may be associated with other designs or procedures. The property is considered to be symmetrical unless otherwise indicated by P69.1 has type. The property is not transitive.
This property is a directed relationship. The P69.1 has type property of P69 has association with allows the nature of the association to be specified reading from domain to range; examples of types of association between instances of E29 Design or Procedure include: has part, follows, requires, etc.
Instances of this property are considered to be symmetric, in case no directed sense is provided for them by the property P69.1 has type.
The property can typically be used to model the decomposition of the description of a complete workflow into a series of separate procedures.</rdfs:comment>
	<rdfs:label xml:lang="fr">est associé à</rdfs:label>
	<rdfs:label xml:lang="en">has association with</rdfs:label>
	<rdfs:label xml:lang="de">ist verbunden mit</rdfs:label>
	<rdfs:label xml:lang="pt">é associado com</rdfs:label>
	<rdfs:label xml:lang="el">σχετίζεται με</rdfs:label>
	<rdfs:label xml:lang="ru">ассоциирован с</rdfs:label>
	<rdfs:label xml:lang="zh">关联</rdfs:label>
</rdf:Description>

<rdf:Description rdf:about="http://www.cidoc-crm.org/cidoc-crm/P69i_is_associated_with">
	<rdf:type rdf:resource="http://www.w3.org/2002/07/owl#ObjectProperty"/>
	<rdfs:domain rdf:resource="http://www.cidoc-crm.org/cidoc-crm/E29_Design_or_Procedure"/>
	<rdfs:range rdf:resource="http://www.cidoc-crm.org/cidoc-crm/E29_Design_or_Procedure"/>
	<rdfs:label xml:lang="fr">est associé à</rdfs:label>
	<rdfs:label xml:lang="en">is associated with</rdfs:label>
</rdf:Description>

<rdf:Description rdf:about="http://www.cidoc-crm.org/cidoc-crm/P70_documents">
	<rdf:type rdf:resource="http://www.w3.org/2002/07/owl#ObjectProperty"/>
	<rdfs:subPropertyOf rdf:resource="http://www.cidoc-crm.org/cidoc-crm/P67_refers_to"/>
	<owl:inverseOf rdf:resource="http://www.cidoc-crm.org/cidoc-crm/P70i_is_documented_in"/>
	<rdfs:domain rdf:resource="http://www.cidoc-crm.org/cidoc-crm/E31_Document"/>
	<rdfs:range rdf:resource="http://www.cidoc-crm.org/cidoc-crm/E1_CRM_Entity"/>
	<rdfs:comment xml:lang="en">This property describes the CRM Entities documented as instances of E31 Document.
Documents may describe any conceivable entity, hence the link to the highest-level entity in the CIDOC CRM class hierarchy. This property is intended for cases where a reference is regarded as making a proposition about reality. This may be of a documentary character, in the scholarly or scientific sense, or a more general statement.</rdfs:comment>
	<rdfs:label xml:lang="de">belegt</rdfs:label>
	<rdfs:label xml:lang="pt">documenta</rdfs:label>
	<rdfs:label xml:lang="fr">documente</rdfs:label>
	<rdfs:label xml:lang="en">documents</rdfs:label>
	<rdfs:label xml:lang="el">τεκμηριώνει</rdfs:label>
	<rdfs:label xml:lang="ru">документирует</rdfs:label>
	<rdfs:label xml:lang="zh">记录了</rdfs:label>
</rdf:Description>

<rdf:Description rdf:about="http://www.cidoc-crm.org/cidoc-crm/P70i_is_documented_in">
	<rdf:type rdf:resource="http://www.w3.org/2002/07/owl#ObjectProperty"/>
	<rdfs:subPropertyOf rdf:resource="http://www.cidoc-crm.org/cidoc-crm/P67i_is_referred_to_by"/>
	<rdfs:domain rdf:resource="http://www.cidoc-crm.org/cidoc-crm/E1_CRM_Entity"/>
	<rdfs:range rdf:resource="http://www.cidoc-crm.org/cidoc-crm/E31_Document"/>
	<rdfs:label xml:lang="fr">est documenté dans</rdfs:label>
	<rdfs:label xml:lang="en">is documented in</rdfs:label>
	<rdfs:label xml:lang="de">wird belegt in</rdfs:label>
	<rdfs:label xml:lang="pt">é documentado em</rdfs:label>
	<rdfs:label xml:lang="el">τεκμηριώνεται σε</rdfs:label>
	<rdfs:label xml:lang="ru">документирован в</rdfs:label>
	<rdfs:label xml:lang="zh">记录在</rdfs:label>
</rdf:Description>

<rdf:Description rdf:about="http://www.cidoc-crm.org/cidoc-crm/P71_lists">
	<rdf:type rdf:resource="http://www.w3.org/2002/07/owl#ObjectProperty"/>
	<rdfs:subPropertyOf rdf:resource="http://www.cidoc-crm.org/cidoc-crm/P67_refers_to"/>
	<owl:inverseOf rdf:resource="http://www.cidoc-crm.org/cidoc-crm/P71i_is_listed_in"/>
	<rdfs:domain rdf:resource="http://www.cidoc-crm.org/cidoc-crm/E32_Authority_Document"/>
	<rdfs:range rdf:resource="http://www.cidoc-crm.org/cidoc-crm/E1_CRM_Entity"/>
	<rdfs:comment xml:lang="en">This property associates an instance of E32 Authority Document with an instance of E1 CRM Entity which it lists for reference purposes.</rdfs:comment>
	<rdfs:label xml:lang="pt">define</rdfs:label>
	<rdfs:label xml:lang="de">listet</rdfs:label>
	<rdfs:label xml:lang="en">lists</rdfs:label>
	<rdfs:label xml:lang="fr">énumère</rdfs:label>
	<rdfs:label xml:lang="el">περιλαμβάνει</rdfs:label>
	<rdfs:label xml:lang="ru">перечисляет</rdfs:label>
	<rdfs:label xml:lang="zh">列出</rdfs:label>
</rdf:Description>

<rdf:Description rdf:about="http://www.cidoc-crm.org/cidoc-crm/P71i_is_listed_in">
	<rdf:type rdf:resource="http://www.w3.org/2002/07/owl#ObjectProperty"/>
	<rdfs:subPropertyOf rdf:resource="http://www.cidoc-crm.org/cidoc-crm/P67i_is_referred_to_by"/>
	<rdfs:domain rdf:resource="http://www.cidoc-crm.org/cidoc-crm/E1_CRM_Entity"/>
	<rdfs:range rdf:resource="http://www.cidoc-crm.org/cidoc-crm/E32_Authority_Document"/>
	<rdfs:label xml:lang="fr">est énuméré par</rdfs:label>
	<rdfs:label xml:lang="en">is listed in</rdfs:label>
	<rdfs:label xml:lang="de">wird aufgelistet in</rdfs:label>
	<rdfs:label xml:lang="pt">é definido por</rdfs:label>
	<rdfs:label xml:lang="el">περιλαμβάνεται σε</rdfs:label>
	<rdfs:label xml:lang="ru">перечислен в</rdfs:label>
	<rdfs:label xml:lang="zh">列于</rdfs:label>
</rdf:Description>

<rdf:Description rdf:about="http://www.cidoc-crm.org/cidoc-crm/P72_has_language">
	<rdf:type rdf:resource="http://www.w3.org/2002/07/owl#ObjectProperty"/>
	<owl:inverseOf rdf:resource="http://www.cidoc-crm.org/cidoc-crm/P72i_is_language_of"/>
	<rdfs:domain rdf:resource="http://www.cidoc-crm.org/cidoc-crm/E33_Linguistic_Object"/>
	<rdfs:range rdf:resource="http://www.cidoc-crm.org/cidoc-crm/E56_Language"/>
	<rdfs:comment xml:lang="en">This property associates an instance(s) of E33 Linguistic Object with an instance of E56 Language in which it is, at least partially, expressed.
Linguistic Objects are composed in one or more human languages. This property allows these languages to be documented.</rdfs:comment>
	<rdfs:label xml:lang="fr">a pour langue</rdfs:label>
	<rdfs:label xml:lang="en">has language</rdfs:label>
	<rdfs:label xml:lang="de">hat Sprache</rdfs:label>
	<rdfs:label xml:lang="pt">é da língua</rdfs:label>
	<rdfs:label xml:lang="el">έχει γλώσσα</rdfs:label>
	<rdfs:label xml:lang="ru">имеет язык</rdfs:label>
	<rdfs:label xml:lang="zh">有语种</rdfs:label>
</rdf:Description>

<rdf:Description rdf:about="http://www.cidoc-crm.org/cidoc-crm/P72i_is_language_of">
	<rdf:type rdf:resource="http://www.w3.org/2002/07/owl#ObjectProperty"/>
	<rdfs:domain rdf:resource="http://www.cidoc-crm.org/cidoc-crm/E56_Language"/>
	<rdfs:range rdf:resource="http://www.cidoc-crm.org/cidoc-crm/E33_Linguistic_Object"/>
	<rdfs:label xml:lang="fr">est la langue de</rdfs:label>
	<rdfs:label xml:lang="en">is language of</rdfs:label>
	<rdfs:label xml:lang="de">ist Sprache von</rdfs:label>
	<rdfs:label xml:lang="pt">é a língua de</rdfs:label>
	<rdfs:label xml:lang="el">είναι γλώσσα του/της</rdfs:label>
	<rdfs:label xml:lang="ru">является языком для</rdfs:label>
	<rdfs:label xml:lang="zh">是语种</rdfs:label>
</rdf:Description>

<rdf:Description rdf:about="http://www.cidoc-crm.org/cidoc-crm/P73_has_translation">
	<rdf:type rdf:resource="http://www.w3.org/2002/07/owl#ObjectProperty"/>
	<rdfs:subPropertyOf rdf:resource="http://www.cidoc-crm.org/cidoc-crm/P130i_features_are_also_found_on"/>
	<owl:inverseOf rdf:resource="http://www.cidoc-crm.org/cidoc-crm/P73i_is_translation_of"/>
	<rdfs:domain rdf:resource="http://www.cidoc-crm.org/cidoc-crm/E33_Linguistic_Object"/>
	<rdfs:range rdf:resource="http://www.cidoc-crm.org/cidoc-crm/E33_Linguistic_Object"/>
	<rdfs:comment xml:lang="en">This property links an instance of E33 Linguistic Object (A), to another instance of E33 Linguistic Object (B) which is the translation of A.
When an instance of E33 Linguistic Object is translated into a new language a new instance of E33 Linguistic Object is created, despite the translation being conceptually similar to the source.
This property is asymmetric.</rdfs:comment>
	<rdfs:label xml:lang="fr">a pour traduction</rdfs:label>
	<rdfs:label xml:lang="en">has translation</rdfs:label>
	<rdfs:label xml:lang="de">hat Übersetzung</rdfs:label>
	<rdfs:label xml:lang="pt">tem tradução</rdfs:label>
	<rdfs:label xml:lang="el">έχει μετάφραση</rdfs:label>
	<rdfs:label xml:lang="ru">имеет перевод</rdfs:label>
	<rdfs:label xml:lang="zh">有译文</rdfs:label>
</rdf:Description>

<rdf:Description rdf:about="http://www.cidoc-crm.org/cidoc-crm/P73i_is_translation_of">
	<rdf:type rdf:resource="http://www.w3.org/2002/07/owl#ObjectProperty"/>
	<rdfs:subPropertyOf rdf:resource="http://www.cidoc-crm.org/cidoc-crm/P130_shows_features_of"/>
	<rdfs:domain rdf:resource="http://www.cidoc-crm.org/cidoc-crm/E33_Linguistic_Object"/>
	<rdfs:range rdf:resource="http://www.cidoc-crm.org/cidoc-crm/E33_Linguistic_Object"/>
	<rdfs:label xml:lang="fr">est traduction de</rdfs:label>
	<rdfs:label xml:lang="en">is translation of</rdfs:label>
	<rdfs:label xml:lang="de">ist Übersetzung von</rdfs:label>
	<rdfs:label xml:lang="pt">é tradução de</rdfs:label>
	<rdfs:label xml:lang="el">είναι μετάφραση του/της</rdfs:label>
	<rdfs:label xml:lang="ru">является переводом</rdfs:label>
	<rdfs:label xml:lang="zh">是译文</rdfs:label>
</rdf:Description>

<rdf:Description rdf:about="http://www.cidoc-crm.org/cidoc-crm/P74_has_current_or_former_residence">
	<rdf:type rdf:resource="http://www.w3.org/2002/07/owl#ObjectProperty"/>
	<owl:inverseOf rdf:resource="http://www.cidoc-crm.org/cidoc-crm/P74i_is_current_or_former_residence_of"/>
	<rdfs:domain rdf:resource="http://www.cidoc-crm.org/cidoc-crm/E39_Actor"/>
	<rdfs:range rdf:resource="http://www.cidoc-crm.org/cidoc-crm/E53_Place"/>
	<rdfs:comment xml:lang="en">This property describes the current or former place of residence (an instance of E53 Place) of an instance of E39 Actor.
The residence may be either the place where the actor resides, or a legally registered address of any kind.</rdfs:comment>
	<rdfs:label xml:lang="fr">a pour résidence actuelle ou antérieure</rdfs:label>
	<rdfs:label xml:lang="en">has current or former residence</rdfs:label>
	<rdfs:label xml:lang="de">hat derzeitigen oder früheren Sitz</rdfs:label>
	<rdfs:label xml:lang="pt">reside ou residiu em</rdfs:label>
	<rdfs:label xml:lang="el">έχει ή είχε κατοικία</rdfs:label>
	<rdfs:label xml:lang="ru">имеет текущее или бывшее местожительства</rdfs:label>
	<rdfs:label xml:lang="zh">有当前或曾经居住地</rdfs:label>
</rdf:Description>

<rdf:Description rdf:about="http://www.cidoc-crm.org/cidoc-crm/P74i_is_current_or_former_residence_of">
	<rdf:type rdf:resource="http://www.w3.org/2002/07/owl#ObjectProperty"/>
	<rdfs:domain rdf:resource="http://www.cidoc-crm.org/cidoc-crm/E53_Place"/>
	<rdfs:range rdf:resource="http://www.cidoc-crm.org/cidoc-crm/E39_Actor"/>
	<rdfs:label xml:lang="fr">est la résidence actuelle ou antérieure de</rdfs:label>
	<rdfs:label xml:lang="en">is current or former residence of</rdfs:label>
	<rdfs:label xml:lang="de">ist derzeitiger oder früherer Sitz von</rdfs:label>
	<rdfs:label xml:lang="pt">é ou foi residência de</rdfs:label>
	<rdfs:label xml:lang="el">είναι ή ήταν κατοικία του/της</rdfs:label>
	<rdfs:label xml:lang="ru">является текущим или бывшим местом жительства для</rdfs:label>
	<rdfs:label xml:lang="zh">是当前或曾经居住地</rdfs:label>
</rdf:Description>

<rdf:Description rdf:about="http://www.cidoc-crm.org/cidoc-crm/P75_possesses">
	<rdf:type rdf:resource="http://www.w3.org/2002/07/owl#ObjectProperty"/>
	<owl:inverseOf rdf:resource="http://www.cidoc-crm.org/cidoc-crm/P75i_is_possessed_by"/>
	<rdfs:domain rdf:resource="http://www.cidoc-crm.org/cidoc-crm/E39_Actor"/>
	<rdfs:range rdf:resource="http://www.cidoc-crm.org/cidoc-crm/E30_Right"/>
	<rdfs:comment xml:lang="en">This property associates an instance of E39 Actor to an instance of E30 Right over which the actor holds or has held a legal claim.</rdfs:comment>
	<rdfs:label xml:lang="de">besitzt</rdfs:label>
	<rdfs:label xml:lang="en">possesses</rdfs:label>
	<rdfs:label xml:lang="fr">possède</rdfs:label>
	<rdfs:label xml:lang="pt">é detentor de</rdfs:label>
	<rdfs:label xml:lang="el">κατέχει</rdfs:label>
	<rdfs:label xml:lang="ru">владеет</rdfs:label>
	<rdfs:label xml:lang="zh">拥有</rdfs:label>
</rdf:Description>

<rdf:Description rdf:about="http://www.cidoc-crm.org/cidoc-crm/P75i_is_possessed_by">
	<rdf:type rdf:resource="http://www.w3.org/2002/07/owl#ObjectProperty"/>
	<rdfs:domain rdf:resource="http://www.cidoc-crm.org/cidoc-crm/E30_Right"/>
	<rdfs:range rdf:resource="http://www.cidoc-crm.org/cidoc-crm/E39_Actor"/>
	<rdfs:label xml:lang="fr">est possédé par</rdfs:label>
	<rdfs:label xml:lang="en">is possessed by</rdfs:label>
	<rdfs:label xml:lang="de">sind im Besitz von</rdfs:label>
	<rdfs:label xml:lang="pt">são detidos por</rdfs:label>
	<rdfs:label xml:lang="el">κατέχεται από</rdfs:label>
	<rdfs:label xml:lang="ru">принадлежит</rdfs:label>
	<rdfs:label xml:lang="zh">被拥有</rdfs:label>
</rdf:Description>

<rdf:Description rdf:about="http://www.cidoc-crm.org/cidoc-crm/P76_has_contact_point">
	<rdf:type rdf:resource="http://www.w3.org/2002/07/owl#ObjectProperty"/>
	<owl:inverseOf rdf:resource="http://www.cidoc-crm.org/cidoc-crm/P76i_provides_access_to"/>
	<rdfs:domain rdf:resource="http://www.cidoc-crm.org/cidoc-crm/E39_Actor"/>
	<rdfs:range rdf:resource="http://www.cidoc-crm.org/cidoc-crm/E41_Appellation"/>
	<rdfs:comment xml:lang="en">This property associates an instance of E39 Actor to an instance of E41 Appellation which a communication service uses to direct communications to this actor, such as an e-mail address, fax number, or postal address.</rdfs:comment>
	<rdfs:label xml:lang="fr">a pour coordonnées</rdfs:label>
	<rdfs:label xml:lang="en">has contact point</rdfs:label>
	<rdfs:label xml:lang="de">hat Kontaktpunkt</rdfs:label>
	<rdfs:label xml:lang="pt">possui ponto de contato</rdfs:label>
	<rdfs:label xml:lang="el">έχει σημείο επικοινωνίας</rdfs:label>
	<rdfs:label xml:lang="ru">имеет контакт</rdfs:label>
	<rdfs:label xml:lang="zh">有联系方式</rdfs:label>
</rdf:Description>

<rdf:Description rdf:about="http://www.cidoc-crm.org/cidoc-crm/P76i_provides_access_to">
	<rdf:type rdf:resource="http://www.w3.org/2002/07/owl#ObjectProperty"/>
	<rdfs:domain rdf:resource="http://www.cidoc-crm.org/cidoc-crm/E41_Appellation"/>
	<rdfs:range rdf:resource="http://www.cidoc-crm.org/cidoc-crm/E39_Actor"/>
	<rdfs:label xml:lang="de">bietet Zugang zu</rdfs:label>
	<rdfs:label xml:lang="fr">permet de contacter</rdfs:label>
	<rdfs:label xml:lang="en">provides access to</rdfs:label>
	<rdfs:label xml:lang="pt">é ponto de contado de</rdfs:label>
	<rdfs:label xml:lang="el">παρέχει πρόσβαση σε</rdfs:label>
	<rdfs:label xml:lang="ru">предоставляет доступ к</rdfs:label>
	<rdfs:label xml:lang="zh">提供访问</rdfs:label>
</rdf:Description>

<rdf:Description rdf:about="http://www.cidoc-crm.org/cidoc-crm/P7_took_place_at">
	<rdf:type rdf:resource="http://www.w3.org/2002/07/owl#ObjectProperty"/>
	<owl:inverseOf rdf:resource="http://www.cidoc-crm.org/cidoc-crm/P7i_witnessed"/>
	<rdfs:domain rdf:resource="http://www.cidoc-crm.org/cidoc-crm/E4_Period"/>
	<rdfs:range rdf:resource="http://www.cidoc-crm.org/cidoc-crm/E53_Place"/>
	<rdfs:comment xml:lang="en">This property describes the spatial location of an instance of E4 Period.
The related instance of E53 Place should be seen as a wider approximation of the geometric area within which the phenomena that characterise the period in question occurred, see below. P7 took place at (witnessed) does not convey any meaning other than spatial positioning (frequently on the surface of the earth). For example, the period “Révolution française” can be said to have taken place in “France in 1789”; the “Victorian” period may be said to have taken place in “Britain from 1837-1901” and its colonies, as well as other parts of Europe and North America. An instance of E4 Period can take place at multiple non-contiguous, non-overlapping locations.
Any place where something happened includes the spatial projection of the happening given in the same geometric reference system. For instance, HMS Victory, as place of Lord Nelson's dying, includes the location of his body relative to the hull of HMS Victory at his time of death as the most precise location of his death. By the definition of P161 has spatial projection, an instance of E4 Period takes place on all its spatial projections to respective reference systems, that is, instances of E53 Place. Therefore, this property implies the more fully developed path from E4 Period through P161 has spatial projection, E53 Place, P89 falls within to E53 Place, where both places are defined in the same geometric reference system. The relation between an instance of E53 Place and its reference system can conveniently be documented via the property P157 is at rest relative to (provides reference space for).
Something that has happened at a given place can also be considered to have happened at a smaller place within it: for example, it is reasonable to say Caesar’s murder took place in Rome, but also on the Forum Romanum, and more precisely in the Curia. It is characteristic for different historical sources to use varying precision in such statements, without being in contradiction with each other. This may be due to lack of knowledge or to the relevance of the precision for the purpose of the statement. In information integration, the more precise statement improves the overall knowledge.</rdfs:comment>
	<rdfs:label xml:lang="fr">a eu lieu dans</rdfs:label>
	<rdfs:label xml:lang="de">fand statt in</rdfs:label>
	<rdfs:label xml:lang="pt">ocorreu em</rdfs:label>
	<rdfs:label xml:lang="en">took place at</rdfs:label>
	<rdfs:label xml:lang="el">έλαβε χώρα σε</rdfs:label>
	<rdfs:label xml:lang="ru">совершался на</rdfs:label>
	<rdfs:label xml:lang="zh">发生地在</rdfs:label>
</rdf:Description>

<rdf:Description rdf:about="http://www.cidoc-crm.org/cidoc-crm/P7i_witnessed">
	<rdf:type rdf:resource="http://www.w3.org/2002/07/owl#ObjectProperty"/>
	<rdfs:domain rdf:resource="http://www.cidoc-crm.org/cidoc-crm/E53_Place"/>
	<rdfs:range rdf:resource="http://www.cidoc-crm.org/cidoc-crm/E4_Period"/>
	<rdfs:label xml:lang="fr">a été témoin de</rdfs:label>
	<rdfs:label xml:lang="de">bezeugte</rdfs:label>
	<rdfs:label xml:lang="pt">testemunhou</rdfs:label>
	<rdfs:label xml:lang="en">witnessed</rdfs:label>
	<rdfs:label xml:lang="el">υπήρξε τόπος του</rdfs:label>
	<rdfs:label xml:lang="ru">был местом совершения</rdfs:label>
	<rdfs:label xml:lang="zh">发生过</rdfs:label>
</rdf:Description>

<rdf:Description rdf:about="http://www.cidoc-crm.org/cidoc-crm/P86_falls_within">
	<rdf:type rdf:resource="http://www.w3.org/2002/07/owl#ObjectProperty"/>
	<owl:inverseOf rdf:resource="http://www.cidoc-crm.org/cidoc-crm/P86i_contains"/>
	<rdfs:domain rdf:resource="http://www.cidoc-crm.org/cidoc-crm/E52_Time-Span"/>
	<rdfs:range rdf:resource="http://www.cidoc-crm.org/cidoc-crm/E52_Time-Span"/>
	<rdfs:comment xml:lang="en">This property describes the inclusion relationship between two instances of E52 Time-Span.
This property supports the notion that the temporal extent of an instance of E52 Time-Span falls within the temporal extent of another instance of E52 Time-Span. It addresses temporal containment only, and no contextual link between the two instances of E52 Time-Span is implied. This property is transitive and reflexive.</rdfs:comment>
	<rdfs:label xml:lang="pt">está contido em</rdfs:label>
	<rdfs:label xml:lang="en">falls within</rdfs:label>
	<rdfs:label xml:lang="de">fällt in</rdfs:label>
	<rdfs:label xml:lang="fr">s’insère dans</rdfs:label>
	<rdfs:label xml:lang="el">περιέχεται σε</rdfs:label>
	<rdfs:label xml:lang="ru">содержится в</rdfs:label>
	<rdfs:label xml:lang="zh">属于</rdfs:label>
</rdf:Description>

<rdf:Description rdf:about="http://www.cidoc-crm.org/cidoc-crm/P86i_contains">
	<rdf:type rdf:resource="http://www.w3.org/2002/07/owl#ObjectProperty"/>
	<rdfs:domain rdf:resource="http://www.cidoc-crm.org/cidoc-crm/E52_Time-Span"/>
	<rdfs:range rdf:resource="http://www.cidoc-crm.org/cidoc-crm/E52_Time-Span"/>
	<rdfs:label xml:lang="en">contains</rdfs:label>
	<rdfs:label xml:lang="fr">contient</rdfs:label>
	<rdfs:label xml:lang="pt">contém</rdfs:label>
	<rdfs:label xml:lang="de">enthält</rdfs:label>
	<rdfs:label xml:lang="el">περιέχει</rdfs:label>
	<rdfs:label xml:lang="ru">содержит</rdfs:label>
	<rdfs:label xml:lang="zh">包含</rdfs:label>
</rdf:Description>

<rdf:Description rdf:about="http://www.cidoc-crm.org/cidoc-crm/P89_falls_within">
	<rdf:type rdf:resource="http://www.w3.org/2002/07/owl#ObjectProperty"/>
	<owl:inverseOf rdf:resource="http://www.cidoc-crm.org/cidoc-crm/P89i_contains"/>
	<rdfs:domain rdf:resource="http://www.cidoc-crm.org/cidoc-crm/E53_Place"/>
	<rdfs:range rdf:resource="http://www.cidoc-crm.org/cidoc-crm/E53_Place"/>
	<rdfs:comment xml:lang="en">This property identifies an instance of E53 Place that falls wholly within the extent of another instance of E53 Place.
It addresses spatial containment only and does not imply any relationship between things or phenomena occupying these places.
This property is transitive and reflexive.</rdfs:comment>
	<rdfs:label xml:lang="pt">está contido em</rdfs:label>
	<rdfs:label xml:lang="en">falls within</rdfs:label>
	<rdfs:label xml:lang="de">fällt in</rdfs:label>
	<rdfs:label xml:lang="fr">s'insère dans</rdfs:label>
	<rdfs:label xml:lang="el">περιέχεται σε</rdfs:label>
	<rdfs:label xml:lang="ru">содержится в</rdfs:label>
	<rdfs:label xml:lang="zh">位于</rdfs:label>
</rdf:Description>

<rdf:Description rdf:about="http://www.cidoc-crm.org/cidoc-crm/P89i_contains">
	<rdf:type rdf:resource="http://www.w3.org/2002/07/owl#ObjectProperty"/>
	<rdfs:domain rdf:resource="http://www.cidoc-crm.org/cidoc-crm/E53_Place"/>
	<rdfs:range rdf:resource="http://www.cidoc-crm.org/cidoc-crm/E53_Place"/>
	<rdfs:label xml:lang="en">contains</rdfs:label>
	<rdfs:label xml:lang="fr">contient</rdfs:label>
	<rdfs:label xml:lang="pt">contém</rdfs:label>
	<rdfs:label xml:lang="de">enthält</rdfs:label>
	<rdfs:label xml:lang="el">περιέχει</rdfs:label>
	<rdfs:label xml:lang="ru">содержит</rdfs:label>
	<rdfs:label xml:lang="zh">包括</rdfs:label>
</rdf:Description>

<rdf:Description rdf:about="http://www.cidoc-crm.org/cidoc-crm/P8_took_place_on_or_within">
	<rdf:type rdf:resource="http://www.w3.org/2002/07/owl#ObjectProperty"/>
	<owl:inverseOf rdf:resource="http://www.cidoc-crm.org/cidoc-crm/P8i_witnessed"/>
	<rdfs:domain rdf:resource="http://www.cidoc-crm.org/cidoc-crm/E4_Period"/>
	<rdfs:range rdf:resource="http://www.cidoc-crm.org/cidoc-crm/E18_Physical_Thing"/>
	<rdfs:comment xml:lang="en">This property describes the location of an instance of E4 Period with respect to an instance of E18 Physical Thing.
This property is a shortcut of the more fully developed path from E4 Period through P7 took place at, E53 Place, P156i is occupied by to E18 Physical Thing.
It describes a period that can be located with respect to the space defined by an E19 Physical Object such as a ship or a building. The precise geographical location of the object during the period in question may be unknown or unimportant.
For example, the French and German armistice of 22-nd June 1940 was signed in the same railway carriage as the armistice of 11-th November 1918.</rdfs:comment>
	<rdfs:label xml:lang="fr">a eu lieu à</rdfs:label>
	<rdfs:label xml:lang="de">fand statt auf oder innerhalb von</rdfs:label>
	<rdfs:label xml:lang="pt">ocorreu em ou dentro</rdfs:label>
	<rdfs:label xml:lang="en">took place on or within</rdfs:label>
	<rdfs:label xml:lang="el">έλαβε χώρα σε ή εντός</rdfs:label>
	<rdfs:label xml:lang="ru">имел место на или в</rdfs:label>
	<rdfs:label xml:lang="zh">发生的所在对象是</rdfs:label>
</rdf:Description>

<rdf:Description rdf:about="http://www.cidoc-crm.org/cidoc-crm/P8i_witnessed">
	<rdf:type rdf:resource="http://www.w3.org/2002/07/owl#ObjectProperty"/>
	<rdfs:domain rdf:resource="http://www.cidoc-crm.org/cidoc-crm/E18_Physical_Thing"/>
	<rdfs:range rdf:resource="http://www.cidoc-crm.org/cidoc-crm/E4_Period"/>
	<rdfs:label xml:lang="fr">a été témoin de</rdfs:label>
	<rdfs:label xml:lang="de">bezeugte</rdfs:label>
	<rdfs:label xml:lang="pt">testemunhou</rdfs:label>
	<rdfs:label xml:lang="en">witnessed</rdfs:label>
	<rdfs:label xml:lang="el">υπήρξε τόπος του</rdfs:label>
	<rdfs:label xml:lang="ru">являлся местом для</rdfs:label>
	<rdfs:label xml:lang="zh">发生过</rdfs:label>
</rdf:Description>

<rdf:Description rdf:about="http://www.cidoc-crm.org/cidoc-crm/P91_has_unit">
	<rdf:type rdf:resource="http://www.w3.org/2002/07/owl#ObjectProperty"/>
	<owl:inverseOf rdf:resource="http://www.cidoc-crm.org/cidoc-crm/P91i_is_unit_of"/>
	<rdfs:domain rdf:resource="http://www.cidoc-crm.org/cidoc-crm/E54_Dimension"/>
	<rdfs:range rdf:resource="http://www.cidoc-crm.org/cidoc-crm/E58_Measurement_Unit"/>
	<rdfs:comment xml:lang="en">This property shows the type of unit an instance of E54 Dimension was expressed in.</rdfs:comment>
	<rdfs:label xml:lang="fr">a pour unité de mesure</rdfs:label>
	<rdfs:label xml:lang="en">has unit</rdfs:label>
	<rdfs:label xml:lang="de">hat Einheit</rdfs:label>
	<rdfs:label xml:lang="pt">tem unidade</rdfs:label>
	<rdfs:label xml:lang="el">έχει μονάδα μέτρησης</rdfs:label>
	<rdfs:label xml:lang="ru">имеет единицу</rdfs:label>
	<rdfs:label xml:lang="zh">有单位</rdfs:label>
</rdf:Description>

<rdf:Description rdf:about="http://www.cidoc-crm.org/cidoc-crm/P91i_is_unit_of">
	<rdf:type rdf:resource="http://www.w3.org/2002/07/owl#ObjectProperty"/>
	<rdfs:domain rdf:resource="http://www.cidoc-crm.org/cidoc-crm/E58_Measurement_Unit"/>
	<rdfs:range rdf:resource="http://www.cidoc-crm.org/cidoc-crm/E54_Dimension"/>
	<rdfs:label xml:lang="fr">est l’unité de mesure de</rdfs:label>
	<rdfs:label xml:lang="en">is unit of</rdfs:label>
	<rdfs:label xml:lang="de">ist Einheit von</rdfs:label>
	<rdfs:label xml:lang="pt">é unidade de</rdfs:label>
	<rdfs:label xml:lang="el">αποτελεί μονάδα μέτρησης του/της</rdfs:label>
	<rdfs:label xml:lang="ru">является единицей для</rdfs:label>
	<rdfs:label xml:lang="zh">所属单位</rdfs:label>
</rdf:Description>

<rdf:Description rdf:about="http://www.cidoc-crm.org/cidoc-crm/P92_brought_into_existence">
	<rdf:type rdf:resource="http://www.w3.org/2002/07/owl#ObjectProperty"/>
	<rdfs:subPropertyOf rdf:resource="http://www.cidoc-crm.org/cidoc-crm/P12_occurred_in_the_presence_of"/>
	<owl:inverseOf rdf:resource="http://www.cidoc-crm.org/cidoc-crm/P92i_was_brought_into_existence_by"/>
	<rdfs:domain rdf:resource="http://www.cidoc-crm.org/cidoc-crm/E63_Beginning_of_Existence"/>
	<rdfs:range rdf:resource="http://www.cidoc-crm.org/cidoc-crm/E77_Persistent_Item"/>
	<rdfs:comment xml:lang="en">This property links an instance of E63 Beginning of Existence to the instance of E77 Persistent Item brought into existence by it.
It allows a “start” to be attached to any instance of E77 Persistent Item being documented, i.e., as instances of E70 Thing, E72 Legal Object, E39 Actor, E41 Appellation and E55 Type.</rdfs:comment>
	<rdfs:label xml:lang="fr">a fait exister</rdfs:label>
	<rdfs:label xml:lang="de">brachte in Existenz</rdfs:label>
	<rdfs:label xml:lang="en">brought into existence</rdfs:label>
	<rdfs:label xml:lang="pt">trouxe à existência</rdfs:label>
	<rdfs:label xml:lang="el">γέννησε</rdfs:label>
	<rdfs:label xml:lang="ru">создал</rdfs:label>
	<rdfs:label xml:lang="zh">导致存在的是</rdfs:label>
</rdf:Description>

<rdf:Description rdf:about="http://www.cidoc-crm.org/cidoc-crm/P92i_was_brought_into_existence_by">
	<rdf:type rdf:resource="http://www.w3.org/2002/07/owl#ObjectProperty"/>
	<rdfs:subPropertyOf rdf:resource="http://www.cidoc-crm.org/cidoc-crm/P12i_was_present_at"/>
	<rdfs:domain rdf:resource="http://www.cidoc-crm.org/cidoc-crm/E77_Persistent_Item"/>
	<rdfs:range rdf:resource="http://www.cidoc-crm.org/cidoc-crm/E63_Beginning_of_Existence"/>
	<rdfs:label xml:lang="fr">a commencé à exister par</rdfs:label>
	<rdfs:label xml:lang="pt">passou a existir por</rdfs:label>
	<rdfs:label xml:lang="en">was brought into existence by</rdfs:label>
	<rdfs:label xml:lang="de">wurde in Existenz gebracht durch</rdfs:label>
	<rdfs:label xml:lang="el">γεννήθηκε από</rdfs:label>
	<rdfs:label xml:lang="ru">был создан посредством</rdfs:label>
	<rdfs:label xml:lang="zh">使导致存在</rdfs:label>
</rdf:Description>

<rdf:Description rdf:about="http://www.cidoc-crm.org/cidoc-crm/P93_took_out_of_existence">
	<rdf:type rdf:resource="http://www.w3.org/2002/07/owl#ObjectProperty"/>
	<rdfs:subPropertyOf rdf:resource="http://www.cidoc-crm.org/cidoc-crm/P12_occurred_in_the_presence_of"/>
	<owl:inverseOf rdf:resource="http://www.cidoc-crm.org/cidoc-crm/P93i_was_taken_out_of_existence_by"/>
	<rdfs:domain rdf:resource="http://www.cidoc-crm.org/cidoc-crm/E64_End_of_Existence"/>
	<rdfs:range rdf:resource="http://www.cidoc-crm.org/cidoc-crm/E77_Persistent_Item"/>
	<rdfs:comment xml:lang="en">This property links an instance of E64 End of Existence to the instance of E77 Persistent Item taken out of existence by it.
In the case of immaterial things, the instance of E64 End of Existence is considered to take place with the destruction of the last physical carrier.
This allows an “end” to be attached to any instance of E77 Persistent Item being documented i.e. instances of E70 Thing, E72 Legal Object, E39 Actor, E41 Appellation, and E55 Type. For many instances of E77 Persistent Item we know the maximum life-span and can infer that they must have ended to exist. We assume in that case an instance of E64 End of Existence, which may be as unnoticeable as forgetting the secret knowledge by the last representative of some indigenous nation.</rdfs:comment>
	<rdfs:label xml:lang="fr">a mis fin à l’existence de</rdfs:label>
	<rdfs:label xml:lang="de">beendete die Existenz von</rdfs:label>
	<rdfs:label xml:lang="pt">cessou a existência de</rdfs:label>
	<rdfs:label xml:lang="en">took out of existence</rdfs:label>
	<rdfs:label xml:lang="el">αναίρεσε</rdfs:label>
	<rdfs:label xml:lang="ru">положил конец существованию</rdfs:label>
	<rdfs:label xml:lang="zh">结束存在的是</rdfs:label>
</rdf:Description>

<rdf:Description rdf:about="http://www.cidoc-crm.org/cidoc-crm/P93i_was_taken_out_of_existence_by">
	<rdf:type rdf:resource="http://www.w3.org/2002/07/owl#ObjectProperty"/>
	<rdfs:subPropertyOf rdf:resource="http://www.cidoc-crm.org/cidoc-crm/P12i_was_present_at"/>
	<rdfs:domain rdf:resource="http://www.cidoc-crm.org/cidoc-crm/E77_Persistent_Item"/>
	<rdfs:range rdf:resource="http://www.cidoc-crm.org/cidoc-crm/E64_End_of_Existence"/>
	<rdfs:label xml:lang="fr">a cessé d’exister par</rdfs:label>
	<rdfs:label xml:lang="pt">deixou de existir</rdfs:label>
	<rdfs:label xml:lang="en">was taken out of existence by</rdfs:label>
	<rdfs:label xml:lang="de">wurde seiner Existenz beraubt durch</rdfs:label>
	<rdfs:label xml:lang="el">αναιρέθηκε από</rdfs:label>
	<rdfs:label xml:lang="ru">прекратил существование посредством</rdfs:label>
	<rdfs:label xml:lang="zh">被结束存在</rdfs:label>
</rdf:Description>

<rdf:Description rdf:about="http://www.cidoc-crm.org/cidoc-crm/P94_has_created">
	<rdf:type rdf:resource="http://www.w3.org/2002/07/owl#ObjectProperty"/>
	<rdfs:subPropertyOf rdf:resource="http://www.cidoc-crm.org/cidoc-crm/P92_brought_into_existence"/>
	<owl:inverseOf rdf:resource="http://www.cidoc-crm.org/cidoc-crm/P94i_was_created_by"/>
	<rdfs:domain rdf:resource="http://www.cidoc-crm.org/cidoc-crm/E65_Creation"/>
	<rdfs:range rdf:resource="http://www.cidoc-crm.org/cidoc-crm/E28_Conceptual_Object"/>
	<rdfs:comment xml:lang="en">This property links an instance of E65 Creation to the instance of E28 Conceptual Object created by it.
It represents the act of conceiving the intellectual content of the instance of E28 Conceptual Object. It does not represent the act of creating the first physical carrier of the instance of E28 Conceptual Object. As an example, this is the composition of a poem, not its commitment to paper.</rdfs:comment>
	<rdfs:label xml:lang="fr">a créé</rdfs:label>
	<rdfs:label xml:lang="pt">criou</rdfs:label>
	<rdfs:label xml:lang="en">has created</rdfs:label>
	<rdfs:label xml:lang="de">hat erschaffen</rdfs:label>
	<rdfs:label xml:lang="el">δημιούργησε</rdfs:label>
	<rdfs:label xml:lang="ru">создал</rdfs:label>
	<rdfs:label xml:lang="zh">已创建了</rdfs:label>
</rdf:Description>

<rdf:Description rdf:about="http://www.cidoc-crm.org/cidoc-crm/P94i_was_created_by">
	<rdf:type rdf:resource="http://www.w3.org/2002/07/owl#ObjectProperty"/>
	<rdfs:subPropertyOf rdf:resource="http://www.cidoc-crm.org/cidoc-crm/P92i_was_brought_into_existence_by"/>
	<rdfs:domain rdf:resource="http://www.cidoc-crm.org/cidoc-crm/E28_Conceptual_Object"/>
	<rdfs:range rdf:resource="http://www.cidoc-crm.org/cidoc-crm/E65_Creation"/>
	<rdfs:label xml:lang="fr">a été créé par</rdfs:label>
	<rdfs:label xml:lang="pt">foi criado por</rdfs:label>
	<rdfs:label xml:lang="en">was created by</rdfs:label>
	<rdfs:label xml:lang="de">wurde erschaffen durch</rdfs:label>
	<rdfs:label xml:lang="el">δημιουργήθηκε από</rdfs:label>
	<rdfs:label xml:lang="ru">был создан посредством</rdfs:label>
	<rdfs:label xml:lang="zh">被创建</rdfs:label>
</rdf:Description>

<rdf:Description rdf:about="http://www.cidoc-crm.org/cidoc-crm/P95_has_formed">
	<rdf:type rdf:resource="http://www.w3.org/2002/07/owl#ObjectProperty"/>
	<rdfs:subPropertyOf rdf:resource="http://www.cidoc-crm.org/cidoc-crm/P92_brought_into_existence"/>
	<owl:inverseOf rdf:resource="http://www.cidoc-crm.org/cidoc-crm/P95i_was_formed_by"/>
	<rdfs:domain rdf:resource="http://www.cidoc-crm.org/cidoc-crm/E66_Formation"/>
	<rdfs:range rdf:resource="http://www.cidoc-crm.org/cidoc-crm/E74_Group"/>
	<rdfs:comment xml:lang="en">This property associates the instance of E66 Formation with the instance of E74 Group that it founded.</rdfs:comment>
	<rdfs:label xml:lang="fr">a fondé</rdfs:label>
	<rdfs:label xml:lang="pt">formou</rdfs:label>
	<rdfs:label xml:lang="en">has formed</rdfs:label>
	<rdfs:label xml:lang="de">hat gebildet</rdfs:label>
	<rdfs:label xml:lang="el">σχημάτισε</rdfs:label>
	<rdfs:label xml:lang="ru">сформировал</rdfs:label>
	<rdfs:label xml:lang="zh">已经组成</rdfs:label>
</rdf:Description>

<rdf:Description rdf:about="http://www.cidoc-crm.org/cidoc-crm/P95i_was_formed_by">
	<rdf:type rdf:resource="http://www.w3.org/2002/07/owl#ObjectProperty"/>
	<rdfs:subPropertyOf rdf:resource="http://www.cidoc-crm.org/cidoc-crm/P92i_was_brought_into_existence_by"/>
	<rdfs:domain rdf:resource="http://www.cidoc-crm.org/cidoc-crm/E74_Group"/>
	<rdfs:range rdf:resource="http://www.cidoc-crm.org/cidoc-crm/E66_Formation"/>
	<rdfs:label xml:lang="fr">a été fondé par</rdfs:label>
	<rdfs:label xml:lang="pt">foi formado por</rdfs:label>
	<rdfs:label xml:lang="en">was formed by</rdfs:label>
	<rdfs:label xml:lang="de">wurde gebildet von</rdfs:label>
	<rdfs:label xml:lang="el">σχηματίστηκε από</rdfs:label>
	<rdfs:label xml:lang="ru">была сформирована посредством</rdfs:label>
	<rdfs:label xml:lang="zh">被组成</rdfs:label>
</rdf:Description>

<rdf:Description rdf:about="http://www.cidoc-crm.org/cidoc-crm/P96_by_mother">
	<rdf:type rdf:resource="http://www.w3.org/2002/07/owl#ObjectProperty"/>
	<rdfs:subPropertyOf rdf:resource="http://www.cidoc-crm.org/cidoc-crm/P11_had_participant"/>
	<owl:inverseOf rdf:resource="http://www.cidoc-crm.org/cidoc-crm/P96i_gave_birth"/>
	<rdfs:domain rdf:resource="http://www.cidoc-crm.org/cidoc-crm/E67_Birth"/>
	<rdfs:range rdf:resource="http://www.cidoc-crm.org/cidoc-crm/E21_Person"/>
	<rdfs:comment xml:lang="en">This property links an instance of E67 Birth to an instance of E21 Person in the role of birth-giving mother.
Note that biological fathers are not necessarily participants in the Birth (see P97 from father (was father for)). The instance of E21 Person being born is linked to the instance of E67 Birth with the property P98 brought into life (was born). This is not intended for use with general natural history material, only people. There is no explicit method for modelling conception and gestation except by using extensions.</rdfs:comment>
	<rdfs:label xml:lang="en">by mother</rdfs:label>
	<rdfs:label xml:lang="fr">de mère</rdfs:label>
	<rdfs:label xml:lang="de">durch Mutter</rdfs:label>
	<rdfs:label xml:lang="pt">pela mãe</rdfs:label>
	<rdfs:label xml:lang="el">είχε μητέρα</rdfs:label>
	<rdfs:label xml:lang="ru">посредством матери</rdfs:label>
	<rdfs:label xml:lang="zh">来自母亲</rdfs:label>
</rdf:Description>

<rdf:Description rdf:about="http://www.cidoc-crm.org/cidoc-crm/P96i_gave_birth">
	<rdf:type rdf:resource="http://www.w3.org/2002/07/owl#ObjectProperty"/>
	<rdfs:subPropertyOf rdf:resource="http://www.cidoc-crm.org/cidoc-crm/P11i_participated_in"/>
	<rdfs:domain rdf:resource="http://www.cidoc-crm.org/cidoc-crm/E21_Person"/>
	<rdfs:range rdf:resource="http://www.cidoc-crm.org/cidoc-crm/E67_Birth"/>
	<rdfs:label xml:lang="fr">a donné naissance à</rdfs:label>
	<rdfs:label xml:lang="pt">deu nascimento</rdfs:label>
	<rdfs:label xml:lang="en">gave birth</rdfs:label>
	<rdfs:label xml:lang="de">gebar</rdfs:label>
	<rdfs:label xml:lang="el">ήταν μητέρα του/της</rdfs:label>
	<rdfs:label xml:lang="ru">дал рождение</rdfs:label>
	<rdfs:label xml:lang="zh">生育</rdfs:label>
</rdf:Description>

<rdf:Description rdf:about="http://www.cidoc-crm.org/cidoc-crm/P97_from_father">
	<rdf:type rdf:resource="http://www.w3.org/2002/07/owl#ObjectProperty"/>
	<owl:inverseOf rdf:resource="http://www.cidoc-crm.org/cidoc-crm/P97i_was_father_for"/>
	<rdfs:domain rdf:resource="http://www.cidoc-crm.org/cidoc-crm/E67_Birth"/>
	<rdfs:range rdf:resource="http://www.cidoc-crm.org/cidoc-crm/E21_Person"/>
	<rdfs:comment xml:lang="en">This property links an instance of E67 Birth to an instance of E21 Person in the role of biological father.
Note that biological fathers are not seen as necessary participants in the birth, whereas birth-giving mothers are (see P96 by mother (gave birth)). The Person being born is linked to the Birth with the property P98 brought into life (was born).
This is not intended for use with general natural history material, only people. There is no explicit method for modelling conception and gestation except by using extensions.
An instance of E67 Birth is normally (but not always) associated with one biological father.</rdfs:comment>
	<rdfs:label xml:lang="fr">de père</rdfs:label>
	<rdfs:label xml:lang="en">from father</rdfs:label>
	<rdfs:label xml:lang="de">gab Vaterschaft</rdfs:label>
	<rdfs:label xml:lang="pt">pelo pai</rdfs:label>
	<rdfs:label xml:lang="el">είχε πατέρα</rdfs:label>
	<rdfs:label xml:lang="ru">от отца</rdfs:label>
	<rdfs:label xml:lang="zh">来自父亲</rdfs:label>
</rdf:Description>

<rdf:Description rdf:about="http://www.cidoc-crm.org/cidoc-crm/P97i_was_father_for">
	<rdf:type rdf:resource="http://www.w3.org/2002/07/owl#ObjectProperty"/>
	<rdfs:domain rdf:resource="http://www.cidoc-crm.org/cidoc-crm/E21_Person"/>
	<rdfs:range rdf:resource="http://www.cidoc-crm.org/cidoc-crm/E67_Birth"/>
	<rdfs:label xml:lang="fr">a été le père pour</rdfs:label>
	<rdfs:label xml:lang="pt">foi pai para</rdfs:label>
	<rdfs:label xml:lang="de">war Vater für</rdfs:label>
	<rdfs:label xml:lang="en">was father for</rdfs:label>
	<rdfs:label xml:lang="el">ήταν πατέρας του/της</rdfs:label>
	<rdfs:label xml:lang="ru">был отцом для</rdfs:label>
	<rdfs:label xml:lang="zh">是父亲</rdfs:label>
</rdf:Description>

<rdf:Description rdf:about="http://www.cidoc-crm.org/cidoc-crm/P98_brought_into_life">
	<rdf:type rdf:resource="http://www.w3.org/2002/07/owl#ObjectProperty"/>
	<rdfs:subPropertyOf rdf:resource="http://www.cidoc-crm.org/cidoc-crm/P92_brought_into_existence"/>
	<owl:inverseOf rdf:resource="http://www.cidoc-crm.org/cidoc-crm/P98i_was_born"/>
	<rdfs:domain rdf:resource="http://www.cidoc-crm.org/cidoc-crm/E67_Birth"/>
	<rdfs:range rdf:resource="http://www.cidoc-crm.org/cidoc-crm/E21_Person"/>
	<rdfs:comment xml:lang="en">This property links an instance of E67 Birth event to an instance of E21 Person in the role of offspring.
Twins, triplets etc. are brought into life by the same instance of E67 Birth. This is not intended for use with general Natural History material, only people. There is no explicit method for modelling conception and gestation except by using extensions.</rdfs:comment>
	<rdfs:label xml:lang="fr">a donné vie à</rdfs:label>
	<rdfs:label xml:lang="de">brachte zur Welt</rdfs:label>
	<rdfs:label xml:lang="en">brought into life</rdfs:label>
	<rdfs:label xml:lang="pt">trouxe à vida</rdfs:label>
	<rdfs:label xml:lang="el">έφερε στη ζωή</rdfs:label>
	<rdfs:label xml:lang="ru">породил</rdfs:label>
	<rdfs:label xml:lang="zh">诞生了</rdfs:label>
</rdf:Description>

<rdf:Description rdf:about="http://www.cidoc-crm.org/cidoc-crm/P98i_was_born">
	<rdf:type rdf:resource="http://www.w3.org/2002/07/owl#ObjectProperty"/>
	<rdfs:subPropertyOf rdf:resource="http://www.cidoc-crm.org/cidoc-crm/P92i_was_brought_into_existence_by"/>
	<rdfs:domain rdf:resource="http://www.cidoc-crm.org/cidoc-crm/E21_Person"/>
	<rdfs:range rdf:resource="http://www.cidoc-crm.org/cidoc-crm/E67_Birth"/>
	<rdfs:label xml:lang="fr">est né</rdfs:label>
	<rdfs:label xml:lang="pt">veio à vida pelo</rdfs:label>
	<rdfs:label xml:lang="en">was born</rdfs:label>
	<rdfs:label xml:lang="de">wurde geboren durch</rdfs:label>
	<rdfs:label xml:lang="el">γεννήθηκε</rdfs:label>
	<rdfs:label xml:lang="ru">был рожден</rdfs:label>
	<rdfs:label xml:lang="zh">被诞生</rdfs:label>
</rdf:Description>

<rdf:Description rdf:about="http://www.cidoc-crm.org/cidoc-crm/P99_dissolved">
	<rdf:type rdf:resource="http://www.w3.org/2002/07/owl#ObjectProperty"/>
	<rdfs:subPropertyOf rdf:resource="http://www.cidoc-crm.org/cidoc-crm/P11_had_participant"/>
	<rdfs:subPropertyOf rdf:resource="http://www.cidoc-crm.org/cidoc-crm/P93_took_out_of_existence"/>
	<owl:inverseOf rdf:resource="http://www.cidoc-crm.org/cidoc-crm/P99i_was_dissolved_by"/>
	<rdfs:domain rdf:resource="http://www.cidoc-crm.org/cidoc-crm/E68_Dissolution"/>
	<rdfs:range rdf:resource="http://www.cidoc-crm.org/cidoc-crm/E74_Group"/>
	<rdfs:comment xml:lang="en">This property associates the instance of E68 Dissolution with the instance of E74 Group that it disbanded.</rdfs:comment>
	<rdfs:label xml:lang="fr">a dissous</rdfs:label>
	<rdfs:label xml:lang="en">dissolved</rdfs:label>
	<rdfs:label xml:lang="pt">dissolveu</rdfs:label>
	<rdfs:label xml:lang="de">löste auf</rdfs:label>
	<rdfs:label xml:lang="el">διέλυσε</rdfs:label>
	<rdfs:label xml:lang="ru">распустил</rdfs:label>
	<rdfs:label xml:lang="zh">解散了</rdfs:label>
</rdf:Description>

<rdf:Description rdf:about="http://www.cidoc-crm.org/cidoc-crm/P99i_was_dissolved_by">
	<rdf:type rdf:resource="http://www.w3.org/2002/07/owl#ObjectProperty"/>
	<rdfs:subPropertyOf rdf:resource="http://www.cidoc-crm.org/cidoc-crm/P11i_participated_in"/>
	<rdfs:subPropertyOf rdf:resource="http://www.cidoc-crm.org/cidoc-crm/P93i_was_taken_out_of_existence_by"/>
	<rdfs:domain rdf:resource="http://www.cidoc-crm.org/cidoc-crm/E74_Group"/>
	<rdfs:range rdf:resource="http://www.cidoc-crm.org/cidoc-crm/E68_Dissolution"/>
	<rdfs:label xml:lang="fr">a été dissous par</rdfs:label>
	<rdfs:label xml:lang="pt">foi dissolvido por</rdfs:label>
	<rdfs:label xml:lang="en">was dissolved by</rdfs:label>
	<rdfs:label xml:lang="de">wurde aufgelöst durch</rdfs:label>
	<rdfs:label xml:lang="el">διαλύθηκε από</rdfs:label>
	<rdfs:label xml:lang="ru">был распущен посредством</rdfs:label>
	<rdfs:label xml:lang="zh">被解散</rdfs:label>
</rdf:Description>

<rdf:Description rdf:about="http://www.cidoc-crm.org/cidoc-crm/P9_consists_of">
	<rdf:type rdf:resource="http://www.w3.org/2002/07/owl#ObjectProperty"/>
	<rdfs:subPropertyOf rdf:resource="http://www.cidoc-crm.org/cidoc-crm/P10i_contains"/>
	<owl:inverseOf rdf:resource="http://www.cidoc-crm.org/cidoc-crm/P9i_forms_part_of"/>
	<rdfs:domain rdf:resource="http://www.cidoc-crm.org/cidoc-crm/E4_Period"/>
	<rdfs:range rdf:resource="http://www.cidoc-crm.org/cidoc-crm/E4_Period"/>
	<rdfs:comment xml:lang="en">This property associates an instance of E4 Period with another instance of E4 Period that is defined by a subset of the phenomena that define the former. Therefore, the spacetime volume of the latter must fall within the spacetime volume of the former.
This property is transitive and asymmetric.</rdfs:comment>
	<rdfs:label xml:lang="fr">comprend</rdfs:label>
	<rdfs:label xml:lang="pt">consiste de</rdfs:label>
	<rdfs:label xml:lang="en">consists of</rdfs:label>
	<rdfs:label xml:lang="de">setzt sich zusammen aus</rdfs:label>
	<rdfs:label xml:lang="el">αποτελείται από</rdfs:label>
	<rdfs:label xml:lang="ru">состоит из</rdfs:label>
	<rdfs:label xml:lang="zh">包括</rdfs:label>
</rdf:Description>

<rdf:Description rdf:about="http://www.cidoc-crm.org/cidoc-crm/P9i_forms_part_of">
	<rdf:type rdf:resource="http://www.w3.org/2002/07/owl#ObjectProperty"/>
	<rdfs:subPropertyOf rdf:resource="http://www.cidoc-crm.org/cidoc-crm/P10_falls_within"/>
	<rdfs:domain rdf:resource="http://www.cidoc-crm.org/cidoc-crm/E4_Period"/>
	<rdfs:range rdf:resource="http://www.cidoc-crm.org/cidoc-crm/E4_Period"/>
	<rdfs:label xml:lang="de">bildet Teil von</rdfs:label>
	<rdfs:label xml:lang="fr">fait partie de</rdfs:label>
	<rdfs:label xml:lang="pt">faz parte de</rdfs:label>
	<rdfs:label xml:lang="en">forms part of</rdfs:label>
	<rdfs:label xml:lang="el">αποτελεί μέρος του/της</rdfs:label>
	<rdfs:label xml:lang="ru">формирует часть</rdfs:label>
	<rdfs:label xml:lang="zh">组成部分</rdfs:label>
</rdf:Description>

<rdf:Description rdf:about="http://www.loa-cnr.it/ontologies/DnS#involves">
	<rdf:type rdf:resource="http://www.w3.org/2002/07/owl#ObjectProperty"/>
	<owl:inverseOf rdf:resource="http://www.loa-cnr.it/ontologies/DnS#nvolved-in"/>
</rdf:Description>

<rdf:Description rdf:about="http://www.loa-cnr.it/ontologies/DnS#nvolved-in">
	<rdf:type rdf:resource="http://www.w3.org/2002/07/owl#ObjectProperty"/>
	<rdfs:subPropertyOf rdf:resource="http://www.w3.org/2002/07/owl#topObjectProperty"/>
	<rdfs:domain rdf:resource="http://www.loa-cnr.it/ontologies/DOLCE-Lite#endurant"/>
	<rdfs:range rdf:resource="http://www.loa-cnr.it/ontologies/DnS#description"/>
</rdf:Description>

<rdf:Description rdf:about="http://www.w3.org/2002/07/owl#topObjectProperty">
	<rdf:type rdf:resource="http://www.w3.org/2002/07/owl#SymmetricProperty"/>
	<rdf:type rdf:resource="http://www.w3.org/2002/07/owl#TransitiveProperty"/>
	<rdf:type rdf:resource="http://www.w3.org/2002/07/owl#ReflexiveProperty"/>
</rdf:Description>

<rdf:Description rdf:about="http://www.w3.org/2004/02/skos/core#broadMatch">
	<rdf:type rdf:resource="http://www.w3.org/2002/07/owl#ObjectProperty"/>
	<rdfs:subPropertyOf rdf:resource="http://www.w3.org/2004/02/skos/core#broader"/>
	<rdfs:subPropertyOf rdf:resource="http://www.w3.org/2004/02/skos/core#mappingRelation"/>
	<owl:inverseOf rdf:resource="http://www.w3.org/2004/02/skos/core#narrowMatch"/>
	<rdfs:isDefinedBy rdf:resource="http://www.w3.org/2004/02/skos/core"/>
	<rdfs:label xml:lang="en">has broader match</rdfs:label>
	<skos:definition xml:lang="en">skos:broadMatch is used to state a hierarchical mapping link between two conceptual resources in different concept schemes.</skos:definition>
</rdf:Description>

<rdf:Description rdf:about="http://www.w3.org/2004/02/skos/core#broader">
	<rdf:type rdf:resource="http://www.w3.org/2002/07/owl#ObjectProperty"/>
	<rdfs:subPropertyOf rdf:resource="http://www.w3.org/2004/02/skos/core#broaderTransitive"/>
	<owl:inverseOf rdf:resource="http://www.w3.org/2004/02/skos/core#narrower"/>
	<rdfs:comment xml:lang="en">Broader concepts are typically rendered as parents in a concept hierarchy (tree).</rdfs:comment>
	<rdfs:isDefinedBy rdf:resource="http://www.w3.org/2004/02/skos/core"/>
	<rdfs:label xml:lang="en">has broader</rdfs:label>
	<skos:definition xml:lang="en">Relates a concept to a concept that is more general in meaning.</skos:definition>
	<skos:scopeNote xml:lang="en">By convention, skos:broader is only used to assert an immediate (i.e. direct) hierarchical link between two conceptual resources.</skos:scopeNote>
</rdf:Description>

<rdf:Description rdf:about="http://www.w3.org/2004/02/skos/core#broaderTransitive">
	<rdf:type rdf:resource="http://www.w3.org/2002/07/owl#ObjectProperty"/>
	<rdfs:subPropertyOf rdf:resource="http://www.w3.org/2004/02/skos/core#semanticRelation"/>
	<owl:inverseOf rdf:resource="http://www.w3.org/2004/02/skos/core#narrowerTransitive"/>
	<rdf:type rdf:resource="http://www.w3.org/2002/07/owl#TransitiveProperty"/>
	<rdfs:isDefinedBy rdf:resource="http://www.w3.org/2004/02/skos/core"/>
	<rdfs:label xml:lang="en">has broader transitive</rdfs:label>
	<skos:definition>skos:broaderTransitive is a transitive superproperty of skos:broader.</skos:definition>
	<skos:scopeNote xml:lang="en">By convention, skos:broaderTransitive is not used to make assertions. Rather, the properties can be used to draw inferences about the transitive closure of the hierarchical relation, which is useful e.g. when implementing a simple query expansion algorithm in a search application.</skos:scopeNote>
</rdf:Description>

<rdf:Description rdf:about="http://www.w3.org/2004/02/skos/core#closeMatch">
	<rdf:type rdf:resource="http://www.w3.org/2002/07/owl#ObjectProperty"/>
	<rdfs:subPropertyOf rdf:resource="http://www.w3.org/2004/02/skos/core#mappingRelation"/>
	<owl:inverseOf rdf:resource="http://www.w3.org/2004/02/skos/core#closeMatch"/>
	<rdf:type rdf:resource="http://www.w3.org/2002/07/owl#SymmetricProperty"/>
	<rdfs:isDefinedBy rdf:resource="http://www.w3.org/2004/02/skos/core"/>
	<rdfs:label xml:lang="en">has close match</rdfs:label>
	<skos:definition xml:lang="en">skos:closeMatch is used to link two concepts that are sufficiently similar that they can be used interchangeably in some information retrieval applications. In order to avoid the possibility of "compound errors" when combining mappings across more than two concept schemes, skos:closeMatch is not declared to be a transitive property.</skos:definition>
</rdf:Description>

<rdf:Description rdf:about="http://www.w3.org/2004/02/skos/core#exactMatch">
	<rdf:type rdf:resource="http://www.w3.org/2002/07/owl#ObjectProperty"/>
	<rdfs:subPropertyOf rdf:resource="http://www.w3.org/2004/02/skos/core#closeMatch"/>
	<owl:inverseOf rdf:resource="http://www.w3.org/2004/02/skos/core#exactMatch"/>
	<rdf:type rdf:resource="http://www.w3.org/2002/07/owl#SymmetricProperty"/>
	<rdf:type rdf:resource="http://www.w3.org/2002/07/owl#TransitiveProperty"/>
	<rdfs:comment xml:lang="en">skos:exactMatch is disjoint with each of the properties skos:broadMatch and skos:relatedMatch.</rdfs:comment>
	<rdfs:isDefinedBy rdf:resource="http://www.w3.org/2004/02/skos/core"/>
	<rdfs:label xml:lang="en">has exact match</rdfs:label>
	<skos:definition xml:lang="en">skos:exactMatch is used to link two concepts, indicating a high degree of confidence that the concepts can be used interchangeably across a wide range of information retrieval applications. skos:exactMatch is a transitive property, and is a sub-property of skos:closeMatch.</skos:definition>
</rdf:Description>

<rdf:Description rdf:about="http://www.w3.org/2004/02/skos/core#hasTopConcept">
	<rdf:type rdf:resource="http://www.w3.org/2002/07/owl#ObjectProperty"/>
	<owl:inverseOf rdf:resource="http://www.w3.org/2004/02/skos/core#topConceptOf"/>
	<rdfs:domain rdf:resource="http://www.w3.org/2004/02/skos/core#ConceptScheme"/>
	<rdfs:range rdf:resource="http://www.w3.org/2004/02/skos/core#Concept"/>
	<rdfs:isDefinedBy rdf:resource="http://www.w3.org/2004/02/skos/core"/>
	<rdfs:label xml:lang="en">has top concept</rdfs:label>
	<skos:definition xml:lang="en">Relates, by convention, a concept scheme to a concept which is topmost in the broader/narrower concept hierarchies for that scheme, providing an entry point to these hierarchies.</skos:definition>
</rdf:Description>

<rdf:Description rdf:about="http://www.w3.org/2004/02/skos/core#inScheme">
	<rdf:type rdf:resource="http://www.w3.org/2002/07/owl#ObjectProperty"/>
	<rdfs:range rdf:resource="http://www.w3.org/2004/02/skos/core#ConceptScheme"/>
	<rdfs:isDefinedBy rdf:resource="http://www.w3.org/2004/02/skos/core"/>
	<rdfs:label xml:lang="en">is in scheme</rdfs:label>
	<skos:definition xml:lang="en">Relates a resource (for example a concept) to a concept scheme in which it is included.</skos:definition>
	<skos:scopeNote xml:lang="en">A concept may be a member of more than one concept scheme.</skos:scopeNote>
</rdf:Description>

<rdf:Description rdf:about="http://www.w3.org/2004/02/skos/core#mappingRelation">
	<rdf:type rdf:resource="http://www.w3.org/2002/07/owl#ObjectProperty"/>
	<rdfs:subPropertyOf rdf:resource="http://www.w3.org/2004/02/skos/core#semanticRelation"/>
	<rdfs:comment xml:lang="en">These concept mapping relations mirror semantic relations, and the data model defined below is similar (with the exception of skos:exactMatch) to the data model defined for semantic relations. A distinct vocabulary is provided for concept mapping relations, to provide a convenient way to differentiate links within a concept scheme from links between concept schemes. However, this pattern of usage is not a formal requirement of the SKOS data model, and relies on informal definitions of best practice.</rdfs:comment>
	<rdfs:isDefinedBy rdf:resource="http://www.w3.org/2004/02/skos/core"/>
	<rdfs:label xml:lang="en">is in mapping relation with</rdfs:label>
	<skos:definition xml:lang="en">Relates two concepts coming, by convention, from different schemes, and that have comparable meanings</skos:definition>
</rdf:Description>

<rdf:Description rdf:about="http://www.w3.org/2004/02/skos/core#member">
	<rdf:type rdf:resource="http://www.w3.org/2002/07/owl#ObjectProperty"/>
	<rdfs:domain rdf:resource="http://www.w3.org/2004/02/skos/core#Collection"/>
	<rdfs:range rdf:nodeID="genid-start-3308b2a0b3545f9b5"/>
</rdf:Description>

<rdf:Description rdf:nodeID="genid-start-3308b2a0b3545f9b5">
	<rdf:type rdf:resource="http://www.w3.org/2002/07/owl#Class"/>
	<owl:unionOf rdf:nodeID="genid-start-3308b2a0b3545f9b6"/>
</rdf:Description>

<rdf:Description rdf:nodeID="genid-start-3308b2a0b3545f9b6">
	<rdf:first rdf:resource="http://www.w3.org/2004/02/skos/core#Collection"/>
	<rdf:rest rdf:nodeID="genid-start-3308b2a0b3545f9b7"/>
</rdf:Description>

<rdf:Description rdf:nodeID="genid-start-3308b2a0b3545f9b7">
	<rdf:first rdf:resource="http://www.w3.org/2004/02/skos/core#Concept"/>
	<rdf:rest rdf:resource="http://www.w3.org/1999/02/22-rdf-syntax-ns#nil"/>
</rdf:Description>

<rdf:Description rdf:about="http://www.w3.org/2004/02/skos/core#member">
	<rdfs:isDefinedBy rdf:resource="http://www.w3.org/2004/02/skos/core"/>
	<rdfs:label xml:lang="en">has member</rdfs:label>
	<skos:definition xml:lang="en">Relates a collection to one of its members.</skos:definition>
</rdf:Description>

<rdf:Description rdf:about="http://www.w3.org/2004/02/skos/core#memberList">
	<rdf:type rdf:resource="http://www.w3.org/2002/07/owl#ObjectProperty"/>
	<rdf:type rdf:resource="http://www.w3.org/2002/07/owl#FunctionalProperty"/>
	<rdfs:domain rdf:resource="http://www.w3.org/2004/02/skos/core#OrderedCollection"/>
	<rdfs:range rdf:resource="http://www.w3.org/1999/02/22-rdf-syntax-ns#List"/>
	<rdfs:comment xml:lang="en">For any resource, every item in the list given as the value of the
      skos:memberList property is also a value of the skos:member property.</rdfs:comment>
	<rdfs:isDefinedBy rdf:resource="http://www.w3.org/2004/02/skos/core"/>
	<rdfs:label xml:lang="en">has member list</rdfs:label>
	<skos:definition xml:lang="en">Relates an ordered collection to the RDF list containing its members.</skos:definition>
</rdf:Description>

<rdf:Description rdf:about="http://www.w3.org/2004/02/skos/core#narrowMatch">
	<rdf:type rdf:resource="http://www.w3.org/2002/07/owl#ObjectProperty"/>
	<rdfs:subPropertyOf rdf:resource="http://www.w3.org/2004/02/skos/core#mappingRelation"/>
	<rdfs:subPropertyOf rdf:resource="http://www.w3.org/2004/02/skos/core#narrower"/>
	<rdfs:isDefinedBy rdf:resource="http://www.w3.org/2004/02/skos/core"/>
	<rdfs:label xml:lang="en">has narrower match</rdfs:label>
	<skos:definition xml:lang="en">skos:narrowMatch is used to state a hierarchical mapping link between two conceptual resources in different concept schemes.</skos:definition>
</rdf:Description>

<rdf:Description rdf:about="http://www.w3.org/2004/02/skos/core#narrower">
	<rdf:type rdf:resource="http://www.w3.org/2002/07/owl#ObjectProperty"/>
	<rdfs:subPropertyOf rdf:resource="http://www.w3.org/2004/02/skos/core#narrowerTransitive"/>
	<rdfs:comment xml:lang="en">Narrower concepts are typically rendered as children in a concept hierarchy (tree).</rdfs:comment>
	<rdfs:isDefinedBy rdf:resource="http://www.w3.org/2004/02/skos/core"/>
	<rdfs:label xml:lang="en">has narrower</rdfs:label>
	<skos:definition xml:lang="en">Relates a concept to a concept that is more specific in meaning.</skos:definition>
	<skos:scopeNote xml:lang="en">By convention, skos:broader is only used to assert an immediate (i.e. direct) hierarchical link between two conceptual resources.</skos:scopeNote>
</rdf:Description>

<rdf:Description rdf:about="http://www.w3.org/2004/02/skos/core#narrowerTransitive">
	<rdf:type rdf:resource="http://www.w3.org/2002/07/owl#ObjectProperty"/>
	<rdfs:subPropertyOf rdf:resource="http://www.w3.org/2004/02/skos/core#semanticRelation"/>
	<rdf:type rdf:resource="http://www.w3.org/2002/07/owl#TransitiveProperty"/>
	<rdfs:isDefinedBy rdf:resource="http://www.w3.org/2004/02/skos/core"/>
	<rdfs:label xml:lang="en">has narrower transitive</rdfs:label>
	<skos:definition>skos:narrowerTransitive is a transitive superproperty of skos:narrower.</skos:definition>
	<skos:scopeNote xml:lang="en">By convention, skos:narrowerTransitive is not used to make assertions. Rather, the properties can be used to draw inferences about the transitive closure of the hierarchical relation, which is useful e.g. when implementing a simple query expansion algorithm in a search application.</skos:scopeNote>
</rdf:Description>

<rdf:Description rdf:about="http://www.w3.org/2004/02/skos/core#related">
	<rdf:type rdf:resource="http://www.w3.org/2002/07/owl#ObjectProperty"/>
	<rdfs:subPropertyOf rdf:resource="http://www.w3.org/2004/02/skos/core#semanticRelation"/>
	<owl:inverseOf rdf:resource="http://www.w3.org/2004/02/skos/core#related"/>
	<rdf:type rdf:resource="http://www.w3.org/2002/07/owl#SymmetricProperty"/>
	<rdfs:comment xml:lang="en">skos:related is disjoint with skos:broaderTransitive</rdfs:comment>
	<rdfs:isDefinedBy rdf:resource="http://www.w3.org/2004/02/skos/core"/>
	<rdfs:label xml:lang="en">has related</rdfs:label>
	<skos:definition xml:lang="en">Relates a concept to a concept with which there is an associative semantic relationship.</skos:definition>
</rdf:Description>

<rdf:Description rdf:about="http://www.w3.org/2004/02/skos/core#relatedMatch">
	<rdf:type rdf:resource="http://www.w3.org/2002/07/owl#ObjectProperty"/>
	<rdfs:subPropertyOf rdf:resource="http://www.w3.org/2004/02/skos/core#mappingRelation"/>
	<rdfs:subPropertyOf rdf:resource="http://www.w3.org/2004/02/skos/core#related"/>
	<owl:inverseOf rdf:resource="http://www.w3.org/2004/02/skos/core#relatedMatch"/>
	<rdf:type rdf:resource="http://www.w3.org/2002/07/owl#SymmetricProperty"/>
	<rdfs:isDefinedBy rdf:resource="http://www.w3.org/2004/02/skos/core"/>
	<rdfs:label xml:lang="en">has related match</rdfs:label>
	<skos:definition xml:lang="en">skos:relatedMatch is used to state an associative mapping link between two conceptual resources in different concept schemes.</skos:definition>
</rdf:Description>

<rdf:Description rdf:about="http://www.w3.org/2004/02/skos/core#semanticRelation">
	<rdf:type rdf:resource="http://www.w3.org/2002/07/owl#ObjectProperty"/>
	<rdfs:domain rdf:resource="http://www.w3.org/2004/02/skos/core#Concept"/>
	<rdfs:range rdf:resource="http://www.w3.org/2004/02/skos/core#Concept"/>
	<rdfs:isDefinedBy rdf:resource="http://www.w3.org/2004/02/skos/core"/>
	<rdfs:label xml:lang="en">is in semantic relation with</rdfs:label>
	<skos:definition xml:lang="en">Links a concept to a concept related by meaning.</skos:definition>
	<skos:scopeNote xml:lang="en">This property should not be used directly, but as a super-property for all properties denoting a relationship of meaning between concepts.</skos:scopeNote>
</rdf:Description>

<rdf:Description rdf:about="http://www.w3.org/2004/02/skos/core#topConceptOf">
	<rdf:type rdf:resource="http://www.w3.org/2002/07/owl#ObjectProperty"/>
	<rdfs:subPropertyOf rdf:resource="http://www.w3.org/2004/02/skos/core#inScheme"/>
	<rdfs:domain rdf:resource="http://www.w3.org/2004/02/skos/core#Concept"/>
	<rdfs:range rdf:resource="http://www.w3.org/2004/02/skos/core#ConceptScheme"/>
	<rdfs:isDefinedBy rdf:resource="http://www.w3.org/2004/02/skos/core"/>
	<rdfs:label xml:lang="en">is top concept in scheme</rdfs:label>
	<skos:definition xml:lang="en">Relates a concept to the concept scheme that it is a top level concept of.</skos:definition>
</rdf:Description>

<rdf:Description rdf:about="http://iflastandards.info/ns/lrm/lrmoo/R33_has_string">
	<rdf:type rdf:resource="http://www.w3.org/2002/07/owl#DatatypeProperty"/>
	<rdfs:subPropertyOf rdf:resource="http://www.cidoc-crm.org/cidoc-crm/P3_has_note"/>
	<rdfs:domain rdf:resource="http://iflastandards.info/ns/lrm/lrmoo/F12_Nomen"/>
	<rdfs:comment xml:lang="en">Quantification: many to one, necessary (1,1:0,n)

Scope note:
This property associates an instance of F12 Nomen with a sign or arrangement of signs that is used to refer to something through that instance of F12 Nomen.

Examples:
- The English word ‘poison’ as a term for toxic substances, in written form in the Latin alphabet (F12) has string the letters p, o, i, s, o, n with no intervening spaces (E62).
- The English word ‘poison’ as a term for toxic substances, notated in the International Phonetic Alphabet (F12) has string the string of characters ['pɔɪz(ə)n] (E62).
- The French word ‘poison’ as a term for toxic substances, in written form in the Latin alphabet (F12) has string the letters p, o, i, s, o, n with no intervening spaces (E62).
- The French word ‘poison’ as a term for toxic substances, notated in the International Phonetic Alphabet (F12) has string the string of characters [pwa'zɔ̃] (E62).
</rdfs:comment>
	<rdfs:label xml:lang="en">R33 has string</rdfs:label>
	<skos:notation>R33</skos:notation>
	<skos:prefLabel xml:lang="en">has string</skos:prefLabel>
</rdf:Description>

<rdf:Description rdf:about="http://www.cidoc-crm.org/cidoc-crm/P168_place_is_defined_by">
	<rdf:type rdf:resource="http://www.w3.org/2002/07/owl#DatatypeProperty"/>
	<rdfs:domain rdf:resource="http://www.cidoc-crm.org/cidoc-crm/E53_Place"/>
	<rdfs:range rdf:resource="http://www.w3.org/2000/01/rdf-schema#Literal"/>
	<rdfs:comment xml:lang="en">This property associates an instance of E53 Place with an instance of E94 Space Primitive that defines it. Syntactic variants or use of different scripts may result in multiple instances of E94 Space Primitive defining exactly the same place. Transformations between different reference systems always result in new definitions of places approximating each other and not in alternative definitions.</rdfs:comment>
	<rdfs:label xml:lang="fr">lieu défini par</rdfs:label>
	<rdfs:label xml:lang="en">place is defined by</rdfs:label>
</rdf:Description>

<rdf:Description rdf:about="http://www.cidoc-crm.org/cidoc-crm/P169i_spacetime_volume_is_defined_by">
	<rdf:type rdf:resource="http://www.w3.org/2002/07/owl#DatatypeProperty"/>
	<rdfs:domain rdf:resource="http://www.cidoc-crm.org/cidoc-crm/E92_Spacetime_Volume"/>
	<rdfs:range rdf:resource="http://www.w3.org/2000/01/rdf-schema#Literal"/>
	<rdfs:comment xml:lang="en">Scope note for 'P169': This property associates an instance of E95 Spacetime Primitive with the instance of E92 Spacetime Volume it defines.</rdfs:comment>
	<rdfs:label xml:lang="en">spacetime volume is defined by</rdfs:label>
	<rdfs:label xml:lang="fr">volume spatio-temporel défini par</rdfs:label>
</rdf:Description>

<rdf:Description rdf:about="http://www.cidoc-crm.org/cidoc-crm/P170i_time_is_defined_by">
	<rdf:type rdf:resource="http://www.w3.org/2002/07/owl#DatatypeProperty"/>
	<rdfs:domain rdf:resource="http://www.cidoc-crm.org/cidoc-crm/E52_Time-Span"/>
	<rdfs:range rdf:resource="http://www.w3.org/2000/01/rdf-schema#Literal"/>
	<rdfs:comment xml:lang="en">Scope note for 'P170': This property associates an instance of E61 Time Primitive with the instance of E52 Time-Span that constitutes the interpretation of the terms of the time primitive as an extent in absolute, real time.
The quantification allows several instances of E61 Time Primitive that are each expressed in different syntactic forms, to define the same instance of E52 Time-Span.</rdfs:comment>
	<rdfs:label xml:lang="fr">temps défini par</rdfs:label>
	<rdfs:label xml:lang="en">time is defined by</rdfs:label>
</rdf:Description>

<rdf:Description rdf:about="http://www.cidoc-crm.org/cidoc-crm/P171_at_some_place_within">
	<rdf:type rdf:resource="http://www.w3.org/2002/07/owl#DatatypeProperty"/>
	<rdfs:domain rdf:resource="http://www.cidoc-crm.org/cidoc-crm/E53_Place"/>
	<rdfs:range rdf:resource="http://www.w3.org/2000/01/rdf-schema#Literal"/>
	<rdfs:comment xml:lang="en">This property describes the maximum spatial extent within which an instance of E53 Place falls. Since instances of E53 Places may not have precisely known spatial extents, the CIDOC CRM supports statements about maximum spatial extents of instances of E53 Place. This property allows an instance of E53 Place’s maximum spatial extent (i.e., its outer boundary) to be assigned an instance of E94 Space Primitive value.
This property is a shortcut of the fully developed path from E53 Place, P89 falls within, E53 Place, P168 place is defined by to E94 Space Primitive through a declarative Place that is not explicitly documented, to a Space Primitive: declarative places are defined in CRMgeo (Doerr and Hiebel 2013).</rdfs:comment>
	<rdfs:label xml:lang="en">at some place within</rdfs:label>
	<rdfs:label xml:lang="fr">quelque part dans</rdfs:label>
</rdf:Description>

<rdf:Description rdf:about="http://www.cidoc-crm.org/cidoc-crm/P172_contains">
	<rdf:type rdf:resource="http://www.w3.org/2002/07/owl#DatatypeProperty"/>
	<rdfs:domain rdf:resource="http://www.cidoc-crm.org/cidoc-crm/E53_Place"/>
	<rdfs:range rdf:resource="http://www.w3.org/2000/01/rdf-schema#Literal"/>
	<rdfs:comment xml:lang="en">This property describes a minimum spatial extent which is contained within an instance of E53 Place. Since instances of E53 Place may not have precisely known spatial extents, the CIDOC CRM supports statements about minimum spatial extents of instances of E53 Place. This property allows an instance of E53 Place’s minimum spatial extent (i.e., its inner boundary or a point being within a Place) to be assigned an instance of E94 Space Primitive value.
This property is a shortcut of the fully developed path from E53 Place, P89i contains, E53 Place, P168 place is defined by to E94 Space Primitive.</rdfs:comment>
	<rdfs:label xml:lang="en">contains</rdfs:label>
	<rdfs:label xml:lang="fr">contient</rdfs:label>
</rdf:Description>

<rdf:Description rdf:about="http://www.cidoc-crm.org/cidoc-crm/P190_has_symbolic_content">
	<rdf:type rdf:resource="http://www.w3.org/2002/07/owl#DatatypeProperty"/>
	<rdfs:subPropertyOf rdf:resource="http://www.cidoc-crm.org/cidoc-crm/P3_has_note"/>
	<rdfs:domain rdf:resource="http://www.cidoc-crm.org/cidoc-crm/E90_Symbolic_Object"/>
	<rdfs:range rdf:resource="http://www.w3.org/2000/01/rdf-schema#Literal"/>
	<rdfs:comment xml:lang="en">This property associates an instance of E90 Symbolic Object with a complete, identifying representation of its content in the form of an instance of E62 String.
This property only applies to instances of E90 Symbolic Object that can be represented completely in this form. The representation may be more specific than the symbolic level defining the identity condition of the represented. This depends on the type of the symbolic object represented. For instance, if a name has type “Modern Greek character sequence”, it may be represented in a loss-free Latin transcription, meaning however the sequence of Greek letters.
As another example, if the represented object has type “English words sequence”, American English or British English spelling variants may be chosen to represent the English word “colour” without defining a different symbolic object. If a name has type “European traditional name”, no particular string may define its content.</rdfs:comment>
	<rdfs:label xml:lang="fr">a pour contenu symbolique</rdfs:label>
	<rdfs:label xml:lang="en">has symbolic content</rdfs:label>
</rdf:Description>

<rdf:Description rdf:about="http://www.cidoc-crm.org/cidoc-crm/P3_has_note">
	<rdf:type rdf:resource="http://www.w3.org/2002/07/owl#DatatypeProperty"/>
	<rdfs:domain rdf:resource="http://www.cidoc-crm.org/cidoc-crm/E1_CRM_Entity"/>
	<rdfs:range rdf:resource="http://www.w3.org/2000/01/rdf-schema#Literal"/>
	<rdfs:comment xml:lang="en">This property is a container for all informal descriptions about an object that have not been expressed in terms of CIDOC CRM constructs.
In particular, it captures the characterisation of the item itself, its internal structures, appearance, etc.
Like property P2 has type (is type of), this property is a consequence of the restricted focus of the CIDOC CRM. The aim is not to capture, in a structured form, everything that can be said about an item; indeed, the CIDOC CRM formalism is not regarded as sufficient to express everything that can be said. Good practice requires use of distinct note fields for different aspects of a characterisation. The P3.1 has type property of P3 has note allows differentiation of specific notes, e.g. “construction”, “decoration”, etc.
An item may have many notes, but a note is attached to a specific item.</rdfs:comment>
	<rdfs:label xml:lang="fr">a pour note</rdfs:label>
	<rdfs:label xml:lang="en">has note</rdfs:label>
	<rdfs:label xml:lang="de">hat Anmerkung</rdfs:label>
	<rdfs:label xml:lang="pt">tem nota</rdfs:label>
	<rdfs:label xml:lang="el">έχει επεξήγηση</rdfs:label>
	<rdfs:label xml:lang="ru">имеет примечание</rdfs:label>
	<rdfs:label xml:lang="zh">有注释</rdfs:label>
</rdf:Description>

<rdf:Description rdf:about="http://www.cidoc-crm.org/cidoc-crm/P57_has_number_of_parts">
	<rdf:type rdf:resource="http://www.w3.org/2002/07/owl#DatatypeProperty"/>
	<rdfs:domain rdf:resource="http://www.cidoc-crm.org/cidoc-crm/E19_Physical_Object"/>
	<rdfs:range rdf:resource="http://www.w3.org/2000/01/rdf-schema#Literal"/>
	<rdfs:comment xml:lang="en">This property documents the number of parts, an instance of E60 Number, of which an instance of E19 Physical Object is composed.
This may be used as a method of checking inventory counts with regard to aggregate or collective objects. What constitutes a part or component depends on the context and requirements of the documentation. Normally, the parts documented in this way would not be considered as worthy of individual attention.
For a more complete description, objects may be decomposed into their components and constituents using P46 is composed of (forms parts of) and P45 consists of (is incorporated in). This allows each element to be described individually.</rdfs:comment>
	<rdfs:label xml:lang="fr">a pour nombre d’éléments</rdfs:label>
	<rdfs:label xml:lang="en">has number of parts</rdfs:label>
	<rdfs:label xml:lang="de">hat Anzahl Teile</rdfs:label>
	<rdfs:label xml:lang="pt">tem número de partes</rdfs:label>
	<rdfs:label xml:lang="el">έχει αριθμό μερών</rdfs:label>
	<rdfs:label xml:lang="ru">имеет число частей</rdfs:label>
	<rdfs:label xml:lang="zh">有组成部分数</rdfs:label>
</rdf:Description>

<rdf:Description rdf:about="http://www.cidoc-crm.org/cidoc-crm/P79_beginning_is_qualified_by">
	<rdf:type rdf:resource="http://www.w3.org/2002/07/owl#DatatypeProperty"/>
	<rdfs:subPropertyOf rdf:resource="http://www.cidoc-crm.org/cidoc-crm/P3_has_note"/>
	<rdfs:domain rdf:resource="http://www.cidoc-crm.org/cidoc-crm/E52_Time-Span"/>
	<rdfs:range rdf:resource="http://www.w3.org/2000/01/rdf-schema#Literal"/>
	<rdfs:comment xml:lang="en">This property associates an instance of E52 Time-Span with a note detailing the scholarly or scientific opinions and justifications about the certainty, precision, sources etc. of its beginning. Such notes may also be used to elaborate arguments about constraints or to give explanations of alternatives.</rdfs:comment>
	<rdfs:label xml:lang="fr">a son début qualifié par</rdfs:label>
	<rdfs:label xml:lang="en">beginning is qualified by</rdfs:label>
	<rdfs:label xml:lang="de">hat Anfangsbegründung</rdfs:label>
	<rdfs:label xml:lang="pt">início é qualificado por</rdfs:label>
	<rdfs:label xml:lang="el">αρχή προσδιορίζεται από</rdfs:label>
	<rdfs:label xml:lang="ru">начало ограничено</rdfs:label>
	<rdfs:label xml:lang="zh">起始限定</rdfs:label>
</rdf:Description>

<rdf:Description rdf:about="http://www.cidoc-crm.org/cidoc-crm/P80_end_is_qualified_by">
	<rdf:type rdf:resource="http://www.w3.org/2002/07/owl#DatatypeProperty"/>
	<rdfs:subPropertyOf rdf:resource="http://www.cidoc-crm.org/cidoc-crm/P3_has_note"/>
	<rdfs:domain rdf:resource="http://www.cidoc-crm.org/cidoc-crm/E52_Time-Span"/>
	<rdfs:range rdf:resource="http://www.w3.org/2000/01/rdf-schema#Literal"/>
	<rdfs:comment xml:lang="en">This property associates an instance of E52 Time-Span with a note detailing the scholarly or scientific opinions and justifications about the end of this time-span concerning certainty, precision, sources etc. This property may also be used to describe arguments constraining possible dates and to distinguish reasons for alternative dates.</rdfs:comment>
	<rdfs:label xml:lang="fr">a sa fin qualifiée par</rdfs:label>
	<rdfs:label xml:lang="en">end is qualified by</rdfs:label>
	<rdfs:label xml:lang="pt">final é qualificado por</rdfs:label>
	<rdfs:label xml:lang="de">hat Begründung des Endes</rdfs:label>
	<rdfs:label xml:lang="el">τέλος προσδιορίζεται από</rdfs:label>
	<rdfs:label xml:lang="ru">конец ограничен</rdfs:label>
	<rdfs:label xml:lang="zh">结束限定</rdfs:label>
</rdf:Description>

<rdf:Description rdf:about="http://www.cidoc-crm.org/cidoc-crm/P81_ongoing_throughout">
	<rdf:type rdf:resource="http://www.w3.org/2002/07/owl#DatatypeProperty"/>
	<rdfs:domain rdf:resource="http://www.cidoc-crm.org/cidoc-crm/E52_Time-Span"/>
	<rdfs:range rdf:resource="http://www.w3.org/2000/01/rdf-schema#Literal"/>
	<rdfs:comment xml:lang="en">This property associates an instance of E52 Time-Span with an instance of E61 Time Primitive specifying a minimum period of time covered by it. Since Time-Spans may not have precisely known temporal extents, the CIDOC CRM supports statements about the minimum and maximum temporal extents of Time-Spans. This property allows a Time-Span’s minimum temporal extent (i.e., its inner boundary) to be assigned an E61 Time Primitive value. Time Primitives are treated by the CIDOC CRM as application or system specific date intervals, and are not further analysed. If different sources of evidence justify different minimum extents without contradicting each other, the smallest interval including all these extents will be the best estimate. This should be taken into account for information integration.</rdfs:comment>
	<rdfs:label xml:lang="fr">a couvert</rdfs:label>
	<rdfs:label xml:lang="pt">abrange no mínimo</rdfs:label>
	<rdfs:label xml:lang="de">andauernd während</rdfs:label>
	<rdfs:label xml:lang="en">ongoing throughout</rdfs:label>
	<rdfs:label xml:lang="el">καθόλη τη διάρκεια του/της</rdfs:label>
	<rdfs:label xml:lang="ru">длится в течение</rdfs:label>
	<rdfs:label xml:lang="zh">最短范围是</rdfs:label>
</rdf:Description>

<rdf:Description rdf:about="http://www.cidoc-crm.org/cidoc-crm/P81a_end_of_the_begin">
	<rdf:type rdf:resource="http://www.w3.org/2002/07/owl#DatatypeProperty"/>
	<rdfs:subPropertyOf rdf:resource="http://www.cidoc-crm.org/cidoc-crm/P81_ongoing_throughout"/>
	<rdfs:domain rdf:resource="http://www.cidoc-crm.org/cidoc-crm/E52_Time-Span"/>
	<rdfs:range rdf:resource="http://www.w3.org/2000/01/rdf-schema#Literal"/>
	<rdfs:label xml:lang="de">Ende des Anfangs</rdfs:label>
	<rdfs:label xml:lang="en">end of the begin</rdfs:label>
	<rdfs:label xml:lang="pt">fim do início</rdfs:label>
	<rdfs:label xml:lang="fr">fin du début</rdfs:label>
	<rdfs:label xml:lang="el">τέλος της αρχής</rdfs:label>
	<rdfs:label xml:lang="ru">конец начала</rdfs:label>
</rdf:Description>

<rdf:Description rdf:about="http://www.cidoc-crm.org/cidoc-crm/P81b_begin_of_the_end">
	<rdf:type rdf:resource="http://www.w3.org/2002/07/owl#DatatypeProperty"/>
	<rdfs:subPropertyOf rdf:resource="http://www.cidoc-crm.org/cidoc-crm/P81_ongoing_throughout"/>
	<rdfs:domain rdf:resource="http://www.cidoc-crm.org/cidoc-crm/E52_Time-Span"/>
	<rdfs:range rdf:resource="http://www.w3.org/2000/01/rdf-schema#Literal"/>
	<rdfs:label xml:lang="de">Anfang vom Ende</rdfs:label>
	<rdfs:label xml:lang="en">begin of the end</rdfs:label>
	<rdfs:label xml:lang="pt">começar do fim</rdfs:label>
	<rdfs:label xml:lang="fr">début de la fin</rdfs:label>
	<rdfs:label xml:lang="el">αρχή του τέλους</rdfs:label>
	<rdfs:label xml:lang="ru">начать в конце</rdfs:label>
</rdf:Description>

<rdf:Description rdf:about="http://www.cidoc-crm.org/cidoc-crm/P82_at_some_time_within">
	<rdf:type rdf:resource="http://www.w3.org/2002/07/owl#DatatypeProperty"/>
	<rdfs:domain rdf:resource="http://www.cidoc-crm.org/cidoc-crm/E52_Time-Span"/>
	<rdfs:range rdf:resource="http://www.w3.org/2000/01/rdf-schema#Literal"/>
	<rdfs:comment xml:lang="en">This property describes the maximum period of time within which an E52 Time-Span falls. Since Time-Spans may not have precisely known temporal extents, the CIDOC CRM supports statements about the minimum and maximum temporal extents of Time-Spans. This property allows a Time-Span’s maximum temporal extent (i.e. its outer boundary) to be assigned an E61 Time Primitive value. Time Primitives are treated by the CIDOC CRM as application or system specific date intervals, and are not further analysed. If different sources of evidence justify different maximum extents without contradicting each other, the resulting intersection of all these extents will be the best estimate. This should be taken into account for information integration.</rdfs:comment>
	<rdfs:label xml:lang="fr">a eu lieu durant</rdfs:label>
	<rdfs:label xml:lang="pt">abrange no máximo</rdfs:label>
	<rdfs:label xml:lang="en">at some time within</rdfs:label>
	<rdfs:label xml:lang="de">irgendwann innerhalb von</rdfs:label>
	<rdfs:label xml:lang="el">κάποτε εντός</rdfs:label>
	<rdfs:label xml:lang="ru">некоторое время в течение</rdfs:label>
	<rdfs:label xml:lang="zh">最长范围是</rdfs:label>
</rdf:Description>

<rdf:Description rdf:about="http://www.cidoc-crm.org/cidoc-crm/P82a_begin_of_the_begin">
	<rdf:type rdf:resource="http://www.w3.org/2002/07/owl#DatatypeProperty"/>
	<rdfs:subPropertyOf rdf:resource="http://www.cidoc-crm.org/cidoc-crm/P82_at_some_time_within"/>
	<rdfs:domain rdf:resource="http://www.cidoc-crm.org/cidoc-crm/E52_Time-Span"/>
	<rdfs:range rdf:resource="http://www.w3.org/2000/01/rdf-schema#Literal"/>
	<rdfs:label xml:lang="de">Anfang des Anfangs</rdfs:label>
	<rdfs:label xml:lang="en">begin of the begin</rdfs:label>
	<rdfs:label xml:lang="pt">começar do início</rdfs:label>
	<rdfs:label xml:lang="fr">début du début</rdfs:label>
	<rdfs:label xml:lang="el">αρχή της αρχής</rdfs:label>
	<rdfs:label xml:lang="ru">начать с начала</rdfs:label>
</rdf:Description>

<rdf:Description rdf:about="http://www.cidoc-crm.org/cidoc-crm/P82b_end_of_the_end">
	<rdf:type rdf:resource="http://www.w3.org/2002/07/owl#DatatypeProperty"/>
	<rdfs:subPropertyOf rdf:resource="http://www.cidoc-crm.org/cidoc-crm/P82_at_some_time_within"/>
	<rdfs:domain rdf:resource="http://www.cidoc-crm.org/cidoc-crm/E52_Time-Span"/>
	<rdfs:range rdf:resource="http://www.w3.org/2000/01/rdf-schema#Literal"/>
	<rdfs:label xml:lang="de">Ende vom Ende</rdfs:label>
	<rdfs:label xml:lang="en">end of the end</rdfs:label>
	<rdfs:label xml:lang="pt">fim do fim</rdfs:label>
	<rdfs:label xml:lang="fr">fin de la fin</rdfs:label>
	<rdfs:label xml:lang="el">τέλος του τέλους</rdfs:label>
	<rdfs:label xml:lang="ru">конец конец</rdfs:label>
</rdf:Description>

<rdf:Description rdf:about="http://www.cidoc-crm.org/cidoc-crm/P90_has_value">
	<rdf:type rdf:resource="http://www.w3.org/2002/07/owl#DatatypeProperty"/>
	<rdfs:domain rdf:resource="http://www.cidoc-crm.org/cidoc-crm/E54_Dimension"/>
	<rdfs:range rdf:resource="http://www.w3.org/2000/01/rdf-schema#Literal"/>
	<rdfs:comment xml:lang="en">This property allows an instance of E54 Dimension to be approximated by an instance of E60 Number primitive.</rdfs:comment>
	<rdfs:label xml:lang="fr">a pour valeur</rdfs:label>
	<rdfs:label xml:lang="en">has value</rdfs:label>
	<rdfs:label xml:lang="de">hat Wert</rdfs:label>
	<rdfs:label xml:lang="pt">tem valor</rdfs:label>
	<rdfs:label xml:lang="el">έχει τιμή</rdfs:label>
	<rdfs:label xml:lang="ru">имеет значение</rdfs:label>
	<rdfs:label xml:lang="zh">有数值</rdfs:label>
</rdf:Description>

<rdf:Description rdf:about="http://www.cidoc-crm.org/cidoc-crm/P90a_has_lower_value_limit">
	<rdf:type rdf:resource="http://www.w3.org/2002/07/owl#DatatypeProperty"/>
	<rdfs:subPropertyOf rdf:resource="http://www.cidoc-crm.org/cidoc-crm/P90_has_value"/>
	<rdfs:domain rdf:resource="http://www.cidoc-crm.org/cidoc-crm/E54_Dimension"/>
	<rdfs:range rdf:resource="http://www.w3.org/2000/01/rdf-schema#Literal"/>
	<rdfs:label xml:lang="en">has lower value limit</rdfs:label>
</rdf:Description>

<rdf:Description rdf:about="http://www.cidoc-crm.org/cidoc-crm/P90b_has_upper_value_limit">
	<rdf:type rdf:resource="http://www.w3.org/2002/07/owl#DatatypeProperty"/>
	<rdfs:subPropertyOf rdf:resource="http://www.cidoc-crm.org/cidoc-crm/P90_has_value"/>
	<rdfs:domain rdf:resource="http://www.cidoc-crm.org/cidoc-crm/E54_Dimension"/>
	<rdfs:range rdf:resource="http://www.w3.org/2000/01/rdf-schema#Literal"/>
	<rdfs:label xml:lang="en">has upper value limit</rdfs:label>
</rdf:Description>

<rdf:Description rdf:about="http://academictourism.com/academictourism#Character_Type">
	<rdf:type rdf:resource="http://www.w3.org/2002/07/owl#Class"/>
	<rdfs:subClassOf rdf:resource="http://www.cidoc-crm.org/cidoc-crm/E55_Type"/>
</rdf:Description>

<rdf:Description rdf:about="http://academictourism.com/academictourism#Course_Subject">
	<rdf:type rdf:resource="http://www.w3.org/2002/07/owl#Class"/>
	<rdfs:subClassOf rdf:resource="http://www.cidoc-crm.org/cidoc-crm/E55_Type"/>
</rdf:Description>

<rdf:Description rdf:about="http://academictourism.com/academictourism#Mode_of_Transportation">
	<rdf:type rdf:resource="http://www.w3.org/2002/07/owl#Class"/>
	<rdfs:subClassOf rdf:resource="http://www.cidoc-crm.org/cidoc-crm/E55_Type"/>
</rdf:Description>

<rdf:Description rdf:about="http://academictourism.com/academictourism#locative_relation">
	<rdf:type rdf:resource="http://www.w3.org/2002/07/owl#Class"/>
	<rdfs:subClassOf rdf:resource="http://www.loa-cnr.it/ontologies/DnS#gestalt"/>
	<rdfs:subClassOf rdf:resource="http://www.loa-cnr.it/ontologies/DnS#relation"/>
</rdf:Description>

<rdf:Description rdf:about="http://iflastandards.info/ns/lrm/lrmoo/F11_Corporate_Body">
	<rdf:type rdf:resource="http://www.w3.org/2002/07/owl#Class"/>
	<rdfs:subClassOf rdf:resource="http://iflastandards.info/ns/lrm/lrmoo/F55_Collective_Agent"/>
	<rdfs:comment xml:lang="en">Scope note:
This class comprises organisations and groups of two or more people and/or organisations acting as a unit.
To be considered an instance of F11 Corporate Body a gathering of people needs to bear a name and exhibit organisational characteristics sufficient to allow the body as a whole to participate in the creation, modification or production of an E73 Information Object. Groups such as conferences, congresses, expeditions, exhibitions, festivals, fairs, etc. are modelled as F11 Corporate Bodies when they are named and can take collective action, such as approving a report or publishing their proceedings.

Examples:
- The International Machaut Society
- The British Library
- The Jackson Five [pop band]
- Municipalité régionale de comté de Portneuf [regional municipality in Quebec]
- Symposium on Glaucoma
</rdfs:comment>
	<rdfs:label xml:lang="en">F11 Corporate Body</rdfs:label>
	<skos:notation>F11</skos:notation>
	<skos:prefLabel xml:lang="en">Corporate Body</skos:prefLabel>
</rdf:Description>

<rdf:Description rdf:about="http://iflastandards.info/ns/lrm/lrmoo/F12_Nomen">
	<rdf:type rdf:resource="http://www.w3.org/2002/07/owl#Class"/>
	<rdfs:subClassOf rdf:resource="http://www.cidoc-crm.org/cidoc-crm/E89_Propositional_Object"/>
	<rdfs:comment xml:lang="en">Scope note:
This class comprises associations between an instance of any class, and signs or arrangements of signs that are used to refer to and identify that instance.
Signs include alphanumeric characters, ideograms, notations such as chemical structure symbols, sound symbols, etc. The scripts or type sets for the symbols used to compose an instance of F12 Nomen have to be sufficiently specified. Spelling variants are regarded as different nomens, whereas the use of different fonts (visual representation variants) or different digital encodings do not change the identity.
An arbitrary combination of signs or symbols cannot be regarded as an appellation or designation until it is associated with something in some context. In that sense, the F12 Nomen class can be understood as the reification of a relationship between an instance of E1 CRM Entity and an instance of E41 Appellation. Two instances of F12 Nomen can happen to be associated with equivalent strings and yet remain distinct, as long as they refer to distinct instances of E1 CRM Entity. Furthermore, two instances of F12 Nomen referring to the same instance of E1 CRM Entity may be associated with equivalent strings, and remain distinct as long as they are associated with distinct properties of the F12 Nomen class (for example, having the same spelling in different languages, or being defined in different controlled vocabularies).
An instance of F12 Nomen associates a combination of signs with an instance of E1 CRM Entity on the basis of a cultural or linguistic convention: by associating a string with anything, the instance of F12 Nomen establishes a meaning that is not inherent in the instance of E62 String that is associated with it. Depending on context of use, nomens associated with equivalent strings can be associated with instances of different things in the real world even within the same language (polysemy and homonymy). Conversely, the same thing can be referred to through any number of nomens (synonymy). In the controlled environment of a bibliographic information system, though, homonymy is avoided.
Instances of F12 Nomen are assigned and associated with instances of E1 CRM Entity either formally (such as by bibliographic agencies) or informally through common usage. When they are assigned formally, the construction of the instances of E62 String that represent them may follow predetermined rules.

Examples:
- ‘杜甫’ as the name for a Chinese poet of the 8(th) century, rendered in simplified Chinese characters
- ‘Du Fu’ as the name for a Chinese poet of the 8(th) century, rendered in Pinyin romanised form
- ‘Tu Fu’ as the name for a Chinese poet of the 8(th) century, rendered in another romanised form
- ‘Thơ Ðô Phủ’ as the name for a Chinese poet of the 8(th) century, rendered in a Vietnamese form
- ‘جامعة صفاقس’ as the name for Sfax University (Tunisia), rendered in Arabic in Arabic script
- ‘Ğāmi‘at̀̀ Ṣafāqis’ as the name for Sfax University (Tunisia), rendered in transliterated Arabic
- ‘Université de Sfax’ as the name for Sfax University (Tunisia), rendered in French
- ‘3-[(2S)-1-methylpyrrolidin-2-yl]pyridine’ as the term for nicotine, rendered in the IUPAC nomenclature of organic chemistry
- ‘Murders in the rue Morgue’ as the title of the textual work by Edgar Allan Poe, in English
- ‘Poe, Edgar Allan, 1809-1849. Murders in the rue Morgue’ as the name of the textual work, formulated as a controlled author/title access point appropriate for an English language catalogue
- ‘modelling’ as the term for the activity, in English using British spelling
- ‘modeling’ as the term for the activity, in English using American spelling
- ‘Maxwell equations’ as the term for these equations, formulated as the preferred subject access point from LCSH, http://lccn.loc.gov/sh85082387, as of 27 March 2012 [date of last update]
- ‘Equations, Maxwell’ as the term for these equations, formulated as a variant subject access point, from the same source
- ‘Gontcharova, Nathalie (1881-1962)’ as the name of the Russian artist, formulated as an preferred access point from the authority file of the National Library of France, http://catalogue.bnf.fr/ark:/12148/cb119547494/PUBLIC, as of 11 March 2015 [date of last update]
- ‘Gončarova, Natalʹâ Sergeevna (1881-1962)’ as the name of the Russian artist, formulated as a variant access point for a personal name, transliterated using ISO 9:1995 ‘Information and documentation — Transliteration of Cyrillic characters into Latin characters — Slavic and non-Slavic languages’, also from the authority file of the National Library of France
- ‘Гончарова, Наталья Сергеевна (1881-1962)’ as the name of the Russian artist, formulated as a variant access point in Cyrillic script, also from the authority file of the National Library of France
- ‘595.7’ as a classification number for insects (the taxonomic class Insecta), in the 23rd edition of the Dewey Decimal Classification
- ‘Insecta’ as a term for insects (the taxonomic class Insecta), used as the caption for the class ‘595.7’ in the English language 23rd edition of the Dewey Decimal Classification
- ‘spa’ as a code to designate the language Spanish, drawn from set 2 (3-letter language identifiers) of ‘ISO 639 – Code for individual languages and language groups’ (ISO 639:2023)
</rdfs:comment>
	<rdfs:label xml:lang="en">F12 Nomen</rdfs:label>
	<skos:notation>F12</skos:notation>
	<skos:prefLabel xml:lang="en">Nomen</skos:prefLabel>
</rdf:Description>

<rdf:Description rdf:about="http://iflastandards.info/ns/lrm/lrmoo/F18_Serial_Work">
	<rdf:type rdf:resource="http://www.w3.org/2002/07/owl#Class"/>
	<rdfs:subClassOf rdf:resource="http://iflastandards.info/ns/lrm/lrmoo/F1_Work"/>
	<rdfs:comment xml:lang="en">Scope note:
This class comprises works that are, or have been, planned to result in sequences of Expressions or Manifestations with common features. Whereas a work can acquire new members during the time it evolves, Expressions and Manifestations are identified with a certain state achieved at a particular point in time. Therefore there is in general no single Expression or Manifestation representing a complete serial work, unless the serial work has ended.
Serial Works may or may not have a plan for an overall expression.
The retrospective reprinting of all issues of a Serial Work at once, in the form of a monograph, is regarded to be another member of the F1 Work, which contains the Serial Work and the Work realised in the monograph. This does not make the monograph part of the Serial Work.

Examples:
- the periodical entitled ‘The UNESCO Courier’, ISSN ‘0041-5278’
- the periodical entitled ‘Courrier de l’UNESCO’, ISSN ‘0304-3118’ [French edition of the periodical titled ‘The UNESCO Courier’, ISSN ‘0041-5278’]
- the series entitled ‘L’évolution de l’humanité’, ISSN ‘0755-1843’ [a monograph series comprising volumes that were published from 1920 on, and some of which were reprinted, with different physical features and rearranged in a different order, from 1968 on, in a distinct series also entitled ‘L’évolution de l’humanité’, ISSN ‘0755-1770’]
</rdfs:comment>
	<rdfs:label xml:lang="en">F18 Serial Work</rdfs:label>
	<skos:notation>F18</skos:notation>
	<skos:prefLabel xml:lang="en">Serial Work</skos:prefLabel>
</rdf:Description>

<rdf:Description rdf:about="http://iflastandards.info/ns/lrm/lrmoo/F1_Work">
	<rdf:type rdf:resource="http://www.w3.org/2002/07/owl#Class"/>
	<rdfs:subClassOf rdf:resource="http://www.cidoc-crm.org/cidoc-crm/E89_Propositional_Object"/>
	<rdfs:comment xml:lang="en">Scope note:
This class comprises distinct intellectual ideas conveyed in artistic and intellectual creations, such a poems, stories or musical compositions.
A Work is the outcome of an intellectual process of one or more persons. Inherent to the notion of work is the existence of recognisable realizations of the work in the form of one or more expressions. Works are often regarded as finished and discrete e.g. when declared as such by the creator of the work or based on the elaboration or logical coherence of its content. However, works may be recognized as existing but unfinished e.g. if the creators deliberately or accidentally never explicitly finished a particular Expression but have left behind partial expressions.
In the absence of explicit information about the initial conception, which is rarely available, the first expression created constitutes witness of the beginning of existence of a Work.
A Work can evolve over time, such as through revised editions. A Work may be elaborated by one or more Actors simultaneously, in parallel, or over time. Additional expressions of a Work can continue to be created over time.
The boundaries of a Work have nothing to do with the value of the intellectual achievement but only with the dominance of a concept.
The main purpose of this class is to enable bringing together intellectually equivalent Expressions in order to display to a user all available alternatives of the same intellectual or artistic content.

Examples:
- Agatha Christie’s ‘Murder on the Orient Express’ [novel]
- Mary Shelley’s ‘Frankenstein, or, The Modern Prometheus’ [novel]
- Ursula K. Le Guin’s ‘The Earthsea trilogy’ [set of novels]
- Ursula K. Le Guin’s ‘The Tombs of Atuan’ [novel which is part of ‘The Earthsea trilogy’]
- Homer’s ‘Odyssey’ [ancient Greek epic poem]
- Dante’s ‘Divina Commedia’ [narrative poem]
- William Shakespeare’s ‘The Tragedy of Hamlet, Prince of Denmark’ [play]
- Henry Gray’s ‘Anatomy of the human body’ [scholarly work / reference work]
- René Goscinny and Albert Uderzo’s ‘Astérix le Gaulois’ [cartoon]
- the ‘Dewey Decimal Classification’ (DDC) [library classification system]
- the Ordnance Survey’s 1:50 000 ‘Landranger series’ [collection of maps]
- Ludwig van Beethoven’s ‘Symphony No. 9 in D minor’ [symphony]
- Johann Sebastian Bach’s ‘Goldberg Variations’ [compositions for keyboard]
- Daniel Humair and Damien Varaillon’s ‘Hommage à John Coltrane’ [musical improvisation]
- John Lennon and Paul McCartney’s ‘I want to hold your hand’ [song]
- François Truffault’s ‘Jules et Jim’ [movie]
- Alfred Hitchcock’s ‘Psycho’ [movie]
- Auguste Rodin’s ‘Le penseur’ (‘The thinker’) [art]
- Pablo Picasso’s ‘Guernica’ [art]
- Katsushika Hokusai’s ‘神奈川沖浪裏’ (‘The Great Wave’) [art]
</rdfs:comment>
	<rdfs:label xml:lang="en">F1 Work</rdfs:label>
	<skos:notation>F1</skos:notation>
	<skos:prefLabel xml:lang="en">Work</skos:prefLabel>
</rdf:Description>

<rdf:Description rdf:about="http://iflastandards.info/ns/lrm/lrmoo/F27_Work_Creation">
	<rdf:type rdf:resource="http://www.w3.org/2002/07/owl#Class"/>
	<rdfs:subClassOf rdf:resource="http://www.cidoc-crm.org/cidoc-crm/E65_Creation"/>
	<rdfs:comment xml:lang="en">Scope note:
This class comprises activities by which instances of F1 Work come into existence. An instance of F27 Work Creation can serve to document the period a work was coming into existence and the circumstances of it, when these are known.
An instance of F27 Work Creation marks the initial creation of an instance of F1 Work through expressions or other externalisations that are sufficiently elaborated so that the characteristic conceptual identity of the work could be recognized as existing.
In many cases this will coincide with the first known complete externalisation of an expression of the work. In other cases, the initial creation of an instance of F1 Work may be inferred from multiple, or later, expressions or other forms of evidence. For instance, commissioning of a work may explicitly be agreed on after the presentation of an already complete and detailed elaboration of the work that was not made public. Performances may be prior to written expressions, as in the case of Shakespeare’s works.
The work, as an intellectual construction, may evolve from its initial creation onwards, until the last known expression of it.
An instance of E39 Actor with which a work is associated through the chain of properties F1 Work. R16i was created by: F27 Work Creation. P14 carried out by (performed): E39 Actor corresponds to the notion of the “creator” of the work.
In the situation where an expression of one instance of F1 Work serves as source material for the creation of the first expression of a new instance of F1 Work, the direct relationship between the works is indicated using the property R2 is derivative of (has derivative) between the two instances of F1 Work. The link to the specific source expression is indicated with the property P16 used specific object (was used for) using the path: F1 Work(1). R3 is realised in: F2 Expression(1). P16i was used for: F27 Work Creation. R16 created: F1 Work(2).

Examples:
- Agatha Christie creating ‘Murder on the Orient Express’
- Mary Shelley creating ‘Frankenstein, or, The Modern Prometheus’
- Dante creating the poem ‘Divina Commedia’
- William Shakespeare creating ‘The Tragedy of Hamlet, Prince of Denmark’
- René Goscinny and Albert Uderzo (collaboratively) creating ‘Astérix le Gaulois’
- Ludwig van Beethoven composing his Symphony No. 9
- Johann Sebastian Bach composing the ‘Goldberg Variations’
- the making of ‘Jules et Jim’, directed by François Truffault
- the making of ‘Psycho’, directed by Alfred Hitchcock
- Auguste Rodin creating ‘Le Penseur’ (‘The Thinker’)
- Picasso creating ‘Guernica’
- Pascal Bonnefois and Marie-Louise Ollier creating ‘Yvain ou Le chevalier au lion : concordance lemmatisée’ [a concordance for the novel ‘Le chevalier au lion’ by Chrétien de Troyes, based on the 1960 edition by Mario Roques]
</rdfs:comment>
	<rdfs:label xml:lang="en">F27 Work Creation</rdfs:label>
	<skos:notation>F27</skos:notation>
	<skos:prefLabel xml:lang="en">Work Creation</skos:prefLabel>
</rdf:Description>

<rdf:Description rdf:about="http://iflastandards.info/ns/lrm/lrmoo/F28_Expression_Creation">
	<rdf:type rdf:resource="http://www.w3.org/2002/07/owl#Class"/>
	<rdfs:subClassOf rdf:resource="http://www.cidoc-crm.org/cidoc-crm/E12_Production"/>
	<rdfs:subClassOf rdf:resource="http://www.cidoc-crm.org/cidoc-crm/E65_Creation"/>
	<rdfs:comment xml:lang="en">Scope note:
This class comprises activities that result in instances of F2 Expression coming into existence. An instance of F2 Expression is considered to be created when it is captured on a carrier other than the creator’s brain.
Although F2 Expression is an abstract entity, a conceptual object, the creation of an expression inevitably also affects the physical world: when you scribble the first draft of a poem on a sheet of paper, you produce an instance of F3 Manifestation and an instance of F5 Item. F28 Expression Creation is a subclass of E12 Production because the recording of the expression causes a physical modification of the E18 Physical Thing that serves as the carrier. The creation of an instance of F2 Expression coincides with the creation of the first instance of F3 Manifestation that R4 embodies (is embodied in) this instance of F2 Expression.
The P2 has type (is type of) property can be used to specify the type of the instance of F28 Expression Creation (i.e., activities such as translating, revising, or arranging music are types of creation process). The type of the process is distinct from the type of result even though the typology frequently used for instances of the resulting F2 Expressions may imply the category of the instance of the F28 Expression Creation.
An instance of F28 Expression Creation may use as source material one or more specific instances of F2 Expression. When the source expression is documented this is also expressed by the property R76 is derivative of (has derivative).

Examples:
- Agatha Christie writing the original manuscript for ‘Murder on the Orient Express’
- Elisabeth van Bebber creating the German translation of ‘Murder on the Orient Express’
- Angela Hewitt performing the ‘Goldberg Variations’ at St. Thomas Church (Leipzig Germany) in November 2020
- Angela Hewitt performing the ‘Goldberg Variations’ in Christuskirche (Berlin) on 14-17 December 2015 (for a CD production)
- Beethoven scripting the original score for the 9(th) symphony
- Jonathan Del Mar editing and creating the score for Beethoven’s 9(th) symphony (as published by Bärenreiter in 1997)
- the making of the original cut of Hitchcock’s movie ‘Psycho’
- the making of the censored version of Hitchcock’s movie ‘Psycho’ that was released in Britain
- Auguste Rodin making the first plaster version of ‘The Thinker’ sculpture
- the making of the large-scale version of ‘The Thinker’ by the ‘Fonderie Alexis Rudier in 1904
</rdfs:comment>
	<rdfs:label xml:lang="en">F28 Expression Creation</rdfs:label>
	<skos:notation>F28</skos:notation>
	<skos:prefLabel xml:lang="en">Expression Creation</skos:prefLabel>
</rdf:Description>

<rdf:Description rdf:about="http://iflastandards.info/ns/lrm/lrmoo/F2_Expression">
	<rdf:type rdf:resource="http://www.w3.org/2002/07/owl#Class"/>
	<rdfs:subClassOf rdf:resource="http://www.cidoc-crm.org/cidoc-crm/E73_Information_Object"/>
	<rdfs:comment xml:lang="en">Scope note:
This class comprises the intellectual or artistic realisations of Works in the form of identifiable immaterial objects, such as texts, poems, jokes, musical or choreographic notations, movement pattern, sound pattern, images, multimedia objects, or any combination of such forms. The substance of F2 Expression is signs.
An Expression is the outcome of the intellectual or creative process of realizing a Work. Subsequent expressions conveying the same work may be created over time.
Expressions do not depend on a specific physical carrier and can exist on one or more carriers simultaneously. As far as bibliographic practice is concerned, only instances of F2 Expression that are externalised on physical carriers other than both the creator’s brain and an auditor’s brain are taken into account.
The form of F2 Expression is an inherent characteristic of the F2 Expression. Differences in form imply different Expressions (e.g., from text to spoken word, a transcript of a recording). Similarly, differences in language or means of performance imply different Expressions (e.g., translations or arrangements for different instruments). Thus, if a text is revised or modified, the result is considered to be a new F2 Expression. While theoretically any change in signs will result in a new Expression, conventionally the context and use will determine the rules for distinguishing among expressions.
An instance of F2 Expression which includes spoken or written text may be multiply instantiated as an instance of E33 Linguistic Object. This allows for the association of the E56 Language of the text with the instance of F2 Expression by using the property P72 has language (is language of).

Examples:
- the original text (in English) by Agatha Christie for her novel ‘Murder on the Orient Express’
- the German text of ‘Murder on the Orient Express’ (as translated by Elisabeth van Bebber and published with the title ‘Mord im Orientexpress’)
- the text of the abridged English version of ‘Murder on the Orient Express’ (as published by HarperCollins)
- the narrated English text of ‘Murder on the Orient Express’ by David Suchet
- the English text of Homer’s ‘Odyssey’ translated by Robert Fagles
- the English text of Homer’s ‘Odyssey’ translated by Richmond Lattimore
- ‘Dewey Decimal Classification’, 23rd edition (DDC23) [English edition]
- ‘Classification décimale de Dewey’, 23e édition [French translation of DDC23]
- the performance of Bach’s ‘Goldberg Variations’ by Angela Hewitt at St. Thomas Church (Leipzig Germany) in November 2020
- the performance of Bach’s ‘Goldberg Variations’ by Angela Hewitt in Christuskirche (Berlin) on 14-17 December 2015
- the musical score for Bach’s ‘Goldberg Variations’ (as published by Balthasar Schmid in 1741)
- Beethoven’s original score for Symphony No. 9 (as expressed by Beethoven’s original hand-written manuscript held by the Berlin State Library)
- the score for Beethoven’s Symphony No. 9 that was edited by Jonathan Del Mar and published by Bärenreiter in 1997
- the original cut of Hitchcock’s movie ‘Psycho’
- the censored version of Hitchcock’s movie ‘Psycho’ that was released in Britain (with stabbing sounds and visible nude shots removed)
- the first plaster version of ‘The Thinker’ sculpture made by Auguste Rodin around 1881
- large scale version of Auguste Rodin’s ‘The Thinker’ created at the Fonderie Alexis Rudier in 1904
</rdfs:comment>
	<rdfs:label xml:lang="en">F2 Expression</rdfs:label>
	<skos:notation>F2</skos:notation>
	<skos:prefLabel xml:lang="en">Expression</skos:prefLabel>
</rdf:Description>

<rdf:Description rdf:about="http://iflastandards.info/ns/lrm/lrmoo/F30_Manifestation_Creation">
	<rdf:type rdf:resource="http://www.w3.org/2002/07/owl#Class"/>
	<rdfs:subClassOf rdf:resource="http://www.cidoc-crm.org/cidoc-crm/E12_Production"/>
	<rdfs:subClassOf rdf:resource="http://www.cidoc-crm.org/cidoc-crm/E65_Creation"/>
	<rdfs:comment xml:lang="en">Scope note:
This class comprises the activities of selecting, arranging and presenting one or more instances of F2 Expression on a carrier or other persistent presentation means with the purpose of communicating it to some public. It includes the specification of the presentation as to sensory impression (such as visual appearance or audio rendition).

Examples:
- the process of creating the publication ‘Murder on the Orient Express / Agatha Christie’, published by HarperCollins in 2017, including deciding the format, typesetting the text, designing the cover and other features of the publication
- the process of making the HTML-version of the English text of Homer’s ‘Odyssey’ (translated by S. H. Butcher and A. Lang), which is available online from the Gutenberg Project
- the process of making the engraved copper plates for the first edition of Bach’s ‘Goldberg Variations’ by Balthasar Schmid
- the process of making the CD publication ‘Bach Goldberg Variations’, published by Hyperion Records in 2016, including the process of recording the performance, editing, and typesetting the booklet, and design of the overall publication
</rdfs:comment>
	<rdfs:label xml:lang="en">F30 Manifestation Creation</rdfs:label>
	<skos:notation>F30</skos:notation>
	<skos:prefLabel xml:lang="en">Manifestation Creation</skos:prefLabel>
</rdf:Description>

<rdf:Description rdf:about="http://iflastandards.info/ns/lrm/lrmoo/F31_Performance">
	<rdf:type rdf:resource="http://www.w3.org/2002/07/owl#Class"/>
	<rdfs:subClassOf rdf:resource="http://www.cidoc-crm.org/cidoc-crm/E7_Activity"/>
	<rdfs:comment xml:lang="en">Scope note:
This class comprises activities where an instance of F1 Work is presented or communicated directly or indirectly to an audience, such as a theatrical play, a musical work or a choreographic work.
Performances can be identified at various levels of granularity, but an instance of F31 Performance is always associated with a single identified instance of F1 Work. An instance of F31 Performance may consist of other instances of F31 Performance as parts, such as a piano concerto that has multiple movements. In addition, a complete run of equivalent performances of the same work can also be seen as an instance of F31 Performance, with the individual performances as parts.
Activities that include performing multiple individual works, e.g., that are put together as a program for a show or concert, but where the activity as a whole is not associated with an instance of F1 Work, should be represented as instances of E7 Activity consisting of individual instances of F31 Performances as parts (the property P9 consists of (forms part of) expresses the relationship).
Instances of F31 Performance may be created according to specific staging directions, be based on specific known instances of F2 Expression (such as translations), or be influenced by or include elements that relate to different works other than the single work the performance is dominated by. This can be documented using the properties P16 used specific object (was used for) or P15 was influenced by (influenced).

Examples:
- the performance of a Yiddish translation of the textual work entitled ‘King Lear’, as directed by Sergei Radlov, in Moscow, at the Moscow State Jewish Theatre, on February 10, 1935
- the performance of the ballet entitled ‘Rite of spring’, as choreographed by Pina Bausch, in Avignon, at the Popes’ Palace, on July 7, 1995
- the performance of the operatic work entitled ‘Dido and Aeneas’, as directed by Edward Gordon Craig and conducted by Martin Shaw, in London, Hampstead Conservatoire, on May 17, 18, and 19, 1900
- the performance of Verdi’s ‘La Traviata’ at the Salzburg Festival in 2005, that was staged by Willy Decker, directed by Brian Large and featuring Anna Netrebko and Rolando Villazón
- the performance of Michel Fokine’s choreography and libretto (choreographic work) for Stravinsky’s ‘The Firebird’ by the Mariinsky Orchestra and Ballet at the Mariinsky Theatre in Saint Petersburg, June 2008
- the performance of Daniel Humair and Damien Varaillon’s improvisation ‘Hommage à John Coltrane’ in the Bal Blomet (Paris), on 18 January 2018
</rdfs:comment>
	<rdfs:label xml:lang="en">F31 Performance</rdfs:label>
	<skos:notation>F31</skos:notation>
	<skos:prefLabel xml:lang="en">Performance</skos:prefLabel>
</rdf:Description>

<rdf:Description rdf:about="http://iflastandards.info/ns/lrm/lrmoo/F32_Item_Production_Event">
	<rdf:type rdf:resource="http://www.w3.org/2002/07/owl#Class"/>
	<rdfs:subClassOf rdf:resource="http://www.cidoc-crm.org/cidoc-crm/E12_Production"/>
	<rdfs:comment xml:lang="en">Scope note:
This class comprises activities that result in one or more instances of F5 Item coming into existence. The production of a series of physical objects (printed books, scores, CDs, DVDs, CD-ROMs, etc.), producing a unique item (writing a manuscript on parchment, painting a watercolour, etc.), and the creation of a new copy of a file on an electronic carrier are all regarded as instances of F32 Item Production Event.
For mass-produced items, the production process (no matter whether it is a book, a sound recording, a DVD, a cartographic resource, etc.) strives to produce items all as similar as possible to a prototype that displays all the features that all the copies of the publication should also display, which is reflected in the property R27 materialized: F3 Manifestation.

Examples:
- the printing and binding of copies of the paperback edition of the HarperCollins 2017 publication ‘Murder on the Orient Express / Agatha Christie’, by CPI Ltd (UK)
- the printing of copies of the score of Bach’s ‘Goldberg Variations’ by Balthasar Schmid in 1741
- the casting of Auguste Rodin’s ‘The Thinker’ at the Fonderie Alexis Rudier in 1904
- the production of the items of the CD publication ‘Bach Goldberg Variations’, published by Hyperion Records in 2016, including the pressing of the CDs, the printing of the booklet and cover, assembling the parts, etc.
</rdfs:comment>
	<rdfs:label xml:lang="en">F32 Item Production Event</rdfs:label>
	<skos:notation>F32</skos:notation>
	<skos:prefLabel xml:lang="en">Item Production Event</skos:prefLabel>
</rdf:Description>

<rdf:Description rdf:about="http://iflastandards.info/ns/lrm/lrmoo/F33_Reproduction_Event">
	<rdf:type rdf:resource="http://www.w3.org/2002/07/owl#Class"/>
	<rdfs:subClassOf rdf:resource="http://iflastandards.info/ns/lrm/lrmoo/F30_Manifestation_Creation"/>
	<rdfs:subClassOf rdf:resource="http://www.cidoc-crm.org/cidoc-crm/E12_Production"/>
	<rdfs:comment xml:lang="en">Scope note:
This class comprises activities that consist in producing items of a new instance of F3 Manifestation that preserve both the content and layout found on items of a pre-existing instance of F3 Manifestation. The individual instance or instances of F5 Item that was or were used as a source for this process may be precisely identified or not. Such activities result in products known as facsimiles, reproductions, reprints, reissues, or new releases.

Examples:
- the 2014 publication of Daniel Wilson’s ‘Caliban: the missing link’ by Cambridge University Press [a facsimile edition of the 1873 publication by Macmillan]
- the 2015 publication of Harry Partch’s ‘Two studies on ancient Greek scales’ by Schott [which reproduces Harry Partch’s holograph manuscript]
- the 2007 publication of Hubert Reeve’s ‘Malicorne: réflexions d’un observateur de la nature’ published by Éditions du Seuil as number 179 in the series ‘Points. Science’ (ISBN ‘978-2-02-096760-0’) [a reprint edition of the 1990 publication by Éditions du Seuil in the series ‘Science ouverte’ (ISBN ‘2-02-012644-3’)]
</rdfs:comment>
	<rdfs:label xml:lang="en">F33 Reproduction Event</rdfs:label>
	<skos:notation>F33</skos:notation>
	<skos:prefLabel xml:lang="en">Reproduction Event</skos:prefLabel>
</rdf:Description>

<rdf:Description rdf:about="http://iflastandards.info/ns/lrm/lrmoo/F36_Script_Conversion">
	<rdf:type rdf:resource="http://www.w3.org/2002/07/owl#Class"/>
	<rdfs:subClassOf rdf:resource="http://www.cidoc-crm.org/cidoc-crm/E29_Design_or_Procedure"/>
	<rdfs:comment xml:lang="en">Scope note:
This class comprises rule sets for converting signs or arrangements of signs from one script or type set to another.

Examples:
- the rules for the transliteration of the Cyrillic script into Latin script codified in ISO 9:1995 ‘Information and documentation — Transliteration of Cyrillic characters into Latin characters — Slavic and non-Slavic languages’ (ISO 9:1995)
</rdfs:comment>
	<rdfs:label xml:lang="en">F36 Script Conversion</rdfs:label>
	<skos:notation>F36</skos:notation>
	<skos:prefLabel xml:lang="en">Script Conversion</skos:prefLabel>
</rdf:Description>

<rdf:Description rdf:about="http://iflastandards.info/ns/lrm/lrmoo/F39_Family">
	<rdf:type rdf:resource="http://www.w3.org/2002/07/owl#Class"/>
	<rdfs:subClassOf rdf:resource="http://iflastandards.info/ns/lrm/lrmoo/F55_Collective_Agent"/>
	<rdfs:comment xml:lang="en">Scope note:
This class comprises groups of two or more persons presented as a family and justified by relationships of birth, marriage, adoption, civil union, or similar social or legal status and an assumed common tradition, including examples such as royal families, dynasties, houses of nobility, etc.

Examples:
- House of Tudor
- the brothers Grimm
</rdfs:comment>
	<rdfs:label xml:lang="en">F39 Family</rdfs:label>
	<skos:notation>F39</skos:notation>
	<skos:prefLabel xml:lang="en">Family</skos:prefLabel>
</rdf:Description>

<rdf:Description rdf:about="http://iflastandards.info/ns/lrm/lrmoo/F3_Manifestation">
	<rdf:type rdf:resource="http://www.w3.org/2002/07/owl#Class"/>
	<rdfs:subClassOf rdf:resource="http://www.cidoc-crm.org/cidoc-crm/E73_Information_Object"/>
	<rdfs:comment xml:lang="en">Scope note:
This class comprises products rendering one or more Expressions. A Manifestation is defined by both the overall content and the form of its presentation. The substance of F3 Manifestation is not only signs, but also the manner in which they are presented to be consumed by users, including the kind of media adopted.
An F3 Manifestation is the outcome of a publication process where one or more F2 Expressions are prepared for public dissemination, but it may also be a unique form created directly on some material carrier without the intent of being formally published.
An instance of F3 Manifestation typically incorporates one or more instances of F2 Expression representing a distinct logical content and all additional input by a publisher such as text layout and cover design. Additionally an F3 Manifestation can be identified by the physical features for the medium of distribution, if applicable. For example, publications in the form of hard-cover and paperback editions would be two distinct instances of F3 Manifestation, even though authorial and editorial content are otherwise identical in both publications.
In the case of industrial products such as printed books or music CDs, but also digital material, an instance of F3 Manifestation can be regarded as the prototype for all copies of it. In these cases, an instance of F3 Manifestation specifies all of the features or traits that instances of F5 Item display in order to be copies of a particular publication. In the case of industrial products, instances of F3 Manifestation are also instances of E99 Product Type, normally nowadays identified by characteristic identifiers such as ISBN numbers.

Examples:
- the publication ‘Murder on the Orient Express / Agatha Christie’, published by Collins Crime Club in 1934
- the publication of ‘Murder on the Orient Express / Agatha Christie’, published by HarperCollins in 2017
- the publication ‘Mord im Orientexpress : ein Hercule-Poirot-Roman / Agatha Christie’, published by Deutscher Bücherbund in 1975
- the publication ‘Murder on The Orient Express / Agatha Christie’, narrated by David Suchet, audio book (audio CD) published by HarperCollins in 2005
- the HTML-version of Homer’s ‘Odyssey’ with English text by S. H. Butcher and A. Lang, available online from the Gutenberg Project
- the publication ‘The Illustrated Odyssey’, published by Sidgwick &amp; Jackson Ltd in 1980, containing the translated text by E.V. Rieu, an introduction by Jacquetta Hawkes and photographs by Tim Mercer
- the publication ‘The Odyssey of Homer’ published by Harper &amp; Row in 1967, containing an introduction and the English translation of the Greek poem by Richmond Lattimore
- the CD publication ‘Bach Goldberg Variations’, published by Hyperion Records in 2016, containing a CD with Angela Hewitt’s performances of Bach’s ‘Goldberg Variations’ recorded in Christuskirche (Berlin) on 14-17 December 2015 and a booklet with an introduction to the music by Angela Hewitt in English, French and German
- the manuscript known as ‘The Book of Kells’
- the publication containing a text entitled ‘Pop Culture’ (authored by a person named ‘Richard Memeteau’), issued in 2014 by the publisher named ‘Zones’ and distributed in EPUB2 format by a distributor named ‘Editis’ and identified by ISBN ‘978-2-35522-085-2’
- the publication entitled ‘Alfred Hitchcock’s Psycho: 60th Anniversary Edition’, containing one Blu-ray disc with two cuts of the movie, released in 2020
</rdfs:comment>
	<rdfs:label xml:lang="en">F3 Manifestation</rdfs:label>
	<skos:notation>F3</skos:notation>
	<skos:prefLabel xml:lang="en">Manifestation</skos:prefLabel>
</rdf:Description>

<rdf:Description rdf:about="http://iflastandards.info/ns/lrm/lrmoo/F55_Collective_Agent">
	<rdf:type rdf:resource="http://www.w3.org/2002/07/owl#Class"/>
	<rdfs:subClassOf rdf:resource="http://www.cidoc-crm.org/cidoc-crm/E74_Group"/>
	<rdfs:comment xml:lang="en">Scope note:
This class comprises recognizable groups or organizations of persons that have the potential of acting as a unit to produce some intentional result of bibliographic interest for which they can be collectively considered responsible.
A group of people becomes an instance of F55 Collective Agent when it identifies itself by a name that identifies it within an appropriate context and exhibits sufficient organizational characteristics to permit it to perform actions that reflect agency. Groups that are constituted as meetings, conferences, congresses, expeditions, festivals, fairs, etc. are examples of F55 Collective Agent as long as they self-identify by a specific name, rather than being referred to by a generic description of the gathering, and can act as a unit (such as by publishing their proceedings, or approving a report). These collective actions may be performed by representatives selected by the whole, rather than by all individual members acting together.
Collective Agents may be members of other Collective Agents, although directly or indirectly all Collective Agents are composed of persons. The membership of many types of Collective Agents will continue to evolve over time. A Collective Agent may continue to exist even if it has no members for a time (for example, a committee whose members all resign prior to the expiration of their terms but then a new complement of members is appointed).
Instances of F55 Collective Agent include instances of its subclass F11 Corporate Body: commercial or corporate entities and other legally registered bodies, as well as organizations and associations, musical, artistic or performing groups, governments, and any of their sub-units.
Married couples and other concepts of family (instances of F39 Family) are instances of a subclass of F55 Collective Agent.
In the wider sense, this class also comprises holders of official positions viewed collectively, independent of the current holder of the office, such as the president of a country. In such cases, it is possible that the instance of F55 Collective Agent has only ever had a single member.
A group of persons known by/using a joint pseudonym (i.e., a name that seems indicative of an individual but that is actually adopted as a persona by two or more people acting together) is a case of F55 Collective Agent.

Examples:
- International Federation of Library Associations and Institutions (F11)
- 81st World Library and Information Conference (F11)
- Bibliothèque nationale de France (F11)
- Exxon-Mobil (F11)
- The Beatles (F11)
- the brothers Grimm (F39)
- the President of the Swiss Confederation
- Nicolas Bourbaki [collective pseudonym of a group of 20(th) century French mathematicians also known as the ‘Association des collaborateurs de Nicolas Bourbaki’]
- Ellery Queen [joint pseudonym for detective fiction of cousins Frederic Dannay and Manfred Bennington Less who also wrote separately]
</rdfs:comment>
	<rdfs:label xml:lang="en">F55 Collective Agent</rdfs:label>
	<skos:notation>F55</skos:notation>
	<skos:prefLabel xml:lang="en">Collective Agent</skos:prefLabel>
</rdf:Description>

<rdf:Description rdf:about="http://iflastandards.info/ns/lrm/lrmoo/F5_Item">
	<rdf:type rdf:resource="http://www.w3.org/2002/07/owl#Class"/>
	<rdfs:subClassOf rdf:resource="http://www.cidoc-crm.org/cidoc-crm/E24_Physical_Human-Made_Thing"/>
	<rdfs:comment xml:lang="en">Scope note:
This class comprises physical objects (printed books, scores, CDs, DVDs, CD-ROMS, etc.) that were produced by (P186i) an industrial process involving a given instance of F3 Manifestation. As a result, all the instances of F5 Item associated with a given instance of F3 Manifestation are expected to carry the content defined in that instance of F3 Manifestation, although some or even all of them may happen to carry a content that significantly differs from it, due to either an accident in the course of industrial production, or subsequent physical modification or degradation.
An instance of F5 Item that consists of a physical object or set of objects with clear physical boundaries is also an instance of E22 Human-Made Object. An instance of F5 Item that is stored on a part of a larger physical support (such as an electronic file among others on a disc) can also be considered to be an instance of E25 Human-Made Feature.
The notion of F5 Item is only relevant with regard to the production process, from a bibliographic point of view. The physical units managed by cultural heritage institutions in their holdings are a distinct notion: a unit of holdings certainly can be equal to an instance of F5 Item, but it also can be either “bigger” than one (e.g., when two instances of F5 Item are bound together (in the case of printed books)), or “smaller” than one (e.g., for incomplete holdings, such as when only one CD from a two-CD set is held). From an operational point of view, cultural heritage institutions typically do not manage instances of F5 Item, but physical holdings units, instances of E19 Physical Object, although for libraries in most cases this is not significant because each item corresponds with a single unit. When this is not the case, the linkage between items and the units relevant for collection management can be recorded through the P46 is composed of (forms part of) property between instances of F5 Item and instances of E19 Physical Object. If needed, an instance of E19 Physical Object can be typed as a unit through the P2 has type (is type of) property.

Examples:
- the copy of ‘Murder on the Orient Express / Agatha Christie’, HarperCollins 2017, that is held by the Deichman public library in Oslo, Norway, and which is identified by inventory number ‘9138513’
- John Smith’s copy of ‘Murder on the Orient Express / Agatha Christie’, HarperCollins 2017, with the owner’s ex libris stamped on the inside of the cover page
- the copy of the first edition of Bach’s ‘Goldberg Variations’ held by the National Library in France with corrections made by the composer, and additional music in the form of fourteen canons on the Goldberg ground
- the manuscript known as the ‘Book of Kells’ (owned by Trinity College in Dublin)
- the bronze statue of Auguste Rodin’s ‘The Thinker’, cast at the Fonderie Alexis Rudier in 1904 held at the Musée Rodin in Paris, France since 1922
- the ebook ‘Pop Culture’ by Richard Memeteau in EPUB2 format, received by the National Library of France through digital legal deposit on 1st February 2016 to which the legal deposit number DLN-20160201-6 has been assigned. In the catalogue, this item is identified with a unique number: LNUM20553886
- the copy of the electronic file named ‘cidoc_crm_version_7.1.3.pdf’ on my hard drive containing the text of official version 7.1.3 of the ‘Definition of the CIDOC Conceptual Reference Model’
</rdfs:comment>
	<rdfs:label xml:lang="en">F5 Item</rdfs:label>
	<skos:notation>F5</skos:notation>
	<skos:prefLabel xml:lang="en">Item</skos:prefLabel>
</rdf:Description>

<rdf:Description rdf:about="http://vocab.getty.edu/page/aat/300004021">
	<rdf:type rdf:resource="http://www.w3.org/2002/07/owl#Class"/>
	<rdfs:subClassOf rdf:resource="http://www.cidoc-crm.org/cidoc-crm/E55_Type"/>
	<rdfs:label>rooms and spaces by function</rdfs:label>
</rdf:Description>

<rdf:Description rdf:about="http://www.cidoc-crm.org/cidoc-crm/E10_Transfer_of_Custody">
	<rdf:type rdf:resource="http://www.w3.org/2002/07/owl#Class"/>
	<rdfs:subClassOf rdf:resource="http://www.cidoc-crm.org/cidoc-crm/E7_Activity"/>
	<rdfs:comment xml:lang="en">This class comprises transfers of the physical custody or the legal responsibility for the physical custody of objects. The recording of the donor or recipient is optional. It is possible that in an instance of E10 Transfer of Custody there is either no donor or no recipient.
Depending on the circumstances, it may describe:
1. the beginning of custody (there is no previous custodian)
2. the end of custody (there is no subsequent custodian)
3. the transfer of custody (transfer from one custodian to the next)
4. the receipt of custody from an unknown source (the previous custodian is unknown)
5. the declared loss of an object (the current or subsequent custodian is unknown)
In the event that only a single kind of transfer of custody occurs, either the legal responsibility for the custody or the actual physical possession of the object but not both, this difference should be expressed using the property P2 has type (is type of).
The sense of physical possession requires that the object of custody be in the hands of the keeper at least with a part representative for the whole. The way, in which a representative part is defined, should ensure that it is unambiguous who keeps a part and who the whole and should be consistent with the identity criteria of the kept instance of E18 Physical Thing.
The interpretation of the museum notion of "accession" differs between institutions. The CIDOC CRM therefore models legal ownership and physical custody separately. Institutions will then model their specific notions of accession and deaccession as combinations of these.
Theft is a specific case of illegal transfer of custody.</rdfs:comment>
	<rdfs:label xml:lang="en">Transfer of Custody</rdfs:label>
	<rdfs:label xml:lang="fr">Transfert de la garde</rdfs:label>
	<rdfs:label xml:lang="pt">Transferência de Custódia</rdfs:label>
	<rdfs:label xml:lang="de">Übertragung des Gewahrsams</rdfs:label>
	<rdfs:label xml:lang="el">Μεταβίβαση Κατοχής</rdfs:label>
	<rdfs:label xml:lang="ru">Передача Опеки</rdfs:label>
	<rdfs:label xml:lang="zh">转移监护权</rdfs:label>
</rdf:Description>

<rdf:Description rdf:about="http://www.cidoc-crm.org/cidoc-crm/E11_Modification">
	<rdf:type rdf:resource="http://www.w3.org/2002/07/owl#Class"/>
	<rdfs:subClassOf rdf:resource="http://www.cidoc-crm.org/cidoc-crm/E7_Activity"/>
	<rdfs:comment xml:lang="en">This class comprises instances of E7 Activity that are undertaken to create, alter or change instances of E24 Physical Human-Made Thing.
This class includes the production of an item from raw materials and other so far undocumented objects. It also includes the conservation treatment of an object.
Since the distinction between modification and production is not always clear, modification is regarded as the more generally applicable concept. This implies that some items may be consumed or destroyed in an instance of E11 Modification, and that others may be produced as a result of it. An event should also be documented using an instance of E81 Transformation if it results in the destruction of one or more objects and the simultaneous production of others using parts or material from the originals. In this case, the new items have separate identities.
An activity undertaken on an object which was designed to alter it, but which, in fact, it did not in any seemingly significant way (such as the application of a solvent during conservation which failed to dissolve any part of the object), is still considered as an instance of E11 Modification. Typically, any such activity will leave at least forensic traces of evidence on the object.
If the instance of E29 Design or Procedure utilized for the modification prescribes the use of specific materials, they should be documented using property P68 foresees use of (use foreseen by): E57 Material of E29 Design or Procedure, rather than via P126 employed (was employed in): E57 Material.</rdfs:comment>
	<rdfs:label xml:lang="de">Bearbeitung</rdfs:label>
	<rdfs:label xml:lang="en">Modification</rdfs:label>
	<rdfs:label xml:lang="fr">Modification</rdfs:label>
	<rdfs:label xml:lang="pt">Modificação</rdfs:label>
	<rdfs:label xml:lang="el">Τροποποίηση</rdfs:label>
	<rdfs:label xml:lang="ru">Событие Изменения</rdfs:label>
	<rdfs:label xml:lang="zh">修改</rdfs:label>
</rdf:Description>

<rdf:Description rdf:about="http://www.cidoc-crm.org/cidoc-crm/E12_Production">
	<rdf:type rdf:resource="http://www.w3.org/2002/07/owl#Class"/>
	<rdfs:subClassOf rdf:resource="http://www.cidoc-crm.org/cidoc-crm/E11_Modification"/>
	<rdfs:subClassOf rdf:resource="http://www.cidoc-crm.org/cidoc-crm/E63_Beginning_of_Existence"/>
	<rdfs:comment xml:lang="en">This class comprises activities that are designed to, and succeed in, creating one or more new items.
It specializes the notion of modification into production. The decision as to whether or not an object is regarded as new is context sensitive. Normally, items are considered “new” if there is no obvious overall similarity between them and the consumed items and material used in their production. In other cases, an item is considered “new” because it becomes relevant to documentation by a modification. For example, the scribbling of a name on a potsherd may make it a voting token. The original potsherd may not be worth documenting, in contrast to the inscribed one.
This entity can be collective: the printing of a thousand books, for example, would normally be considered a single event.
An event should also be documented using an instance of E81 Transformation if it results in the destruction of one or more objects and the simultaneous production of others using parts or material from the originals. In this case, the new items have separate identities and matter is preserved, but identity is not.</rdfs:comment>
	<rdfs:label xml:lang="de">Herstellung</rdfs:label>
	<rdfs:label xml:lang="en">Production</rdfs:label>
	<rdfs:label xml:lang="fr">Production</rdfs:label>
	<rdfs:label xml:lang="pt">Produção</rdfs:label>
	<rdfs:label xml:lang="el">Παραγωγή</rdfs:label>
	<rdfs:label xml:lang="ru">Событие Производства</rdfs:label>
	<rdfs:label xml:lang="zh">生产</rdfs:label>
</rdf:Description>

<rdf:Description rdf:about="http://www.cidoc-crm.org/cidoc-crm/E13_Attribute_Assignment">
	<rdf:type rdf:resource="http://www.w3.org/2002/07/owl#Class"/>
	<rdfs:subClassOf rdf:resource="http://www.cidoc-crm.org/cidoc-crm/E7_Activity"/>
	<rdfs:comment xml:lang="en">This class comprises the actions of making assertions about one property of an object or any single relation between two items or concepts. The type of the property asserted to hold between two items or concepts can be described by the property P177 assigned property of type (is type of property assigned): E55 Type.
For example, the class describes the actions of people making propositions and statements during certain scientific/scholarly procedures, e.g. the person and date when a condition statement was made, an identifier was assigned, the museum object was measured, etc. Which kinds of such assignments and statements need to be documented explicitly in structures of a schema rather than free text, depends on whether this information should be accessible by structured queries.
This class allows for the documentation of how the respective assignment came about, and whose opinion it was. Note that all instances of properties described in a knowledge base are the opinion of someone. Per default, they are the opinion of the team maintaining the knowledge base. This fact must not individually be registered for all instances of properties provided by the maintaining team, because it would result in an endless recursion of whose opinion was the description of an opinion. Therefore, the use of instances of E13 Attribute Assignment marks the fact that the maintaining team is in general neutral to the validity of the respective assertion, but registers someone else’s opinion and how it came about.
All properties assigned in such an action can also be seen as directly relating the respective pair of items or concepts. Multiple use of instances of E13 Attribute Assignment may possibly lead to a collection of contradictory values.</rdfs:comment>
	<rdfs:label xml:lang="fr">Assignation d’attribut</rdfs:label>
	<rdfs:label xml:lang="pt">Atribuição de Característica</rdfs:label>
	<rdfs:label xml:lang="en">Attribute Assignment</rdfs:label>
	<rdfs:label xml:lang="de">Merkmalszuweisung</rdfs:label>
	<rdfs:label xml:lang="el">Απόδοση Ιδιοτήτων</rdfs:label>
	<rdfs:label xml:lang="ru">Присвоение Атрибута</rdfs:label>
	<rdfs:label xml:lang="zh">属性赋值</rdfs:label>
</rdf:Description>

<rdf:Description rdf:about="http://www.cidoc-crm.org/cidoc-crm/E14_Condition_Assessment">
	<rdf:type rdf:resource="http://www.w3.org/2002/07/owl#Class"/>
	<rdfs:subClassOf rdf:resource="http://www.cidoc-crm.org/cidoc-crm/E13_Attribute_Assignment"/>
	<rdfs:comment xml:lang="en">This class describes the act of assessing the state of preservation of an object during a particular period.
The condition assessment may be carried out by inspection, measurement, or through historical research. This class is used to document circumstances of the respective assessment that is relevant to interpret its quality at a later stage, or to continue research on related documents.</rdfs:comment>
	<rdfs:label xml:lang="pt">Avaliação do Estado Material</rdfs:label>
	<rdfs:label xml:lang="en">Condition Assessment</rdfs:label>
	<rdfs:label xml:lang="de">Zustandsfeststellung</rdfs:label>
	<rdfs:label xml:lang="fr">Évaluation d’état matériel</rdfs:label>
	<rdfs:label xml:lang="el">Εκτίμηση Κατάστασης</rdfs:label>
	<rdfs:label xml:lang="ru">Оценка Состояния</rdfs:label>
	<rdfs:label xml:lang="zh">状态评估</rdfs:label>
</rdf:Description>

<rdf:Description rdf:about="http://www.cidoc-crm.org/cidoc-crm/E15_Identifier_Assignment">
	<rdf:type rdf:resource="http://www.w3.org/2002/07/owl#Class"/>
	<rdfs:subClassOf rdf:resource="http://www.cidoc-crm.org/cidoc-crm/E13_Attribute_Assignment"/>
	<rdfs:comment xml:lang="en">This class comprises activities that result in the allocation of an identifier to an instance of E1 CRM Entity. An instance of E15 Identifier Assignment may include the creation of the identifier from multiple constituents, which themselves may be instances of E41 Appellation. The syntax and kinds of constituents to be used may be declared in a rule constituting an instance of E29 Design or Procedure.
Examples of such identifiers include Find Numbers, Inventory Numbers, uniform titles in the sense of librarianship and Digital Object Identifiers (DOI). Documenting the act of identifier assignment and deassignment is especially useful when objects change custody or the identification system of an organization is changed. In order to keep track of the identity of things in such cases, it is important to document by whom, when, and for what purpose an identifier is assigned to an item.
The fact that an identifier is a preferred one for an organisation can be expressed by using the property E1 CRM Entity. P48 has preferred identifier (is preferred identifier of): E42 Identifier. It can better be expressed in a context independent form by assigning a suitable E55 Type, such as “preferred identifier assignment”, to the respective instance of E15 Identifier Assignment through the P2 has type (is type of) property.</rdfs:comment>
	<rdfs:label xml:lang="fr">Assignation d’identifiant</rdfs:label>
	<rdfs:label xml:lang="pt">Atribuição de Identificador</rdfs:label>
	<rdfs:label xml:lang="en">Identifier Assignment</rdfs:label>
	<rdfs:label xml:lang="de">Kennzeichenzuweisung</rdfs:label>
	<rdfs:label xml:lang="el">Απόδοση Αναγνωριστικού</rdfs:label>
	<rdfs:label xml:lang="ru">Назначение Идентификатора</rdfs:label>
	<rdfs:label xml:lang="zh">标识符赋值</rdfs:label>
</rdf:Description>

<rdf:Description rdf:about="http://www.cidoc-crm.org/cidoc-crm/E16_Measurement">
	<rdf:type rdf:resource="http://www.w3.org/2002/07/owl#Class"/>
	<rdfs:subClassOf rdf:resource="http://www.cidoc-crm.org/cidoc-crm/E13_Attribute_Assignment"/>
	<rdfs:comment xml:lang="en">This class comprises actions measuring physical properties and other values that can be determined by a systematic, objective procedure of direct observation of particular states of physical reality.
An instance of E16 Measurement may use simple counting or tools, such as yardsticks or radiation detection devices. The interest is in the method and care applied, so that the reliability of the result may be judged at a later stage, or research continued on the associated documents. The date of the event is important for dimensions, which may change value over time, such as the length of an object subject to shrinkage. Methods and devices employed should be associated with instances of E16 Measurement by properties such as P33 used specific technique: E29 Design or Procedure, P125 used object of type: E55 Type, P16 used specific object (was used for): E70 Thing, whereas basic techniques such as "carbon-14 dating" should be encoded using P2 has type (is type of): E55 Type. Details of methods and devices reused or reusable in other instances of E16 Measurement should be documented for these entities rather than the measurements themselves, whereas details of particular execution may be documented by free text or by instantiating adequate sub-activities, if the detail may be of interest for an overarching query.
Regardless whether a measurement is made by an instrument or by human senses, it represents the initial transition from physical reality to information without any other documented information object in between within the reasoning chain that would represent the result of the interaction of the observer or device with reality. Therefore, determining properties of an instance of E90 Symbolic Object is regarded as an instance of E13 Attribute Assignment, which may be inferred from observing and measuring representative carriers. In the case that the carrier can be named, the property P16 used specific object (was used for) should be used to indicate the instance(s) of E18 Physical Thing that was used as the empirical basis for the attribute assignment. For instance, inferring properties of depicted items using image material, such as satellite images, is not regarded as an instance of E16 Measurement, but as a subsequent instance of E13 Attribute Assignment. Rather, only the production of the images, understood as arrays of radiation intensities, is regarded as an instance of E16 Measurement. The same reasoning holds for other sensor data.</rdfs:comment>
	<rdfs:label xml:lang="en">Measurement</rdfs:label>
	<rdfs:label xml:lang="pt">Medição</rdfs:label>
	<rdfs:label xml:lang="de">Messung</rdfs:label>
	<rdfs:label xml:lang="fr">Mesurage</rdfs:label>
	<rdfs:label xml:lang="el">Μέτρηση</rdfs:label>
	<rdfs:label xml:lang="ru">Событие Измерения</rdfs:label>
	<rdfs:label xml:lang="zh">测量</rdfs:label>
</rdf:Description>

<rdf:Description rdf:about="http://www.cidoc-crm.org/cidoc-crm/E17_Type_Assignment">
	<rdf:type rdf:resource="http://www.w3.org/2002/07/owl#Class"/>
	<rdfs:subClassOf rdf:resource="http://www.cidoc-crm.org/cidoc-crm/E13_Attribute_Assignment"/>
	<rdfs:comment xml:lang="en">This class comprises the actions of classifying items of whatever kind. Such items include objects, specimens, people, actions, and concepts.
This class allows for the documentation of the context of classification acts in cases where the value of the classification depends on the personal opinion of the classifier, and the date that the classification was made. This class also encompasses the notion of “determination,” i.e. the systematic and molecular identification of a specimen in biology.</rdfs:comment>
	<rdfs:label xml:lang="fr">Assignation de type</rdfs:label>
	<rdfs:label xml:lang="pt">Atribuição de Tipo</rdfs:label>
	<rdfs:label xml:lang="en">Type Assignment</rdfs:label>
	<rdfs:label xml:lang="de">Typuszuweisung</rdfs:label>
	<rdfs:label xml:lang="el">Απόδοση Τύπου</rdfs:label>
	<rdfs:label xml:lang="ru">Присвоение Типа</rdfs:label>
	<rdfs:label xml:lang="zh">类型赋值</rdfs:label>
</rdf:Description>

<rdf:Description rdf:about="http://www.cidoc-crm.org/cidoc-crm/E18_Physical_Thing">
	<rdf:type rdf:resource="http://www.w3.org/2002/07/owl#Class"/>
	<rdfs:subClassOf rdf:resource="http://www.cidoc-crm.org/cidoc-crm/E72_Legal_Object"/>
	<rdfs:comment>E19 Physical Thing refers to tangible, persistent physical entities that can be seen and interacted with, such as buildings, towns, or natural landscapes. For example, when the narrator describes seeing towns like Wolfsänger and Bökshausen during their journey, they are observing the physical structures and landscapes of these towns, which are instances of E19 Physical Thing, not just abstract locations.</rdfs:comment>
	<rdfs:comment xml:lang="en">This class comprises all persistent physical items with a relatively stable form, human-made or natural.
Depending on the existence of natural boundaries of such things, the CIDOC CRM distinguishes the instances of E19 Physical Object from instances of E26 Physical Feature, such as holes, rivers, pieces of land, etc. Most instances of E19 Physical Object can be moved (if not too heavy), whereas features are integral to the surrounding matter.
An instance of E18 Physical Thing occupies not only a particular geometric space at any instant of its existence, but in the course of its existence it also forms a trajectory through spacetime, which occupies a real, that is phenomenal, volume in spacetime. We include in the occupied space the space filled by the matter of the physical thing and all its inner spaces, such as the interior of a box. For the purpose of more detailed descriptions of the presence of an instance of E18 Physical Thing in space and time it can be associated with its specific instance of E92 Spacetime Volume by the property P196 defines (is defined by).
The CIDOC CRM is generally not concerned with amounts of matter in fluid or gaseous states, as long as they are not confined in an identifiable way for an identifiable minimal time-span.</rdfs:comment>
	<rdfs:label xml:lang="fr">Chose matérielle</rdfs:label>
	<rdfs:label xml:lang="pt">Coisa Material</rdfs:label>
	<rdfs:label xml:lang="de">Materielles</rdfs:label>
	<rdfs:label xml:lang="en">Physical Thing</rdfs:label>
	<rdfs:label xml:lang="el">Υλικό Πράγμα</rdfs:label>
	<rdfs:label xml:lang="ru">Физическая Вещь</rdfs:label>
	<rdfs:label xml:lang="zh">实物</rdfs:label>
</rdf:Description>

<rdf:Description rdf:about="http://www.cidoc-crm.org/cidoc-crm/E19_Physical_Object">
	<rdf:type rdf:resource="http://www.w3.org/2002/07/owl#Class"/>
	<rdfs:subClassOf rdf:resource="http://www.cidoc-crm.org/cidoc-crm/E18_Physical_Thing"/>
	<rdfs:comment xml:lang="en">This class comprises items of a material nature that are units for documentation and have physical boundaries that separate them completely in an objective way from other objects.
The class also includes all aggregates of objects made for functional purposes of whatever kind, independent of physical coherence, such as a set of chessmen. Typically, instances of E19 Physical Object can be moved (if not too heavy).
In some contexts, such objects, except for aggregates, are also called “bona fide objects”, i.e. naturally defined objects (Smith &amp;amp; Varzi, 2000).
The decision as to what is documented as a complete item, rather than by its parts or components, may be purely administrative or may be a result of the order in which the item was acquired.</rdfs:comment>
	<rdfs:label xml:lang="de">Materieller Gegenstand</rdfs:label>
	<rdfs:label xml:lang="fr">Objet matériel</rdfs:label>
	<rdfs:label xml:lang="pt">Objeto Material</rdfs:label>
	<rdfs:label xml:lang="en">Physical Object</rdfs:label>
	<rdfs:label xml:lang="el">Υλικό Αντικείμενο</rdfs:label>
	<rdfs:label xml:lang="ru">Физический Объект</rdfs:label>
	<rdfs:label xml:lang="zh">物质对象</rdfs:label>
</rdf:Description>

<rdf:Description rdf:about="http://www.cidoc-crm.org/cidoc-crm/E1_CRM_Entity">
	<rdf:type rdf:resource="http://www.w3.org/2002/07/owl#Class"/>
	<rdfs:comment xml:lang="en">This class comprises all things in the universe of discourse of the CIDOC Conceptual Reference Model.
It is an abstract concept providing for three general properties:
Identification by name or appellation, and in particular by a preferred identifier
Classification by type, allowing further refinement of the specific subclass to which an instance belongs
Attachment of free text and other unstructured data for the expression of anything not captured by formal properties
All other classes within the CIDOC CRM are directly or indirectly specialisations of E1 CRM Entity.</rdfs:comment>
	<rdfs:label xml:lang="en">CRM Entity</rdfs:label>
	<rdfs:label xml:lang="de">CRM Entität</rdfs:label>
	<rdfs:label xml:lang="ru">CRM Сущность</rdfs:label>
	<rdfs:label xml:lang="zh">CRM实体</rdfs:label>
	<rdfs:label xml:lang="pt">Entidade CRM</rdfs:label>
	<rdfs:label xml:lang="fr">Entité CRM</rdfs:label>
	<rdfs:label xml:lang="el">Οντότητα CIDOC CRM</rdfs:label>
</rdf:Description>

<rdf:Description rdf:about="http://www.cidoc-crm.org/cidoc-crm/E20_Biological_Object">
	<rdf:type rdf:resource="http://www.w3.org/2002/07/owl#Class"/>
	<rdfs:subClassOf rdf:resource="http://www.cidoc-crm.org/cidoc-crm/E19_Physical_Object"/>
	<rdfs:comment xml:lang="en">This class comprises individual items of a material nature, which live, have lived, or are natural products of or from living organisms.
Artificial objects that incorporate biological elements, such as Victorian butterfly frames, can be documented as both instances of E20 Biological Object and E22 Human-Made Object.</rdfs:comment>
	<rdfs:label xml:lang="en">Biological Object</rdfs:label>
	<rdfs:label xml:lang="de">Biologischer Gegenstand</rdfs:label>
	<rdfs:label xml:lang="fr">Objet biologique</rdfs:label>
	<rdfs:label xml:lang="pt">Objeto Biológico</rdfs:label>
	<rdfs:label xml:lang="el">Βιολογικό Ακτικείμενο</rdfs:label>
	<rdfs:label xml:lang="ru">Биологический Объект</rdfs:label>
	<rdfs:label xml:lang="zh">生物对象</rdfs:label>
</rdf:Description>

<rdf:Description rdf:about="http://www.cidoc-crm.org/cidoc-crm/E21_Person">
	<rdf:type rdf:resource="http://www.w3.org/2002/07/owl#Class"/>
	<rdfs:subClassOf rdf:resource="http://www.cidoc-crm.org/cidoc-crm/E20_Biological_Object"/>
	<rdfs:subClassOf rdf:resource="http://www.cidoc-crm.org/cidoc-crm/E39_Actor"/>
	<rdfs:comment xml:lang="en">This class comprises real persons who live or are assumed to have lived.
Legendary figures that may have existed, such as Ulysses and King Arthur, fall into this class if the documentation refers to them as historical figures. In cases where doubt exists as to whether several persons are in fact identical, multiple instances can be created and linked to indicate their relationship. The CIDOC CRM does not propose a specific form to support reasoning about possible identity.
In a bibliographic context, a name presented following the conventions usually employed for personal names will be assumed to correspond to an actual real person (an instance of E21 Person), unless evidence is available to indicate that this is not the case. The fact that a persona may erroneously be classified as an instance of E21 Person does not imply that the concept comprises personae.</rdfs:comment>
	<rdfs:label xml:lang="de">Person</rdfs:label>
	<rdfs:label xml:lang="en">Person</rdfs:label>
	<rdfs:label xml:lang="fr">Personne</rdfs:label>
	<rdfs:label xml:lang="pt">Pessoa</rdfs:label>
	<rdfs:label xml:lang="el">Πρόσωπο</rdfs:label>
	<rdfs:label xml:lang="ru">Личность</rdfs:label>
	<rdfs:label xml:lang="zh">人物</rdfs:label>
</rdf:Description>

<rdf:Description rdf:about="http://www.cidoc-crm.org/cidoc-crm/E22_Human-Made_Object">
	<rdf:type rdf:resource="http://www.w3.org/2002/07/owl#Class"/>
	<rdfs:subClassOf rdf:resource="http://www.cidoc-crm.org/cidoc-crm/E19_Physical_Object"/>
	<rdfs:subClassOf rdf:resource="http://www.cidoc-crm.org/cidoc-crm/E24_Physical_Human-Made_Thing"/>
	<rdfs:comment xml:lang="en">This class comprises all persistent physical objects of any size that are purposely created by human activity and have physical boundaries that separate them completely in an objective way from other objects.
The class also includes all aggregates of objects made for functional purposes of whatever kind, independent of physical coherence, such as a set of chessmen.</rdfs:comment>
	<rdfs:label xml:lang="en">Human-Made Object</rdfs:label>
	<rdfs:label xml:lang="fr">Objet élaboré par l’humain</rdfs:label>
</rdf:Description>

<rdf:Description rdf:about="http://www.cidoc-crm.org/cidoc-crm/E24_Physical_Human-Made_Thing">
	<rdf:type rdf:resource="http://www.w3.org/2002/07/owl#Class"/>
	<rdfs:subClassOf rdf:resource="http://www.cidoc-crm.org/cidoc-crm/E18_Physical_Thing"/>
	<rdfs:subClassOf rdf:resource="http://www.cidoc-crm.org/cidoc-crm/E71_Human-Made_Thing"/>
	<rdfs:comment xml:lang="en">This class comprises all persistent physical items of any size that are purposely created by human activity. This class comprises, besides others, human-made objects, such as a sword, and human-made features, such as rock art. For example, a “cup and ring” carving on bedrock is regarded as instance of E24 Physical Human-Made Thing.
Instances of E24 Physical Human-Made Thing may be the result of modifying pre-existing physical things, preserving larger parts or most of the original matter and structure, which poses the question if they are new or even human-made, the respective interventions of production made on such original material should be obvious and sufficient to regard that the product has a new, distinct identity and intended function and is human-made. Substantial continuity of the previous matter and structure in the new product can be documented by describing the production process also as an instance of E81 Transformation.
Whereas interventions of conservation and repair are not regarded to produce a new instance of E24 Physical Human-Made Thing, the results of preparation of natural history specimens that substantially change their natural or original state should be regarded as instances of E24 Physical Human-Made Things, including the uncovering of petrified biological features from a solid piece of stone. On the other side, scribbling a museum number on a natural object should not be regarded to make it human-made. This notwithstanding, parts, sections, segments, or features of an instance of E24 Physical Human-Made Thing may continue to be non-human-made and preserved during the production process, for example natural pearls used as a part of an eardrop.</rdfs:comment>
	<rdfs:label xml:lang="fr">Chose matérielle élaborée par l’humain</rdfs:label>
	<rdfs:label xml:lang="en">Physical Human-Made Thing</rdfs:label>
</rdf:Description>

<rdf:Description rdf:about="http://www.cidoc-crm.org/cidoc-crm/E25_Human-Made_Feature">
	<rdf:type rdf:resource="http://www.w3.org/2002/07/owl#Class"/>
	<rdfs:subClassOf rdf:resource="http://www.cidoc-crm.org/cidoc-crm/E24_Physical_Human-Made_Thing"/>
	<rdfs:subClassOf rdf:resource="http://www.cidoc-crm.org/cidoc-crm/E26_Physical_Feature"/>
	<rdfs:comment xml:lang="en">This class comprises physical features that are purposely created by human activity, such as scratches, artificial caves, artificial water channels, etc. In particular, it includes the information encoding features on mechanical or digital carriers.</rdfs:comment>
	<rdfs:label xml:lang="fr">Caractéristique élaborée par l'humain</rdfs:label>
	<rdfs:label xml:lang="en">Human-Made Feature</rdfs:label>
</rdf:Description>

<rdf:Description rdf:about="http://www.cidoc-crm.org/cidoc-crm/E26_Physical_Feature">
	<rdf:type rdf:resource="http://www.w3.org/2002/07/owl#Class"/>
	<rdfs:subClassOf rdf:resource="http://www.cidoc-crm.org/cidoc-crm/E18_Physical_Thing"/>
	<rdfs:comment xml:lang="en">This class comprises identifiable features that are physically attached in an integral way to particular physical objects.
Instances of E26 Physical Feature share many of the attributes of instances of E19 Physical Object. They may have a one-dimensional, two-dimensional, or three-dimensional geometric extent, but there are no natural borders that separate them completely in an objective way from the carrier objects. For example, a doorway is a feature but the door itself, being attached by hinges, is not.
Instances of E26 Physical Feature can be features in a narrower sense, such as scratches, holes, reliefs, surface colours, reflection zones in an opal crystal or a density change in a piece of wood. In the wider sense, they are portions of particular objects with partially imaginary borders, such as the core of the Earth, an area of property on the surface of the Earth, a landscape or the head of a contiguous marble statue. They can be measured and dated, and it is sometimes possible to state who or what is or was responsible for them. They cannot be separated from the carrier object, but a segment of the carrier object may be identified (or sometimes removed) carrying the complete feature.
This definition coincides with the definition of “fiat objects”, with the exception of aggregates of “bona fide objects” (Smith &amp;amp; Varzi, 2000).</rdfs:comment>
	<rdfs:label xml:lang="pt">Característica Material</rdfs:label>
	<rdfs:label xml:lang="fr">Caractéristique physique</rdfs:label>
	<rdfs:label xml:lang="de">Materielles Merkmal</rdfs:label>
	<rdfs:label xml:lang="en">Physical Feature</rdfs:label>
	<rdfs:label xml:lang="el">Υλικό Μόρφωμα</rdfs:label>
	<rdfs:label xml:lang="ru">Физический Признак</rdfs:label>
	<rdfs:label xml:lang="zh">物理特征</rdfs:label>
</rdf:Description>

<rdf:Description rdf:about="http://www.cidoc-crm.org/cidoc-crm/E27_Site">
	<rdf:type rdf:resource="http://www.w3.org/2002/07/owl#Class"/>
	<rdfs:subClassOf rdf:resource="http://www.cidoc-crm.org/cidoc-crm/E26_Physical_Feature"/>
	<rdfs:comment xml:lang="en">This class comprises pieces of land or sea floor.
In contrast to the purely geometric notion of E53 Place, this class describes constellations of matter on the surface of the Earth or other celestial body, which can be represented by photographs, paintings, and maps.
Instances of E27 Site are composed of relatively immobile material items and features in a particular configuration at a particular location.</rdfs:comment>
	<rdfs:label xml:lang="de">Gelände</rdfs:label>
	<rdfs:label xml:lang="pt">Lugar</rdfs:label>
	<rdfs:label xml:lang="en">Site</rdfs:label>
	<rdfs:label xml:lang="fr">Site</rdfs:label>
	<rdfs:label xml:lang="el">Φυσικός Χώρος</rdfs:label>
	<rdfs:label xml:lang="ru">Участок</rdfs:label>
	<rdfs:label xml:lang="zh">场地</rdfs:label>
</rdf:Description>

<rdf:Description rdf:about="http://www.cidoc-crm.org/cidoc-crm/E28_Conceptual_Object">
	<rdf:type rdf:resource="http://www.w3.org/2002/07/owl#Class"/>
	<rdfs:subClassOf rdf:resource="http://www.cidoc-crm.org/cidoc-crm/E71_Human-Made_Thing"/>
	<rdfs:comment xml:lang="en">This class comprises non-material products of our minds and other human produced data that have become objects of a discourse about their identity, circumstances of creation, or historical implication. The production of such information might have been supported by the use of technical devices such as cameras or computers.
Characteristically, instances of this class are created, invented or thought by someone, and then may be documented or communicated between persons. Instances of E28 Conceptual Object have the ability to exist on more than one particular carrier at the same time, such as paper, electronic signals, marks, audio media, paintings, photos, human memories, etc.
They cannot be destroyed. They exist as long as they can be found on at least one carrier or in at least one human memory. Their existence ends when the last carrier and the last memory are lost.</rdfs:comment>
	<rdfs:label xml:lang="de">Begrifflicher Gegenstand</rdfs:label>
	<rdfs:label xml:lang="en">Conceptual Object</rdfs:label>
	<rdfs:label xml:lang="fr">Objet conceptuel</rdfs:label>
	<rdfs:label xml:lang="pt">Objeto Conceitual</rdfs:label>
	<rdfs:label xml:lang="el">Νοητικό Αντικείμενο</rdfs:label>
	<rdfs:label xml:lang="ru">Концептуальный Объект</rdfs:label>
	<rdfs:label xml:lang="zh">概念对象</rdfs:label>
</rdf:Description>

<rdf:Description rdf:about="http://www.cidoc-crm.org/cidoc-crm/E29_Design_or_Procedure">
	<rdf:type rdf:resource="http://www.w3.org/2002/07/owl#Class"/>
	<rdfs:subClassOf rdf:resource="http://www.cidoc-crm.org/cidoc-crm/E73_Information_Object"/>
	<rdfs:comment xml:lang="en">This class comprises documented plans for the execution of actions in order to achieve a result of a specific quality, form, or contents. In particular, it comprises plans for deliberate human activities that may result in new instances of E71 Human-Made Thing or for shaping or guiding the execution of an instance of E7 Activity.
Instances of E29 Design or Procedure can be structured in parts and sequences or depend on others.
This is modelled using P69 has association with (is associated with): E29 Design or Procedure.
Designs or procedures can be seen as one of the following:
1. A schema for the activities it describes
2. A schema of the products that result from their application
3. An independent intellectual product that may have never been applied, such as Leonardo da Vinci’s famous plans for flying machines
Because designs or procedures may never be applied or only partially executed, the CIDOC CRM models a loose relationship between the plan and the respective product.</rdfs:comment>
	<rdfs:label xml:lang="fr">Conceptualisation ou procédure</rdfs:label>
	<rdfs:label xml:lang="en">Design or Procedure</rdfs:label>
	<rdfs:label xml:lang="de">Entwurf oder Verfahren</rdfs:label>
	<rdfs:label xml:lang="pt">Projeto ou Procedimento</rdfs:label>
	<rdfs:label xml:lang="el">Σχέδιο</rdfs:label>
	<rdfs:label xml:lang="ru">Проект или Процедура</rdfs:label>
	<rdfs:label xml:lang="zh">设计或程序</rdfs:label>
</rdf:Description>

<rdf:Description rdf:about="http://www.cidoc-crm.org/cidoc-crm/E2_Temporal_Entity">
	<rdf:type rdf:resource="http://www.w3.org/2002/07/owl#Class"/>
	<rdfs:subClassOf rdf:resource="http://www.cidoc-crm.org/cidoc-crm/E1_CRM_Entity"/>
	<rdfs:subClassOf rdf:resource="http://www.loa-cnr.it/ontologies/DOLCE-Lite#perdurant"/>
	<rdfs:comment xml:lang="en">This class comprises all phenomena, such as the instances of E4 Periods and E5 Events, which happen over a limited extent in time. This extent in time must be contiguous, i.e., without gaps. In case the defining kinds of phenomena for an instance of E2 Temporal Entity cease to happen, and occur later again at another time, we regard that the former instance of E2 Temporal Entity has ended and a new instance has come into existence. In more intuitive terms, the same event cannot happen twice.
In some contexts, such phenomena are also called perdurants. This class is disjoint from E77 Persistent Item and is an abstract class that typically has no direct instances. E2 Temporal Entity is specialized into E4 Period, which applies to a particular geographic area (defined with a greater or lesser degree of precision), and E3 Condition State, which applies to instances of E18 Physical Thing.</rdfs:comment>
	<rdfs:label xml:lang="pt">Entidade Temporal</rdfs:label>
	<rdfs:label xml:lang="fr">Entité temporelle</rdfs:label>
	<rdfs:label xml:lang="de">Geschehendes</rdfs:label>
	<rdfs:label xml:lang="en">Temporal Entity</rdfs:label>
	<rdfs:label xml:lang="el">Έγχρονη Οντότητα</rdfs:label>
	<rdfs:label xml:lang="ru">Временная Сущность</rdfs:label>
	<rdfs:label xml:lang="zh">时序实体</rdfs:label>
</rdf:Description>

<rdf:Description rdf:about="http://www.cidoc-crm.org/cidoc-crm/E30_Right">
	<rdf:type rdf:resource="http://www.w3.org/2002/07/owl#Class"/>
	<rdfs:subClassOf rdf:resource="http://www.cidoc-crm.org/cidoc-crm/E89_Propositional_Object"/>
	<rdfs:comment xml:lang="en">This class comprises legal privileges concerning material and immaterial things or their derivatives.
These include reproduction and property rights.</rdfs:comment>
	<rdfs:label xml:lang="pt">Direitos</rdfs:label>
	<rdfs:label xml:lang="fr">Droit</rdfs:label>
	<rdfs:label xml:lang="de">Recht</rdfs:label>
	<rdfs:label xml:lang="en">Right</rdfs:label>
	<rdfs:label xml:lang="el">Δικαίωμα</rdfs:label>
	<rdfs:label xml:lang="ru">Право</rdfs:label>
	<rdfs:label xml:lang="zh">权限</rdfs:label>
</rdf:Description>

<rdf:Description rdf:about="http://www.cidoc-crm.org/cidoc-crm/E31_Document">
	<rdf:type rdf:resource="http://www.w3.org/2002/07/owl#Class"/>
	<rdfs:subClassOf rdf:resource="http://www.cidoc-crm.org/cidoc-crm/E73_Information_Object"/>
	<rdfs:comment xml:lang="en">This class comprises identifiable immaterial items that make propositions about reality.
These propositions may be expressed in text, graphics, images, audiograms, videograms, or by other similar means. Documentation databases are regarded as instances of E31 Document. This class should not be confused with the concept “document” in Information Technology, which is compatible with E73 Information Object.</rdfs:comment>
	<rdfs:label xml:lang="en">Document</rdfs:label>
	<rdfs:label xml:lang="fr">Document</rdfs:label>
	<rdfs:label xml:lang="pt">Documento</rdfs:label>
	<rdfs:label xml:lang="de">Dokument</rdfs:label>
	<rdfs:label xml:lang="el">Τεκμήριο</rdfs:label>
	<rdfs:label xml:lang="ru">Документ</rdfs:label>
	<rdfs:label xml:lang="zh">文献</rdfs:label>
</rdf:Description>

<rdf:Description rdf:about="http://www.cidoc-crm.org/cidoc-crm/E32_Authority_Document">
	<rdf:type rdf:resource="http://www.w3.org/2002/07/owl#Class"/>
	<rdfs:subClassOf rdf:resource="http://www.cidoc-crm.org/cidoc-crm/E31_Document"/>
	<rdfs:comment xml:lang="en">This class comprises encyclopaedia, thesauri, authority lists and other documents that define terminology or conceptual systems for consistent use.</rdfs:comment>
	<rdfs:label xml:lang="en">Authority Document</rdfs:label>
	<rdfs:label xml:lang="fr">Document de référence</rdfs:label>
	<rdfs:label xml:lang="pt">Documento de Referência</rdfs:label>
	<rdfs:label xml:lang="de">Referenzdokument</rdfs:label>
	<rdfs:label xml:lang="el">Πηγή Καθιερωμένων Όρων</rdfs:label>
	<rdfs:label xml:lang="ru">Официальный Документ</rdfs:label>
	<rdfs:label xml:lang="zh">规范文档</rdfs:label>
</rdf:Description>

<rdf:Description rdf:about="http://www.cidoc-crm.org/cidoc-crm/E33_E41_Linguistic_Appellation">
	<rdf:type rdf:resource="http://www.w3.org/2002/07/owl#Class"/>
	<rdfs:subClassOf rdf:resource="http://www.cidoc-crm.org/cidoc-crm/E33_Linguistic_Object"/>
	<rdfs:subClassOf rdf:resource="http://www.cidoc-crm.org/cidoc-crm/E41_Appellation"/>
	<rdfs:label xml:lang="en">Linguistic Appellation</rdfs:label>
</rdf:Description>

<rdf:Description rdf:about="http://www.cidoc-crm.org/cidoc-crm/E33_Linguistic_Object">
	<rdf:type rdf:resource="http://www.w3.org/2002/07/owl#Class"/>
	<rdfs:subClassOf rdf:resource="http://www.cidoc-crm.org/cidoc-crm/E73_Information_Object"/>
	<rdfs:comment xml:lang="en">This class comprises identifiable expressions in natural language or languages.
Instances of E33 Linguistic Object can be expressed in many ways: e.g. as written texts, recorded speech, or sign language. However, the CIDOC CRM treats instances of E33 Linguistic Object independently from the medium or method by which they are expressed. Expressions in formal languages, such as computer code or mathematical formulae, are not treated as instances of E33 Linguistic Object by the CIDOC CRM. These should be modelled as instances of E73 Information Object.
In general, an instance of E33 Linguistic Object may also contain non-linguistic information, often of artistic or aesthetic value. Only in cases in which the content of an instance of E33 Linguistic Object can completely be expressed by a series of binary-encoded symbols, its content may be documented within a respective knowledge base by the property P190 has symbolic content: E62 String. Otherwise, it should be understood as an identifiable digital resource only available independently from the respective knowledge base.
In other cases, such as pages of an illuminated manuscript or recordings containing speech in a language supported by a writing system, the linguistic part of the content of an instance of E33 Linguistic Object may be documented within a respective knowledge base in a note by P3 has note: E62 String. Otherwise, it may be described using the property P165 incorporates (is incorporated in): E73 Information Object as a different object with its own identity.</rdfs:comment>
	<rdfs:label xml:lang="en">Linguistic Object</rdfs:label>
	<rdfs:label xml:lang="fr">Objet linguistique</rdfs:label>
	<rdfs:label xml:lang="pt">Objeto Lingüístico</rdfs:label>
	<rdfs:label xml:lang="de">Sprachlicher Gegenstand</rdfs:label>
	<rdfs:label xml:lang="el">Γλωσσικό Αντικείμενο</rdfs:label>
	<rdfs:label xml:lang="ru">Линвистический Объект</rdfs:label>
	<rdfs:label xml:lang="zh">语言对象</rdfs:label>
</rdf:Description>

<rdf:Description rdf:about="http://www.cidoc-crm.org/cidoc-crm/E34_Inscription">
	<rdf:type rdf:resource="http://www.w3.org/2002/07/owl#Class"/>
	<rdfs:subClassOf rdf:resource="http://www.cidoc-crm.org/cidoc-crm/E33_Linguistic_Object"/>
	<rdfs:subClassOf rdf:resource="http://www.cidoc-crm.org/cidoc-crm/E37_Mark"/>
	<rdfs:comment xml:lang="en">This class comprises recognisable texts that can be attached to instances of E24 Physical Human-Made Thing.
The transcription of the text can be documented in a note by P3 has note: E62 String. The alphabet used can be documented by P2 has type: E55 Type. This class is not intended to describe the idiosyncratic characteristics of an individual physical embodiment of an inscription, but the underlying prototype. The physical embodiment is modelled in the CIDOC CRM as instances of E24 Physical Human-Made Thing.
The relationship of a physical copy of a book to the text it contains is modelled using E18 Physical Thing. P128 carries (is carried by): E33 Linguistic Object.</rdfs:comment>
	<rdfs:label xml:lang="de">Inschrift</rdfs:label>
	<rdfs:label xml:lang="en">Inscription</rdfs:label>
	<rdfs:label xml:lang="fr">Inscription</rdfs:label>
	<rdfs:label xml:lang="pt">Inscrição</rdfs:label>
	<rdfs:label xml:lang="el">Επιγραφή</rdfs:label>
	<rdfs:label xml:lang="ru">Надпись</rdfs:label>
	<rdfs:label xml:lang="zh">题识</rdfs:label>
</rdf:Description>

<rdf:Description rdf:about="http://www.cidoc-crm.org/cidoc-crm/E35_Title">
	<rdf:type rdf:resource="http://www.w3.org/2002/07/owl#Class"/>
	<rdfs:subClassOf rdf:resource="http://www.cidoc-crm.org/cidoc-crm/E33_Linguistic_Object"/>
	<rdfs:subClassOf rdf:resource="http://www.cidoc-crm.org/cidoc-crm/E41_Appellation"/>
	<rdfs:comment xml:lang="en">This class comprises the textual strings that within a cultural context can be clearly identified as titles due to their form. Being a subclass of E41 Appellation, E35 Title can only be used when such a string is actually used as a title of a work, such as a text, an artwork, or a piece of music.
Titles are proper noun phrases or verbal phrases, and should not be confused with generic object names such as “chair”, “painting”, or “book” (the latter are common nouns that stand for instances of E55 Type). Titles may be assigned by the creator of the work itself, or by a social group.
This class also comprises the translations of titles that are used as surrogates for the original titles in different social contexts.</rdfs:comment>
	<rdfs:label xml:lang="de">Titel</rdfs:label>
	<rdfs:label xml:lang="en">Title</rdfs:label>
	<rdfs:label xml:lang="fr">Titre</rdfs:label>
	<rdfs:label xml:lang="pt">Título</rdfs:label>
	<rdfs:label xml:lang="el">Τίτλος</rdfs:label>
	<rdfs:label xml:lang="ru">Заголовок</rdfs:label>
	<rdfs:label xml:lang="zh">题名</rdfs:label>
</rdf:Description>

<rdf:Description rdf:about="http://www.cidoc-crm.org/cidoc-crm/E36_Visual_Item">
	<rdf:type rdf:resource="http://www.w3.org/2002/07/owl#Class"/>
	<rdfs:subClassOf rdf:resource="http://www.cidoc-crm.org/cidoc-crm/E73_Information_Object"/>
	<rdfs:comment xml:lang="en">This class comprises the intellectual or conceptual aspects of recognisable marks and images.
This class does not intend to describe the idiosyncratic characteristics of an individual physical embodiment of a visual item, but the underlying prototype. For example, a mark such as the ICOM logo is generally considered to be the same logo when used on any number of publications. The size, orientation, and colour may change, but the logo remains uniquely identifiable. The same is true of images that are reproduced many times. This means that visual items are independent of their physical support.
The E36 Visual Item class provides a means of identifying and linking together instances of E24 Physical Human-Made Thing that carry the same visual symbols, marks, or images, etc. The property P62 depicts (is depicted by) between E24 Physical Human-Made Thing and the depicted subjects (E1 CRM Entity) can be regarded as a shortcut of the more fully developed path from E24 Physical Human-Made Thing through P65 shows visual item (is shown by), E36 Visual Item, P138 represents (has representation) to E1 CRM Entity, which in addition captures the optical features of the depiction.</rdfs:comment>
	<rdfs:label xml:lang="de">Bildliches</rdfs:label>
	<rdfs:label xml:lang="fr">Entité visuelle</rdfs:label>
	<rdfs:label xml:lang="pt">Item Visual</rdfs:label>
	<rdfs:label xml:lang="en">Visual Item</rdfs:label>
	<rdfs:label xml:lang="el">Οπτικό Στοιχείο</rdfs:label>
	<rdfs:label xml:lang="ru">Визуальный Предмет</rdfs:label>
	<rdfs:label xml:lang="zh">可视项</rdfs:label>
</rdf:Description>

<rdf:Description rdf:about="http://www.cidoc-crm.org/cidoc-crm/E37_Mark">
	<rdf:type rdf:resource="http://www.w3.org/2002/07/owl#Class"/>
	<rdfs:subClassOf rdf:resource="http://www.cidoc-crm.org/cidoc-crm/E36_Visual_Item"/>
	<rdfs:comment xml:lang="en">This class comprises symbols, signs, signatures, or short texts applied to instances of E24 Physical Human-Made Thing by arbitrary techniques, often in order to indicate such things as creator, owner, dedications, purpose, or to communicate information generally. Instances of E37 Mark do not represent the actual image of a mark, but the abstract ideal (or archetype) as used for codification in reference documents forming cultural documentation.
This class specifically excludes features that have no semantic significance, such as scratches or tool marks. These should be documented as instances of E25 Human-Made Feature.</rdfs:comment>
	<rdfs:label xml:lang="pt">Marca</rdfs:label>
	<rdfs:label xml:lang="en">Mark</rdfs:label>
	<rdfs:label xml:lang="de">Marke</rdfs:label>
	<rdfs:label xml:lang="fr">Marque</rdfs:label>
	<rdfs:label xml:lang="el">Σήμανση</rdfs:label>
	<rdfs:label xml:lang="ru">Пометка</rdfs:label>
	<rdfs:label xml:lang="zh">标记</rdfs:label>
</rdf:Description>

<rdf:Description rdf:about="http://www.cidoc-crm.org/cidoc-crm/E39_Actor">
	<rdf:type rdf:resource="http://www.w3.org/2002/07/owl#Class"/>
	<rdfs:subClassOf rdf:resource="http://www.cidoc-crm.org/cidoc-crm/E77_Persistent_Item"/>
	<rdfs:subClassOf rdf:resource="http://www.loa-cnr.it/ontologies/DOLCE-Lite#endurant"/>
	<rdfs:comment xml:lang="en">This class comprises people, either individually or in groups, who have the potential to perform intentional actions of kinds for which they can be held responsible.</rdfs:comment>
	<rdfs:label xml:lang="fr">Actant</rdfs:label>
	<rdfs:label xml:lang="en">Actor</rdfs:label>
	<rdfs:label xml:lang="pt">Agente</rdfs:label>
	<rdfs:label xml:lang="de">Akteur</rdfs:label>
	<rdfs:label xml:lang="el">Δράστης</rdfs:label>
	<rdfs:label xml:lang="ru">Агент</rdfs:label>
	<rdfs:label xml:lang="zh">参与者</rdfs:label>
</rdf:Description>

<rdf:Description rdf:about="http://www.cidoc-crm.org/cidoc-crm/E3_Condition_State">
	<rdf:type rdf:resource="http://www.w3.org/2002/07/owl#Class"/>
	<rdfs:subClassOf rdf:resource="http://www.cidoc-crm.org/cidoc-crm/E2_Temporal_Entity"/>
	<rdfs:comment xml:lang="en">This class comprises the states of objects characterised by a certain condition over a time-span.
An instance of this class describes the prevailing physical condition of any material object or feature during a specific instance of E52 Time-Span. In general, the time-span for which a certain condition can be asserted may be shorter than the real time-span, for which this condition held.
The nature of that condition can be described using P2 has type. For example, the instance of E3 Condition State “condition of the SS Great Britain between 22-nd September 1846 and 27-th August 1847” can be characterized as an instance “wrecked” of E55 Type.</rdfs:comment>
	<rdfs:label xml:lang="en">Condition State</rdfs:label>
	<rdfs:label xml:lang="pt">Estado Material</rdfs:label>
	<rdfs:label xml:lang="de">Zustandsphase</rdfs:label>
	<rdfs:label xml:lang="fr">État matériel</rdfs:label>
	<rdfs:label xml:lang="el">Κατάσταση</rdfs:label>
	<rdfs:label xml:lang="ru">Состояние</rdfs:label>
	<rdfs:label xml:lang="zh">条件状态</rdfs:label>
</rdf:Description>

<rdf:Description rdf:about="http://www.cidoc-crm.org/cidoc-crm/E41_Appellation">
	<rdf:type rdf:resource="http://www.w3.org/2002/07/owl#Class"/>
	<rdfs:subClassOf rdf:resource="http://www.cidoc-crm.org/cidoc-crm/E90_Symbolic_Object"/>
	<rdfs:comment xml:lang="en">This class comprises all signs, either meaningful or not, or arrangements of signs following a specific syntax, that are used or can be used to refer to and identify a specific instance of some class within a certain context.
Instances of E41 Appellation do not identify things by their meaning, even if they happen to have one, but by convention, tradition, or agreement. Instances of E41 Appellation are cultural constructs; as such, they have a context, a history, and a use in time and space by some group of users. A given instance of E41 Appellation can have alternative forms, i.e. other instances of E41 Appellation that are regarded as equivalent, regardless of the thing it denotes.
Different languages may use different appellations for the same thing, such as the names of major cities. Some appellations may be formulated using a valid noun phrase of a particular language. In these cases, the respective instances of E41 Appellation should also be declared as instances of E33 Linguistic Object. Then the language using the appellation can be declared with the property P72 has language: E56 Language.
Instances of E41 Appellation may be used to identify any instance of E1 CRM Entity and sometimes are characteristic for instances of more specific subclasses of E1 CRM Entity, such as for instances of E52 Time-Span (for instance “dates”), E39 Actor, E53 Place or E28 Conceptual Object. Postal addresses and E-mail addresses are characteristic examples of identifiers used by services transporting things between clients.
Even numerically expressed identifiers for extents in space or time are also regarded as instances of E41 Appellation, such as Gregorian dates or spatial coordinates, even though they allow for determining some time or location by a known procedure starting from a reference point and by virtue of that fact play a double role as instances of E59 Primitive Value.
E41 Appellation should not be confused with the act of naming something. Cf. E15 Identifier Assignment.</rdfs:comment>
	<rdfs:label xml:lang="en">Appellation</rdfs:label>
	<rdfs:label xml:lang="fr">Appellation</rdfs:label>
	<rdfs:label xml:lang="de">Benennung</rdfs:label>
	<rdfs:label xml:lang="pt">Designação</rdfs:label>
	<rdfs:label xml:lang="el">Ονομασία</rdfs:label>
	<rdfs:label xml:lang="ru">Обозначение</rdfs:label>
	<rdfs:label xml:lang="zh">称谓</rdfs:label>
</rdf:Description>

<rdf:Description rdf:about="http://www.cidoc-crm.org/cidoc-crm/E42_Identifier">
	<rdf:type rdf:resource="http://www.w3.org/2002/07/owl#Class"/>
	<rdfs:subClassOf rdf:resource="http://www.cidoc-crm.org/cidoc-crm/E41_Appellation"/>
	<rdfs:comment xml:lang="en">This class comprises strings or codes assigned to instances of E1 CRM Entity in order to identify them uniquely and permanently within the context of one or more organisations. Such codes are often known as inventory numbers, registration codes, etc. and are typically composed of alphanumeric sequences. Postal addresses, telephone numbers, URLs and e-mail addresses are characteristic examples of identifiers used by services transporting things between clients.
The class E42 Identifier is not normally used for machine-generated identifiers used for automated processing unless these are also used by human agents.</rdfs:comment>
	<rdfs:label xml:lang="fr">Identifiant</rdfs:label>
	<rdfs:label xml:lang="pt">Identificador de Objeto</rdfs:label>
	<rdfs:label xml:lang="en">Identifier</rdfs:label>
	<rdfs:label xml:lang="de">Kennung</rdfs:label>
	<rdfs:label xml:lang="el">Κωδικός Αναγνώρισης</rdfs:label>
	<rdfs:label xml:lang="ru">Идентификатор Объекта</rdfs:label>
	<rdfs:label xml:lang="zh">标识符</rdfs:label>
</rdf:Description>

<rdf:Description rdf:about="http://www.cidoc-crm.org/cidoc-crm/E4_Period">
	<rdf:type rdf:resource="http://www.w3.org/2002/07/owl#Class"/>
	<rdfs:subClassOf rdf:resource="http://www.cidoc-crm.org/cidoc-crm/E2_Temporal_Entity"/>
	<rdfs:subClassOf rdf:resource="http://www.cidoc-crm.org/cidoc-crm/E92_Spacetime_Volume"/>
	<rdfs:comment xml:lang="en">This class comprises sets of coherent phenomena or cultural manifestations occurring in time and space.
It is the social or physical coherence of these phenomena that identify an instance of E4 Period and not the associated spatiotemporal extent. This extent is only the “ground” or space in an abstract physical sense that the actual process of growth, spread and retreat has covered. Consequently, different periods can overlap and coexist in time and space, such as when a nomadic culture exists in the same area and time as a sedentary culture. This also means that overlapping land use rights, common among first nations, amounts to overlapping periods.
Often, this class is used to describe prehistoric or historic periods such as the “Neolithic Period”, the “Ming Dynasty” or the “McCarthy Era”, but also geopolitical units and activities of settlements are regarded as special cases of E4 Period. However, there are no assumptions about the scale of the associated phenomena. In particular all events are seen as synthetic processes consisting of coherent phenomena. Therefore, E4 Period is a superclass of E5 Event. For example, a modern clinical birth, an instance of E67 Birth, can be seen as both a single event, i.e. an instance of E5 Event, and as an extended period, i.e. an instance of E4 Period, that consists of multiple physical processes and complementary activities performed by multiple instances of E39 Actor.
E4 Period is a subclass of E2 Temporal Entity and of E92 Spacetime Volume. The latter is intended as a phenomenal spacetime volume as defined in CIDOC CRMgeo (Doerr &amp;amp; Hiebel, 2013). By virtue of this multiple inheritance, it is possible to discuss the physical extent of an instance of E4 Period without representing each instance of it together with an instance of its associated spacetime volume. This model combines two quite different kinds of substance: an instance of E4 Period is a phenomenon while an instance of E92 Spacetime Volume is an aggregation of points in spacetime. However, the real spatiotemporal extent of an instance of E4 Period is regarded to be unique to it due to all its details and fuzziness; its identity and existence depends uniquely on the identity of the instance of E4 Period. Therefore, this multiple inheritance is unambiguous and effective and furthermore corresponds to the intuitions of natural language.
Typical use of this class in cultural heritage documentation is for documenting cultural and artistic periods. There are two different conceptualisations of ‘artistic style’, defined either by physical features or by historical context. For example, “Impressionism” can be viewed as a period in the European sphere of influence lasting from approximately 1870 to 1905 during which paintings with particular characteristics were produced by a group of artists that included (among others) Monet, Renoir, Pissarro, Sisley and Degas. Alternatively, it can be regarded as a style applicable to all paintings sharing the characteristics of the works produced by the Impressionist painters, regardless of historical context. The first interpretation is an instance of E4 Period, and the second defines morphological object types that fall under E55 Type.
A geopolitical unit as a specific case of an instance of E4 Period is the set of activities and phenomena related to the claim of power, the consequences of belonging to a jurisdictional area and an administrative system that establishes a geopolitical unit. Examples from the modern period are countries or administrative areas of countries such as districts whose actions and structures define activities and phenomena in the area that they intend to govern. The borders of geopolitical units are often defined in contracts or treaties although they may deviate from the actual practice. The spatiotemporal properties of Geopolitical units can be modelled through the properties inherited from E92 Spacetime Volume.
Another specific case of an instance of E4 Period is the actual extent of the set of activities and phenomena as evidenced by their physical traces that define a settlement, such as the populated period of Nineveh.</rdfs:comment>
	<rdfs:label xml:lang="en">Period</rdfs:label>
	<rdfs:label xml:lang="pt">Período</rdfs:label>
	<rdfs:label xml:lang="de">Phase</rdfs:label>
	<rdfs:label xml:lang="fr">Période</rdfs:label>
	<rdfs:label xml:lang="el">Περίοδος</rdfs:label>
	<rdfs:label xml:lang="ru">Период</rdfs:label>
	<rdfs:label xml:lang="zh">时期</rdfs:label>
</rdf:Description>

<rdf:Description rdf:about="http://www.cidoc-crm.org/cidoc-crm/E52_Time-Span">
	<rdf:type rdf:resource="http://www.w3.org/2002/07/owl#Class"/>
	<rdfs:subClassOf rdf:resource="http://www.cidoc-crm.org/cidoc-crm/E1_CRM_Entity"/>
	<rdfs:comment xml:lang="en">This class comprises abstract temporal extents, in the sense of Galilean physics, having a beginning, an end, and a duration.
Instances of E52 Time-Span have no semantic connotations about phenomena happening within the temporal extent they represent. They do not convey any meaning other than a positioning on the “time-line” of chronology. The actual extent of an instance of E52 Time-Span can be approximated by properties of E52 Time-Span giving inner and outer bounds in the form of dates (instances of E61 Time Primitive). Comparing knowledge about time-spans is fundamental for chronological reasoning.
Some instances of E52 Time-Span may be defined as the actual, in principle observable, temporal extent of instances of E2 Temporal Entity via the property P4 has time-span (is time-span of): E52 Time-Span. They constitute phenomenal time-spans as defined in CRMgeo (Doerr &amp;amp; Hiebel 2013). Since our knowledge of history is imperfect and physical phenomena are fuzzy in nature, the extent of phenomenal time-spans can only be described in approximation. An extreme case of approximation, might, for example, define an instance of E52 Time-Span having unknown beginning, end and duration. It may, nevertheless, be associated with other descriptions by which people can infer knowledge about it, such as in relative chronologies.
Some instances of E52 may be defined precisely as representing a declaration of a temporal extent, as, for instance, done in a business contract. They constitute declarative time-spans as defined in CRMgeo (Doerr &amp;amp; Hiebel 2013) and can be described via the property E61 Time Primitive P170 defines time (time is defined by): E52 Time-Span.
When used as a common E52 Time-Span for two events, it will nevertheless describe them as being simultaneous, even if nothing else is known.</rdfs:comment>
	<rdfs:label xml:lang="fr">Intervalle temporel</rdfs:label>
	<rdfs:label xml:lang="pt">Período de Tempo</rdfs:label>
	<rdfs:label xml:lang="en">Time-Span</rdfs:label>
	<rdfs:label xml:lang="de">Zeitspanne</rdfs:label>
	<rdfs:label xml:lang="el">Χρονικό Διάστημα</rdfs:label>
	<rdfs:label xml:lang="ru">Интервал Времени</rdfs:label>
	<rdfs:label xml:lang="zh">时段</rdfs:label>
</rdf:Description>

<rdf:Description rdf:about="http://www.cidoc-crm.org/cidoc-crm/E53_Place">
	<rdf:type rdf:resource="http://www.w3.org/2002/07/owl#Class"/>
	<rdfs:subClassOf rdf:resource="http://www.cidoc-crm.org/cidoc-crm/E1_CRM_Entity"/>
	<rdfs:comment>E53 Place refers to an abstract location or position. It represents the spatial area associated with a geographical location, such as a town or city, but not the physical structures within that area. For example, while traveling, one might refer to the position of a town as an E53 Place, but the town itself, with its buildings and streets, is not an E53 Place.</rdfs:comment>
	<rdfs:comment xml:lang="en">This class comprises extents in the natural space where people live, in particular on the surface of the Earth, in the pure sense of physics: independent from temporal phenomena and matter. They may serve describing the physical location of things or phenomena or other areas of interest. Geometrically, instances of E53 Place constitute single contiguous areas or a finite aggregation of disjoint areas in space which are each individually contiguous. They may have fuzzy boundaries.
The instances of E53 Place are usually determined by reference to the position of “immobile” objects such as buildings, cities, mountains, rivers, or dedicated geodetic marks, but may also be determined by reference to mobile objects. A Place can be determined by combining a frame of reference and a location with respect to this frame.
It is sometimes argued that instances of E53 Place are best identified by global coordinates or absolute reference systems. However, relative references are often more relevant in the context of cultural documentation and tend to be more precise. In particular, people are often interested in position in relation to large, mobile objects, such as ships. For example, the Place at which Nelson died is known with reference to a large mobile object, i.e. H.M.S Victory. A resolution of this Place in terms of absolute coordinates would require knowledge of the movements of the vessel and the precise time of death, either of which may be revised, and the result would lack historical and cultural relevance.
Any instance of E18 Physical Thing can serve as a frame of reference for an instance of E53 Place. This may be documented using the property P157 is at rest relative to (provides reference space for).</rdfs:comment>
	<rdfs:label xml:lang="fr">Lieu</rdfs:label>
	<rdfs:label xml:lang="pt">Local</rdfs:label>
	<rdfs:label xml:lang="de">Ort</rdfs:label>
	<rdfs:label xml:lang="en">Place</rdfs:label>
	<rdfs:label xml:lang="el">Τόπος</rdfs:label>
	<rdfs:label xml:lang="ru">Место</rdfs:label>
	<rdfs:label xml:lang="zh">地点</rdfs:label>
</rdf:Description>

<rdf:Description rdf:about="http://www.cidoc-crm.org/cidoc-crm/E54_Dimension">
	<rdf:type rdf:resource="http://www.w3.org/2002/07/owl#Class"/>
	<rdfs:subClassOf rdf:resource="http://www.cidoc-crm.org/cidoc-crm/E1_CRM_Entity"/>
	<rdfs:comment xml:lang="en">This class comprises quantifiable properties that can be measured by some calibrated means and can be approximated by values, i.e. points or regions in a mathematical or conceptual space, such as natural or real numbers, RGB values, etc.
An instance of E54 Dimension represents the empirical or theoretically derived quantity, including the precision tolerances resulting from the particular method or calculation. The identity of an instance of E54 Dimension depends on the method of its determination because each method may produce different values even when determining comparable qualities. For instance, the wingspan of a bird alive or dead is a different dimension. Thermoluminescence dating and Rehydroxylation [RHX] dating are different dimensions of temporal distance from now, even if they aim at dating the same object. The method of determination should be expressed using the property P2 has type (is type of). Note that simple terms such as “diameter” or “length” are normally insufficient to unambiguously describe a respective dimension. In contrast, “maximum linear extent” may be sufficient.
The properties of the class E54 Dimension allow for expressing the numerical approximation of the values of instances of E54 Dimension adequate to the precision of the applied method of determination. If the respective quantity belongs to a non-discrete space according to the laws of physics, such as spatial distances, it is recommended to record them as approximations by intervals or regions of indeterminacy enclosing the assumed true values. For instance, a length of 5 cm may be recorded as 4.5-5.5 cm, according to the precision of the respective observation. Note, that comparability of values described in different units depends critically on the representation as value regions.
Numerical approximations in archaic instances of E58 Measurement Unit used in historical records should be preserved. Equivalents corresponding to current knowledge should be recorded as additional instances of E54 Dimension, as appropriate.</rdfs:comment>
	<rdfs:label xml:lang="en">Dimension</rdfs:label>
	<rdfs:label xml:lang="fr">Dimension</rdfs:label>
	<rdfs:label xml:lang="pt">Dimensão</rdfs:label>
	<rdfs:label xml:lang="de">Maß</rdfs:label>
	<rdfs:label xml:lang="el">Μέγεθος</rdfs:label>
	<rdfs:label xml:lang="ru">Величина</rdfs:label>
	<rdfs:label xml:lang="zh">度量规格</rdfs:label>
</rdf:Description>

<rdf:Description rdf:about="http://www.cidoc-crm.org/cidoc-crm/E55_Type">
	<rdf:type rdf:resource="http://www.w3.org/2002/07/owl#Class"/>
	<rdfs:subClassOf rdf:resource="http://www.cidoc-crm.org/cidoc-crm/E28_Conceptual_Object"/>
	<rdfs:comment xml:lang="en">This class comprises concepts denoted by terms from thesauri and controlled vocabularies used to characterize and classify instances of CIDOC CRM classes. Instances of E55 Type represent concepts, in contrast to instances of E41 Appellation which are used to name instances of CIDOC CRM classes.
E55 Type provides an interface to domain specific ontologies and thesauri. These can be represented in the CIDOC CRM as subclasses of E55 Type, forming hierarchies of terms, i.e. instances of E55 Type linked via P127 has broader term (has narrower term): E55 Type. Such hierarchies may be extended with additional properties.</rdfs:comment>
	<rdfs:label xml:lang="pt">Tipo</rdfs:label>
	<rdfs:label xml:lang="en">Type</rdfs:label>
	<rdfs:label xml:lang="fr">Type</rdfs:label>
	<rdfs:label xml:lang="de">Typus</rdfs:label>
	<rdfs:label xml:lang="el">Τύπος</rdfs:label>
	<rdfs:label xml:lang="ru">Тип</rdfs:label>
	<rdfs:label xml:lang="zh">类型</rdfs:label>
</rdf:Description>

<rdf:Description rdf:about="http://www.cidoc-crm.org/cidoc-crm/E56_Language">
	<rdf:type rdf:resource="http://www.w3.org/2002/07/owl#Class"/>
	<rdfs:subClassOf rdf:resource="http://www.cidoc-crm.org/cidoc-crm/E55_Type"/>
	<rdfs:comment xml:lang="en">This class is a specialization of E55 Type and comprises the natural languages in the sense of concepts.
This type is used categorically in the model without reference to instances of it, i.e. the Model does not foresee the description of instances of instances of E56 Language, e.g. “instances of Mandarin Chinese”.
It is recommended that internationally or nationally agreed codes and terminology should be used to denote instances of E56 Language, such as those defined in ISO 639-3:2007 and later versions.</rdfs:comment>
	<rdfs:label xml:lang="en">Language</rdfs:label>
	<rdfs:label xml:lang="fr">Langue</rdfs:label>
	<rdfs:label xml:lang="pt">Língua</rdfs:label>
	<rdfs:label xml:lang="de">Sprache</rdfs:label>
	<rdfs:label xml:lang="el">Γλώσσα</rdfs:label>
	<rdfs:label xml:lang="ru">Язык</rdfs:label>
	<rdfs:label xml:lang="zh">语种</rdfs:label>
</rdf:Description>

<rdf:Description rdf:about="http://www.cidoc-crm.org/cidoc-crm/E57_Material">
	<rdf:type rdf:resource="http://www.w3.org/2002/07/owl#Class"/>
	<rdfs:subClassOf rdf:resource="http://www.cidoc-crm.org/cidoc-crm/E55_Type"/>
	<rdfs:comment xml:lang="en">This class is a specialization of E55 Type and comprises the concepts of materials.
Instances of E57 Material may denote properties of matter before its use, during its use, and as incorporated in an object, such as ultramarine powder, tempera paste, reinforced concrete. Discrete pieces of raw-materials kept in museums, such as bricks, sheets of fabric, pieces of metal, should be modelled individually in the same way as other objects. Discrete used or processed pieces, such as the stones from Nefer Titi's temple, should be modelled as parts (cf. P46 is composed of (forms part of): E18 Physical Thing).
This type is used categorically in the model without reference to instances of it, i.e. the Model does not foresee the description of instances of instances of E57 Material, e.g. “instances of gold”.
It is recommended that internationally or nationally agreed codes and terminology should be used.</rdfs:comment>
	<rdfs:label xml:lang="de">Material</rdfs:label>
	<rdfs:label xml:lang="en">Material</rdfs:label>
	<rdfs:label xml:lang="pt">Material</rdfs:label>
	<rdfs:label xml:lang="fr">Matériau</rdfs:label>
	<rdfs:label xml:lang="el">Υλικό</rdfs:label>
	<rdfs:label xml:lang="ru">Материал</rdfs:label>
	<rdfs:label xml:lang="zh">材质</rdfs:label>
</rdf:Description>

<rdf:Description rdf:about="http://www.cidoc-crm.org/cidoc-crm/E58_Measurement_Unit">
	<rdf:type rdf:resource="http://www.w3.org/2002/07/owl#Class"/>
	<rdfs:subClassOf rdf:resource="http://www.cidoc-crm.org/cidoc-crm/E55_Type"/>
	<rdfs:comment xml:lang="en">This class is a specialization of E55 Type and comprises the types of measurement units: feet, inches, centimetres, litres, lumens, etc.
This type is used categorically in the model without reference to instances of it, i.e. the model does not foresee the description of instances of instances of E58 Measurement Unit, e.g. “instances of cm”.
Système International (SI) units or internationally recognized non-SI terms should be used whenever possible, such as those defined by ISO80000:2009. Archaic Measurement Units used in historical records should be preserved.</rdfs:comment>
	<rdfs:label xml:lang="de">Maßeinheit</rdfs:label>
	<rdfs:label xml:lang="en">Measurement Unit</rdfs:label>
	<rdfs:label xml:lang="pt">Unidade de Medida</rdfs:label>
	<rdfs:label xml:lang="fr">Unité de mesure</rdfs:label>
	<rdfs:label xml:lang="el">Μονάδα Μέτρησης</rdfs:label>
	<rdfs:label xml:lang="ru">Единица Измерения</rdfs:label>
	<rdfs:label xml:lang="zh">测量单位</rdfs:label>
</rdf:Description>

<rdf:Description rdf:about="http://www.cidoc-crm.org/cidoc-crm/E5_Event">
	<rdf:type rdf:resource="http://www.w3.org/2002/07/owl#Class"/>
	<rdfs:subClassOf rdf:resource="http://www.cidoc-crm.org/cidoc-crm/E4_Period"/>
	<rdfs:comment xml:lang="en">This class comprises distinct, delimited and coherent processes and interactions of a material nature, in cultural, social or physical systems, involving and affecting instances of E77 Persistent Item in a way characteristic of the kind of process. Typical examples are meetings, births, deaths, actions of decision taking, making or inventing things, but also more complex and extended ones such as conferences, elections, building of a castle, or battles.
While the continuous growth of a tree lacks the limits characteristic of an event, its germination from a seed does qualify as an event. Similarly, the blowing of the wind lacks the distinctness and limits of an event, but a hurricane, flood or earthquake would qualify as an event. Mental processes are considered as events, in cases where they are connected with the material externalization of their results; for example, the creation of a poem, a performance or a change of intention that becomes obvious from subsequent actions or declarations.
The effects of an instance of E5 Event may not lead to relevant permanent changes of properties or relations of the items involved in it, for example an unrecorded performance. Of course, in order to be documented, some kind of evidence for an event must exist, be it witnesses, traces or products of the event.
While instances of E4 Period always require some form of coherence between its constituent phenomena, in addition, the essential constituents of instances of E5 Event should contribute to an overall effect; for example, the statements made during a meeting and the listening of the audience.
Viewed at a coarse level of detail, an instance of E5 Event may appear as if it had an ‘instantaneous’ overall effect, but any process or interaction of material nature in reality have an extent in time and space. At a fine level, instances of E5 Event may be analysed into component phenomena and phases within a space and timeframe, and as such can be seen as a period, regardless of the size of the phenomena. The reverse is not necessarily the case: not all instances of E4 Period give rise to a noteworthy overall effect and are thus not instances of E5 Event.</rdfs:comment>
	<rdfs:label xml:lang="de">Ereignis</rdfs:label>
	<rdfs:label xml:lang="en">Event</rdfs:label>
	<rdfs:label xml:lang="pt">Evento</rdfs:label>
	<rdfs:label xml:lang="fr">Évènement</rdfs:label>
	<rdfs:label xml:lang="el">Συμβάν</rdfs:label>
	<rdfs:label xml:lang="ru">Событие</rdfs:label>
	<rdfs:label xml:lang="zh">事件</rdfs:label>
</rdf:Description>

<rdf:Description rdf:about="http://www.cidoc-crm.org/cidoc-crm/E63_Beginning_of_Existence">
	<rdf:type rdf:resource="http://www.w3.org/2002/07/owl#Class"/>
	<rdfs:subClassOf rdf:resource="http://www.cidoc-crm.org/cidoc-crm/E5_Event"/>
	<rdfs:comment xml:lang="en">This class comprises events that bring into existence any instance of E77 Persistent Item.
It may be used for temporal reasoning about things (intellectual products, physical items, groups of people, living beings) beginning to exist; it serves as a hook for both a terminus post quem and a terminus ante quem.</rdfs:comment>
	<rdfs:label xml:lang="en">Beginning of Existence</rdfs:label>
	<rdfs:label xml:lang="de">Daseinsbeginn</rdfs:label>
	<rdfs:label xml:lang="fr">Début d’existence</rdfs:label>
	<rdfs:label xml:lang="pt">Início da Existência</rdfs:label>
	<rdfs:label xml:lang="el">Αρχή Ύπαρξης</rdfs:label>
	<rdfs:label xml:lang="ru">Начало Существования</rdfs:label>
	<rdfs:label xml:lang="zh">初始</rdfs:label>
</rdf:Description>

<rdf:Description rdf:about="http://www.cidoc-crm.org/cidoc-crm/E64_End_of_Existence">
	<rdf:type rdf:resource="http://www.w3.org/2002/07/owl#Class"/>
	<rdfs:subClassOf rdf:resource="http://www.cidoc-crm.org/cidoc-crm/E5_Event"/>
	<rdfs:comment xml:lang="en">This class comprises events that end the existence of any instance of E77 Persistent Item.
It may be used for temporal reasoning about things (physical items, groups of people, living beings) ceasing to exist; it serves as a hook both a terminus post quem and a terminus ante quem. In cases where substance from an instance of E77 Persistent Item continues to exist in a new form, the process would be documented as instances of E81 Transformation.</rdfs:comment>
	<rdfs:label xml:lang="de">Daseinsende</rdfs:label>
	<rdfs:label xml:lang="en">End of Existence</rdfs:label>
	<rdfs:label xml:lang="pt">Fim da Existência</rdfs:label>
	<rdfs:label xml:lang="fr">Fin d’existence</rdfs:label>
	<rdfs:label xml:lang="el">Τέλος Ύπαρξης</rdfs:label>
	<rdfs:label xml:lang="ru">Конец Существования</rdfs:label>
	<rdfs:label xml:lang="zh">结束</rdfs:label>
</rdf:Description>

<rdf:Description rdf:about="http://www.cidoc-crm.org/cidoc-crm/E65_Creation">
	<rdf:type rdf:resource="http://www.w3.org/2002/07/owl#Class"/>
	<rdfs:subClassOf rdf:resource="http://www.cidoc-crm.org/cidoc-crm/E63_Beginning_of_Existence"/>
	<rdfs:subClassOf rdf:resource="http://www.cidoc-crm.org/cidoc-crm/E7_Activity"/>
	<rdfs:comment xml:lang="en">This class comprises events that result in the creation of conceptual items or immaterial products, such as legends, poems, texts, music, images, movies, laws, types, etc.</rdfs:comment>
	<rdfs:label xml:lang="de">Begriffliche Schöpfung</rdfs:label>
	<rdfs:label xml:lang="en">Creation</rdfs:label>
	<rdfs:label xml:lang="pt">Criação</rdfs:label>
	<rdfs:label xml:lang="fr">Création</rdfs:label>
	<rdfs:label xml:lang="el">Δημιουργία</rdfs:label>
	<rdfs:label xml:lang="ru">Событие Творения</rdfs:label>
	<rdfs:label xml:lang="zh">创建</rdfs:label>
</rdf:Description>

<rdf:Description rdf:about="http://www.cidoc-crm.org/cidoc-crm/E66_Formation">
	<rdf:type rdf:resource="http://www.w3.org/2002/07/owl#Class"/>
	<rdfs:subClassOf rdf:resource="http://www.cidoc-crm.org/cidoc-crm/E63_Beginning_of_Existence"/>
	<rdfs:subClassOf rdf:resource="http://www.cidoc-crm.org/cidoc-crm/E7_Activity"/>
	<rdfs:comment xml:lang="en">This class comprises events that result in the formation of a formal or informal E74 Group of people, such as a club, society, association, corporation, or nation.
E66 Formation does not include the arbitrary aggregation of people who do not act as a collective.
The formation of an instance of E74 Group does not require that the group is populated with members at the time of formation. In order to express the joining of members at the time of formation, the respective activity should be simultaneously an instance of both E66 Formation and E85 Joining.</rdfs:comment>
	<rdfs:label xml:lang="en">Formation</rdfs:label>
	<rdfs:label xml:lang="fr">Formation</rdfs:label>
	<rdfs:label xml:lang="pt">Formação</rdfs:label>
	<rdfs:label xml:lang="de">Gruppenbildung</rdfs:label>
	<rdfs:label xml:lang="el">Συγκρότηση Ομάδας</rdfs:label>
	<rdfs:label xml:lang="ru">Событие Формирования</rdfs:label>
	<rdfs:label xml:lang="zh">组成</rdfs:label>
</rdf:Description>

<rdf:Description rdf:about="http://www.cidoc-crm.org/cidoc-crm/E67_Birth">
	<rdf:type rdf:resource="http://www.w3.org/2002/07/owl#Class"/>
	<rdfs:subClassOf rdf:resource="http://www.cidoc-crm.org/cidoc-crm/E63_Beginning_of_Existence"/>
	<rdfs:comment xml:lang="en">This class comprises the births of human beings. E67 Birth is a biological event focussing on the context of people coming into life. (E63 Beginning of Existence comprises the coming into life of any living being.)
Twins, triplets, etc. are brought into life by the same instance of E67 Birth. The introduction of the E67 Birth event as a documentation element allows the description of a range of family relationships in a simple model. Suitable extensions may describe more details and the complexity of motherhood since the advent of modern medicine. In this model, the biological father is not seen as a necessary participant in the E67 Birth.</rdfs:comment>
	<rdfs:label xml:lang="en">Birth</rdfs:label>
	<rdfs:label xml:lang="de">Geburt</rdfs:label>
	<rdfs:label xml:lang="fr">Naissance</rdfs:label>
	<rdfs:label xml:lang="pt">Nascimento</rdfs:label>
	<rdfs:label xml:lang="el">Γέννηση</rdfs:label>
	<rdfs:label xml:lang="ru">Рождение</rdfs:label>
	<rdfs:label xml:lang="zh">出生</rdfs:label>
</rdf:Description>

<rdf:Description rdf:about="http://www.cidoc-crm.org/cidoc-crm/E68_Dissolution">
	<rdf:type rdf:resource="http://www.w3.org/2002/07/owl#Class"/>
	<rdfs:subClassOf rdf:resource="http://www.cidoc-crm.org/cidoc-crm/E64_End_of_Existence"/>
	<rdfs:comment xml:lang="en">This class comprises the events that result in the formal or informal termination of an instance of E74 Group.
If the dissolution was deliberate, the Dissolution event should also be instantiated as an instance of E7 Activity.</rdfs:comment>
	<rdfs:label xml:lang="en">Dissolution</rdfs:label>
	<rdfs:label xml:lang="fr">Dissolution</rdfs:label>
	<rdfs:label xml:lang="pt">Dissolução</rdfs:label>
	<rdfs:label xml:lang="de">Gruppenauflösung</rdfs:label>
	<rdfs:label xml:lang="el">Διάλυση Ομάδας</rdfs:label>
	<rdfs:label xml:lang="ru">Роспуск</rdfs:label>
	<rdfs:label xml:lang="zh">解散</rdfs:label>
</rdf:Description>

<rdf:Description rdf:about="http://www.cidoc-crm.org/cidoc-crm/E69_Death">
	<rdf:type rdf:resource="http://www.w3.org/2002/07/owl#Class"/>
	<rdfs:subClassOf rdf:resource="http://www.cidoc-crm.org/cidoc-crm/E64_End_of_Existence"/>
	<rdfs:comment xml:lang="en">This class comprises the deaths of human beings.
If a person is killed, their death should be instantiated as E69 Death and as E7 Activity. The death or perishing of other living beings should be documented as instances of E64 End of Existence.</rdfs:comment>
	<rdfs:label xml:lang="en">Death</rdfs:label>
	<rdfs:label xml:lang="fr">Mort</rdfs:label>
	<rdfs:label xml:lang="pt">Morte</rdfs:label>
	<rdfs:label xml:lang="de">Tod</rdfs:label>
	<rdfs:label xml:lang="el">Θάνατος</rdfs:label>
	<rdfs:label xml:lang="ru">Смерть</rdfs:label>
	<rdfs:label xml:lang="zh">死亡</rdfs:label>
</rdf:Description>

<rdf:Description rdf:about="http://www.cidoc-crm.org/cidoc-crm/E6_Destruction">
	<rdf:type rdf:resource="http://www.w3.org/2002/07/owl#Class"/>
	<rdfs:subClassOf rdf:resource="http://www.cidoc-crm.org/cidoc-crm/E64_End_of_Existence"/>
	<rdfs:comment xml:lang="en">This class comprises events that destroy one or more instances of E18 Physical Thing, such that they lose their identity as the subjects of documentation.
Some destruction events are intentional, while others are independent of human activity. Intentional destruction can be documented by classifying the event as both an instance of E6 Destruction and of E7 Activity.
The decision to document an object as destroyed, transformed, or modified is context-sensitive:
1. If the matter remaining from the destruction is not documented, the event is modelled solely as an instance of E6 Destruction.
2. An event should also be documented using E81 Transformation if it results in the destruction of one or more objects and the simultaneous production of others using parts or material from the original. In this case, the new items have separate identities. Matter is preserved, but identity is not.
3. When the initial identity of the changed instance of E18 Physical Thing is preserved, the event should be documented as an instance of E11 Modification.</rdfs:comment>
	<rdfs:label xml:lang="en">Destruction</rdfs:label>
	<rdfs:label xml:lang="fr">Destruction</rdfs:label>
	<rdfs:label xml:lang="pt">Destruição</rdfs:label>
	<rdfs:label xml:lang="de">Zerstörung</rdfs:label>
	<rdfs:label xml:lang="el">Καταστροφή</rdfs:label>
	<rdfs:label xml:lang="ru">Разрушение</rdfs:label>
	<rdfs:label xml:lang="zh">破坏</rdfs:label>
</rdf:Description>

<rdf:Description rdf:about="http://www.cidoc-crm.org/cidoc-crm/E70_Thing">
	<rdf:type rdf:resource="http://www.w3.org/2002/07/owl#Class"/>
	<rdfs:subClassOf rdf:resource="http://www.cidoc-crm.org/cidoc-crm/E77_Persistent_Item"/>
	<rdfs:subClassOf rdf:resource="http://www.loa-cnr.it/ontologies/DOLCE-Lite#endurant"/>
	<rdfs:comment xml:lang="en">This general class comprises discrete, identifiable, instances of E77 Persistent Item that are documented as single units, that either consist of matter or depend on being carried by matter and are characterized by relative stability.
They may be intellectual products or physical things. They may, for instance, have a solid physical form, an electronic encoding, or they may be a logical concept or structure.</rdfs:comment>
	<rdfs:label xml:lang="fr">Chose</rdfs:label>
	<rdfs:label xml:lang="pt">Coisa</rdfs:label>
	<rdfs:label xml:lang="de">Sache</rdfs:label>
	<rdfs:label xml:lang="en">Thing</rdfs:label>
	<rdfs:label xml:lang="el">Πράγμα</rdfs:label>
	<rdfs:label xml:lang="ru">Вещь</rdfs:label>
	<rdfs:label xml:lang="zh">事物</rdfs:label>
</rdf:Description>

<rdf:Description rdf:about="http://www.cidoc-crm.org/cidoc-crm/E71_Human-Made_Thing">
	<rdf:type rdf:resource="http://www.w3.org/2002/07/owl#Class"/>
	<rdfs:subClassOf rdf:resource="http://www.cidoc-crm.org/cidoc-crm/E70_Thing"/>
	<rdfs:comment xml:lang="en">This class comprises discrete, identifiable human-made items that are documented as single units.
These items are either intellectual products or human-made physical things, and are characterized by relative stability. They may, for instance, have a solid physical form, an electronic encoding, or they may be logical concepts or structures.</rdfs:comment>
	<rdfs:label xml:lang="fr">Chose élaborée par l’humain</rdfs:label>
	<rdfs:label xml:lang="en">Human-Made Thing</rdfs:label>
</rdf:Description>

<rdf:Description rdf:about="http://www.cidoc-crm.org/cidoc-crm/E72_Legal_Object">
	<rdf:type rdf:resource="http://www.w3.org/2002/07/owl#Class"/>
	<rdfs:subClassOf rdf:resource="http://www.cidoc-crm.org/cidoc-crm/E70_Thing"/>
	<rdfs:comment xml:lang="en">This class comprises those material or immaterial items to which instances of E30 Right, such as the right of ownership or use, can be applied.
This is generally true for all instances of E18 Physical Thing. In the case of instances of E28 Conceptual Object, however, the identity of an instance of E28 Conceptual Object or the method of its use may be too ambiguous to reliably establish instances of E30 Right, as in the case of taxa and inspirations. Ownership of corporations is currently regarded as out of scope of the CIDOC CRM.</rdfs:comment>
	<rdfs:label xml:lang="en">Legal Object</rdfs:label>
	<rdfs:label xml:lang="fr">Objet juridique</rdfs:label>
	<rdfs:label xml:lang="pt">Objeto Jurídico</rdfs:label>
	<rdfs:label xml:lang="de">Rechtsobjekt</rdfs:label>
	<rdfs:label xml:lang="el">Νομικό Αντικείμενο</rdfs:label>
	<rdfs:label xml:lang="ru">Объект Права</rdfs:label>
	<rdfs:label xml:lang="zh">法律对象</rdfs:label>
</rdf:Description>

<rdf:Description rdf:about="http://www.cidoc-crm.org/cidoc-crm/E73_Information_Object">
	<rdf:type rdf:resource="http://www.w3.org/2002/07/owl#Class"/>
	<rdfs:subClassOf rdf:resource="http://www.cidoc-crm.org/cidoc-crm/E89_Propositional_Object"/>
	<rdfs:subClassOf rdf:resource="http://www.cidoc-crm.org/cidoc-crm/E90_Symbolic_Object"/>
	<rdfs:comment xml:lang="en">This class comprises identifiable immaterial items, such as poems, jokes, data sets, images, texts, multimedia objects, procedural prescriptions, computer program code, algorithm or mathematical formulae, that have an objectively recognizable structure and are documented as single units. The encoding structure known as a “named graph” also falls under this class, so that each “named graph” is an instance of E73 Information Object.
An instance of E73 Information Object does not depend on a specific physical carrier, which can include human memory, and it can exist on one or more carriers simultaneously.
Instances of E73 Information Object of a linguistic nature should be declared as instances of the E33 Linguistic Object subclass. Instances of E73 Information Object of a documentary nature should be declared as instances of the E31 Document subclass. Conceptual items such as types and classes are not instances of E73 Information Object, nor are ideas without a reproducible expression.</rdfs:comment>
	<rdfs:label xml:lang="en">Information Object</rdfs:label>
	<rdfs:label xml:lang="de">Informationsgegenstand</rdfs:label>
	<rdfs:label xml:lang="fr">Objet informationnel</rdfs:label>
	<rdfs:label xml:lang="pt">Objeto de Informação</rdfs:label>
	<rdfs:label xml:lang="el">Πληροφοριακό Αντικείμενο</rdfs:label>
	<rdfs:label xml:lang="ru">Информационный Объект</rdfs:label>
	<rdfs:label xml:lang="zh">信息对象</rdfs:label>
</rdf:Description>

<rdf:Description rdf:about="http://www.cidoc-crm.org/cidoc-crm/E74_Group">
	<rdf:type rdf:resource="http://www.w3.org/2002/07/owl#Class"/>
	<rdfs:subClassOf rdf:resource="http://www.cidoc-crm.org/cidoc-crm/E39_Actor"/>
	<rdfs:comment xml:lang="en">This class comprises any gatherings or organizations of human individuals or groups that act collectively or in a similar way due to any form of unifying relationship. In the wider sense this class also comprises official positions which used to be regarded in certain contexts as one actor, independent of the current holder of the office, such as the president of a country. In such cases, it may happen that the group never had more than one member. A joint pseudonym (i.e. a name that seems indicative of an individual but that is actually used as a persona by two or more people) is a particular case of E74 Group.
A gathering of people becomes an instance of E74 Group when it exhibits organizational characteristics usually typified by a set of ideas or beliefs held in common, or actions performed together. These might be communication, creating some common artifact, a common purpose such as study, worship, business, sports, etc. Nationality can be modelled as membership in an instance of E74 Group. Married couples and other concepts of family are regarded as particular examples of E74 Group.</rdfs:comment>
	<rdfs:label xml:lang="en">Group</rdfs:label>
	<rdfs:label xml:lang="fr">Groupe</rdfs:label>
	<rdfs:label xml:lang="pt">Grupo</rdfs:label>
	<rdfs:label xml:lang="de">Menschliche Gruppe</rdfs:label>
	<rdfs:label xml:lang="el">Ομάδα</rdfs:label>
	<rdfs:label xml:lang="ru">Группа</rdfs:label>
	<rdfs:label xml:lang="zh">团体</rdfs:label>
</rdf:Description>

<rdf:Description rdf:about="http://www.cidoc-crm.org/cidoc-crm/E77_Persistent_Item">
	<rdf:type rdf:resource="http://www.w3.org/2002/07/owl#Class"/>
	<owl:equivalentClass rdf:resource="http://www.loa-cnr.it/ontologies/DOLCE-Lite#endurant"/>
	<rdfs:subClassOf rdf:resource="http://www.cidoc-crm.org/cidoc-crm/E1_CRM_Entity"/>
	<rdfs:comment xml:lang="en">This class comprises items that have persistent characteristics of structural nature substantially related to their identity and their integrity, sometimes known as “endurants” in philosophy. Persistent Items may be physical entities, such as people, animals or things, conceptual entities such as ideas, concepts, products of the imagination or even names.
Instances of E77 Persistent Item may be present or be part of interactions in different periods or events. They can repeatedly be recognized at disparate occasions during their existence by characteristics of structural nature. The respective characteristics need not be exactly the same during all the existence of an instance of E77 Persistent Item. Often, they undergo gradual change, still bearing some similarities with that of previous times, or disappear completely and new emerge. For instance, a person, from the time of being born on, will gradually change all its features and acquire new ones, such as a scar. Even the DNA in different body cells will develop defects and mutations. Nevertheless, relevant characteristics used should be sufficiently similar to recognize the instance for some substantial period of time.
The more specific criteria that determine the identity of instances of subclasses of E77 Persistent Item may vary considerably and are described or referred to in the respective scope notes. The decision about which exact criteria to use depends on whether the observable behaviour of the respective part of reality such confined conforms to the reasoning the user is interested in. For example, a building can be regarded as no longer existing if it is dismantled and the materials reused in a different configuration. On the other hand, human beings go through radical and profound changes during their life-span, affecting both material composition and form, yet preserve their identity by other criteria, such as being bodily separated from other persons. Similarly, inanimate objects may be subject to exchange of parts and matter. On the opposite, the identity of a (version of a) text of a scientific publication is given by the exact arrangement of its relevant symbols.
The main classes of objects that fall outside the scope of the E77 Persistent Item class are temporal objects such as periods, events and acts, and descriptive properties.
An instance of E77 Persistent Item does not require actual knowledge of the identifying features of the instance being currently known. There may be cases, where the actual identifying features of an instance of E77 Persistent Item are not decidable at a particular state of knowledge.</rdfs:comment>
	<rdfs:label xml:lang="pt">Entidade Persistente</rdfs:label>
	<rdfs:label xml:lang="fr">Entité persistante</rdfs:label>
	<rdfs:label xml:lang="en">Persistent Item</rdfs:label>
	<rdfs:label xml:lang="de">Seiendes</rdfs:label>
	<rdfs:label xml:lang="el">Ον</rdfs:label>
	<rdfs:label xml:lang="ru">Постоянная Сущность</rdfs:label>
	<rdfs:label xml:lang="zh">持久项</rdfs:label>
</rdf:Description>

<rdf:Description rdf:about="http://www.cidoc-crm.org/cidoc-crm/E78_Curated_Holding">
	<rdf:type rdf:resource="http://www.w3.org/2002/07/owl#Class"/>
	<rdfs:subClassOf rdf:resource="http://www.cidoc-crm.org/cidoc-crm/E24_Physical_Human-Made_Thing"/>
	<rdfs:comment xml:lang="en">This class comprises aggregations of instances of E18 Physical Thing that are assembled and maintained (“curated” and “preserved,” in museological terminology) by one or more instances of E39 Actor over time for a specific purpose and audience, and according to a particular collection development plan. Typical instances of curated holdings are museum collections, archives, library holdings and digital libraries. A digital library is regarded as an instance of E18 Physical Thing because it requires keeping physical carriers of the electronic content.
Items may be added or removed from an E78 Curated Holding in pursuit of this plan. This class should not be confused with the E39 Actor maintaining the E78 Curated Holding who is often referred to using the name of the E78 Curated Holding (e.g. “The Wallace Collection decided…”).
Collective objects in the general sense, like a tomb full of gifts, a folder with stamps, or a set of chessmen, should be documented as instances of E19 Physical Object, and not as instances of E78 Curated Holding. This is because they form wholes, either because they are physically bound together or because they are kept together for their functionality.</rdfs:comment>
	<rdfs:label xml:lang="fr">Collection</rdfs:label>
	<rdfs:label xml:lang="en">Curated Holding</rdfs:label>
</rdf:Description>

<rdf:Description rdf:about="http://www.cidoc-crm.org/cidoc-crm/E79_Part_Addition">
	<rdf:type rdf:resource="http://www.w3.org/2002/07/owl#Class"/>
	<rdfs:subClassOf rdf:resource="http://www.cidoc-crm.org/cidoc-crm/E11_Modification"/>
	<rdfs:comment xml:lang="en">This class comprises activities that result in an instance of E18 Physical Thing being increased, enlarged, or augmented by the addition of a part.
Typical scenarios include the attachment of an accessory, the integration of a component, the addition of an element to an aggregate object, or the accessioning of an object into a curated instance of E78 Curated Holding. Both the E18 Physical Thing being augmented and the E18 Physical Thing that is being added are treated as separate identifiable wholes prior to the instance of E79 Part Addition. Following the addition of parts, the resulting assemblages are treated objectively as single identifiable wholes, made up of constituent or component parts bound together either physically (for example the engine becoming a part of the car), or by sharing a common purpose (such as the 32 chess pieces that make up a chess set). This class of activities forms a basis for reasoning about the history and continuity of identity of objects that are integrated into other objects over time, such as precious gemstones being repeatedly incorporated into different items of jewellery, or cultural artefacts being added to different museum instances of E78 Curated Holding over their lifespan.</rdfs:comment>
	<rdfs:label xml:lang="pt">Adição de Parte</rdfs:label>
	<rdfs:label xml:lang="fr">Ajout d'élément</rdfs:label>
	<rdfs:label xml:lang="en">Part Addition</rdfs:label>
	<rdfs:label xml:lang="de">Teilhinzufügung</rdfs:label>
	<rdfs:label xml:lang="el">Προσθήκη Μερών</rdfs:label>
	<rdfs:label xml:lang="ru">Добавление Части</rdfs:label>
	<rdfs:label xml:lang="zh">部分增加</rdfs:label>
</rdf:Description>

<rdf:Description rdf:about="http://www.cidoc-crm.org/cidoc-crm/E7_Activity">
	<rdf:type rdf:resource="http://www.w3.org/2002/07/owl#Class"/>
	<rdfs:subClassOf rdf:resource="http://www.cidoc-crm.org/cidoc-crm/E5_Event"/>
	<rdfs:comment xml:lang="en">This class comprises actions intentionally carried out by instances of E39 Actor that result in changes of state in the cultural, social, or physical systems documented.
This notion includes complex, composite, and long-lasting actions such as the building of a settlement or a war, as well as simple, short-lived actions such as the opening of a door.</rdfs:comment>
	<rdfs:label xml:lang="en">Activity</rdfs:label>
	<rdfs:label xml:lang="fr">Activité</rdfs:label>
	<rdfs:label xml:lang="pt">Atividade</rdfs:label>
	<rdfs:label xml:lang="de">Handlung</rdfs:label>
	<rdfs:label xml:lang="el">Δράση</rdfs:label>
	<rdfs:label xml:lang="ru">Деятельность</rdfs:label>
	<rdfs:label xml:lang="zh">活动</rdfs:label>
</rdf:Description>

<rdf:Description rdf:about="http://www.cidoc-crm.org/cidoc-crm/E80_Part_Removal">
	<rdf:type rdf:resource="http://www.w3.org/2002/07/owl#Class"/>
	<rdfs:subClassOf rdf:resource="http://www.cidoc-crm.org/cidoc-crm/E11_Modification"/>
	<rdfs:comment xml:lang="en">This class comprises the activities that result in an instance of E18 Physical Thing being decreased by the removal of a part.
Typical scenarios include the detachment of an accessory, the removal of a component or part of a composite object, or the deaccessioning of an object from a curated collection, an instance of E78 Curated Holding. If the instance of E80 Part Removal results in the total decomposition of the original object into pieces, such that the whole ceases to exist, the activity should instead be modelled as an instance of E81 Transformation, i.e. a simultaneous destruction and production. In cases where the part removed has no discernible identity prior to its removal but does have an identity subsequent to its removal, the activity should be modelled as both an instance of E80 Part Removal and E12 Production. This class of activities forms a basis for reasoning about the history, and continuity of identity over time, of objects that are removed from other objects, such as precious gemstones being extracted from different items of jewellery, or cultural artifacts being deaccessioned from different museum collections over their lifespan.</rdfs:comment>
	<rdfs:label xml:lang="en">Part Removal</rdfs:label>
	<rdfs:label xml:lang="pt">Remoção de Parte</rdfs:label>
	<rdfs:label xml:lang="fr">Retrait d'élément</rdfs:label>
	<rdfs:label xml:lang="de">Teilentfernung</rdfs:label>
	<rdfs:label xml:lang="el">Αφαίρεση Μερών</rdfs:label>
	<rdfs:label xml:lang="ru">Удаление Части</rdfs:label>
	<rdfs:label xml:lang="zh">部分去除</rdfs:label>
</rdf:Description>

<rdf:Description rdf:about="http://www.cidoc-crm.org/cidoc-crm/E81_Transformation">
	<rdf:type rdf:resource="http://www.w3.org/2002/07/owl#Class"/>
	<rdfs:subClassOf rdf:resource="http://www.cidoc-crm.org/cidoc-crm/E63_Beginning_of_Existence"/>
	<rdfs:subClassOf rdf:resource="http://www.cidoc-crm.org/cidoc-crm/E64_End_of_Existence"/>
	<rdfs:comment xml:lang="en">This class comprises the events that result in the simultaneous destruction of one or more than one E18 Physical Thing and the creation of one or more than one E18 Physical Thing that preserves recognizable substance and structure from the first one(s) but has fundamentally different nature or identity.
Although the old and the new instances of E18 Physical Thing are treated as discrete entities having separate, unique identities, they are causally connected through the E81 Transformation; the destruction of the old E18 Physical Thing(s) directly causes the creation of the new one(s) using or preserving some relevant substance and structure. Instances of E81 Transformation are therefore distinct from re-classifications (documented using E17 Type Assignment) or modifications (documented using E11 Modification) of objects that do not fundamentally change their nature or identity. Characteristic cases are reconstructions and repurposing of historical buildings or ruins, fires leaving buildings in ruins, taxidermy of specimen in natural history.
Even though such instances of E81 Transformation are often motivated by a change of intended use, substantial material changes should justify the documentation of the result as a new instance of E18 Physical Thing and not just the change of function. The latter may be documented as an extended activity (instance of E7 Activity) of using it.</rdfs:comment>
	<rdfs:label xml:lang="en">Transformation</rdfs:label>
	<rdfs:label xml:lang="fr">Transformation</rdfs:label>
	<rdfs:label xml:lang="pt">Transformação</rdfs:label>
	<rdfs:label xml:lang="de">Umwandlung</rdfs:label>
	<rdfs:label xml:lang="el">Μετατροπή</rdfs:label>
	<rdfs:label xml:lang="ru">Трансформация</rdfs:label>
	<rdfs:label xml:lang="zh">转变</rdfs:label>
</rdf:Description>

<rdf:Description rdf:about="http://www.cidoc-crm.org/cidoc-crm/E83_Type_Creation">
	<rdf:type rdf:resource="http://www.w3.org/2002/07/owl#Class"/>
	<rdfs:subClassOf rdf:resource="http://www.cidoc-crm.org/cidoc-crm/E65_Creation"/>
	<rdfs:comment xml:lang="en">This class comprises activities formally defining new types of items.
It is typically a rigorous scholarly or scientific process that ensures a type is exhaustively described and appropriately named. In some cases, particularly in archaeology and the life sciences, E83 Type Creation requires the identification of an exemplary specimen and the publication of the type definition in an appropriate scholarly forum. The activity modelled as an instance of E83 Type Creation is central to research in the life sciences, where a type would be referred to as a “taxon,” the type description as a “protologue,” and the exemplary specimens as “original element” or “holotype”.</rdfs:comment>
	<rdfs:label xml:lang="pt">Criação de Tipo</rdfs:label>
	<rdfs:label xml:lang="fr">Création de type</rdfs:label>
	<rdfs:label xml:lang="en">Type Creation</rdfs:label>
	<rdfs:label xml:lang="de">Typuserfindung</rdfs:label>
	<rdfs:label xml:lang="el">Δημιουργία Τύπου</rdfs:label>
	<rdfs:label xml:lang="ru">Создание Типа</rdfs:label>
	<rdfs:label xml:lang="zh">类型创建</rdfs:label>
</rdf:Description>

<rdf:Description rdf:about="http://www.cidoc-crm.org/cidoc-crm/E85_Joining">
	<rdf:type rdf:resource="http://www.w3.org/2002/07/owl#Class"/>
	<rdfs:subClassOf rdf:resource="http://www.cidoc-crm.org/cidoc-crm/E7_Activity"/>
	<rdfs:comment xml:lang="en">This class comprises the activities that result in an instance of E39 Actor becoming a member of an instance of E74 Group. This class does not imply initiative by either party. It may be the initiative of a third party.
Typical scenarios include becoming a member of a social organisation, becoming an employee of a company, marriage, the adoption of a child by a family, and the inauguration of somebody into an official position.</rdfs:comment>
	<rdfs:label xml:lang="fr">Adhésion</rdfs:label>
	<rdfs:label xml:lang="de">Beitritt</rdfs:label>
	<rdfs:label xml:lang="en">Joining</rdfs:label>
	<rdfs:label xml:lang="zh">加入</rdfs:label>
</rdf:Description>

<rdf:Description rdf:about="http://www.cidoc-crm.org/cidoc-crm/E86_Leaving">
	<rdf:type rdf:resource="http://www.w3.org/2002/07/owl#Class"/>
	<rdfs:subClassOf rdf:resource="http://www.cidoc-crm.org/cidoc-crm/E7_Activity"/>
	<rdfs:comment xml:lang="en">This class comprises the activities that result in an instance of E39 Actor to be disassociated from an instance of E74 Group. This class does not imply initiative by either party. It may be the initiative of a third party.
Typical scenarios include the termination of membership in a social organisation, ending the employment at a company, divorce, and the end of tenure of somebody in an official position.</rdfs:comment>
	<rdfs:label xml:lang="de">Austritt</rdfs:label>
	<rdfs:label xml:lang="fr">Départ</rdfs:label>
	<rdfs:label xml:lang="en">Leaving</rdfs:label>
	<rdfs:label xml:lang="zh">离开</rdfs:label>
</rdf:Description>

<rdf:Description rdf:about="http://www.cidoc-crm.org/cidoc-crm/E87_Curation_Activity">
	<rdf:type rdf:resource="http://www.w3.org/2002/07/owl#Class"/>
	<rdfs:subClassOf rdf:resource="http://www.cidoc-crm.org/cidoc-crm/E7_Activity"/>
	<rdfs:comment xml:lang="en">This class comprises the activities that contribute to the management and the preservation and evolution of instances of E78 Curated Holding, following an implicit or explicit curation plan.
It specializes the notion of activity into the curation of a collection and allows the history of curation to be recorded.
Items are accumulated and organized following criteria such as subject, chronological period, material type, style of art, etc., and can be added or removed from an instance of E78 Curated Holding for a specific purpose and/or audience. The initial aggregation of items to form a collection is regarded as an instance of E12 Production Event, while the activities of evolving, preserving, and promoting a collection are regarded as instances of E87 Curation Activity.</rdfs:comment>
	<rdfs:label xml:lang="fr">Activité curatoriale</rdfs:label>
	<rdfs:label xml:lang="en">Curation Activity</rdfs:label>
	<rdfs:label xml:lang="de">Kuratorische Tätigkeit</rdfs:label>
	<rdfs:label xml:lang="zh">管理</rdfs:label>
</rdf:Description>

<rdf:Description rdf:about="http://www.cidoc-crm.org/cidoc-crm/E89_Propositional_Object">
	<rdf:type rdf:resource="http://www.w3.org/2002/07/owl#Class"/>
	<rdfs:subClassOf rdf:resource="http://www.cidoc-crm.org/cidoc-crm/E28_Conceptual_Object"/>
	<rdfs:comment xml:lang="en">This class comprises immaterial items, including but not limited to stories, plots, procedural prescriptions, algorithms, laws of physics or images that are, or represent in some sense, sets of propositions about real or imaginary things and that are documented as single units or serve as topic of discourse.
This class also comprises items that are “about” something in the sense of a subject. In the wider sense, this class includes expressions of psychological value such as non-figural art and musical themes. However, conceptual items such as types and classes are not instances of E89 Propositional Object. This should not be confused with the definition of a type, which is indeed an instance of E89 Propositional Object.</rdfs:comment>
	<rdfs:label xml:lang="de">Aussagenobjekt</rdfs:label>
	<rdfs:label xml:lang="fr">Objet propositionnel</rdfs:label>
	<rdfs:label xml:lang="en">Propositional Object</rdfs:label>
	<rdfs:label xml:lang="zh">命题对象</rdfs:label>
</rdf:Description>

<rdf:Description rdf:about="http://www.cidoc-crm.org/cidoc-crm/E8_Acquisition">
	<rdf:type rdf:resource="http://www.w3.org/2002/07/owl#Class"/>
	<rdfs:subClassOf rdf:resource="http://www.cidoc-crm.org/cidoc-crm/E7_Activity"/>
	<rdfs:comment xml:lang="en">This class comprises transfers of legal ownership from one or more instances of E39 Actor to one or more other instances of E39 Actor.
The class also applies to the establishment or loss of ownership of instances of E18 Physical Thing. It does not, however, imply changes of any other kinds of rights. The recording of the donor and/or recipient is optional. It is possible that in an instance of E8 Acquisition there is either no donor or no recipient. Depending on the circumstances, it may describe:
1. the beginning of ownership
2. the end of ownership
3. the transfer of ownership
4. the acquisition from an unknown source
5. the loss of title due to destruction of the item
It may also describe events where a collector appropriates legal title, for example, by annexation or field collection. The interpretation of the museum notion of “accession” differs between institutions. The CIDOC CRM therefore models legal ownership (E8 Acquisition) and physical custody (E10 Transfer of Custody) separately. Institutions will then model their specific notions of accession and deaccession as combinations of these.</rdfs:comment>
	<rdfs:label xml:lang="en">Acquisition</rdfs:label>
	<rdfs:label xml:lang="fr">Acquisition</rdfs:label>
	<rdfs:label xml:lang="pt">Aquisição</rdfs:label>
	<rdfs:label xml:lang="de">Erwerb</rdfs:label>
	<rdfs:label xml:lang="el">Απόκτηση</rdfs:label>
	<rdfs:label xml:lang="ru">Событие Приобретения</rdfs:label>
	<rdfs:label xml:lang="zh">采访</rdfs:label>
</rdf:Description>

<rdf:Description rdf:about="http://www.cidoc-crm.org/cidoc-crm/E90_Symbolic_Object">
	<rdf:type rdf:resource="http://www.w3.org/2002/07/owl#Class"/>
	<rdfs:subClassOf rdf:resource="http://www.cidoc-crm.org/cidoc-crm/E28_Conceptual_Object"/>
	<rdfs:subClassOf rdf:resource="http://www.cidoc-crm.org/cidoc-crm/E72_Legal_Object"/>
	<rdfs:comment xml:lang="en">This class comprises identifiable symbols and any aggregation of symbols, such as characters, identifiers, traffic signs, emblems, texts, data sets, images, musical scores, multimedia objects, computer program code, or mathematical formulae that have an objectively recognizable structure and that are documented as single units.
It includes sets of signs of any nature, which may serve to designate something, or to communicate some propositional content. An instance of E90 Symbolic Object may or may not have a specific meaning, for example an arbitrary character string.
In some cases, the content of an instance of E90 Symbolic Object may completely be represented by a serialized digital content model, such as a sequence of ASCII-encoded characters, an XML or HTML document, or a TIFF image. The property P3 has note and its subproperty P190 has symbolic content allow for the description of this content model. In order to disambiguate which symbolic level is the carrier of the meaning, the property P3.1 has type can be used to specify the encoding (e.g. “bit”, “Latin character”, RGB pixel).</rdfs:comment>
	<rdfs:label xml:lang="fr">Objet symbolique</rdfs:label>
	<rdfs:label xml:lang="en">Symbolic Object</rdfs:label>
	<rdfs:label xml:lang="de">Symbolisches Objekt</rdfs:label>
	<rdfs:label xml:lang="zh">符号对象</rdfs:label>
</rdf:Description>

<rdf:Description rdf:about="http://www.cidoc-crm.org/cidoc-crm/E92_Spacetime_Volume">
	<rdf:type rdf:resource="http://www.w3.org/2002/07/owl#Class"/>
	<rdfs:subClassOf rdf:resource="http://www.cidoc-crm.org/cidoc-crm/E1_CRM_Entity"/>
	<rdfs:subClassOf rdf:resource="http://www.loa-cnr.it/ontologies/DOLCE-Lite#perdurant"/>
	<rdfs:comment xml:lang="en">This class comprises 4-dimensional point sets (volumes) in physical spacetime (in contrast to mathematical models of it) regardless of their true geometric forms. They may derive their identity from being the extent of a material phenomenon or from being the interpretation of an expression defining an extent in spacetime. Intersections of instances of E92 Spacetime Volume, E53 Place, and E52 Time-Span are also regarded as instances of E92 Spacetime Volume. An instance of E92 Spacetime Volume is either contiguous or composed of a finite number of contiguous subsets. Its boundaries may be fuzzy due to the properties of the phenomena it derives from or due to the limited precision up to which defining expression can be identified with a real extent in spacetime. The duration of existence of an instance of E92 Spacetime Volume is its projection on time.</rdfs:comment>
	<rdfs:label xml:lang="en">Spacetime Volume</rdfs:label>
	<rdfs:label xml:lang="fr">Volume spatio-temporel</rdfs:label>
</rdf:Description>

<rdf:Description rdf:about="http://www.cidoc-crm.org/cidoc-crm/E93_Presence">
	<rdf:type rdf:resource="http://www.w3.org/2002/07/owl#Class"/>
	<rdfs:subClassOf rdf:resource="http://www.cidoc-crm.org/cidoc-crm/E92_Spacetime_Volume"/>
	<rdfs:comment xml:lang="en">This class comprises instances of E92 Spacetime Volume, whose temporal extent has been chosen in order to determine the spatial extent of a phenomenon over the chosen time-span. Respective phenomena may, for instance, be historical events or periods, but can also be the diachronic extent and existence of physical things. In other words, instances of this class fix a slice of another instance of E92 Spacetime Volume in time.
The temporal extent of an instance of E93 Presence typically is predetermined by the researcher so as to focus the investigation particularly on finding the spatial extent of the phenomenon by testing for its characteristic features. There are at least two basic directions such investigations might take. The investigation may wish to determine where something was during some time or it may wish to reconstruct the total passage of a phenomenon’s spacetime volume through an examination of discrete presences. Observation and measurement of features indicating the presence or absence of a phenomenon in some space allows for the progressive approximation of spatial extents through argumentation typically based on inclusion, exclusion and various overlaps.</rdfs:comment>
	<rdfs:label xml:lang="en">Presence</rdfs:label>
	<rdfs:label xml:lang="fr">Présence</rdfs:label>
</rdf:Description>

<rdf:Description rdf:about="http://www.cidoc-crm.org/cidoc-crm/E96_Purchase">
	<rdf:type rdf:resource="http://www.w3.org/2002/07/owl#Class"/>
	<rdfs:subClassOf rdf:resource="http://www.cidoc-crm.org/cidoc-crm/E8_Acquisition"/>
	<rdfs:comment xml:lang="en">This class comprises transfers of legal ownership from one or more instances of E39 Actor to one or more different instances of E39 Actor, where the transferring party is completely compensated by the payment of a monetary amount. In more detail, a purchase agreement establishes a fixed monetary obligation at its initialization on the receiving party, to the giving party. An instance of E96 Purchase begins with the contract or equivalent agreement and ends with the fulfilment of all contractual obligations. In the case that the activity is abandoned before both parties have fulfilled these obligations, the activity is not regarded as an instance of E96 Purchase.
This class is a very specific case of the much more complex social business practices of exchange of goods and the creation and satisfaction of related social obligations. Purchase activities which define individual sales prices per object can be modelled by instantiating E96 Purchase for each object individually and as part of an overall instance of E96 Purchase transaction.</rdfs:comment>
	<rdfs:label xml:lang="fr">Achat</rdfs:label>
	<rdfs:label xml:lang="en">Purchase</rdfs:label>
</rdf:Description>

<rdf:Description rdf:about="http://www.cidoc-crm.org/cidoc-crm/E97_Monetary_Amount">
	<rdf:type rdf:resource="http://www.w3.org/2002/07/owl#Class"/>
	<rdfs:subClassOf rdf:resource="http://www.cidoc-crm.org/cidoc-crm/E54_Dimension"/>
	<rdfs:comment xml:lang="en">This class comprises quantities of monetary possessions or obligations in terms of their nominal value with respect to a particular currency. These quantities may be abstract accounting units, the nominal value of a heap of coins or bank notes at the time of validity of the respective currency, the nominal value of a bill of exchange or other documents expressing monetary claims or obligations. It specifically excludes amounts expressed in terms of weights of valuable items, like gold and diamonds, and quantities of other non-currency items, like goats or stocks and bonds.</rdfs:comment>
	<rdfs:label xml:lang="en">Monetary Amount</rdfs:label>
	<rdfs:label xml:lang="fr">Valeur monétaire</rdfs:label>
</rdf:Description>

<rdf:Description rdf:about="http://www.cidoc-crm.org/cidoc-crm/E98_Currency">
	<rdf:type rdf:resource="http://www.w3.org/2002/07/owl#Class"/>
	<rdfs:subClassOf rdf:resource="http://www.cidoc-crm.org/cidoc-crm/E58_Measurement_Unit"/>
	<rdfs:comment xml:lang="en">This class comprises the units in which a monetary system, supported by an administrative authority or other community, quantifies and arithmetically compares all monetary amounts declared in the unit. The unit of a monetary system must describe a nominal value which is kept constant by its administrative authority and an associated banking system if it exists, and not by market value. For instance, one may pay with grams of gold, but the respective monetary amount would have been agreed as the gold price in US dollars on the day of the payment. Under this definition, British Pounds, U.S. Dollars, and European Euros are examples of currency, but “grams of gold” is not. One monetary system has one and only one currency. Instances of this class must not be confused with coin denominations, such as “Dime” or “Sestertius”. Non-monetary exchange of value in terms of quantities of a particular type of goods, such as cows, do not constitute a currency.</rdfs:comment>
	<rdfs:label xml:lang="en">Currency</rdfs:label>
	<rdfs:label xml:lang="fr">Unité monétaire</rdfs:label>
</rdf:Description>

<rdf:Description rdf:about="http://www.cidoc-crm.org/cidoc-crm/E99_Product_Type">
	<rdf:type rdf:resource="http://www.w3.org/2002/07/owl#Class"/>
	<rdfs:subClassOf rdf:resource="http://www.cidoc-crm.org/cidoc-crm/E55_Type"/>
	<rdfs:comment xml:lang="en">This class comprises types that stand as the models for instances of E22 Human-Made Object that are produced as the result of production activities using plans exact enough to result in one or more series of uniform, functionally and aesthetically identical and interchangeable items. The product type is the intended ideal form of the manufacture process. It is typical of instances of E22 Human-Made Object that conform to an instance of E99 Product Type that its component parts are interchangeable with component parts of other instances of E22 Human-Made Object made after the model of the same instance of E99 Product Type. Frequently, the uniform production according to a given instance of E99 Product Type is achieved by creating individual tools, such as moulds or print plates that are themselves carriers of the design of the product type. Modern tools may use the flexibility of electronically controlled devices to achieve such uniformity. The product type itself, i.e. the potentially unlimited series of aesthetically equivalent items, may be the target of artistic design, rather than the individual object. In extreme cases, only one instance of a product type may have been produced, such as in a “print on demand” process which was only triggered once. However, this should not be confused with industrial prototypes, such as car prototypes, which are produced prior to the production line being set up, or test the production line itself.</rdfs:comment>
	<rdfs:label xml:lang="fr">Modèle de produit</rdfs:label>
	<rdfs:label xml:lang="en">Product Type</rdfs:label>
</rdf:Description>

<rdf:Description rdf:about="http://www.cidoc-crm.org/cidoc-crm/E9_Move">
	<rdf:type rdf:resource="http://www.w3.org/2002/07/owl#Class"/>
	<rdfs:subClassOf rdf:resource="http://www.cidoc-crm.org/cidoc-crm/E7_Activity"/>
	<rdfs:comment xml:lang="en">This class comprises changes of the physical location of the instances of E19 Physical Object.
Note, that the class E9 Move inherits the property P7 took place at (witnessed): E53 Place. This property should be used to describe the trajectory or a larger area within which a move takes place, whereas the properties P26 moved to (was destination of), P27 moved from (was origin of) describe the start and end points only. Moves may also be documented to consist of other moves (via P9 consists of (forms part of)), in order to describe intermediate stages on a trajectory. In that case, start and end points of the partial moves should match appropriately between each other and with the overall event.</rdfs:comment>
	<rdfs:label xml:lang="fr">Déplacement</rdfs:label>
	<rdfs:label xml:lang="pt">Locomoção</rdfs:label>
	<rdfs:label xml:lang="en">Move</rdfs:label>
	<rdfs:label xml:lang="de">Objektbewegung</rdfs:label>
	<rdfs:label xml:lang="el">Μετακίνηση</rdfs:label>
	<rdfs:label xml:lang="ru">Перемещение</rdfs:label>
	<rdfs:label xml:lang="zh">移动</rdfs:label>
</rdf:Description>

<rdf:Description rdf:about="http://www.loa-cnr.it/ontologies/Actions#cognitive-event">
	<rdf:type rdf:resource="http://www.w3.org/2002/07/owl#Class"/>
	<rdfs:subClassOf rdf:resource="http://www.cidoc-crm.org/cidoc-crm/E5_Event"/>
</rdf:Description>

<rdf:Description rdf:about="http://www.loa-cnr.it/ontologies/DOLCE-Lite#endurant">
	<rdf:type rdf:resource="http://www.w3.org/2002/07/owl#Class"/>
	<rdfs:subClassOf rdf:resource="http://www.cidoc-crm.org/cidoc-crm/E1_CRM_Entity"/>
</rdf:Description>

<rdf:Description rdf:about="http://www.loa-cnr.it/ontologies/DOLCE-Lite#perdurant">
	<rdf:type rdf:resource="http://www.w3.org/2002/07/owl#Class"/>
</rdf:Description>

<rdf:Description rdf:about="http://www.loa-cnr.it/ontologies/DnS#description">
	<rdf:type rdf:resource="http://www.w3.org/2002/07/owl#Class"/>
	<rdfs:subClassOf rdf:resource="http://www.cidoc-crm.org/cidoc-crm/E28_Conceptual_Object"/>
	<rdfs:subClassOf rdf:resource="http://www.loa-cnr.it/ontologies/DOLCE-Lite#endurant"/>
</rdf:Description>

<rdf:Description rdf:about="http://www.loa-cnr.it/ontologies/DnS#gestalt">
	<rdf:type rdf:resource="http://www.w3.org/2002/07/owl#Class"/>
	<rdfs:subClassOf rdf:resource="http://www.loa-cnr.it/ontologies/DnS#theory"/>
</rdf:Description>

<rdf:Description rdf:about="http://www.loa-cnr.it/ontologies/DnS#relation">
	<rdf:type rdf:resource="http://www.w3.org/2002/07/owl#Class"/>
	<rdfs:subClassOf rdf:resource="http://www.loa-cnr.it/ontologies/DnS#theory"/>
</rdf:Description>

<rdf:Description rdf:about="http://www.loa-cnr.it/ontologies/DnS#theory">
	<rdf:type rdf:resource="http://www.w3.org/2002/07/owl#Class"/>
	<rdfs:subClassOf rdf:resource="http://www.loa-cnr.it/ontologies/DnS#description"/>
</rdf:Description>

<rdf:Description rdf:about="http://www.w3.org/1999/02/22-rdf-syntax-ns#List">
	<rdf:type rdf:resource="http://www.w3.org/2002/07/owl#Class"/>
</rdf:Description>

<rdf:Description rdf:about="http://www.w3.org/2004/02/skos/core#Collection">
	<rdf:type rdf:resource="http://www.w3.org/2002/07/owl#Class"/>
	<owl:disjointWith rdf:resource="http://www.w3.org/2004/02/skos/core#Concept"/>
	<owl:disjointWith rdf:resource="http://www.w3.org/2004/02/skos/core#ConceptScheme"/>
	<rdfs:isDefinedBy rdf:resource="http://www.w3.org/2004/02/skos/core"/>
	<rdfs:label xml:lang="en">Collection</rdfs:label>
	<skos:definition xml:lang="en">A meaningful collection of concepts.</skos:definition>
	<skos:scopeNote xml:lang="en">Labelled collections can be used where you would like a set of concepts to be displayed under a 'node label' in the hierarchy.</skos:scopeNote>
</rdf:Description>

<rdf:Description rdf:about="http://www.w3.org/2004/02/skos/core#Concept">
	<rdf:type rdf:resource="http://www.w3.org/2002/07/owl#Class"/>
	<owl:disjointWith rdf:resource="http://www.w3.org/2004/02/skos/core#ConceptScheme"/>
	<owl:disjointWith rdf:resource="http://www.w3.org/2004/02/skos/core#OrderedCollection"/>
	<rdfs:isDefinedBy rdf:resource="http://www.w3.org/2004/02/skos/core"/>
	<rdfs:label xml:lang="en">Concept</rdfs:label>
	<skos:definition xml:lang="en">An idea or notion; a unit of thought.</skos:definition>
</rdf:Description>

<rdf:Description rdf:about="http://www.w3.org/2004/02/skos/core#ConceptScheme">
	<rdf:type rdf:resource="http://www.w3.org/2002/07/owl#Class"/>
	<owl:disjointWith rdf:resource="http://www.w3.org/2004/02/skos/core#OrderedCollection"/>
	<rdfs:isDefinedBy rdf:resource="http://www.w3.org/2004/02/skos/core"/>
	<rdfs:label xml:lang="en">Concept Scheme</rdfs:label>
	<skos:definition xml:lang="en">A set of concepts, optionally including statements about semantic relationships between those concepts.</skos:definition>
	<skos:example xml:lang="en">Thesauri, classification schemes, subject heading lists, taxonomies, 'folksonomies', and other types of controlled vocabulary are all examples of concept schemes. Concept schemes are also embedded in glossaries and terminologies.</skos:example>
	<skos:scopeNote xml:lang="en">A concept scheme may be defined to include concepts from different sources.</skos:scopeNote>
</rdf:Description>

<rdf:Description rdf:about="http://www.w3.org/2004/02/skos/core#OrderedCollection">
	<rdf:type rdf:resource="http://www.w3.org/2002/07/owl#Class"/>
	<rdfs:subClassOf rdf:resource="http://www.w3.org/2004/02/skos/core#Collection"/>
	<rdfs:isDefinedBy rdf:resource="http://www.w3.org/2004/02/skos/core"/>
	<rdfs:label xml:lang="en">Ordered Collection</rdfs:label>
	<skos:definition xml:lang="en">An ordered collection of concepts, where both the grouping and the ordering are meaningful.</skos:definition>
	<skos:scopeNote xml:lang="en">Ordered collections can be used where you would like a set of concepts to be displayed in a specific order, and optionally under a 'node label'.</skos:scopeNote>
</rdf:Description>

<rdf:Description rdf:about="http://academictourism.com/TS.BRF0004.RS.RS0006.RS0001">
	<rdf:type rdf:resource="http://www.w3.org/2002/07/owl#NamedIndividual"/>
	<rdf:type rdf:resource="http://www.cidoc-crm.org/cidoc-crm/E1_CRM_Entity"/>
	<rdf:type rdf:resource="http://www.cidoc-crm.org/cidoc-crm/E52_Time-Span"/>
	<cidoc-crm:P4i_is_time-span_of rdf:resource="http://academictourism.com/entity/BRF0004.RS.RS0006.RS0001"/>
	<cidoc-crm:P170i_time_is_defined_by rdf:datatype="http://www.w3.org/2001/XMLSchema#dateTime">1816-07-09T04:00:00+01:00</cidoc-crm:P170i_time_is_defined_by>
</rdf:Description>

<rdf:Description rdf:about="http://academictourism.com/entity/BE.LOC0003.CS">
	<rdf:type rdf:resource="http://www.w3.org/2002/07/owl#NamedIndividual"/>
	<rdf:type rdf:resource="http://www.cidoc-crm.org/cidoc-crm/E1_CRM_Entity"/>
	<rdf:type rdf:resource="http://www.cidoc-crm.org/cidoc-crm/E2_Temporal_Entity"/>
	<rdf:type rdf:resource="http://www.cidoc-crm.org/cidoc-crm/E4_Period"/>
	<rdf:type rdf:resource="http://www.cidoc-crm.org/cidoc-crm/E5_Event"/>
	<rdf:type rdf:resource="http://www.cidoc-crm.org/cidoc-crm/E63_Beginning_of_Existence"/>
	<rdf:type rdf:resource="http://www.cidoc-crm.org/cidoc-crm/E92_Spacetime_Volume"/>
	<rdf:type rdf:resource="http://www.loa-cnr.it/ontologies/DOLCE-Lite#perdurant"/>
	<cidoc-crm:P11_had_participant rdf:resource="http://academictourism.com/entity/PER0011"/>
	<cidoc-crm:P11_had_participant rdf:resource="http://academictourism.com/entity/PER0012"/>
	<cidoc-crm:P11_had_participant rdf:resource="http://academictourism.com/entity/PER0016"/>
	<cidoc-crm:P12_occurred_in_the_presence_of rdf:resource="http://academictourism.com/entity/LOC0003.CS"/>
	<cidoc-crm:P12_occurred_in_the_presence_of rdf:resource="http://academictourism.com/entity/PER0011"/>
	<cidoc-crm:P12_occurred_in_the_presence_of rdf:resource="http://academictourism.com/entity/PER0012"/>
	<cidoc-crm:P12_occurred_in_the_presence_of rdf:resource="http://academictourism.com/entity/PER0016"/>
	<cidoc-crm:P92_brought_into_existence rdf:resource="http://academictourism.com/entity/LOC0003.CS"/>
	<rdfs:label>Construction of Wilhelmshöhe</rdfs:label>
</rdf:Description>

<rdf:Description rdf:about="http://academictourism.com/entity/BE.MISC0001">
	<rdf:type rdf:resource="http://www.w3.org/2002/07/owl#NamedIndividual"/>
	<rdf:type rdf:resource="http://www.cidoc-crm.org/cidoc-crm/E1_CRM_Entity"/>
	<rdf:type rdf:resource="http://www.cidoc-crm.org/cidoc-crm/E2_Temporal_Entity"/>
	<rdf:type rdf:resource="http://www.cidoc-crm.org/cidoc-crm/E4_Period"/>
	<rdf:type rdf:resource="http://www.cidoc-crm.org/cidoc-crm/E5_Event"/>
	<rdf:type rdf:resource="http://www.cidoc-crm.org/cidoc-crm/E63_Beginning_of_Existence"/>
	<rdf:type rdf:resource="http://www.cidoc-crm.org/cidoc-crm/E92_Spacetime_Volume"/>
	<rdf:type rdf:resource="http://www.loa-cnr.it/ontologies/DOLCE-Lite#perdurant"/>
	<cidoc-crm:P11_had_participant rdf:resource="http://academictourism.com/entity/PER0015"/>
	<cidoc-crm:P12_occurred_in_the_presence_of rdf:resource="http://academictourism.com/entity/MISC0001"/>
	<cidoc-crm:P12_occurred_in_the_presence_of rdf:resource="http://academictourism.com/entity/PER0015"/>
	<cidoc-crm:P92_brought_into_existence rdf:resource="http://academictourism.com/entity/MISC0001"/>
	<rdfs:label>Construction of Casernes</rdfs:label>
</rdf:Description>

<rdf:Description rdf:about="http://academictourism.com/entity/BE.MISC0003">
	<rdf:type rdf:resource="http://www.w3.org/2002/07/owl#NamedIndividual"/>
	<rdf:type rdf:resource="http://www.cidoc-crm.org/cidoc-crm/E1_CRM_Entity"/>
	<rdf:type rdf:resource="http://www.cidoc-crm.org/cidoc-crm/E2_Temporal_Entity"/>
	<rdf:type rdf:resource="http://www.cidoc-crm.org/cidoc-crm/E4_Period"/>
	<rdf:type rdf:resource="http://www.cidoc-crm.org/cidoc-crm/E5_Event"/>
	<rdf:type rdf:resource="http://www.cidoc-crm.org/cidoc-crm/E63_Beginning_of_Existence"/>
	<rdf:type rdf:resource="http://www.cidoc-crm.org/cidoc-crm/E7_Activity"/>
	<rdf:type rdf:resource="http://www.cidoc-crm.org/cidoc-crm/E92_Spacetime_Volume"/>
	<rdf:type rdf:resource="http://www.loa-cnr.it/ontologies/DOLCE-Lite#perdurant"/>
	<cidoc-crm:P11_had_participant rdf:resource="http://academictourism.com/entity/PER0009"/>
	<cidoc-crm:P12_occurred_in_the_presence_of rdf:resource="http://academictourism.com/entity/MISC0003"/>
	<cidoc-crm:P12_occurred_in_the_presence_of rdf:resource="http://academictourism.com/entity/PER0009"/>
	<cidoc-crm:P14_carried_out_by rdf:resource="http://academictourism.com/entity/PER0009"/>
	<cidoc-crm:P15_was_influenced_by rdf:resource="http://academictourism.com/entity/MISC0018"/>
	<cidoc-crm:P15_was_influenced_by rdf:resource="http://academictourism.com/entity/MISC0021"/>
	<cidoc-crm:P67i_is_referred_to_by rdf:resource="http://academictourism.com/entity/MISC0022"/>
	<cidoc-crm:P70i_is_documented_in rdf:resource="http://academictourism.com/entity/MISC0022"/>
	<cidoc-crm:P92_brought_into_existence rdf:resource="http://academictourism.com/entity/MISC0003"/>
	<rdfs:label>Creation of Wilhelmshöhe schilderyen</rdfs:label>
</rdf:Description>

<rdf:Description rdf:about="http://academictourism.com/entity/BE.MISC0009">
	<rdf:type rdf:resource="http://www.w3.org/2002/07/owl#NamedIndividual"/>
	<rdf:type rdf:resource="http://www.cidoc-crm.org/cidoc-crm/E1_CRM_Entity"/>
	<rdf:type rdf:resource="http://www.cidoc-crm.org/cidoc-crm/E2_Temporal_Entity"/>
	<rdf:type rdf:resource="http://www.cidoc-crm.org/cidoc-crm/E4_Period"/>
	<rdf:type rdf:resource="http://www.cidoc-crm.org/cidoc-crm/E5_Event"/>
	<rdf:type rdf:resource="http://www.cidoc-crm.org/cidoc-crm/E63_Beginning_of_Existence"/>
	<rdf:type rdf:resource="http://www.cidoc-crm.org/cidoc-crm/E92_Spacetime_Volume"/>
	<rdf:type rdf:resource="http://www.loa-cnr.it/ontologies/DOLCE-Lite#perdurant"/>
	<cidoc-crm:P12_occurred_in_the_presence_of rdf:resource="http://academictourism.com/entity/MISC0009"/>
	<cidoc-crm:P4_has_time-span rdf:resource="http://academictourism.com/entity/TS.BE.MISC0009"/>
	<cidoc-crm:P92_brought_into_existence rdf:resource="http://academictourism.com/entity/MISC0009"/>
	<rdfs:label>Creation of Hercules Monument</rdfs:label>
</rdf:Description>

<rdf:Description rdf:about="http://academictourism.com/entity/BE.MISC0018">
	<rdf:type rdf:resource="http://www.w3.org/2002/07/owl#NamedIndividual"/>
	<rdf:type rdf:resource="http://www.cidoc-crm.org/cidoc-crm/E1_CRM_Entity"/>
	<rdf:type rdf:resource="http://www.cidoc-crm.org/cidoc-crm/E2_Temporal_Entity"/>
	<rdf:type rdf:resource="http://www.cidoc-crm.org/cidoc-crm/E4_Period"/>
	<rdf:type rdf:resource="http://www.cidoc-crm.org/cidoc-crm/E5_Event"/>
	<rdf:type rdf:resource="http://www.cidoc-crm.org/cidoc-crm/E63_Beginning_of_Existence"/>
	<rdf:type rdf:resource="http://www.cidoc-crm.org/cidoc-crm/E92_Spacetime_Volume"/>
	<rdf:type rdf:resource="http://www.loa-cnr.it/ontologies/DOLCE-Lite#perdurant"/>
	<cidoc-crm:P11_had_participant rdf:resource="http://academictourism.com/entity/PER0010"/>
	<cidoc-crm:P12_occurred_in_the_presence_of rdf:resource="http://academictourism.com/entity/MISC0018"/>
	<cidoc-crm:P12_occurred_in_the_presence_of rdf:resource="http://academictourism.com/entity/PER0010"/>
	<cidoc-crm:P92_brought_into_existence rdf:resource="http://academictourism.com/entity/MISC0018"/>
	<rdfs:label>Creation of Oberon</rdfs:label>
</rdf:Description>

<rdf:Description rdf:about="http://academictourism.com/entity/BE.MISC0019">
	<rdf:type rdf:resource="http://www.w3.org/2002/07/owl#NamedIndividual"/>
	<rdf:type rdf:resource="http://www.cidoc-crm.org/cidoc-crm/E1_CRM_Entity"/>
	<rdf:type rdf:resource="http://www.cidoc-crm.org/cidoc-crm/E2_Temporal_Entity"/>
	<rdf:type rdf:resource="http://www.cidoc-crm.org/cidoc-crm/E4_Period"/>
	<rdf:type rdf:resource="http://www.cidoc-crm.org/cidoc-crm/E5_Event"/>
	<rdf:type rdf:resource="http://www.cidoc-crm.org/cidoc-crm/E63_Beginning_of_Existence"/>
	<rdf:type rdf:resource="http://www.cidoc-crm.org/cidoc-crm/E92_Spacetime_Volume"/>
	<rdf:type rdf:resource="http://www.loa-cnr.it/ontologies/DOLCE-Lite#perdurant"/>
	<cidoc-crm:P11_had_participant rdf:resource="http://academictourism.com/entity/PER0016"/>
	<cidoc-crm:P12_occurred_in_the_presence_of rdf:resource="http://academictourism.com/entity/MISC0019"/>
	<cidoc-crm:P12_occurred_in_the_presence_of rdf:resource="http://academictourism.com/entity/PER0016"/>
	<cidoc-crm:P4_has_time-span rdf:resource="http://academictourism.com/entity/TS.BE.MISC0019"/>
	<cidoc-crm:P92_brought_into_existence rdf:resource="http://academictourism.com/entity/MISC0019"/>
	<rdfs:label>Constrcution of Octogoon</rdfs:label>
</rdf:Description>

<rdf:Description rdf:about="http://academictourism.com/entity/BE.MISC0021">
	<rdf:type rdf:resource="http://www.w3.org/2002/07/owl#NamedIndividual"/>
	<rdf:type rdf:resource="http://www.cidoc-crm.org/cidoc-crm/E1_CRM_Entity"/>
	<rdf:type rdf:resource="http://www.cidoc-crm.org/cidoc-crm/E2_Temporal_Entity"/>
	<rdf:type rdf:resource="http://www.cidoc-crm.org/cidoc-crm/E4_Period"/>
	<rdf:type rdf:resource="http://www.cidoc-crm.org/cidoc-crm/E5_Event"/>
	<rdf:type rdf:resource="http://www.cidoc-crm.org/cidoc-crm/E63_Beginning_of_Existence"/>
	<rdf:type rdf:resource="http://www.cidoc-crm.org/cidoc-crm/E92_Spacetime_Volume"/>
	<rdf:type rdf:resource="http://www.loa-cnr.it/ontologies/DOLCE-Lite#perdurant"/>
	<cidoc-crm:P11_had_participant rdf:resource="http://academictourism.com/entity/PER0013"/>
	<cidoc-crm:P12_occurred_in_the_presence_of rdf:resource="http://academictourism.com/entity/MISC0021"/>
	<cidoc-crm:P12_occurred_in_the_presence_of rdf:resource="http://academictourism.com/entity/PER0013"/>
	<cidoc-crm:P92_brought_into_existence rdf:resource="http://academictourism.com/entity/MISC0021"/>
	<rdfs:label>Creation of La Gerusalemme liberata</rdfs:label>
</rdf:Description>

<rdf:Description rdf:about="http://academictourism.com/entity/BE.MISC0022">
	<rdf:type rdf:resource="http://www.w3.org/2002/07/owl#NamedIndividual"/>
	<rdf:type rdf:resource="http://www.cidoc-crm.org/cidoc-crm/E1_CRM_Entity"/>
	<rdf:type rdf:resource="http://www.cidoc-crm.org/cidoc-crm/E2_Temporal_Entity"/>
	<rdf:type rdf:resource="http://www.cidoc-crm.org/cidoc-crm/E4_Period"/>
	<rdf:type rdf:resource="http://www.cidoc-crm.org/cidoc-crm/E5_Event"/>
	<rdf:type rdf:resource="http://www.cidoc-crm.org/cidoc-crm/E63_Beginning_of_Existence"/>
	<rdf:type rdf:resource="http://www.cidoc-crm.org/cidoc-crm/E92_Spacetime_Volume"/>
	<rdf:type rdf:resource="http://www.loa-cnr.it/ontologies/DOLCE-Lite#perdurant"/>
	<cidoc-crm:P11_had_participant rdf:resource="http://academictourism.com/entity/PER0014"/>
	<cidoc-crm:P12_occurred_in_the_presence_of rdf:resource="http://academictourism.com/entity/MISC0022"/>
	<cidoc-crm:P12_occurred_in_the_presence_of rdf:resource="http://academictourism.com/entity/PER0014"/>
	<cidoc-crm:P4_has_time-span rdf:resource="http://academictourism.com/entity/TS.BE.MISC0022"/>
	<cidoc-crm:P92_brought_into_existence rdf:resource="http://academictourism.com/entity/MISC0022"/>
	<rdfs:label>Creation of beschreibung des Kurfürstlichen Landsitzes Wilhelmshöhe bey Cassel</rdfs:label>
</rdf:Description>

<rdf:Description rdf:about="http://academictourism.com/entity/BRF0004">
	<rdf:type rdf:resource="http://www.w3.org/2002/07/owl#NamedIndividual"/>
	<rdf:type rdf:resource="http://iflastandards.info/ns/lrm/lrmoo/F2_Expression"/>
	<rdf:type rdf:resource="http://www.cidoc-crm.org/cidoc-crm/E1_CRM_Entity"/>
	<rdf:type rdf:resource="http://www.cidoc-crm.org/cidoc-crm/E28_Conceptual_Object"/>
	<rdf:type rdf:resource="http://www.cidoc-crm.org/cidoc-crm/E70_Thing"/>
	<rdf:type rdf:resource="http://www.cidoc-crm.org/cidoc-crm/E71_Human-Made_Thing"/>
	<rdf:type rdf:resource="http://www.cidoc-crm.org/cidoc-crm/E72_Legal_Object"/>
	<rdf:type rdf:resource="http://www.cidoc-crm.org/cidoc-crm/E73_Information_Object"/>
	<rdf:type rdf:resource="http://www.cidoc-crm.org/cidoc-crm/E77_Persistent_Item"/>
	<rdf:type rdf:resource="http://www.cidoc-crm.org/cidoc-crm/E89_Propositional_Object"/>
	<rdf:type rdf:resource="http://www.cidoc-crm.org/cidoc-crm/E90_Symbolic_Object"/>
	<rdf:type rdf:resource="http://www.loa-cnr.it/ontologies/DOLCE-Lite#endurant"/>
	<lrmoo:R17i_was_created_by rdf:resource="http://academictourism.com/entity/BRF0004.SCH"/>
	<cidoc-crm:P129_is_about rdf:resource="http://academictourism.com/entity/BRF0004.RS"/>
	<cidoc-crm:P12i_was_present_at rdf:resource="http://academictourism.com/entity/BRF0004.SCH"/>
	<cidoc-crm:P67_refers_to rdf:resource="http://academictourism.com/entity/BRF0004.RS"/>
	<cidoc-crm:P92i_was_brought_into_existence_by rdf:resource="http://academictourism.com/entity/BRF0004.SCH"/>
	<cidoc-crm:P94i_was_created_by rdf:resource="http://academictourism.com/entity/BRF0004.SCH"/>
	<rdfs:comment>Brief IV
Uit Göttingen van den 9 July 1816

Iets in ’t algemeen over Wilhelmshöhe – De Zondag het geschikst om dit lustslot te bezoeken – Paleis van Wilhelmshöhe – Voorval op de bibliotheek – Schilderyen van Tischbein in de eene vleugel van het gebouw – beschryving van den Leeuwenburg – Burggraaf – Wapenkamer – Kapel – Eetzaal – Ridderzaal – Anecdote van Jerome Napoleon – Wandeling naar de Winterkasten – Octogoon – beschryving van dezelve en van de metalen Hercules – Begin der waterwerken aan de voet van den Octogoon – Kop van Euceladus – Waterorgel en de grot van Polypheem – Zoogenaamde bedriegertjes – Cascade van de Winterkasten – Tweede val van het water – Duivelsbrug – Groote waterval van den Aqueduct – Het springen der groote fonteyn – Verdere wandeling op Wilhelmshöhe – Terugwandeling naar Cassel – Vertrek van een gedeelte van ons reisgezelschap – Waarom een gedeelte gebleven – Slegt weder – Voortreflyk uitzigt van de Kamers van het logement – Afscheid van den Heer van Assen – Vertrek van Cassel – Dikke nevel – Heerlyk gezigt op Munden – Deeze stad is weder op Hannoversch grondgebied – Knalhütte – Sterke daling van eene berg – Bedrieglyke afstand – Aankomst te Göttingen – Bladz 26.</rdfs:comment>
</rdf:Description>

<rdf:Description rdf:about="http://academictourism.com/entity/BRF0004.RS">
	<rdf:type rdf:resource="http://www.w3.org/2002/07/owl#NamedIndividual"/>
	<rdf:type rdf:resource="http://www.cidoc-crm.org/cidoc-crm/E1_CRM_Entity"/>
	<rdf:type rdf:resource="http://www.cidoc-crm.org/cidoc-crm/E2_Temporal_Entity"/>
	<rdf:type rdf:resource="http://www.cidoc-crm.org/cidoc-crm/E4_Period"/>
	<rdf:type rdf:resource="http://www.cidoc-crm.org/cidoc-crm/E5_Event"/>
	<rdf:type rdf:resource="http://www.cidoc-crm.org/cidoc-crm/E7_Activity"/>
	<rdf:type rdf:resource="http://www.cidoc-crm.org/cidoc-crm/E92_Spacetime_Volume"/>
	<rdf:type rdf:resource="http://www.cidoc-crm.org/cidoc-crm/E9_Move"/>
	<rdf:type rdf:resource="http://www.loa-cnr.it/ontologies/DOLCE-Lite#perdurant"/>
	<cidoc-crm:P10i_contains rdf:resource="http://academictourism.com/entity/BRF0004.RS.RS0001"/>
	<cidoc-crm:P10i_contains rdf:resource="http://academictourism.com/entity/BRF0004.RS.RS0002"/>
	<cidoc-crm:P10i_contains rdf:resource="http://academictourism.com/entity/BRF0004.RS.RS0003"/>
	<cidoc-crm:P10i_contains rdf:resource="http://academictourism.com/entity/BRF0004.RS.RS0004"/>
	<cidoc-crm:P10i_contains rdf:resource="http://academictourism.com/entity/BRF0004.RS.RS0005"/>
	<cidoc-crm:P10i_contains rdf:resource="http://academictourism.com/entity/BRF0004.RS.RS0006"/>
	<cidoc-crm:P11_had_participant rdf:resource="http://academictourism.com/entity/TG"/>
	<cidoc-crm:P129i_is_subject_of rdf:resource="http://academictourism.com/entity/BRF0004"/>
	<cidoc-crm:P12_occurred_in_the_presence_of rdf:resource="http://academictourism.com/entity/TG"/>
	<cidoc-crm:P132_spatiotemporally_overlaps_with rdf:resource="http://academictourism.com/entity/BRF0004.RS.RS0001"/>
	<cidoc-crm:P132_spatiotemporally_overlaps_with rdf:resource="http://academictourism.com/entity/BRF0004.RS.RS0002"/>
	<cidoc-crm:P132_spatiotemporally_overlaps_with rdf:resource="http://academictourism.com/entity/BRF0004.RS.RS0003"/>
	<cidoc-crm:P132_spatiotemporally_overlaps_with rdf:resource="http://academictourism.com/entity/BRF0004.RS.RS0004"/>
	<cidoc-crm:P132_spatiotemporally_overlaps_with rdf:resource="http://academictourism.com/entity/BRF0004.RS.RS0005"/>
	<cidoc-crm:P132_spatiotemporally_overlaps_with rdf:resource="http://academictourism.com/entity/BRF0004.RS.RS0006"/>
	<cidoc-crm:P173_starts_before_or_with_the_end_of rdf:resource="http://academictourism.com/entity/BRF0005.RS"/>
	<cidoc-crm:P173i_ends_after_or_with_the_start_of rdf:resource="http://academictourism.com/entity/J0002"/>
	<cidoc-crm:P174_starts_before_the_end_of rdf:resource="http://academictourism.com/entity/BRF0005.RS"/>
	<cidoc-crm:P174i_ends_after_the_start_of rdf:resource="http://academictourism.com/entity/J0002"/>
	<cidoc-crm:P175_starts_before_or_with_the_start_of rdf:resource="http://academictourism.com/entity/BRF0005.RS"/>
	<cidoc-crm:P175i_starts_after_or_with_the_start_of rdf:resource="http://academictourism.com/entity/J0002"/>
	<cidoc-crm:P176_starts_before_the_start_of rdf:resource="http://academictourism.com/entity/BRF0005.RS"/>
	<cidoc-crm:P176i_starts_after_the_start_of rdf:resource="http://academictourism.com/entity/J0002"/>
	<cidoc-crm:P182_ends_before_or_with_the_start_of rdf:resource="http://academictourism.com/entity/BRF0005.RS"/>
	<cidoc-crm:P182i_starts_after_or_with_the_end_of rdf:resource="http://academictourism.com/entity/J0002"/>
	<cidoc-crm:P183_ends_before_the_start_of rdf:resource="http://academictourism.com/entity/BRF0005.RS"/>
	<cidoc-crm:P183i_starts_after_the_end_of rdf:resource="http://academictourism.com/entity/J0002"/>
	<cidoc-crm:P184_ends_before_or_with_the_end_of rdf:resource="http://academictourism.com/entity/BRF0005.RS"/>
	<cidoc-crm:P184i_ends_with_or_after_the_end_of rdf:resource="http://academictourism.com/entity/J0002"/>
	<cidoc-crm:P185_ends_before_the_end_of rdf:resource="http://academictourism.com/entity/BRF0005.RS"/>
	<cidoc-crm:P185i_ends_after_the_end_of rdf:resource="http://academictourism.com/entity/J0002"/>
	<cidoc-crm:P26_moved_to rdf:resource="http://academictourism.com/entity/LOC0002"/>
	<cidoc-crm:P27_moved_from rdf:resource="http://academictourism.com/entity/LOC0001"/>
	<cidoc-crm:P67i_is_referred_to_by rdf:resource="http://academictourism.com/entity/BRF0004"/>
	<rdfs:label>Tour in letter 4</rdfs:label>
</rdf:Description>

<rdf:Description rdf:about="http://academictourism.com/entity/BRF0004.RS.RS0001">
	<rdf:type rdf:resource="http://www.w3.org/2002/07/owl#NamedIndividual"/>
	<rdf:type rdf:resource="http://www.cidoc-crm.org/cidoc-crm/E1_CRM_Entity"/>
	<rdf:type rdf:resource="http://www.cidoc-crm.org/cidoc-crm/E2_Temporal_Entity"/>
	<rdf:type rdf:resource="http://www.cidoc-crm.org/cidoc-crm/E4_Period"/>
	<rdf:type rdf:resource="http://www.cidoc-crm.org/cidoc-crm/E5_Event"/>
	<rdf:type rdf:resource="http://www.cidoc-crm.org/cidoc-crm/E7_Activity"/>
	<rdf:type rdf:resource="http://www.cidoc-crm.org/cidoc-crm/E92_Spacetime_Volume"/>
	<rdf:type rdf:resource="http://www.cidoc-crm.org/cidoc-crm/E9_Move"/>
	<rdf:type rdf:resource="http://www.loa-cnr.it/ontologies/DOLCE-Lite#perdurant"/>
	<cidoc-crm:P10_falls_within rdf:resource="http://academictourism.com/entity/BRF0004.RS"/>
	<cidoc-crm:P11_had_participant rdf:resource="http://academictourism.com/entity/TG"/>
	<cidoc-crm:P12_occurred_in_the_presence_of rdf:resource="http://academictourism.com/entity/MISC0001"/>
	<cidoc-crm:P12_occurred_in_the_presence_of rdf:resource="http://academictourism.com/entity/TG"/>
	<cidoc-crm:P132_spatiotemporally_overlaps_with rdf:resource="http://academictourism.com/entity/BRF0004.RS"/>
	<cidoc-crm:P173_starts_before_or_with_the_end_of rdf:resource="http://academictourism.com/entity/BRF0004.RS.RS0002"/>
	<cidoc-crm:P174_starts_before_the_end_of rdf:resource="http://academictourism.com/entity/BRF0004.RS.RS0002"/>
	<cidoc-crm:P175_starts_before_or_with_the_start_of rdf:resource="http://academictourism.com/entity/BRF0004.RS.RS0002"/>
	<cidoc-crm:P176_starts_before_the_start_of rdf:resource="http://academictourism.com/entity/BRF0004.RS.RS0002"/>
	<cidoc-crm:P182_ends_before_or_with_the_start_of rdf:resource="http://academictourism.com/entity/BRF0004.RS.RS0002"/>
	<cidoc-crm:P183_ends_before_the_start_of rdf:resource="http://academictourism.com/entity/BRF0004.RS.RS0002"/>
	<cidoc-crm:P184_ends_before_or_with_the_end_of rdf:resource="http://academictourism.com/entity/BRF0004.RS.RS0002"/>
	<cidoc-crm:P185_ends_before_the_end_of rdf:resource="http://academictourism.com/entity/BRF0004.RS.RS0002"/>
	<cidoc-crm:P26_moved_to rdf:resource="http://academictourism.com/entity/LOC0003.CS"/>
	<cidoc-crm:P27_moved_from rdf:resource="http://academictourism.com/entity/LOC0001"/>
	<cidoc-crm:P2_has_type rdf:resource="http://vocab.getty.edu/page/aat/300248181"/>
	<cidoc-crm:P4_has_time-span rdf:resource="http://academictourism.com/entity/TS.BRF0004.RS.RS0001"/>
	<rdfs:label>Move from Kassel to Wilhelmshöhe</rdfs:label>
</rdf:Description>

<rdf:Description rdf:about="http://academictourism.com/entity/BRF0004.RS.RS0002">
	<rdf:type rdf:resource="http://www.w3.org/2002/07/owl#NamedIndividual"/>
	<rdf:type rdf:resource="http://www.cidoc-crm.org/cidoc-crm/E1_CRM_Entity"/>
	<rdf:type rdf:resource="http://www.cidoc-crm.org/cidoc-crm/E2_Temporal_Entity"/>
	<rdf:type rdf:resource="http://www.cidoc-crm.org/cidoc-crm/E4_Period"/>
	<rdf:type rdf:resource="http://www.cidoc-crm.org/cidoc-crm/E5_Event"/>
	<rdf:type rdf:resource="http://www.cidoc-crm.org/cidoc-crm/E7_Activity"/>
	<rdf:type rdf:resource="http://www.cidoc-crm.org/cidoc-crm/E92_Spacetime_Volume"/>
	<rdf:type rdf:resource="http://www.loa-cnr.it/ontologies/DOLCE-Lite#perdurant"/>
	<cidoc-crm:P10_falls_within rdf:resource="http://academictourism.com/entity/BRF0004.RS"/>
	<cidoc-crm:P10i_contains rdf:resource="http://academictourism.com/entity/BRF0004.RS.RS0002.RS0001"/>
	<cidoc-crm:P10i_contains rdf:resource="http://academictourism.com/entity/BRF0004.RS.RS0002.RS0002"/>
	<cidoc-crm:P10i_contains rdf:resource="http://academictourism.com/entity/BRF0004.RS.RS0002.RS0003"/>
	<cidoc-crm:P11_had_participant rdf:resource="http://academictourism.com/entity/TG"/>
	<cidoc-crm:P12_occurred_in_the_presence_of rdf:resource="http://academictourism.com/entity/TG"/>
	<cidoc-crm:P132_spatiotemporally_overlaps_with rdf:resource="http://academictourism.com/entity/BRF0004.RS"/>
	<cidoc-crm:P132_spatiotemporally_overlaps_with rdf:resource="http://academictourism.com/entity/BRF0004.RS.RS0002.RS0001"/>
	<cidoc-crm:P132_spatiotemporally_overlaps_with rdf:resource="http://academictourism.com/entity/BRF0004.RS.RS0002.RS0002"/>
	<cidoc-crm:P132_spatiotemporally_overlaps_with rdf:resource="http://academictourism.com/entity/BRF0004.RS.RS0002.RS0003"/>
	<cidoc-crm:P173_starts_before_or_with_the_end_of rdf:resource="http://academictourism.com/entity/BRF0004.RS.RS0003"/>
	<cidoc-crm:P173i_ends_after_or_with_the_start_of rdf:resource="http://academictourism.com/entity/BRF0004.RS.RS0001"/>
	<cidoc-crm:P174_starts_before_the_end_of rdf:resource="http://academictourism.com/entity/BRF0004.RS.RS0003"/>
	<cidoc-crm:P174i_ends_after_the_start_of rdf:resource="http://academictourism.com/entity/BRF0004.RS.RS0001"/>
	<cidoc-crm:P175_starts_before_or_with_the_start_of rdf:resource="http://academictourism.com/entity/BRF0004.RS.RS0003"/>
	<cidoc-crm:P175i_starts_after_or_with_the_start_of rdf:resource="http://academictourism.com/entity/BRF0004.RS.RS0001"/>
	<cidoc-crm:P176_starts_before_the_start_of rdf:resource="http://academictourism.com/entity/BRF0004.RS.RS0003"/>
	<cidoc-crm:P176i_starts_after_the_start_of rdf:resource="http://academictourism.com/entity/BRF0004.RS.RS0001"/>
	<cidoc-crm:P182_ends_before_or_with_the_start_of rdf:resource="http://academictourism.com/entity/BRF0004.RS.RS0003"/>
	<cidoc-crm:P182i_starts_after_or_with_the_end_of rdf:resource="http://academictourism.com/entity/BRF0004.RS.RS0001"/>
	<cidoc-crm:P183_ends_before_the_start_of rdf:resource="http://academictourism.com/entity/BRF0004.RS.RS0003"/>
	<cidoc-crm:P183i_starts_after_the_end_of rdf:resource="http://academictourism.com/entity/BRF0004.RS.RS0001"/>
	<cidoc-crm:P184_ends_before_or_with_the_end_of rdf:resource="http://academictourism.com/entity/BRF0004.RS.RS0003"/>
	<cidoc-crm:P184i_ends_with_or_after_the_end_of rdf:resource="http://academictourism.com/entity/BRF0004.RS.RS0001"/>
	<cidoc-crm:P185_ends_before_the_end_of rdf:resource="http://academictourism.com/entity/BRF0004.RS.RS0003"/>
	<cidoc-crm:P185i_ends_after_the_end_of rdf:resource="http://academictourism.com/entity/BRF0004.RS.RS0001"/>
	<cidoc-crm:P8_took_place_on_or_within rdf:resource="http://academictourism.com/entity/LOC0003.CS"/>
	<rdfs:label>Wilhelmshöhe indoor tour</rdfs:label>
</rdf:Description>

<rdf:Description rdf:about="http://academictourism.com/entity/BRF0004.RS.RS0002.RS0001">
	<rdf:type rdf:resource="http://www.w3.org/2002/07/owl#NamedIndividual"/>
	<rdf:type rdf:resource="http://www.cidoc-crm.org/cidoc-crm/E1_CRM_Entity"/>
	<rdf:type rdf:resource="http://www.cidoc-crm.org/cidoc-crm/E2_Temporal_Entity"/>
	<rdf:type rdf:resource="http://www.cidoc-crm.org/cidoc-crm/E4_Period"/>
	<rdf:type rdf:resource="http://www.cidoc-crm.org/cidoc-crm/E5_Event"/>
	<rdf:type rdf:resource="http://www.cidoc-crm.org/cidoc-crm/E7_Activity"/>
	<rdf:type rdf:resource="http://www.cidoc-crm.org/cidoc-crm/E92_Spacetime_Volume"/>
	<rdf:type rdf:resource="http://www.loa-cnr.it/ontologies/DOLCE-Lite#perdurant"/>
	<cidoc-crm:P10_falls_within rdf:resource="http://academictourism.com/entity/BRF0004.RS.RS0002"/>
	<cidoc-crm:P11_had_participant rdf:resource="http://academictourism.com/entity/TG"/>
	<cidoc-crm:P12_occurred_in_the_presence_of rdf:resource="http://academictourism.com/entity/MISC0002"/>
	<cidoc-crm:P12_occurred_in_the_presence_of rdf:resource="http://academictourism.com/entity/TG"/>
	<cidoc-crm:P132_spatiotemporally_overlaps_with rdf:resource="http://academictourism.com/entity/BRF0004.RS.RS0002"/>
	<cidoc-crm:P173_starts_before_or_with_the_end_of rdf:resource="http://academictourism.com/entity/BRF0004.RS.RS0002.RS0002"/>
	<cidoc-crm:P174_starts_before_the_end_of rdf:resource="http://academictourism.com/entity/BRF0004.RS.RS0002.RS0002"/>
	<cidoc-crm:P175_starts_before_or_with_the_start_of rdf:resource="http://academictourism.com/entity/BRF0004.RS.RS0002.RS0002"/>
	<cidoc-crm:P176_starts_before_the_start_of rdf:resource="http://academictourism.com/entity/BRF0004.RS.RS0002.RS0002"/>
	<cidoc-crm:P182_ends_before_or_with_the_start_of rdf:resource="http://academictourism.com/entity/BRF0004.RS.RS0002.RS0002"/>
	<cidoc-crm:P183_ends_before_the_start_of rdf:resource="http://academictourism.com/entity/BRF0004.RS.RS0002.RS0002"/>
	<cidoc-crm:P184_ends_before_or_with_the_end_of rdf:resource="http://academictourism.com/entity/BRF0004.RS.RS0002.RS0002"/>
	<cidoc-crm:P185_ends_before_the_end_of rdf:resource="http://academictourism.com/entity/BRF0004.RS.RS0002.RS0002"/>
	<cidoc-crm:P7_took_place_at rdf:resource="http://academictourism.com/entity/LOC0003.CS.K001"/>
	<rdfs:label>Tour at Wilhelmshöhe galery</rdfs:label>
</rdf:Description>

<rdf:Description rdf:about="http://academictourism.com/entity/BRF0004.RS.RS0002.RS0002">
	<rdf:type rdf:resource="http://www.w3.org/2002/07/owl#NamedIndividual"/>
	<rdf:type rdf:resource="http://www.cidoc-crm.org/cidoc-crm/E1_CRM_Entity"/>
	<rdf:type rdf:resource="http://www.cidoc-crm.org/cidoc-crm/E2_Temporal_Entity"/>
	<rdf:type rdf:resource="http://www.cidoc-crm.org/cidoc-crm/E4_Period"/>
	<rdf:type rdf:resource="http://www.cidoc-crm.org/cidoc-crm/E5_Event"/>
	<rdf:type rdf:resource="http://www.cidoc-crm.org/cidoc-crm/E7_Activity"/>
	<rdf:type rdf:resource="http://www.cidoc-crm.org/cidoc-crm/E92_Spacetime_Volume"/>
	<rdf:type rdf:resource="http://www.loa-cnr.it/ontologies/DOLCE-Lite#perdurant"/>
	<cidoc-crm:P10_falls_within rdf:resource="http://academictourism.com/entity/BRF0004.RS.RS0002"/>
	<cidoc-crm:P11_had_participant rdf:resource="http://academictourism.com/entity/TG"/>
	<cidoc-crm:P12_occurred_in_the_presence_of rdf:resource="http://academictourism.com/entity/TG"/>
	<cidoc-crm:P132_spatiotemporally_overlaps_with rdf:resource="http://academictourism.com/entity/BRF0004.RS.RS0002"/>
	<cidoc-crm:P173_starts_before_or_with_the_end_of rdf:resource="http://academictourism.com/entity/BRF0004.RS.RS0002.RS0003"/>
	<cidoc-crm:P173i_ends_after_or_with_the_start_of rdf:resource="http://academictourism.com/entity/BRF0004.RS.RS0002.RS0001"/>
	<cidoc-crm:P174_starts_before_the_end_of rdf:resource="http://academictourism.com/entity/BRF0004.RS.RS0002.RS0003"/>
	<cidoc-crm:P174i_ends_after_the_start_of rdf:resource="http://academictourism.com/entity/BRF0004.RS.RS0002.RS0001"/>
	<cidoc-crm:P175_starts_before_or_with_the_start_of rdf:resource="http://academictourism.com/entity/BRF0004.RS.RS0002.RS0003"/>
	<cidoc-crm:P175i_starts_after_or_with_the_start_of rdf:resource="http://academictourism.com/entity/BRF0004.RS.RS0002.RS0001"/>
	<cidoc-crm:P176_starts_before_the_start_of rdf:resource="http://academictourism.com/entity/BRF0004.RS.RS0002.RS0003"/>
	<cidoc-crm:P176i_starts_after_the_start_of rdf:resource="http://academictourism.com/entity/BRF0004.RS.RS0002.RS0001"/>
	<cidoc-crm:P182_ends_before_or_with_the_start_of rdf:resource="http://academictourism.com/entity/BRF0004.RS.RS0002.RS0003"/>
	<cidoc-crm:P182i_starts_after_or_with_the_end_of rdf:resource="http://academictourism.com/entity/BRF0004.RS.RS0002.RS0001"/>
	<cidoc-crm:P183_ends_before_the_start_of rdf:resource="http://academictourism.com/entity/BRF0004.RS.RS0002.RS0003"/>
	<cidoc-crm:P183i_starts_after_the_end_of rdf:resource="http://academictourism.com/entity/BRF0004.RS.RS0002.RS0001"/>
	<cidoc-crm:P184_ends_before_or_with_the_end_of rdf:resource="http://academictourism.com/entity/BRF0004.RS.RS0002.RS0003"/>
	<cidoc-crm:P184i_ends_with_or_after_the_end_of rdf:resource="http://academictourism.com/entity/BRF0004.RS.RS0002.RS0001"/>
	<cidoc-crm:P185_ends_before_the_end_of rdf:resource="http://academictourism.com/entity/BRF0004.RS.RS0002.RS0003"/>
	<cidoc-crm:P185i_ends_after_the_end_of rdf:resource="http://academictourism.com/entity/BRF0004.RS.RS0002.RS0001"/>
	<cidoc-crm:P7_took_place_at rdf:resource="http://academictourism.com/entity/LOC0003.CS.K002"/>
	<rdfs:label>Tour at Wilhelmshöhe slaapkmer</rdfs:label>
</rdf:Description>

<rdf:Description rdf:about="http://academictourism.com/entity/BRF0004.RS.RS0002.RS0003">
	<rdf:type rdf:resource="http://www.w3.org/2002/07/owl#NamedIndividual"/>
	<rdf:type rdf:resource="http://www.cidoc-crm.org/cidoc-crm/E1_CRM_Entity"/>
	<rdf:type rdf:resource="http://www.cidoc-crm.org/cidoc-crm/E2_Temporal_Entity"/>
	<rdf:type rdf:resource="http://www.cidoc-crm.org/cidoc-crm/E4_Period"/>
	<rdf:type rdf:resource="http://www.cidoc-crm.org/cidoc-crm/E5_Event"/>
	<rdf:type rdf:resource="http://www.cidoc-crm.org/cidoc-crm/E7_Activity"/>
	<rdf:type rdf:resource="http://www.cidoc-crm.org/cidoc-crm/E92_Spacetime_Volume"/>
	<rdf:type rdf:resource="http://www.loa-cnr.it/ontologies/DOLCE-Lite#perdurant"/>
	<cidoc-crm:P10_falls_within rdf:resource="http://academictourism.com/entity/BRF0004.RS.RS0002"/>
	<cidoc-crm:P11_had_participant rdf:resource="http://academictourism.com/entity/TG"/>
	<cidoc-crm:P12_occurred_in_the_presence_of rdf:resource="http://academictourism.com/entity/TG"/>
	<cidoc-crm:P132_spatiotemporally_overlaps_with rdf:resource="http://academictourism.com/entity/BRF0004.RS.RS0002"/>
	<cidoc-crm:P173_starts_before_or_with_the_end_of rdf:resource="http://academictourism.com/entity/BRF0004.RS.RS0002.RS0004"/>
	<cidoc-crm:P173i_ends_after_or_with_the_start_of rdf:resource="http://academictourism.com/entity/BRF0004.RS.RS0002.RS0002"/>
	<cidoc-crm:P174_starts_before_the_end_of rdf:resource="http://academictourism.com/entity/BRF0004.RS.RS0002.RS0004"/>
	<cidoc-crm:P174i_ends_after_the_start_of rdf:resource="http://academictourism.com/entity/BRF0004.RS.RS0002.RS0002"/>
	<cidoc-crm:P175_starts_before_or_with_the_start_of rdf:resource="http://academictourism.com/entity/BRF0004.RS.RS0002.RS0004"/>
	<cidoc-crm:P175i_starts_after_or_with_the_start_of rdf:resource="http://academictourism.com/entity/BRF0004.RS.RS0002.RS0002"/>
	<cidoc-crm:P176_starts_before_the_start_of rdf:resource="http://academictourism.com/entity/BRF0004.RS.RS0002.RS0004"/>
	<cidoc-crm:P176i_starts_after_the_start_of rdf:resource="http://academictourism.com/entity/BRF0004.RS.RS0002.RS0002"/>
	<cidoc-crm:P182_ends_before_or_with_the_start_of rdf:resource="http://academictourism.com/entity/BRF0004.RS.RS0002.RS0004"/>
	<cidoc-crm:P182i_starts_after_or_with_the_end_of rdf:resource="http://academictourism.com/entity/BRF0004.RS.RS0002.RS0002"/>
	<cidoc-crm:P183_ends_before_the_start_of rdf:resource="http://academictourism.com/entity/BRF0004.RS.RS0002.RS0004"/>
	<cidoc-crm:P183i_starts_after_the_end_of rdf:resource="http://academictourism.com/entity/BRF0004.RS.RS0002.RS0002"/>
	<cidoc-crm:P184_ends_before_or_with_the_end_of rdf:resource="http://academictourism.com/entity/BRF0004.RS.RS0002.RS0004"/>
	<cidoc-crm:P184i_ends_with_or_after_the_end_of rdf:resource="http://academictourism.com/entity/BRF0004.RS.RS0002.RS0002"/>
	<cidoc-crm:P185_ends_before_the_end_of rdf:resource="http://academictourism.com/entity/BRF0004.RS.RS0002.RS0004"/>
	<cidoc-crm:P185i_ends_after_the_end_of rdf:resource="http://academictourism.com/entity/BRF0004.RS.RS0002.RS0002"/>
	<cidoc-crm:P7_took_place_at rdf:resource="http://academictourism.com/entity/LOC0003.CS.K003"/>
	<rdfs:label>Tour at Wilhelmshöhe bibiliotheek</rdfs:label>
</rdf:Description>

<rdf:Description rdf:about="http://academictourism.com/entity/BRF0004.RS.RS0002.RS0004">
	<rdf:type rdf:resource="http://www.w3.org/2002/07/owl#NamedIndividual"/>
	<rdf:type rdf:resource="http://www.cidoc-crm.org/cidoc-crm/E1_CRM_Entity"/>
	<rdf:type rdf:resource="http://www.cidoc-crm.org/cidoc-crm/E2_Temporal_Entity"/>
	<rdf:type rdf:resource="http://www.cidoc-crm.org/cidoc-crm/E4_Period"/>
	<rdf:type rdf:resource="http://www.cidoc-crm.org/cidoc-crm/E5_Event"/>
	<rdf:type rdf:resource="http://www.cidoc-crm.org/cidoc-crm/E7_Activity"/>
	<rdf:type rdf:resource="http://www.cidoc-crm.org/cidoc-crm/E92_Spacetime_Volume"/>
	<rdf:type rdf:resource="http://www.loa-cnr.it/ontologies/DOLCE-Lite#perdurant"/>
	<cidoc-crm:P12_occurred_in_the_presence_of rdf:resource="http://academictourism.com/entity/MISC0003"/>
	<cidoc-crm:P173i_ends_after_or_with_the_start_of rdf:resource="http://academictourism.com/entity/BRF0004.RS.RS0002.RS0003"/>
	<cidoc-crm:P174i_ends_after_the_start_of rdf:resource="http://academictourism.com/entity/BRF0004.RS.RS0002.RS0003"/>
	<cidoc-crm:P175i_starts_after_or_with_the_start_of rdf:resource="http://academictourism.com/entity/BRF0004.RS.RS0002.RS0003"/>
	<cidoc-crm:P176i_starts_after_the_start_of rdf:resource="http://academictourism.com/entity/BRF0004.RS.RS0002.RS0003"/>
	<cidoc-crm:P182i_starts_after_or_with_the_end_of rdf:resource="http://academictourism.com/entity/BRF0004.RS.RS0002.RS0003"/>
	<cidoc-crm:P183i_starts_after_the_end_of rdf:resource="http://academictourism.com/entity/BRF0004.RS.RS0002.RS0003"/>
	<cidoc-crm:P184i_ends_with_or_after_the_end_of rdf:resource="http://academictourism.com/entity/BRF0004.RS.RS0002.RS0003"/>
	<cidoc-crm:P185i_ends_after_the_end_of rdf:resource="http://academictourism.com/entity/BRF0004.RS.RS0002.RS0003"/>
	<cidoc-crm:P7_took_place_at rdf:resource="http://academictourism.com/entity/LOC0003.CS.K004"/>
</rdf:Description>

<rdf:Description rdf:about="http://academictourism.com/entity/BRF0004.RS.RS0003">
	<rdf:type rdf:resource="http://www.w3.org/2002/07/owl#NamedIndividual"/>
	<rdf:type rdf:resource="http://www.cidoc-crm.org/cidoc-crm/E1_CRM_Entity"/>
	<rdf:type rdf:resource="http://www.cidoc-crm.org/cidoc-crm/E2_Temporal_Entity"/>
	<rdf:type rdf:resource="http://www.cidoc-crm.org/cidoc-crm/E4_Period"/>
	<rdf:type rdf:resource="http://www.cidoc-crm.org/cidoc-crm/E5_Event"/>
	<rdf:type rdf:resource="http://www.cidoc-crm.org/cidoc-crm/E7_Activity"/>
	<rdf:type rdf:resource="http://www.cidoc-crm.org/cidoc-crm/E92_Spacetime_Volume"/>
	<rdf:type rdf:resource="http://www.loa-cnr.it/ontologies/DOLCE-Lite#perdurant"/>
	<cidoc-crm:P10_falls_within rdf:resource="http://academictourism.com/entity/BRF0004.RS"/>
	<cidoc-crm:P11_had_participant rdf:resource="http://academictourism.com/entity/TG"/>
	<cidoc-crm:P12_occurred_in_the_presence_of rdf:resource="http://academictourism.com/entity/LOC0004.CS"/>
	<cidoc-crm:P12_occurred_in_the_presence_of rdf:resource="http://academictourism.com/entity/MISC0004"/>
	<cidoc-crm:P12_occurred_in_the_presence_of rdf:resource="http://academictourism.com/entity/MISC0005"/>
	<cidoc-crm:P12_occurred_in_the_presence_of rdf:resource="http://academictourism.com/entity/MISC0006"/>
	<cidoc-crm:P12_occurred_in_the_presence_of rdf:resource="http://academictourism.com/entity/TG"/>
	<cidoc-crm:P132_spatiotemporally_overlaps_with rdf:resource="http://academictourism.com/entity/BRF0004.RS"/>
	<cidoc-crm:P173_starts_before_or_with_the_end_of rdf:resource="http://academictourism.com/entity/BRF0004.RS.RS0004"/>
	<cidoc-crm:P173i_ends_after_or_with_the_start_of rdf:resource="http://academictourism.com/entity/BRF0004.RS.RS0002"/>
	<cidoc-crm:P174_starts_before_the_end_of rdf:resource="http://academictourism.com/entity/BRF0004.RS.RS0004"/>
	<cidoc-crm:P174i_ends_after_the_start_of rdf:resource="http://academictourism.com/entity/BRF0004.RS.RS0002"/>
	<cidoc-crm:P175_starts_before_or_with_the_start_of rdf:resource="http://academictourism.com/entity/BRF0004.RS.RS0004"/>
	<cidoc-crm:P175i_starts_after_or_with_the_start_of rdf:resource="http://academictourism.com/entity/BRF0004.RS.RS0002"/>
	<cidoc-crm:P176_starts_before_the_start_of rdf:resource="http://academictourism.com/entity/BRF0004.RS.RS0004"/>
	<cidoc-crm:P176i_starts_after_the_start_of rdf:resource="http://academictourism.com/entity/BRF0004.RS.RS0002"/>
	<cidoc-crm:P182_ends_before_or_with_the_start_of rdf:resource="http://academictourism.com/entity/BRF0004.RS.RS0004"/>
	<cidoc-crm:P182i_starts_after_or_with_the_end_of rdf:resource="http://academictourism.com/entity/BRF0004.RS.RS0002"/>
	<cidoc-crm:P183_ends_before_the_start_of rdf:resource="http://academictourism.com/entity/BRF0004.RS.RS0004"/>
	<cidoc-crm:P183i_starts_after_the_end_of rdf:resource="http://academictourism.com/entity/BRF0004.RS.RS0002"/>
	<cidoc-crm:P184_ends_before_or_with_the_end_of rdf:resource="http://academictourism.com/entity/BRF0004.RS.RS0004"/>
	<cidoc-crm:P184i_ends_with_or_after_the_end_of rdf:resource="http://academictourism.com/entity/BRF0004.RS.RS0002"/>
	<cidoc-crm:P185_ends_before_the_end_of rdf:resource="http://academictourism.com/entity/BRF0004.RS.RS0004"/>
	<cidoc-crm:P185i_ends_after_the_end_of rdf:resource="http://academictourism.com/entity/BRF0004.RS.RS0002"/>
	<cidoc-crm:P7_took_place_at rdf:resource="http://academictourism.com/entity/LOC0004.CS"/>
	<cidoc-crm:P8_took_place_on_or_within rdf:resource="http://academictourism.com/entity/LOC0004.CS"/>
	<rdfs:label>Leeuwenburg tour</rdfs:label>
</rdf:Description>

<rdf:Description rdf:about="http://academictourism.com/entity/BRF0004.RS.RS0003.RS0001">
	<rdf:type rdf:resource="http://www.w3.org/2002/07/owl#NamedIndividual"/>
	<rdf:type rdf:resource="http://www.cidoc-crm.org/cidoc-crm/E1_CRM_Entity"/>
	<rdf:type rdf:resource="http://www.cidoc-crm.org/cidoc-crm/E2_Temporal_Entity"/>
	<rdf:type rdf:resource="http://www.cidoc-crm.org/cidoc-crm/E4_Period"/>
	<rdf:type rdf:resource="http://www.cidoc-crm.org/cidoc-crm/E5_Event"/>
	<rdf:type rdf:resource="http://www.cidoc-crm.org/cidoc-crm/E7_Activity"/>
	<rdf:type rdf:resource="http://www.cidoc-crm.org/cidoc-crm/E92_Spacetime_Volume"/>
	<rdf:type rdf:resource="http://www.loa-cnr.it/ontologies/DOLCE-Lite#perdurant"/>
	<cidoc-crm:P173_starts_before_or_with_the_end_of rdf:resource="http://academictourism.com/entity/BRF0004.RS.RS0003.RS0002"/>
	<cidoc-crm:P174_starts_before_the_end_of rdf:resource="http://academictourism.com/entity/BRF0004.RS.RS0003.RS0002"/>
	<cidoc-crm:P175_starts_before_or_with_the_start_of rdf:resource="http://academictourism.com/entity/BRF0004.RS.RS0003.RS0002"/>
	<cidoc-crm:P176_starts_before_the_start_of rdf:resource="http://academictourism.com/entity/BRF0004.RS.RS0003.RS0002"/>
	<cidoc-crm:P182_ends_before_or_with_the_start_of rdf:resource="http://academictourism.com/entity/BRF0004.RS.RS0003.RS0002"/>
	<cidoc-crm:P183_ends_before_the_start_of rdf:resource="http://academictourism.com/entity/BRF0004.RS.RS0003.RS0002"/>
	<cidoc-crm:P184_ends_before_or_with_the_end_of rdf:resource="http://academictourism.com/entity/BRF0004.RS.RS0003.RS0002"/>
	<cidoc-crm:P185_ends_before_the_end_of rdf:resource="http://academictourism.com/entity/BRF0004.RS.RS0003.RS0002"/>
	<cidoc-crm:P7_took_place_at rdf:resource="http://academictourism.com/entity/LOC0004.CS.K001"/>
	<rdfs:label>Tour at Löwenburg Chaple</rdfs:label>
</rdf:Description>

<rdf:Description rdf:about="http://academictourism.com/entity/BRF0004.RS.RS0003.RS0002">
	<rdf:type rdf:resource="http://www.w3.org/2002/07/owl#NamedIndividual"/>
	<rdf:type rdf:resource="http://www.cidoc-crm.org/cidoc-crm/E1_CRM_Entity"/>
	<rdf:type rdf:resource="http://www.cidoc-crm.org/cidoc-crm/E2_Temporal_Entity"/>
	<rdf:type rdf:resource="http://www.cidoc-crm.org/cidoc-crm/E4_Period"/>
	<rdf:type rdf:resource="http://www.cidoc-crm.org/cidoc-crm/E5_Event"/>
	<rdf:type rdf:resource="http://www.cidoc-crm.org/cidoc-crm/E7_Activity"/>
	<rdf:type rdf:resource="http://www.cidoc-crm.org/cidoc-crm/E92_Spacetime_Volume"/>
	<rdf:type rdf:resource="http://www.loa-cnr.it/ontologies/DOLCE-Lite#perdurant"/>
	<cidoc-crm:P12_occurred_in_the_presence_of rdf:resource="http://academictourism.com/entity/MISC0004"/>
	<cidoc-crm:P12_occurred_in_the_presence_of rdf:resource="http://academictourism.com/entity/MISC0005"/>
	<cidoc-crm:P173_starts_before_or_with_the_end_of rdf:resource="http://academictourism.com/entity/BRF0004.RS.RS0003.RS0003"/>
	<cidoc-crm:P173i_ends_after_or_with_the_start_of rdf:resource="http://academictourism.com/entity/BRF0004.RS.RS0003.RS0001"/>
	<cidoc-crm:P174_starts_before_the_end_of rdf:resource="http://academictourism.com/entity/BRF0004.RS.RS0003.RS0003"/>
	<cidoc-crm:P174i_ends_after_the_start_of rdf:resource="http://academictourism.com/entity/BRF0004.RS.RS0003.RS0001"/>
	<cidoc-crm:P175_starts_before_or_with_the_start_of rdf:resource="http://academictourism.com/entity/BRF0004.RS.RS0003.RS0003"/>
	<cidoc-crm:P175i_starts_after_or_with_the_start_of rdf:resource="http://academictourism.com/entity/BRF0004.RS.RS0003.RS0001"/>
	<cidoc-crm:P176_starts_before_the_start_of rdf:resource="http://academictourism.com/entity/BRF0004.RS.RS0003.RS0003"/>
	<cidoc-crm:P176i_starts_after_the_start_of rdf:resource="http://academictourism.com/entity/BRF0004.RS.RS0003.RS0001"/>
	<cidoc-crm:P182_ends_before_or_with_the_start_of rdf:resource="http://academictourism.com/entity/BRF0004.RS.RS0003.RS0003"/>
	<cidoc-crm:P182i_starts_after_or_with_the_end_of rdf:resource="http://academictourism.com/entity/BRF0004.RS.RS0003.RS0001"/>
	<cidoc-crm:P183_ends_before_the_start_of rdf:resource="http://academictourism.com/entity/BRF0004.RS.RS0003.RS0003"/>
	<cidoc-crm:P183i_starts_after_the_end_of rdf:resource="http://academictourism.com/entity/BRF0004.RS.RS0003.RS0001"/>
	<cidoc-crm:P184_ends_before_or_with_the_end_of rdf:resource="http://academictourism.com/entity/BRF0004.RS.RS0003.RS0003"/>
	<cidoc-crm:P184i_ends_with_or_after_the_end_of rdf:resource="http://academictourism.com/entity/BRF0004.RS.RS0003.RS0001"/>
	<cidoc-crm:P185_ends_before_the_end_of rdf:resource="http://academictourism.com/entity/BRF0004.RS.RS0003.RS0003"/>
	<cidoc-crm:P185i_ends_after_the_end_of rdf:resource="http://academictourism.com/entity/BRF0004.RS.RS0003.RS0001"/>
	<cidoc-crm:P7_took_place_at rdf:resource="http://academictourism.com/entity/LOC0004.CS.K002"/>
	<rdfs:label>Tour at Löwenburg Main building</rdfs:label>
</rdf:Description>

<rdf:Description rdf:about="http://academictourism.com/entity/BRF0004.RS.RS0003.RS0003">
	<rdf:type rdf:resource="http://www.w3.org/2002/07/owl#NamedIndividual"/>
	<rdf:type rdf:resource="http://www.cidoc-crm.org/cidoc-crm/E1_CRM_Entity"/>
	<rdf:type rdf:resource="http://www.cidoc-crm.org/cidoc-crm/E2_Temporal_Entity"/>
	<rdf:type rdf:resource="http://www.cidoc-crm.org/cidoc-crm/E4_Period"/>
	<rdf:type rdf:resource="http://www.cidoc-crm.org/cidoc-crm/E5_Event"/>
	<rdf:type rdf:resource="http://www.cidoc-crm.org/cidoc-crm/E7_Activity"/>
	<rdf:type rdf:resource="http://www.cidoc-crm.org/cidoc-crm/E92_Spacetime_Volume"/>
	<rdf:type rdf:resource="http://www.loa-cnr.it/ontologies/DOLCE-Lite#perdurant"/>
	<cidoc-crm:P173_starts_before_or_with_the_end_of rdf:resource="http://academictourism.com/entity/BRF0004.RS.RS0003.RS0004"/>
	<cidoc-crm:P173i_ends_after_or_with_the_start_of rdf:resource="http://academictourism.com/entity/BRF0004.RS.RS0003.RS0002"/>
	<cidoc-crm:P174_starts_before_the_end_of rdf:resource="http://academictourism.com/entity/BRF0004.RS.RS0003.RS0004"/>
	<cidoc-crm:P174i_ends_after_the_start_of rdf:resource="http://academictourism.com/entity/BRF0004.RS.RS0003.RS0002"/>
	<cidoc-crm:P175_starts_before_or_with_the_start_of rdf:resource="http://academictourism.com/entity/BRF0004.RS.RS0003.RS0004"/>
	<cidoc-crm:P175i_starts_after_or_with_the_start_of rdf:resource="http://academictourism.com/entity/BRF0004.RS.RS0003.RS0002"/>
	<cidoc-crm:P176_starts_before_the_start_of rdf:resource="http://academictourism.com/entity/BRF0004.RS.RS0003.RS0004"/>
	<cidoc-crm:P176i_starts_after_the_start_of rdf:resource="http://academictourism.com/entity/BRF0004.RS.RS0003.RS0002"/>
	<cidoc-crm:P182_ends_before_or_with_the_start_of rdf:resource="http://academictourism.com/entity/BRF0004.RS.RS0003.RS0004"/>
	<cidoc-crm:P182i_starts_after_or_with_the_end_of rdf:resource="http://academictourism.com/entity/BRF0004.RS.RS0003.RS0002"/>
	<cidoc-crm:P183_ends_before_the_start_of rdf:resource="http://academictourism.com/entity/BRF0004.RS.RS0003.RS0004"/>
	<cidoc-crm:P183i_starts_after_the_end_of rdf:resource="http://academictourism.com/entity/BRF0004.RS.RS0003.RS0002"/>
	<cidoc-crm:P184_ends_before_or_with_the_end_of rdf:resource="http://academictourism.com/entity/BRF0004.RS.RS0003.RS0004"/>
	<cidoc-crm:P184i_ends_with_or_after_the_end_of rdf:resource="http://academictourism.com/entity/BRF0004.RS.RS0003.RS0002"/>
	<cidoc-crm:P185_ends_before_the_end_of rdf:resource="http://academictourism.com/entity/BRF0004.RS.RS0003.RS0004"/>
	<cidoc-crm:P185i_ends_after_the_end_of rdf:resource="http://academictourism.com/entity/BRF0004.RS.RS0003.RS0002"/>
	<cidoc-crm:P7_took_place_at rdf:resource="http://academictourism.com/entity/LOC0004.CS.K003"/>
	<rdfs:label>Tour at Löwenburg Dining Hall</rdfs:label>
</rdf:Description>

<rdf:Description rdf:about="http://academictourism.com/entity/BRF0004.RS.RS0003.RS0004">
	<rdf:type rdf:resource="http://www.w3.org/2002/07/owl#NamedIndividual"/>
	<rdf:type rdf:resource="http://www.cidoc-crm.org/cidoc-crm/E1_CRM_Entity"/>
	<rdf:type rdf:resource="http://www.cidoc-crm.org/cidoc-crm/E2_Temporal_Entity"/>
	<rdf:type rdf:resource="http://www.cidoc-crm.org/cidoc-crm/E4_Period"/>
	<rdf:type rdf:resource="http://www.cidoc-crm.org/cidoc-crm/E5_Event"/>
	<rdf:type rdf:resource="http://www.cidoc-crm.org/cidoc-crm/E7_Activity"/>
	<rdf:type rdf:resource="http://www.cidoc-crm.org/cidoc-crm/E92_Spacetime_Volume"/>
	<rdf:type rdf:resource="http://www.loa-cnr.it/ontologies/DOLCE-Lite#perdurant"/>
	<cidoc-crm:P173_starts_before_or_with_the_end_of rdf:resource="http://academictourism.com/entity/BRF0004.RS.RS0003.RS0005"/>
	<cidoc-crm:P173i_ends_after_or_with_the_start_of rdf:resource="http://academictourism.com/entity/BRF0004.RS.RS0003.RS0003"/>
	<cidoc-crm:P174_starts_before_the_end_of rdf:resource="http://academictourism.com/entity/BRF0004.RS.RS0003.RS0005"/>
	<cidoc-crm:P174i_ends_after_the_start_of rdf:resource="http://academictourism.com/entity/BRF0004.RS.RS0003.RS0003"/>
	<cidoc-crm:P175_starts_before_or_with_the_start_of rdf:resource="http://academictourism.com/entity/BRF0004.RS.RS0003.RS0005"/>
	<cidoc-crm:P175i_starts_after_or_with_the_start_of rdf:resource="http://academictourism.com/entity/BRF0004.RS.RS0003.RS0003"/>
	<cidoc-crm:P176_starts_before_the_start_of rdf:resource="http://academictourism.com/entity/BRF0004.RS.RS0003.RS0005"/>
	<cidoc-crm:P176i_starts_after_the_start_of rdf:resource="http://academictourism.com/entity/BRF0004.RS.RS0003.RS0003"/>
	<cidoc-crm:P182_ends_before_or_with_the_start_of rdf:resource="http://academictourism.com/entity/BRF0004.RS.RS0003.RS0005"/>
	<cidoc-crm:P182i_starts_after_or_with_the_end_of rdf:resource="http://academictourism.com/entity/BRF0004.RS.RS0003.RS0003"/>
	<cidoc-crm:P183_ends_before_the_start_of rdf:resource="http://academictourism.com/entity/BRF0004.RS.RS0003.RS0005"/>
	<cidoc-crm:P183i_starts_after_the_end_of rdf:resource="http://academictourism.com/entity/BRF0004.RS.RS0003.RS0003"/>
	<cidoc-crm:P184_ends_before_or_with_the_end_of rdf:resource="http://academictourism.com/entity/BRF0004.RS.RS0003.RS0005"/>
	<cidoc-crm:P184i_ends_with_or_after_the_end_of rdf:resource="http://academictourism.com/entity/BRF0004.RS.RS0003.RS0003"/>
	<cidoc-crm:P185_ends_before_the_end_of rdf:resource="http://academictourism.com/entity/BRF0004.RS.RS0003.RS0005"/>
	<cidoc-crm:P185i_ends_after_the_end_of rdf:resource="http://academictourism.com/entity/BRF0004.RS.RS0003.RS0003"/>
	<cidoc-crm:P7_took_place_at rdf:resource="http://academictourism.com/entity/LOC0004.CS.K004"/>
	<rdfs:label>Tour at Löwenburg Knights' Hall</rdfs:label>
</rdf:Description>

<rdf:Description rdf:about="http://academictourism.com/entity/BRF0004.RS.RS0003.RS0005">
	<rdf:type rdf:resource="http://www.w3.org/2002/07/owl#NamedIndividual"/>
	<rdf:type rdf:resource="http://www.cidoc-crm.org/cidoc-crm/E1_CRM_Entity"/>
	<rdf:type rdf:resource="http://www.cidoc-crm.org/cidoc-crm/E2_Temporal_Entity"/>
	<rdf:type rdf:resource="http://www.cidoc-crm.org/cidoc-crm/E4_Period"/>
	<rdf:type rdf:resource="http://www.cidoc-crm.org/cidoc-crm/E5_Event"/>
	<rdf:type rdf:resource="http://www.cidoc-crm.org/cidoc-crm/E7_Activity"/>
	<rdf:type rdf:resource="http://www.cidoc-crm.org/cidoc-crm/E92_Spacetime_Volume"/>
	<rdf:type rdf:resource="http://www.loa-cnr.it/ontologies/DOLCE-Lite#perdurant"/>
	<cidoc-crm:P173i_ends_after_or_with_the_start_of rdf:resource="http://academictourism.com/entity/BRF0004.RS.RS0003.RS0004"/>
	<cidoc-crm:P174i_ends_after_the_start_of rdf:resource="http://academictourism.com/entity/BRF0004.RS.RS0003.RS0004"/>
	<cidoc-crm:P175i_starts_after_or_with_the_start_of rdf:resource="http://academictourism.com/entity/BRF0004.RS.RS0003.RS0004"/>
	<cidoc-crm:P176i_starts_after_the_start_of rdf:resource="http://academictourism.com/entity/BRF0004.RS.RS0003.RS0004"/>
	<cidoc-crm:P182i_starts_after_or_with_the_end_of rdf:resource="http://academictourism.com/entity/BRF0004.RS.RS0003.RS0004"/>
	<cidoc-crm:P183i_starts_after_the_end_of rdf:resource="http://academictourism.com/entity/BRF0004.RS.RS0003.RS0004"/>
	<cidoc-crm:P184i_ends_with_or_after_the_end_of rdf:resource="http://academictourism.com/entity/BRF0004.RS.RS0003.RS0004"/>
	<cidoc-crm:P185i_ends_after_the_end_of rdf:resource="http://academictourism.com/entity/BRF0004.RS.RS0003.RS0004"/>
	<cidoc-crm:P7_took_place_at rdf:resource="http://academictourism.com/entity/LOC0004.CS.K005"/>
	<rdfs:label>Tour at Löwenburg Library</rdfs:label>
</rdf:Description>

<rdf:Description rdf:about="http://academictourism.com/entity/BRF0004.RS.RS0004">
	<rdf:type rdf:resource="http://www.w3.org/2002/07/owl#NamedIndividual"/>
	<rdf:type rdf:resource="http://www.cidoc-crm.org/cidoc-crm/E1_CRM_Entity"/>
	<rdf:type rdf:resource="http://www.cidoc-crm.org/cidoc-crm/E2_Temporal_Entity"/>
	<rdf:type rdf:resource="http://www.cidoc-crm.org/cidoc-crm/E4_Period"/>
	<rdf:type rdf:resource="http://www.cidoc-crm.org/cidoc-crm/E5_Event"/>
	<rdf:type rdf:resource="http://www.cidoc-crm.org/cidoc-crm/E7_Activity"/>
	<rdf:type rdf:resource="http://www.cidoc-crm.org/cidoc-crm/E92_Spacetime_Volume"/>
	<rdf:type rdf:resource="http://www.loa-cnr.it/ontologies/DOLCE-Lite#perdurant"/>
	<cidoc-crm:P10_falls_within rdf:resource="http://academictourism.com/entity/BRF0004.RS"/>
	<cidoc-crm:P10i_contains rdf:resource="http://academictourism.com/entity/BRF0004.RS.RS0004.RS0001"/>
	<cidoc-crm:P10i_contains rdf:resource="http://academictourism.com/entity/BRF0004.RS.RS0004.RS0002"/>
	<cidoc-crm:P10i_contains rdf:resource="http://academictourism.com/entity/BRF0004.RS.RS0004.RS0003"/>
	<cidoc-crm:P10i_contains rdf:resource="http://academictourism.com/entity/BRF0004.RS.RS0004.RS0004"/>
	<cidoc-crm:P11_had_participant rdf:resource="http://academictourism.com/entity/TG"/>
	<cidoc-crm:P12_occurred_in_the_presence_of rdf:resource="http://academictourism.com/entity/TG"/>
	<cidoc-crm:P132_spatiotemporally_overlaps_with rdf:resource="http://academictourism.com/entity/BRF0004.RS"/>
	<cidoc-crm:P132_spatiotemporally_overlaps_with rdf:resource="http://academictourism.com/entity/BRF0004.RS.RS0004.RS0001"/>
	<cidoc-crm:P132_spatiotemporally_overlaps_with rdf:resource="http://academictourism.com/entity/BRF0004.RS.RS0004.RS0002"/>
	<cidoc-crm:P132_spatiotemporally_overlaps_with rdf:resource="http://academictourism.com/entity/BRF0004.RS.RS0004.RS0003"/>
	<cidoc-crm:P132_spatiotemporally_overlaps_with rdf:resource="http://academictourism.com/entity/BRF0004.RS.RS0004.RS0004"/>
	<cidoc-crm:P173_starts_before_or_with_the_end_of rdf:resource="http://academictourism.com/entity/BRF0004.RS.RS0005"/>
	<cidoc-crm:P173i_ends_after_or_with_the_start_of rdf:resource="http://academictourism.com/entity/BRF0004.RS.RS0003"/>
	<cidoc-crm:P174_starts_before_the_end_of rdf:resource="http://academictourism.com/entity/BRF0004.RS.RS0005"/>
	<cidoc-crm:P174i_ends_after_the_start_of rdf:resource="http://academictourism.com/entity/BRF0004.RS.RS0003"/>
	<cidoc-crm:P175_starts_before_or_with_the_start_of rdf:resource="http://academictourism.com/entity/BRF0004.RS.RS0005"/>
	<cidoc-crm:P175i_starts_after_or_with_the_start_of rdf:resource="http://academictourism.com/entity/BRF0004.RS.RS0003"/>
	<cidoc-crm:P176_starts_before_the_start_of rdf:resource="http://academictourism.com/entity/BRF0004.RS.RS0005"/>
	<cidoc-crm:P176i_starts_after_the_start_of rdf:resource="http://academictourism.com/entity/BRF0004.RS.RS0003"/>
	<cidoc-crm:P182_ends_before_or_with_the_start_of rdf:resource="http://academictourism.com/entity/BRF0004.RS.RS0005"/>
	<cidoc-crm:P182i_starts_after_or_with_the_end_of rdf:resource="http://academictourism.com/entity/BRF0004.RS.RS0003"/>
	<cidoc-crm:P183_ends_before_the_start_of rdf:resource="http://academictourism.com/entity/BRF0004.RS.RS0005"/>
	<cidoc-crm:P183i_starts_after_the_end_of rdf:resource="http://academictourism.com/entity/BRF0004.RS.RS0003"/>
	<cidoc-crm:P184_ends_before_or_with_the_end_of rdf:resource="http://academictourism.com/entity/BRF0004.RS.RS0005"/>
	<cidoc-crm:P184i_ends_with_or_after_the_end_of rdf:resource="http://academictourism.com/entity/BRF0004.RS.RS0003"/>
	<cidoc-crm:P185_ends_before_the_end_of rdf:resource="http://academictourism.com/entity/BRF0004.RS.RS0005"/>
	<cidoc-crm:P185i_ends_after_the_end_of rdf:resource="http://academictourism.com/entity/BRF0004.RS.RS0003"/>
	<cidoc-crm:P7_took_place_at rdf:resource="http://academictourism.com/entity/LOC0003.CS"/>
	<rdfs:comment>Wilhelmshöhe outdoor tour</rdfs:comment>
</rdf:Description>

<rdf:Description rdf:about="http://academictourism.com/entity/BRF0004.RS.RS0004.RS0001">
	<rdf:type rdf:resource="http://www.w3.org/2002/07/owl#NamedIndividual"/>
	<rdf:type rdf:resource="http://www.cidoc-crm.org/cidoc-crm/E1_CRM_Entity"/>
	<rdf:type rdf:resource="http://www.cidoc-crm.org/cidoc-crm/E2_Temporal_Entity"/>
	<rdf:type rdf:resource="http://www.cidoc-crm.org/cidoc-crm/E4_Period"/>
	<rdf:type rdf:resource="http://www.cidoc-crm.org/cidoc-crm/E5_Event"/>
	<rdf:type rdf:resource="http://www.cidoc-crm.org/cidoc-crm/E7_Activity"/>
	<rdf:type rdf:resource="http://www.cidoc-crm.org/cidoc-crm/E92_Spacetime_Volume"/>
	<rdf:type rdf:resource="http://www.loa-cnr.it/ontologies/DOLCE-Lite#perdurant"/>
	<cidoc-crm:P10_falls_within rdf:resource="http://academictourism.com/entity/BRF0004.RS.RS0004"/>
	<cidoc-crm:P11_had_participant rdf:resource="http://academictourism.com/entity/TG"/>
	<cidoc-crm:P12_occurred_in_the_presence_of rdf:resource="http://academictourism.com/entity/MISC0019"/>
	<cidoc-crm:P12_occurred_in_the_presence_of rdf:resource="http://academictourism.com/entity/TG"/>
	<cidoc-crm:P132_spatiotemporally_overlaps_with rdf:resource="http://academictourism.com/entity/BRF0004.RS.RS0004"/>
	<cidoc-crm:P173_starts_before_or_with_the_end_of rdf:resource="http://academictourism.com/entity/BRF0004.RS.RS0004.RS0002"/>
	<cidoc-crm:P174_starts_before_the_end_of rdf:resource="http://academictourism.com/entity/BRF0004.RS.RS0004.RS0002"/>
	<cidoc-crm:P175_starts_before_or_with_the_start_of rdf:resource="http://academictourism.com/entity/BRF0004.RS.RS0004.RS0002"/>
	<cidoc-crm:P176_starts_before_the_start_of rdf:resource="http://academictourism.com/entity/BRF0004.RS.RS0004.RS0002"/>
	<cidoc-crm:P182_ends_before_or_with_the_start_of rdf:resource="http://academictourism.com/entity/BRF0004.RS.RS0004.RS0002"/>
	<cidoc-crm:P183_ends_before_the_start_of rdf:resource="http://academictourism.com/entity/BRF0004.RS.RS0004.RS0002"/>
	<cidoc-crm:P184_ends_before_or_with_the_end_of rdf:resource="http://academictourism.com/entity/BRF0004.RS.RS0004.RS0002"/>
	<cidoc-crm:P185_ends_before_the_end_of rdf:resource="http://academictourism.com/entity/BRF0004.RS.RS0004.RS0002"/>
	<rdfs:comment>Na alles hier rondgezien en opgenomen te hebben begaven wy ons naar de herberg aan de voet der Octogoon</rdfs:comment>
	<rdfs:label>short stay around Octogoon</rdfs:label>
</rdf:Description>

<rdf:Description rdf:about="http://academictourism.com/entity/BRF0004.RS.RS0004.RS0002">
	<rdf:type rdf:resource="http://www.w3.org/2002/07/owl#NamedIndividual"/>
	<rdf:type rdf:resource="http://www.cidoc-crm.org/cidoc-crm/E1_CRM_Entity"/>
	<rdf:type rdf:resource="http://www.cidoc-crm.org/cidoc-crm/E2_Temporal_Entity"/>
	<rdf:type rdf:resource="http://www.cidoc-crm.org/cidoc-crm/E4_Period"/>
	<rdf:type rdf:resource="http://www.cidoc-crm.org/cidoc-crm/E5_Event"/>
	<rdf:type rdf:resource="http://www.cidoc-crm.org/cidoc-crm/E7_Activity"/>
	<rdf:type rdf:resource="http://www.cidoc-crm.org/cidoc-crm/E92_Spacetime_Volume"/>
	<rdf:type rdf:resource="http://www.cidoc-crm.org/cidoc-crm/E9_Move"/>
	<rdf:type rdf:resource="http://www.loa-cnr.it/ontologies/DOLCE-Lite#perdurant"/>
	<cidoc-crm:P10_falls_within rdf:resource="http://academictourism.com/entity/BRF0004.RS.RS0004"/>
	<cidoc-crm:P11_had_participant rdf:resource="http://academictourism.com/entity/TG"/>
	<cidoc-crm:P125_used_object_of_type rdf:resource="http://vocab.getty.edu/page/aat/300248181"/>
	<cidoc-crm:P12_occurred_in_the_presence_of rdf:resource="http://academictourism.com/entity/LOC0001"/>
	<cidoc-crm:P12_occurred_in_the_presence_of rdf:resource="http://academictourism.com/entity/MISC0007"/>
	<cidoc-crm:P12_occurred_in_the_presence_of rdf:resource="http://academictourism.com/entity/MISC0008"/>
	<cidoc-crm:P12_occurred_in_the_presence_of rdf:resource="http://academictourism.com/entity/MISC0009"/>
	<cidoc-crm:P12_occurred_in_the_presence_of rdf:resource="http://academictourism.com/entity/TG"/>
	<cidoc-crm:P132_spatiotemporally_overlaps_with rdf:resource="http://academictourism.com/entity/BRF0004.RS.RS0004"/>
	<cidoc-crm:P173_starts_before_or_with_the_end_of rdf:resource="http://academictourism.com/entity/BRF0004.RS.RS0004.RS0003"/>
	<cidoc-crm:P173i_ends_after_or_with_the_start_of rdf:resource="http://academictourism.com/entity/BRF0004.RS.RS0004.RS0001"/>
	<cidoc-crm:P174_starts_before_the_end_of rdf:resource="http://academictourism.com/entity/BRF0004.RS.RS0004.RS0003"/>
	<cidoc-crm:P174i_ends_after_the_start_of rdf:resource="http://academictourism.com/entity/BRF0004.RS.RS0004.RS0001"/>
	<cidoc-crm:P175_starts_before_or_with_the_start_of rdf:resource="http://academictourism.com/entity/BRF0004.RS.RS0004.RS0003"/>
	<cidoc-crm:P175i_starts_after_or_with_the_start_of rdf:resource="http://academictourism.com/entity/BRF0004.RS.RS0004.RS0001"/>
	<cidoc-crm:P176_starts_before_the_start_of rdf:resource="http://academictourism.com/entity/BRF0004.RS.RS0004.RS0003"/>
	<cidoc-crm:P176i_starts_after_the_start_of rdf:resource="http://academictourism.com/entity/BRF0004.RS.RS0004.RS0001"/>
	<cidoc-crm:P182_ends_before_or_with_the_start_of rdf:resource="http://academictourism.com/entity/BRF0004.RS.RS0004.RS0003"/>
	<cidoc-crm:P182i_starts_after_or_with_the_end_of rdf:resource="http://academictourism.com/entity/BRF0004.RS.RS0004.RS0001"/>
	<cidoc-crm:P183_ends_before_the_start_of rdf:resource="http://academictourism.com/entity/BRF0004.RS.RS0004.RS0003"/>
	<cidoc-crm:P183i_starts_after_the_end_of rdf:resource="http://academictourism.com/entity/BRF0004.RS.RS0004.RS0001"/>
	<cidoc-crm:P184_ends_before_or_with_the_end_of rdf:resource="http://academictourism.com/entity/BRF0004.RS.RS0004.RS0003"/>
	<cidoc-crm:P184i_ends_with_or_after_the_end_of rdf:resource="http://academictourism.com/entity/BRF0004.RS.RS0004.RS0001"/>
	<cidoc-crm:P185_ends_before_the_end_of rdf:resource="http://academictourism.com/entity/BRF0004.RS.RS0004.RS0003"/>
	<cidoc-crm:P185i_ends_after_the_end_of rdf:resource="http://academictourism.com/entity/BRF0004.RS.RS0004.RS0001"/>
	<cidoc-crm:P32_used_general_technique rdf:resource="http://vocab.getty.edu/page/aat/300248181"/>
	<cidoc-crm:P8_took_place_on_or_within rdf:resource="http://academictourism.com/entity/R.BRF0004.RS.RS0004.RS0002"/>
	<rdfs:label>Move from the bottom of Octogoon to Hercules</rdfs:label>
</rdf:Description>

<rdf:Description rdf:about="http://academictourism.com/entity/BRF0004.RS.RS0004.RS0003">
	<rdf:type rdf:resource="http://www.w3.org/2002/07/owl#NamedIndividual"/>
	<rdf:type rdf:resource="http://www.cidoc-crm.org/cidoc-crm/E1_CRM_Entity"/>
	<rdf:type rdf:resource="http://www.cidoc-crm.org/cidoc-crm/E2_Temporal_Entity"/>
	<rdf:type rdf:resource="http://www.cidoc-crm.org/cidoc-crm/E4_Period"/>
	<rdf:type rdf:resource="http://www.cidoc-crm.org/cidoc-crm/E5_Event"/>
	<rdf:type rdf:resource="http://www.cidoc-crm.org/cidoc-crm/E7_Activity"/>
	<rdf:type rdf:resource="http://www.cidoc-crm.org/cidoc-crm/E92_Spacetime_Volume"/>
	<rdf:type rdf:resource="http://www.cidoc-crm.org/cidoc-crm/E9_Move"/>
	<rdf:type rdf:resource="http://www.loa-cnr.it/ontologies/DOLCE-Lite#perdurant"/>
	<cidoc-crm:P10_falls_within rdf:resource="http://academictourism.com/entity/BRF0004.RS.RS0004"/>
	<cidoc-crm:P11_had_participant rdf:resource="http://academictourism.com/entity/TG"/>
	<cidoc-crm:P12_occurred_in_the_presence_of rdf:resource="http://academictourism.com/entity/TG"/>
	<cidoc-crm:P132_spatiotemporally_overlaps_with rdf:resource="http://academictourism.com/entity/BRF0004.RS.RS0004"/>
	<cidoc-crm:P173_starts_before_or_with_the_end_of rdf:resource="http://academictourism.com/entity/BRF0004.RS.RS0004.RS0004"/>
	<cidoc-crm:P173i_ends_after_or_with_the_start_of rdf:resource="http://academictourism.com/entity/BRF0004.RS.RS0004.RS0002"/>
	<cidoc-crm:P174_starts_before_the_end_of rdf:resource="http://academictourism.com/entity/BRF0004.RS.RS0004.RS0004"/>
	<cidoc-crm:P174i_ends_after_the_start_of rdf:resource="http://academictourism.com/entity/BRF0004.RS.RS0004.RS0002"/>
	<cidoc-crm:P175_starts_before_or_with_the_start_of rdf:resource="http://academictourism.com/entity/BRF0004.RS.RS0004.RS0004"/>
	<cidoc-crm:P175i_starts_after_or_with_the_start_of rdf:resource="http://academictourism.com/entity/BRF0004.RS.RS0004.RS0002"/>
	<cidoc-crm:P176_starts_before_the_start_of rdf:resource="http://academictourism.com/entity/BRF0004.RS.RS0004.RS0004"/>
	<cidoc-crm:P176i_starts_after_the_start_of rdf:resource="http://academictourism.com/entity/BRF0004.RS.RS0004.RS0002"/>
	<cidoc-crm:P182_ends_before_or_with_the_start_of rdf:resource="http://academictourism.com/entity/BRF0004.RS.RS0004.RS0004"/>
	<cidoc-crm:P182i_starts_after_or_with_the_end_of rdf:resource="http://academictourism.com/entity/BRF0004.RS.RS0004.RS0002"/>
	<cidoc-crm:P183_ends_before_the_start_of rdf:resource="http://academictourism.com/entity/BRF0004.RS.RS0004.RS0004"/>
	<cidoc-crm:P183i_starts_after_the_end_of rdf:resource="http://academictourism.com/entity/BRF0004.RS.RS0004.RS0002"/>
	<cidoc-crm:P184_ends_before_or_with_the_end_of rdf:resource="http://academictourism.com/entity/BRF0004.RS.RS0004.RS0004"/>
	<cidoc-crm:P184i_ends_with_or_after_the_end_of rdf:resource="http://academictourism.com/entity/BRF0004.RS.RS0004.RS0002"/>
	<cidoc-crm:P185_ends_before_the_end_of rdf:resource="http://academictourism.com/entity/BRF0004.RS.RS0004.RS0004"/>
	<cidoc-crm:P185i_ends_after_the_end_of rdf:resource="http://academictourism.com/entity/BRF0004.RS.RS0004.RS0002"/>
	<rdfs:comment>Move from Hercules to the bottom of Octogoon</rdfs:comment>
</rdf:Description>

<rdf:Description rdf:about="http://academictourism.com/entity/BRF0004.RS.RS0004.RS0004">
	<rdf:type rdf:resource="http://www.w3.org/2002/07/owl#NamedIndividual"/>
	<rdf:type rdf:resource="http://www.cidoc-crm.org/cidoc-crm/E1_CRM_Entity"/>
	<rdf:type rdf:resource="http://www.cidoc-crm.org/cidoc-crm/E2_Temporal_Entity"/>
	<rdf:type rdf:resource="http://www.cidoc-crm.org/cidoc-crm/E4_Period"/>
	<rdf:type rdf:resource="http://www.cidoc-crm.org/cidoc-crm/E5_Event"/>
	<rdf:type rdf:resource="http://www.cidoc-crm.org/cidoc-crm/E7_Activity"/>
	<rdf:type rdf:resource="http://www.cidoc-crm.org/cidoc-crm/E92_Spacetime_Volume"/>
	<rdf:type rdf:resource="http://www.loa-cnr.it/ontologies/DOLCE-Lite#perdurant"/>
	<cidoc-crm:P10_falls_within rdf:resource="http://academictourism.com/entity/BRF0004.RS.RS0004"/>
	<cidoc-crm:P11_had_participant rdf:resource="http://academictourism.com/entity/TG"/>
	<cidoc-crm:P12_occurred_in_the_presence_of rdf:resource="http://academictourism.com/entity/MISC0010"/>
	<cidoc-crm:P12_occurred_in_the_presence_of rdf:resource="http://academictourism.com/entity/MISC0011"/>
	<cidoc-crm:P12_occurred_in_the_presence_of rdf:resource="http://academictourism.com/entity/MISC0012"/>
	<cidoc-crm:P12_occurred_in_the_presence_of rdf:resource="http://academictourism.com/entity/MISC0013"/>
	<cidoc-crm:P12_occurred_in_the_presence_of rdf:resource="http://academictourism.com/entity/MISC0014"/>
	<cidoc-crm:P12_occurred_in_the_presence_of rdf:resource="http://academictourism.com/entity/MISC0015"/>
	<cidoc-crm:P12_occurred_in_the_presence_of rdf:resource="http://academictourism.com/entity/MISC0016"/>
	<cidoc-crm:P12_occurred_in_the_presence_of rdf:resource="http://academictourism.com/entity/MISC0017"/>
	<cidoc-crm:P12_occurred_in_the_presence_of rdf:resource="http://academictourism.com/entity/MISC0023"/>
	<cidoc-crm:P12_occurred_in_the_presence_of rdf:resource="http://academictourism.com/entity/TG"/>
	<cidoc-crm:P132_spatiotemporally_overlaps_with rdf:resource="http://academictourism.com/entity/BRF0004.RS.RS0004"/>
	<cidoc-crm:P173_starts_before_or_with_the_end_of rdf:resource="http://academictourism.com/entity/BRF0004.RS.RS0005"/>
	<cidoc-crm:P173i_ends_after_or_with_the_start_of rdf:resource="http://academictourism.com/entity/BRF0004.RS.RS0004.RS0003"/>
	<cidoc-crm:P174_starts_before_the_end_of rdf:resource="http://academictourism.com/entity/BRF0004.RS.RS0005"/>
	<cidoc-crm:P174i_ends_after_the_start_of rdf:resource="http://academictourism.com/entity/BRF0004.RS.RS0004.RS0003"/>
	<cidoc-crm:P175_starts_before_or_with_the_start_of rdf:resource="http://academictourism.com/entity/BRF0004.RS.RS0005"/>
	<cidoc-crm:P175i_starts_after_or_with_the_start_of rdf:resource="http://academictourism.com/entity/BRF0004.RS.RS0004.RS0003"/>
	<cidoc-crm:P176_starts_before_the_start_of rdf:resource="http://academictourism.com/entity/BRF0004.RS.RS0005"/>
	<cidoc-crm:P176i_starts_after_the_start_of rdf:resource="http://academictourism.com/entity/BRF0004.RS.RS0004.RS0003"/>
	<cidoc-crm:P182_ends_before_or_with_the_start_of rdf:resource="http://academictourism.com/entity/BRF0004.RS.RS0005"/>
	<cidoc-crm:P182i_starts_after_or_with_the_end_of rdf:resource="http://academictourism.com/entity/BRF0004.RS.RS0004.RS0003"/>
	<cidoc-crm:P183_ends_before_the_start_of rdf:resource="http://academictourism.com/entity/BRF0004.RS.RS0005"/>
	<cidoc-crm:P183i_starts_after_the_end_of rdf:resource="http://academictourism.com/entity/BRF0004.RS.RS0004.RS0003"/>
	<cidoc-crm:P184_ends_before_or_with_the_end_of rdf:resource="http://academictourism.com/entity/BRF0004.RS.RS0005"/>
	<cidoc-crm:P184i_ends_with_or_after_the_end_of rdf:resource="http://academictourism.com/entity/BRF0004.RS.RS0004.RS0003"/>
	<cidoc-crm:P185_ends_before_the_end_of rdf:resource="http://academictourism.com/entity/BRF0004.RS.RS0005"/>
	<cidoc-crm:P185i_ends_after_the_end_of rdf:resource="http://academictourism.com/entity/BRF0004.RS.RS0004.RS0003"/>
	<rdfs:comment>Various activities in the Bergpark Wilhelmshöhe</rdfs:comment>
</rdf:Description>

<rdf:Description rdf:about="http://academictourism.com/entity/BRF0004.RS.RS0005">
	<rdf:type rdf:resource="http://www.w3.org/2002/07/owl#NamedIndividual"/>
	<rdf:type rdf:resource="http://www.cidoc-crm.org/cidoc-crm/E1_CRM_Entity"/>
	<rdf:type rdf:resource="http://www.cidoc-crm.org/cidoc-crm/E2_Temporal_Entity"/>
	<rdf:type rdf:resource="http://www.cidoc-crm.org/cidoc-crm/E4_Period"/>
	<rdf:type rdf:resource="http://www.cidoc-crm.org/cidoc-crm/E5_Event"/>
	<rdf:type rdf:resource="http://www.cidoc-crm.org/cidoc-crm/E7_Activity"/>
	<rdf:type rdf:resource="http://www.cidoc-crm.org/cidoc-crm/E92_Spacetime_Volume"/>
	<rdf:type rdf:resource="http://www.cidoc-crm.org/cidoc-crm/E9_Move"/>
	<rdf:type rdf:resource="http://www.loa-cnr.it/ontologies/DOLCE-Lite#perdurant"/>
	<cidoc-crm:P10_falls_within rdf:resource="http://academictourism.com/entity/BRF0004.RS"/>
	<cidoc-crm:P10i_contains rdf:resource="http://academictourism.com/entity/BRF0004.RS.RS0005.RS0001"/>
	<cidoc-crm:P11_had_participant rdf:resource="http://academictourism.com/entity/TG"/>
	<cidoc-crm:P12_occurred_in_the_presence_of rdf:resource="http://academictourism.com/entity/TG"/>
	<cidoc-crm:P132_spatiotemporally_overlaps_with rdf:resource="http://academictourism.com/entity/BRF0004.RS"/>
	<cidoc-crm:P132_spatiotemporally_overlaps_with rdf:resource="http://academictourism.com/entity/BRF0004.RS.RS0005.RS0001"/>
	<cidoc-crm:P173_starts_before_or_with_the_end_of rdf:resource="http://academictourism.com/entity/BRF0004.RS.RS0006"/>
	<cidoc-crm:P173i_ends_after_or_with_the_start_of rdf:resource="http://academictourism.com/entity/BRF0004.RS.RS0004"/>
	<cidoc-crm:P173i_ends_after_or_with_the_start_of rdf:resource="http://academictourism.com/entity/BRF0004.RS.RS0004.RS0004"/>
	<cidoc-crm:P174_starts_before_the_end_of rdf:resource="http://academictourism.com/entity/BRF0004.RS.RS0006"/>
	<cidoc-crm:P174i_ends_after_the_start_of rdf:resource="http://academictourism.com/entity/BRF0004.RS.RS0004"/>
	<cidoc-crm:P174i_ends_after_the_start_of rdf:resource="http://academictourism.com/entity/BRF0004.RS.RS0004.RS0004"/>
	<cidoc-crm:P175_starts_before_or_with_the_start_of rdf:resource="http://academictourism.com/entity/BRF0004.RS.RS0006"/>
	<cidoc-crm:P175i_starts_after_or_with_the_start_of rdf:resource="http://academictourism.com/entity/BRF0004.RS.RS0004"/>
	<cidoc-crm:P175i_starts_after_or_with_the_start_of rdf:resource="http://academictourism.com/entity/BRF0004.RS.RS0004.RS0004"/>
	<cidoc-crm:P176_starts_before_the_start_of rdf:resource="http://academictourism.com/entity/BRF0004.RS.RS0006"/>
	<cidoc-crm:P176i_starts_after_the_start_of rdf:resource="http://academictourism.com/entity/BRF0004.RS.RS0004"/>
	<cidoc-crm:P176i_starts_after_the_start_of rdf:resource="http://academictourism.com/entity/BRF0004.RS.RS0004.RS0004"/>
	<cidoc-crm:P182_ends_before_or_with_the_start_of rdf:resource="http://academictourism.com/entity/BRF0004.RS.RS0006"/>
	<cidoc-crm:P182i_starts_after_or_with_the_end_of rdf:resource="http://academictourism.com/entity/BRF0004.RS.RS0004"/>
	<cidoc-crm:P182i_starts_after_or_with_the_end_of rdf:resource="http://academictourism.com/entity/BRF0004.RS.RS0004.RS0004"/>
	<cidoc-crm:P183_ends_before_the_start_of rdf:resource="http://academictourism.com/entity/BRF0004.RS.RS0006"/>
	<cidoc-crm:P183i_starts_after_the_end_of rdf:resource="http://academictourism.com/entity/BRF0004.RS.RS0004"/>
	<cidoc-crm:P183i_starts_after_the_end_of rdf:resource="http://academictourism.com/entity/BRF0004.RS.RS0004.RS0004"/>
	<cidoc-crm:P184_ends_before_or_with_the_end_of rdf:resource="http://academictourism.com/entity/BRF0004.RS.RS0006"/>
	<cidoc-crm:P184i_ends_with_or_after_the_end_of rdf:resource="http://academictourism.com/entity/BRF0004.RS.RS0004"/>
	<cidoc-crm:P184i_ends_with_or_after_the_end_of rdf:resource="http://academictourism.com/entity/BRF0004.RS.RS0004.RS0004"/>
	<cidoc-crm:P185_ends_before_the_end_of rdf:resource="http://academictourism.com/entity/BRF0004.RS.RS0006"/>
	<cidoc-crm:P185i_ends_after_the_end_of rdf:resource="http://academictourism.com/entity/BRF0004.RS.RS0004"/>
	<cidoc-crm:P185i_ends_after_the_end_of rdf:resource="http://academictourism.com/entity/BRF0004.RS.RS0004.RS0004"/>
	<cidoc-crm:P26_moved_to rdf:resource="http://academictourism.com/entity/LOC0001"/>
	<cidoc-crm:P27_moved_from rdf:resource="http://academictourism.com/entity/LOC0003.CS"/>
	<rdfs:label>Move from Wilhelmshöhe to Kassel</rdfs:label>
</rdf:Description>

<rdf:Description rdf:about="http://academictourism.com/entity/BRF0004.RS.RS0005.RS0001">
	<rdf:type rdf:resource="http://www.w3.org/2002/07/owl#NamedIndividual"/>
	<rdf:type rdf:resource="http://www.cidoc-crm.org/cidoc-crm/E1_CRM_Entity"/>
	<rdf:type rdf:resource="http://www.cidoc-crm.org/cidoc-crm/E2_Temporal_Entity"/>
	<rdf:type rdf:resource="http://www.cidoc-crm.org/cidoc-crm/E4_Period"/>
	<rdf:type rdf:resource="http://www.cidoc-crm.org/cidoc-crm/E5_Event"/>
	<rdf:type rdf:resource="http://www.cidoc-crm.org/cidoc-crm/E7_Activity"/>
	<rdf:type rdf:resource="http://www.cidoc-crm.org/cidoc-crm/E92_Spacetime_Volume"/>
	<rdf:type rdf:resource="http://www.loa-cnr.it/ontologies/DOLCE-Lite#perdurant"/>
	<cidoc-crm:P10_falls_within rdf:resource="http://academictourism.com/entity/BRF0004.RS.RS0005"/>
	<cidoc-crm:P11_had_participant rdf:resource="http://academictourism.com/entity/TG"/>
	<cidoc-crm:P12_occurred_in_the_presence_of rdf:resource="http://academictourism.com/entity/TG"/>
	<cidoc-crm:P132_spatiotemporally_overlaps_with rdf:resource="http://academictourism.com/entity/BRF0004.RS.RS0005"/>
	<cidoc-crm:P4_has_time-span rdf:resource="http://academictourism.com/entity/TS.BRF0004.RS.RS0005.RS0001"/>
	<cidoc-crm:P7_took_place_at rdf:resource="http://academictourism.com/entity/LOC0001"/>
	<rdfs:label>arrival in Kassel</rdfs:label>
</rdf:Description>

<rdf:Description rdf:about="http://academictourism.com/entity/BRF0004.RS.RS0006">
	<rdf:type rdf:resource="http://www.w3.org/2002/07/owl#NamedIndividual"/>
	<rdf:type rdf:resource="http://www.cidoc-crm.org/cidoc-crm/E1_CRM_Entity"/>
	<rdf:type rdf:resource="http://www.cidoc-crm.org/cidoc-crm/E2_Temporal_Entity"/>
	<rdf:type rdf:resource="http://www.cidoc-crm.org/cidoc-crm/E4_Period"/>
	<rdf:type rdf:resource="http://www.cidoc-crm.org/cidoc-crm/E5_Event"/>
	<rdf:type rdf:resource="http://www.cidoc-crm.org/cidoc-crm/E7_Activity"/>
	<rdf:type rdf:resource="http://www.cidoc-crm.org/cidoc-crm/E92_Spacetime_Volume"/>
	<rdf:type rdf:resource="http://www.cidoc-crm.org/cidoc-crm/E9_Move"/>
	<rdf:type rdf:resource="http://www.loa-cnr.it/ontologies/DOLCE-Lite#perdurant"/>
	<cidoc-crm:P10_falls_within rdf:resource="http://academictourism.com/entity/BRF0004.RS"/>
	<cidoc-crm:P10i_contains rdf:resource="http://academictourism.com/entity/BRF0004.RS.RS0006.RS0001"/>
	<cidoc-crm:P10i_contains rdf:resource="http://academictourism.com/entity/BRF0004.RS.RS0006.RS0002"/>
	<cidoc-crm:P10i_contains rdf:resource="http://academictourism.com/entity/BRF0004.RS.RS0006.RS0003"/>
	<cidoc-crm:P10i_contains rdf:resource="http://academictourism.com/entity/BRF0004.RS.RS0006.RS0004"/>
	<cidoc-crm:P10i_contains rdf:resource="http://academictourism.com/entity/BRF0004.RS.RS0006.RS0005"/>
	<cidoc-crm:P11_had_participant rdf:resource="http://academictourism.com/entity/TG"/>
	<cidoc-crm:P12_occurred_in_the_presence_of rdf:resource="http://academictourism.com/entity/TG"/>
	<cidoc-crm:P132_spatiotemporally_overlaps_with rdf:resource="http://academictourism.com/entity/BRF0004.RS"/>
	<cidoc-crm:P132_spatiotemporally_overlaps_with rdf:resource="http://academictourism.com/entity/BRF0004.RS.RS0006.RS0001"/>
	<cidoc-crm:P132_spatiotemporally_overlaps_with rdf:resource="http://academictourism.com/entity/BRF0004.RS.RS0006.RS0002"/>
	<cidoc-crm:P132_spatiotemporally_overlaps_with rdf:resource="http://academictourism.com/entity/BRF0004.RS.RS0006.RS0003"/>
	<cidoc-crm:P132_spatiotemporally_overlaps_with rdf:resource="http://academictourism.com/entity/BRF0004.RS.RS0006.RS0004"/>
	<cidoc-crm:P132_spatiotemporally_overlaps_with rdf:resource="http://academictourism.com/entity/BRF0004.RS.RS0006.RS0005"/>
	<cidoc-crm:P173i_ends_after_or_with_the_start_of rdf:resource="http://academictourism.com/entity/BRF0004.RS.RS0005"/>
	<cidoc-crm:P174i_ends_after_the_start_of rdf:resource="http://academictourism.com/entity/BRF0004.RS.RS0005"/>
	<cidoc-crm:P175i_starts_after_or_with_the_start_of rdf:resource="http://academictourism.com/entity/BRF0004.RS.RS0005"/>
	<cidoc-crm:P176i_starts_after_the_start_of rdf:resource="http://academictourism.com/entity/BRF0004.RS.RS0005"/>
	<cidoc-crm:P182i_starts_after_or_with_the_end_of rdf:resource="http://academictourism.com/entity/BRF0004.RS.RS0005"/>
	<cidoc-crm:P183i_starts_after_the_end_of rdf:resource="http://academictourism.com/entity/BRF0004.RS.RS0005"/>
	<cidoc-crm:P184i_ends_with_or_after_the_end_of rdf:resource="http://academictourism.com/entity/BRF0004.RS.RS0005"/>
	<cidoc-crm:P185i_ends_after_the_end_of rdf:resource="http://academictourism.com/entity/BRF0004.RS.RS0005"/>
	<cidoc-crm:P26_moved_to rdf:resource="http://academictourism.com/entity/LOC0002"/>
	<cidoc-crm:P27_moved_from rdf:resource="http://academictourism.com/entity/LOC0001"/>
	<cidoc-crm:P2_has_type rdf:resource="https://www.wikidata.org/wiki/Q235356"/>
	<cidoc-crm:P4_has_time-span rdf:resource="http://academictourism.com/entity/TS.BRF0004.RS.RS0006"/>
	<rdfs:label>Move from Kassel to Göttingen</rdfs:label>
</rdf:Description>

<rdf:Description rdf:about="http://academictourism.com/entity/BRF0004.RS.RS0006.RS0001">
	<rdf:type rdf:resource="http://www.w3.org/2002/07/owl#NamedIndividual"/>
	<rdf:type rdf:resource="http://www.cidoc-crm.org/cidoc-crm/E1_CRM_Entity"/>
	<rdf:type rdf:resource="http://www.cidoc-crm.org/cidoc-crm/E2_Temporal_Entity"/>
	<rdf:type rdf:resource="http://www.cidoc-crm.org/cidoc-crm/E4_Period"/>
	<rdf:type rdf:resource="http://www.cidoc-crm.org/cidoc-crm/E5_Event"/>
	<rdf:type rdf:resource="http://www.cidoc-crm.org/cidoc-crm/E7_Activity"/>
	<rdf:type rdf:resource="http://www.cidoc-crm.org/cidoc-crm/E92_Spacetime_Volume"/>
	<rdf:type rdf:resource="http://www.loa-cnr.it/ontologies/DOLCE-Lite#perdurant"/>
	<cidoc-crm:P10_falls_within rdf:resource="http://academictourism.com/entity/BRF0004.RS.RS0006"/>
	<cidoc-crm:P11_had_participant rdf:resource="http://academictourism.com/entity/TG"/>
	<cidoc-crm:P12_occurred_in_the_presence_of rdf:resource="http://academictourism.com/entity/TG"/>
	<cidoc-crm:P132_spatiotemporally_overlaps_with rdf:resource="http://academictourism.com/entity/BRF0004.RS.RS0006"/>
	<cidoc-crm:P173_starts_before_or_with_the_end_of rdf:resource="http://academictourism.com/entity/BRF0004.RS.RS0006.RS0002"/>
	<cidoc-crm:P173i_ends_after_or_with_the_start_of rdf:resource="http://academictourism.com/entity/L0001"/>
	<cidoc-crm:P174_starts_before_the_end_of rdf:resource="http://academictourism.com/entity/BRF0004.RS.RS0006.RS0002"/>
	<cidoc-crm:P174i_ends_after_the_start_of rdf:resource="http://academictourism.com/entity/L0001"/>
	<cidoc-crm:P175_starts_before_or_with_the_start_of rdf:resource="http://academictourism.com/entity/BRF0004.RS.RS0006.RS0002"/>
	<cidoc-crm:P175i_starts_after_or_with_the_start_of rdf:resource="http://academictourism.com/entity/L0001"/>
	<cidoc-crm:P176_starts_before_the_start_of rdf:resource="http://academictourism.com/entity/BRF0004.RS.RS0006.RS0002"/>
	<cidoc-crm:P176i_starts_after_the_start_of rdf:resource="http://academictourism.com/entity/L0001"/>
	<cidoc-crm:P182_ends_before_or_with_the_start_of rdf:resource="http://academictourism.com/entity/BRF0004.RS.RS0006.RS0002"/>
	<cidoc-crm:P182i_starts_after_or_with_the_end_of rdf:resource="http://academictourism.com/entity/L0001"/>
	<cidoc-crm:P183_ends_before_the_start_of rdf:resource="http://academictourism.com/entity/BRF0004.RS.RS0006.RS0002"/>
	<cidoc-crm:P183i_starts_after_the_end_of rdf:resource="http://academictourism.com/entity/L0001"/>
	<cidoc-crm:P184_ends_before_or_with_the_end_of rdf:resource="http://academictourism.com/entity/BRF0004.RS.RS0006.RS0002"/>
	<cidoc-crm:P184i_ends_with_or_after_the_end_of rdf:resource="http://academictourism.com/entity/L0001"/>
	<cidoc-crm:P185_ends_before_the_end_of rdf:resource="http://academictourism.com/entity/BRF0004.RS.RS0006.RS0002"/>
	<cidoc-crm:P185i_ends_after_the_end_of rdf:resource="http://academictourism.com/entity/L0001"/>
	<cidoc-crm:P4_has_time-span rdf:resource="http://academictourism.com/TS.BRF0004.RS.RS0006.RS0001"/>
	<cidoc-crm:P7_took_place_at rdf:resource="http://academictourism.com/entity/LOC0001"/>
	<rdfs:label>departure from Kassel</rdfs:label>
</rdf:Description>

<rdf:Description rdf:about="http://academictourism.com/entity/BRF0004.RS.RS0006.RS0002">
	<rdf:type rdf:resource="http://www.w3.org/2002/07/owl#NamedIndividual"/>
	<rdf:type rdf:resource="http://www.cidoc-crm.org/cidoc-crm/E1_CRM_Entity"/>
	<rdf:type rdf:resource="http://www.cidoc-crm.org/cidoc-crm/E2_Temporal_Entity"/>
	<rdf:type rdf:resource="http://www.cidoc-crm.org/cidoc-crm/E4_Period"/>
	<rdf:type rdf:resource="http://www.cidoc-crm.org/cidoc-crm/E5_Event"/>
	<rdf:type rdf:resource="http://www.cidoc-crm.org/cidoc-crm/E7_Activity"/>
	<rdf:type rdf:resource="http://www.cidoc-crm.org/cidoc-crm/E92_Spacetime_Volume"/>
	<rdf:type rdf:resource="http://www.loa-cnr.it/ontologies/DOLCE-Lite#perdurant"/>
	<cidoc-crm:P10_falls_within rdf:resource="http://academictourism.com/entity/BRF0004.RS.RS0006"/>
	<cidoc-crm:P11_had_participant rdf:resource="http://academictourism.com/entity/TG"/>
	<cidoc-crm:P12_occurred_in_the_presence_of rdf:resource="http://academictourism.com/entity/TG"/>
	<cidoc-crm:P132_spatiotemporally_overlaps_with rdf:resource="http://academictourism.com/entity/BRF0004.RS.RS0006"/>
	<cidoc-crm:P173_starts_before_or_with_the_end_of rdf:resource="http://academictourism.com/entity/BRF0004.RS.RS0006.RS0003"/>
	<cidoc-crm:P173i_ends_after_or_with_the_start_of rdf:resource="http://academictourism.com/entity/BRF0004.RS.RS0006.RS0001"/>
	<cidoc-crm:P174_starts_before_the_end_of rdf:resource="http://academictourism.com/entity/BRF0004.RS.RS0006.RS0003"/>
	<cidoc-crm:P174i_ends_after_the_start_of rdf:resource="http://academictourism.com/entity/BRF0004.RS.RS0006.RS0001"/>
	<cidoc-crm:P175_starts_before_or_with_the_start_of rdf:resource="http://academictourism.com/entity/BRF0004.RS.RS0006.RS0003"/>
	<cidoc-crm:P175i_starts_after_or_with_the_start_of rdf:resource="http://academictourism.com/entity/BRF0004.RS.RS0006.RS0001"/>
	<cidoc-crm:P176_starts_before_the_start_of rdf:resource="http://academictourism.com/entity/BRF0004.RS.RS0006.RS0003"/>
	<cidoc-crm:P176i_starts_after_the_start_of rdf:resource="http://academictourism.com/entity/BRF0004.RS.RS0006.RS0001"/>
	<cidoc-crm:P182_ends_before_or_with_the_start_of rdf:resource="http://academictourism.com/entity/BRF0004.RS.RS0006.RS0003"/>
	<cidoc-crm:P182i_starts_after_or_with_the_end_of rdf:resource="http://academictourism.com/entity/BRF0004.RS.RS0006.RS0001"/>
	<cidoc-crm:P183_ends_before_the_start_of rdf:resource="http://academictourism.com/entity/BRF0004.RS.RS0006.RS0003"/>
	<cidoc-crm:P183i_starts_after_the_end_of rdf:resource="http://academictourism.com/entity/BRF0004.RS.RS0006.RS0001"/>
	<cidoc-crm:P184_ends_before_or_with_the_end_of rdf:resource="http://academictourism.com/entity/BRF0004.RS.RS0006.RS0003"/>
	<cidoc-crm:P184i_ends_with_or_after_the_end_of rdf:resource="http://academictourism.com/entity/BRF0004.RS.RS0006.RS0001"/>
	<cidoc-crm:P185_ends_before_the_end_of rdf:resource="http://academictourism.com/entity/BRF0004.RS.RS0006.RS0003"/>
	<cidoc-crm:P185i_ends_after_the_end_of rdf:resource="http://academictourism.com/entity/BRF0004.RS.RS0006.RS0001"/>
	<cidoc-crm:P7_took_place_at rdf:resource="http://academictourism.com/entity/LOC0005"/>
	<rdfs:label>short_stay_Munden</rdfs:label>
</rdf:Description>

<rdf:Description rdf:about="http://academictourism.com/entity/BRF0004.RS.RS0006.RS0003">
	<rdf:type rdf:resource="http://www.w3.org/2002/07/owl#NamedIndividual"/>
	<rdf:type rdf:resource="http://www.cidoc-crm.org/cidoc-crm/E1_CRM_Entity"/>
	<rdf:type rdf:resource="http://www.cidoc-crm.org/cidoc-crm/E2_Temporal_Entity"/>
	<rdf:type rdf:resource="http://www.cidoc-crm.org/cidoc-crm/E4_Period"/>
	<rdf:type rdf:resource="http://www.cidoc-crm.org/cidoc-crm/E5_Event"/>
	<rdf:type rdf:resource="http://www.cidoc-crm.org/cidoc-crm/E7_Activity"/>
	<rdf:type rdf:resource="http://www.cidoc-crm.org/cidoc-crm/E92_Spacetime_Volume"/>
	<rdf:type rdf:resource="http://www.loa-cnr.it/ontologies/DOLCE-Lite#perdurant"/>
	<cidoc-crm:P10_falls_within rdf:resource="http://academictourism.com/entity/BRF0004.RS.RS0006"/>
	<cidoc-crm:P11_had_participant rdf:resource="http://academictourism.com/entity/TG"/>
	<cidoc-crm:P12_occurred_in_the_presence_of rdf:resource="http://academictourism.com/entity/TG"/>
	<cidoc-crm:P132_spatiotemporally_overlaps_with rdf:resource="http://academictourism.com/entity/BRF0004.RS.RS0006"/>
	<cidoc-crm:P173_starts_before_or_with_the_end_of rdf:resource="http://academictourism.com/entity/BRF0004.RS.RS0006.RS0004"/>
	<cidoc-crm:P173i_ends_after_or_with_the_start_of rdf:resource="http://academictourism.com/entity/BRF0004.RS.RS0006.RS0002"/>
	<cidoc-crm:P174_starts_before_the_end_of rdf:resource="http://academictourism.com/entity/BRF0004.RS.RS0006.RS0004"/>
	<cidoc-crm:P174i_ends_after_the_start_of rdf:resource="http://academictourism.com/entity/BRF0004.RS.RS0006.RS0002"/>
	<cidoc-crm:P175_starts_before_or_with_the_start_of rdf:resource="http://academictourism.com/entity/BRF0004.RS.RS0006.RS0004"/>
	<cidoc-crm:P175i_starts_after_or_with_the_start_of rdf:resource="http://academictourism.com/entity/BRF0004.RS.RS0006.RS0002"/>
	<cidoc-crm:P176_starts_before_the_start_of rdf:resource="http://academictourism.com/entity/BRF0004.RS.RS0006.RS0004"/>
	<cidoc-crm:P176i_starts_after_the_start_of rdf:resource="http://academictourism.com/entity/BRF0004.RS.RS0006.RS0002"/>
	<cidoc-crm:P182_ends_before_or_with_the_start_of rdf:resource="http://academictourism.com/entity/BRF0004.RS.RS0006.RS0004"/>
	<cidoc-crm:P182i_starts_after_or_with_the_end_of rdf:resource="http://academictourism.com/entity/BRF0004.RS.RS0006.RS0002"/>
	<cidoc-crm:P183_ends_before_the_start_of rdf:resource="http://academictourism.com/entity/BRF0004.RS.RS0006.RS0004"/>
	<cidoc-crm:P183i_starts_after_the_end_of rdf:resource="http://academictourism.com/entity/BRF0004.RS.RS0006.RS0002"/>
	<cidoc-crm:P184_ends_before_or_with_the_end_of rdf:resource="http://academictourism.com/entity/BRF0004.RS.RS0006.RS0004"/>
	<cidoc-crm:P184i_ends_with_or_after_the_end_of rdf:resource="http://academictourism.com/entity/BRF0004.RS.RS0006.RS0002"/>
	<cidoc-crm:P185_ends_before_the_end_of rdf:resource="http://academictourism.com/entity/BRF0004.RS.RS0006.RS0004"/>
	<cidoc-crm:P185i_ends_after_the_end_of rdf:resource="http://academictourism.com/entity/BRF0004.RS.RS0006.RS0002"/>
	<cidoc-crm:P7_took_place_at rdf:resource="http://academictourism.com/entity/LOC0006"/>
	<rdfs:label>short_stay_Dransfeld</rdfs:label>
</rdf:Description>

<rdf:Description rdf:about="http://academictourism.com/entity/BRF0004.RS.RS0006.RS0004">
	<rdf:type rdf:resource="http://www.w3.org/2002/07/owl#NamedIndividual"/>
	<rdf:type rdf:resource="http://www.cidoc-crm.org/cidoc-crm/E1_CRM_Entity"/>
	<rdf:type rdf:resource="http://www.cidoc-crm.org/cidoc-crm/E2_Temporal_Entity"/>
	<rdf:type rdf:resource="http://www.cidoc-crm.org/cidoc-crm/E4_Period"/>
	<rdf:type rdf:resource="http://www.cidoc-crm.org/cidoc-crm/E5_Event"/>
	<rdf:type rdf:resource="http://www.cidoc-crm.org/cidoc-crm/E7_Activity"/>
	<rdf:type rdf:resource="http://www.cidoc-crm.org/cidoc-crm/E92_Spacetime_Volume"/>
	<rdf:type rdf:resource="http://www.loa-cnr.it/ontologies/DOLCE-Lite#perdurant"/>
	<cidoc-crm:P10_falls_within rdf:resource="http://academictourism.com/entity/BRF0004.RS.RS0006"/>
	<cidoc-crm:P11_had_participant rdf:resource="http://academictourism.com/entity/TG"/>
	<cidoc-crm:P12_occurred_in_the_presence_of rdf:resource="http://academictourism.com/entity/TG"/>
	<cidoc-crm:P132_spatiotemporally_overlaps_with rdf:resource="http://academictourism.com/entity/BRF0004.RS.RS0006"/>
	<cidoc-crm:P173_starts_before_or_with_the_end_of rdf:resource="http://academictourism.com/entity/BRF0004.RS.RS0006.RS0005"/>
	<cidoc-crm:P173i_ends_after_or_with_the_start_of rdf:resource="http://academictourism.com/entity/BRF0004.RS.RS0006.RS0003"/>
	<cidoc-crm:P174_starts_before_the_end_of rdf:resource="http://academictourism.com/entity/BRF0004.RS.RS0006.RS0005"/>
	<cidoc-crm:P174i_ends_after_the_start_of rdf:resource="http://academictourism.com/entity/BRF0004.RS.RS0006.RS0003"/>
	<cidoc-crm:P175_starts_before_or_with_the_start_of rdf:resource="http://academictourism.com/entity/BRF0004.RS.RS0006.RS0005"/>
	<cidoc-crm:P175i_starts_after_or_with_the_start_of rdf:resource="http://academictourism.com/entity/BRF0004.RS.RS0006.RS0003"/>
	<cidoc-crm:P176_starts_before_the_start_of rdf:resource="http://academictourism.com/entity/BRF0004.RS.RS0006.RS0005"/>
	<cidoc-crm:P176i_starts_after_the_start_of rdf:resource="http://academictourism.com/entity/BRF0004.RS.RS0006.RS0003"/>
	<cidoc-crm:P182_ends_before_or_with_the_start_of rdf:resource="http://academictourism.com/entity/BRF0004.RS.RS0006.RS0005"/>
	<cidoc-crm:P182i_starts_after_or_with_the_end_of rdf:resource="http://academictourism.com/entity/BRF0004.RS.RS0006.RS0003"/>
	<cidoc-crm:P183_ends_before_the_start_of rdf:resource="http://academictourism.com/entity/BRF0004.RS.RS0006.RS0005"/>
	<cidoc-crm:P183i_starts_after_the_end_of rdf:resource="http://academictourism.com/entity/BRF0004.RS.RS0006.RS0003"/>
	<cidoc-crm:P184_ends_before_or_with_the_end_of rdf:resource="http://academictourism.com/entity/BRF0004.RS.RS0006.RS0005"/>
	<cidoc-crm:P184i_ends_with_or_after_the_end_of rdf:resource="http://academictourism.com/entity/BRF0004.RS.RS0006.RS0003"/>
	<cidoc-crm:P185_ends_before_the_end_of rdf:resource="http://academictourism.com/entity/BRF0004.RS.RS0006.RS0005"/>
	<cidoc-crm:P185i_ends_after_the_end_of rdf:resource="http://academictourism.com/entity/BRF0004.RS.RS0006.RS0003"/>
	<cidoc-crm:P7_took_place_at rdf:resource="http://academictourism.com/entity/LOC0008"/>
	<rdfs:label>Stay_Knalhutte</rdfs:label>
</rdf:Description>

<rdf:Description rdf:about="http://academictourism.com/entity/BRF0004.RS.RS0006.RS0005">
	<rdf:type rdf:resource="http://www.w3.org/2002/07/owl#NamedIndividual"/>
	<rdf:type rdf:resource="http://www.cidoc-crm.org/cidoc-crm/E1_CRM_Entity"/>
	<rdf:type rdf:resource="http://www.cidoc-crm.org/cidoc-crm/E2_Temporal_Entity"/>
	<rdf:type rdf:resource="http://www.cidoc-crm.org/cidoc-crm/E4_Period"/>
	<rdf:type rdf:resource="http://www.cidoc-crm.org/cidoc-crm/E5_Event"/>
	<rdf:type rdf:resource="http://www.cidoc-crm.org/cidoc-crm/E7_Activity"/>
	<rdf:type rdf:resource="http://www.cidoc-crm.org/cidoc-crm/E92_Spacetime_Volume"/>
	<rdf:type rdf:resource="http://www.loa-cnr.it/ontologies/DOLCE-Lite#perdurant"/>
	<cidoc-crm:P10_falls_within rdf:resource="http://academictourism.com/entity/BRF0004.RS.RS0006"/>
	<cidoc-crm:P11_had_participant rdf:resource="http://academictourism.com/entity/TG"/>
	<cidoc-crm:P12_occurred_in_the_presence_of rdf:resource="http://academictourism.com/entity/TG"/>
	<cidoc-crm:P132_spatiotemporally_overlaps_with rdf:resource="http://academictourism.com/entity/BRF0004.RS.RS0006"/>
	<cidoc-crm:P173i_ends_after_or_with_the_start_of rdf:resource="http://academictourism.com/entity/BRF0004.RS.RS0006.RS0004"/>
	<cidoc-crm:P174i_ends_after_the_start_of rdf:resource="http://academictourism.com/entity/BRF0004.RS.RS0006.RS0004"/>
	<cidoc-crm:P175i_starts_after_or_with_the_start_of rdf:resource="http://academictourism.com/entity/BRF0004.RS.RS0006.RS0004"/>
	<cidoc-crm:P176i_starts_after_the_start_of rdf:resource="http://academictourism.com/entity/BRF0004.RS.RS0006.RS0004"/>
	<cidoc-crm:P182i_starts_after_or_with_the_end_of rdf:resource="http://academictourism.com/entity/BRF0004.RS.RS0006.RS0004"/>
	<cidoc-crm:P183i_starts_after_the_end_of rdf:resource="http://academictourism.com/entity/BRF0004.RS.RS0006.RS0004"/>
	<cidoc-crm:P184i_ends_with_or_after_the_end_of rdf:resource="http://academictourism.com/entity/BRF0004.RS.RS0006.RS0004"/>
	<cidoc-crm:P185i_ends_after_the_end_of rdf:resource="http://academictourism.com/entity/BRF0004.RS.RS0006.RS0004"/>
	<cidoc-crm:P4_has_time-span rdf:resource="http://academictourism.com/entity/TS.BRF0004.RS.RS0006.RS0005"/>
	<cidoc-crm:P7_took_place_at rdf:resource="http://academictourism.com/entity/LOC0002"/>
	<rdfs:label>Arrival in Gottingen</rdfs:label>
</rdf:Description>

<rdf:Description rdf:about="http://academictourism.com/entity/BRF0004.SCH">
	<rdf:type rdf:resource="http://www.w3.org/2002/07/owl#NamedIndividual"/>
	<rdf:type rdf:resource="http://iflastandards.info/ns/lrm/lrmoo/F28_Expression_Creation"/>
	<rdf:type rdf:resource="http://www.cidoc-crm.org/cidoc-crm/E11_Modification"/>
	<rdf:type rdf:resource="http://www.cidoc-crm.org/cidoc-crm/E12_Production"/>
	<rdf:type rdf:resource="http://www.cidoc-crm.org/cidoc-crm/E1_CRM_Entity"/>
	<rdf:type rdf:resource="http://www.cidoc-crm.org/cidoc-crm/E2_Temporal_Entity"/>
	<rdf:type rdf:resource="http://www.cidoc-crm.org/cidoc-crm/E4_Period"/>
	<rdf:type rdf:resource="http://www.cidoc-crm.org/cidoc-crm/E5_Event"/>
	<rdf:type rdf:resource="http://www.cidoc-crm.org/cidoc-crm/E63_Beginning_of_Existence"/>
	<rdf:type rdf:resource="http://www.cidoc-crm.org/cidoc-crm/E65_Creation"/>
	<rdf:type rdf:resource="http://www.cidoc-crm.org/cidoc-crm/E7_Activity"/>
	<rdf:type rdf:resource="http://www.cidoc-crm.org/cidoc-crm/E92_Spacetime_Volume"/>
	<rdf:type rdf:resource="http://www.loa-cnr.it/ontologies/DOLCE-Lite#perdurant"/>
	<lrmoo:R17_created rdf:resource="http://academictourism.com/entity/BRF0004"/>
	<cidoc-crm:P11_had_participant rdf:resource="http://academictourism.com/entity/PER0001"/>
	<cidoc-crm:P12_occurred_in_the_presence_of rdf:resource="http://academictourism.com/entity/BRF0004"/>
	<cidoc-crm:P12_occurred_in_the_presence_of rdf:resource="http://academictourism.com/entity/PER0001"/>
	<cidoc-crm:P14_carried_out_by rdf:resource="http://academictourism.com/entity/PER0001"/>
	<cidoc-crm:P92_brought_into_existence rdf:resource="http://academictourism.com/entity/BRF0004"/>
	<cidoc-crm:P94_has_created rdf:resource="http://academictourism.com/entity/BRF0004"/>
	<rdfs:label>Writing letter 4</rdfs:label>
</rdf:Description>

<rdf:Description rdf:about="http://academictourism.com/entity/BRF0005">
	<rdf:type rdf:resource="http://www.w3.org/2002/07/owl#NamedIndividual"/>
	<rdf:type rdf:resource="http://iflastandards.info/ns/lrm/lrmoo/F2_Expression"/>
	<rdf:type rdf:resource="http://www.cidoc-crm.org/cidoc-crm/E1_CRM_Entity"/>
	<rdf:type rdf:resource="http://www.cidoc-crm.org/cidoc-crm/E28_Conceptual_Object"/>
	<rdf:type rdf:resource="http://www.cidoc-crm.org/cidoc-crm/E70_Thing"/>
	<rdf:type rdf:resource="http://www.cidoc-crm.org/cidoc-crm/E71_Human-Made_Thing"/>
	<rdf:type rdf:resource="http://www.cidoc-crm.org/cidoc-crm/E72_Legal_Object"/>
	<rdf:type rdf:resource="http://www.cidoc-crm.org/cidoc-crm/E73_Information_Object"/>
	<rdf:type rdf:resource="http://www.cidoc-crm.org/cidoc-crm/E77_Persistent_Item"/>
	<rdf:type rdf:resource="http://www.cidoc-crm.org/cidoc-crm/E89_Propositional_Object"/>
	<rdf:type rdf:resource="http://www.cidoc-crm.org/cidoc-crm/E90_Symbolic_Object"/>
	<rdf:type rdf:resource="http://www.loa-cnr.it/ontologies/DOLCE-Lite#endurant"/>
	<lrmoo:R17i_was_created_by rdf:resource="http://academictourism.com/entity/BRF0005.SCH"/>
	<cidoc-crm:P129_is_about rdf:resource="http://academictourism.com/entity/BRF0005.RS"/>
	<cidoc-crm:P12i_was_present_at rdf:resource="http://academictourism.com/entity/BRF0005.SCH"/>
	<cidoc-crm:P67_refers_to rdf:resource="http://academictourism.com/entity/BRF0005.RS"/>
	<cidoc-crm:P92i_was_brought_into_existence_by rdf:resource="http://academictourism.com/entity/BRF0005.SCH"/>
	<cidoc-crm:P94i_was_created_by rdf:resource="http://academictourism.com/entity/BRF0005.SCH"/>
	<rdfs:comment>Brief V
Uit Göttingen van den 12 July 1816.

Uitmuntende bibliotheek te Göttingen – Moeylyke post van bibliothecaris – De boeken worden ook mede naar huis gegeven – Bustes &amp; beelden op de bibliotheek – Getal der gewone en buitengewone Hoogleeraren – Collegie van Profr Hugo – Gedistingueerde plaats op de colleges voor Graven – Voorlezingen van Professor Heeren en van Professor Bauer – [IV] Verscheiden colleges van den Hoogleeraar Blumenbach – Zonderlinge uitdrukkingen en gewoonten van dien man – Een onzer hoort van Z Hoog Geleer. woordelyk hetzelfde collegie als voor 7 jaar – Schedel cabinet van Blumenbach – Overig kabinet niet kunnen zien – Redenen daarvan – Observatorium – Entbindungshaus – Chirurgisch hospitaal – Museum – Iets over de Studenten – Duelleeren aan de ordre van den dag – Oude Academiekennis aangetroffen – Afscheid en vertrek van den Heer de Geer – Staaltje van Duitsche manieren – Bladz 36.</rdfs:comment>
</rdf:Description>

<rdf:Description rdf:about="http://academictourism.com/entity/BRF0005.RS">
	<rdf:type rdf:resource="http://www.w3.org/2002/07/owl#NamedIndividual"/>
	<rdf:type rdf:resource="http://www.cidoc-crm.org/cidoc-crm/E1_CRM_Entity"/>
	<rdf:type rdf:resource="http://www.cidoc-crm.org/cidoc-crm/E2_Temporal_Entity"/>
	<rdf:type rdf:resource="http://www.cidoc-crm.org/cidoc-crm/E4_Period"/>
	<rdf:type rdf:resource="http://www.cidoc-crm.org/cidoc-crm/E5_Event"/>
	<rdf:type rdf:resource="http://www.cidoc-crm.org/cidoc-crm/E7_Activity"/>
	<rdf:type rdf:resource="http://www.cidoc-crm.org/cidoc-crm/E92_Spacetime_Volume"/>
	<rdf:type rdf:resource="http://www.loa-cnr.it/ontologies/DOLCE-Lite#perdurant"/>
	<cidoc-crm:P10i_contains rdf:resource="http://academictourism.com/entity/BRF0005.RS.L0001"/>
	<cidoc-crm:P10i_contains rdf:resource="http://academictourism.com/entity/BRF0005.RS.L0002"/>
	<cidoc-crm:P10i_contains rdf:resource="http://academictourism.com/entity/BRF0005.RS.L0003"/>
	<cidoc-crm:P10i_contains rdf:resource="http://academictourism.com/entity/BRF0005.RS.L0004"/>
	<cidoc-crm:P11_had_participant rdf:resource="http://academictourism.com/entity/TG"/>
	<cidoc-crm:P129i_is_subject_of rdf:resource="http://academictourism.com/entity/BRF0005"/>
	<cidoc-crm:P12_occurred_in_the_presence_of rdf:resource="http://academictourism.com/entity/TG"/>
	<cidoc-crm:P132_spatiotemporally_overlaps_with rdf:resource="http://academictourism.com/entity/BRF0005.RS.L0001"/>
	<cidoc-crm:P132_spatiotemporally_overlaps_with rdf:resource="http://academictourism.com/entity/BRF0005.RS.L0002"/>
	<cidoc-crm:P132_spatiotemporally_overlaps_with rdf:resource="http://academictourism.com/entity/BRF0005.RS.L0003"/>
	<cidoc-crm:P132_spatiotemporally_overlaps_with rdf:resource="http://academictourism.com/entity/BRF0005.RS.L0004"/>
	<cidoc-crm:P173i_ends_after_or_with_the_start_of rdf:resource="http://academictourism.com/entity/BRF0004.RS"/>
	<cidoc-crm:P174i_ends_after_the_start_of rdf:resource="http://academictourism.com/entity/BRF0004.RS"/>
	<cidoc-crm:P175i_starts_after_or_with_the_start_of rdf:resource="http://academictourism.com/entity/BRF0004.RS"/>
	<cidoc-crm:P176i_starts_after_the_start_of rdf:resource="http://academictourism.com/entity/BRF0004.RS"/>
	<cidoc-crm:P182i_starts_after_or_with_the_end_of rdf:resource="http://academictourism.com/entity/BRF0004.RS"/>
	<cidoc-crm:P183i_starts_after_the_end_of rdf:resource="http://academictourism.com/entity/BRF0004.RS"/>
	<cidoc-crm:P184i_ends_with_or_after_the_end_of rdf:resource="http://academictourism.com/entity/BRF0004.RS"/>
	<cidoc-crm:P185i_ends_after_the_end_of rdf:resource="http://academictourism.com/entity/BRF0004.RS"/>
	<cidoc-crm:P67i_is_referred_to_by rdf:resource="http://academictourism.com/entity/BRF0005"/>
	<cidoc-crm:P8_took_place_on_or_within rdf:resource="http://academictourism.com/entity/LOC0007"/>
	<rdfs:label>Tour in letter 5</rdfs:label>
</rdf:Description>

<rdf:Description rdf:about="http://academictourism.com/entity/BRF0005.RS.L0001">
	<rdf:type rdf:resource="http://www.w3.org/2002/07/owl#NamedIndividual"/>
	<rdf:type rdf:resource="http://www.cidoc-crm.org/cidoc-crm/E1_CRM_Entity"/>
	<rdf:type rdf:resource="http://www.cidoc-crm.org/cidoc-crm/E2_Temporal_Entity"/>
	<rdf:type rdf:resource="http://www.cidoc-crm.org/cidoc-crm/E4_Period"/>
	<rdf:type rdf:resource="http://www.cidoc-crm.org/cidoc-crm/E5_Event"/>
	<rdf:type rdf:resource="http://www.cidoc-crm.org/cidoc-crm/E7_Activity"/>
	<rdf:type rdf:resource="http://www.cidoc-crm.org/cidoc-crm/E92_Spacetime_Volume"/>
	<rdf:type rdf:resource="http://www.loa-cnr.it/ontologies/DOLCE-Lite#perdurant"/>
	<academictourism:conveys rdf:resource="http://academictourism.com/entity/CT.BRF0005.RS.L0001"/>
	<cidoc-crm:P10_falls_within rdf:resource="http://academictourism.com/entity/BRF0005.RS"/>
	<cidoc-crm:P11_had_participant rdf:resource="http://academictourism.com/entity/PER0005"/>
	<cidoc-crm:P11_had_participant rdf:resource="http://academictourism.com/entity/TG"/>
	<cidoc-crm:P12_occurred_in_the_presence_of rdf:resource="http://academictourism.com/entity/PER0005"/>
	<cidoc-crm:P12_occurred_in_the_presence_of rdf:resource="http://academictourism.com/entity/TG"/>
	<cidoc-crm:P132_spatiotemporally_overlaps_with rdf:resource="http://academictourism.com/entity/BRF0005.RS"/>
	<cidoc-crm:P14_carried_out_by rdf:resource="http://academictourism.com/entity/PER0005"/>
	<cidoc-crm:P2_has_type rdf:resource="http://vocab.getty.edu/page/aat/300026673"/>
	<cidoc-crm:P7_took_place_at rdf:resource="http://academictourism.com/entity/LOC0007.KM001"/>
	<rdfs:label>Lecture1</rdfs:label>
</rdf:Description>

<rdf:Description rdf:about="http://academictourism.com/entity/BRF0005.RS.L0002">
	<rdf:type rdf:resource="http://www.w3.org/2002/07/owl#NamedIndividual"/>
	<rdf:type rdf:resource="http://www.cidoc-crm.org/cidoc-crm/E1_CRM_Entity"/>
	<rdf:type rdf:resource="http://www.cidoc-crm.org/cidoc-crm/E2_Temporal_Entity"/>
	<rdf:type rdf:resource="http://www.cidoc-crm.org/cidoc-crm/E4_Period"/>
	<rdf:type rdf:resource="http://www.cidoc-crm.org/cidoc-crm/E5_Event"/>
	<rdf:type rdf:resource="http://www.cidoc-crm.org/cidoc-crm/E7_Activity"/>
	<rdf:type rdf:resource="http://www.cidoc-crm.org/cidoc-crm/E92_Spacetime_Volume"/>
	<rdf:type rdf:resource="http://www.loa-cnr.it/ontologies/DOLCE-Lite#perdurant"/>
	<academictourism:conveys rdf:resource="http://academictourism.com/entity/CT.BRF0005.RS.L0002"/>
	<cidoc-crm:P10_falls_within rdf:resource="http://academictourism.com/entity/BRF0005.RS"/>
	<cidoc-crm:P11_had_participant rdf:resource="http://academictourism.com/entity/PER0006"/>
	<cidoc-crm:P11_had_participant rdf:resource="http://academictourism.com/entity/TG"/>
	<cidoc-crm:P12_occurred_in_the_presence_of rdf:resource="http://academictourism.com/entity/PER0006"/>
	<cidoc-crm:P12_occurred_in_the_presence_of rdf:resource="http://academictourism.com/entity/TG"/>
	<cidoc-crm:P132_spatiotemporally_overlaps_with rdf:resource="http://academictourism.com/entity/BRF0005.RS"/>
	<cidoc-crm:P14_carried_out_by rdf:resource="http://academictourism.com/entity/PER0006"/>
	<cidoc-crm:P2_has_type rdf:resource="http://vocab.getty.edu/page/aat/300026673"/>
	<cidoc-crm:P7_took_place_at rdf:resource="http://academictourism.com/entity/LOC0007.KM001"/>
	<rdfs:label>Lecture2</rdfs:label>
</rdf:Description>

<rdf:Description rdf:about="http://academictourism.com/entity/BRF0005.RS.L0003">
	<rdf:type rdf:resource="http://www.w3.org/2002/07/owl#NamedIndividual"/>
	<rdf:type rdf:resource="http://www.cidoc-crm.org/cidoc-crm/E1_CRM_Entity"/>
	<rdf:type rdf:resource="http://www.cidoc-crm.org/cidoc-crm/E2_Temporal_Entity"/>
	<rdf:type rdf:resource="http://www.cidoc-crm.org/cidoc-crm/E4_Period"/>
	<rdf:type rdf:resource="http://www.cidoc-crm.org/cidoc-crm/E5_Event"/>
	<rdf:type rdf:resource="http://www.cidoc-crm.org/cidoc-crm/E7_Activity"/>
	<rdf:type rdf:resource="http://www.cidoc-crm.org/cidoc-crm/E92_Spacetime_Volume"/>
	<rdf:type rdf:resource="http://www.loa-cnr.it/ontologies/DOLCE-Lite#perdurant"/>
	<academictourism:conveys rdf:resource="http://academictourism.com/entity/CT.BRF0005.RS.L0003"/>
	<cidoc-crm:P10_falls_within rdf:resource="http://academictourism.com/entity/BRF0005.RS"/>
	<cidoc-crm:P11_had_participant rdf:resource="http://academictourism.com/entity/PER0007"/>
	<cidoc-crm:P11_had_participant rdf:resource="http://academictourism.com/entity/TG"/>
	<cidoc-crm:P12_occurred_in_the_presence_of rdf:resource="http://academictourism.com/entity/PER0007"/>
	<cidoc-crm:P12_occurred_in_the_presence_of rdf:resource="http://academictourism.com/entity/TG"/>
	<cidoc-crm:P132_spatiotemporally_overlaps_with rdf:resource="http://academictourism.com/entity/BRF0005.RS"/>
	<cidoc-crm:P14_carried_out_by rdf:resource="http://academictourism.com/entity/PER0007"/>
	<cidoc-crm:P2_has_type rdf:resource="http://vocab.getty.edu/page/aat/300026673"/>
	<cidoc-crm:P7_took_place_at rdf:resource="http://academictourism.com/entity/LOC0007.KM001"/>
	<rdfs:label>Lecture3</rdfs:label>
</rdf:Description>

<rdf:Description rdf:about="http://academictourism.com/entity/BRF0005.RS.L0004">
	<rdf:type rdf:resource="http://www.w3.org/2002/07/owl#NamedIndividual"/>
	<rdf:type rdf:resource="http://www.cidoc-crm.org/cidoc-crm/E1_CRM_Entity"/>
	<rdf:type rdf:resource="http://www.cidoc-crm.org/cidoc-crm/E2_Temporal_Entity"/>
	<rdf:type rdf:resource="http://www.cidoc-crm.org/cidoc-crm/E4_Period"/>
	<rdf:type rdf:resource="http://www.cidoc-crm.org/cidoc-crm/E5_Event"/>
	<rdf:type rdf:resource="http://www.cidoc-crm.org/cidoc-crm/E7_Activity"/>
	<rdf:type rdf:resource="http://www.cidoc-crm.org/cidoc-crm/E92_Spacetime_Volume"/>
	<rdf:type rdf:resource="http://www.loa-cnr.it/ontologies/DOLCE-Lite#perdurant"/>
	<academictourism:conveys rdf:resource="http://academictourism.com/entity/CT.BRF0005.RS.L0004"/>
	<cidoc-crm:P10_falls_within rdf:resource="http://academictourism.com/entity/BRF0005.RS"/>
	<cidoc-crm:P11_had_participant rdf:resource="http://academictourism.com/entity/PER0008"/>
	<cidoc-crm:P11_had_participant rdf:resource="http://academictourism.com/entity/TG"/>
	<cidoc-crm:P12_occurred_in_the_presence_of rdf:resource="http://academictourism.com/entity/PER0008"/>
	<cidoc-crm:P12_occurred_in_the_presence_of rdf:resource="http://academictourism.com/entity/TG"/>
	<cidoc-crm:P132_spatiotemporally_overlaps_with rdf:resource="http://academictourism.com/entity/BRF0005.RS"/>
	<cidoc-crm:P14_carried_out_by rdf:resource="http://academictourism.com/entity/PER0008"/>
	<cidoc-crm:P2_has_type rdf:resource="http://vocab.getty.edu/page/aat/300026673"/>
	<cidoc-crm:P7_took_place_at rdf:resource="http://academictourism.com/entity/LOC0007.KM001"/>
	<rdfs:label>Lecture4</rdfs:label>
</rdf:Description>

<rdf:Description rdf:about="http://academictourism.com/entity/BRF0005.SCH">
	<rdf:type rdf:resource="http://www.w3.org/2002/07/owl#NamedIndividual"/>
	<rdf:type rdf:resource="http://iflastandards.info/ns/lrm/lrmoo/F28_Expression_Creation"/>
	<rdf:type rdf:resource="http://www.cidoc-crm.org/cidoc-crm/E11_Modification"/>
	<rdf:type rdf:resource="http://www.cidoc-crm.org/cidoc-crm/E12_Production"/>
	<rdf:type rdf:resource="http://www.cidoc-crm.org/cidoc-crm/E1_CRM_Entity"/>
	<rdf:type rdf:resource="http://www.cidoc-crm.org/cidoc-crm/E2_Temporal_Entity"/>
	<rdf:type rdf:resource="http://www.cidoc-crm.org/cidoc-crm/E4_Period"/>
	<rdf:type rdf:resource="http://www.cidoc-crm.org/cidoc-crm/E5_Event"/>
	<rdf:type rdf:resource="http://www.cidoc-crm.org/cidoc-crm/E63_Beginning_of_Existence"/>
	<rdf:type rdf:resource="http://www.cidoc-crm.org/cidoc-crm/E65_Creation"/>
	<rdf:type rdf:resource="http://www.cidoc-crm.org/cidoc-crm/E7_Activity"/>
	<rdf:type rdf:resource="http://www.cidoc-crm.org/cidoc-crm/E92_Spacetime_Volume"/>
	<rdf:type rdf:resource="http://www.loa-cnr.it/ontologies/DOLCE-Lite#perdurant"/>
	<lrmoo:R17_created rdf:resource="http://academictourism.com/entity/BRF0005"/>
	<cidoc-crm:P11_had_participant rdf:resource="http://academictourism.com/entity/PER0001"/>
	<cidoc-crm:P12_occurred_in_the_presence_of rdf:resource="http://academictourism.com/entity/BRF0005"/>
	<cidoc-crm:P12_occurred_in_the_presence_of rdf:resource="http://academictourism.com/entity/PER0001"/>
	<cidoc-crm:P14_carried_out_by rdf:resource="http://academictourism.com/entity/PER0001"/>
	<cidoc-crm:P92_brought_into_existence rdf:resource="http://academictourism.com/entity/BRF0005"/>
	<cidoc-crm:P94_has_created rdf:resource="http://academictourism.com/entity/BRF0005"/>
	<rdfs:label>Writing letter 5</rdfs:label>
</rdf:Description>

<rdf:Description rdf:about="http://academictourism.com/entity/CT.BRF0005.RS.L0001">
	<rdf:type rdf:resource="http://www.w3.org/2002/07/owl#NamedIndividual"/>
	<rdf:type rdf:resource="http://www.cidoc-crm.org/cidoc-crm/E1_CRM_Entity"/>
	<rdf:type rdf:resource="http://www.cidoc-crm.org/cidoc-crm/E28_Conceptual_Object"/>
	<rdf:type rdf:resource="http://www.cidoc-crm.org/cidoc-crm/E70_Thing"/>
	<rdf:type rdf:resource="http://www.cidoc-crm.org/cidoc-crm/E71_Human-Made_Thing"/>
	<rdf:type rdf:resource="http://www.cidoc-crm.org/cidoc-crm/E77_Persistent_Item"/>
	<rdf:type rdf:resource="http://www.cidoc-crm.org/cidoc-crm/E89_Propositional_Object"/>
	<rdf:type rdf:resource="http://www.loa-cnr.it/ontologies/DOLCE-Lite#endurant"/>
	<academictourism:is_conveyed_by rdf:resource="http://academictourism.com/entity/BRF0005.RS.L0001"/>
	<cidoc-crm:P129_is_about rdf:resource="https://www.wikidata.org/wiki/Q131552"/>
	<cidoc-crm:P129_is_about rdf:resource="https://www.wikidata.org/wiki/Q132545"/>
	<cidoc-crm:P129_is_about rdf:resource="https://www.wikidata.org/wiki/Q170022"/>
	<cidoc-crm:P129_is_about rdf:resource="https://www.wikidata.org/wiki/Q187719"/>
	<cidoc-crm:P129_is_about rdf:resource="https://www.wikidata.org/wiki/Q4932206"/>
	<cidoc-crm:P67_refers_to rdf:resource="https://www.wikidata.org/wiki/Q131552"/>
	<cidoc-crm:P67_refers_to rdf:resource="https://www.wikidata.org/wiki/Q132545"/>
	<cidoc-crm:P67_refers_to rdf:resource="https://www.wikidata.org/wiki/Q170022"/>
	<cidoc-crm:P67_refers_to rdf:resource="https://www.wikidata.org/wiki/Q187719"/>
	<cidoc-crm:P67_refers_to rdf:resource="https://www.wikidata.org/wiki/Q4932206"/>
</rdf:Description>

<rdf:Description rdf:about="http://academictourism.com/entity/CT.BRF0005.RS.L0002">
	<rdf:type rdf:resource="http://www.w3.org/2002/07/owl#NamedIndividual"/>
	<rdf:type rdf:resource="http://www.cidoc-crm.org/cidoc-crm/E1_CRM_Entity"/>
	<rdf:type rdf:resource="http://www.cidoc-crm.org/cidoc-crm/E28_Conceptual_Object"/>
	<rdf:type rdf:resource="http://www.cidoc-crm.org/cidoc-crm/E70_Thing"/>
	<rdf:type rdf:resource="http://www.cidoc-crm.org/cidoc-crm/E71_Human-Made_Thing"/>
	<rdf:type rdf:resource="http://www.cidoc-crm.org/cidoc-crm/E77_Persistent_Item"/>
	<rdf:type rdf:resource="http://www.cidoc-crm.org/cidoc-crm/E89_Propositional_Object"/>
	<rdf:type rdf:resource="http://www.loa-cnr.it/ontologies/DOLCE-Lite#endurant"/>
	<academictourism:is_conveyed_by rdf:resource="http://academictourism.com/entity/BRF0005.RS.L0002"/>
	<cidoc-crm:P129_is_about rdf:resource="https://www.wikidata.org/wiki/Q908578"/>
	<cidoc-crm:P67_refers_to rdf:resource="https://www.wikidata.org/wiki/Q908578"/>
</rdf:Description>

<rdf:Description rdf:about="http://academictourism.com/entity/CT.BRF0005.RS.L0003">
	<rdf:type rdf:resource="http://www.w3.org/2002/07/owl#NamedIndividual"/>
	<rdf:type rdf:resource="http://www.cidoc-crm.org/cidoc-crm/E1_CRM_Entity"/>
	<rdf:type rdf:resource="http://www.cidoc-crm.org/cidoc-crm/E28_Conceptual_Object"/>
	<rdf:type rdf:resource="http://www.cidoc-crm.org/cidoc-crm/E70_Thing"/>
	<rdf:type rdf:resource="http://www.cidoc-crm.org/cidoc-crm/E71_Human-Made_Thing"/>
	<rdf:type rdf:resource="http://www.cidoc-crm.org/cidoc-crm/E77_Persistent_Item"/>
	<rdf:type rdf:resource="http://www.cidoc-crm.org/cidoc-crm/E89_Propositional_Object"/>
	<rdf:type rdf:resource="http://www.loa-cnr.it/ontologies/DOLCE-Lite#endurant"/>
	<academictourism:is_conveyed_by rdf:resource="http://academictourism.com/entity/BRF0005.RS.L0003"/>
	<cidoc-crm:P129_is_about rdf:resource="https://www.wikidata.org/wiki/Q29524"/>
	<cidoc-crm:P67_refers_to rdf:resource="https://www.wikidata.org/wiki/Q29524"/>
</rdf:Description>

<rdf:Description rdf:about="http://academictourism.com/entity/CT.BRF0005.RS.L0004">
	<rdf:type rdf:resource="http://www.w3.org/2002/07/owl#NamedIndividual"/>
	<rdf:type rdf:resource="http://www.cidoc-crm.org/cidoc-crm/E1_CRM_Entity"/>
	<rdf:type rdf:resource="http://www.cidoc-crm.org/cidoc-crm/E28_Conceptual_Object"/>
	<rdf:type rdf:resource="http://www.cidoc-crm.org/cidoc-crm/E70_Thing"/>
	<rdf:type rdf:resource="http://www.cidoc-crm.org/cidoc-crm/E71_Human-Made_Thing"/>
	<rdf:type rdf:resource="http://www.cidoc-crm.org/cidoc-crm/E77_Persistent_Item"/>
	<rdf:type rdf:resource="http://www.cidoc-crm.org/cidoc-crm/E89_Propositional_Object"/>
	<rdf:type rdf:resource="http://www.loa-cnr.it/ontologies/DOLCE-Lite#endurant"/>
	<academictourism:is_conveyed_by rdf:resource="http://academictourism.com/entity/BRF0005.RS.L0004"/>
	<cidoc-crm:P129_is_about rdf:resource="https://www.wikidata.org/wiki/Q484591"/>
	<cidoc-crm:P129_is_about rdf:resource="https://www.wikidata.org/wiki/Q521"/>
	<cidoc-crm:P67_refers_to rdf:resource="https://www.wikidata.org/wiki/Q484591"/>
	<cidoc-crm:P67_refers_to rdf:resource="https://www.wikidata.org/wiki/Q521"/>
</rdf:Description>

<rdf:Description rdf:about="http://academictourism.com/entity/DM.MISC0002">
	<rdf:type rdf:resource="http://www.w3.org/2002/07/owl#NamedIndividual"/>
	<rdf:type rdf:resource="http://www.cidoc-crm.org/cidoc-crm/E1_CRM_Entity"/>
	<rdf:type rdf:resource="http://www.cidoc-crm.org/cidoc-crm/E54_Dimension"/>
	<cidoc-crm:P43i_is_dimension_of rdf:resource="http://academictourism.com/entity/MISC0002"/>
	<cidoc-crm:P3_has_note>7 voet breed en 9½ voet hoog</cidoc-crm:P3_has_note>
</rdf:Description>

<rdf:Description rdf:about="http://academictourism.com/entity/DR.BRF0004.RS.RS0001">
	<rdf:type rdf:resource="http://www.w3.org/2002/07/owl#NamedIndividual"/>
	<rdf:type rdf:resource="http://www.cidoc-crm.org/cidoc-crm/E1_CRM_Entity"/>
	<rdf:type rdf:resource="http://www.cidoc-crm.org/cidoc-crm/E54_Dimension"/>
	<lrmoo:R70i_is_dimension_of rdf:resource="http://academictourism.com/entity/TS.BRF0004.RS.RS0001"/>
	<cidoc-crm:P43i_is_dimension_of rdf:resource="http://academictourism.com/entity/TS.BRF0004.RS.RS0001"/>
	<cidoc-crm:P3_has_note>more than 1 hour</cidoc-crm:P3_has_note>
</rdf:Description>

<rdf:Description rdf:about="http://academictourism.com/entity/DR.BRF0004.RS.RS0006">
	<rdf:type rdf:resource="http://www.w3.org/2002/07/owl#NamedIndividual"/>
	<rdf:type rdf:resource="http://www.cidoc-crm.org/cidoc-crm/E1_CRM_Entity"/>
	<rdf:type rdf:resource="http://www.cidoc-crm.org/cidoc-crm/E54_Dimension"/>
	<cidoc-crm:P43i_is_dimension_of rdf:resource="http://academictourism.com/entity/TS.BRF0004.RS.RS0006"/>
	<cidoc-crm:P91_has_unit rdf:resource="http://academictourism.com/entity/U0001"/>
	<cidoc-crm:P90_has_value rdf:datatype="http://www.w3.org/2001/XMLSchema#integer">10</cidoc-crm:P90_has_value>
</rdf:Description>

<rdf:Description rdf:about="http://academictourism.com/entity/DT.BRF0004.RS.RS0004.RS0002">
	<rdf:type rdf:resource="http://www.w3.org/2002/07/owl#NamedIndividual"/>
	<rdf:type rdf:resource="http://www.cidoc-crm.org/cidoc-crm/E1_CRM_Entity"/>
	<rdf:type rdf:resource="http://www.cidoc-crm.org/cidoc-crm/E54_Dimension"/>
	<cidoc-crm:P43i_is_dimension_of rdf:resource="http://academictourism.com/entity/R.BRF0004.RS.RS0004.RS0002"/>
	<cidoc-crm:P3_has_note>900 trappen</cidoc-crm:P3_has_note>
</rdf:Description>

<rdf:Description rdf:about="http://academictourism.com/entity/J0001">
	<rdf:type rdf:resource="http://www.w3.org/2002/07/owl#NamedIndividual"/>
	<rdf:type rdf:resource="http://www.cidoc-crm.org/cidoc-crm/E1_CRM_Entity"/>
	<rdf:type rdf:resource="http://www.cidoc-crm.org/cidoc-crm/E2_Temporal_Entity"/>
	<rdf:type rdf:resource="http://www.cidoc-crm.org/cidoc-crm/E4_Period"/>
	<rdf:type rdf:resource="http://www.cidoc-crm.org/cidoc-crm/E5_Event"/>
	<rdf:type rdf:resource="http://www.cidoc-crm.org/cidoc-crm/E7_Activity"/>
	<rdf:type rdf:resource="http://www.cidoc-crm.org/cidoc-crm/E85_Joining"/>
	<rdf:type rdf:resource="http://www.cidoc-crm.org/cidoc-crm/E92_Spacetime_Volume"/>
	<rdf:type rdf:resource="http://www.loa-cnr.it/ontologies/DOLCE-Lite#perdurant"/>
	<cidoc-crm:P11_had_participant rdf:resource="http://academictourism.com/entity/PER0002"/>
	<cidoc-crm:P11_had_participant rdf:resource="http://academictourism.com/entity/PER0003"/>
	<cidoc-crm:P11_had_participant rdf:resource="http://academictourism.com/entity/PER0004"/>
	<cidoc-crm:P11_had_participant rdf:resource="http://academictourism.com/entity/TG"/>
	<cidoc-crm:P12_occurred_in_the_presence_of rdf:resource="http://academictourism.com/entity/PER0002"/>
	<cidoc-crm:P12_occurred_in_the_presence_of rdf:resource="http://academictourism.com/entity/PER0003"/>
	<cidoc-crm:P12_occurred_in_the_presence_of rdf:resource="http://academictourism.com/entity/PER0004"/>
	<cidoc-crm:P12_occurred_in_the_presence_of rdf:resource="http://academictourism.com/entity/TG"/>
	<cidoc-crm:P143_joined rdf:resource="http://academictourism.com/entity/PER0003"/>
	<cidoc-crm:P143_joined rdf:resource="http://academictourism.com/entity/PER0004"/>
	<cidoc-crm:P144_joined_with rdf:resource="http://academictourism.com/entity/TG"/>
	<cidoc-crm:P173_starts_before_or_with_the_end_of rdf:resource="http://academictourism.com/entity/J0002"/>
	<cidoc-crm:P174_starts_before_the_end_of rdf:resource="http://academictourism.com/entity/J0002"/>
	<cidoc-crm:P175_starts_before_or_with_the_start_of rdf:resource="http://academictourism.com/entity/J0002"/>
	<cidoc-crm:P176_starts_before_the_start_of rdf:resource="http://academictourism.com/entity/J0002"/>
	<cidoc-crm:P182_ends_before_or_with_the_start_of rdf:resource="http://academictourism.com/entity/J0002"/>
	<cidoc-crm:P183_ends_before_the_start_of rdf:resource="http://academictourism.com/entity/J0002"/>
	<cidoc-crm:P184_ends_before_or_with_the_end_of rdf:resource="http://academictourism.com/entity/J0002"/>
	<cidoc-crm:P185_ends_before_the_end_of rdf:resource="http://academictourism.com/entity/J0002"/>
	<cidoc-crm:P7_took_place_at rdf:resource="http://academictourism.com/entity/LOC0001"/>
</rdf:Description>

<rdf:Description rdf:about="http://academictourism.com/entity/J0002">
	<rdf:type rdf:resource="http://www.w3.org/2002/07/owl#NamedIndividual"/>
	<rdf:type rdf:resource="http://www.cidoc-crm.org/cidoc-crm/E1_CRM_Entity"/>
	<rdf:type rdf:resource="http://www.cidoc-crm.org/cidoc-crm/E2_Temporal_Entity"/>
	<rdf:type rdf:resource="http://www.cidoc-crm.org/cidoc-crm/E4_Period"/>
	<rdf:type rdf:resource="http://www.cidoc-crm.org/cidoc-crm/E5_Event"/>
	<rdf:type rdf:resource="http://www.cidoc-crm.org/cidoc-crm/E7_Activity"/>
	<rdf:type rdf:resource="http://www.cidoc-crm.org/cidoc-crm/E85_Joining"/>
	<rdf:type rdf:resource="http://www.cidoc-crm.org/cidoc-crm/E92_Spacetime_Volume"/>
	<rdf:type rdf:resource="http://www.loa-cnr.it/ontologies/DOLCE-Lite#perdurant"/>
	<cidoc-crm:P11_had_participant rdf:resource="http://academictourism.com/entity/PER0001"/>
	<cidoc-crm:P11_had_participant rdf:resource="http://academictourism.com/entity/TG"/>
	<cidoc-crm:P12_occurred_in_the_presence_of rdf:resource="http://academictourism.com/entity/PER0001"/>
	<cidoc-crm:P12_occurred_in_the_presence_of rdf:resource="http://academictourism.com/entity/TG"/>
	<cidoc-crm:P143_joined rdf:resource="http://academictourism.com/entity/PER0001"/>
	<cidoc-crm:P144_joined_with rdf:resource="http://academictourism.com/entity/TG"/>
	<cidoc-crm:P173_starts_before_or_with_the_end_of rdf:resource="http://academictourism.com/entity/BRF0004.RS"/>
	<cidoc-crm:P173i_ends_after_or_with_the_start_of rdf:resource="http://academictourism.com/entity/J0001"/>
	<cidoc-crm:P174_starts_before_the_end_of rdf:resource="http://academictourism.com/entity/BRF0004.RS"/>
	<cidoc-crm:P174i_ends_after_the_start_of rdf:resource="http://academictourism.com/entity/J0001"/>
	<cidoc-crm:P175_starts_before_or_with_the_start_of rdf:resource="http://academictourism.com/entity/BRF0004.RS"/>
	<cidoc-crm:P175i_starts_after_or_with_the_start_of rdf:resource="http://academictourism.com/entity/J0001"/>
	<cidoc-crm:P176_starts_before_the_start_of rdf:resource="http://academictourism.com/entity/BRF0004.RS"/>
	<cidoc-crm:P176i_starts_after_the_start_of rdf:resource="http://academictourism.com/entity/J0001"/>
	<cidoc-crm:P182_ends_before_or_with_the_start_of rdf:resource="http://academictourism.com/entity/BRF0004.RS"/>
	<cidoc-crm:P182i_starts_after_or_with_the_end_of rdf:resource="http://academictourism.com/entity/J0001"/>
	<cidoc-crm:P183_ends_before_the_start_of rdf:resource="http://academictourism.com/entity/BRF0004.RS"/>
	<cidoc-crm:P183i_starts_after_the_end_of rdf:resource="http://academictourism.com/entity/J0001"/>
	<cidoc-crm:P184_ends_before_or_with_the_end_of rdf:resource="http://academictourism.com/entity/BRF0004.RS"/>
	<cidoc-crm:P184i_ends_with_or_after_the_end_of rdf:resource="http://academictourism.com/entity/J0001"/>
	<cidoc-crm:P185_ends_before_the_end_of rdf:resource="http://academictourism.com/entity/BRF0004.RS"/>
	<cidoc-crm:P185i_ends_after_the_end_of rdf:resource="http://academictourism.com/entity/J0001"/>
	<cidoc-crm:P4_has_time-span rdf:resource="http://academictourism.com/entity/TS.BRF0004.RS.RS0001"/>
	<cidoc-crm:P7_took_place_at rdf:resource="http://academictourism.com/entity/LOC0001"/>
</rdf:Description>

<rdf:Description rdf:about="http://academictourism.com/entity/L0001">
	<rdf:type rdf:resource="http://www.w3.org/2002/07/owl#NamedIndividual"/>
	<rdf:type rdf:resource="http://www.cidoc-crm.org/cidoc-crm/E1_CRM_Entity"/>
	<rdf:type rdf:resource="http://www.cidoc-crm.org/cidoc-crm/E2_Temporal_Entity"/>
	<rdf:type rdf:resource="http://www.cidoc-crm.org/cidoc-crm/E4_Period"/>
	<rdf:type rdf:resource="http://www.cidoc-crm.org/cidoc-crm/E5_Event"/>
	<rdf:type rdf:resource="http://www.cidoc-crm.org/cidoc-crm/E7_Activity"/>
	<rdf:type rdf:resource="http://www.cidoc-crm.org/cidoc-crm/E86_Leaving"/>
	<rdf:type rdf:resource="http://www.cidoc-crm.org/cidoc-crm/E92_Spacetime_Volume"/>
	<rdf:type rdf:resource="http://www.loa-cnr.it/ontologies/DOLCE-Lite#perdurant"/>
	<cidoc-crm:P11_had_participant rdf:resource="http://academictourism.com/entity/PER0003"/>
	<cidoc-crm:P11_had_participant rdf:resource="http://academictourism.com/entity/PER0004"/>
	<cidoc-crm:P11_had_participant rdf:resource="http://academictourism.com/entity/TG"/>
	<cidoc-crm:P12_occurred_in_the_presence_of rdf:resource="http://academictourism.com/entity/PER0003"/>
	<cidoc-crm:P12_occurred_in_the_presence_of rdf:resource="http://academictourism.com/entity/PER0004"/>
	<cidoc-crm:P12_occurred_in_the_presence_of rdf:resource="http://academictourism.com/entity/TG"/>
	<cidoc-crm:P145_separated rdf:resource="http://academictourism.com/entity/PER0003"/>
	<cidoc-crm:P145_separated rdf:resource="http://academictourism.com/entity/PER0004"/>
	<cidoc-crm:P146_separated_from rdf:resource="http://academictourism.com/entity/TG"/>
	<cidoc-crm:P173_starts_before_or_with_the_end_of rdf:resource="http://academictourism.com/entity/BRF0004.RS.RS0006.RS0001"/>
	<cidoc-crm:P173_starts_before_or_with_the_end_of rdf:resource="http://academictourism.com/entity/L0002"/>
	<cidoc-crm:P174_starts_before_the_end_of rdf:resource="http://academictourism.com/entity/BRF0004.RS.RS0006.RS0001"/>
	<cidoc-crm:P174_starts_before_the_end_of rdf:resource="http://academictourism.com/entity/L0002"/>
	<cidoc-crm:P175_starts_before_or_with_the_start_of rdf:resource="http://academictourism.com/entity/BRF0004.RS.RS0006.RS0001"/>
	<cidoc-crm:P175_starts_before_or_with_the_start_of rdf:resource="http://academictourism.com/entity/L0002"/>
	<cidoc-crm:P176_starts_before_the_start_of rdf:resource="http://academictourism.com/entity/BRF0004.RS.RS0006.RS0001"/>
	<cidoc-crm:P176_starts_before_the_start_of rdf:resource="http://academictourism.com/entity/L0002"/>
	<cidoc-crm:P182_ends_before_or_with_the_start_of rdf:resource="http://academictourism.com/entity/BRF0004.RS.RS0006.RS0001"/>
	<cidoc-crm:P182_ends_before_or_with_the_start_of rdf:resource="http://academictourism.com/entity/L0002"/>
	<cidoc-crm:P183_ends_before_the_start_of rdf:resource="http://academictourism.com/entity/BRF0004.RS.RS0006.RS0001"/>
	<cidoc-crm:P183_ends_before_the_start_of rdf:resource="http://academictourism.com/entity/L0002"/>
	<cidoc-crm:P184_ends_before_or_with_the_end_of rdf:resource="http://academictourism.com/entity/BRF0004.RS.RS0006.RS0001"/>
	<cidoc-crm:P184_ends_before_or_with_the_end_of rdf:resource="http://academictourism.com/entity/L0002"/>
	<cidoc-crm:P185_ends_before_the_end_of rdf:resource="http://academictourism.com/entity/BRF0004.RS.RS0006.RS0001"/>
	<cidoc-crm:P185_ends_before_the_end_of rdf:resource="http://academictourism.com/entity/L0002"/>
	<cidoc-crm:P7_took_place_at rdf:resource="http://academictourism.com/entity/LOC0001"/>
</rdf:Description>

<rdf:Description rdf:about="http://academictourism.com/entity/L0002">
	<rdf:type rdf:resource="http://www.w3.org/2002/07/owl#NamedIndividual"/>
	<rdf:type rdf:resource="http://www.cidoc-crm.org/cidoc-crm/E1_CRM_Entity"/>
	<rdf:type rdf:resource="http://www.cidoc-crm.org/cidoc-crm/E2_Temporal_Entity"/>
	<rdf:type rdf:resource="http://www.cidoc-crm.org/cidoc-crm/E4_Period"/>
	<rdf:type rdf:resource="http://www.cidoc-crm.org/cidoc-crm/E5_Event"/>
	<rdf:type rdf:resource="http://www.cidoc-crm.org/cidoc-crm/E7_Activity"/>
	<rdf:type rdf:resource="http://www.cidoc-crm.org/cidoc-crm/E86_Leaving"/>
	<rdf:type rdf:resource="http://www.cidoc-crm.org/cidoc-crm/E92_Spacetime_Volume"/>
	<rdf:type rdf:resource="http://www.loa-cnr.it/ontologies/DOLCE-Lite#perdurant"/>
	<cidoc-crm:P11_had_participant rdf:resource="http://academictourism.com/entity/PER0001"/>
	<cidoc-crm:P11_had_participant rdf:resource="http://academictourism.com/entity/PER0002"/>
	<cidoc-crm:P12_occurred_in_the_presence_of rdf:resource="http://academictourism.com/entity/PER0001"/>
	<cidoc-crm:P12_occurred_in_the_presence_of rdf:resource="http://academictourism.com/entity/PER0002"/>
	<cidoc-crm:P145_separated rdf:resource="http://academictourism.com/entity/PER0001"/>
	<cidoc-crm:P145_separated rdf:resource="http://academictourism.com/entity/PER0002"/>
	<cidoc-crm:P173i_ends_after_or_with_the_start_of rdf:resource="http://academictourism.com/entity/L0001"/>
	<cidoc-crm:P174i_ends_after_the_start_of rdf:resource="http://academictourism.com/entity/L0001"/>
	<cidoc-crm:P175i_starts_after_or_with_the_start_of rdf:resource="http://academictourism.com/entity/L0001"/>
	<cidoc-crm:P176i_starts_after_the_start_of rdf:resource="http://academictourism.com/entity/L0001"/>
	<cidoc-crm:P182i_starts_after_or_with_the_end_of rdf:resource="http://academictourism.com/entity/L0001"/>
	<cidoc-crm:P183i_starts_after_the_end_of rdf:resource="http://academictourism.com/entity/L0001"/>
	<cidoc-crm:P184i_ends_with_or_after_the_end_of rdf:resource="http://academictourism.com/entity/L0001"/>
	<cidoc-crm:P185i_ends_after_the_end_of rdf:resource="http://academictourism.com/entity/L0001"/>
</rdf:Description>

<rdf:Description rdf:about="http://academictourism.com/entity/LOC0001">
	<rdf:type rdf:resource="http://www.w3.org/2002/07/owl#NamedIndividual"/>
	<rdf:type rdf:resource="http://www.cidoc-crm.org/cidoc-crm/E18_Physical_Thing"/>
	<rdf:type rdf:resource="http://www.cidoc-crm.org/cidoc-crm/E1_CRM_Entity"/>
	<rdf:type rdf:resource="http://www.cidoc-crm.org/cidoc-crm/E53_Place"/>
	<rdf:type rdf:resource="http://www.cidoc-crm.org/cidoc-crm/E70_Thing"/>
	<rdf:type rdf:resource="http://www.cidoc-crm.org/cidoc-crm/E72_Legal_Object"/>
	<rdf:type rdf:resource="http://www.cidoc-crm.org/cidoc-crm/E77_Persistent_Item"/>
	<rdf:type rdf:resource="http://www.loa-cnr.it/ontologies/DOLCE-Lite#endurant"/>
	<rdf:type rdf:resource="http://www.w3.org/2004/02/skos/core#Concept"/>
	<cidoc-crm:P12i_was_present_at rdf:resource="http://academictourism.com/entity/BRF0004.RS.RS0004.RS0002"/>
	<cidoc-crm:P26i_was_destination_of rdf:resource="http://academictourism.com/entity/BRF0004.RS.RS0005"/>
	<cidoc-crm:P27i_was_origin_of rdf:resource="http://academictourism.com/entity/BRF0004.RS"/>
	<cidoc-crm:P27i_was_origin_of rdf:resource="http://academictourism.com/entity/BRF0004.RS.RS0001"/>
	<cidoc-crm:P27i_was_origin_of rdf:resource="http://academictourism.com/entity/BRF0004.RS.RS0006"/>
	<cidoc-crm:P7i_witnessed rdf:resource="http://academictourism.com/entity/BRF0004.RS.RS0005.RS0001"/>
	<cidoc-crm:P7i_witnessed rdf:resource="http://academictourism.com/entity/BRF0004.RS.RS0006.RS0001"/>
	<cidoc-crm:P7i_witnessed rdf:resource="http://academictourism.com/entity/J0001"/>
	<cidoc-crm:P7i_witnessed rdf:resource="http://academictourism.com/entity/J0002"/>
	<cidoc-crm:P7i_witnessed rdf:resource="http://academictourism.com/entity/L0001"/>
	<skos:closeMatch rdf:resource="http://vocab.getty.edu/page/tgn/7004431"/>
	<skos:closeMatch rdf:resource="https://www.wikidata.org/wiki/Q2865"/>
	<skos:mappingRelation rdf:resource="http://vocab.getty.edu/page/tgn/7004431"/>
	<skos:mappingRelation rdf:resource="https://www.wikidata.org/wiki/Q2865"/>
	<skos:semanticRelation rdf:resource="http://vocab.getty.edu/page/tgn/7004431"/>
	<skos:semanticRelation rdf:resource="https://www.wikidata.org/wiki/Q2865"/>
	<rdfs:seeAlso rdf:datatype="http://www.w3.org/2001/XMLSchema#anyURI">https://www.oldmapsonline.org/en/Kassel?gid=53394b71-c230-569c-9ddc-5eea8a458b21#position=11.6651/51.3181/9.4756&amp;year=1809</rdfs:seeAlso>
	<skos:altLabel xml:lang="fr">Cassel</skos:altLabel>
	<skos:altLabel xml:lang="en">Kassel</skos:altLabel>
	<skos:altLabel xml:lang="nl">Kassel</skos:altLabel>
	<skos:prefLabel xml:lang="de">Kassel</skos:prefLabel>
</rdf:Description>

<rdf:Description rdf:about="http://academictourism.com/entity/LOC0002">
	<rdf:type rdf:resource="http://www.w3.org/2002/07/owl#NamedIndividual"/>
	<rdf:type rdf:resource="http://www.cidoc-crm.org/cidoc-crm/E1_CRM_Entity"/>
	<rdf:type rdf:resource="http://www.cidoc-crm.org/cidoc-crm/E53_Place"/>
	<rdf:type rdf:resource="http://www.w3.org/2004/02/skos/core#Concept"/>
	<cidoc-crm:P26i_was_destination_of rdf:resource="http://academictourism.com/entity/BRF0004.RS"/>
	<cidoc-crm:P26i_was_destination_of rdf:resource="http://academictourism.com/entity/BRF0004.RS.RS0006"/>
	<cidoc-crm:P7i_witnessed rdf:resource="http://academictourism.com/entity/BRF0004.RS.RS0006.RS0005"/>
	<cidoc-crm:P89i_contains rdf:resource="http://academictourism.com/entity/LOC0007"/>
	<skos:closeMatch rdf:resource="http://vocab.getty.edu/page/tgn/1039172"/>
	<skos:closeMatch rdf:resource="https://www.wikidata.org/wiki/Q3033"/>
	<skos:mappingRelation rdf:resource="http://vocab.getty.edu/page/tgn/1039172"/>
	<skos:mappingRelation rdf:resource="https://www.wikidata.org/wiki/Q3033"/>
	<skos:semanticRelation rdf:resource="http://vocab.getty.edu/page/tgn/1039172"/>
	<skos:semanticRelation rdf:resource="https://www.wikidata.org/wiki/Q3033"/>
	<rdfs:seeAlso>https://www.oldmapsonline.org/en/G%C3%B6ttingen_(district)?gid=a82eeedf-7eaa-5d9d-a961-57ca17d65fad#position=8.1654/51.526/9.64&amp;year=1801</rdfs:seeAlso>
	<skos:altLabel xml:lang="en">Göttingen</skos:altLabel>
	<skos:altLabel xml:lang="fr">Göttingen</skos:altLabel>
	<skos:altLabel xml:lang="nl">Göttingen</skos:altLabel>
	<skos:prefLabel xml:lang="de">Göttingen</skos:prefLabel>
</rdf:Description>

<rdf:Description rdf:about="http://academictourism.com/entity/LOC0003">
	<rdf:type rdf:resource="http://www.w3.org/2002/07/owl#NamedIndividual"/>
	<rdf:type rdf:resource="http://www.cidoc-crm.org/cidoc-crm/E1_CRM_Entity"/>
	<rdf:type rdf:resource="http://www.cidoc-crm.org/cidoc-crm/E53_Place"/>
	<rdf:type rdf:resource="http://www.w3.org/2004/02/skos/core#Concept"/>
	<cidoc-crm:P89i_contains rdf:resource="http://academictourism.com/entity/LOC0003.CS"/>
	<skos:closeMatch rdf:resource="https://www.wikidata.org/wiki/Q447441"/>
	<skos:mappingRelation rdf:resource="https://www.wikidata.org/wiki/Q447441"/>
	<skos:semanticRelation rdf:resource="https://www.wikidata.org/wiki/Q447441"/>
	<skos:altLabel xml:lang="en">Bergpark Wilhelmshöhe</skos:altLabel>
	<skos:altLabel xml:lang="nl">Bergpark Wilhelmshöhe</skos:altLabel>
	<skos:prefLabel xml:lang="de">Bergpark Wilhelmshöhe</skos:prefLabel>
</rdf:Description>

<rdf:Description rdf:about="http://academictourism.com/entity/LOC0003.CS">
	<rdf:type rdf:resource="http://www.w3.org/2002/07/owl#NamedIndividual"/>
	<rdf:type rdf:resource="http://www.cidoc-crm.org/cidoc-crm/E18_Physical_Thing"/>
	<rdf:type rdf:resource="http://www.cidoc-crm.org/cidoc-crm/E1_CRM_Entity"/>
	<rdf:type rdf:resource="http://www.cidoc-crm.org/cidoc-crm/E53_Place"/>
	<rdf:type rdf:resource="http://www.cidoc-crm.org/cidoc-crm/E70_Thing"/>
	<rdf:type rdf:resource="http://www.cidoc-crm.org/cidoc-crm/E72_Legal_Object"/>
	<rdf:type rdf:resource="http://www.cidoc-crm.org/cidoc-crm/E77_Persistent_Item"/>
	<rdf:type rdf:resource="http://www.loa-cnr.it/ontologies/DOLCE-Lite#endurant"/>
	<rdf:type rdf:resource="http://www.w3.org/2004/02/skos/core#Concept"/>
	<cidoc-crm:P12i_was_present_at rdf:resource="http://academictourism.com/entity/BE.LOC0003.CS"/>
	<cidoc-crm:P157i_provides_reference_space_for rdf:resource="http://academictourism.com/entity/LOC0003.CS.K001"/>
	<cidoc-crm:P157i_provides_reference_space_for rdf:resource="http://academictourism.com/entity/LOC0003.CS.K002"/>
	<cidoc-crm:P157i_provides_reference_space_for rdf:resource="http://academictourism.com/entity/LOC0003.CS.K003"/>
	<cidoc-crm:P157i_provides_reference_space_for rdf:resource="http://academictourism.com/entity/LOC0003.CS.K004"/>
	<cidoc-crm:P26i_was_destination_of rdf:resource="http://academictourism.com/entity/BRF0004.RS.RS0001"/>
	<cidoc-crm:P27i_was_origin_of rdf:resource="http://academictourism.com/entity/BRF0004.RS.RS0005"/>
	<cidoc-crm:P51_has_former_or_current_owner rdf:resource="http://academictourism.com/entity/PER0016"/>
	<cidoc-crm:P59_has_section rdf:resource="http://academictourism.com/entity/LOC0003.CS.K001"/>
	<cidoc-crm:P59_has_section rdf:resource="http://academictourism.com/entity/LOC0003.CS.K002"/>
	<cidoc-crm:P59_has_section rdf:resource="http://academictourism.com/entity/LOC0003.CS.K003"/>
	<cidoc-crm:P59_has_section rdf:resource="http://academictourism.com/entity/LOC0003.CS.K004"/>
	<cidoc-crm:P7i_witnessed rdf:resource="http://academictourism.com/entity/BRF0004.RS.RS0004"/>
	<cidoc-crm:P89_falls_within rdf:resource="http://academictourism.com/entity/LOC0003"/>
	<cidoc-crm:P8i_witnessed rdf:resource="http://academictourism.com/entity/BRF0004.RS.RS0002"/>
	<cidoc-crm:P92i_was_brought_into_existence_by rdf:resource="http://academictourism.com/entity/BE.LOC0003.CS"/>
	<skos:closeMatch rdf:resource="http://vocab.getty.edu/page/tgn/7077709"/>
	<skos:closeMatch rdf:resource="https://www.wikidata.org/wiki/Q687186"/>
	<skos:mappingRelation rdf:resource="http://vocab.getty.edu/page/tgn/7077709"/>
	<skos:mappingRelation rdf:resource="https://www.wikidata.org/wiki/Q687186"/>
	<skos:semanticRelation rdf:resource="http://vocab.getty.edu/page/tgn/7077709"/>
	<skos:semanticRelation rdf:resource="https://www.wikidata.org/wiki/Q687186"/>
	<skos:altLabel xml:lang="de">Napoleonshöhe</skos:altLabel>
	<skos:altLabel xml:lang="de">Schloss Wilhelmshöhe</skos:altLabel>
	<skos:altLabel xml:lang="de">Weissenstein</skos:altLabel>
	<skos:prefLabel xml:lang="de">Wilhelmshöhe</skos:prefLabel>
</rdf:Description>

<rdf:Description rdf:about="http://academictourism.com/entity/LOC0003.CS.K001">
	<rdf:type rdf:resource="http://www.w3.org/2002/07/owl#NamedIndividual"/>
	<rdf:type rdf:resource="http://www.cidoc-crm.org/cidoc-crm/E1_CRM_Entity"/>
	<rdf:type rdf:resource="http://www.cidoc-crm.org/cidoc-crm/E53_Place"/>
	<cidoc-crm:P157_is_at_rest_relative_to rdf:resource="http://academictourism.com/entity/LOC0003.CS"/>
	<cidoc-crm:P2_has_type rdf:resource="http://vocab.getty.edu/page/aat/300240057"/>
	<cidoc-crm:P53i_is_former_or_current_location_of rdf:resource="http://academictourism.com/entity/MISC0002"/>
	<cidoc-crm:P59i_is_located_on_or_within rdf:resource="http://academictourism.com/entity/LOC0003.CS"/>
	<cidoc-crm:P7i_witnessed rdf:resource="http://academictourism.com/entity/BRF0004.RS.RS0002.RS0001"/>
	<rdfs:label>Wilhelmshöhe galery</rdfs:label>
</rdf:Description>

<rdf:Description rdf:about="http://academictourism.com/entity/LOC0003.CS.K002">
	<rdf:type rdf:resource="http://www.w3.org/2002/07/owl#NamedIndividual"/>
	<rdf:type rdf:resource="http://www.cidoc-crm.org/cidoc-crm/E1_CRM_Entity"/>
	<rdf:type rdf:resource="http://www.cidoc-crm.org/cidoc-crm/E53_Place"/>
	<cidoc-crm:P157_is_at_rest_relative_to rdf:resource="http://academictourism.com/entity/LOC0003.CS"/>
	<cidoc-crm:P2_has_type rdf:resource="http://vocab.getty.edu/page/aat/300004362"/>
	<cidoc-crm:P59i_is_located_on_or_within rdf:resource="http://academictourism.com/entity/LOC0003.CS"/>
	<cidoc-crm:P7i_witnessed rdf:resource="http://academictourism.com/entity/BRF0004.RS.RS0002.RS0002"/>
	<rdfs:label>Wilhelmshöhe slaapkamer</rdfs:label>
</rdf:Description>

<rdf:Description rdf:about="http://academictourism.com/entity/LOC0003.CS.K003">
	<rdf:type rdf:resource="http://www.w3.org/2002/07/owl#NamedIndividual"/>
	<rdf:type rdf:resource="http://www.cidoc-crm.org/cidoc-crm/E1_CRM_Entity"/>
	<rdf:type rdf:resource="http://www.cidoc-crm.org/cidoc-crm/E53_Place"/>
	<cidoc-crm:P157_is_at_rest_relative_to rdf:resource="http://academictourism.com/entity/LOC0003.CS"/>
	<cidoc-crm:P2_has_type rdf:resource="http://vocab.getty.edu/page/aat/300004433"/>
	<cidoc-crm:P59i_is_located_on_or_within rdf:resource="http://academictourism.com/entity/LOC0003.CS"/>
	<cidoc-crm:P7i_witnessed rdf:resource="http://academictourism.com/entity/BRF0004.RS.RS0002.RS0003"/>
	<cidoc-crm:P3_has_note>"Eene gansche reeks van kamers nog passeerende kwamen wy boven op de bibliotheek (location), die er uitwendig goed uitziet zynde alle boeken prachtig ingebonden en agter glazen deuren geplaats of het inwendige aan het uiterlyke beantwoort durf ik niet bepalen."</cidoc-crm:P3_has_note>
	<rdfs:label>Wilhelmshöhe bibliotheek</rdfs:label>
</rdf:Description>

<rdf:Description rdf:about="http://academictourism.com/entity/LOC0003.CS.K004">
	<rdf:type rdf:resource="http://www.w3.org/2002/07/owl#NamedIndividual"/>
	<rdf:type rdf:resource="http://www.cidoc-crm.org/cidoc-crm/E1_CRM_Entity"/>
	<rdf:type rdf:resource="http://www.cidoc-crm.org/cidoc-crm/E53_Place"/>
	<cidoc-crm:P157_is_at_rest_relative_to rdf:resource="http://academictourism.com/entity/LOC0003.CS"/>
	<cidoc-crm:P2_has_type rdf:resource="http://vocab.getty.edu/page/aat/300133704"/>
	<cidoc-crm:P53i_is_former_or_current_location_of rdf:resource="http://academictourism.com/entity/MISC0003"/>
	<cidoc-crm:P59i_is_located_on_or_within rdf:resource="http://academictourism.com/entity/LOC0003.CS"/>
	<cidoc-crm:P7i_witnessed rdf:resource="http://academictourism.com/entity/BRF0004.RS.RS0002.RS0004"/>
	<rdfs:label>Wilhelmshöhe zaal</rdfs:label>
</rdf:Description>

<rdf:Description rdf:about="http://academictourism.com/entity/LOC0004.CS">
	<rdf:type rdf:resource="http://www.w3.org/2002/07/owl#NamedIndividual"/>
	<rdf:type rdf:resource="http://www.cidoc-crm.org/cidoc-crm/E18_Physical_Thing"/>
	<rdf:type rdf:resource="http://www.cidoc-crm.org/cidoc-crm/E1_CRM_Entity"/>
	<rdf:type rdf:resource="http://www.cidoc-crm.org/cidoc-crm/E53_Place"/>
	<rdf:type rdf:resource="http://www.cidoc-crm.org/cidoc-crm/E70_Thing"/>
	<rdf:type rdf:resource="http://www.cidoc-crm.org/cidoc-crm/E72_Legal_Object"/>
	<rdf:type rdf:resource="http://www.cidoc-crm.org/cidoc-crm/E77_Persistent_Item"/>
	<rdf:type rdf:resource="http://www.loa-cnr.it/ontologies/DOLCE-Lite#endurant"/>
	<rdf:type rdf:resource="http://www.w3.org/2004/02/skos/core#Concept"/>
	<cidoc-crm:P12i_was_present_at rdf:resource="http://academictourism.com/entity/BRF0004.RS.RS0003"/>
	<cidoc-crm:P157i_provides_reference_space_for rdf:resource="http://academictourism.com/entity/LOC0004.CS.K001"/>
	<cidoc-crm:P157i_provides_reference_space_for rdf:resource="http://academictourism.com/entity/LOC0004.CS.K002"/>
	<cidoc-crm:P157i_provides_reference_space_for rdf:resource="http://academictourism.com/entity/LOC0004.CS.K003"/>
	<cidoc-crm:P157i_provides_reference_space_for rdf:resource="http://academictourism.com/entity/LOC0004.CS.K004"/>
	<cidoc-crm:P157i_provides_reference_space_for rdf:resource="http://academictourism.com/entity/LOC0004.CS.K005"/>
	<cidoc-crm:P59_has_section rdf:resource="http://academictourism.com/entity/LOC0004.CS.K001"/>
	<cidoc-crm:P59_has_section rdf:resource="http://academictourism.com/entity/LOC0004.CS.K002"/>
	<cidoc-crm:P59_has_section rdf:resource="http://academictourism.com/entity/LOC0004.CS.K003"/>
	<cidoc-crm:P59_has_section rdf:resource="http://academictourism.com/entity/LOC0004.CS.K004"/>
	<cidoc-crm:P59_has_section rdf:resource="http://academictourism.com/entity/LOC0004.CS.K005"/>
	<cidoc-crm:P7i_witnessed rdf:resource="http://academictourism.com/entity/BRF0004.RS.RS0003"/>
	<cidoc-crm:P8i_witnessed rdf:resource="http://academictourism.com/entity/BRF0004.RS.RS0003"/>
	<DnS:nvolved-in rdf:resource="http://academictourism.com/entity/ocative_relation1"/>
	<skos:closeMatch rdf:resource="http://vocab.getty.edu/page/tgn/4005920"/>
	<skos:closeMatch rdf:resource="https://www.wikidata.org/wiki/Q1651504"/>
	<skos:mappingRelation rdf:resource="http://vocab.getty.edu/page/tgn/4005920"/>
	<skos:mappingRelation rdf:resource="https://www.wikidata.org/wiki/Q1651504"/>
	<skos:semanticRelation rdf:resource="http://vocab.getty.edu/page/tgn/4005920"/>
	<skos:semanticRelation rdf:resource="https://www.wikidata.org/wiki/Q1651504"/>
	<skos:altLabel xml:lang="en">Löwenburg</skos:altLabel>
	<skos:prefLabel xml:lang="de">Löwenburg</skos:prefLabel>
</rdf:Description>

<rdf:Description rdf:about="http://academictourism.com/entity/LOC0004.CS.K001">
	<rdf:type rdf:resource="http://www.w3.org/2002/07/owl#NamedIndividual"/>
	<rdf:type rdf:resource="http://www.cidoc-crm.org/cidoc-crm/E1_CRM_Entity"/>
	<rdf:type rdf:resource="http://www.cidoc-crm.org/cidoc-crm/E53_Place"/>
	<cidoc-crm:P157_is_at_rest_relative_to rdf:resource="http://academictourism.com/entity/LOC0004.CS"/>
	<cidoc-crm:P59i_is_located_on_or_within rdf:resource="http://academictourism.com/entity/LOC0004.CS"/>
	<cidoc-crm:P7i_witnessed rdf:resource="http://academictourism.com/entity/BRF0004.RS.RS0003.RS0001"/>
	<rdfs:label>Leeuwenburg chapel</rdfs:label>
</rdf:Description>

<rdf:Description rdf:about="http://academictourism.com/entity/LOC0004.CS.K002">
	<rdf:type rdf:resource="http://www.w3.org/2002/07/owl#NamedIndividual"/>
	<rdf:type rdf:resource="http://www.cidoc-crm.org/cidoc-crm/E1_CRM_Entity"/>
	<rdf:type rdf:resource="http://www.cidoc-crm.org/cidoc-crm/E53_Place"/>
	<cidoc-crm:P157_is_at_rest_relative_to rdf:resource="http://academictourism.com/entity/LOC0004.CS"/>
	<cidoc-crm:P59i_is_located_on_or_within rdf:resource="http://academictourism.com/entity/LOC0004.CS"/>
	<cidoc-crm:P7i_witnessed rdf:resource="http://academictourism.com/entity/BRF0004.RS.RS0003.RS0002"/>
	<rdfs:label>Löwenburg Main Building</rdfs:label>
</rdf:Description>

<rdf:Description rdf:about="http://academictourism.com/entity/LOC0004.CS.K003">
	<rdf:type rdf:resource="http://www.w3.org/2002/07/owl#NamedIndividual"/>
	<rdf:type rdf:resource="http://www.cidoc-crm.org/cidoc-crm/E1_CRM_Entity"/>
	<rdf:type rdf:resource="http://www.cidoc-crm.org/cidoc-crm/E53_Place"/>
	<cidoc-crm:P157_is_at_rest_relative_to rdf:resource="http://academictourism.com/entity/LOC0004.CS"/>
	<cidoc-crm:P59i_is_located_on_or_within rdf:resource="http://academictourism.com/entity/LOC0004.CS"/>
	<cidoc-crm:P7i_witnessed rdf:resource="http://academictourism.com/entity/BRF0004.RS.RS0003.RS0003"/>
	<rdfs:label>Löwenburg Dining Hall</rdfs:label>
</rdf:Description>

<rdf:Description rdf:about="http://academictourism.com/entity/LOC0004.CS.K004">
	<rdf:type rdf:resource="http://www.w3.org/2002/07/owl#NamedIndividual"/>
	<rdf:type rdf:resource="http://www.cidoc-crm.org/cidoc-crm/E1_CRM_Entity"/>
	<rdf:type rdf:resource="http://www.cidoc-crm.org/cidoc-crm/E53_Place"/>
	<cidoc-crm:P157_is_at_rest_relative_to rdf:resource="http://academictourism.com/entity/LOC0004.CS"/>
	<cidoc-crm:P59i_is_located_on_or_within rdf:resource="http://academictourism.com/entity/LOC0004.CS"/>
	<cidoc-crm:P7i_witnessed rdf:resource="http://academictourism.com/entity/BRF0004.RS.RS0003.RS0004"/>
	<rdfs:label>Löwenburg Knights' Hall</rdfs:label>
</rdf:Description>

<rdf:Description rdf:about="http://academictourism.com/entity/LOC0004.CS.K005">
	<rdf:type rdf:resource="http://www.w3.org/2002/07/owl#NamedIndividual"/>
	<rdf:type rdf:resource="http://www.cidoc-crm.org/cidoc-crm/E1_CRM_Entity"/>
	<rdf:type rdf:resource="http://www.cidoc-crm.org/cidoc-crm/E53_Place"/>
	<cidoc-crm:P157_is_at_rest_relative_to rdf:resource="http://academictourism.com/entity/LOC0004.CS"/>
	<cidoc-crm:P59i_is_located_on_or_within rdf:resource="http://academictourism.com/entity/LOC0004.CS"/>
	<cidoc-crm:P7i_witnessed rdf:resource="http://academictourism.com/entity/BRF0004.RS.RS0003.RS0005"/>
	<rdfs:label>Löwenburg Library</rdfs:label>
</rdf:Description>

<rdf:Description rdf:about="http://academictourism.com/entity/LOC0005">
	<rdf:type rdf:resource="http://www.w3.org/2002/07/owl#NamedIndividual"/>
	<rdf:type rdf:resource="http://www.cidoc-crm.org/cidoc-crm/E1_CRM_Entity"/>
	<rdf:type rdf:resource="http://www.cidoc-crm.org/cidoc-crm/E53_Place"/>
	<rdf:type rdf:resource="http://www.w3.org/2004/02/skos/core#Concept"/>
	<cidoc-crm:P7i_witnessed rdf:resource="http://academictourism.com/entity/BRF0004.RS.RS0006.RS0002"/>
	<skos:closeMatch rdf:resource="http://vocab.getty.edu/page/tgn/7133622"/>
	<skos:closeMatch rdf:resource="https://www.wikidata.org/wiki/Q1305418"/>
	<skos:mappingRelation rdf:resource="http://vocab.getty.edu/page/tgn/7133622"/>
	<skos:mappingRelation rdf:resource="https://www.wikidata.org/wiki/Q1305418"/>
	<skos:semanticRelation rdf:resource="http://vocab.getty.edu/page/tgn/7133622"/>
	<skos:semanticRelation rdf:resource="https://www.wikidata.org/wiki/Q1305418"/>
	<skos:altLabel xml:lang="en">Münden</skos:altLabel>
	<skos:prefLabel xml:lang="de">Münden</skos:prefLabel>
</rdf:Description>

<rdf:Description rdf:about="http://academictourism.com/entity/LOC0006">
	<rdf:type rdf:resource="http://www.w3.org/2002/07/owl#NamedIndividual"/>
	<rdf:type rdf:resource="http://www.cidoc-crm.org/cidoc-crm/E1_CRM_Entity"/>
	<rdf:type rdf:resource="http://www.cidoc-crm.org/cidoc-crm/E53_Place"/>
	<rdf:type rdf:resource="http://www.w3.org/2004/02/skos/core#Concept"/>
	<cidoc-crm:P7i_witnessed rdf:resource="http://academictourism.com/entity/BRF0004.RS.RS0006.RS0003"/>
	<skos:closeMatch rdf:resource="http://vocab.getty.edu/page/tgn/1038862"/>
	<skos:closeMatch rdf:resource="https://www.wikidata.org/wiki/Q512225"/>
	<skos:mappingRelation rdf:resource="http://vocab.getty.edu/page/tgn/1038862"/>
	<skos:mappingRelation rdf:resource="https://www.wikidata.org/wiki/Q512225"/>
	<skos:semanticRelation rdf:resource="http://vocab.getty.edu/page/tgn/1038862"/>
	<skos:semanticRelation rdf:resource="https://www.wikidata.org/wiki/Q512225"/>
	<skos:altLabel xml:lang="en">Dransfeld</skos:altLabel>
	<skos:altLabel xml:lang="fr">Dransfeld</skos:altLabel>
	<skos:altLabel xml:lang="nl">Dransfeld</skos:altLabel>
	<skos:prefLabel xml:lang="de">Dransfeld</skos:prefLabel>
</rdf:Description>

<rdf:Description rdf:about="http://academictourism.com/entity/LOC0007">
	<rdf:type rdf:resource="http://www.w3.org/2002/07/owl#NamedIndividual"/>
	<rdf:type rdf:resource="http://www.cidoc-crm.org/cidoc-crm/E18_Physical_Thing"/>
	<rdf:type rdf:resource="http://www.cidoc-crm.org/cidoc-crm/E1_CRM_Entity"/>
	<rdf:type rdf:resource="http://www.cidoc-crm.org/cidoc-crm/E53_Place"/>
	<rdf:type rdf:resource="http://www.cidoc-crm.org/cidoc-crm/E70_Thing"/>
	<rdf:type rdf:resource="http://www.cidoc-crm.org/cidoc-crm/E72_Legal_Object"/>
	<rdf:type rdf:resource="http://www.cidoc-crm.org/cidoc-crm/E77_Persistent_Item"/>
	<rdf:type rdf:resource="http://www.loa-cnr.it/ontologies/DOLCE-Lite#endurant"/>
	<rdf:type rdf:resource="http://www.w3.org/2004/02/skos/core#Concept"/>
	<cidoc-crm:P89_falls_within rdf:resource="http://academictourism.com/entity/LOC0002"/>
	<cidoc-crm:P8i_witnessed rdf:resource="http://academictourism.com/entity/BRF0005.RS"/>
	<skos:closeMatch rdf:resource="https://www.wikidata.org/wiki/Q152838"/>
	<skos:mappingRelation rdf:resource="https://www.wikidata.org/wiki/Q152838"/>
	<skos:semanticRelation rdf:resource="https://www.wikidata.org/wiki/Q152838"/>
	<rdfs:seeAlso rdf:datatype="http://www.w3.org/2001/XMLSchema#anyURI">https://en.wikipedia.org/wiki/University_of_G%C3%B6ttingen</rdfs:seeAlso>
	<rdfs:seeAlso rdf:datatype="http://www.w3.org/2001/XMLSchema#anyURI">https://www.uni-goettingen.de/en/1.html</rdfs:seeAlso>
	<skos:altLabel xml:lang="en">Georg August University of Göttingen</skos:altLabel>
	<skos:altLabel xml:lang="en">University of Göttingen</skos:altLabel>
	<skos:prefLabel xml:lang="de">Georg-August-Universität Göttingen</skos:prefLabel>
</rdf:Description>

<rdf:Description rdf:about="http://academictourism.com/entity/LOC0007.KM001">
	<rdf:type rdf:resource="http://www.w3.org/2002/07/owl#NamedIndividual"/>
	<rdf:type rdf:resource="http://www.cidoc-crm.org/cidoc-crm/E1_CRM_Entity"/>
	<rdf:type rdf:resource="http://www.cidoc-crm.org/cidoc-crm/E53_Place"/>
	<cidoc-crm:P2_has_type rdf:resource="http://vocab.getty.edu/page/aat/300004433"/>
	<cidoc-crm:P7i_witnessed rdf:resource="http://academictourism.com/entity/BRF0005.RS.L0001"/>
	<cidoc-crm:P7i_witnessed rdf:resource="http://academictourism.com/entity/BRF0005.RS.L0002"/>
	<cidoc-crm:P7i_witnessed rdf:resource="http://academictourism.com/entity/BRF0005.RS.L0003"/>
	<cidoc-crm:P7i_witnessed rdf:resource="http://academictourism.com/entity/BRF0005.RS.L0004"/>
	<rdfs:label>University of Göttingen Library</rdfs:label>
</rdf:Description>

<rdf:Description rdf:about="http://academictourism.com/entity/LOC0008">
	<rdf:type rdf:resource="http://www.w3.org/2002/07/owl#NamedIndividual"/>
	<rdf:type rdf:resource="http://www.cidoc-crm.org/cidoc-crm/E1_CRM_Entity"/>
	<rdf:type rdf:resource="http://www.cidoc-crm.org/cidoc-crm/E53_Place"/>
	<cidoc-crm:P2_has_type rdf:resource="http://vocab.getty.edu/page/aat/300007170"/>
	<cidoc-crm:P7i_witnessed rdf:resource="http://academictourism.com/entity/BRF0004.RS.RS0006.RS0004"/>
	<rdfs:label>Knalhutte</rdfs:label>
</rdf:Description>

<rdf:Description rdf:about="http://academictourism.com/entity/MISC0001">
	<rdf:type rdf:resource="http://www.w3.org/2002/07/owl#NamedIndividual"/>
	<rdf:type rdf:resource="http://www.cidoc-crm.org/cidoc-crm/E18_Physical_Thing"/>
	<rdf:type rdf:resource="http://www.cidoc-crm.org/cidoc-crm/E19_Physical_Object"/>
	<rdf:type rdf:resource="http://www.cidoc-crm.org/cidoc-crm/E1_CRM_Entity"/>
	<rdf:type rdf:resource="http://www.cidoc-crm.org/cidoc-crm/E22_Human-Made_Object"/>
	<rdf:type rdf:resource="http://www.cidoc-crm.org/cidoc-crm/E24_Physical_Human-Made_Thing"/>
	<rdf:type rdf:resource="http://www.cidoc-crm.org/cidoc-crm/E70_Thing"/>
	<rdf:type rdf:resource="http://www.cidoc-crm.org/cidoc-crm/E71_Human-Made_Thing"/>
	<rdf:type rdf:resource="http://www.cidoc-crm.org/cidoc-crm/E72_Legal_Object"/>
	<rdf:type rdf:resource="http://www.cidoc-crm.org/cidoc-crm/E77_Persistent_Item"/>
	<rdf:type rdf:resource="http://www.loa-cnr.it/ontologies/DOLCE-Lite#endurant"/>
	<cidoc-crm:P12i_was_present_at rdf:resource="http://academictourism.com/entity/BE.MISC0001"/>
	<cidoc-crm:P12i_was_present_at rdf:resource="http://academictourism.com/entity/BRF0004.RS.RS0001"/>
	<cidoc-crm:P2_has_type rdf:resource="http://vocab.getty.edu/page/aat/300005665"/>
	<cidoc-crm:P92i_was_brought_into_existence_by rdf:resource="http://academictourism.com/entity/BE.MISC0001"/>
	<rdfs:label>Casernes</rdfs:label>
</rdf:Description>

<rdf:Description rdf:about="http://academictourism.com/entity/MISC0002">
	<rdf:type rdf:resource="http://www.w3.org/2002/07/owl#NamedIndividual"/>
	<rdf:type rdf:resource="http://www.cidoc-crm.org/cidoc-crm/E18_Physical_Thing"/>
	<rdf:type rdf:resource="http://www.cidoc-crm.org/cidoc-crm/E19_Physical_Object"/>
	<rdf:type rdf:resource="http://www.cidoc-crm.org/cidoc-crm/E1_CRM_Entity"/>
	<rdf:type rdf:resource="http://www.cidoc-crm.org/cidoc-crm/E22_Human-Made_Object"/>
	<rdf:type rdf:resource="http://www.cidoc-crm.org/cidoc-crm/E24_Physical_Human-Made_Thing"/>
	<rdf:type rdf:resource="http://www.cidoc-crm.org/cidoc-crm/E70_Thing"/>
	<rdf:type rdf:resource="http://www.cidoc-crm.org/cidoc-crm/E71_Human-Made_Thing"/>
	<rdf:type rdf:resource="http://www.cidoc-crm.org/cidoc-crm/E72_Legal_Object"/>
	<rdf:type rdf:resource="http://www.cidoc-crm.org/cidoc-crm/E77_Persistent_Item"/>
	<rdf:type rdf:resource="http://www.loa-cnr.it/ontologies/DOLCE-Lite#endurant"/>
	<cidoc-crm:P12i_was_present_at rdf:resource="http://academictourism.com/entity/BRF0004.RS.RS0002.RS0001"/>
	<cidoc-crm:P2_has_type rdf:resource="http://vocab.getty.edu/page/aat/300037682"/>
	<cidoc-crm:P43_has_dimension rdf:resource="http://academictourism.com/entity/DM.MISC0002"/>
	<cidoc-crm:P53_has_former_or_current_location rdf:resource="http://academictourism.com/entity/LOC0003.CS.K001"/>
	<rdfs:label>Wilhelmshöhe spiegels</rdfs:label>
</rdf:Description>

<rdf:Description rdf:about="http://academictourism.com/entity/MISC0003">
	<rdf:type rdf:resource="http://www.w3.org/2002/07/owl#NamedIndividual"/>
	<rdf:type rdf:resource="http://iflastandards.info/ns/lrm/lrmoo/F2_Expression"/>
	<rdf:type rdf:resource="http://www.cidoc-crm.org/cidoc-crm/E18_Physical_Thing"/>
	<rdf:type rdf:resource="http://www.cidoc-crm.org/cidoc-crm/E1_CRM_Entity"/>
	<rdf:type rdf:resource="http://www.cidoc-crm.org/cidoc-crm/E28_Conceptual_Object"/>
	<rdf:type rdf:resource="http://www.cidoc-crm.org/cidoc-crm/E70_Thing"/>
	<rdf:type rdf:resource="http://www.cidoc-crm.org/cidoc-crm/E71_Human-Made_Thing"/>
	<rdf:type rdf:resource="http://www.cidoc-crm.org/cidoc-crm/E72_Legal_Object"/>
	<rdf:type rdf:resource="http://www.cidoc-crm.org/cidoc-crm/E73_Information_Object"/>
	<rdf:type rdf:resource="http://www.cidoc-crm.org/cidoc-crm/E77_Persistent_Item"/>
	<rdf:type rdf:resource="http://www.cidoc-crm.org/cidoc-crm/E89_Propositional_Object"/>
	<rdf:type rdf:resource="http://www.cidoc-crm.org/cidoc-crm/E90_Symbolic_Object"/>
	<rdf:type rdf:resource="http://www.loa-cnr.it/ontologies/DOLCE-Lite#endurant"/>
	<cidoc-crm:P12i_was_present_at rdf:resource="http://academictourism.com/entity/BE.MISC0003"/>
	<cidoc-crm:P12i_was_present_at rdf:resource="http://academictourism.com/entity/BRF0004.RS.RS0002.RS0004"/>
	<cidoc-crm:P2_has_type rdf:resource="http://vocab.getty.edu/page/aat/300033618"/>
	<cidoc-crm:P53_has_former_or_current_location rdf:resource="http://academictourism.com/entity/LOC0003.CS.K004"/>
	<cidoc-crm:P92i_was_brought_into_existence_by rdf:resource="http://academictourism.com/entity/BE.MISC0003"/>
	<rdfs:label>Wilhelmshöhe schilderyen</rdfs:label>
</rdf:Description>

<rdf:Description rdf:about="http://academictourism.com/entity/MISC0004">
	<rdf:type rdf:resource="http://www.w3.org/2002/07/owl#NamedIndividual"/>
	<rdf:type rdf:resource="http://www.cidoc-crm.org/cidoc-crm/E18_Physical_Thing"/>
	<rdf:type rdf:resource="http://www.cidoc-crm.org/cidoc-crm/E19_Physical_Object"/>
	<rdf:type rdf:resource="http://www.cidoc-crm.org/cidoc-crm/E1_CRM_Entity"/>
	<rdf:type rdf:resource="http://www.cidoc-crm.org/cidoc-crm/E22_Human-Made_Object"/>
	<rdf:type rdf:resource="http://www.cidoc-crm.org/cidoc-crm/E24_Physical_Human-Made_Thing"/>
	<rdf:type rdf:resource="http://www.cidoc-crm.org/cidoc-crm/E70_Thing"/>
	<rdf:type rdf:resource="http://www.cidoc-crm.org/cidoc-crm/E71_Human-Made_Thing"/>
	<rdf:type rdf:resource="http://www.cidoc-crm.org/cidoc-crm/E72_Legal_Object"/>
	<rdf:type rdf:resource="http://www.cidoc-crm.org/cidoc-crm/E77_Persistent_Item"/>
	<rdf:type rdf:resource="http://www.loa-cnr.it/ontologies/DOLCE-Lite#endurant"/>
	<cidoc-crm:P12i_was_present_at rdf:resource="http://academictourism.com/entity/BRF0004.RS.RS0003"/>
	<cidoc-crm:P12i_was_present_at rdf:resource="http://academictourism.com/entity/BRF0004.RS.RS0003.RS0002"/>
	<cidoc-crm:P2_has_type rdf:resource="http://vocab.getty.edu/page/aat/300417950"/>
	<rdfs:label>Stone bust of an armored knight</rdfs:label>
</rdf:Description>

<rdf:Description rdf:about="http://academictourism.com/entity/MISC0005">
	<rdf:type rdf:resource="http://www.w3.org/2002/07/owl#NamedIndividual"/>
	<rdf:type rdf:resource="http://iflastandards.info/ns/lrm/lrmoo/F2_Expression"/>
	<rdf:type rdf:resource="http://www.cidoc-crm.org/cidoc-crm/E1_CRM_Entity"/>
	<rdf:type rdf:resource="http://www.cidoc-crm.org/cidoc-crm/E28_Conceptual_Object"/>
	<rdf:type rdf:resource="http://www.cidoc-crm.org/cidoc-crm/E70_Thing"/>
	<rdf:type rdf:resource="http://www.cidoc-crm.org/cidoc-crm/E71_Human-Made_Thing"/>
	<rdf:type rdf:resource="http://www.cidoc-crm.org/cidoc-crm/E72_Legal_Object"/>
	<rdf:type rdf:resource="http://www.cidoc-crm.org/cidoc-crm/E73_Information_Object"/>
	<rdf:type rdf:resource="http://www.cidoc-crm.org/cidoc-crm/E77_Persistent_Item"/>
	<rdf:type rdf:resource="http://www.cidoc-crm.org/cidoc-crm/E89_Propositional_Object"/>
	<rdf:type rdf:resource="http://www.cidoc-crm.org/cidoc-crm/E90_Symbolic_Object"/>
	<rdf:type rdf:resource="http://www.loa-cnr.it/ontologies/DOLCE-Lite#endurant"/>
	<cidoc-crm:P12i_was_present_at rdf:resource="http://academictourism.com/entity/BRF0004.RS.RS0003"/>
	<cidoc-crm:P12i_was_present_at rdf:resource="http://academictourism.com/entity/BRF0004.RS.RS0003.RS0002"/>
	<cidoc-crm:P2_has_type rdf:resource="http://vocab.getty.edu/page/aat/300205002"/>
	<rdfs:label>Tapestries depicted knightly battles and tournaments</rdfs:label>
</rdf:Description>

<rdf:Description rdf:about="http://academictourism.com/entity/MISC0006">
	<rdf:type rdf:resource="http://www.w3.org/2002/07/owl#NamedIndividual"/>
	<rdf:type rdf:resource="http://iflastandards.info/ns/lrm/lrmoo/F2_Expression"/>
	<rdf:type rdf:resource="http://www.cidoc-crm.org/cidoc-crm/E1_CRM_Entity"/>
	<rdf:type rdf:resource="http://www.cidoc-crm.org/cidoc-crm/E28_Conceptual_Object"/>
	<rdf:type rdf:resource="http://www.cidoc-crm.org/cidoc-crm/E70_Thing"/>
	<rdf:type rdf:resource="http://www.cidoc-crm.org/cidoc-crm/E71_Human-Made_Thing"/>
	<rdf:type rdf:resource="http://www.cidoc-crm.org/cidoc-crm/E72_Legal_Object"/>
	<rdf:type rdf:resource="http://www.cidoc-crm.org/cidoc-crm/E73_Information_Object"/>
	<rdf:type rdf:resource="http://www.cidoc-crm.org/cidoc-crm/E77_Persistent_Item"/>
	<rdf:type rdf:resource="http://www.cidoc-crm.org/cidoc-crm/E89_Propositional_Object"/>
	<rdf:type rdf:resource="http://www.cidoc-crm.org/cidoc-crm/E90_Symbolic_Object"/>
	<rdf:type rdf:resource="http://www.loa-cnr.it/ontologies/DOLCE-Lite#endurant"/>
	<cidoc-crm:P12i_was_present_at rdf:resource="http://academictourism.com/entity/BRF0004.RS.RS0003"/>
	<cidoc-crm:P2_has_type rdf:resource="http://vocab.getty.edu/page/aat/300015637"/>
	<rdfs:label>Portraits of old Hessian princes</rdfs:label>
</rdf:Description>

<rdf:Description rdf:about="http://academictourism.com/entity/MISC0007">
	<rdf:type rdf:resource="http://www.w3.org/2002/07/owl#NamedIndividual"/>
	<rdf:type rdf:resource="http://www.cidoc-crm.org/cidoc-crm/E18_Physical_Thing"/>
	<rdf:type rdf:resource="http://www.cidoc-crm.org/cidoc-crm/E1_CRM_Entity"/>
	<rdf:type rdf:resource="http://www.cidoc-crm.org/cidoc-crm/E70_Thing"/>
	<rdf:type rdf:resource="http://www.cidoc-crm.org/cidoc-crm/E72_Legal_Object"/>
	<rdf:type rdf:resource="http://www.cidoc-crm.org/cidoc-crm/E77_Persistent_Item"/>
	<rdf:type rdf:resource="http://www.loa-cnr.it/ontologies/DOLCE-Lite#endurant"/>
	<cidoc-crm:P12i_was_present_at rdf:resource="http://academictourism.com/entity/BRF0004.RS.RS0004.RS0002"/>
	<cidoc-crm:P2_has_type rdf:resource="http://vocab.getty.edu/page/aat/300387598"/>
	<rdfs:label>Havikswoud</rdfs:label>
</rdf:Description>

<rdf:Description rdf:about="http://academictourism.com/entity/MISC0008">
	<rdf:type rdf:resource="http://www.w3.org/2002/07/owl#NamedIndividual"/>
	<rdf:type rdf:resource="http://www.cidoc-crm.org/cidoc-crm/E18_Physical_Thing"/>
	<rdf:type rdf:resource="http://www.cidoc-crm.org/cidoc-crm/E1_CRM_Entity"/>
	<rdf:type rdf:resource="http://www.cidoc-crm.org/cidoc-crm/E70_Thing"/>
	<rdf:type rdf:resource="http://www.cidoc-crm.org/cidoc-crm/E72_Legal_Object"/>
	<rdf:type rdf:resource="http://www.cidoc-crm.org/cidoc-crm/E77_Persistent_Item"/>
	<rdf:type rdf:resource="http://www.loa-cnr.it/ontologies/DOLCE-Lite#endurant"/>
	<cidoc-crm:P12i_was_present_at rdf:resource="http://academictourism.com/entity/BRF0004.RS.RS0004.RS0002"/>
	<cidoc-crm:P2_has_type rdf:resource="http://vocab.getty.edu/page/aat/300006215"/>
	<rdfs:label>waterwerk</rdfs:label>
</rdf:Description>

<rdf:Description rdf:about="http://academictourism.com/entity/MISC0009">
	<rdf:type rdf:resource="http://www.w3.org/2002/07/owl#NamedIndividual"/>
	<rdf:type rdf:resource="http://www.cidoc-crm.org/cidoc-crm/E18_Physical_Thing"/>
	<rdf:type rdf:resource="http://www.cidoc-crm.org/cidoc-crm/E1_CRM_Entity"/>
	<rdf:type rdf:resource="http://www.cidoc-crm.org/cidoc-crm/E70_Thing"/>
	<rdf:type rdf:resource="http://www.cidoc-crm.org/cidoc-crm/E72_Legal_Object"/>
	<rdf:type rdf:resource="http://www.cidoc-crm.org/cidoc-crm/E77_Persistent_Item"/>
	<rdf:type rdf:resource="http://www.loa-cnr.it/ontologies/DOLCE-Lite#endurant"/>
	<cidoc-crm:P12i_was_present_at rdf:resource="http://academictourism.com/entity/BE.MISC0009"/>
	<cidoc-crm:P12i_was_present_at rdf:resource="http://academictourism.com/entity/BRF0004.RS.RS0004.RS0002"/>
	<cidoc-crm:P92i_was_brought_into_existence_by rdf:resource="http://academictourism.com/entity/BE.MISC0009"/>
	<rdfs:label>Hercules Monument</rdfs:label>
</rdf:Description>

<rdf:Description rdf:about="http://academictourism.com/entity/MISC0010">
	<rdf:type rdf:resource="http://www.w3.org/2002/07/owl#NamedIndividual"/>
	<rdf:type rdf:resource="http://www.cidoc-crm.org/cidoc-crm/E18_Physical_Thing"/>
	<rdf:type rdf:resource="http://www.cidoc-crm.org/cidoc-crm/E19_Physical_Object"/>
	<rdf:type rdf:resource="http://www.cidoc-crm.org/cidoc-crm/E1_CRM_Entity"/>
	<rdf:type rdf:resource="http://www.cidoc-crm.org/cidoc-crm/E22_Human-Made_Object"/>
	<rdf:type rdf:resource="http://www.cidoc-crm.org/cidoc-crm/E24_Physical_Human-Made_Thing"/>
	<rdf:type rdf:resource="http://www.cidoc-crm.org/cidoc-crm/E70_Thing"/>
	<rdf:type rdf:resource="http://www.cidoc-crm.org/cidoc-crm/E71_Human-Made_Thing"/>
	<rdf:type rdf:resource="http://www.cidoc-crm.org/cidoc-crm/E72_Legal_Object"/>
	<rdf:type rdf:resource="http://www.cidoc-crm.org/cidoc-crm/E77_Persistent_Item"/>
	<rdf:type rdf:resource="http://www.loa-cnr.it/ontologies/DOLCE-Lite#endurant"/>
	<cidoc-crm:P12i_was_present_at rdf:resource="http://academictourism.com/entity/BRF0004.RS.RS0004.RS0004"/>
	<cidoc-crm:P2_has_type rdf:resource="http://vocab.getty.edu/page/aat/300006179"/>
	<rdfs:label>fonteyn</rdfs:label>
</rdf:Description>

<rdf:Description rdf:about="http://academictourism.com/entity/MISC0011">
	<rdf:type rdf:resource="http://www.w3.org/2002/07/owl#NamedIndividual"/>
	<rdf:type rdf:resource="http://www.cidoc-crm.org/cidoc-crm/E18_Physical_Thing"/>
	<rdf:type rdf:resource="http://www.cidoc-crm.org/cidoc-crm/E19_Physical_Object"/>
	<rdf:type rdf:resource="http://www.cidoc-crm.org/cidoc-crm/E1_CRM_Entity"/>
	<rdf:type rdf:resource="http://www.cidoc-crm.org/cidoc-crm/E22_Human-Made_Object"/>
	<rdf:type rdf:resource="http://www.cidoc-crm.org/cidoc-crm/E24_Physical_Human-Made_Thing"/>
	<rdf:type rdf:resource="http://www.cidoc-crm.org/cidoc-crm/E70_Thing"/>
	<rdf:type rdf:resource="http://www.cidoc-crm.org/cidoc-crm/E71_Human-Made_Thing"/>
	<rdf:type rdf:resource="http://www.cidoc-crm.org/cidoc-crm/E72_Legal_Object"/>
	<rdf:type rdf:resource="http://www.cidoc-crm.org/cidoc-crm/E77_Persistent_Item"/>
	<rdf:type rdf:resource="http://www.loa-cnr.it/ontologies/DOLCE-Lite#endurant"/>
	<cidoc-crm:P12i_was_present_at rdf:resource="http://academictourism.com/entity/BRF0004.RS.RS0004.RS0004"/>
	<rdfs:label>waterorgel</rdfs:label>
</rdf:Description>

<rdf:Description rdf:about="http://academictourism.com/entity/MISC0012">
	<rdf:type rdf:resource="http://www.w3.org/2002/07/owl#NamedIndividual"/>
	<rdf:type rdf:resource="http://www.cidoc-crm.org/cidoc-crm/E18_Physical_Thing"/>
	<rdf:type rdf:resource="http://www.cidoc-crm.org/cidoc-crm/E19_Physical_Object"/>
	<rdf:type rdf:resource="http://www.cidoc-crm.org/cidoc-crm/E1_CRM_Entity"/>
	<rdf:type rdf:resource="http://www.cidoc-crm.org/cidoc-crm/E22_Human-Made_Object"/>
	<rdf:type rdf:resource="http://www.cidoc-crm.org/cidoc-crm/E24_Physical_Human-Made_Thing"/>
	<rdf:type rdf:resource="http://www.cidoc-crm.org/cidoc-crm/E70_Thing"/>
	<rdf:type rdf:resource="http://www.cidoc-crm.org/cidoc-crm/E71_Human-Made_Thing"/>
	<rdf:type rdf:resource="http://www.cidoc-crm.org/cidoc-crm/E72_Legal_Object"/>
	<rdf:type rdf:resource="http://www.cidoc-crm.org/cidoc-crm/E77_Persistent_Item"/>
	<rdf:type rdf:resource="http://www.loa-cnr.it/ontologies/DOLCE-Lite#endurant"/>
	<cidoc-crm:P12i_was_present_at rdf:resource="http://academictourism.com/entity/BRF0004.RS.RS0004.RS0004"/>
	<cidoc-crm:P2_has_type rdf:resource="http://vocab.getty.edu/page/aat/300006792"/>
	<rdfs:label>waterval</rdfs:label>
</rdf:Description>

<rdf:Description rdf:about="http://academictourism.com/entity/MISC0013">
	<rdf:type rdf:resource="http://www.w3.org/2002/07/owl#NamedIndividual"/>
	<rdf:type rdf:resource="http://www.cidoc-crm.org/cidoc-crm/E18_Physical_Thing"/>
	<rdf:type rdf:resource="http://www.cidoc-crm.org/cidoc-crm/E1_CRM_Entity"/>
	<rdf:type rdf:resource="http://www.cidoc-crm.org/cidoc-crm/E70_Thing"/>
	<rdf:type rdf:resource="http://www.cidoc-crm.org/cidoc-crm/E72_Legal_Object"/>
	<rdf:type rdf:resource="http://www.cidoc-crm.org/cidoc-crm/E77_Persistent_Item"/>
	<rdf:type rdf:resource="http://www.loa-cnr.it/ontologies/DOLCE-Lite#endurant"/>
	<cidoc-crm:P12i_was_present_at rdf:resource="http://academictourism.com/entity/BRF0004.RS.RS0004.RS0004"/>
	<cidoc-crm:P2_has_type rdf:resource="http://vocab.getty.edu/page/aat/300007117"/>
	<rdfs:label>Schouwburg</rdfs:label>
</rdf:Description>

<rdf:Description rdf:about="http://academictourism.com/entity/MISC0014">
	<rdf:type rdf:resource="http://www.w3.org/2002/07/owl#NamedIndividual"/>
	<rdf:type rdf:resource="http://www.cidoc-crm.org/cidoc-crm/E18_Physical_Thing"/>
	<rdf:type rdf:resource="http://www.cidoc-crm.org/cidoc-crm/E1_CRM_Entity"/>
	<rdf:type rdf:resource="http://www.cidoc-crm.org/cidoc-crm/E70_Thing"/>
	<rdf:type rdf:resource="http://www.cidoc-crm.org/cidoc-crm/E72_Legal_Object"/>
	<rdf:type rdf:resource="http://www.cidoc-crm.org/cidoc-crm/E77_Persistent_Item"/>
	<rdf:type rdf:resource="http://www.loa-cnr.it/ontologies/DOLCE-Lite#endurant"/>
	<cidoc-crm:P12i_was_present_at rdf:resource="http://academictourism.com/entity/BRF0004.RS.RS0004.RS0004"/>
	<cidoc-crm:P2_has_type rdf:resource="http://vocab.getty.edu/page/aat/300005907"/>
	<rdfs:label>graf van Vergilius</rdfs:label>
</rdf:Description>

<rdf:Description rdf:about="http://academictourism.com/entity/MISC0015">
	<rdf:type rdf:resource="http://www.w3.org/2002/07/owl#NamedIndividual"/>
	<rdf:type rdf:resource="http://www.cidoc-crm.org/cidoc-crm/E18_Physical_Thing"/>
	<rdf:type rdf:resource="http://www.cidoc-crm.org/cidoc-crm/E1_CRM_Entity"/>
	<rdf:type rdf:resource="http://www.cidoc-crm.org/cidoc-crm/E70_Thing"/>
	<rdf:type rdf:resource="http://www.cidoc-crm.org/cidoc-crm/E72_Legal_Object"/>
	<rdf:type rdf:resource="http://www.cidoc-crm.org/cidoc-crm/E77_Persistent_Item"/>
	<rdf:type rdf:resource="http://www.loa-cnr.it/ontologies/DOLCE-Lite#endurant"/>
	<cidoc-crm:P12i_was_present_at rdf:resource="http://academictourism.com/entity/BRF0004.RS.RS0004.RS0004"/>
	<cidoc-crm:P2_has_type rdf:resource="http://vocab.getty.edu/page/aat/300007595"/>
	<rdfs:label>tempel van Apollo</rdfs:label>
</rdf:Description>

<rdf:Description rdf:about="http://academictourism.com/entity/MISC0016">
	<rdf:type rdf:resource="http://www.w3.org/2002/07/owl#NamedIndividual"/>
	<rdf:type rdf:resource="http://www.cidoc-crm.org/cidoc-crm/E18_Physical_Thing"/>
	<rdf:type rdf:resource="http://www.cidoc-crm.org/cidoc-crm/E1_CRM_Entity"/>
	<rdf:type rdf:resource="http://www.cidoc-crm.org/cidoc-crm/E70_Thing"/>
	<rdf:type rdf:resource="http://www.cidoc-crm.org/cidoc-crm/E72_Legal_Object"/>
	<rdf:type rdf:resource="http://www.cidoc-crm.org/cidoc-crm/E77_Persistent_Item"/>
	<rdf:type rdf:resource="http://www.loa-cnr.it/ontologies/DOLCE-Lite#endurant"/>
	<cidoc-crm:P12i_was_present_at rdf:resource="http://academictourism.com/entity/BRF0004.RS.RS0004.RS0004"/>
	<cidoc-crm:P2_has_type rdf:resource="http://vocab.getty.edu/page/aat/300007595"/>
	<rdfs:label>tempel van Mercurius</rdfs:label>
</rdf:Description>

<rdf:Description rdf:about="http://academictourism.com/entity/MISC0017">
	<rdf:type rdf:resource="http://www.w3.org/2002/07/owl#NamedIndividual"/>
	<rdf:type rdf:resource="http://www.cidoc-crm.org/cidoc-crm/E18_Physical_Thing"/>
	<rdf:type rdf:resource="http://www.cidoc-crm.org/cidoc-crm/E1_CRM_Entity"/>
	<rdf:type rdf:resource="http://www.cidoc-crm.org/cidoc-crm/E70_Thing"/>
	<rdf:type rdf:resource="http://www.cidoc-crm.org/cidoc-crm/E72_Legal_Object"/>
	<rdf:type rdf:resource="http://www.cidoc-crm.org/cidoc-crm/E77_Persistent_Item"/>
	<rdf:type rdf:resource="http://www.loa-cnr.it/ontologies/DOLCE-Lite#endurant"/>
	<cidoc-crm:P12i_was_present_at rdf:resource="http://academictourism.com/entity/BRF0004.RS.RS0004.RS0004"/>
	<cidoc-crm:P2_has_type rdf:resource="http://vocab.getty.edu/page/aat/300008746"/>
	<rdfs:label>grot van Pluto</rdfs:label>
</rdf:Description>

<rdf:Description rdf:about="http://academictourism.com/entity/MISC0018">
	<rdf:type rdf:resource="http://www.w3.org/2002/07/owl#NamedIndividual"/>
	<rdf:type rdf:resource="http://iflastandards.info/ns/lrm/lrmoo/F2_Expression"/>
	<rdf:type rdf:resource="http://www.cidoc-crm.org/cidoc-crm/E1_CRM_Entity"/>
	<rdf:type rdf:resource="http://www.cidoc-crm.org/cidoc-crm/E28_Conceptual_Object"/>
	<rdf:type rdf:resource="http://www.cidoc-crm.org/cidoc-crm/E70_Thing"/>
	<rdf:type rdf:resource="http://www.cidoc-crm.org/cidoc-crm/E71_Human-Made_Thing"/>
	<rdf:type rdf:resource="http://www.cidoc-crm.org/cidoc-crm/E72_Legal_Object"/>
	<rdf:type rdf:resource="http://www.cidoc-crm.org/cidoc-crm/E73_Information_Object"/>
	<rdf:type rdf:resource="http://www.cidoc-crm.org/cidoc-crm/E77_Persistent_Item"/>
	<rdf:type rdf:resource="http://www.cidoc-crm.org/cidoc-crm/E89_Propositional_Object"/>
	<rdf:type rdf:resource="http://www.cidoc-crm.org/cidoc-crm/E90_Symbolic_Object"/>
	<rdf:type rdf:resource="http://www.loa-cnr.it/ontologies/DOLCE-Lite#endurant"/>
	<cidoc-crm:P12i_was_present_at rdf:resource="http://academictourism.com/entity/BE.MISC0018"/>
	<cidoc-crm:P15i_influenced rdf:resource="http://academictourism.com/entity/BE.MISC0003"/>
	<cidoc-crm:P92i_was_brought_into_existence_by rdf:resource="http://academictourism.com/entity/BE.MISC0018"/>
	<terms:title>Oberon</terms:title>
	<rdfs:label>Oberon</rdfs:label>
	<rdfs:seeAlso rdf:datatype="http://www.w3.org/2001/XMLSchema#anyURI">https://en.wikipedia.org/wiki/Oberon_(poem)</rdfs:seeAlso>
</rdf:Description>

<rdf:Description rdf:about="http://academictourism.com/entity/MISC0019">
	<rdf:type rdf:resource="http://www.w3.org/2002/07/owl#NamedIndividual"/>
	<rdf:type rdf:resource="http://www.cidoc-crm.org/cidoc-crm/E18_Physical_Thing"/>
	<rdf:type rdf:resource="http://www.cidoc-crm.org/cidoc-crm/E19_Physical_Object"/>
	<rdf:type rdf:resource="http://www.cidoc-crm.org/cidoc-crm/E1_CRM_Entity"/>
	<rdf:type rdf:resource="http://www.cidoc-crm.org/cidoc-crm/E22_Human-Made_Object"/>
	<rdf:type rdf:resource="http://www.cidoc-crm.org/cidoc-crm/E24_Physical_Human-Made_Thing"/>
	<rdf:type rdf:resource="http://www.cidoc-crm.org/cidoc-crm/E70_Thing"/>
	<rdf:type rdf:resource="http://www.cidoc-crm.org/cidoc-crm/E71_Human-Made_Thing"/>
	<rdf:type rdf:resource="http://www.cidoc-crm.org/cidoc-crm/E72_Legal_Object"/>
	<rdf:type rdf:resource="http://www.cidoc-crm.org/cidoc-crm/E77_Persistent_Item"/>
	<rdf:type rdf:resource="http://www.loa-cnr.it/ontologies/DOLCE-Lite#endurant"/>
	<rdf:type rdf:resource="http://www.w3.org/2004/02/skos/core#Concept"/>
	<cidoc-crm:P12i_was_present_at rdf:resource="http://academictourism.com/entity/BE.MISC0019"/>
	<cidoc-crm:P12i_was_present_at rdf:resource="http://academictourism.com/entity/BRF0004.RS.RS0004.RS0001"/>
	<cidoc-crm:P92i_was_brought_into_existence_by rdf:resource="http://academictourism.com/entity/BE.MISC0019"/>
	<skos:closeMatch rdf:resource="https://www.wikidata.org/wiki/Q1501427"/>
	<skos:mappingRelation rdf:resource="https://www.wikidata.org/wiki/Q1501427"/>
	<skos:semanticRelation rdf:resource="https://www.wikidata.org/wiki/Q1501427"/>
	<rdfs:label>Octogoon</rdfs:label>
</rdf:Description>

<rdf:Description rdf:about="http://academictourism.com/entity/MISC0020">
	<rdf:type rdf:resource="http://www.w3.org/2002/07/owl#NamedIndividual"/>
	<rdf:type rdf:resource="http://iflastandards.info/ns/lrm/lrmoo/F2_Expression"/>
	<rdf:type rdf:resource="http://www.cidoc-crm.org/cidoc-crm/E1_CRM_Entity"/>
	<rdf:type rdf:resource="http://www.cidoc-crm.org/cidoc-crm/E28_Conceptual_Object"/>
	<rdf:type rdf:resource="http://www.cidoc-crm.org/cidoc-crm/E70_Thing"/>
	<rdf:type rdf:resource="http://www.cidoc-crm.org/cidoc-crm/E71_Human-Made_Thing"/>
	<rdf:type rdf:resource="http://www.cidoc-crm.org/cidoc-crm/E72_Legal_Object"/>
	<rdf:type rdf:resource="http://www.cidoc-crm.org/cidoc-crm/E73_Information_Object"/>
	<rdf:type rdf:resource="http://www.cidoc-crm.org/cidoc-crm/E77_Persistent_Item"/>
	<rdf:type rdf:resource="http://www.cidoc-crm.org/cidoc-crm/E89_Propositional_Object"/>
	<rdf:type rdf:resource="http://www.cidoc-crm.org/cidoc-crm/E90_Symbolic_Object"/>
	<rdf:type rdf:resource="http://www.loa-cnr.it/ontologies/DOLCE-Lite#endurant"/>
	<rdf:type rdf:resource="http://www.w3.org/2004/02/skos/core#Concept"/>
	<cidoc-crm:P129_is_about rdf:resource="http://academictourism.com/entity/MISC0020"/>
	<cidoc-crm:P129i_is_subject_of rdf:resource="http://academictourism.com/entity/MISC0020"/>
	<cidoc-crm:P67_refers_to rdf:resource="http://academictourism.com/entity/MISC0020"/>
	<cidoc-crm:P67i_is_referred_to_by rdf:resource="http://academictourism.com/entity/MISC0020"/>
	<skos:closeMatch rdf:resource="https://www.wikidata.org/wiki/Q838526"/>
	<skos:mappingRelation rdf:resource="https://www.wikidata.org/wiki/Q838526"/>
	<skos:semanticRelation rdf:resource="https://www.wikidata.org/wiki/Q838526"/>
	<terms:title>Pandecten</terms:title>
	<rdfs:label>Pandecten</rdfs:label>
	<rdfs:seeAlso rdf:datatype="http://www.w3.org/2001/XMLSchema#anyURI">https://en.wikipedia.org/wiki/Digest_(Roman_law)</rdfs:seeAlso>
</rdf:Description>

<rdf:Description rdf:about="http://academictourism.com/entity/MISC0021">
	<rdf:type rdf:resource="http://www.w3.org/2002/07/owl#NamedIndividual"/>
	<rdf:type rdf:resource="http://iflastandards.info/ns/lrm/lrmoo/F2_Expression"/>
	<rdf:type rdf:resource="http://www.cidoc-crm.org/cidoc-crm/E1_CRM_Entity"/>
	<rdf:type rdf:resource="http://www.cidoc-crm.org/cidoc-crm/E28_Conceptual_Object"/>
	<rdf:type rdf:resource="http://www.cidoc-crm.org/cidoc-crm/E70_Thing"/>
	<rdf:type rdf:resource="http://www.cidoc-crm.org/cidoc-crm/E71_Human-Made_Thing"/>
	<rdf:type rdf:resource="http://www.cidoc-crm.org/cidoc-crm/E72_Legal_Object"/>
	<rdf:type rdf:resource="http://www.cidoc-crm.org/cidoc-crm/E73_Information_Object"/>
	<rdf:type rdf:resource="http://www.cidoc-crm.org/cidoc-crm/E77_Persistent_Item"/>
	<rdf:type rdf:resource="http://www.cidoc-crm.org/cidoc-crm/E89_Propositional_Object"/>
	<rdf:type rdf:resource="http://www.cidoc-crm.org/cidoc-crm/E90_Symbolic_Object"/>
	<rdf:type rdf:resource="http://www.loa-cnr.it/ontologies/DOLCE-Lite#endurant"/>
	<rdf:type rdf:resource="http://www.w3.org/2004/02/skos/core#Concept"/>
	<cidoc-crm:P12i_was_present_at rdf:resource="http://academictourism.com/entity/BE.MISC0021"/>
	<cidoc-crm:P15i_influenced rdf:resource="http://academictourism.com/entity/BE.MISC0003"/>
	<cidoc-crm:P92i_was_brought_into_existence_by rdf:resource="http://academictourism.com/entity/BE.MISC0021"/>
	<skos:closeMatch rdf:resource="http://academictourism.com/entity/MISC0021"/>
	<skos:closeMatch rdf:resource="https://www.wikidata.org/wiki/Q1053313"/>
	<skos:exactMatch rdf:resource="http://academictourism.com/entity/MISC0021"/>
	<skos:exactMatch rdf:resource="https://www.wikidata.org/wiki/Q1053313"/>
	<skos:mappingRelation rdf:resource="http://academictourism.com/entity/MISC0021"/>
	<skos:mappingRelation rdf:resource="https://www.wikidata.org/wiki/Q1053313"/>
	<skos:semanticRelation rdf:resource="http://academictourism.com/entity/MISC0021"/>
	<skos:semanticRelation rdf:resource="https://www.wikidata.org/wiki/Q1053313"/>
	<terms:title>La Gerusalemme liberata</terms:title>
	<rdfs:label>La Gerusalemme liberata</rdfs:label>
	<rdfs:seeAlso rdf:datatype="http://www.w3.org/2001/XMLSchema#anyURI">https://en.wikipedia.org/wiki/Jerusalem_Delivered</rdfs:seeAlso>
</rdf:Description>

<rdf:Description rdf:about="http://academictourism.com/entity/MISC0022">
	<rdf:type rdf:resource="http://www.w3.org/2002/07/owl#NamedIndividual"/>
	<rdf:type rdf:resource="http://iflastandards.info/ns/lrm/lrmoo/F3_Manifestation"/>
	<rdf:type rdf:resource="http://www.cidoc-crm.org/cidoc-crm/E1_CRM_Entity"/>
	<rdf:type rdf:resource="http://www.cidoc-crm.org/cidoc-crm/E28_Conceptual_Object"/>
	<rdf:type rdf:resource="http://www.cidoc-crm.org/cidoc-crm/E31_Document"/>
	<rdf:type rdf:resource="http://www.cidoc-crm.org/cidoc-crm/E70_Thing"/>
	<rdf:type rdf:resource="http://www.cidoc-crm.org/cidoc-crm/E71_Human-Made_Thing"/>
	<rdf:type rdf:resource="http://www.cidoc-crm.org/cidoc-crm/E72_Legal_Object"/>
	<rdf:type rdf:resource="http://www.cidoc-crm.org/cidoc-crm/E73_Information_Object"/>
	<rdf:type rdf:resource="http://www.cidoc-crm.org/cidoc-crm/E77_Persistent_Item"/>
	<rdf:type rdf:resource="http://www.cidoc-crm.org/cidoc-crm/E89_Propositional_Object"/>
	<rdf:type rdf:resource="http://www.cidoc-crm.org/cidoc-crm/E90_Symbolic_Object"/>
	<rdf:type rdf:resource="http://www.loa-cnr.it/ontologies/DOLCE-Lite#endurant"/>
	<cidoc-crm:P12i_was_present_at rdf:resource="http://academictourism.com/entity/BE.MISC0022"/>
	<cidoc-crm:P67_refers_to rdf:resource="http://academictourism.com/entity/BE.MISC0003"/>
	<cidoc-crm:P70_documents rdf:resource="http://academictourism.com/entity/BE.MISC0003"/>
	<cidoc-crm:P92i_was_brought_into_existence_by rdf:resource="http://academictourism.com/entity/BE.MISC0022"/>
	<terms:title>beschreibung des Kurfürstlichen Landsitzes Wilhelmshöhe bey Cassel</terms:title>
	<rdfs:label>beschreibung des Kurfürstlichen Landsitzes Wilhelmshöhe bey Cassel</rdfs:label>
</rdf:Description>

<rdf:Description rdf:about="http://academictourism.com/entity/MISC0023">
	<rdf:type rdf:resource="http://www.w3.org/2002/07/owl#NamedIndividual"/>
	<rdf:type rdf:resource="http://www.cidoc-crm.org/cidoc-crm/E18_Physical_Thing"/>
	<rdf:type rdf:resource="http://www.cidoc-crm.org/cidoc-crm/E1_CRM_Entity"/>
	<rdf:type rdf:resource="http://www.cidoc-crm.org/cidoc-crm/E70_Thing"/>
	<rdf:type rdf:resource="http://www.cidoc-crm.org/cidoc-crm/E72_Legal_Object"/>
	<rdf:type rdf:resource="http://www.cidoc-crm.org/cidoc-crm/E77_Persistent_Item"/>
	<rdf:type rdf:resource="http://www.loa-cnr.it/ontologies/DOLCE-Lite#endurant"/>
	<cidoc-crm:P12i_was_present_at rdf:resource="http://academictourism.com/entity/BRF0004.RS.RS0004.RS0004"/>
	<cidoc-crm:P2_has_type rdf:resource="http://vocab.getty.edu/page/aat/300000348"/>
	<rdfs:label>dierentuin</rdfs:label>
</rdf:Description>

<rdf:Description rdf:about="http://academictourism.com/entity/PER0001">
	<rdf:type rdf:resource="http://www.w3.org/2002/07/owl#NamedIndividual"/>
	<rdf:type rdf:resource="http://www.cidoc-crm.org/cidoc-crm/E18_Physical_Thing"/>
	<rdf:type rdf:resource="http://www.cidoc-crm.org/cidoc-crm/E19_Physical_Object"/>
	<rdf:type rdf:resource="http://www.cidoc-crm.org/cidoc-crm/E1_CRM_Entity"/>
	<rdf:type rdf:resource="http://www.cidoc-crm.org/cidoc-crm/E20_Biological_Object"/>
	<rdf:type rdf:resource="http://www.cidoc-crm.org/cidoc-crm/E21_Person"/>
	<rdf:type rdf:resource="http://www.cidoc-crm.org/cidoc-crm/E39_Actor"/>
	<rdf:type rdf:resource="http://www.cidoc-crm.org/cidoc-crm/E70_Thing"/>
	<rdf:type rdf:resource="http://www.cidoc-crm.org/cidoc-crm/E72_Legal_Object"/>
	<rdf:type rdf:resource="http://www.cidoc-crm.org/cidoc-crm/E77_Persistent_Item"/>
	<rdf:type rdf:resource="http://www.loa-cnr.it/ontologies/DOLCE-Lite#endurant"/>
	<cidoc-crm:P107i_is_current_or_former_member_of rdf:resource="http://academictourism.com/entity/TG"/>
	<cidoc-crm:P11i_participated_in rdf:resource="http://academictourism.com/entity/BRF0004.SCH"/>
	<cidoc-crm:P11i_participated_in rdf:resource="http://academictourism.com/entity/BRF0005.SCH"/>
	<cidoc-crm:P11i_participated_in rdf:resource="http://academictourism.com/entity/J0002"/>
	<cidoc-crm:P11i_participated_in rdf:resource="http://academictourism.com/entity/L0002"/>
	<cidoc-crm:P12i_was_present_at rdf:resource="http://academictourism.com/entity/BRF0004.SCH"/>
	<cidoc-crm:P12i_was_present_at rdf:resource="http://academictourism.com/entity/BRF0005.SCH"/>
	<cidoc-crm:P12i_was_present_at rdf:resource="http://academictourism.com/entity/J0002"/>
	<cidoc-crm:P12i_was_present_at rdf:resource="http://academictourism.com/entity/L0002"/>
	<cidoc-crm:P143i_was_joined_by rdf:resource="http://academictourism.com/entity/J0002"/>
	<cidoc-crm:P145i_left_by rdf:resource="http://academictourism.com/entity/L0002"/>
	<cidoc-crm:P14i_performed rdf:resource="http://academictourism.com/entity/BRF0004.SCH"/>
	<cidoc-crm:P14i_performed rdf:resource="http://academictourism.com/entity/BRF0005.SCH"/>
	<cidoc-crm:P2_has_type rdf:resource="http://vocab.getty.edu/page/aat/300025492"/>
	<cidoc-crm:P2_has_type rdf:resource="http://vocab.getty.edu/page/aat/300025879"/>
	<DnS:nvolved-in rdf:resource="http://academictourism.com/entity/ocative_relation1"/>
	<rdfs:comment>We bezitten drie verslagen van de reizen, geschreven in de vorm van brieven gericht aan fictieve ontvangers. Die van de reis van 1809 werd gedrukt: Brieven, geschreven op eene wandeling door een gedeelte van Duitschland en Holland, in den zomer van 1809 (2 delen; Groningen 1809-1810). Auteurs waren Barthold Henrik Lulofs (1787-1849), Theodorus van Swinderen (1784-1852) en Jan Jacob Modderman (1786-1809). Lulofs en Van Swinderen waren in 1809 nog student, maar zouden kort nadien hoogleraar worden: de eerste in de Nederlandse Letterkunde en Welsprekendheid (in 1815), de tweede in de Natuurlijke Historie (in 1814). Ze groeiden uit tot coryfeeën van de Groningse academie. Bij de verslagen van de reizen van 1816 en 1819 gaat het om handschriften. Dat van 1816 is van de hand van Reneke de Marees van Swinderen (1796-1828) en bevindt zich in de Groninger Archieven. Dat van 1819 werd geschreven door Ulrich Herman Wielinga Huber (1792-1871) en wordt bewaard in Treseor in Leeuwarden. De reis van 1816 stond onder leiding van eerdergenoemde Theodorus van Swinderen, een neef van Reneke de Marees van Swinderen. De drie reizen overlappen elkaar in hoge mate wat betreft route, bezochte plaatsen en activiteiten. De reizigers in 1816 gebruikten het gedrukte verslag van de reis van 1809 zelfs als reisgids.</rdfs:comment>
	<skos:prefLabel>Narrator of the travelogue</skos:prefLabel>
</rdf:Description>

<rdf:Description rdf:about="http://academictourism.com/entity/PER0002">
	<rdf:type rdf:resource="http://www.w3.org/2002/07/owl#NamedIndividual"/>
	<rdf:type rdf:resource="http://www.cidoc-crm.org/cidoc-crm/E18_Physical_Thing"/>
	<rdf:type rdf:resource="http://www.cidoc-crm.org/cidoc-crm/E19_Physical_Object"/>
	<rdf:type rdf:resource="http://www.cidoc-crm.org/cidoc-crm/E1_CRM_Entity"/>
	<rdf:type rdf:resource="http://www.cidoc-crm.org/cidoc-crm/E20_Biological_Object"/>
	<rdf:type rdf:resource="http://www.cidoc-crm.org/cidoc-crm/E21_Person"/>
	<rdf:type rdf:resource="http://www.cidoc-crm.org/cidoc-crm/E39_Actor"/>
	<rdf:type rdf:resource="http://www.cidoc-crm.org/cidoc-crm/E70_Thing"/>
	<rdf:type rdf:resource="http://www.cidoc-crm.org/cidoc-crm/E72_Legal_Object"/>
	<rdf:type rdf:resource="http://www.cidoc-crm.org/cidoc-crm/E77_Persistent_Item"/>
	<rdf:type rdf:resource="http://www.loa-cnr.it/ontologies/DOLCE-Lite#endurant"/>
	<cidoc-crm:P107i_is_current_or_former_member_of rdf:resource="http://academictourism.com/entity/TG"/>
	<cidoc-crm:P11i_participated_in rdf:resource="http://academictourism.com/entity/J0001"/>
	<cidoc-crm:P11i_participated_in rdf:resource="http://academictourism.com/entity/L0002"/>
	<cidoc-crm:P12i_was_present_at rdf:resource="http://academictourism.com/entity/J0001"/>
	<cidoc-crm:P12i_was_present_at rdf:resource="http://academictourism.com/entity/L0002"/>
	<cidoc-crm:P145i_left_by rdf:resource="http://academictourism.com/entity/L0002"/>
	<cidoc-crm:P2_has_type rdf:resource="http://vocab.getty.edu/page/aat/300025879"/>
	<cidoc-crm:P2_has_type rdf:resource="http://vocab.getty.edu/page/aat/300025909"/>
	<skos:prefLabel>Hogendorp</skos:prefLabel>
</rdf:Description>

<rdf:Description rdf:about="http://academictourism.com/entity/PER0003">
	<rdf:type rdf:resource="http://www.w3.org/2002/07/owl#NamedIndividual"/>
	<rdf:type rdf:resource="http://www.cidoc-crm.org/cidoc-crm/E18_Physical_Thing"/>
	<rdf:type rdf:resource="http://www.cidoc-crm.org/cidoc-crm/E19_Physical_Object"/>
	<rdf:type rdf:resource="http://www.cidoc-crm.org/cidoc-crm/E1_CRM_Entity"/>
	<rdf:type rdf:resource="http://www.cidoc-crm.org/cidoc-crm/E20_Biological_Object"/>
	<rdf:type rdf:resource="http://www.cidoc-crm.org/cidoc-crm/E21_Person"/>
	<rdf:type rdf:resource="http://www.cidoc-crm.org/cidoc-crm/E39_Actor"/>
	<rdf:type rdf:resource="http://www.cidoc-crm.org/cidoc-crm/E70_Thing"/>
	<rdf:type rdf:resource="http://www.cidoc-crm.org/cidoc-crm/E72_Legal_Object"/>
	<rdf:type rdf:resource="http://www.cidoc-crm.org/cidoc-crm/E77_Persistent_Item"/>
	<rdf:type rdf:resource="http://www.loa-cnr.it/ontologies/DOLCE-Lite#endurant"/>
	<cidoc-crm:P107i_is_current_or_former_member_of rdf:resource="http://academictourism.com/entity/TG"/>
	<cidoc-crm:P11i_participated_in rdf:resource="http://academictourism.com/entity/J0001"/>
	<cidoc-crm:P11i_participated_in rdf:resource="http://academictourism.com/entity/L0001"/>
	<cidoc-crm:P12i_was_present_at rdf:resource="http://academictourism.com/entity/J0001"/>
	<cidoc-crm:P12i_was_present_at rdf:resource="http://academictourism.com/entity/L0001"/>
	<cidoc-crm:P143i_was_joined_by rdf:resource="http://academictourism.com/entity/J0001"/>
	<cidoc-crm:P145i_left_by rdf:resource="http://academictourism.com/entity/L0001"/>
	<cidoc-crm:P2_has_type rdf:resource="http://vocab.getty.edu/page/aat/300025879"/>
	<cidoc-crm:P2_has_type rdf:resource="http://vocab.getty.edu/page/aat/300137147"/>
	<skos:prefLabel>Hr van Assen</skos:prefLabel>
</rdf:Description>

<rdf:Description rdf:about="http://academictourism.com/entity/PER0004">
	<rdf:type rdf:resource="http://www.w3.org/2002/07/owl#NamedIndividual"/>
	<rdf:type rdf:resource="http://www.cidoc-crm.org/cidoc-crm/E18_Physical_Thing"/>
	<rdf:type rdf:resource="http://www.cidoc-crm.org/cidoc-crm/E19_Physical_Object"/>
	<rdf:type rdf:resource="http://www.cidoc-crm.org/cidoc-crm/E1_CRM_Entity"/>
	<rdf:type rdf:resource="http://www.cidoc-crm.org/cidoc-crm/E20_Biological_Object"/>
	<rdf:type rdf:resource="http://www.cidoc-crm.org/cidoc-crm/E21_Person"/>
	<rdf:type rdf:resource="http://www.cidoc-crm.org/cidoc-crm/E39_Actor"/>
	<rdf:type rdf:resource="http://www.cidoc-crm.org/cidoc-crm/E70_Thing"/>
	<rdf:type rdf:resource="http://www.cidoc-crm.org/cidoc-crm/E72_Legal_Object"/>
	<rdf:type rdf:resource="http://www.cidoc-crm.org/cidoc-crm/E77_Persistent_Item"/>
	<rdf:type rdf:resource="http://www.loa-cnr.it/ontologies/DOLCE-Lite#endurant"/>
	<cidoc-crm:P107i_is_current_or_former_member_of rdf:resource="http://academictourism.com/entity/TG"/>
	<cidoc-crm:P11i_participated_in rdf:resource="http://academictourism.com/entity/J0001"/>
	<cidoc-crm:P11i_participated_in rdf:resource="http://academictourism.com/entity/L0001"/>
	<cidoc-crm:P12i_was_present_at rdf:resource="http://academictourism.com/entity/J0001"/>
	<cidoc-crm:P12i_was_present_at rdf:resource="http://academictourism.com/entity/L0001"/>
	<cidoc-crm:P143i_was_joined_by rdf:resource="http://academictourism.com/entity/J0001"/>
	<cidoc-crm:P145i_left_by rdf:resource="http://academictourism.com/entity/L0001"/>
	<cidoc-crm:P2_has_type rdf:resource="http://vocab.getty.edu/page/aat/300025879"/>
	<skos:prefLabel>Hr de Geer</skos:prefLabel>
</rdf:Description>

<rdf:Description rdf:about="http://academictourism.com/entity/PER0005">
	<rdf:type rdf:resource="http://www.w3.org/2002/07/owl#NamedIndividual"/>
	<rdf:type rdf:resource="http://www.cidoc-crm.org/cidoc-crm/E18_Physical_Thing"/>
	<rdf:type rdf:resource="http://www.cidoc-crm.org/cidoc-crm/E19_Physical_Object"/>
	<rdf:type rdf:resource="http://www.cidoc-crm.org/cidoc-crm/E1_CRM_Entity"/>
	<rdf:type rdf:resource="http://www.cidoc-crm.org/cidoc-crm/E20_Biological_Object"/>
	<rdf:type rdf:resource="http://www.cidoc-crm.org/cidoc-crm/E21_Person"/>
	<rdf:type rdf:resource="http://www.cidoc-crm.org/cidoc-crm/E39_Actor"/>
	<rdf:type rdf:resource="http://www.cidoc-crm.org/cidoc-crm/E70_Thing"/>
	<rdf:type rdf:resource="http://www.cidoc-crm.org/cidoc-crm/E72_Legal_Object"/>
	<rdf:type rdf:resource="http://www.cidoc-crm.org/cidoc-crm/E77_Persistent_Item"/>
	<rdf:type rdf:resource="http://www.loa-cnr.it/ontologies/DOLCE-Lite#endurant"/>
	<rdf:type rdf:resource="http://www.w3.org/2004/02/skos/core#Concept"/>
	<cidoc-crm:P11i_participated_in rdf:resource="http://academictourism.com/entity/BRF0005.RS.L0001"/>
	<cidoc-crm:P12i_was_present_at rdf:resource="http://academictourism.com/entity/BRF0005.RS.L0001"/>
	<cidoc-crm:P14i_performed rdf:resource="http://academictourism.com/entity/BRF0005.RS.L0001"/>
	<cidoc-crm:P2_has_type rdf:resource="http://vocab.getty.edu/page/aat/300025533"/>
	<skos:closeMatch rdf:resource="http://academictourism.com/entity/PER0005"/>
	<skos:closeMatch rdf:resource="http://viaf.org/viaf/24668261"/>
	<skos:exactMatch rdf:resource="http://academictourism.com/entity/PER0005"/>
	<skos:exactMatch rdf:resource="http://viaf.org/viaf/24668261"/>
	<skos:mappingRelation rdf:resource="http://academictourism.com/entity/PER0005"/>
	<skos:mappingRelation rdf:resource="http://viaf.org/viaf/24668261"/>
	<skos:semanticRelation rdf:resource="http://academictourism.com/entity/PER0005"/>
	<skos:semanticRelation rdf:resource="http://viaf.org/viaf/24668261"/>
	<rdfs:seeAlso rdf:datatype="http://www.w3.org/2001/XMLSchema#anyURI">https://de.wikipedia.org/wiki/Gustav_Hugo</rdfs:seeAlso>
	<skos:prefLabel>Gustav Hugo</skos:prefLabel>
</rdf:Description>

<rdf:Description rdf:about="http://academictourism.com/entity/PER0006">
	<rdf:type rdf:resource="http://www.w3.org/2002/07/owl#NamedIndividual"/>
	<rdf:type rdf:resource="http://www.cidoc-crm.org/cidoc-crm/E18_Physical_Thing"/>
	<rdf:type rdf:resource="http://www.cidoc-crm.org/cidoc-crm/E19_Physical_Object"/>
	<rdf:type rdf:resource="http://www.cidoc-crm.org/cidoc-crm/E1_CRM_Entity"/>
	<rdf:type rdf:resource="http://www.cidoc-crm.org/cidoc-crm/E20_Biological_Object"/>
	<rdf:type rdf:resource="http://www.cidoc-crm.org/cidoc-crm/E21_Person"/>
	<rdf:type rdf:resource="http://www.cidoc-crm.org/cidoc-crm/E39_Actor"/>
	<rdf:type rdf:resource="http://www.cidoc-crm.org/cidoc-crm/E70_Thing"/>
	<rdf:type rdf:resource="http://www.cidoc-crm.org/cidoc-crm/E72_Legal_Object"/>
	<rdf:type rdf:resource="http://www.cidoc-crm.org/cidoc-crm/E77_Persistent_Item"/>
	<rdf:type rdf:resource="http://www.loa-cnr.it/ontologies/DOLCE-Lite#endurant"/>
	<rdf:type rdf:resource="http://www.w3.org/2004/02/skos/core#Concept"/>
	<cidoc-crm:P11i_participated_in rdf:resource="http://academictourism.com/entity/BRF0005.RS.L0002"/>
	<cidoc-crm:P12i_was_present_at rdf:resource="http://academictourism.com/entity/BRF0005.RS.L0002"/>
	<cidoc-crm:P14i_performed rdf:resource="http://academictourism.com/entity/BRF0005.RS.L0002"/>
	<cidoc-crm:P2_has_type rdf:resource="http://vocab.getty.edu/page/aat/300025533"/>
	<skos:closeMatch rdf:resource="http://academictourism.com/entity/PER0006"/>
	<skos:closeMatch rdf:resource="http://viaf.org/viaf/71547594"/>
	<skos:exactMatch rdf:resource="http://academictourism.com/entity/PER0006"/>
	<skos:exactMatch rdf:resource="http://viaf.org/viaf/71547594"/>
	<skos:mappingRelation rdf:resource="http://academictourism.com/entity/PER0006"/>
	<skos:mappingRelation rdf:resource="http://viaf.org/viaf/71547594"/>
	<skos:semanticRelation rdf:resource="http://academictourism.com/entity/PER0006"/>
	<skos:semanticRelation rdf:resource="http://viaf.org/viaf/71547594"/>
	<skos:prefLabel>Arnold Hermann Ludwig Heeren</skos:prefLabel>
	<skos:prefLabel>https://en.wikipedia.org/wiki/Arnold_Hermann_Ludwig_Heeren</skos:prefLabel>
</rdf:Description>

<rdf:Description rdf:about="http://academictourism.com/entity/PER0007">
	<rdf:type rdf:resource="http://www.w3.org/2002/07/owl#NamedIndividual"/>
	<rdf:type rdf:resource="http://www.cidoc-crm.org/cidoc-crm/E18_Physical_Thing"/>
	<rdf:type rdf:resource="http://www.cidoc-crm.org/cidoc-crm/E19_Physical_Object"/>
	<rdf:type rdf:resource="http://www.cidoc-crm.org/cidoc-crm/E1_CRM_Entity"/>
	<rdf:type rdf:resource="http://www.cidoc-crm.org/cidoc-crm/E20_Biological_Object"/>
	<rdf:type rdf:resource="http://www.cidoc-crm.org/cidoc-crm/E21_Person"/>
	<rdf:type rdf:resource="http://www.cidoc-crm.org/cidoc-crm/E39_Actor"/>
	<rdf:type rdf:resource="http://www.cidoc-crm.org/cidoc-crm/E70_Thing"/>
	<rdf:type rdf:resource="http://www.cidoc-crm.org/cidoc-crm/E72_Legal_Object"/>
	<rdf:type rdf:resource="http://www.cidoc-crm.org/cidoc-crm/E77_Persistent_Item"/>
	<rdf:type rdf:resource="http://www.loa-cnr.it/ontologies/DOLCE-Lite#endurant"/>
	<cidoc-crm:P11i_participated_in rdf:resource="http://academictourism.com/entity/BRF0005.RS.L0003"/>
	<cidoc-crm:P12i_was_present_at rdf:resource="http://academictourism.com/entity/BRF0005.RS.L0003"/>
	<cidoc-crm:P14i_performed rdf:resource="http://academictourism.com/entity/BRF0005.RS.L0003"/>
	<cidoc-crm:P2_has_type rdf:resource="http://vocab.getty.edu/page/aat/300025533"/>
	<skos:prefLabel>Prof. Bauer</skos:prefLabel>
</rdf:Description>

<rdf:Description rdf:about="http://academictourism.com/entity/PER0008">
	<rdf:type rdf:resource="http://www.w3.org/2002/07/owl#NamedIndividual"/>
	<rdf:type rdf:resource="http://www.cidoc-crm.org/cidoc-crm/E18_Physical_Thing"/>
	<rdf:type rdf:resource="http://www.cidoc-crm.org/cidoc-crm/E19_Physical_Object"/>
	<rdf:type rdf:resource="http://www.cidoc-crm.org/cidoc-crm/E1_CRM_Entity"/>
	<rdf:type rdf:resource="http://www.cidoc-crm.org/cidoc-crm/E20_Biological_Object"/>
	<rdf:type rdf:resource="http://www.cidoc-crm.org/cidoc-crm/E21_Person"/>
	<rdf:type rdf:resource="http://www.cidoc-crm.org/cidoc-crm/E39_Actor"/>
	<rdf:type rdf:resource="http://www.cidoc-crm.org/cidoc-crm/E70_Thing"/>
	<rdf:type rdf:resource="http://www.cidoc-crm.org/cidoc-crm/E72_Legal_Object"/>
	<rdf:type rdf:resource="http://www.cidoc-crm.org/cidoc-crm/E77_Persistent_Item"/>
	<rdf:type rdf:resource="http://www.loa-cnr.it/ontologies/DOLCE-Lite#endurant"/>
	<rdf:type rdf:resource="http://www.w3.org/2004/02/skos/core#Concept"/>
	<cidoc-crm:P11i_participated_in rdf:resource="http://academictourism.com/entity/BRF0005.RS.L0004"/>
	<cidoc-crm:P12i_was_present_at rdf:resource="http://academictourism.com/entity/BRF0005.RS.L0004"/>
	<cidoc-crm:P14i_performed rdf:resource="http://academictourism.com/entity/BRF0005.RS.L0004"/>
	<cidoc-crm:P2_has_type rdf:resource="http://vocab.getty.edu/page/aat/300025533"/>
	<skos:closeMatch rdf:resource="http://academictourism.com/entity/PER0008"/>
	<skos:closeMatch rdf:resource="http://viaf.org/viaf/71570755"/>
	<skos:exactMatch rdf:resource="http://academictourism.com/entity/PER0008"/>
	<skos:exactMatch rdf:resource="http://viaf.org/viaf/71570755"/>
	<skos:mappingRelation rdf:resource="http://academictourism.com/entity/PER0008"/>
	<skos:mappingRelation rdf:resource="http://viaf.org/viaf/71570755"/>
	<skos:semanticRelation rdf:resource="http://academictourism.com/entity/PER0008"/>
	<skos:semanticRelation rdf:resource="http://viaf.org/viaf/71570755"/>
	<rdfs:seeAlso rdf:datatype="http://www.w3.org/2001/XMLSchema#anyURI">https://de.wikipedia.org/wiki/Johann_Friedrich_Blumenbach</rdfs:seeAlso>
	<skos:prefLabel>Prof. Blumenbach</skos:prefLabel>
</rdf:Description>

<rdf:Description rdf:about="http://academictourism.com/entity/PER0009">
	<rdf:type rdf:resource="http://www.w3.org/2002/07/owl#NamedIndividual"/>
	<rdf:type rdf:resource="http://www.cidoc-crm.org/cidoc-crm/E18_Physical_Thing"/>
	<rdf:type rdf:resource="http://www.cidoc-crm.org/cidoc-crm/E19_Physical_Object"/>
	<rdf:type rdf:resource="http://www.cidoc-crm.org/cidoc-crm/E1_CRM_Entity"/>
	<rdf:type rdf:resource="http://www.cidoc-crm.org/cidoc-crm/E20_Biological_Object"/>
	<rdf:type rdf:resource="http://www.cidoc-crm.org/cidoc-crm/E21_Person"/>
	<rdf:type rdf:resource="http://www.cidoc-crm.org/cidoc-crm/E39_Actor"/>
	<rdf:type rdf:resource="http://www.cidoc-crm.org/cidoc-crm/E70_Thing"/>
	<rdf:type rdf:resource="http://www.cidoc-crm.org/cidoc-crm/E72_Legal_Object"/>
	<rdf:type rdf:resource="http://www.cidoc-crm.org/cidoc-crm/E77_Persistent_Item"/>
	<rdf:type rdf:resource="http://www.loa-cnr.it/ontologies/DOLCE-Lite#endurant"/>
	<rdf:type rdf:resource="http://www.w3.org/2004/02/skos/core#Concept"/>
	<cidoc-crm:P11i_participated_in rdf:resource="http://academictourism.com/entity/BE.MISC0003"/>
	<cidoc-crm:P12i_was_present_at rdf:resource="http://academictourism.com/entity/BE.MISC0003"/>
	<cidoc-crm:P14i_performed rdf:resource="http://academictourism.com/entity/BE.MISC0003"/>
	<cidoc-crm:P2_has_type rdf:resource="http://vocab.getty.edu/page/aat/300025136"/>
	<skos:closeMatch rdf:resource="http://academictourism.com/entity/PER0009"/>
	<skos:closeMatch rdf:resource="http://viaf.org/viaf/61536450"/>
	<skos:exactMatch rdf:resource="http://academictourism.com/entity/PER0009"/>
	<skos:exactMatch rdf:resource="http://viaf.org/viaf/61536450"/>
	<skos:mappingRelation rdf:resource="http://academictourism.com/entity/PER0009"/>
	<skos:mappingRelation rdf:resource="http://viaf.org/viaf/61536450"/>
	<skos:semanticRelation rdf:resource="http://academictourism.com/entity/PER0009"/>
	<skos:semanticRelation rdf:resource="http://viaf.org/viaf/61536450"/>
	<rdfs:seeAlso rdf:datatype="http://www.w3.org/2001/XMLSchema#anyURI">https://en.wikipedia.org/wiki/Johann_Heinrich_Wilhelm_Tischbein</rdfs:seeAlso>
	<skos:prefLabel>Johann Heinrich Wilhelm Tischbein</skos:prefLabel>
</rdf:Description>

<rdf:Description rdf:about="http://academictourism.com/entity/PER0010">
	<rdf:type rdf:resource="http://www.w3.org/2002/07/owl#NamedIndividual"/>
	<rdf:type rdf:resource="http://www.cidoc-crm.org/cidoc-crm/E18_Physical_Thing"/>
	<rdf:type rdf:resource="http://www.cidoc-crm.org/cidoc-crm/E19_Physical_Object"/>
	<rdf:type rdf:resource="http://www.cidoc-crm.org/cidoc-crm/E1_CRM_Entity"/>
	<rdf:type rdf:resource="http://www.cidoc-crm.org/cidoc-crm/E20_Biological_Object"/>
	<rdf:type rdf:resource="http://www.cidoc-crm.org/cidoc-crm/E21_Person"/>
	<rdf:type rdf:resource="http://www.cidoc-crm.org/cidoc-crm/E39_Actor"/>
	<rdf:type rdf:resource="http://www.cidoc-crm.org/cidoc-crm/E70_Thing"/>
	<rdf:type rdf:resource="http://www.cidoc-crm.org/cidoc-crm/E72_Legal_Object"/>
	<rdf:type rdf:resource="http://www.cidoc-crm.org/cidoc-crm/E77_Persistent_Item"/>
	<rdf:type rdf:resource="http://www.loa-cnr.it/ontologies/DOLCE-Lite#endurant"/>
	<rdf:type rdf:resource="http://www.w3.org/2004/02/skos/core#Concept"/>
	<cidoc-crm:P11i_participated_in rdf:resource="http://academictourism.com/entity/BE.MISC0018"/>
	<cidoc-crm:P12i_was_present_at rdf:resource="http://academictourism.com/entity/BE.MISC0018"/>
	<skos:closeMatch rdf:resource="http://academictourism.com/entity/PER0010"/>
	<skos:closeMatch rdf:resource="http://viaf.org/viaf/9856912"/>
	<skos:exactMatch rdf:resource="http://academictourism.com/entity/PER0010"/>
	<skos:exactMatch rdf:resource="http://viaf.org/viaf/9856912"/>
	<skos:mappingRelation rdf:resource="http://academictourism.com/entity/PER0010"/>
	<skos:mappingRelation rdf:resource="http://viaf.org/viaf/9856912"/>
	<skos:semanticRelation rdf:resource="http://academictourism.com/entity/PER0010"/>
	<skos:semanticRelation rdf:resource="http://viaf.org/viaf/9856912"/>
	<rdfs:seeAlso rdf:datatype="http://www.w3.org/2001/XMLSchema#anyURI">https://en.wikipedia.org/wiki/Christoph_Martin_Wieland</rdfs:seeAlso>
	<skos:prefLabel>Christoph Martin Wieland</skos:prefLabel>
</rdf:Description>

<rdf:Description rdf:about="http://academictourism.com/entity/PER0011">
	<rdf:type rdf:resource="http://www.w3.org/2002/07/owl#NamedIndividual"/>
	<rdf:type rdf:resource="http://www.cidoc-crm.org/cidoc-crm/E18_Physical_Thing"/>
	<rdf:type rdf:resource="http://www.cidoc-crm.org/cidoc-crm/E19_Physical_Object"/>
	<rdf:type rdf:resource="http://www.cidoc-crm.org/cidoc-crm/E1_CRM_Entity"/>
	<rdf:type rdf:resource="http://www.cidoc-crm.org/cidoc-crm/E20_Biological_Object"/>
	<rdf:type rdf:resource="http://www.cidoc-crm.org/cidoc-crm/E21_Person"/>
	<rdf:type rdf:resource="http://www.cidoc-crm.org/cidoc-crm/E39_Actor"/>
	<rdf:type rdf:resource="http://www.cidoc-crm.org/cidoc-crm/E70_Thing"/>
	<rdf:type rdf:resource="http://www.cidoc-crm.org/cidoc-crm/E72_Legal_Object"/>
	<rdf:type rdf:resource="http://www.cidoc-crm.org/cidoc-crm/E77_Persistent_Item"/>
	<rdf:type rdf:resource="http://www.loa-cnr.it/ontologies/DOLCE-Lite#endurant"/>
	<rdf:type rdf:resource="http://www.w3.org/2004/02/skos/core#Concept"/>
	<cidoc-crm:P11i_participated_in rdf:resource="http://academictourism.com/entity/BE.LOC0003.CS"/>
	<cidoc-crm:P12i_was_present_at rdf:resource="http://academictourism.com/entity/BE.LOC0003.CS"/>
	<skos:closeMatch rdf:resource="http://academictourism.com/entity/PER0011"/>
	<skos:closeMatch rdf:resource="https://viaf.org/viaf/47863906"/>
	<skos:exactMatch rdf:resource="http://academictourism.com/entity/PER0011"/>
	<skos:exactMatch rdf:resource="https://viaf.org/viaf/47863906"/>
	<skos:mappingRelation rdf:resource="http://academictourism.com/entity/PER0011"/>
	<skos:mappingRelation rdf:resource="https://viaf.org/viaf/47863906"/>
	<skos:semanticRelation rdf:resource="http://academictourism.com/entity/PER0011"/>
	<skos:semanticRelation rdf:resource="https://viaf.org/viaf/47863906"/>
	<rdfs:seeAlso rdf:datatype="http://www.w3.org/2001/XMLSchema#anyURI">https://en.wikipedia.org/wiki/Frederick_II,_Landgrave_of_Hesse-Kassel</rdfs:seeAlso>
	<skos:prefLabel>Frederik_de_II</skos:prefLabel>
</rdf:Description>

<rdf:Description rdf:about="http://academictourism.com/entity/PER0012">
	<rdf:type rdf:resource="http://www.w3.org/2002/07/owl#NamedIndividual"/>
	<rdf:type rdf:resource="http://www.cidoc-crm.org/cidoc-crm/E18_Physical_Thing"/>
	<rdf:type rdf:resource="http://www.cidoc-crm.org/cidoc-crm/E19_Physical_Object"/>
	<rdf:type rdf:resource="http://www.cidoc-crm.org/cidoc-crm/E1_CRM_Entity"/>
	<rdf:type rdf:resource="http://www.cidoc-crm.org/cidoc-crm/E20_Biological_Object"/>
	<rdf:type rdf:resource="http://www.cidoc-crm.org/cidoc-crm/E21_Person"/>
	<rdf:type rdf:resource="http://www.cidoc-crm.org/cidoc-crm/E39_Actor"/>
	<rdf:type rdf:resource="http://www.cidoc-crm.org/cidoc-crm/E70_Thing"/>
	<rdf:type rdf:resource="http://www.cidoc-crm.org/cidoc-crm/E72_Legal_Object"/>
	<rdf:type rdf:resource="http://www.cidoc-crm.org/cidoc-crm/E77_Persistent_Item"/>
	<rdf:type rdf:resource="http://www.loa-cnr.it/ontologies/DOLCE-Lite#endurant"/>
	<rdf:type rdf:resource="http://www.w3.org/2004/02/skos/core#Concept"/>
	<cidoc-crm:P11i_participated_in rdf:resource="http://academictourism.com/entity/BE.LOC0003.CS"/>
	<cidoc-crm:P12i_was_present_at rdf:resource="http://academictourism.com/entity/BE.LOC0003.CS"/>
	<skos:closeMatch rdf:resource="http://academictourism.com/entity/PER0012"/>
	<skos:closeMatch rdf:resource="https://viaf.org/viaf/264553004"/>
	<skos:exactMatch rdf:resource="http://academictourism.com/entity/PER0012"/>
	<skos:exactMatch rdf:resource="https://viaf.org/viaf/264553004"/>
	<skos:mappingRelation rdf:resource="http://academictourism.com/entity/PER0012"/>
	<skos:mappingRelation rdf:resource="https://viaf.org/viaf/264553004"/>
	<skos:semanticRelation rdf:resource="http://academictourism.com/entity/PER0012"/>
	<skos:semanticRelation rdf:resource="https://viaf.org/viaf/264553004"/>
	<rdfs:seeAlso rdf:datatype="http://www.w3.org/2001/XMLSchema#anyURI">https://en.wikipedia.org/wiki/William_I,_Elector_of_Hesse</rdfs:seeAlso>
	<skos:prefLabel>Wilhelm_IX</skos:prefLabel>
</rdf:Description>

<rdf:Description rdf:about="http://academictourism.com/entity/PER0013">
	<rdf:type rdf:resource="http://www.w3.org/2002/07/owl#NamedIndividual"/>
	<rdf:type rdf:resource="http://www.cidoc-crm.org/cidoc-crm/E18_Physical_Thing"/>
	<rdf:type rdf:resource="http://www.cidoc-crm.org/cidoc-crm/E19_Physical_Object"/>
	<rdf:type rdf:resource="http://www.cidoc-crm.org/cidoc-crm/E1_CRM_Entity"/>
	<rdf:type rdf:resource="http://www.cidoc-crm.org/cidoc-crm/E20_Biological_Object"/>
	<rdf:type rdf:resource="http://www.cidoc-crm.org/cidoc-crm/E21_Person"/>
	<rdf:type rdf:resource="http://www.cidoc-crm.org/cidoc-crm/E39_Actor"/>
	<rdf:type rdf:resource="http://www.cidoc-crm.org/cidoc-crm/E70_Thing"/>
	<rdf:type rdf:resource="http://www.cidoc-crm.org/cidoc-crm/E72_Legal_Object"/>
	<rdf:type rdf:resource="http://www.cidoc-crm.org/cidoc-crm/E77_Persistent_Item"/>
	<rdf:type rdf:resource="http://www.loa-cnr.it/ontologies/DOLCE-Lite#endurant"/>
	<rdf:type rdf:resource="http://www.w3.org/2004/02/skos/core#Concept"/>
	<cidoc-crm:P11i_participated_in rdf:resource="http://academictourism.com/entity/BE.MISC0021"/>
	<cidoc-crm:P12i_was_present_at rdf:resource="http://academictourism.com/entity/BE.MISC0021"/>
	<skos:closeMatch rdf:resource="http://academictourism.com/entity/PER0013"/>
	<skos:closeMatch rdf:resource="http://viaf.org/viaf/4936996"/>
	<skos:exactMatch rdf:resource="http://academictourism.com/entity/PER0013"/>
	<skos:exactMatch rdf:resource="http://viaf.org/viaf/4936996"/>
	<skos:mappingRelation rdf:resource="http://academictourism.com/entity/PER0013"/>
	<skos:mappingRelation rdf:resource="http://viaf.org/viaf/4936996"/>
	<skos:semanticRelation rdf:resource="http://academictourism.com/entity/PER0013"/>
	<skos:semanticRelation rdf:resource="http://viaf.org/viaf/4936996"/>
	<rdfs:comment>Torquato Tasso</rdfs:comment>
	<rdfs:seeAlso rdf:datatype="http://www.w3.org/2001/XMLSchema#anyURI">https://en.wikipedia.org/wiki/Torquato_Tasso</rdfs:seeAlso>
</rdf:Description>

<rdf:Description rdf:about="http://academictourism.com/entity/PER0014">
	<rdf:type rdf:resource="http://www.w3.org/2002/07/owl#NamedIndividual"/>
	<rdf:type rdf:resource="http://www.cidoc-crm.org/cidoc-crm/E18_Physical_Thing"/>
	<rdf:type rdf:resource="http://www.cidoc-crm.org/cidoc-crm/E19_Physical_Object"/>
	<rdf:type rdf:resource="http://www.cidoc-crm.org/cidoc-crm/E1_CRM_Entity"/>
	<rdf:type rdf:resource="http://www.cidoc-crm.org/cidoc-crm/E20_Biological_Object"/>
	<rdf:type rdf:resource="http://www.cidoc-crm.org/cidoc-crm/E21_Person"/>
	<rdf:type rdf:resource="http://www.cidoc-crm.org/cidoc-crm/E39_Actor"/>
	<rdf:type rdf:resource="http://www.cidoc-crm.org/cidoc-crm/E70_Thing"/>
	<rdf:type rdf:resource="http://www.cidoc-crm.org/cidoc-crm/E72_Legal_Object"/>
	<rdf:type rdf:resource="http://www.cidoc-crm.org/cidoc-crm/E77_Persistent_Item"/>
	<rdf:type rdf:resource="http://www.loa-cnr.it/ontologies/DOLCE-Lite#endurant"/>
	<rdf:type rdf:resource="http://www.w3.org/2004/02/skos/core#Concept"/>
	<cidoc-crm:P11i_participated_in rdf:resource="http://academictourism.com/entity/BE.MISC0022"/>
	<cidoc-crm:P12i_was_present_at rdf:resource="http://academictourism.com/entity/BE.MISC0022"/>
	<skos:closeMatch rdf:resource="http://academictourism.com/entity/PER0014"/>
	<skos:closeMatch rdf:resource="http://viaf.org/viaf/185047668"/>
	<skos:exactMatch rdf:resource="http://academictourism.com/entity/PER0014"/>
	<skos:exactMatch rdf:resource="http://viaf.org/viaf/185047668"/>
	<skos:mappingRelation rdf:resource="http://academictourism.com/entity/PER0014"/>
	<skos:mappingRelation rdf:resource="http://viaf.org/viaf/185047668"/>
	<skos:semanticRelation rdf:resource="http://academictourism.com/entity/PER0014"/>
	<skos:semanticRelation rdf:resource="http://viaf.org/viaf/185047668"/>
	<skos:prefLabel>Johann Wilhelm Döring</skos:prefLabel>
</rdf:Description>

<rdf:Description rdf:about="http://academictourism.com/entity/PER0015">
	<rdf:type rdf:resource="http://www.w3.org/2002/07/owl#NamedIndividual"/>
	<rdf:type rdf:resource="http://www.cidoc-crm.org/cidoc-crm/E18_Physical_Thing"/>
	<rdf:type rdf:resource="http://www.cidoc-crm.org/cidoc-crm/E19_Physical_Object"/>
	<rdf:type rdf:resource="http://www.cidoc-crm.org/cidoc-crm/E1_CRM_Entity"/>
	<rdf:type rdf:resource="http://www.cidoc-crm.org/cidoc-crm/E20_Biological_Object"/>
	<rdf:type rdf:resource="http://www.cidoc-crm.org/cidoc-crm/E21_Person"/>
	<rdf:type rdf:resource="http://www.cidoc-crm.org/cidoc-crm/E39_Actor"/>
	<rdf:type rdf:resource="http://www.cidoc-crm.org/cidoc-crm/E70_Thing"/>
	<rdf:type rdf:resource="http://www.cidoc-crm.org/cidoc-crm/E72_Legal_Object"/>
	<rdf:type rdf:resource="http://www.cidoc-crm.org/cidoc-crm/E77_Persistent_Item"/>
	<rdf:type rdf:resource="http://www.loa-cnr.it/ontologies/DOLCE-Lite#endurant"/>
	<cidoc-crm:P11i_participated_in rdf:resource="http://academictourism.com/entity/BE.MISC0001"/>
	<cidoc-crm:P12i_was_present_at rdf:resource="http://academictourism.com/entity/BE.MISC0001"/>
	<skos:prefLabel>Jerome</skos:prefLabel>
</rdf:Description>

<rdf:Description rdf:about="http://academictourism.com/entity/PER0016">
	<rdf:type rdf:resource="http://www.w3.org/2002/07/owl#NamedIndividual"/>
	<rdf:type rdf:resource="http://www.cidoc-crm.org/cidoc-crm/E18_Physical_Thing"/>
	<rdf:type rdf:resource="http://www.cidoc-crm.org/cidoc-crm/E19_Physical_Object"/>
	<rdf:type rdf:resource="http://www.cidoc-crm.org/cidoc-crm/E1_CRM_Entity"/>
	<rdf:type rdf:resource="http://www.cidoc-crm.org/cidoc-crm/E20_Biological_Object"/>
	<rdf:type rdf:resource="http://www.cidoc-crm.org/cidoc-crm/E21_Person"/>
	<rdf:type rdf:resource="http://www.cidoc-crm.org/cidoc-crm/E39_Actor"/>
	<rdf:type rdf:resource="http://www.cidoc-crm.org/cidoc-crm/E70_Thing"/>
	<rdf:type rdf:resource="http://www.cidoc-crm.org/cidoc-crm/E72_Legal_Object"/>
	<rdf:type rdf:resource="http://www.cidoc-crm.org/cidoc-crm/E77_Persistent_Item"/>
	<rdf:type rdf:resource="http://www.loa-cnr.it/ontologies/DOLCE-Lite#endurant"/>
	<rdf:type rdf:resource="http://www.w3.org/2004/02/skos/core#Concept"/>
	<cidoc-crm:P11i_participated_in rdf:resource="http://academictourism.com/entity/BE.LOC0003.CS"/>
	<cidoc-crm:P11i_participated_in rdf:resource="http://academictourism.com/entity/BE.MISC0019"/>
	<cidoc-crm:P12i_was_present_at rdf:resource="http://academictourism.com/entity/BE.LOC0003.CS"/>
	<cidoc-crm:P12i_was_present_at rdf:resource="http://academictourism.com/entity/BE.MISC0019"/>
	<cidoc-crm:P51i_is_former_or_current_owner_of rdf:resource="http://academictourism.com/entity/LOC0003.CS"/>
	<skos:closeMatch rdf:resource="http://academictourism.com/entity/PER0016"/>
	<skos:closeMatch rdf:resource="https://viaf.org/viaf/29528071"/>
	<skos:exactMatch rdf:resource="http://academictourism.com/entity/PER0016"/>
	<skos:exactMatch rdf:resource="https://viaf.org/viaf/29528071"/>
	<skos:mappingRelation rdf:resource="http://academictourism.com/entity/PER0016"/>
	<skos:mappingRelation rdf:resource="https://viaf.org/viaf/29528071"/>
	<skos:semanticRelation rdf:resource="http://academictourism.com/entity/PER0016"/>
	<skos:semanticRelation rdf:resource="https://viaf.org/viaf/29528071"/>
	<rdfs:seeAlso>https://en.wikipedia.org/wiki/Charles_I,_Landgrave_of_Hesse-Kassel</rdfs:seeAlso>
	<skos:prefLabel>landgraven_Karel</skos:prefLabel>
</rdf:Description>

<rdf:Description rdf:about="http://academictourism.com/entity/R.BRF0004.RS.RS0004.RS0002">
	<rdf:type rdf:resource="http://www.w3.org/2002/07/owl#NamedIndividual"/>
	<rdf:type rdf:resource="http://www.cidoc-crm.org/cidoc-crm/E18_Physical_Thing"/>
	<rdf:type rdf:resource="http://www.cidoc-crm.org/cidoc-crm/E1_CRM_Entity"/>
	<rdf:type rdf:resource="http://www.cidoc-crm.org/cidoc-crm/E70_Thing"/>
	<rdf:type rdf:resource="http://www.cidoc-crm.org/cidoc-crm/E72_Legal_Object"/>
	<rdf:type rdf:resource="http://www.cidoc-crm.org/cidoc-crm/E77_Persistent_Item"/>
	<rdf:type rdf:resource="http://www.loa-cnr.it/ontologies/DOLCE-Lite#endurant"/>
	<cidoc-crm:P43_has_dimension rdf:resource="http://academictourism.com/entity/DT.BRF0004.RS.RS0004.RS0002"/>
	<cidoc-crm:P8i_witnessed rdf:resource="http://academictourism.com/entity/BRF0004.RS.RS0004.RS0002"/>
	<rdfs:label>route from bottom of Octogoon to Hercules</rdfs:label>
</rdf:Description>

<rdf:Description rdf:about="http://academictourism.com/entity/TG">
	<rdf:type rdf:resource="http://www.w3.org/2002/07/owl#NamedIndividual"/>
	<rdf:type rdf:resource="http://www.cidoc-crm.org/cidoc-crm/E1_CRM_Entity"/>
	<rdf:type rdf:resource="http://www.cidoc-crm.org/cidoc-crm/E39_Actor"/>
	<rdf:type rdf:resource="http://www.cidoc-crm.org/cidoc-crm/E74_Group"/>
	<rdf:type rdf:resource="http://www.cidoc-crm.org/cidoc-crm/E77_Persistent_Item"/>
	<rdf:type rdf:resource="http://www.loa-cnr.it/ontologies/DOLCE-Lite#endurant"/>
	<cidoc-crm:P107_has_current_or_former_member rdf:resource="http://academictourism.com/entity/PER0001"/>
	<cidoc-crm:P107_has_current_or_former_member rdf:resource="http://academictourism.com/entity/PER0002"/>
	<cidoc-crm:P107_has_current_or_former_member rdf:resource="http://academictourism.com/entity/PER0003"/>
	<cidoc-crm:P107_has_current_or_former_member rdf:resource="http://academictourism.com/entity/PER0004"/>
	<cidoc-crm:P11i_participated_in rdf:resource="http://academictourism.com/entity/BRF0004.RS"/>
	<cidoc-crm:P11i_participated_in rdf:resource="http://academictourism.com/entity/BRF0004.RS.RS0001"/>
	<cidoc-crm:P11i_participated_in rdf:resource="http://academictourism.com/entity/BRF0004.RS.RS0002"/>
	<cidoc-crm:P11i_participated_in rdf:resource="http://academictourism.com/entity/BRF0004.RS.RS0002.RS0001"/>
	<cidoc-crm:P11i_participated_in rdf:resource="http://academictourism.com/entity/BRF0004.RS.RS0002.RS0002"/>
	<cidoc-crm:P11i_participated_in rdf:resource="http://academictourism.com/entity/BRF0004.RS.RS0002.RS0003"/>
	<cidoc-crm:P11i_participated_in rdf:resource="http://academictourism.com/entity/BRF0004.RS.RS0003"/>
	<cidoc-crm:P11i_participated_in rdf:resource="http://academictourism.com/entity/BRF0004.RS.RS0004"/>
	<cidoc-crm:P11i_participated_in rdf:resource="http://academictourism.com/entity/BRF0004.RS.RS0004.RS0001"/>
	<cidoc-crm:P11i_participated_in rdf:resource="http://academictourism.com/entity/BRF0004.RS.RS0004.RS0002"/>
	<cidoc-crm:P11i_participated_in rdf:resource="http://academictourism.com/entity/BRF0004.RS.RS0004.RS0003"/>
	<cidoc-crm:P11i_participated_in rdf:resource="http://academictourism.com/entity/BRF0004.RS.RS0004.RS0004"/>
	<cidoc-crm:P11i_participated_in rdf:resource="http://academictourism.com/entity/BRF0004.RS.RS0005"/>
	<cidoc-crm:P11i_participated_in rdf:resource="http://academictourism.com/entity/BRF0004.RS.RS0005.RS0001"/>
	<cidoc-crm:P11i_participated_in rdf:resource="http://academictourism.com/entity/BRF0004.RS.RS0006"/>
	<cidoc-crm:P11i_participated_in rdf:resource="http://academictourism.com/entity/BRF0004.RS.RS0006.RS0001"/>
	<cidoc-crm:P11i_participated_in rdf:resource="http://academictourism.com/entity/BRF0004.RS.RS0006.RS0002"/>
	<cidoc-crm:P11i_participated_in rdf:resource="http://academictourism.com/entity/BRF0004.RS.RS0006.RS0003"/>
	<cidoc-crm:P11i_participated_in rdf:resource="http://academictourism.com/entity/BRF0004.RS.RS0006.RS0004"/>
	<cidoc-crm:P11i_participated_in rdf:resource="http://academictourism.com/entity/BRF0004.RS.RS0006.RS0005"/>
	<cidoc-crm:P11i_participated_in rdf:resource="http://academictourism.com/entity/BRF0005.RS"/>
	<cidoc-crm:P11i_participated_in rdf:resource="http://academictourism.com/entity/BRF0005.RS.L0001"/>
	<cidoc-crm:P11i_participated_in rdf:resource="http://academictourism.com/entity/BRF0005.RS.L0002"/>
	<cidoc-crm:P11i_participated_in rdf:resource="http://academictourism.com/entity/BRF0005.RS.L0003"/>
	<cidoc-crm:P11i_participated_in rdf:resource="http://academictourism.com/entity/BRF0005.RS.L0004"/>
	<cidoc-crm:P11i_participated_in rdf:resource="http://academictourism.com/entity/J0001"/>
	<cidoc-crm:P11i_participated_in rdf:resource="http://academictourism.com/entity/J0002"/>
	<cidoc-crm:P11i_participated_in rdf:resource="http://academictourism.com/entity/L0001"/>
	<cidoc-crm:P12i_was_present_at rdf:resource="http://academictourism.com/entity/BRF0004.RS"/>
	<cidoc-crm:P12i_was_present_at rdf:resource="http://academictourism.com/entity/BRF0004.RS.RS0001"/>
	<cidoc-crm:P12i_was_present_at rdf:resource="http://academictourism.com/entity/BRF0004.RS.RS0002"/>
	<cidoc-crm:P12i_was_present_at rdf:resource="http://academictourism.com/entity/BRF0004.RS.RS0002.RS0001"/>
	<cidoc-crm:P12i_was_present_at rdf:resource="http://academictourism.com/entity/BRF0004.RS.RS0002.RS0002"/>
	<cidoc-crm:P12i_was_present_at rdf:resource="http://academictourism.com/entity/BRF0004.RS.RS0002.RS0003"/>
	<cidoc-crm:P12i_was_present_at rdf:resource="http://academictourism.com/entity/BRF0004.RS.RS0003"/>
	<cidoc-crm:P12i_was_present_at rdf:resource="http://academictourism.com/entity/BRF0004.RS.RS0004"/>
	<cidoc-crm:P12i_was_present_at rdf:resource="http://academictourism.com/entity/BRF0004.RS.RS0004.RS0001"/>
	<cidoc-crm:P12i_was_present_at rdf:resource="http://academictourism.com/entity/BRF0004.RS.RS0004.RS0002"/>
	<cidoc-crm:P12i_was_present_at rdf:resource="http://academictourism.com/entity/BRF0004.RS.RS0004.RS0003"/>
	<cidoc-crm:P12i_was_present_at rdf:resource="http://academictourism.com/entity/BRF0004.RS.RS0004.RS0004"/>
	<cidoc-crm:P12i_was_present_at rdf:resource="http://academictourism.com/entity/BRF0004.RS.RS0005"/>
	<cidoc-crm:P12i_was_present_at rdf:resource="http://academictourism.com/entity/BRF0004.RS.RS0005.RS0001"/>
	<cidoc-crm:P12i_was_present_at rdf:resource="http://academictourism.com/entity/BRF0004.RS.RS0006"/>
	<cidoc-crm:P12i_was_present_at rdf:resource="http://academictourism.com/entity/BRF0004.RS.RS0006.RS0001"/>
	<cidoc-crm:P12i_was_present_at rdf:resource="http://academictourism.com/entity/BRF0004.RS.RS0006.RS0002"/>
	<cidoc-crm:P12i_was_present_at rdf:resource="http://academictourism.com/entity/BRF0004.RS.RS0006.RS0003"/>
	<cidoc-crm:P12i_was_present_at rdf:resource="http://academictourism.com/entity/BRF0004.RS.RS0006.RS0004"/>
	<cidoc-crm:P12i_was_present_at rdf:resource="http://academictourism.com/entity/BRF0004.RS.RS0006.RS0005"/>
	<cidoc-crm:P12i_was_present_at rdf:resource="http://academictourism.com/entity/BRF0005.RS"/>
	<cidoc-crm:P12i_was_present_at rdf:resource="http://academictourism.com/entity/BRF0005.RS.L0001"/>
	<cidoc-crm:P12i_was_present_at rdf:resource="http://academictourism.com/entity/BRF0005.RS.L0002"/>
	<cidoc-crm:P12i_was_present_at rdf:resource="http://academictourism.com/entity/BRF0005.RS.L0003"/>
	<cidoc-crm:P12i_was_present_at rdf:resource="http://academictourism.com/entity/BRF0005.RS.L0004"/>
	<cidoc-crm:P12i_was_present_at rdf:resource="http://academictourism.com/entity/J0001"/>
	<cidoc-crm:P12i_was_present_at rdf:resource="http://academictourism.com/entity/J0002"/>
	<cidoc-crm:P12i_was_present_at rdf:resource="http://academictourism.com/entity/L0001"/>
	<cidoc-crm:P144i_gained_member_by rdf:resource="http://academictourism.com/entity/J0001"/>
	<cidoc-crm:P144i_gained_member_by rdf:resource="http://academictourism.com/entity/J0002"/>
	<cidoc-crm:P146i_lost_member_by rdf:resource="http://academictourism.com/entity/L0001"/>
	<skos:prefLabel>Tourism Group</skos:prefLabel>
</rdf:Description>

<rdf:Description rdf:about="http://academictourism.com/entity/TS.BE.MISC0009">
	<rdf:type rdf:resource="http://www.w3.org/2002/07/owl#NamedIndividual"/>
	<rdf:type rdf:resource="http://www.cidoc-crm.org/cidoc-crm/E1_CRM_Entity"/>
	<rdf:type rdf:resource="http://www.cidoc-crm.org/cidoc-crm/E52_Time-Span"/>
	<cidoc-crm:P4i_is_time-span_of rdf:resource="http://academictourism.com/entity/BE.MISC0009"/>
	<cidoc-crm:P82_at_some_time_within rdf:datatype="http://www.w3.org/2001/XMLSchema#integer">1717</cidoc-crm:P82_at_some_time_within>
</rdf:Description>

<rdf:Description rdf:about="http://academictourism.com/entity/TS.BE.MISC0019">
	<rdf:type rdf:resource="http://www.w3.org/2002/07/owl#NamedIndividual"/>
	<rdf:type rdf:resource="http://www.cidoc-crm.org/cidoc-crm/E1_CRM_Entity"/>
	<rdf:type rdf:resource="http://www.cidoc-crm.org/cidoc-crm/E52_Time-Span"/>
	<rdf:type rdf:resource="http://www.cidoc-crm.org/cidoc-crm/E53_Place"/>
	<cidoc-crm:P4i_is_time-span_of rdf:resource="http://academictourism.com/entity/BE.MISC0019"/>
	<cidoc-crm:P171_at_some_place_within>1696-1714</cidoc-crm:P171_at_some_place_within>
</rdf:Description>

<rdf:Description rdf:about="http://academictourism.com/entity/TS.BE.MISC0022">
	<rdf:type rdf:resource="http://www.w3.org/2002/07/owl#NamedIndividual"/>
	<rdf:type rdf:resource="http://www.cidoc-crm.org/cidoc-crm/E1_CRM_Entity"/>
	<rdf:type rdf:resource="http://www.cidoc-crm.org/cidoc-crm/E52_Time-Span"/>
	<cidoc-crm:P4i_is_time-span_of rdf:resource="http://academictourism.com/entity/BE.MISC0022"/>
	<cidoc-crm:P82_at_some_time_within rdf:datatype="http://www.w3.org/2001/XMLSchema#integer">1804</cidoc-crm:P82_at_some_time_within>
</rdf:Description>

<rdf:Description rdf:about="http://academictourism.com/entity/TS.BRF0004.RS.RS0001">
	<rdf:type rdf:resource="http://www.w3.org/2002/07/owl#NamedIndividual"/>
	<rdf:type rdf:resource="http://iflastandards.info/ns/lrm/lrmoo/F3_Manifestation"/>
	<rdf:type rdf:resource="http://www.cidoc-crm.org/cidoc-crm/E1_CRM_Entity"/>
	<rdf:type rdf:resource="http://www.cidoc-crm.org/cidoc-crm/E28_Conceptual_Object"/>
	<rdf:type rdf:resource="http://www.cidoc-crm.org/cidoc-crm/E52_Time-Span"/>
	<rdf:type rdf:resource="http://www.cidoc-crm.org/cidoc-crm/E70_Thing"/>
	<rdf:type rdf:resource="http://www.cidoc-crm.org/cidoc-crm/E71_Human-Made_Thing"/>
	<rdf:type rdf:resource="http://www.cidoc-crm.org/cidoc-crm/E72_Legal_Object"/>
	<rdf:type rdf:resource="http://www.cidoc-crm.org/cidoc-crm/E73_Information_Object"/>
	<rdf:type rdf:resource="http://www.cidoc-crm.org/cidoc-crm/E77_Persistent_Item"/>
	<rdf:type rdf:resource="http://www.cidoc-crm.org/cidoc-crm/E89_Propositional_Object"/>
	<rdf:type rdf:resource="http://www.cidoc-crm.org/cidoc-crm/E90_Symbolic_Object"/>
	<rdf:type rdf:resource="http://www.loa-cnr.it/ontologies/DOLCE-Lite#endurant"/>
	<lrmoo:R70_has_dimension rdf:resource="http://academictourism.com/entity/DR.BRF0004.RS.RS0001"/>
	<cidoc-crm:P43_has_dimension rdf:resource="http://academictourism.com/entity/DR.BRF0004.RS.RS0001"/>
	<cidoc-crm:P4i_is_time-span_of rdf:resource="http://academictourism.com/entity/BRF0004.RS.RS0001"/>
	<cidoc-crm:P4i_is_time-span_of rdf:resource="http://academictourism.com/entity/J0002"/>
	<cidoc-crm:P82_at_some_time_within>7 July 1816</cidoc-crm:P82_at_some_time_within>
</rdf:Description>

<rdf:Description rdf:about="http://academictourism.com/entity/TS.BRF0004.RS.RS0005.RS0001">
	<rdf:type rdf:resource="http://www.w3.org/2002/07/owl#NamedIndividual"/>
	<rdf:type rdf:resource="http://www.cidoc-crm.org/cidoc-crm/E1_CRM_Entity"/>
	<rdf:type rdf:resource="http://www.cidoc-crm.org/cidoc-crm/E52_Time-Span"/>
	<cidoc-crm:P4i_is_time-span_of rdf:resource="http://academictourism.com/entity/BRF0004.RS.RS0005.RS0001"/>
	<cidoc-crm:P170i_time_is_defined_by rdf:datatype="http://www.w3.org/2001/XMLSchema#dateTime">1816-07-08T09:01:00+01:00</cidoc-crm:P170i_time_is_defined_by>
</rdf:Description>

<rdf:Description rdf:about="http://academictourism.com/entity/TS.BRF0004.RS.RS0006">
	<rdf:type rdf:resource="http://www.w3.org/2002/07/owl#NamedIndividual"/>
	<rdf:type rdf:resource="http://www.cidoc-crm.org/cidoc-crm/E1_CRM_Entity"/>
	<rdf:type rdf:resource="http://www.cidoc-crm.org/cidoc-crm/E52_Time-Span"/>
	<rdf:type rdf:resource="http://www.cidoc-crm.org/cidoc-crm/E70_Thing"/>
	<rdf:type rdf:resource="http://www.cidoc-crm.org/cidoc-crm/E77_Persistent_Item"/>
	<rdf:type rdf:resource="http://www.loa-cnr.it/ontologies/DOLCE-Lite#endurant"/>
	<cidoc-crm:P43_has_dimension rdf:resource="http://academictourism.com/entity/DR.BRF0004.RS.RS0006"/>
	<cidoc-crm:P4i_is_time-span_of rdf:resource="http://academictourism.com/entity/BRF0004.RS.RS0006"/>
</rdf:Description>

<rdf:Description rdf:about="http://academictourism.com/entity/TS.BRF0004.RS.RS0006.RS0005">
	<rdf:type rdf:resource="http://www.w3.org/2002/07/owl#NamedIndividual"/>
	<rdf:type rdf:resource="http://www.cidoc-crm.org/cidoc-crm/E1_CRM_Entity"/>
	<rdf:type rdf:resource="http://www.cidoc-crm.org/cidoc-crm/E52_Time-Span"/>
	<cidoc-crm:P4i_is_time-span_of rdf:resource="http://academictourism.com/entity/BRF0004.RS.RS0006.RS0005"/>
	<cidoc-crm:P170i_time_is_defined_by rdf:datatype="http://www.w3.org/2001/XMLSchema#dateTime">1816-07-09T11:00:00+01:00</cidoc-crm:P170i_time_is_defined_by>
</rdf:Description>

<rdf:Description rdf:about="http://academictourism.com/entity/U0001">
	<rdf:type rdf:resource="http://www.w3.org/2002/07/owl#NamedIndividual"/>
	<rdf:type rdf:resource="http://www.cidoc-crm.org/cidoc-crm/E1_CRM_Entity"/>
	<rdf:type rdf:resource="http://www.cidoc-crm.org/cidoc-crm/E28_Conceptual_Object"/>
	<rdf:type rdf:resource="http://www.cidoc-crm.org/cidoc-crm/E55_Type"/>
	<rdf:type rdf:resource="http://www.cidoc-crm.org/cidoc-crm/E58_Measurement_Unit"/>
	<rdf:type rdf:resource="http://www.cidoc-crm.org/cidoc-crm/E70_Thing"/>
	<rdf:type rdf:resource="http://www.cidoc-crm.org/cidoc-crm/E71_Human-Made_Thing"/>
	<rdf:type rdf:resource="http://www.cidoc-crm.org/cidoc-crm/E77_Persistent_Item"/>
	<rdf:type rdf:resource="http://www.loa-cnr.it/ontologies/DOLCE-Lite#endurant"/>
	<cidoc-crm:P91i_is_unit_of rdf:resource="http://academictourism.com/entity/DR.BRF0004.RS.RS0006"/>
	<rdfs:label>hours</rdfs:label>
</rdf:Description>

<rdf:Description rdf:about="http://academictourism.com/entity/ocative_relation1">
	<rdf:type rdf:resource="http://www.w3.org/2002/07/owl#NamedIndividual"/>
	<rdf:type rdf:resource="http://academictourism.com/academictourism#locative_relation"/>
	<rdf:type rdf:resource="http://www.cidoc-crm.org/cidoc-crm/E1_CRM_Entity"/>
	<rdf:type rdf:resource="http://www.cidoc-crm.org/cidoc-crm/E28_Conceptual_Object"/>
	<rdf:type rdf:resource="http://www.cidoc-crm.org/cidoc-crm/E70_Thing"/>
	<rdf:type rdf:resource="http://www.cidoc-crm.org/cidoc-crm/E71_Human-Made_Thing"/>
	<rdf:type rdf:resource="http://www.cidoc-crm.org/cidoc-crm/E77_Persistent_Item"/>
	<rdf:type rdf:resource="http://www.loa-cnr.it/ontologies/DOLCE-Lite#endurant"/>
	<rdf:type rdf:resource="http://www.loa-cnr.it/ontologies/DnS#description"/>
	<rdf:type rdf:resource="http://www.loa-cnr.it/ontologies/DnS#gestalt"/>
	<rdf:type rdf:resource="http://www.loa-cnr.it/ontologies/DnS#relation"/>
	<rdf:type rdf:resource="http://www.loa-cnr.it/ontologies/DnS#theory"/>
	<DnS:involves rdf:resource="http://academictourism.com/entity/LOC0004.CS"/>
	<DnS:involves rdf:resource="http://academictourism.com/entity/PER0001"/>
</rdf:Description>

<rdf:Description rdf:about="http://viaf.org/viaf/185047668">
	<rdf:type rdf:resource="http://www.w3.org/2002/07/owl#NamedIndividual"/>
	<rdf:type rdf:resource="http://www.cidoc-crm.org/cidoc-crm/E18_Physical_Thing"/>
	<rdf:type rdf:resource="http://www.cidoc-crm.org/cidoc-crm/E19_Physical_Object"/>
	<rdf:type rdf:resource="http://www.cidoc-crm.org/cidoc-crm/E1_CRM_Entity"/>
	<rdf:type rdf:resource="http://www.cidoc-crm.org/cidoc-crm/E20_Biological_Object"/>
	<rdf:type rdf:resource="http://www.cidoc-crm.org/cidoc-crm/E21_Person"/>
	<rdf:type rdf:resource="http://www.cidoc-crm.org/cidoc-crm/E39_Actor"/>
	<rdf:type rdf:resource="http://www.cidoc-crm.org/cidoc-crm/E70_Thing"/>
	<rdf:type rdf:resource="http://www.cidoc-crm.org/cidoc-crm/E72_Legal_Object"/>
	<rdf:type rdf:resource="http://www.cidoc-crm.org/cidoc-crm/E77_Persistent_Item"/>
	<rdf:type rdf:resource="http://www.loa-cnr.it/ontologies/DOLCE-Lite#endurant"/>
	<rdf:type rdf:resource="http://www.w3.org/2004/02/skos/core#Concept"/>
	<skos:closeMatch rdf:resource="http://academictourism.com/entity/PER0014"/>
	<skos:closeMatch rdf:resource="http://viaf.org/viaf/185047668"/>
	<skos:exactMatch rdf:resource="http://academictourism.com/entity/PER0014"/>
	<skos:exactMatch rdf:resource="http://viaf.org/viaf/185047668"/>
	<skos:mappingRelation rdf:resource="http://academictourism.com/entity/PER0014"/>
	<skos:mappingRelation rdf:resource="http://viaf.org/viaf/185047668"/>
	<skos:semanticRelation rdf:resource="http://academictourism.com/entity/PER0014"/>
	<skos:semanticRelation rdf:resource="http://viaf.org/viaf/185047668"/>
	<skos:prefLabel>Döring, Johann Wilhelm 1760-1815</skos:prefLabel>
</rdf:Description>

<rdf:Description rdf:about="http://viaf.org/viaf/24668261">
	<rdf:type rdf:resource="http://www.w3.org/2002/07/owl#NamedIndividual"/>
	<rdf:type rdf:resource="http://www.cidoc-crm.org/cidoc-crm/E18_Physical_Thing"/>
	<rdf:type rdf:resource="http://www.cidoc-crm.org/cidoc-crm/E19_Physical_Object"/>
	<rdf:type rdf:resource="http://www.cidoc-crm.org/cidoc-crm/E1_CRM_Entity"/>
	<rdf:type rdf:resource="http://www.cidoc-crm.org/cidoc-crm/E20_Biological_Object"/>
	<rdf:type rdf:resource="http://www.cidoc-crm.org/cidoc-crm/E21_Person"/>
	<rdf:type rdf:resource="http://www.cidoc-crm.org/cidoc-crm/E39_Actor"/>
	<rdf:type rdf:resource="http://www.cidoc-crm.org/cidoc-crm/E70_Thing"/>
	<rdf:type rdf:resource="http://www.cidoc-crm.org/cidoc-crm/E72_Legal_Object"/>
	<rdf:type rdf:resource="http://www.cidoc-crm.org/cidoc-crm/E77_Persistent_Item"/>
	<rdf:type rdf:resource="http://www.loa-cnr.it/ontologies/DOLCE-Lite#endurant"/>
	<rdf:type rdf:resource="http://www.w3.org/2004/02/skos/core#Concept"/>
	<skos:closeMatch rdf:resource="http://academictourism.com/entity/PER0005"/>
	<skos:closeMatch rdf:resource="http://viaf.org/viaf/24668261"/>
	<skos:exactMatch rdf:resource="http://academictourism.com/entity/PER0005"/>
	<skos:exactMatch rdf:resource="http://viaf.org/viaf/24668261"/>
	<skos:mappingRelation rdf:resource="http://academictourism.com/entity/PER0005"/>
	<skos:mappingRelation rdf:resource="http://viaf.org/viaf/24668261"/>
	<skos:semanticRelation rdf:resource="http://academictourism.com/entity/PER0005"/>
	<skos:semanticRelation rdf:resource="http://viaf.org/viaf/24668261"/>
	<skos:prefLabel>Hugo, Gustav, 1764-1844</skos:prefLabel>
</rdf:Description>

<rdf:Description rdf:about="http://viaf.org/viaf/4936996">
	<rdf:type rdf:resource="http://www.w3.org/2002/07/owl#NamedIndividual"/>
	<rdf:type rdf:resource="http://www.cidoc-crm.org/cidoc-crm/E18_Physical_Thing"/>
	<rdf:type rdf:resource="http://www.cidoc-crm.org/cidoc-crm/E19_Physical_Object"/>
	<rdf:type rdf:resource="http://www.cidoc-crm.org/cidoc-crm/E1_CRM_Entity"/>
	<rdf:type rdf:resource="http://www.cidoc-crm.org/cidoc-crm/E20_Biological_Object"/>
	<rdf:type rdf:resource="http://www.cidoc-crm.org/cidoc-crm/E21_Person"/>
	<rdf:type rdf:resource="http://www.cidoc-crm.org/cidoc-crm/E39_Actor"/>
	<rdf:type rdf:resource="http://www.cidoc-crm.org/cidoc-crm/E70_Thing"/>
	<rdf:type rdf:resource="http://www.cidoc-crm.org/cidoc-crm/E72_Legal_Object"/>
	<rdf:type rdf:resource="http://www.cidoc-crm.org/cidoc-crm/E77_Persistent_Item"/>
	<rdf:type rdf:resource="http://www.loa-cnr.it/ontologies/DOLCE-Lite#endurant"/>
	<rdf:type rdf:resource="http://www.w3.org/2004/02/skos/core#Concept"/>
	<skos:closeMatch rdf:resource="http://academictourism.com/entity/PER0013"/>
	<skos:closeMatch rdf:resource="http://viaf.org/viaf/4936996"/>
	<skos:exactMatch rdf:resource="http://academictourism.com/entity/PER0013"/>
	<skos:exactMatch rdf:resource="http://viaf.org/viaf/4936996"/>
	<skos:mappingRelation rdf:resource="http://academictourism.com/entity/PER0013"/>
	<skos:mappingRelation rdf:resource="http://viaf.org/viaf/4936996"/>
	<skos:semanticRelation rdf:resource="http://academictourism.com/entity/PER0013"/>
	<skos:semanticRelation rdf:resource="http://viaf.org/viaf/4936996"/>
	<skos:prefLabel>Tasso, Torquato, 1544-1595</skos:prefLabel>
</rdf:Description>

<rdf:Description rdf:about="http://viaf.org/viaf/61536450">
	<rdf:type rdf:resource="http://www.w3.org/2002/07/owl#NamedIndividual"/>
	<rdf:type rdf:resource="http://www.cidoc-crm.org/cidoc-crm/E18_Physical_Thing"/>
	<rdf:type rdf:resource="http://www.cidoc-crm.org/cidoc-crm/E19_Physical_Object"/>
	<rdf:type rdf:resource="http://www.cidoc-crm.org/cidoc-crm/E1_CRM_Entity"/>
	<rdf:type rdf:resource="http://www.cidoc-crm.org/cidoc-crm/E20_Biological_Object"/>
	<rdf:type rdf:resource="http://www.cidoc-crm.org/cidoc-crm/E21_Person"/>
	<rdf:type rdf:resource="http://www.cidoc-crm.org/cidoc-crm/E39_Actor"/>
	<rdf:type rdf:resource="http://www.cidoc-crm.org/cidoc-crm/E70_Thing"/>
	<rdf:type rdf:resource="http://www.cidoc-crm.org/cidoc-crm/E72_Legal_Object"/>
	<rdf:type rdf:resource="http://www.cidoc-crm.org/cidoc-crm/E77_Persistent_Item"/>
	<rdf:type rdf:resource="http://www.loa-cnr.it/ontologies/DOLCE-Lite#endurant"/>
	<rdf:type rdf:resource="http://www.w3.org/2004/02/skos/core#Concept"/>
	<skos:closeMatch rdf:resource="http://academictourism.com/entity/PER0009"/>
	<skos:closeMatch rdf:resource="http://viaf.org/viaf/61536450"/>
	<skos:exactMatch rdf:resource="http://academictourism.com/entity/PER0009"/>
	<skos:exactMatch rdf:resource="http://viaf.org/viaf/61536450"/>
	<skos:mappingRelation rdf:resource="http://academictourism.com/entity/PER0009"/>
	<skos:mappingRelation rdf:resource="http://viaf.org/viaf/61536450"/>
	<skos:semanticRelation rdf:resource="http://academictourism.com/entity/PER0009"/>
	<skos:semanticRelation rdf:resource="http://viaf.org/viaf/61536450"/>
	<skos:prefLabel>Tischbein, Johann Heinrich Wilhelm, 1751-1829</skos:prefLabel>
</rdf:Description>

<rdf:Description rdf:about="http://viaf.org/viaf/71547594">
	<rdf:type rdf:resource="http://www.w3.org/2002/07/owl#NamedIndividual"/>
	<rdf:type rdf:resource="http://www.cidoc-crm.org/cidoc-crm/E18_Physical_Thing"/>
	<rdf:type rdf:resource="http://www.cidoc-crm.org/cidoc-crm/E19_Physical_Object"/>
	<rdf:type rdf:resource="http://www.cidoc-crm.org/cidoc-crm/E1_CRM_Entity"/>
	<rdf:type rdf:resource="http://www.cidoc-crm.org/cidoc-crm/E20_Biological_Object"/>
	<rdf:type rdf:resource="http://www.cidoc-crm.org/cidoc-crm/E21_Person"/>
	<rdf:type rdf:resource="http://www.cidoc-crm.org/cidoc-crm/E39_Actor"/>
	<rdf:type rdf:resource="http://www.cidoc-crm.org/cidoc-crm/E70_Thing"/>
	<rdf:type rdf:resource="http://www.cidoc-crm.org/cidoc-crm/E72_Legal_Object"/>
	<rdf:type rdf:resource="http://www.cidoc-crm.org/cidoc-crm/E77_Persistent_Item"/>
	<rdf:type rdf:resource="http://www.loa-cnr.it/ontologies/DOLCE-Lite#endurant"/>
	<rdf:type rdf:resource="http://www.w3.org/2004/02/skos/core#Concept"/>
	<skos:closeMatch rdf:resource="http://academictourism.com/entity/PER0006"/>
	<skos:closeMatch rdf:resource="http://viaf.org/viaf/71547594"/>
	<skos:exactMatch rdf:resource="http://academictourism.com/entity/PER0006"/>
	<skos:exactMatch rdf:resource="http://viaf.org/viaf/71547594"/>
	<skos:mappingRelation rdf:resource="http://academictourism.com/entity/PER0006"/>
	<skos:mappingRelation rdf:resource="http://viaf.org/viaf/71547594"/>
	<skos:semanticRelation rdf:resource="http://academictourism.com/entity/PER0006"/>
	<skos:semanticRelation rdf:resource="http://viaf.org/viaf/71547594"/>
	<skos:prefLabel>Heeren, Arnold Hermann Ludwig, 1760-1842</skos:prefLabel>
</rdf:Description>

<rdf:Description rdf:about="http://viaf.org/viaf/71570755">
	<rdf:type rdf:resource="http://www.w3.org/2002/07/owl#NamedIndividual"/>
	<rdf:type rdf:resource="http://www.cidoc-crm.org/cidoc-crm/E18_Physical_Thing"/>
	<rdf:type rdf:resource="http://www.cidoc-crm.org/cidoc-crm/E19_Physical_Object"/>
	<rdf:type rdf:resource="http://www.cidoc-crm.org/cidoc-crm/E1_CRM_Entity"/>
	<rdf:type rdf:resource="http://www.cidoc-crm.org/cidoc-crm/E20_Biological_Object"/>
	<rdf:type rdf:resource="http://www.cidoc-crm.org/cidoc-crm/E21_Person"/>
	<rdf:type rdf:resource="http://www.cidoc-crm.org/cidoc-crm/E39_Actor"/>
	<rdf:type rdf:resource="http://www.cidoc-crm.org/cidoc-crm/E70_Thing"/>
	<rdf:type rdf:resource="http://www.cidoc-crm.org/cidoc-crm/E72_Legal_Object"/>
	<rdf:type rdf:resource="http://www.cidoc-crm.org/cidoc-crm/E77_Persistent_Item"/>
	<rdf:type rdf:resource="http://www.loa-cnr.it/ontologies/DOLCE-Lite#endurant"/>
	<rdf:type rdf:resource="http://www.w3.org/2004/02/skos/core#Concept"/>
	<skos:closeMatch rdf:resource="http://academictourism.com/entity/PER0008"/>
	<skos:closeMatch rdf:resource="http://viaf.org/viaf/71570755"/>
	<skos:exactMatch rdf:resource="http://academictourism.com/entity/PER0008"/>
	<skos:exactMatch rdf:resource="http://viaf.org/viaf/71570755"/>
	<skos:mappingRelation rdf:resource="http://academictourism.com/entity/PER0008"/>
	<skos:mappingRelation rdf:resource="http://viaf.org/viaf/71570755"/>
	<skos:semanticRelation rdf:resource="http://academictourism.com/entity/PER0008"/>
	<skos:semanticRelation rdf:resource="http://viaf.org/viaf/71570755"/>
	<skos:prefLabel>Blumenbach, Johann Friedrich, 1752-1840</skos:prefLabel>
</rdf:Description>

<rdf:Description rdf:about="http://viaf.org/viaf/9856912">
	<rdf:type rdf:resource="http://www.w3.org/2002/07/owl#NamedIndividual"/>
	<rdf:type rdf:resource="http://www.w3.org/2004/02/skos/core#Concept"/>
	<skos:closeMatch rdf:resource="http://academictourism.com/entity/PER0010"/>
	<skos:closeMatch rdf:resource="http://viaf.org/viaf/9856912"/>
	<skos:exactMatch rdf:resource="http://academictourism.com/entity/PER0010"/>
	<skos:exactMatch rdf:resource="http://viaf.org/viaf/9856912"/>
	<skos:mappingRelation rdf:resource="http://academictourism.com/entity/PER0010"/>
	<skos:mappingRelation rdf:resource="http://viaf.org/viaf/9856912"/>
	<skos:semanticRelation rdf:resource="http://academictourism.com/entity/PER0010"/>
	<skos:semanticRelation rdf:resource="http://viaf.org/viaf/9856912"/>
	<skos:prefLabel>Wieland, Christoph Martin, 1733-1813</skos:prefLabel>
</rdf:Description>

<rdf:Description rdf:about="http://vocab.getty.edu/page/aat/300000348">
	<rdf:type rdf:resource="http://www.w3.org/2002/07/owl#NamedIndividual"/>
	<rdf:type rdf:resource="http://www.cidoc-crm.org/cidoc-crm/E1_CRM_Entity"/>
	<rdf:type rdf:resource="http://www.cidoc-crm.org/cidoc-crm/E28_Conceptual_Object"/>
	<rdf:type rdf:resource="http://www.cidoc-crm.org/cidoc-crm/E55_Type"/>
	<rdf:type rdf:resource="http://www.cidoc-crm.org/cidoc-crm/E70_Thing"/>
	<rdf:type rdf:resource="http://www.cidoc-crm.org/cidoc-crm/E71_Human-Made_Thing"/>
	<rdf:type rdf:resource="http://www.cidoc-crm.org/cidoc-crm/E77_Persistent_Item"/>
	<rdf:type rdf:resource="http://www.loa-cnr.it/ontologies/DOLCE-Lite#endurant"/>
	<cidoc-crm:P2i_is_type_of rdf:resource="http://academictourism.com/entity/MISC0023"/>
	<skos:prefLabel>zoos (built complexes)</skos:prefLabel>
</rdf:Description>

<rdf:Description rdf:about="http://vocab.getty.edu/page/aat/300004362">
	<rdf:type rdf:resource="http://www.w3.org/2002/07/owl#NamedIndividual"/>
	<rdf:type rdf:resource="http://vocab.getty.edu/page/aat/300004021"/>
	<rdf:type rdf:resource="http://www.cidoc-crm.org/cidoc-crm/E1_CRM_Entity"/>
	<rdf:type rdf:resource="http://www.cidoc-crm.org/cidoc-crm/E28_Conceptual_Object"/>
	<rdf:type rdf:resource="http://www.cidoc-crm.org/cidoc-crm/E55_Type"/>
	<rdf:type rdf:resource="http://www.cidoc-crm.org/cidoc-crm/E70_Thing"/>
	<rdf:type rdf:resource="http://www.cidoc-crm.org/cidoc-crm/E71_Human-Made_Thing"/>
	<rdf:type rdf:resource="http://www.cidoc-crm.org/cidoc-crm/E77_Persistent_Item"/>
	<rdf:type rdf:resource="http://www.loa-cnr.it/ontologies/DOLCE-Lite#endurant"/>
	<cidoc-crm:P2i_is_type_of rdf:resource="http://academictourism.com/entity/LOC0003.CS.K002"/>
	<rdfs:label>sleeping spaces</rdfs:label>
</rdf:Description>

<rdf:Description rdf:about="http://vocab.getty.edu/page/aat/300004433">
	<rdf:type rdf:resource="http://www.w3.org/2002/07/owl#NamedIndividual"/>
	<rdf:type rdf:resource="http://vocab.getty.edu/page/aat/300004021"/>
	<rdf:type rdf:resource="http://www.cidoc-crm.org/cidoc-crm/E1_CRM_Entity"/>
	<rdf:type rdf:resource="http://www.cidoc-crm.org/cidoc-crm/E28_Conceptual_Object"/>
	<rdf:type rdf:resource="http://www.cidoc-crm.org/cidoc-crm/E55_Type"/>
	<rdf:type rdf:resource="http://www.cidoc-crm.org/cidoc-crm/E70_Thing"/>
	<rdf:type rdf:resource="http://www.cidoc-crm.org/cidoc-crm/E71_Human-Made_Thing"/>
	<rdf:type rdf:resource="http://www.cidoc-crm.org/cidoc-crm/E77_Persistent_Item"/>
	<rdf:type rdf:resource="http://www.loa-cnr.it/ontologies/DOLCE-Lite#endurant"/>
	<cidoc-crm:P2i_is_type_of rdf:resource="http://academictourism.com/entity/LOC0003.CS.K003"/>
	<cidoc-crm:P2i_is_type_of rdf:resource="http://academictourism.com/entity/LOC0007.KM001"/>
	<rdfs:label>libraries</rdfs:label>
</rdf:Description>

<rdf:Description rdf:about="http://vocab.getty.edu/page/aat/300005665">
	<rdf:type rdf:resource="http://www.w3.org/2002/07/owl#NamedIndividual"/>
	<rdf:type rdf:resource="http://www.cidoc-crm.org/cidoc-crm/E1_CRM_Entity"/>
	<rdf:type rdf:resource="http://www.cidoc-crm.org/cidoc-crm/E28_Conceptual_Object"/>
	<rdf:type rdf:resource="http://www.cidoc-crm.org/cidoc-crm/E55_Type"/>
	<rdf:type rdf:resource="http://www.cidoc-crm.org/cidoc-crm/E70_Thing"/>
	<rdf:type rdf:resource="http://www.cidoc-crm.org/cidoc-crm/E71_Human-Made_Thing"/>
	<rdf:type rdf:resource="http://www.cidoc-crm.org/cidoc-crm/E77_Persistent_Item"/>
	<rdf:type rdf:resource="http://www.loa-cnr.it/ontologies/DOLCE-Lite#endurant"/>
	<cidoc-crm:P2i_is_type_of rdf:resource="http://academictourism.com/entity/MISC0001"/>
	<rdfs:label>barracks</rdfs:label>
</rdf:Description>

<rdf:Description rdf:about="http://vocab.getty.edu/page/aat/300005907">
	<rdf:type rdf:resource="http://www.w3.org/2002/07/owl#NamedIndividual"/>
	<rdf:type rdf:resource="http://www.cidoc-crm.org/cidoc-crm/E1_CRM_Entity"/>
	<rdf:type rdf:resource="http://www.cidoc-crm.org/cidoc-crm/E28_Conceptual_Object"/>
	<rdf:type rdf:resource="http://www.cidoc-crm.org/cidoc-crm/E55_Type"/>
	<rdf:type rdf:resource="http://www.cidoc-crm.org/cidoc-crm/E70_Thing"/>
	<rdf:type rdf:resource="http://www.cidoc-crm.org/cidoc-crm/E71_Human-Made_Thing"/>
	<rdf:type rdf:resource="http://www.cidoc-crm.org/cidoc-crm/E77_Persistent_Item"/>
	<rdf:type rdf:resource="http://www.loa-cnr.it/ontologies/DOLCE-Lite#endurant"/>
	<cidoc-crm:P2i_is_type_of rdf:resource="http://academictourism.com/entity/MISC0014"/>
	<rdfs:label>graves</rdfs:label>
</rdf:Description>

<rdf:Description rdf:about="http://vocab.getty.edu/page/aat/300006179">
	<rdf:type rdf:resource="http://www.w3.org/2002/07/owl#NamedIndividual"/>
	<rdf:type rdf:resource="http://www.cidoc-crm.org/cidoc-crm/E1_CRM_Entity"/>
	<rdf:type rdf:resource="http://www.cidoc-crm.org/cidoc-crm/E28_Conceptual_Object"/>
	<rdf:type rdf:resource="http://www.cidoc-crm.org/cidoc-crm/E55_Type"/>
	<rdf:type rdf:resource="http://www.cidoc-crm.org/cidoc-crm/E70_Thing"/>
	<rdf:type rdf:resource="http://www.cidoc-crm.org/cidoc-crm/E71_Human-Made_Thing"/>
	<rdf:type rdf:resource="http://www.cidoc-crm.org/cidoc-crm/E77_Persistent_Item"/>
	<rdf:type rdf:resource="http://www.loa-cnr.it/ontologies/DOLCE-Lite#endurant"/>
	<cidoc-crm:P2i_is_type_of rdf:resource="http://academictourism.com/entity/MISC0010"/>
	<rdfs:label>fountains</rdfs:label>
</rdf:Description>

<rdf:Description rdf:about="http://vocab.getty.edu/page/aat/300006215">
	<rdf:type rdf:resource="http://www.w3.org/2002/07/owl#NamedIndividual"/>
	<rdf:type rdf:resource="http://www.cidoc-crm.org/cidoc-crm/E1_CRM_Entity"/>
	<rdf:type rdf:resource="http://www.cidoc-crm.org/cidoc-crm/E28_Conceptual_Object"/>
	<rdf:type rdf:resource="http://www.cidoc-crm.org/cidoc-crm/E55_Type"/>
	<rdf:type rdf:resource="http://www.cidoc-crm.org/cidoc-crm/E70_Thing"/>
	<rdf:type rdf:resource="http://www.cidoc-crm.org/cidoc-crm/E71_Human-Made_Thing"/>
	<rdf:type rdf:resource="http://www.cidoc-crm.org/cidoc-crm/E77_Persistent_Item"/>
	<rdf:type rdf:resource="http://www.loa-cnr.it/ontologies/DOLCE-Lite#endurant"/>
	<cidoc-crm:P2i_is_type_of rdf:resource="http://academictourism.com/entity/MISC0008"/>
	<rdfs:comment>waterworks</rdfs:comment>
</rdf:Description>

<rdf:Description rdf:about="http://vocab.getty.edu/page/aat/300006792">
	<rdf:type rdf:resource="http://www.w3.org/2002/07/owl#NamedIndividual"/>
	<rdf:type rdf:resource="http://www.cidoc-crm.org/cidoc-crm/E1_CRM_Entity"/>
	<rdf:type rdf:resource="http://www.cidoc-crm.org/cidoc-crm/E28_Conceptual_Object"/>
	<rdf:type rdf:resource="http://www.cidoc-crm.org/cidoc-crm/E55_Type"/>
	<rdf:type rdf:resource="http://www.cidoc-crm.org/cidoc-crm/E70_Thing"/>
	<rdf:type rdf:resource="http://www.cidoc-crm.org/cidoc-crm/E71_Human-Made_Thing"/>
	<rdf:type rdf:resource="http://www.cidoc-crm.org/cidoc-crm/E77_Persistent_Item"/>
	<rdf:type rdf:resource="http://www.loa-cnr.it/ontologies/DOLCE-Lite#endurant"/>
	<cidoc-crm:P2i_is_type_of rdf:resource="http://academictourism.com/entity/MISC0012"/>
	<rdfs:label>cascades (water features)</rdfs:label>
</rdf:Description>

<rdf:Description rdf:about="http://vocab.getty.edu/page/aat/300007117">
	<rdf:type rdf:resource="http://www.w3.org/2002/07/owl#NamedIndividual"/>
	<rdf:type rdf:resource="http://www.cidoc-crm.org/cidoc-crm/E1_CRM_Entity"/>
	<rdf:type rdf:resource="http://www.cidoc-crm.org/cidoc-crm/E28_Conceptual_Object"/>
	<rdf:type rdf:resource="http://www.cidoc-crm.org/cidoc-crm/E55_Type"/>
	<rdf:type rdf:resource="http://www.cidoc-crm.org/cidoc-crm/E70_Thing"/>
	<rdf:type rdf:resource="http://www.cidoc-crm.org/cidoc-crm/E71_Human-Made_Thing"/>
	<rdf:type rdf:resource="http://www.cidoc-crm.org/cidoc-crm/E77_Persistent_Item"/>
	<rdf:type rdf:resource="http://www.loa-cnr.it/ontologies/DOLCE-Lite#endurant"/>
	<cidoc-crm:P2i_is_type_of rdf:resource="http://academictourism.com/entity/MISC0013"/>
	<rdfs:label>theaters</rdfs:label>
</rdf:Description>

<rdf:Description rdf:about="http://vocab.getty.edu/page/aat/300007170">
	<rdf:type rdf:resource="http://www.w3.org/2002/07/owl#NamedIndividual"/>
	<rdf:type rdf:resource="http://www.cidoc-crm.org/cidoc-crm/E1_CRM_Entity"/>
	<rdf:type rdf:resource="http://www.cidoc-crm.org/cidoc-crm/E28_Conceptual_Object"/>
	<rdf:type rdf:resource="http://www.cidoc-crm.org/cidoc-crm/E55_Type"/>
	<rdf:type rdf:resource="http://www.cidoc-crm.org/cidoc-crm/E70_Thing"/>
	<rdf:type rdf:resource="http://www.cidoc-crm.org/cidoc-crm/E71_Human-Made_Thing"/>
	<rdf:type rdf:resource="http://www.cidoc-crm.org/cidoc-crm/E77_Persistent_Item"/>
	<rdf:type rdf:resource="http://www.loa-cnr.it/ontologies/DOLCE-Lite#endurant"/>
	<cidoc-crm:P2i_is_type_of rdf:resource="http://academictourism.com/entity/LOC0008"/>
	<rdfs:comment>inns</rdfs:comment>
</rdf:Description>

<rdf:Description rdf:about="http://vocab.getty.edu/page/aat/300007595">
	<rdf:type rdf:resource="http://www.w3.org/2002/07/owl#NamedIndividual"/>
	<rdf:type rdf:resource="http://www.cidoc-crm.org/cidoc-crm/E1_CRM_Entity"/>
	<rdf:type rdf:resource="http://www.cidoc-crm.org/cidoc-crm/E28_Conceptual_Object"/>
	<rdf:type rdf:resource="http://www.cidoc-crm.org/cidoc-crm/E55_Type"/>
	<rdf:type rdf:resource="http://www.cidoc-crm.org/cidoc-crm/E70_Thing"/>
	<rdf:type rdf:resource="http://www.cidoc-crm.org/cidoc-crm/E71_Human-Made_Thing"/>
	<rdf:type rdf:resource="http://www.cidoc-crm.org/cidoc-crm/E77_Persistent_Item"/>
	<rdf:type rdf:resource="http://www.loa-cnr.it/ontologies/DOLCE-Lite#endurant"/>
	<cidoc-crm:P2i_is_type_of rdf:resource="http://academictourism.com/entity/MISC0015"/>
	<cidoc-crm:P2i_is_type_of rdf:resource="http://academictourism.com/entity/MISC0016"/>
	<rdfs:label>temples</rdfs:label>
</rdf:Description>

<rdf:Description rdf:about="http://vocab.getty.edu/page/aat/300008746">
	<rdf:type rdf:resource="http://www.w3.org/2002/07/owl#NamedIndividual"/>
	<rdf:type rdf:resource="http://www.cidoc-crm.org/cidoc-crm/E1_CRM_Entity"/>
	<rdf:type rdf:resource="http://www.cidoc-crm.org/cidoc-crm/E28_Conceptual_Object"/>
	<rdf:type rdf:resource="http://www.cidoc-crm.org/cidoc-crm/E55_Type"/>
	<rdf:type rdf:resource="http://www.cidoc-crm.org/cidoc-crm/E70_Thing"/>
	<rdf:type rdf:resource="http://www.cidoc-crm.org/cidoc-crm/E71_Human-Made_Thing"/>
	<rdf:type rdf:resource="http://www.cidoc-crm.org/cidoc-crm/E77_Persistent_Item"/>
	<rdf:type rdf:resource="http://www.loa-cnr.it/ontologies/DOLCE-Lite#endurant"/>
	<cidoc-crm:P2i_is_type_of rdf:resource="http://academictourism.com/entity/MISC0017"/>
	<rdfs:label>caves</rdfs:label>
</rdf:Description>

<rdf:Description rdf:about="http://vocab.getty.edu/page/aat/300015637">
	<rdf:type rdf:resource="http://www.w3.org/2002/07/owl#NamedIndividual"/>
	<rdf:type rdf:resource="http://www.cidoc-crm.org/cidoc-crm/E1_CRM_Entity"/>
	<rdf:type rdf:resource="http://www.cidoc-crm.org/cidoc-crm/E28_Conceptual_Object"/>
	<rdf:type rdf:resource="http://www.cidoc-crm.org/cidoc-crm/E55_Type"/>
	<rdf:type rdf:resource="http://www.cidoc-crm.org/cidoc-crm/E70_Thing"/>
	<rdf:type rdf:resource="http://www.cidoc-crm.org/cidoc-crm/E71_Human-Made_Thing"/>
	<rdf:type rdf:resource="http://www.cidoc-crm.org/cidoc-crm/E77_Persistent_Item"/>
	<rdf:type rdf:resource="http://www.loa-cnr.it/ontologies/DOLCE-Lite#endurant"/>
	<cidoc-crm:P2i_is_type_of rdf:resource="http://academictourism.com/entity/MISC0006"/>
	<rdfs:label>portraits</rdfs:label>
</rdf:Description>

<rdf:Description rdf:about="http://vocab.getty.edu/page/aat/300025136">
	<rdf:type rdf:resource="http://www.w3.org/2002/07/owl#NamedIndividual"/>
	<rdf:type rdf:resource="http://academictourism.com/academictourism#Character_Type"/>
	<rdf:type rdf:resource="http://www.cidoc-crm.org/cidoc-crm/E1_CRM_Entity"/>
	<rdf:type rdf:resource="http://www.cidoc-crm.org/cidoc-crm/E28_Conceptual_Object"/>
	<rdf:type rdf:resource="http://www.cidoc-crm.org/cidoc-crm/E55_Type"/>
	<rdf:type rdf:resource="http://www.cidoc-crm.org/cidoc-crm/E70_Thing"/>
	<rdf:type rdf:resource="http://www.cidoc-crm.org/cidoc-crm/E71_Human-Made_Thing"/>
	<rdf:type rdf:resource="http://www.cidoc-crm.org/cidoc-crm/E77_Persistent_Item"/>
	<rdf:type rdf:resource="http://www.loa-cnr.it/ontologies/DOLCE-Lite#endurant"/>
	<cidoc-crm:P2i_is_type_of rdf:resource="http://academictourism.com/entity/PER0009"/>
	<rdfs:label>painters</rdfs:label>
</rdf:Description>

<rdf:Description rdf:about="http://vocab.getty.edu/page/aat/300025492">
	<rdf:type rdf:resource="http://www.w3.org/2002/07/owl#NamedIndividual"/>
	<rdf:type rdf:resource="http://academictourism.com/academictourism#Character_Type"/>
	<rdf:type rdf:resource="http://www.cidoc-crm.org/cidoc-crm/E1_CRM_Entity"/>
	<rdf:type rdf:resource="http://www.cidoc-crm.org/cidoc-crm/E28_Conceptual_Object"/>
	<rdf:type rdf:resource="http://www.cidoc-crm.org/cidoc-crm/E55_Type"/>
	<rdf:type rdf:resource="http://www.cidoc-crm.org/cidoc-crm/E70_Thing"/>
	<rdf:type rdf:resource="http://www.cidoc-crm.org/cidoc-crm/E71_Human-Made_Thing"/>
	<rdf:type rdf:resource="http://www.cidoc-crm.org/cidoc-crm/E77_Persistent_Item"/>
	<rdf:type rdf:resource="http://www.loa-cnr.it/ontologies/DOLCE-Lite#endurant"/>
	<cidoc-crm:P2i_is_type_of rdf:resource="http://academictourism.com/entity/PER0001"/>
	<rdfs:label>authors</rdfs:label>
</rdf:Description>

<rdf:Description rdf:about="http://vocab.getty.edu/page/aat/300025533">
	<rdf:type rdf:resource="http://www.w3.org/2002/07/owl#NamedIndividual"/>
	<rdf:type rdf:resource="http://academictourism.com/academictourism#Character_Type"/>
	<rdf:type rdf:resource="http://www.cidoc-crm.org/cidoc-crm/E1_CRM_Entity"/>
	<rdf:type rdf:resource="http://www.cidoc-crm.org/cidoc-crm/E28_Conceptual_Object"/>
	<rdf:type rdf:resource="http://www.cidoc-crm.org/cidoc-crm/E55_Type"/>
	<rdf:type rdf:resource="http://www.cidoc-crm.org/cidoc-crm/E70_Thing"/>
	<rdf:type rdf:resource="http://www.cidoc-crm.org/cidoc-crm/E71_Human-Made_Thing"/>
	<rdf:type rdf:resource="http://www.cidoc-crm.org/cidoc-crm/E77_Persistent_Item"/>
	<rdf:type rdf:resource="http://www.loa-cnr.it/ontologies/DOLCE-Lite#endurant"/>
	<cidoc-crm:P2i_is_type_of rdf:resource="http://academictourism.com/entity/PER0005"/>
	<cidoc-crm:P2i_is_type_of rdf:resource="http://academictourism.com/entity/PER0006"/>
	<cidoc-crm:P2i_is_type_of rdf:resource="http://academictourism.com/entity/PER0007"/>
	<cidoc-crm:P2i_is_type_of rdf:resource="http://academictourism.com/entity/PER0008"/>
	<rdfs:label>professors</rdfs:label>
</rdf:Description>

<rdf:Description rdf:about="http://vocab.getty.edu/page/aat/300025879">
	<rdf:type rdf:resource="http://www.w3.org/2002/07/owl#NamedIndividual"/>
	<rdf:type rdf:resource="http://academictourism.com/academictourism#Character_Type"/>
	<rdf:type rdf:resource="http://www.cidoc-crm.org/cidoc-crm/E1_CRM_Entity"/>
	<rdf:type rdf:resource="http://www.cidoc-crm.org/cidoc-crm/E28_Conceptual_Object"/>
	<rdf:type rdf:resource="http://www.cidoc-crm.org/cidoc-crm/E55_Type"/>
	<rdf:type rdf:resource="http://www.cidoc-crm.org/cidoc-crm/E70_Thing"/>
	<rdf:type rdf:resource="http://www.cidoc-crm.org/cidoc-crm/E71_Human-Made_Thing"/>
	<rdf:type rdf:resource="http://www.cidoc-crm.org/cidoc-crm/E77_Persistent_Item"/>
	<rdf:type rdf:resource="http://www.loa-cnr.it/ontologies/DOLCE-Lite#endurant"/>
	<cidoc-crm:P2i_is_type_of rdf:resource="http://academictourism.com/entity/PER0001"/>
	<cidoc-crm:P2i_is_type_of rdf:resource="http://academictourism.com/entity/PER0002"/>
	<cidoc-crm:P2i_is_type_of rdf:resource="http://academictourism.com/entity/PER0003"/>
	<cidoc-crm:P2i_is_type_of rdf:resource="http://academictourism.com/entity/PER0004"/>
	<rdfs:label>travelers</rdfs:label>
</rdf:Description>

<rdf:Description rdf:about="http://vocab.getty.edu/page/aat/300025909">
	<rdf:type rdf:resource="http://www.w3.org/2002/07/owl#NamedIndividual"/>
	<rdf:type rdf:resource="http://academictourism.com/academictourism#Character_Type"/>
	<rdf:type rdf:resource="http://www.cidoc-crm.org/cidoc-crm/E1_CRM_Entity"/>
	<rdf:type rdf:resource="http://www.cidoc-crm.org/cidoc-crm/E28_Conceptual_Object"/>
	<rdf:type rdf:resource="http://www.cidoc-crm.org/cidoc-crm/E55_Type"/>
	<rdf:type rdf:resource="http://www.cidoc-crm.org/cidoc-crm/E70_Thing"/>
	<rdf:type rdf:resource="http://www.cidoc-crm.org/cidoc-crm/E71_Human-Made_Thing"/>
	<rdf:type rdf:resource="http://www.cidoc-crm.org/cidoc-crm/E77_Persistent_Item"/>
	<rdf:type rdf:resource="http://www.loa-cnr.it/ontologies/DOLCE-Lite#endurant"/>
	<cidoc-crm:P2i_is_type_of rdf:resource="http://academictourism.com/entity/PER0002"/>
	<rdfs:label>students</rdfs:label>
</rdf:Description>

<rdf:Description rdf:about="http://vocab.getty.edu/page/aat/300026673">
	<rdf:type rdf:resource="http://www.w3.org/2002/07/owl#NamedIndividual"/>
	<rdf:type rdf:resource="http://www.cidoc-crm.org/cidoc-crm/E1_CRM_Entity"/>
	<rdf:type rdf:resource="http://www.cidoc-crm.org/cidoc-crm/E28_Conceptual_Object"/>
	<rdf:type rdf:resource="http://www.cidoc-crm.org/cidoc-crm/E55_Type"/>
	<rdf:type rdf:resource="http://www.cidoc-crm.org/cidoc-crm/E70_Thing"/>
	<rdf:type rdf:resource="http://www.cidoc-crm.org/cidoc-crm/E71_Human-Made_Thing"/>
	<rdf:type rdf:resource="http://www.cidoc-crm.org/cidoc-crm/E77_Persistent_Item"/>
	<rdf:type rdf:resource="http://www.loa-cnr.it/ontologies/DOLCE-Lite#endurant"/>
	<cidoc-crm:P2i_is_type_of rdf:resource="http://academictourism.com/entity/BRF0005.RS.L0001"/>
	<cidoc-crm:P2i_is_type_of rdf:resource="http://academictourism.com/entity/BRF0005.RS.L0002"/>
	<cidoc-crm:P2i_is_type_of rdf:resource="http://academictourism.com/entity/BRF0005.RS.L0003"/>
	<cidoc-crm:P2i_is_type_of rdf:resource="http://academictourism.com/entity/BRF0005.RS.L0004"/>
	<rdfs:label>lectures</rdfs:label>
</rdf:Description>

<rdf:Description rdf:about="http://vocab.getty.edu/page/aat/300033618">
	<rdf:type rdf:resource="http://www.w3.org/2002/07/owl#NamedIndividual"/>
	<rdf:type rdf:resource="http://www.cidoc-crm.org/cidoc-crm/E1_CRM_Entity"/>
	<rdf:type rdf:resource="http://www.cidoc-crm.org/cidoc-crm/E28_Conceptual_Object"/>
	<rdf:type rdf:resource="http://www.cidoc-crm.org/cidoc-crm/E55_Type"/>
	<rdf:type rdf:resource="http://www.cidoc-crm.org/cidoc-crm/E70_Thing"/>
	<rdf:type rdf:resource="http://www.cidoc-crm.org/cidoc-crm/E71_Human-Made_Thing"/>
	<rdf:type rdf:resource="http://www.cidoc-crm.org/cidoc-crm/E77_Persistent_Item"/>
	<rdf:type rdf:resource="http://www.loa-cnr.it/ontologies/DOLCE-Lite#endurant"/>
	<cidoc-crm:P2i_is_type_of rdf:resource="http://academictourism.com/entity/MISC0003"/>
	<rdfs:label>paintings</rdfs:label>
</rdf:Description>

<rdf:Description rdf:about="http://vocab.getty.edu/page/aat/300037682">
	<rdf:type rdf:resource="http://www.w3.org/2002/07/owl#NamedIndividual"/>
	<rdf:type rdf:resource="http://www.cidoc-crm.org/cidoc-crm/E1_CRM_Entity"/>
	<rdf:type rdf:resource="http://www.cidoc-crm.org/cidoc-crm/E28_Conceptual_Object"/>
	<rdf:type rdf:resource="http://www.cidoc-crm.org/cidoc-crm/E55_Type"/>
	<rdf:type rdf:resource="http://www.cidoc-crm.org/cidoc-crm/E70_Thing"/>
	<rdf:type rdf:resource="http://www.cidoc-crm.org/cidoc-crm/E71_Human-Made_Thing"/>
	<rdf:type rdf:resource="http://www.cidoc-crm.org/cidoc-crm/E77_Persistent_Item"/>
	<rdf:type rdf:resource="http://www.loa-cnr.it/ontologies/DOLCE-Lite#endurant"/>
	<cidoc-crm:P2i_is_type_of rdf:resource="http://academictourism.com/entity/MISC0002"/>
	<rdfs:label>mirrors</rdfs:label>
</rdf:Description>

<rdf:Description rdf:about="http://vocab.getty.edu/page/aat/300133704">
	<rdf:type rdf:resource="http://www.w3.org/2002/07/owl#NamedIndividual"/>
	<rdf:type rdf:resource="http://vocab.getty.edu/page/aat/300004021"/>
	<rdf:type rdf:resource="http://www.cidoc-crm.org/cidoc-crm/E1_CRM_Entity"/>
	<rdf:type rdf:resource="http://www.cidoc-crm.org/cidoc-crm/E28_Conceptual_Object"/>
	<rdf:type rdf:resource="http://www.cidoc-crm.org/cidoc-crm/E55_Type"/>
	<rdf:type rdf:resource="http://www.cidoc-crm.org/cidoc-crm/E70_Thing"/>
	<rdf:type rdf:resource="http://www.cidoc-crm.org/cidoc-crm/E71_Human-Made_Thing"/>
	<rdf:type rdf:resource="http://www.cidoc-crm.org/cidoc-crm/E77_Persistent_Item"/>
	<rdf:type rdf:resource="http://www.loa-cnr.it/ontologies/DOLCE-Lite#endurant"/>
	<cidoc-crm:P2i_is_type_of rdf:resource="http://academictourism.com/entity/LOC0003.CS.K004"/>
	<rdfs:label>room</rdfs:label>
</rdf:Description>

<rdf:Description rdf:about="http://vocab.getty.edu/page/aat/300137147">
	<rdf:type rdf:resource="http://www.w3.org/2002/07/owl#NamedIndividual"/>
	<rdf:type rdf:resource="http://academictourism.com/academictourism#Character_Type"/>
	<rdf:type rdf:resource="http://www.cidoc-crm.org/cidoc-crm/E1_CRM_Entity"/>
	<rdf:type rdf:resource="http://www.cidoc-crm.org/cidoc-crm/E28_Conceptual_Object"/>
	<rdf:type rdf:resource="http://www.cidoc-crm.org/cidoc-crm/E55_Type"/>
	<rdf:type rdf:resource="http://www.cidoc-crm.org/cidoc-crm/E70_Thing"/>
	<rdf:type rdf:resource="http://www.cidoc-crm.org/cidoc-crm/E71_Human-Made_Thing"/>
	<rdf:type rdf:resource="http://www.cidoc-crm.org/cidoc-crm/E77_Persistent_Item"/>
	<rdf:type rdf:resource="http://www.loa-cnr.it/ontologies/DOLCE-Lite#endurant"/>
	<cidoc-crm:P2i_is_type_of rdf:resource="http://academictourism.com/entity/PER0003"/>
	<rdfs:label>secretaries</rdfs:label>
</rdf:Description>

<rdf:Description rdf:about="http://vocab.getty.edu/page/aat/300205002">
	<rdf:type rdf:resource="http://www.w3.org/2002/07/owl#NamedIndividual"/>
	<rdf:type rdf:resource="http://www.cidoc-crm.org/cidoc-crm/E1_CRM_Entity"/>
	<rdf:type rdf:resource="http://www.cidoc-crm.org/cidoc-crm/E28_Conceptual_Object"/>
	<rdf:type rdf:resource="http://www.cidoc-crm.org/cidoc-crm/E55_Type"/>
	<rdf:type rdf:resource="http://www.cidoc-crm.org/cidoc-crm/E70_Thing"/>
	<rdf:type rdf:resource="http://www.cidoc-crm.org/cidoc-crm/E71_Human-Made_Thing"/>
	<rdf:type rdf:resource="http://www.cidoc-crm.org/cidoc-crm/E77_Persistent_Item"/>
	<rdf:type rdf:resource="http://www.loa-cnr.it/ontologies/DOLCE-Lite#endurant"/>
	<cidoc-crm:P2i_is_type_of rdf:resource="http://academictourism.com/entity/MISC0005"/>
	<rdfs:label>tapestries</rdfs:label>
</rdf:Description>

<rdf:Description rdf:about="http://vocab.getty.edu/page/aat/300240057">
	<rdf:type rdf:resource="http://www.w3.org/2002/07/owl#NamedIndividual"/>
	<rdf:type rdf:resource="http://vocab.getty.edu/page/aat/300004021"/>
	<rdf:type rdf:resource="http://www.cidoc-crm.org/cidoc-crm/E1_CRM_Entity"/>
	<rdf:type rdf:resource="http://www.cidoc-crm.org/cidoc-crm/E28_Conceptual_Object"/>
	<rdf:type rdf:resource="http://www.cidoc-crm.org/cidoc-crm/E55_Type"/>
	<rdf:type rdf:resource="http://www.cidoc-crm.org/cidoc-crm/E70_Thing"/>
	<rdf:type rdf:resource="http://www.cidoc-crm.org/cidoc-crm/E71_Human-Made_Thing"/>
	<rdf:type rdf:resource="http://www.cidoc-crm.org/cidoc-crm/E77_Persistent_Item"/>
	<rdf:type rdf:resource="http://www.loa-cnr.it/ontologies/DOLCE-Lite#endurant"/>
	<cidoc-crm:P2i_is_type_of rdf:resource="http://academictourism.com/entity/LOC0003.CS.K001"/>
	<rdfs:label>galleries</rdfs:label>
</rdf:Description>

<rdf:Description rdf:about="http://vocab.getty.edu/page/aat/300248181">
	<rdf:type rdf:resource="http://www.w3.org/2002/07/owl#NamedIndividual"/>
	<rdf:type rdf:resource="http://academictourism.com/academictourism#Mode_of_Transportation"/>
	<rdf:type rdf:resource="http://www.cidoc-crm.org/cidoc-crm/E1_CRM_Entity"/>
	<rdf:type rdf:resource="http://www.cidoc-crm.org/cidoc-crm/E28_Conceptual_Object"/>
	<rdf:type rdf:resource="http://www.cidoc-crm.org/cidoc-crm/E55_Type"/>
	<rdf:type rdf:resource="http://www.cidoc-crm.org/cidoc-crm/E70_Thing"/>
	<rdf:type rdf:resource="http://www.cidoc-crm.org/cidoc-crm/E71_Human-Made_Thing"/>
	<rdf:type rdf:resource="http://www.cidoc-crm.org/cidoc-crm/E77_Persistent_Item"/>
	<rdf:type rdf:resource="http://www.loa-cnr.it/ontologies/DOLCE-Lite#endurant"/>
	<cidoc-crm:P125i_was_type_of_object_used_in rdf:resource="http://academictourism.com/entity/BRF0004.RS.RS0004.RS0002"/>
	<cidoc-crm:P2i_is_type_of rdf:resource="http://academictourism.com/entity/BRF0004.RS.RS0001"/>
	<cidoc-crm:P32i_was_technique_of rdf:resource="http://academictourism.com/entity/BRF0004.RS.RS0004.RS0002"/>
	<rdfs:label>walking</rdfs:label>
</rdf:Description>

<rdf:Description rdf:about="http://vocab.getty.edu/page/aat/300387598">
	<rdf:type rdf:resource="http://www.w3.org/2002/07/owl#NamedIndividual"/>
	<rdf:type rdf:resource="http://www.cidoc-crm.org/cidoc-crm/E1_CRM_Entity"/>
	<rdf:type rdf:resource="http://www.cidoc-crm.org/cidoc-crm/E28_Conceptual_Object"/>
	<rdf:type rdf:resource="http://www.cidoc-crm.org/cidoc-crm/E55_Type"/>
	<rdf:type rdf:resource="http://www.cidoc-crm.org/cidoc-crm/E70_Thing"/>
	<rdf:type rdf:resource="http://www.cidoc-crm.org/cidoc-crm/E71_Human-Made_Thing"/>
	<rdf:type rdf:resource="http://www.cidoc-crm.org/cidoc-crm/E77_Persistent_Item"/>
	<rdf:type rdf:resource="http://www.loa-cnr.it/ontologies/DOLCE-Lite#endurant"/>
	<cidoc-crm:P2i_is_type_of rdf:resource="http://academictourism.com/entity/MISC0007"/>
	<rdfs:comment>forests</rdfs:comment>
</rdf:Description>

<rdf:Description rdf:about="http://vocab.getty.edu/page/aat/300417950">
	<rdf:type rdf:resource="http://www.w3.org/2002/07/owl#NamedIndividual"/>
	<rdf:type rdf:resource="http://www.cidoc-crm.org/cidoc-crm/E1_CRM_Entity"/>
	<rdf:type rdf:resource="http://www.cidoc-crm.org/cidoc-crm/E28_Conceptual_Object"/>
	<rdf:type rdf:resource="http://www.cidoc-crm.org/cidoc-crm/E55_Type"/>
	<rdf:type rdf:resource="http://www.cidoc-crm.org/cidoc-crm/E70_Thing"/>
	<rdf:type rdf:resource="http://www.cidoc-crm.org/cidoc-crm/E71_Human-Made_Thing"/>
	<rdf:type rdf:resource="http://www.cidoc-crm.org/cidoc-crm/E77_Persistent_Item"/>
	<rdf:type rdf:resource="http://www.loa-cnr.it/ontologies/DOLCE-Lite#endurant"/>
	<cidoc-crm:P2i_is_type_of rdf:resource="http://academictourism.com/entity/MISC0004"/>
	<rdfs:label>busts</rdfs:label>
</rdf:Description>

<rdf:Description rdf:about="http://vocab.getty.edu/page/tgn/1038862">
	<rdf:type rdf:resource="http://www.w3.org/2002/07/owl#NamedIndividual"/>
	<rdf:type rdf:resource="http://www.cidoc-crm.org/cidoc-crm/E1_CRM_Entity"/>
	<rdf:type rdf:resource="http://www.cidoc-crm.org/cidoc-crm/E53_Place"/>
	<rdf:type rdf:resource="http://www.w3.org/2004/02/skos/core#Concept"/>
	<skos:closeMatch rdf:resource="http://academictourism.com/entity/LOC0006"/>
	<skos:mappingRelation rdf:resource="http://academictourism.com/entity/LOC0006"/>
	<skos:semanticRelation rdf:resource="http://academictourism.com/entity/LOC0006"/>
	<skos:prefLabel>Dransfeld</skos:prefLabel>
</rdf:Description>

<rdf:Description rdf:about="http://vocab.getty.edu/page/tgn/1039172">
	<rdf:type rdf:resource="http://www.w3.org/2002/07/owl#NamedIndividual"/>
	<rdf:type rdf:resource="http://www.cidoc-crm.org/cidoc-crm/E1_CRM_Entity"/>
	<rdf:type rdf:resource="http://www.cidoc-crm.org/cidoc-crm/E53_Place"/>
	<rdf:type rdf:resource="http://www.w3.org/2004/02/skos/core#Concept"/>
	<skos:closeMatch rdf:resource="http://academictourism.com/entity/LOC0002"/>
	<skos:mappingRelation rdf:resource="http://academictourism.com/entity/LOC0002"/>
	<skos:semanticRelation rdf:resource="http://academictourism.com/entity/LOC0002"/>
	<skos:prefLabel>Göttingen</skos:prefLabel>
</rdf:Description>

<rdf:Description rdf:about="http://vocab.getty.edu/page/tgn/4005920">
	<rdf:type rdf:resource="http://www.w3.org/2002/07/owl#NamedIndividual"/>
	<rdf:type rdf:resource="http://www.cidoc-crm.org/cidoc-crm/E1_CRM_Entity"/>
	<rdf:type rdf:resource="http://www.cidoc-crm.org/cidoc-crm/E53_Place"/>
	<rdf:type rdf:resource="http://www.w3.org/2004/02/skos/core#Concept"/>
	<skos:closeMatch rdf:resource="http://academictourism.com/entity/LOC0004.CS"/>
	<skos:mappingRelation rdf:resource="http://academictourism.com/entity/LOC0004.CS"/>
	<skos:semanticRelation rdf:resource="http://academictourism.com/entity/LOC0004.CS"/>
	<skos:prefLabel>Löwenburg</skos:prefLabel>
</rdf:Description>

<rdf:Description rdf:about="http://vocab.getty.edu/page/tgn/7004431">
	<rdf:type rdf:resource="http://www.w3.org/2002/07/owl#NamedIndividual"/>
	<rdf:type rdf:resource="http://www.cidoc-crm.org/cidoc-crm/E1_CRM_Entity"/>
	<rdf:type rdf:resource="http://www.cidoc-crm.org/cidoc-crm/E53_Place"/>
	<rdf:type rdf:resource="http://www.w3.org/2004/02/skos/core#Concept"/>
	<skos:closeMatch rdf:resource="http://academictourism.com/entity/LOC0001"/>
	<skos:mappingRelation rdf:resource="http://academictourism.com/entity/LOC0001"/>
	<skos:semanticRelation rdf:resource="http://academictourism.com/entity/LOC0001"/>
	<skos:prefLabel>Kassel</skos:prefLabel>
</rdf:Description>

<rdf:Description rdf:about="http://vocab.getty.edu/page/tgn/7077709">
	<rdf:type rdf:resource="http://www.w3.org/2002/07/owl#NamedIndividual"/>
	<rdf:type rdf:resource="http://www.cidoc-crm.org/cidoc-crm/E1_CRM_Entity"/>
	<rdf:type rdf:resource="http://www.cidoc-crm.org/cidoc-crm/E53_Place"/>
	<rdf:type rdf:resource="http://www.w3.org/2004/02/skos/core#Concept"/>
	<skos:closeMatch rdf:resource="http://academictourism.com/entity/LOC0003.CS"/>
	<skos:mappingRelation rdf:resource="http://academictourism.com/entity/LOC0003.CS"/>
	<skos:semanticRelation rdf:resource="http://academictourism.com/entity/LOC0003.CS"/>
	<skos:prefLabel>Schloß Wilhelmshöhe (castle)</skos:prefLabel>
</rdf:Description>

<rdf:Description rdf:about="http://vocab.getty.edu/page/tgn/7133622">
	<rdf:type rdf:resource="http://www.w3.org/2002/07/owl#NamedIndividual"/>
	<rdf:type rdf:resource="http://www.cidoc-crm.org/cidoc-crm/E1_CRM_Entity"/>
	<rdf:type rdf:resource="http://www.cidoc-crm.org/cidoc-crm/E53_Place"/>
	<rdf:type rdf:resource="http://www.w3.org/2004/02/skos/core#Concept"/>
	<skos:closeMatch rdf:resource="http://academictourism.com/entity/LOC0005"/>
	<skos:mappingRelation rdf:resource="http://academictourism.com/entity/LOC0005"/>
	<skos:semanticRelation rdf:resource="http://academictourism.com/entity/LOC0005"/>
	<skos:prefLabel>Münden</skos:prefLabel>
</rdf:Description>

<rdf:Description rdf:about="https://viaf.org/viaf/264553004">
	<rdf:type rdf:resource="http://www.w3.org/2002/07/owl#NamedIndividual"/>
	<rdf:type rdf:resource="http://www.cidoc-crm.org/cidoc-crm/E18_Physical_Thing"/>
	<rdf:type rdf:resource="http://www.cidoc-crm.org/cidoc-crm/E19_Physical_Object"/>
	<rdf:type rdf:resource="http://www.cidoc-crm.org/cidoc-crm/E1_CRM_Entity"/>
	<rdf:type rdf:resource="http://www.cidoc-crm.org/cidoc-crm/E20_Biological_Object"/>
	<rdf:type rdf:resource="http://www.cidoc-crm.org/cidoc-crm/E21_Person"/>
	<rdf:type rdf:resource="http://www.cidoc-crm.org/cidoc-crm/E39_Actor"/>
	<rdf:type rdf:resource="http://www.cidoc-crm.org/cidoc-crm/E70_Thing"/>
	<rdf:type rdf:resource="http://www.cidoc-crm.org/cidoc-crm/E72_Legal_Object"/>
	<rdf:type rdf:resource="http://www.cidoc-crm.org/cidoc-crm/E77_Persistent_Item"/>
	<rdf:type rdf:resource="http://www.loa-cnr.it/ontologies/DOLCE-Lite#endurant"/>
	<rdf:type rdf:resource="http://www.w3.org/2004/02/skos/core#Concept"/>
	<skos:closeMatch rdf:resource="http://academictourism.com/entity/PER0012"/>
	<skos:closeMatch rdf:resource="https://viaf.org/viaf/264553004"/>
	<skos:exactMatch rdf:resource="http://academictourism.com/entity/PER0012"/>
	<skos:exactMatch rdf:resource="https://viaf.org/viaf/264553004"/>
	<skos:mappingRelation rdf:resource="http://academictourism.com/entity/PER0012"/>
	<skos:mappingRelation rdf:resource="https://viaf.org/viaf/264553004"/>
	<skos:semanticRelation rdf:resource="http://academictourism.com/entity/PER0012"/>
	<skos:semanticRelation rdf:resource="https://viaf.org/viaf/264553004"/>
	<skos:prefLabel>Wilhelm IX., Landgraf von Hessen-Kassel 1743-1821</skos:prefLabel>
</rdf:Description>

<rdf:Description rdf:about="https://viaf.org/viaf/29528071">
	<rdf:type rdf:resource="http://www.w3.org/2002/07/owl#NamedIndividual"/>
	<rdf:type rdf:resource="http://www.w3.org/2004/02/skos/core#Concept"/>
	<skos:closeMatch rdf:resource="http://academictourism.com/entity/PER0016"/>
	<skos:closeMatch rdf:resource="https://viaf.org/viaf/29528071"/>
	<skos:exactMatch rdf:resource="http://academictourism.com/entity/PER0016"/>
	<skos:exactMatch rdf:resource="https://viaf.org/viaf/29528071"/>
	<skos:mappingRelation rdf:resource="http://academictourism.com/entity/PER0016"/>
	<skos:mappingRelation rdf:resource="https://viaf.org/viaf/29528071"/>
	<skos:semanticRelation rdf:resource="http://academictourism.com/entity/PER0016"/>
	<skos:semanticRelation rdf:resource="https://viaf.org/viaf/29528071"/>
	<skos:prefLabel>Karl, Landgraf von Hessen-Kassel, 1654-1730</skos:prefLabel>
</rdf:Description>

<rdf:Description rdf:about="https://viaf.org/viaf/47863906">
	<rdf:type rdf:resource="http://www.w3.org/2002/07/owl#NamedIndividual"/>
	<rdf:type rdf:resource="http://www.w3.org/2004/02/skos/core#Concept"/>
	<skos:closeMatch rdf:resource="http://academictourism.com/entity/PER0011"/>
	<skos:closeMatch rdf:resource="https://viaf.org/viaf/47863906"/>
	<skos:exactMatch rdf:resource="http://academictourism.com/entity/PER0011"/>
	<skos:exactMatch rdf:resource="https://viaf.org/viaf/47863906"/>
	<skos:mappingRelation rdf:resource="http://academictourism.com/entity/PER0011"/>
	<skos:mappingRelation rdf:resource="https://viaf.org/viaf/47863906"/>
	<skos:semanticRelation rdf:resource="http://academictourism.com/entity/PER0011"/>
	<skos:semanticRelation rdf:resource="https://viaf.org/viaf/47863906"/>
	<skos:prefLabel>Friedrich II. Hessen-Kassel, Landgraf 1720-1785</skos:prefLabel>
</rdf:Description>

<rdf:Description rdf:about="https://www.wikidata.org/wiki/Q1053313">
	<rdf:type rdf:resource="http://www.w3.org/2002/07/owl#NamedIndividual"/>
	<rdf:type rdf:resource="http://iflastandards.info/ns/lrm/lrmoo/F2_Expression"/>
	<rdf:type rdf:resource="http://www.cidoc-crm.org/cidoc-crm/E1_CRM_Entity"/>
	<rdf:type rdf:resource="http://www.cidoc-crm.org/cidoc-crm/E28_Conceptual_Object"/>
	<rdf:type rdf:resource="http://www.cidoc-crm.org/cidoc-crm/E70_Thing"/>
	<rdf:type rdf:resource="http://www.cidoc-crm.org/cidoc-crm/E71_Human-Made_Thing"/>
	<rdf:type rdf:resource="http://www.cidoc-crm.org/cidoc-crm/E72_Legal_Object"/>
	<rdf:type rdf:resource="http://www.cidoc-crm.org/cidoc-crm/E73_Information_Object"/>
	<rdf:type rdf:resource="http://www.cidoc-crm.org/cidoc-crm/E77_Persistent_Item"/>
	<rdf:type rdf:resource="http://www.cidoc-crm.org/cidoc-crm/E89_Propositional_Object"/>
	<rdf:type rdf:resource="http://www.cidoc-crm.org/cidoc-crm/E90_Symbolic_Object"/>
	<rdf:type rdf:resource="http://www.loa-cnr.it/ontologies/DOLCE-Lite#endurant"/>
	<rdf:type rdf:resource="http://www.w3.org/2004/02/skos/core#Concept"/>
	<skos:closeMatch rdf:resource="http://academictourism.com/entity/MISC0021"/>
	<skos:closeMatch rdf:resource="https://www.wikidata.org/wiki/Q1053313"/>
	<skos:exactMatch rdf:resource="http://academictourism.com/entity/MISC0021"/>
	<skos:exactMatch rdf:resource="https://www.wikidata.org/wiki/Q1053313"/>
	<skos:mappingRelation rdf:resource="http://academictourism.com/entity/MISC0021"/>
	<skos:mappingRelation rdf:resource="https://www.wikidata.org/wiki/Q1053313"/>
	<skos:semanticRelation rdf:resource="http://academictourism.com/entity/MISC0021"/>
	<skos:semanticRelation rdf:resource="https://www.wikidata.org/wiki/Q1053313"/>
</rdf:Description>

<rdf:Description rdf:about="https://www.wikidata.org/wiki/Q1305418">
	<rdf:type rdf:resource="http://www.w3.org/2002/07/owl#NamedIndividual"/>
	<rdf:type rdf:resource="http://www.cidoc-crm.org/cidoc-crm/E1_CRM_Entity"/>
	<rdf:type rdf:resource="http://www.cidoc-crm.org/cidoc-crm/E53_Place"/>
	<rdf:type rdf:resource="http://www.w3.org/2004/02/skos/core#Concept"/>
	<skos:closeMatch rdf:resource="http://academictourism.com/entity/LOC0005"/>
	<skos:mappingRelation rdf:resource="http://academictourism.com/entity/LOC0005"/>
	<skos:semanticRelation rdf:resource="http://academictourism.com/entity/LOC0005"/>
</rdf:Description>

<rdf:Description rdf:about="https://www.wikidata.org/wiki/Q131552">
	<rdf:type rdf:resource="http://www.w3.org/2002/07/owl#NamedIndividual"/>
	<rdf:type rdf:resource="http://www.cidoc-crm.org/cidoc-crm/E18_Physical_Thing"/>
	<rdf:type rdf:resource="http://www.cidoc-crm.org/cidoc-crm/E19_Physical_Object"/>
	<rdf:type rdf:resource="http://www.cidoc-crm.org/cidoc-crm/E1_CRM_Entity"/>
	<rdf:type rdf:resource="http://www.cidoc-crm.org/cidoc-crm/E20_Biological_Object"/>
	<rdf:type rdf:resource="http://www.cidoc-crm.org/cidoc-crm/E21_Person"/>
	<rdf:type rdf:resource="http://www.cidoc-crm.org/cidoc-crm/E39_Actor"/>
	<rdf:type rdf:resource="http://www.cidoc-crm.org/cidoc-crm/E70_Thing"/>
	<rdf:type rdf:resource="http://www.cidoc-crm.org/cidoc-crm/E72_Legal_Object"/>
	<rdf:type rdf:resource="http://www.cidoc-crm.org/cidoc-crm/E77_Persistent_Item"/>
	<rdf:type rdf:resource="http://www.loa-cnr.it/ontologies/DOLCE-Lite#endurant"/>
	<cidoc-crm:P129i_is_subject_of rdf:resource="http://academictourism.com/entity/CT.BRF0005.RS.L0001"/>
	<cidoc-crm:P67i_is_referred_to_by rdf:resource="http://academictourism.com/entity/CT.BRF0005.RS.L0001"/>
	<skos:prefLabel>Catherine de' Medici</skos:prefLabel>
</rdf:Description>

<rdf:Description rdf:about="https://www.wikidata.org/wiki/Q132545">
	<rdf:type rdf:resource="http://www.w3.org/2002/07/owl#NamedIndividual"/>
	<rdf:type rdf:resource="http://www.cidoc-crm.org/cidoc-crm/E18_Physical_Thing"/>
	<rdf:type rdf:resource="http://www.cidoc-crm.org/cidoc-crm/E19_Physical_Object"/>
	<rdf:type rdf:resource="http://www.cidoc-crm.org/cidoc-crm/E1_CRM_Entity"/>
	<rdf:type rdf:resource="http://www.cidoc-crm.org/cidoc-crm/E20_Biological_Object"/>
	<rdf:type rdf:resource="http://www.cidoc-crm.org/cidoc-crm/E21_Person"/>
	<rdf:type rdf:resource="http://www.cidoc-crm.org/cidoc-crm/E39_Actor"/>
	<rdf:type rdf:resource="http://www.cidoc-crm.org/cidoc-crm/E70_Thing"/>
	<rdf:type rdf:resource="http://www.cidoc-crm.org/cidoc-crm/E72_Legal_Object"/>
	<rdf:type rdf:resource="http://www.cidoc-crm.org/cidoc-crm/E77_Persistent_Item"/>
	<rdf:type rdf:resource="http://www.loa-cnr.it/ontologies/DOLCE-Lite#endurant"/>
	<cidoc-crm:P129i_is_subject_of rdf:resource="http://academictourism.com/entity/CT.BRF0005.RS.L0001"/>
	<cidoc-crm:P67i_is_referred_to_by rdf:resource="http://academictourism.com/entity/CT.BRF0005.RS.L0001"/>
	<skos:prefLabel>Henry II of France</skos:prefLabel>
</rdf:Description>

<rdf:Description rdf:about="https://www.wikidata.org/wiki/Q1501427">
	<rdf:type rdf:resource="http://www.w3.org/2002/07/owl#NamedIndividual"/>
	<rdf:type rdf:resource="http://www.cidoc-crm.org/cidoc-crm/E1_CRM_Entity"/>
	<rdf:type rdf:resource="http://www.cidoc-crm.org/cidoc-crm/E28_Conceptual_Object"/>
	<rdf:type rdf:resource="http://www.cidoc-crm.org/cidoc-crm/E55_Type"/>
	<rdf:type rdf:resource="http://www.cidoc-crm.org/cidoc-crm/E70_Thing"/>
	<rdf:type rdf:resource="http://www.cidoc-crm.org/cidoc-crm/E71_Human-Made_Thing"/>
	<rdf:type rdf:resource="http://www.cidoc-crm.org/cidoc-crm/E77_Persistent_Item"/>
	<rdf:type rdf:resource="http://www.loa-cnr.it/ontologies/DOLCE-Lite#endurant"/>
	<rdf:type rdf:resource="http://www.w3.org/2004/02/skos/core#Concept"/>
	<skos:closeMatch rdf:resource="http://academictourism.com/entity/MISC0019"/>
	<skos:mappingRelation rdf:resource="http://academictourism.com/entity/MISC0019"/>
	<skos:semanticRelation rdf:resource="http://academictourism.com/entity/MISC0019"/>
</rdf:Description>

<rdf:Description rdf:about="https://www.wikidata.org/wiki/Q152838">
	<rdf:type rdf:resource="http://www.w3.org/2002/07/owl#NamedIndividual"/>
	<rdf:type rdf:resource="http://www.cidoc-crm.org/cidoc-crm/E1_CRM_Entity"/>
	<rdf:type rdf:resource="http://www.cidoc-crm.org/cidoc-crm/E53_Place"/>
	<rdf:type rdf:resource="http://www.w3.org/2004/02/skos/core#Concept"/>
	<skos:closeMatch rdf:resource="http://academictourism.com/entity/LOC0007"/>
	<skos:mappingRelation rdf:resource="http://academictourism.com/entity/LOC0007"/>
	<skos:semanticRelation rdf:resource="http://academictourism.com/entity/LOC0007"/>
</rdf:Description>

<rdf:Description rdf:about="https://www.wikidata.org/wiki/Q1651504">
	<rdf:type rdf:resource="http://www.w3.org/2002/07/owl#NamedIndividual"/>
	<rdf:type rdf:resource="http://www.cidoc-crm.org/cidoc-crm/E1_CRM_Entity"/>
	<rdf:type rdf:resource="http://www.cidoc-crm.org/cidoc-crm/E53_Place"/>
	<rdf:type rdf:resource="http://www.w3.org/2004/02/skos/core#Concept"/>
	<skos:closeMatch rdf:resource="http://academictourism.com/entity/LOC0004.CS"/>
	<skos:mappingRelation rdf:resource="http://academictourism.com/entity/LOC0004.CS"/>
	<skos:semanticRelation rdf:resource="http://academictourism.com/entity/LOC0004.CS"/>
</rdf:Description>

<rdf:Description rdf:about="https://www.wikidata.org/wiki/Q170022">
	<rdf:type rdf:resource="http://www.w3.org/2002/07/owl#NamedIndividual"/>
	<rdf:type rdf:resource="http://iflastandards.info/ns/lrm/lrmoo/F39_Family"/>
	<rdf:type rdf:resource="http://iflastandards.info/ns/lrm/lrmoo/F55_Collective_Agent"/>
	<rdf:type rdf:resource="http://www.cidoc-crm.org/cidoc-crm/E1_CRM_Entity"/>
	<rdf:type rdf:resource="http://www.cidoc-crm.org/cidoc-crm/E39_Actor"/>
	<rdf:type rdf:resource="http://www.cidoc-crm.org/cidoc-crm/E74_Group"/>
	<rdf:type rdf:resource="http://www.cidoc-crm.org/cidoc-crm/E77_Persistent_Item"/>
	<rdf:type rdf:resource="http://www.loa-cnr.it/ontologies/DOLCE-Lite#endurant"/>
	<cidoc-crm:P129i_is_subject_of rdf:resource="http://academictourism.com/entity/CT.BRF0005.RS.L0001"/>
	<cidoc-crm:P67i_is_referred_to_by rdf:resource="http://academictourism.com/entity/CT.BRF0005.RS.L0001"/>
	<rdfs:seeAlso rdf:datatype="http://www.w3.org/2001/XMLSchema#anyURI">https://en.wikipedia.org/wiki/House_of_Medici</rdfs:seeAlso>
	<skos:prefLabel>House of Medici</skos:prefLabel>
</rdf:Description>

<rdf:Description rdf:about="https://www.wikidata.org/wiki/Q187719">
	<rdf:type rdf:resource="http://www.w3.org/2002/07/owl#NamedIndividual"/>
	<rdf:type rdf:resource="http://iflastandards.info/ns/lrm/lrmoo/F2_Expression"/>
	<rdf:type rdf:resource="http://www.cidoc-crm.org/cidoc-crm/E1_CRM_Entity"/>
	<rdf:type rdf:resource="http://www.cidoc-crm.org/cidoc-crm/E28_Conceptual_Object"/>
	<rdf:type rdf:resource="http://www.cidoc-crm.org/cidoc-crm/E70_Thing"/>
	<rdf:type rdf:resource="http://www.cidoc-crm.org/cidoc-crm/E71_Human-Made_Thing"/>
	<rdf:type rdf:resource="http://www.cidoc-crm.org/cidoc-crm/E72_Legal_Object"/>
	<rdf:type rdf:resource="http://www.cidoc-crm.org/cidoc-crm/E73_Information_Object"/>
	<rdf:type rdf:resource="http://www.cidoc-crm.org/cidoc-crm/E77_Persistent_Item"/>
	<rdf:type rdf:resource="http://www.cidoc-crm.org/cidoc-crm/E89_Propositional_Object"/>
	<rdf:type rdf:resource="http://www.cidoc-crm.org/cidoc-crm/E90_Symbolic_Object"/>
	<rdf:type rdf:resource="http://www.loa-cnr.it/ontologies/DOLCE-Lite#endurant"/>
	<cidoc-crm:P129i_is_subject_of rdf:resource="http://academictourism.com/entity/CT.BRF0005.RS.L0001"/>
	<cidoc-crm:P67i_is_referred_to_by rdf:resource="http://academictourism.com/entity/CT.BRF0005.RS.L0001"/>
	<rdfs:label>Corpus Juris Civilis</rdfs:label>
	<rdfs:seeAlso rdf:datatype="http://www.w3.org/2001/XMLSchema#anyURI">https://nl.wikipedia.org/wiki/Corpus_Iuris_Civilis</rdfs:seeAlso>
</rdf:Description>

<rdf:Description rdf:about="https://www.wikidata.org/wiki/Q235356">
	<rdf:type rdf:resource="http://www.w3.org/2002/07/owl#NamedIndividual"/>
	<rdf:type rdf:resource="http://academictourism.com/academictourism#Mode_of_Transportation"/>
	<rdf:type rdf:resource="http://www.cidoc-crm.org/cidoc-crm/E1_CRM_Entity"/>
	<rdf:type rdf:resource="http://www.cidoc-crm.org/cidoc-crm/E28_Conceptual_Object"/>
	<rdf:type rdf:resource="http://www.cidoc-crm.org/cidoc-crm/E55_Type"/>
	<rdf:type rdf:resource="http://www.cidoc-crm.org/cidoc-crm/E70_Thing"/>
	<rdf:type rdf:resource="http://www.cidoc-crm.org/cidoc-crm/E71_Human-Made_Thing"/>
	<rdf:type rdf:resource="http://www.cidoc-crm.org/cidoc-crm/E77_Persistent_Item"/>
	<rdf:type rdf:resource="http://www.loa-cnr.it/ontologies/DOLCE-Lite#endurant"/>
	<cidoc-crm:P2i_is_type_of rdf:resource="http://academictourism.com/entity/BRF0004.RS.RS0006"/>
	<rdfs:comment>carriage</rdfs:comment>
</rdf:Description>

<rdf:Description rdf:about="https://www.wikidata.org/wiki/Q2865">
	<rdf:type rdf:resource="http://www.w3.org/2002/07/owl#NamedIndividual"/>
	<rdf:type rdf:resource="http://www.cidoc-crm.org/cidoc-crm/E1_CRM_Entity"/>
	<rdf:type rdf:resource="http://www.cidoc-crm.org/cidoc-crm/E53_Place"/>
	<rdf:type rdf:resource="http://www.w3.org/2004/02/skos/core#Concept"/>
	<skos:closeMatch rdf:resource="http://academictourism.com/entity/LOC0001"/>
	<skos:mappingRelation rdf:resource="http://academictourism.com/entity/LOC0001"/>
	<skos:semanticRelation rdf:resource="http://academictourism.com/entity/LOC0001"/>
</rdf:Description>

<rdf:Description rdf:about="https://www.wikidata.org/wiki/Q29524">
	<rdf:type rdf:resource="http://www.w3.org/2002/07/owl#NamedIndividual"/>
	<rdf:type rdf:resource="http://academictourism.com/academictourism#Course_Subject"/>
	<rdf:type rdf:resource="http://www.cidoc-crm.org/cidoc-crm/E1_CRM_Entity"/>
	<rdf:type rdf:resource="http://www.cidoc-crm.org/cidoc-crm/E28_Conceptual_Object"/>
	<rdf:type rdf:resource="http://www.cidoc-crm.org/cidoc-crm/E55_Type"/>
	<rdf:type rdf:resource="http://www.cidoc-crm.org/cidoc-crm/E70_Thing"/>
	<rdf:type rdf:resource="http://www.cidoc-crm.org/cidoc-crm/E71_Human-Made_Thing"/>
	<rdf:type rdf:resource="http://www.cidoc-crm.org/cidoc-crm/E77_Persistent_Item"/>
	<rdf:type rdf:resource="http://www.loa-cnr.it/ontologies/DOLCE-Lite#endurant"/>
	<cidoc-crm:P129i_is_subject_of rdf:resource="http://academictourism.com/entity/CT.BRF0005.RS.L0003"/>
	<cidoc-crm:P67i_is_referred_to_by rdf:resource="http://academictourism.com/entity/CT.BRF0005.RS.L0003"/>
	<rdfs:seeAlso rdf:datatype="http://www.w3.org/2001/XMLSchema#anyURI">natural law</rdfs:seeAlso>
</rdf:Description>

<rdf:Description rdf:about="https://www.wikidata.org/wiki/Q3033">
	<rdf:type rdf:resource="http://www.w3.org/2002/07/owl#NamedIndividual"/>
	<rdf:type rdf:resource="http://www.cidoc-crm.org/cidoc-crm/E1_CRM_Entity"/>
	<rdf:type rdf:resource="http://www.cidoc-crm.org/cidoc-crm/E53_Place"/>
	<rdf:type rdf:resource="http://www.w3.org/2004/02/skos/core#Concept"/>
	<skos:closeMatch rdf:resource="http://academictourism.com/entity/LOC0002"/>
	<skos:mappingRelation rdf:resource="http://academictourism.com/entity/LOC0002"/>
	<skos:semanticRelation rdf:resource="http://academictourism.com/entity/LOC0002"/>
</rdf:Description>

<rdf:Description rdf:about="https://www.wikidata.org/wiki/Q447441">
	<rdf:type rdf:resource="http://www.w3.org/2002/07/owl#NamedIndividual"/>
	<rdf:type rdf:resource="http://www.cidoc-crm.org/cidoc-crm/E1_CRM_Entity"/>
	<rdf:type rdf:resource="http://www.cidoc-crm.org/cidoc-crm/E53_Place"/>
	<rdf:type rdf:resource="http://www.w3.org/2004/02/skos/core#Concept"/>
	<skos:closeMatch rdf:resource="http://academictourism.com/entity/LOC0003"/>
	<skos:mappingRelation rdf:resource="http://academictourism.com/entity/LOC0003"/>
	<skos:semanticRelation rdf:resource="http://academictourism.com/entity/LOC0003"/>
	<rdfs:comment xml:lang="de">Bergpark Wilhelmshöhe</rdfs:comment>
	<rdfs:comment xml:lang="en">Bergpark Wilhelmshöhe</rdfs:comment>
</rdf:Description>

<rdf:Description rdf:about="https://www.wikidata.org/wiki/Q484591">
	<rdf:type rdf:resource="http://www.w3.org/2002/07/owl#NamedIndividual"/>
	<rdf:type rdf:resource="http://academictourism.com/academictourism#Course_Subject"/>
	<rdf:type rdf:resource="http://www.cidoc-crm.org/cidoc-crm/E1_CRM_Entity"/>
	<rdf:type rdf:resource="http://www.cidoc-crm.org/cidoc-crm/E28_Conceptual_Object"/>
	<rdf:type rdf:resource="http://www.cidoc-crm.org/cidoc-crm/E55_Type"/>
	<rdf:type rdf:resource="http://www.cidoc-crm.org/cidoc-crm/E70_Thing"/>
	<rdf:type rdf:resource="http://www.cidoc-crm.org/cidoc-crm/E71_Human-Made_Thing"/>
	<rdf:type rdf:resource="http://www.cidoc-crm.org/cidoc-crm/E77_Persistent_Item"/>
	<rdf:type rdf:resource="http://www.loa-cnr.it/ontologies/DOLCE-Lite#endurant"/>
	<cidoc-crm:P129i_is_subject_of rdf:resource="http://academictourism.com/entity/CT.BRF0005.RS.L0004"/>
	<cidoc-crm:P67i_is_referred_to_by rdf:resource="http://academictourism.com/entity/CT.BRF0005.RS.L0004"/>
	<rdfs:seeAlso rdf:datatype="http://www.w3.org/2001/XMLSchema#anyURI">natural history</rdfs:seeAlso>
</rdf:Description>

<rdf:Description rdf:about="https://www.wikidata.org/wiki/Q4932206">
	<rdf:type rdf:resource="http://www.w3.org/2002/07/owl#NamedIndividual"/>
	<rdf:type rdf:resource="http://academictourism.com/academictourism#Course_Subject"/>
	<rdf:type rdf:resource="http://www.cidoc-crm.org/cidoc-crm/E1_CRM_Entity"/>
	<rdf:type rdf:resource="http://www.cidoc-crm.org/cidoc-crm/E28_Conceptual_Object"/>
	<rdf:type rdf:resource="http://www.cidoc-crm.org/cidoc-crm/E55_Type"/>
	<rdf:type rdf:resource="http://www.cidoc-crm.org/cidoc-crm/E70_Thing"/>
	<rdf:type rdf:resource="http://www.cidoc-crm.org/cidoc-crm/E71_Human-Made_Thing"/>
	<rdf:type rdf:resource="http://www.cidoc-crm.org/cidoc-crm/E77_Persistent_Item"/>
	<rdf:type rdf:resource="http://www.loa-cnr.it/ontologies/DOLCE-Lite#endurant"/>
	<cidoc-crm:P129i_is_subject_of rdf:resource="http://academictourism.com/entity/CT.BRF0005.RS.L0001"/>
	<cidoc-crm:P67i_is_referred_to_by rdf:resource="http://academictourism.com/entity/CT.BRF0005.RS.L0001"/>
	<cidoc-crm:P3_has_note>literär Geschichte der Rechtswissenschaft  vorzüglich der Bürgerlichen</cidoc-crm:P3_has_note>
	<rdfs:label>jurisprudence</rdfs:label>
</rdf:Description>

<rdf:Description rdf:about="https://www.wikidata.org/wiki/Q512225">
	<rdf:type rdf:resource="http://www.w3.org/2002/07/owl#NamedIndividual"/>
	<rdf:type rdf:resource="http://www.cidoc-crm.org/cidoc-crm/E1_CRM_Entity"/>
	<rdf:type rdf:resource="http://www.cidoc-crm.org/cidoc-crm/E53_Place"/>
	<rdf:type rdf:resource="http://www.w3.org/2004/02/skos/core#Concept"/>
	<skos:closeMatch rdf:resource="http://academictourism.com/entity/LOC0006"/>
	<skos:mappingRelation rdf:resource="http://academictourism.com/entity/LOC0006"/>
	<skos:semanticRelation rdf:resource="http://academictourism.com/entity/LOC0006"/>
</rdf:Description>

<rdf:Description rdf:about="https://www.wikidata.org/wiki/Q521">
	<rdf:type rdf:resource="http://www.w3.org/2002/07/owl#NamedIndividual"/>
	<rdf:type rdf:resource="http://academictourism.com/academictourism#Course_Subject"/>
	<rdf:type rdf:resource="http://www.cidoc-crm.org/cidoc-crm/E1_CRM_Entity"/>
	<rdf:type rdf:resource="http://www.cidoc-crm.org/cidoc-crm/E28_Conceptual_Object"/>
	<rdf:type rdf:resource="http://www.cidoc-crm.org/cidoc-crm/E55_Type"/>
	<rdf:type rdf:resource="http://www.cidoc-crm.org/cidoc-crm/E70_Thing"/>
	<rdf:type rdf:resource="http://www.cidoc-crm.org/cidoc-crm/E71_Human-Made_Thing"/>
	<rdf:type rdf:resource="http://www.cidoc-crm.org/cidoc-crm/E77_Persistent_Item"/>
	<rdf:type rdf:resource="http://www.loa-cnr.it/ontologies/DOLCE-Lite#endurant"/>
	<cidoc-crm:P129i_is_subject_of rdf:resource="http://academictourism.com/entity/CT.BRF0005.RS.L0004"/>
	<cidoc-crm:P67i_is_referred_to_by rdf:resource="http://academictourism.com/entity/CT.BRF0005.RS.L0004"/>
	<rdfs:seeAlso rdf:datatype="http://www.w3.org/2001/XMLSchema#anyURI">Physiology</rdfs:seeAlso>
</rdf:Description>

<rdf:Description rdf:about="https://www.wikidata.org/wiki/Q687186">
	<rdf:type rdf:resource="http://www.w3.org/2002/07/owl#NamedIndividual"/>
	<rdf:type rdf:resource="http://www.cidoc-crm.org/cidoc-crm/E1_CRM_Entity"/>
	<rdf:type rdf:resource="http://www.cidoc-crm.org/cidoc-crm/E53_Place"/>
	<rdf:type rdf:resource="http://www.w3.org/2004/02/skos/core#Concept"/>
	<skos:closeMatch rdf:resource="http://academictourism.com/entity/LOC0003.CS"/>
	<skos:mappingRelation rdf:resource="http://academictourism.com/entity/LOC0003.CS"/>
	<skos:semanticRelation rdf:resource="http://academictourism.com/entity/LOC0003.CS"/>
</rdf:Description>

<rdf:Description rdf:about="https://www.wikidata.org/wiki/Q838526">
	<rdf:type rdf:resource="http://www.w3.org/2002/07/owl#NamedIndividual"/>
	<rdf:type rdf:resource="http://iflastandards.info/ns/lrm/lrmoo/F2_Expression"/>
	<rdf:type rdf:resource="http://www.cidoc-crm.org/cidoc-crm/E1_CRM_Entity"/>
	<rdf:type rdf:resource="http://www.cidoc-crm.org/cidoc-crm/E28_Conceptual_Object"/>
	<rdf:type rdf:resource="http://www.cidoc-crm.org/cidoc-crm/E70_Thing"/>
	<rdf:type rdf:resource="http://www.cidoc-crm.org/cidoc-crm/E71_Human-Made_Thing"/>
	<rdf:type rdf:resource="http://www.cidoc-crm.org/cidoc-crm/E72_Legal_Object"/>
	<rdf:type rdf:resource="http://www.cidoc-crm.org/cidoc-crm/E73_Information_Object"/>
	<rdf:type rdf:resource="http://www.cidoc-crm.org/cidoc-crm/E77_Persistent_Item"/>
	<rdf:type rdf:resource="http://www.cidoc-crm.org/cidoc-crm/E89_Propositional_Object"/>
	<rdf:type rdf:resource="http://www.cidoc-crm.org/cidoc-crm/E90_Symbolic_Object"/>
	<rdf:type rdf:resource="http://www.loa-cnr.it/ontologies/DOLCE-Lite#endurant"/>
	<rdf:type rdf:resource="http://www.w3.org/2004/02/skos/core#Concept"/>
	<skos:closeMatch rdf:resource="http://academictourism.com/entity/MISC0020"/>
	<skos:mappingRelation rdf:resource="http://academictourism.com/entity/MISC0020"/>
	<skos:semanticRelation rdf:resource="http://academictourism.com/entity/MISC0020"/>
</rdf:Description>

<rdf:Description rdf:about="https://www.wikidata.org/wiki/Q908578">
	<rdf:type rdf:resource="http://www.w3.org/2002/07/owl#NamedIndividual"/>
	<rdf:type rdf:resource="http://academictourism.com/academictourism#Course_Subject"/>
	<rdf:type rdf:resource="http://www.cidoc-crm.org/cidoc-crm/E1_CRM_Entity"/>
	<rdf:type rdf:resource="http://www.cidoc-crm.org/cidoc-crm/E28_Conceptual_Object"/>
	<rdf:type rdf:resource="http://www.cidoc-crm.org/cidoc-crm/E55_Type"/>
	<rdf:type rdf:resource="http://www.cidoc-crm.org/cidoc-crm/E70_Thing"/>
	<rdf:type rdf:resource="http://www.cidoc-crm.org/cidoc-crm/E71_Human-Made_Thing"/>
	<rdf:type rdf:resource="http://www.cidoc-crm.org/cidoc-crm/E77_Persistent_Item"/>
	<rdf:type rdf:resource="http://www.loa-cnr.it/ontologies/DOLCE-Lite#endurant"/>
	<cidoc-crm:P129i_is_subject_of rdf:resource="http://academictourism.com/entity/CT.BRF0005.RS.L0002"/>
	<cidoc-crm:P67i_is_referred_to_by rdf:resource="http://academictourism.com/entity/CT.BRF0005.RS.L0002"/>
	<rdfs:label>history of Greek</rdfs:label>
</rdf:Description>

<rdf:Description rdf:about="https://www.wikidata.org/wiki/Q918236">
	<rdf:type rdf:resource="http://www.w3.org/2002/07/owl#NamedIndividual"/>
	<rdf:type rdf:resource="http://www.cidoc-crm.org/cidoc-crm/E1_CRM_Entity"/>
	<rdf:type rdf:resource="http://www.cidoc-crm.org/cidoc-crm/E28_Conceptual_Object"/>
	<rdf:type rdf:resource="http://www.cidoc-crm.org/cidoc-crm/E55_Type"/>
	<rdf:type rdf:resource="http://www.cidoc-crm.org/cidoc-crm/E70_Thing"/>
	<rdf:type rdf:resource="http://www.cidoc-crm.org/cidoc-crm/E71_Human-Made_Thing"/>
	<rdf:type rdf:resource="http://www.cidoc-crm.org/cidoc-crm/E77_Persistent_Item"/>
	<rdf:type rdf:resource="http://www.loa-cnr.it/ontologies/DOLCE-Lite#endurant"/>
	<cidoc-crm:P2_has_type rdf:resource="https://www.wikidata.org/wiki/Q918236"/>
	<cidoc-crm:P2i_is_type_of rdf:resource="https://www.wikidata.org/wiki/Q918236"/>
	<rdfs:label>water organ</rdfs:label>
</rdf:Description>

<rdf:Description rdf:about="http://www.w3.org/2004/02/skos/core#changeNote">
	<rdfs:isDefinedBy rdf:resource="http://www.w3.org/2004/02/skos/core"/>
	<rdfs:label xml:lang="en">change note</rdfs:label>
	<skos:definition xml:lang="en">A note about a modification to a concept.</skos:definition>
</rdf:Description>

<rdf:Description rdf:about="http://www.w3.org/2004/02/skos/core#editorialNote">
	<rdfs:isDefinedBy rdf:resource="http://www.w3.org/2004/02/skos/core"/>
	<rdfs:label xml:lang="en">editorial note</rdfs:label>
	<skos:definition xml:lang="en">A note for an editor, translator or maintainer of the vocabulary.</skos:definition>
</rdf:Description>

<rdf:Description rdf:about="http://www.w3.org/2004/02/skos/core#hiddenLabel">
	<rdfs:comment xml:lang="en">The range of skos:hiddenLabel is the class of RDF plain literals.</rdfs:comment>
	<rdfs:comment xml:lang="en">skos:prefLabel, skos:altLabel and skos:hiddenLabel are pairwise disjoint properties.</rdfs:comment>
	<rdfs:isDefinedBy rdf:resource="http://www.w3.org/2004/02/skos/core"/>
	<rdfs:label xml:lang="en">hidden label</rdfs:label>
	<skos:definition xml:lang="en">A lexical label for a resource that should be hidden when generating visual displays of the resource, but should still be accessible to free text search operations.</skos:definition>
</rdf:Description>

<rdf:Description rdf:about="http://www.w3.org/2004/02/skos/core#historyNote">
	<rdfs:isDefinedBy rdf:resource="http://www.w3.org/2004/02/skos/core"/>
	<rdfs:label xml:lang="en">history note</rdfs:label>
	<skos:definition xml:lang="en">A note about the past state/use/meaning of a concept.</skos:definition>
</rdf:Description>

<rdf:Description rdf:about="http://www.w3.org/2004/02/skos/core#note">
	<rdfs:isDefinedBy rdf:resource="http://www.w3.org/2004/02/skos/core"/>
	<rdfs:label xml:lang="en">note</rdfs:label>
	<skos:definition xml:lang="en">A general note, for any purpose.</skos:definition>
	<skos:scopeNote xml:lang="en">This property may be used directly, or as a super-property for more specific note types.</skos:scopeNote>
</rdf:Description>

<rdf:Description rdf:about="http://academictourism.com/entity/PER0002">
	<cidoc-crm:P143i_was_joined_by rdf:resource="http://academictourism.com/entity/J0001"/>
</rdf:Description>

<rdf:Description rdf:about="http://academictourism.com/entity/BRF0004.RS.RS0002.RS0003">
	<cidoc-crm:P8_took_place_on_or_within rdf:resource="http://academictourism.com/entity/LOC0003.CS.K003"/>
</rdf:Description>

<rdf:Description rdf:about="http://academictourism.com/entity/BRF0004.RS.RS0004.RS0003">
	<rdfs:label>Move from Hercules to the bottom of Octogoon</rdfs:label>
</rdf:Description>

<rdf:Description rdf:about="http://academictourism.com/entity/BRF0004.RS.RS0004.RS0004">
	<cidoc-crm:P7_took_place_at rdf:resource="http://academictourism.com/entity/LOC0003"/>
</rdf:Description>

<rdf:Description rdf:about="http://academictourism.com/entity/BRF0004.RS.RS0004.RS0003">
	<cidoc-crm:P7_took_place_at rdf:resource="http://academictourism.com/entity/LOC0003"/>
</rdf:Description>

<rdf:Description rdf:about="http://academictourism.com/entity/BRF0001.RS.RS0004.RS0003">
	<cidoc-crm:P7_took_place_at rdf:resource="http://academictourism.com/entity/LOC0003"/>
</rdf:Description>

<rdf:Description rdf:about="http://academictourism.com/entity/BRF0002.RS.RS0004.RS0003">
	<cidoc-crm:P7_took_place_at rdf:resource="http://academictourism.com/entity/LOC0003"/>
</rdf:Description>

<rdf:Description rdf:about="http://academictourism.com/entity/BRF0004.RS.RS0004.RS0001">
	<cidoc-crm:P7_took_place_at rdf:resource="http://academictourism.com/entity/LOC0003"/>
</rdf:Description>

<rdf:Description rdf:about="http://academictourism.com/entity/BRF0004.RS.RS0004.RS0002">
	<cidoc-crm:P7_took_place_at rdf:resource="http://academictourism.com/entity/LOC0003"/>
</rdf:Description>

</rdf:RDF>